<?xml version="1.0"?>
<rdf:RDF xmlns="http://www.theworldavatar.com/kg/ontodatadoc#"
     xml:base="http://www.theworldavatar.com/kg/ontodatadoc"
     xmlns:dc="http://purl.org/dc/elements/1.1/"
     xmlns:owl="http://www.w3.org/2002/07/owl#"
     xmlns:rdf="http://www.w3.org/1999/02/22-rdf-syntax-ns#"
     xmlns:xml="http://www.w3.org/XML/1998/namespace"
     xmlns:xsd="http://www.w3.org/2001/XMLSchema#"
     xmlns:rdfs="http://www.w3.org/2000/01/rdf-schema#"
     xmlns:ontodatadoc="http://www.theworldavatar.com/kg/ontodatadoc#">
    <owl:Ontology rdf:about="http://www.theworldavatar.com/kg/ontodatadoc">
        <dc:date>04 May 2024</dc:date>
        <gitCommitHash>c0599beca8df55873a1ab061dee64e52c510c6a0</gitCommitHash>
        <rdfs:comment>OntoDataDoc is an ontology developed for representing data documentation.</rdfs:comment>
        <owl:versionInfo>1</owl:versionInfo>
    </owl:Ontology>
    


    <!-- 
    ///////////////////////////////////////////////////////////////////////////////////////
    //
    // Annotation properties
    //
    ///////////////////////////////////////////////////////////////////////////////////////
     -->


    


    <!-- http://purl.org/dc/elements/1.1/date -->


    <owl:AnnotationProperty rdf:about="http://purl.org/dc/elements/1.1/date"/>
    


    <!-- http://www.theworldavatar.com/kg/ontodatadoc#gitCommitHash -->


    <owl:AnnotationProperty rdf:about="http://www.theworldavatar.com/kg/ontodatadoc#gitCommitHash"/>
    


    <!-- 
    ///////////////////////////////////////////////////////////////////////////////////////
    //
    // Object Properties
    //
    ///////////////////////////////////////////////////////////////////////////////////////
     -->


    


    <!-- http://purl.org/dc/terms/accessRights -->


    <owl:ObjectProperty rdf:about="http://purl.org/dc/terms/accessRights">
        <rdfs:domain rdf:resource="http://www.theworldavatar.com/kg/ontodatadoc#UsageGuideline"/>
        <rdfs:range rdf:resource="http://purl.org/dc/terms/RightsStatement"/>
        <rdfs:comment>Establishes the access restrictions to indicate permissions and limitations on who can access the data</rdfs:comment>
        <rdfs:isDefinedBy rdf:resource="http://purl.org/dc/terms/"/>
        <rdfs:label>has Access Rights</rdfs:label>
    </owl:ObjectProperty>
    


    <!-- http://purl.org/dc/terms/contributor -->


    <owl:ObjectProperty rdf:about="http://purl.org/dc/terms/contributor">
        <rdfs:domain rdf:resource="http://www.theworldavatar.com/kg/ontodatadoc#Dataset"/>
        <rdfs:range rdf:resource="http://www.w3.org/ns/prov#Agent"/>
        <rdfs:comment>A relation that establishes a link between a dataset and its contributors, recognizing individuals or entities who have contributed to the dataset beyond its creation</rdfs:comment>
        <rdfs:isDefinedBy rdf:resource="http://purl.org/dc/terms/"/>
        <rdfs:label>has Contributor</rdfs:label>
    </owl:ObjectProperty>
    


    <!-- http://purl.org/dc/terms/creator -->


    <owl:ObjectProperty rdf:about="http://purl.org/dc/terms/creator">
        <rdfs:domain rdf:resource="http://www.theworldavatar.com/kg/ontodatadoc#Dataset"/>
        <rdfs:range rdf:resource="http://www.w3.org/ns/prov#Agent"/>
        <rdfs:comment>A relation between a dataset and its creator, identifying the individual or entity responsible for the initial development or generation of the data</rdfs:comment>
        <rdfs:isDefinedBy rdf:resource="http://purl.org/dc/terms/"/>
        <rdfs:label>has Creator</rdfs:label>
    </owl:ObjectProperty>
    


    <!-- http://purl.org/dc/terms/distribution -->


    <owl:ObjectProperty rdf:about="http://purl.org/dc/terms/distribution">
        <rdfs:domain rdf:resource="http://www.theworldavatar.com/kg/ontodatadoc#Dataset"/>
        <rdfs:range rdf:resource="http://www.theworldavatar.com/kg/ontodatadoc#DataFormat"/>
        <rdfs:comment>A relation that indicates a format or data structure in which the dataset is presented or stored</rdfs:comment>
        <rdfs:isDefinedBy rdf:resource="http://purl.org/dc/terms/"/>
        <rdfs:label>has Data Format</rdfs:label>
    </owl:ObjectProperty>
    


    <!-- http://purl.org/dc/terms/hasVersion -->


    <owl:ObjectProperty rdf:about="http://purl.org/dc/terms/hasVersion">
        <rdfs:domain rdf:resource="http://www.theworldavatar.com/kg/ontodatadoc#QualityControl"/>
        <rdfs:range rdf:resource="http://www.theworldavatar.com/kg/ontodatadoc#Versioning"/>
        <rdfs:comment>Specifies the version or iteration of the dataset, offering insights into the evolution and changes made over time</rdfs:comment>
        <rdfs:isDefinedBy rdf:resource="http://purl.org/dc/terms/"/>
        <rdfs:label>has Version</rdfs:label>
    </owl:ObjectProperty>
    


    <!-- http://purl.org/dc/terms/language -->


    <owl:ObjectProperty rdf:about="http://purl.org/dc/terms/language">
        <rdfs:domain rdf:resource="http://www.theworldavatar.com/kg/ontodatadoc#Dataset"/>
        <rdfs:range rdf:resource="http://www.theworldavatar.com/kg/ontodatadoc#LinguisticSystem"/>
        <rdfs:comment>Establishes the linguistic context or the language of the dataset</rdfs:comment>
        <rdfs:isDefinedBy rdf:resource="http://purl.org/dc/terms/"/>
        <rdfs:label>has Language</rdfs:label>
    </owl:ObjectProperty>
    


    <!-- http://purl.org/dc/terms/license -->


    <owl:ObjectProperty rdf:about="http://purl.org/dc/terms/license">
        <rdfs:domain rdf:resource="http://www.theworldavatar.com/kg/ontodatadoc#UsageGuideline"/>
        <rdfs:range rdf:resource="http://purl.org/dc/terms/LicenseDocument"/>
        <rdfs:isDefinedBy rdf:resource="http://purl.org/dc/terms/"/>
        <rdfs:label>License  </rdfs:label>
    </owl:ObjectProperty>
    


    <!-- http://purl.org/dc/terms/rightHolder -->


    <owl:ObjectProperty rdf:about="http://purl.org/dc/terms/rightHolder">
        <rdfs:domain rdf:resource="http://www.theworldavatar.com/kg/ontodatadoc#UsageGuideline"/>
        <rdfs:range rdf:resource="http://www.w3.org/ns/prov#Agent"/>
        <rdfs:isDefinedBy rdf:resource="http://purl.org/dc/terms/"/>
        <rdfs:label>has Right Holder</rdfs:label>
    </owl:ObjectProperty>
    


    <!-- http://purl.org/dc/terms/rights -->


    <owl:ObjectProperty rdf:about="http://purl.org/dc/terms/rights">
        <rdfs:domain rdf:resource="http://www.theworldavatar.com/kg/ontodatadoc#UsageGuideline"/>
        <rdfs:range rdf:resource="http://purl.org/dc/terms/RightsStatement"/>
        <rdfs:isDefinedBy rdf:resource="http://purl.org/dc/terms/"/>
        <rdfs:label>has Rights</rdfs:label>
    </owl:ObjectProperty>
    


    <!-- http://purl.org/dc/terms/spatial -->


    <owl:ObjectProperty rdf:about="http://purl.org/dc/terms/spatial">
        <rdfs:domain rdf:resource="http://www.theworldavatar.com/kg/ontodatadoc#Dataset"/>
        <rdfs:range rdf:resource="http://purl.org/dc/terms/Location"/>
        <rdfs:isDefinedBy rdf:resource="http://purl.org/dc/terms/"/>
        <rdfs:label>has Coverage</rdfs:label>
    </owl:ObjectProperty>
    


    <!-- http://purl.org/dc/terms/subject -->


    <owl:ObjectProperty rdf:about="http://purl.org/dc/terms/subject">
        <rdfs:domain rdf:resource="http://www.theworldavatar.com/kg/ontodatadoc#Dataset"/>
        <rdfs:range rdf:resource="http://www.theworldavatar.com/kg/ontodatadoc#Subject"/>
        <rdfs:comment>Identifies the main topic or theme of the dataset, providing a concise description of the primary focus or purpose of the data</rdfs:comment>
        <rdfs:isDefinedBy rdf:resource="http://purl.org/dc/terms/"/>
        <rdfs:label>has Subject</rdfs:label>
    </owl:ObjectProperty>
    


    <!-- http://www.ontology-of-units-of-measure.org/resource/om-2/hasUnit -->


    <owl:ObjectProperty rdf:about="http://www.ontology-of-units-of-measure.org/resource/om-2/hasUnit">
        <rdfs:domain rdf:resource="http://www.theworldavatar.com/kg/ontodatadoc#QuantitativeCharacteristic"/>
        <rdfs:range rdf:resource="http://www.theworldavatar.com/kg/ontodatadoc#Unit"/>
        <rdfs:comment>A relation between a data content and its measurement units for quantitative data</rdfs:comment>
        <rdfs:isDefinedBy rdf:resource="http://www.ontology-of-units-of-measure.org/resource/om-2/"/>
        <rdfs:label>has Unit</rdfs:label>
    </owl:ObjectProperty>
    


    <!-- http://www.theworldavatar.com/kg/ontodatadoc#dependsOn -->


    <owl:ObjectProperty rdf:about="http://www.theworldavatar.com/kg/ontodatadoc#dependsOn">
        <rdfs:domain rdf:resource="http://www.theworldavatar.com/kg/ontodatadoc#DependentContent"/>
        <rdfs:range rdf:resource="http://www.theworldavatar.com/kg/ontodatadoc#DataContent"/>
        <rdfs:comment>Specifies dependency on a data content</rdfs:comment>
        <rdfs:isDefinedBy rdf:resource="http://www.theworldavatar.com/kg/ontodatadoc/"/>
        <rdfs:label>depends On</rdfs:label>
    </owl:ObjectProperty>
    


    <!-- http://www.theworldavatar.com/kg/ontodatadoc#extractedFrom -->


    <owl:ObjectProperty rdf:about="http://www.theworldavatar.com/kg/ontodatadoc#extractedFrom">
        <rdfs:domain rdf:resource="http://www.theworldavatar.com/kg/ontodatadoc#Dataset"/>
        <rdfs:range rdf:resource="http://www.theworldavatar.com/kg/ontodatadoc#DataSource"/>
        <rdfs:comment>Specifies the source or origin from which the dataset was extracted, offering insights into the data&apos;s provenance</rdfs:comment>
        <rdfs:isDefinedBy rdf:resource="http://www.theworldavatar.com/kg/ontodatadoc/"/>
        <rdfs:label>extracted From</rdfs:label>
    </owl:ObjectProperty>
    


    <!-- http://www.theworldavatar.com/kg/ontodatadoc#hasCharacteristic -->


    <owl:ObjectProperty rdf:about="http://www.theworldavatar.com/kg/ontodatadoc#hasCharacteristic">
        <rdfs:domain rdf:resource="http://www.theworldavatar.com/kg/ontodatadoc#DataContent"/>
        <rdfs:range rdf:resource="http://www.theworldavatar.com/kg/ontodatadoc#Characteristic"/>
        <rdfs:comment>A relation between a data content and its distinctive qualitative or quantitative characteristic</rdfs:comment>
        <rdfs:isDefinedBy rdf:resource="http://www.theworldavatar.com/kg/ontodatadoc/"/>
        <rdfs:label>has Characteristic</rdfs:label>
    </owl:ObjectProperty>
    


    <!-- http://www.theworldavatar.com/kg/ontodatadoc#hasConsistencyCheck -->


    <owl:ObjectProperty rdf:about="http://www.theworldavatar.com/kg/ontodatadoc#hasConsistencyCheck">
        <rdfs:domain rdf:resource="http://www.theworldavatar.com/kg/ontodatadoc#QualityControl"/>
        <rdfs:range rdf:resource="http://www.theworldavatar.com/kg/ontodatadoc#ConsistencyCheck"/>
        <rdfs:comment>A relation between a dataset and its consistency checking processes used to maintain uniformity within the data</rdfs:comment>
        <rdfs:isDefinedBy rdf:resource="http://www.theworldavatar.com/kg/ontodatadoc/"/>
        <rdfs:label>has Consistency Check</rdfs:label>
    </owl:ObjectProperty>
    


    <!-- http://www.theworldavatar.com/kg/ontodatadoc#hasContent -->


    <owl:ObjectProperty rdf:about="http://www.theworldavatar.com/kg/ontodatadoc#hasContent">
        <rdfs:domain rdf:resource="http://www.theworldavatar.com/kg/ontodatadoc#Dataset"/>
        <rdfs:range rdf:resource="http://www.theworldavatar.com/kg/ontodatadoc#DataContent"/>
        <rdfs:comment>A relation between a dataset and its content or variable</rdfs:comment>
        <rdfs:isDefinedBy rdf:resource="http://www.theworldavatar.com/kg/ontodatadoc/"/>
        <rdfs:label>has Content</rdfs:label>
    </owl:ObjectProperty>
    


    <!-- http://www.theworldavatar.com/kg/ontodatadoc#hasDataCategory -->


    <owl:ObjectProperty rdf:about="http://www.theworldavatar.com/kg/ontodatadoc#hasDataCategory">
        <rdfs:domain rdf:resource="http://www.theworldavatar.com/kg/ontodatadoc#Dataset"/>
        <rdfs:range rdf:resource="http://www.theworldavatar.com/kg/ontodatadoc#DataCategory"/>
        <rdfs:comment>Specifies the category or classification to which the dataset belongs</rdfs:comment>
        <rdfs:isDefinedBy rdf:resource="http://www.theworldavatar.com/kg/ontodatadoc/"/>
        <rdfs:label>has Data Category</rdfs:label>
    </owl:ObjectProperty>
    


    <!-- http://www.theworldavatar.com/kg/ontodatadoc#hasDataValidation -->


    <owl:ObjectProperty rdf:about="http://www.theworldavatar.com/kg/ontodatadoc#hasDataValidation">
        <rdfs:domain rdf:resource="http://www.theworldavatar.com/kg/ontodatadoc#QualityControl"/>
        <rdfs:range rdf:resource="http://www.theworldavatar.com/kg/ontodatadoc#DataValidation"/>
        <rdfs:comment>A relation between a dataset and its validation processes to ensure the accuracy and reliability of the data</rdfs:comment>
        <rdfs:isDefinedBy rdf:resource="http://www.theworldavatar.com/kg/ontodatadoc/"/>
        <rdfs:label>has Data Validation</rdfs:label>
    </owl:ObjectProperty>
    


    <!-- http://www.theworldavatar.com/kg/ontodatadoc#hasElement -->


    <owl:ObjectProperty rdf:about="http://www.theworldavatar.com/kg/ontodatadoc#hasElement">
        <rdfs:domain rdf:resource="http://www.theworldavatar.com/kg/ontodatadoc#DataContent"/>
        <rdfs:range rdf:resource="http://www.theworldavatar.com/kg/ontodatadoc#Element"/>
        <rdfs:comment>A relation between a data content and its basic building blocks or components</rdfs:comment>
        <rdfs:isDefinedBy rdf:resource="http://www.theworldavatar.com/kg/ontodatadoc/"/>
        <rdfs:label>has Element</rdfs:label>
    </owl:ObjectProperty>
    


    <!-- http://www.theworldavatar.com/kg/ontodatadoc#hasMissingData -->


    <owl:ObjectProperty rdf:about="http://www.theworldavatar.com/kg/ontodatadoc#hasMissingData">
        <rdfs:domain rdf:resource="http://www.theworldavatar.com/kg/ontodatadoc#QualityControl"/>
        <rdfs:range rdf:resource="http://www.theworldavatar.com/kg/ontodatadoc#MissingData"/>
        <rdfs:comment>Establishes a connection between a dataset and its missing data information to indicate the absence or incompleteness of data</rdfs:comment>
        <rdfs:isDefinedBy rdf:resource="http://www.theworldavatar.com/kg/ontodatadoc/"/>
        <rdfs:label>has Missing Data</rdfs:label>
    </owl:ObjectProperty>
    


    <!-- http://www.theworldavatar.com/kg/ontodatadoc#hasPublication -->


    <owl:ObjectProperty rdf:about="http://www.theworldavatar.com/kg/ontodatadoc#hasPublication">
        <rdfs:domain rdf:resource="http://www.theworldavatar.com/kg/ontodatadoc#Dataset"/>
        <rdfs:range rdf:resource="http://www.theworldavatar.com/kg/ontodatadoc#Publication"/>
        <rdfs:comment>A relation between a dataset and its publication, indicating when and where the dataset was officially released or made public</rdfs:comment>
        <rdfs:isDefinedBy rdf:resource="http://www.theworldavatar.com/kg/ontodatadoc/"/>
        <rdfs:label>has Publication</rdfs:label>
    </owl:ObjectProperty>
    


    <!-- http://www.theworldavatar.com/kg/ontodatadoc#hasQualityControlPass -->


    <owl:ObjectProperty rdf:about="http://www.theworldavatar.com/kg/ontodatadoc#hasQualityControlPass">
        <rdfs:domain rdf:resource="http://www.theworldavatar.com/kg/ontodatadoc#Dataset"/>
        <rdfs:range rdf:resource="http://www.theworldavatar.com/kg/ontodatadoc#QualityControl"/>
        <rdfs:comment>A relation between a dataset and its quality check or control pass</rdfs:comment>
        <rdfs:isDefinedBy rdf:resource="http://www.theworldavatar.com/kg/ontodatadoc/"/>
        <rdfs:label>has Quality Control Pass</rdfs:label>
    </owl:ObjectProperty>
    


    <!-- http://www.theworldavatar.com/kg/ontodatadoc#hasRelation -->


    <owl:ObjectProperty rdf:about="http://www.theworldavatar.com/kg/ontodatadoc#hasRelation">
        <rdfs:domain rdf:resource="http://www.theworldavatar.com/kg/ontodatadoc#Dataset"/>
        <rdfs:range rdf:resource="http://www.theworldavatar.com/kg/ontodatadoc#Dataset"/>
        <rdfs:comment>Specifies related datasets or data entities</rdfs:comment>
        <rdfs:isDefinedBy rdf:resource="http://www.theworldavatar.com/kg/ontodatadoc/"/>
        <rdfs:label>has Relation</rdfs:label>
    </owl:ObjectProperty>
    


    <!-- http://www.theworldavatar.com/kg/ontodatadoc#hasTermsAndConditions -->


    <owl:ObjectProperty rdf:about="http://www.theworldavatar.com/kg/ontodatadoc#hasTermsAndConditions">
        <rdfs:domain rdf:resource="http://www.theworldavatar.com/kg/ontodatadoc#UsageGuideline"/>
        <rdfs:range rdf:resource="http://www.theworldavatar.com/kg/ontodatadoc#TermsAndConditions"/>
        <rdfs:comment>Establishes a relation to outline the legal and contractual obligations associated with the data</rdfs:comment>
        <rdfs:isDefinedBy rdf:resource="http://www.theworldavatar.com/kg/ontodatadoc/"/>
        <rdfs:label>has Terms and Conditions</rdfs:label>
    </owl:ObjectProperty>
    


    <!-- http://www.theworldavatar.com/kg/ontodatadoc#hasUsabilityTesting -->


    <owl:ObjectProperty rdf:about="http://www.theworldavatar.com/kg/ontodatadoc#hasUsabilityTesting">
        <rdfs:domain rdf:resource="http://www.theworldavatar.com/kg/ontodatadoc#QualityControl"/>
        <rdfs:range rdf:resource="http://www.theworldavatar.com/kg/ontodatadoc#UsabilityTesting"/>
        <rdfs:comment>A relation between a dataset and usability testing, indicating efforts to assess the dataset&apos;s user-friendliness and accessibility</rdfs:comment>
        <rdfs:isDefinedBy rdf:resource="http://www.theworldavatar.com/kg/ontodatadoc/"/>
        <rdfs:label>has Usability Testing</rdfs:label>
    </owl:ObjectProperty>
    


    <!-- http://www.theworldavatar.com/kg/ontodatadoc#hasUsageGuideline -->


    <owl:ObjectProperty rdf:about="http://www.theworldavatar.com/kg/ontodatadoc#hasUsageGuideline">
        <rdfs:domain rdf:resource="http://www.theworldavatar.com/kg/ontodatadoc#Dataset"/>
        <rdfs:range rdf:resource="http://www.theworldavatar.com/kg/ontodatadoc#UsageGuideline"/>
        <rdfs:comment>Establishes a relation between a dataset and its usage guidelines, providing recommendations and best practices for utilizing the data</rdfs:comment>
        <rdfs:isDefinedBy rdf:resource="http://www.theworldavatar.com/kg/ontodatadoc/"/>
        <rdfs:label>has Usage Guideline</rdfs:label>
    </owl:ObjectProperty>
    


    <!-- http://www.theworldavatar.com/kg/ontodatadoc#hasUserReview -->


    <owl:ObjectProperty rdf:about="http://www.theworldavatar.com/kg/ontodatadoc#hasUserReview">
        <rdfs:domain rdf:resource="http://www.theworldavatar.com/kg/ontodatadoc#QualityControl"/>
        <rdfs:range rdf:resource="http://www.theworldavatar.com/kg/ontodatadoc#UserReview"/>
        <rdfs:comment>A relation between a dataset and user reviews, capturing feedback and insights from individuals who have interacted with the data</rdfs:comment>
        <rdfs:isDefinedBy rdf:resource="http://www.theworldavatar.com/kg/ontodatadoc/"/>
        <rdfs:label>has User Review</rdfs:label>
    </owl:ObjectProperty>
    


    <!-- http://www.w3.org/ns/odrl/2/hasPolicy -->


    <owl:ObjectProperty rdf:about="http://www.w3.org/ns/odrl/2/hasPolicy">
        <rdfs:domain rdf:resource="http://www.theworldavatar.com/kg/ontodatadoc#UsageGuideline"/>
        <rdfs:range rdf:resource="http://www.w3.org/ns/odrl/2/Policy"/>
        <rdfs:isDefinedBy rdf:resource="http://www.w3.org/ns/odrl/2/"/>
        <rdfs:label>has Policy</rdfs:label>
    </owl:ObjectProperty>
    


    <!-- http://www.w3.org/ns/prov#wasAssociatedWith -->


    <owl:ObjectProperty rdf:about="http://www.w3.org/ns/prov#wasAssociatedWith">
        <rdfs:domain rdf:resource="http://www.w3.org/ns/prov#Activity"/>
        <rdfs:range rdf:resource="http://www.w3.org/ns/prov#Agent"/>
        <rdfs:isDefinedBy rdf:resource="http://www.w3.org/ns/prov#"/>
        <rdfs:label>was Associated With</rdfs:label>
    </owl:ObjectProperty>
    


    <!-- http://www.w3.org/ns/prov#wasGeneratedBy -->


    <owl:ObjectProperty rdf:about="http://www.w3.org/ns/prov#wasGeneratedBy">
        <rdfs:domain rdf:resource="http://www.theworldavatar.com/kg/ontodatadoc#Dataset"/>
        <rdfs:range rdf:resource="http://www.w3.org/ns/prov#Activity"/>
        <rdfs:isDefinedBy rdf:resource="http://www.w3.org/ns/prov#"/>
        <rdfs:label>was Generated By</rdfs:label>
    </owl:ObjectProperty>
    


    <!-- 
    ///////////////////////////////////////////////////////////////////////////////////////
    //
    // Data properties
    //
    ///////////////////////////////////////////////////////////////////////////////////////
     -->


    


    <!-- http://purl.org/dc/terms/bibliographicCitation -->


    <owl:DatatypeProperty rdf:about="http://purl.org/dc/terms/bibliographicCitation">
        <rdfs:domain rdf:resource="http://www.theworldavatar.com/kg/ontodatadoc#UsageGuideline"/>
        <rdfs:range rdf:resource="http://www.w3.org/2001/XMLSchema#string"/>
        <rdfs:isDefinedBy rdf:resource="http://purl.org/dc/terms/"/>
        <rdfs:label>has Bibliographic Citation</rdfs:label>
    </owl:DatatypeProperty>
    


    <!-- http://purl.org/dc/terms/dateCopyrighted -->


    <owl:DatatypeProperty rdf:about="http://purl.org/dc/terms/dateCopyrighted">
        <rdfs:domain rdf:resource="http://www.theworldavatar.com/kg/ontodatadoc#UsageGuideline"/>
        <rdfs:range rdf:resource="http://www.w3.org/2001/XMLSchema#string"/>
        <rdfs:comment>Specifies the date of copyright information at which the dataset to indicate ownership and intellectual property rights</rdfs:comment>
        <rdfs:isDefinedBy rdf:resource="http://purl.org/dc/terms/"/>
        <rdfs:label>has Copyright</rdfs:label>
    </owl:DatatypeProperty>
    


    <!-- http://purl.org/dc/terms/description -->


    <owl:DatatypeProperty rdf:about="http://purl.org/dc/terms/description">
        <rdfs:domain rdf:resource="http://www.theworldavatar.com/kg/ontodatadoc#Dataset"/>
        <rdfs:range rdf:resource="http://www.w3.org/2001/XMLSchema#string"/>
        <rdfs:comment>Provides a textual description of the dataset</rdfs:comment>
        <rdfs:isDefinedBy rdf:resource="http://purl.org/dc/terms/"/>
        <rdfs:label>has Description</rdfs:label>
    </owl:DatatypeProperty>
    


    <!-- http://purl.org/dc/terms/identifier -->


    <owl:DatatypeProperty rdf:about="http://purl.org/dc/terms/identifier">
        <rdfs:domain rdf:resource="http://www.theworldavatar.com/kg/ontodatadoc#Dataset"/>
        <rdfs:range rdf:resource="http://www.w3.org/2001/XMLSchema#string"/>
        <rdfs:isDefinedBy rdf:resource="http://purl.org/dc/terms/"/>
        <rdfs:label>has Identifier</rdfs:label>
    </owl:DatatypeProperty>
    


    <!-- http://purl.org/dc/terms/title -->


    <owl:DatatypeProperty rdf:about="http://purl.org/dc/terms/title">
        <rdfs:domain rdf:resource="http://www.theworldavatar.com/kg/ontodatadoc#Dataset"/>
        <rdfs:range rdf:resource="http://www.w3.org/2001/XMLSchema#string"/>
        <rdfs:isDefinedBy rdf:resource="http://purl.org/dc/terms/"/>
        <rdfs:label>has Title</rdfs:label>
    </owl:DatatypeProperty>
    


    <!-- http://purl.org/ontology/bibo/doi -->


    <owl:DatatypeProperty rdf:about="http://purl.org/ontology/bibo/doi">
        <rdfs:domain rdf:resource="http://www.theworldavatar.com/kg/ontodatadoc#Publication"/>
        <rdfs:range rdf:resource="http://www.w3.org/2001/XMLSchema#string"/>
        <rdfs:comment>A relation that specifies Digital Object Identifier (DOI) of a published entity to make it publicly available</rdfs:comment>
        <rdfs:label>has DOI</rdfs:label>
    </owl:DatatypeProperty>
    


    <!-- http://www.theworldavatar.com/kg/ontodatadoc#hasContact -->


    <owl:DatatypeProperty rdf:about="http://www.theworldavatar.com/kg/ontodatadoc#hasContact">
        <rdfs:domain rdf:resource="http://www.theworldavatar.com/kg/ontodatadoc#UsageGuideline"/>
        <rdfs:range rdf:resource="http://www.w3.org/2001/XMLSchema#string"/>
        <rdfs:comment>specifies the contact information of an authority to discuss about the dataset as a usage guideline</rdfs:comment>
        <rdfs:isDefinedBy rdf:resource="http://www.theworldavatar.com/kg/ontodatadoc/"/>
        <rdfs:label>has Contact</rdfs:label>
    </owl:DatatypeProperty>
    


    <!-- http://www.theworldavatar.com/kg/ontodatadoc#hasIllustration -->


    <owl:DatatypeProperty rdf:about="http://www.theworldavatar.com/kg/ontodatadoc#hasIllustration">
        <rdfs:domain rdf:resource="http://www.theworldavatar.com/kg/ontodatadoc#DataContent"/>
        <rdfs:range rdf:resource="http://www.w3.org/2001/XMLSchema#string"/>
        <rdfs:comment>Specifies a comprehensive description of a Data content</rdfs:comment>
        <rdfs:isDefinedBy rdf:resource="http://www.theworldavatar.com/kg/ontodatadoc/"/>
        <rdfs:label>has Illustration</rdfs:label>
    </owl:DatatypeProperty>
    


    <!-- http://www.theworldavatar.com/kg/ontodatadoc#hasMaximumValue -->


    <owl:DatatypeProperty rdf:about="http://www.theworldavatar.com/kg/ontodatadoc#hasMaximumValue">
        <rdfs:domain rdf:resource="http://www.theworldavatar.com/kg/ontodatadoc#DataRange"/>
        <rdfs:range rdf:resource="http://www.w3.org/2001/XMLSchema#float"/>
        <rdfs:comment>Specifies the maximum value</rdfs:comment>
        <rdfs:isDefinedBy rdf:resource="http://www.theworldavatar.com/kg/ontodatadoc/"/>
        <rdfs:label>has Maximum Value</rdfs:label>
    </owl:DatatypeProperty>
    


    <!-- http://www.theworldavatar.com/kg/ontodatadoc#hasMinimumValue -->


    <owl:DatatypeProperty rdf:about="http://www.theworldavatar.com/kg/ontodatadoc#hasMinimumValue">
        <rdfs:domain rdf:resource="http://www.theworldavatar.com/kg/ontodatadoc#DataRange"/>
        <rdfs:range rdf:resource="http://www.w3.org/2001/XMLSchema#float"/>
        <rdfs:comment>Specifies the minimum value</rdfs:comment>
        <rdfs:isDefinedBy rdf:resource="http://www.theworldavatar.com/kg/ontodatadoc/"/>
        <rdfs:label>has Minimum Value</rdfs:label>
    </owl:DatatypeProperty>
    


    <!-- http://www.theworldavatar.com/kg/ontodatadoc#hasObjective -->


    <owl:DatatypeProperty rdf:about="http://www.theworldavatar.com/kg/ontodatadoc#hasObjective">
        <rdfs:domain rdf:resource="http://www.theworldavatar.com/kg/ontodatadoc#Dataset"/>
        <rdfs:range rdf:resource="http://www.w3.org/2001/XMLSchema#string"/>
        <rdfs:comment>Specifies objectives or goals associated with the dataset</rdfs:comment>
        <rdfs:isDefinedBy rdf:resource="http://www.theworldavatar.com/kg/ontodatadoc/"/>
        <rdfs:label>has Objective</rdfs:label>
    </owl:DatatypeProperty>
    


    <!-- http://www.theworldavatar.com/kg/ontodatadoc#hasPurpose -->


    <owl:DatatypeProperty rdf:about="http://www.theworldavatar.com/kg/ontodatadoc#hasPurpose">
        <rdfs:domain rdf:resource="http://www.theworldavatar.com/kg/ontodatadoc#Dataset"/>
        <rdfs:range rdf:resource="http://www.w3.org/2001/XMLSchema#string"/>
        <rdfs:comment>Describes the purpose or intended use of the dataset</rdfs:comment>
        <rdfs:isDefinedBy rdf:resource="http://www.theworldavatar.com/kg/ontodatadoc/"/>
        <rdfs:label>has Purpose</rdfs:label>
    </owl:DatatypeProperty>
    


    <!-- http://www.theworldavatar.com/kg/ontodatadoc#providedBy -->


    <owl:DatatypeProperty rdf:about="http://www.theworldavatar.com/kg/ontodatadoc#providedBy">
        <rdfs:domain rdf:resource="http://www.theworldavatar.com/kg/ontodatadoc#Dataset"/>
        <rdfs:range rdf:resource="http://www.w3.org/2001/XMLSchema#string"/>
        <rdfs:comment>Specifies a person or organisation that provides the dataset</rdfs:comment>
        <rdfs:isDefinedBy rdf:resource="http://www.theworldavatar.com/kg/ontodatadoc/"/>
        <rdfs:label>provided By</rdfs:label>
    </owl:DatatypeProperty>
    


    <!-- http://www.w3.org/ns/dcat#keyword -->


    <owl:DatatypeProperty rdf:about="http://www.w3.org/ns/dcat#keyword">
        <rdfs:domain rdf:resource="http://www.theworldavatar.com/kg/ontodatadoc#Dataset"/>
        <rdfs:range rdf:resource="http://www.w3.org/2001/XMLSchema#string"/>
        <rdfs:comment>Specifies the contact details for individuals or entities responsible for inquiries or further information related to the dataset usage</rdfs:comment>
        <rdfs:isDefinedBy rdf:resource="http://www.w3.org/ns/dcat#"/>
        <rdfs:label>has Keyword</rdfs:label>
    </owl:DatatypeProperty>
    


    <!-- http://www.w3.org/ns/prov#endedAtTime -->


    <owl:DatatypeProperty rdf:about="http://www.w3.org/ns/prov#endedAtTime">
        <rdfs:domain rdf:resource="http://www.w3.org/ns/prov#Activity"/>
        <rdfs:range rdf:resource="http://www.w3.org/2001/XMLSchema#dateTime"/>
        <rdfs:isDefinedBy rdf:resource="http://www.w3.org/ns/prov#"/>
        <rdfs:label>ended At Time</rdfs:label>
    </owl:DatatypeProperty>
    


    <!-- http://www.w3.org/ns/prov#startedAtTime -->


    <owl:DatatypeProperty rdf:about="http://www.w3.org/ns/prov#startedAtTime">
        <rdfs:domain rdf:resource="http://www.w3.org/ns/prov#Activity"/>
        <rdfs:range rdf:resource="http://www.w3.org/2001/XMLSchema#dateTime"/>
        <rdfs:isDefinedBy rdf:resource="http://www.w3.org/ns/prov#"/>
        <rdfs:label>started At Time</rdfs:label>
    </owl:DatatypeProperty>
    


    <!-- https://schema.org/contentSize -->


    <owl:DatatypeProperty rdf:about="https://schema.org/contentSize">
        <rdfs:domain rdf:resource="http://www.theworldavatar.com/kg/ontodatadoc#QualityControl"/>
        <rdfs:range rdf:resource="http://www.w3.org/2001/XMLSchema#float"/>
        <rdfs:comment>Specifies the size of the dataset</rdfs:comment>
        <rdfs:isDefinedBy rdf:resource="https://schema.org/"/>
        <rdfs:label>has Content Size</rdfs:label>
    </owl:DatatypeProperty>
    


    <!-- https://schema.org/dateCreated -->


    <owl:DatatypeProperty rdf:about="https://schema.org/dateCreated">
        <rdfs:domain rdf:resource="http://www.theworldavatar.com/kg/ontodatadoc#Dataset"/>
        <rdfs:range rdf:resource="http://www.w3.org/2001/XMLSchema#dateTime"/>
        <rdfs:comment>Specifies a date when the dataset was originally created</rdfs:comment>
        <rdfs:isDefinedBy rdf:resource="https://schema.org/"/>
        <rdfs:label>has Date Created</rdfs:label>
    </owl:DatatypeProperty>
    


    <!-- https://schema.org/dateModified -->


    <owl:DatatypeProperty rdf:about="https://schema.org/dateModified">
        <rdfs:domain rdf:resource="http://www.theworldavatar.com/kg/ontodatadoc#Dataset"/>
        <rdfs:range rdf:resource="http://www.w3.org/2001/XMLSchema#dateTime"/>
        <rdfs:isDefinedBy rdf:resource="https://schema.org/"/>
        <rdfs:label>has Date Modified</rdfs:label>
    </owl:DatatypeProperty>
    


    <!-- https://schema.org/name -->


    <owl:DatatypeProperty rdf:about="https://schema.org/name">
        <rdfs:domain rdf:resource="http://www.theworldavatar.com/kg/ontodatadoc#DataContent"/>
        <rdfs:range rdf:resource="http://www.w3.org/2001/XMLSchema#string"/>
        <rdfs:comment>Specifies the identified name of a Data content for popular referencing and identification</rdfs:comment>
        <rdfs:isDefinedBy rdf:resource="https://schema.org/"/>
        <rdfs:label>has Name</rdfs:label>
    </owl:DatatypeProperty>
    


    <!-- https://schema.org/url -->


    <owl:DatatypeProperty rdf:about="https://schema.org/url">
        <rdfs:domain rdf:resource="http://www.theworldavatar.com/kg/ontodatadoc#UsageGuideline"/>
        <rdfs:range rdf:resource="http://www.w3.org/2001/XMLSchema#anyURI"/>
        <rdfs:comment>Specifies how the dataset should be cited</rdfs:comment>
        <rdfs:isDefinedBy rdf:resource="https://schema.org/"/>
        <rdfs:label>has URL</rdfs:label>
    </owl:DatatypeProperty>
    


    <!-- 
    ///////////////////////////////////////////////////////////////////////////////////////
    //
    // Classes
    //
    ///////////////////////////////////////////////////////////////////////////////////////
     -->


    


    <!-- http://purl.org/dc/terms/LicenseDocument -->


    <owl:Class rdf:about="http://purl.org/dc/terms/LicenseDocument">
        <rdfs:isDefinedBy rdf:resource="http://purl.org/dc/terms/"/>
        <rdfs:label>License Document</rdfs:label>
    </owl:Class>
    


    <!-- http://purl.org/dc/terms/LinguisticSystem -->


    <owl:Class rdf:about="http://purl.org/dc/terms/LinguisticSystem">
        <rdfs:comment>A linguistic system indicates the linguistic context in which the dataset is presented</rdfs:comment>
        <rdfs:isDefinedBy rdf:resource="http://purl.org/dc/terms/"/>
        <rdfs:label>Linguistic System</rdfs:label>
    </owl:Class>
    


    <!-- http://purl.org/dc/terms/Location -->


    <owl:Class rdf:about="http://purl.org/dc/terms/Location">
        <rdfs:isDefinedBy rdf:resource="http://purl.org/dc/terms/"/>
        <rdfs:label>Location</rdfs:label>
    </owl:Class>
    


    <!-- http://purl.org/dc/terms/RightsStatement -->


    <owl:Class rdf:about="http://purl.org/dc/terms/RightsStatement">
        <rdfs:comment>The access rights specify the permissions and restrictions based on user roles and requirements associated with accessing the dataset</rdfs:comment>
        <rdfs:isDefinedBy rdf:resource="http://purl.org/dc/terms/"/>
        <rdfs:label>Rights Statement</rdfs:label>
    </owl:Class>
    


    <!-- http://www.ontology-of-units-of-measure.org/resource/om-2/Unit -->


    <owl:Class rdf:about="http://www.ontology-of-units-of-measure.org/resource/om-2/Unit">
        <rdfs:comment>A unit specifies a measurement unit associated with quantitative data, ensuring proper interpretation and analysis</rdfs:comment>
        <rdfs:isDefinedBy rdf:resource="http://www.ontology-of-units-of-measure.org/resource/om-2/"/>
        <rdfs:label>Unit</rdfs:label>
    </owl:Class>
    


    <!-- http://www.theworldavatar.com/kg/ontodatadoc#Characteristic -->


    <owl:Class rdf:about="http://www.theworldavatar.com/kg/ontodatadoc#Characteristic">
        <rdfs:comment>The characteristic outlines the distinctive features such as quantitative or qualitative nature of a data content</rdfs:comment>
        <rdfs:isDefinedBy rdf:resource="http://www.theworldavatar.com/kg/ontodatadoc/"/>
        <rdfs:label>Characteristic</rdfs:label>
    </owl:Class>
    


    <!-- http://www.theworldavatar.com/kg/ontodatadoc#ConsistencyCheck -->


    <owl:Class rdf:about="http://www.theworldavatar.com/kg/ontodatadoc#ConsistencyCheck">
        <rdfs:comment>The consistency check refers to a process or procedure implemented to ensure uniformity and coherence within the dataset</rdfs:comment>
        <rdfs:isDefinedBy rdf:resource="http://www.theworldavatar.com/kg/ontodatadoc/"/>
        <rdfs:label>Consistency Check</rdfs:label>
    </owl:Class>
    


    <!-- http://www.theworldavatar.com/kg/ontodatadoc#ControlledContent -->


    <owl:Class rdf:about="http://www.theworldavatar.com/kg/ontodatadoc#ControlledContent">
        <rdfs:subClassOf rdf:resource="http://www.theworldavatar.com/kg/ontodatadoc#DataContent"/>
        <rdfs:comment>A controlled content indicates data that is subject to specific constraints or regulations</rdfs:comment>
        <rdfs:isDefinedBy rdf:resource="http://www.theworldavatar.com/kg/ontodatadoc/"/>
        <rdfs:label>Controlled Content</rdfs:label>
    </owl:Class>
    


    <!-- http://www.theworldavatar.com/kg/ontodatadoc#DataCategory -->


    <owl:Class rdf:about="http://www.theworldavatar.com/kg/ontodatadoc#DataCategory">
        <rdfs:comment>A data category categorizes the dataset into broader thematic groups or domains</rdfs:comment>
        <rdfs:isDefinedBy rdf:resource="http://www.theworldavatar.com/kg/ontodatadoc/"/>
        <rdfs:label>Data Category</rdfs:label>
    </owl:Class>
    


    <!-- http://www.theworldavatar.com/kg/ontodatadoc#DataContent -->


    <owl:Class rdf:about="http://www.theworldavatar.com/kg/ontodatadoc#DataContent">
        <rdfs:comment>A data content describes the content and relations, characteristic, and fundamental elements within the dataset</rdfs:comment>
        <rdfs:isDefinedBy rdf:resource="http://www.theworldavatar.com/kg/ontodatadoc/"/>
        <rdfs:label>Data Content</rdfs:label>
    </owl:Class>
    


    <!-- http://www.theworldavatar.com/kg/ontodatadoc#DataFormat -->


    <owl:Class rdf:about="http://www.theworldavatar.com/kg/ontodatadoc#DataFormat"/>
    


    <!-- http://www.theworldavatar.com/kg/ontodatadoc#DataRange -->


    <owl:Class rdf:about="http://www.theworldavatar.com/kg/ontodatadoc#DataRange">
        <rdfs:comment>A data range defines the allowable values or scope for data points, that is, an acceptable range of variations</rdfs:comment>
        <rdfs:isDefinedBy rdf:resource="http://www.theworldavatar.com/kg/ontodatadoc/"/>
        <rdfs:label>Data Range</rdfs:label>
    </owl:Class>
    


    <!-- http://www.theworldavatar.com/kg/ontodatadoc#DataSource -->


    <owl:Class rdf:about="http://www.theworldavatar.com/kg/ontodatadoc#DataSource">
        <rdfs:comment>A data source identifies the origin of the data</rdfs:comment>
        <rdfs:isDefinedBy rdf:resource="http://www.theworldavatar.com/kg/ontodatadoc/"/>
        <rdfs:label>Data Source</rdfs:label>
    </owl:Class>
    


    <!-- http://www.theworldavatar.com/kg/ontodatadoc#DataValidation -->


    <owl:Class rdf:about="http://www.theworldavatar.com/kg/ontodatadoc#DataValidation">
        <rdfs:comment>The data validation encompasses processes or mechanisms used to ensure the accuracy and integrity of the dataset</rdfs:comment>
        <rdfs:isDefinedBy rdf:resource="http://www.theworldavatar.com/kg/ontodatadoc/"/>
        <rdfs:label>Data Validation</rdfs:label>
    </owl:Class>
    


    <!-- http://www.theworldavatar.com/kg/ontodatadoc#Dataset -->


    <owl:Class rdf:about="http://www.theworldavatar.com/kg/ontodatadoc#Dataset">
        <rdfs:comment>The fundamental unit of data, encapsulating a collection of related information for organizing and referencing specific sets of data.</rdfs:comment>
        <rdfs:isDefinedBy rdf:resource="http://www.theworldavatar.com/kg/ontodatadoc/"/>
        <rdfs:label>Dataset</rdfs:label>
    </owl:Class>
    


    <!-- http://www.theworldavatar.com/kg/ontodatadoc#DependentContent -->


    <owl:Class rdf:about="http://www.theworldavatar.com/kg/ontodatadoc#DependentContent">
        <rdfs:subClassOf rdf:resource="http://www.theworldavatar.com/kg/ontodatadoc#DataContent"/>
        <rdfs:comment>A dependent content signifies data points that rely on or are influenced by others</rdfs:comment>
        <rdfs:isDefinedBy rdf:resource="http://www.theworldavatar.com/kg/ontodatadoc/"/>
        <rdfs:label>Dependent Content</rdfs:label>
    </owl:Class>
    


    <!-- http://www.theworldavatar.com/kg/ontodatadoc#Element -->


    <owl:Class rdf:about="http://www.theworldavatar.com/kg/ontodatadoc#Element"/>
    


    <!-- http://www.theworldavatar.com/kg/ontodatadoc#IndependentContent -->


    <owl:Class rdf:about="http://www.theworldavatar.com/kg/ontodatadoc#IndependentContent">
        <rdfs:subClassOf rdf:resource="http://www.theworldavatar.com/kg/ontodatadoc#DataContent"/>
        <rdfs:comment>An independent content represents data points that stand alone and are not influenced by others</rdfs:comment>
        <rdfs:isDefinedBy rdf:resource="http://www.theworldavatar.com/kg/ontodatadoc/"/>
        <rdfs:label>Independent Content</rdfs:label>
    </owl:Class>
    


    <!-- http://www.theworldavatar.com/kg/ontodatadoc#LinguisticSystem -->


    <owl:Class rdf:about="http://www.theworldavatar.com/kg/ontodatadoc#LinguisticSystem"/>
    


    <!-- http://www.theworldavatar.com/kg/ontodatadoc#MissingData -->


    <owl:Class rdf:about="http://www.theworldavatar.com/kg/ontodatadoc#MissingData">
        <rdfs:comment>The missing data identifies instances where data points are absent or incomplete</rdfs:comment>
        <rdfs:isDefinedBy rdf:resource="http://www.theworldavatar.com/kg/ontodatadoc/"/>
        <rdfs:label>Missing Data</rdfs:label>
    </owl:Class>
    


    <!-- http://www.theworldavatar.com/kg/ontodatadoc#Publication -->


    <owl:Class rdf:about="http://www.theworldavatar.com/kg/ontodatadoc#Publication">
        <rdfs:comment>The publication documents the details related to the release or dissemination of the dataset</rdfs:comment>
        <rdfs:isDefinedBy rdf:resource="http://www.theworldavatar.com/kg/ontodatadoc/"/>
        <rdfs:label>Publication</rdfs:label>
    </owl:Class>
    


    <!-- http://www.theworldavatar.com/kg/ontodatadoc#Publisher -->


    <owl:Class rdf:about="http://www.theworldavatar.com/kg/ontodatadoc#Publisher">
        <rdfs:comment>The publisher specifies the entity or organisation responsible for making the dataset publicly available</rdfs:comment>
        <rdfs:isDefinedBy rdf:resource="http://www.theworldavatar.com/kg/ontodatadoc/"/>
        <rdfs:label>Publisher</rdfs:label>
    </owl:Class>
    


    <!-- http://www.theworldavatar.com/kg/ontodatadoc#QualitativeCharacteristic -->


    <owl:Class rdf:about="http://www.theworldavatar.com/kg/ontodatadoc#QualitativeCharacteristic">
        <rdfs:subClassOf rdf:resource="http://www.theworldavatar.com/kg/ontodatadoc#Characteristic"/>
        <rdfs:comment>The qualitative concept denotes data that is descriptive, non-numeric attributed, or categorical in nature</rdfs:comment>
        <rdfs:isDefinedBy rdf:resource="http://www.theworldavatar.com/kg/ontodatadoc/"/>
        <rdfs:label>QualitativeCharacteristic</rdfs:label>
    </owl:Class>
    


    <!-- http://www.theworldavatar.com/kg/ontodatadoc#QualityControl -->


    <owl:Class rdf:about="http://www.theworldavatar.com/kg/ontodatadoc#QualityControl">
        <rdfs:comment>The systematic process of verifying and validating data to ensure it meets standards of accuracy, completeness, consistency, and reliability.</rdfs:comment>
        <rdfs:isDefinedBy rdf:resource="http://www.theworldavatar.com/kg/ontodatadoc/"/>
        <rdfs:label>Quality Control</rdfs:label>
    </owl:Class>
    


    <!-- http://www.theworldavatar.com/kg/ontodatadoc#QuantitativeCharacteristic -->


    <owl:Class rdf:about="http://www.theworldavatar.com/kg/ontodatadoc#QuantitativeCharacteristic">
        <rdfs:subClassOf rdf:resource="http://www.theworldavatar.com/kg/ontodatadoc#Characteristic"/>
        <rdfs:comment>The quantitative concept signifies data content that is numerical or measurable</rdfs:comment>
        <rdfs:isDefinedBy rdf:resource="http://www.theworldavatar.com/kg/ontodatadoc/"/>
        <rdfs:label>QuantitativeCharacteristic</rdfs:label>
    </owl:Class>
    


    <!-- http://www.theworldavatar.com/kg/ontodatadoc#Subject -->


    <owl:Class rdf:about="http://www.theworldavatar.com/kg/ontodatadoc#Subject">
        <rdfs:comment>A subject captures the main topic or theme or concise description of the dataset</rdfs:comment>
        <rdfs:isDefinedBy rdf:resource="http://www.theworldavatar.com/kg/ontodatadoc/"/>
        <rdfs:label>Subject</rdfs:label>
    </owl:Class>
    


    <!-- http://www.theworldavatar.com/kg/ontodatadoc#TermsAndConditions -->


    <owl:Class rdf:about="http://www.theworldavatar.com/kg/ontodatadoc#TermsAndConditions">
        <rdfs:comment>The terms and conditions outline the legal and contractual terms such as  licensing, usage restrictions, and obligations associated with the dataset&apos;s usage</rdfs:comment>
        <rdfs:isDefinedBy rdf:resource="http://www.theworldavatar.com/kg/ontodatadoc/"/>
        <rdfs:label>Terms and Conditions</rdfs:label>
    </owl:Class>
    


    <!-- http://www.theworldavatar.com/kg/ontodatadoc#Unit -->


    <owl:Class rdf:about="http://www.theworldavatar.com/kg/ontodatadoc#Unit"/>
    


    <!-- http://www.theworldavatar.com/kg/ontodatadoc#UsabilityTesting -->


    <owl:Class rdf:about="http://www.theworldavatar.com/kg/ontodatadoc#UsabilityTesting">
        <rdfs:comment>The usability testing assesses the dataset&apos;s user-friendliness and ease of use</rdfs:comment>
        <rdfs:isDefinedBy rdf:resource="http://www.theworldavatar.com/kg/ontodatadoc/"/>
        <rdfs:label>Usability Testing</rdfs:label>
    </owl:Class>
    


    <!-- http://www.theworldavatar.com/kg/ontodatadoc#UsageGuideline -->


    <owl:Class rdf:about="http://www.theworldavatar.com/kg/ontodatadoc#UsageGuideline">
        <rdfs:subClassOf>
            <owl:Restriction>
                <owl:onProperty rdf:resource="http://purl.org/dc/terms/accessRights"/>
                <owl:someValuesFrom rdf:resource="http://purl.org/dc/terms/RightsStatement"/>
            </owl:Restriction>
        </rdfs:subClassOf>
        <rdfs:comment>The usage guideline instance outlines recommendations, terms and conditions, rights permission, etc. for effectively utilizing the dataset</rdfs:comment>
        <rdfs:isDefinedBy rdf:resource="http://www.theworldavatar.com/kg/ontodatadoc/"/>
        <rdfs:label>Usage Guideline</rdfs:label>
    </owl:Class>
    


    <!-- http://www.theworldavatar.com/kg/ontodatadoc#UserReview -->


    <owl:Class rdf:about="http://www.theworldavatar.com/kg/ontodatadoc#UserReview">
        <rdfs:comment>The user review captures feedback and reviews from users to increase the trust nd reliability</rdfs:comment>
        <rdfs:isDefinedBy rdf:resource="http://www.theworldavatar.com/kg/ontodatadoc/"/>
        <rdfs:label>User Review</rdfs:label>
    </owl:Class>
    


    <!-- http://www.theworldavatar.com/kg/ontodatadoc#Versioning -->


    <owl:Class rdf:about="http://www.theworldavatar.com/kg/ontodatadoc#Versioning">
        <rdfs:comment>A versioning instance tracks different versions or iterations of the dataset</rdfs:comment>
        <rdfs:isDefinedBy rdf:resource="http://www.theworldavatar.com/kg/ontodatadoc/"/>
        <rdfs:label>Versioning</rdfs:label>
    </owl:Class>
    


    <!-- http://www.w3.org/ns/dcat#Distribution -->


    <owl:Class rdf:about="http://www.w3.org/ns/dcat#Distribution">
        <rdfs:isDefinedBy rdf:resource="http://www.w3.org/ns/dcat"/>
        <rdfs:label>Distribution</rdfs:label>
    </owl:Class>
    


    <!-- http://www.w3.org/ns/odrl/2/Policy -->


    <owl:Class rdf:about="http://www.w3.org/ns/odrl/2/Policy">
        <rdfs:isDefinedBy rdf:resource="http://www.w3.org/ns/odrl/2/"/>
        <rdfs:label>Policy</rdfs:label>
    </owl:Class>
    


    <!-- http://www.w3.org/ns/prov#Activity -->


    <owl:Class rdf:about="http://www.w3.org/ns/prov#Activity"/>
    


    <!-- http://www.w3.org/ns/prov#Agent -->


    <owl:Class rdf:about="http://www.w3.org/ns/prov#Agent">
        <rdfs:comment>Agent can be a person, an organisation, and/or a software</rdfs:comment>
        <rdfs:isDefinedBy rdf:resource="http://www.w3.org/ns/prov"/>
        <rdfs:label>Agent</rdfs:label>
    </owl:Class>
</rdf:RDF>



<!-- Generated by the OWL API (version 5.5.0.2023-01-14T12:41:38Z) https://github.com/owlcs/owlapi/ -->


