<?xml version="1.0"?>
<rdf:RDF xmlns="https://www.theworldavatar.com/kg/ontobuiltenv/"
     xml:base="https://www.theworldavatar.com/kg/ontobuiltenv/"
     xmlns:dc="http://purl.org/dc/elements/1.1/"
     xmlns:owl="http://www.w3.org/2002/07/owl#"
     xmlns:rdf="http://www.w3.org/1999/02/22-rdf-syntax-ns#"
     xmlns:xml="http://www.w3.org/XML/1998/namespace"
     xmlns:xsd="http://www.w3.org/2001/XMLSchema#"
     xmlns:rdfs="http://www.w3.org/2000/01/rdf-schema#"
     xmlns:ontobuiltenv="https://www.theworldavatar.com/kg/ontobuiltenv/">
    <owl:Ontology rdf:about="https://www.theworldavatar.com/kg/ontobuiltenv/">
        <dc:date>20 May 2024</dc:date>
        <rdfs:comment>The Ontology for the Built Environment (OntoBuiltEnv) is an ontology developed for representing key information about properties (i.e. buildings as well as flats/apartments). It combines information about building usage, key construction characteristics, location and address, and estimated property value. More detailed geometric information can be retrieved from the associated OntoCityGml representation.</rdfs:comment>
        <owl:versionInfo>1</owl:versionInfo>
        <gitCommitHash>c0599beca8df55873a1ab061dee64e52c510c6a0</gitCommitHash>
    </owl:Ontology>
    


    <!-- 
    ///////////////////////////////////////////////////////////////////////////////////////
    //
    // Annotation properties
    //
    ///////////////////////////////////////////////////////////////////////////////////////
     -->


    


    <!-- http://purl.org/dc/elements/1.1/date -->


    <owl:AnnotationProperty rdf:about="http://purl.org/dc/elements/1.1/date"/>
    


    <!-- https://www.theworldavatar.com/kg/ontobuiltenv/gitCommitHash -->


    <owl:AnnotationProperty rdf:about="https://www.theworldavatar.com/kg/ontobuiltenv/gitCommitHash"/>
    


    <!-- 
    ///////////////////////////////////////////////////////////////////////////////////////
    //
    // Datatypes
    //
    ///////////////////////////////////////////////////////////////////////////////////////
     -->


    


    <!-- http://www.bigdata.com/rdf/geospatial/literals/v1#lat-lon -->


    <rdfs:Datatype rdf:about="http://www.bigdata.com/rdf/geospatial/literals/v1#lat-lon"/>
    


    <!-- 
    ///////////////////////////////////////////////////////////////////////////////////////
    //
    // Object Properties
    //
    ///////////////////////////////////////////////////////////////////////////////////////
     -->


    


    <!-- http://www.ontology-of-units-of-measure.org/resource/om-2/hasUnit -->


    <owl:ObjectProperty rdf:about="http://www.ontology-of-units-of-measure.org/resource/om-2/hasUnit">
        <rdfs:domain rdf:resource="http://www.ontology-of-units-of-measure.org/resource/om-2/Measure"/>
        <rdfs:range rdf:resource="http://www.ontology-of-units-of-measure.org/resource/om-2/Unit"/>
        <rdfs:isDefinedBy rdf:resource="http://www.ontology-of-units-of-measure.org/resource/om-2/"/>
        <rdfs:label>has unit</rdfs:label>
    </owl:ObjectProperty>
    


    <!-- http://www.ontology-of-units-of-measure.org/resource/om-2/hasValue -->


    <owl:ObjectProperty rdf:about="http://www.ontology-of-units-of-measure.org/resource/om-2/hasValue">
        <rdfs:domain>
            <owl:Class>
                <owl:unionOf rdf:parseType="Collection">
                    <rdf:Description rdf:about="http://www.ontology-of-units-of-measure.org/resource/om-2/AmountOfMoney"/>
                    <rdf:Description rdf:about="http://www.ontology-of-units-of-measure.org/resource/om-2/Area"/>
                    <rdf:Description rdf:about="http://www.ontology-of-units-of-measure.org/resource/om-2/Height"/>
                    <rdf:Description rdf:about="https://www.theworldavatar.com/kg/ontobuiltenv/AveragePricePerSqm"/>
                </owl:unionOf>
            </owl:Class>
        </rdfs:domain>
        <rdfs:range rdf:resource="http://www.ontology-of-units-of-measure.org/resource/om-2/Measure"/>
        <rdfs:isDefinedBy rdf:resource="http://www.ontology-of-units-of-measure.org/resource/om-2/"/>
        <rdfs:label>has value</rdfs:label>
    </owl:ObjectProperty>
    


    <!-- http://www.w3.org/2006/time#hasBeginning -->


    <owl:ObjectProperty rdf:about="http://www.w3.org/2006/time#hasBeginning">
        <rdfs:domain rdf:resource="http://www.w3.org/2006/time#Interval"/>
        <rdfs:range rdf:resource="http://www.w3.org/2006/time#Instant"/>
        <rdfs:isDefinedBy rdf:resource="http://www.w3.org/2006/time"/>
        <rdfs:label>has beginning</rdfs:label>
    </owl:ObjectProperty>
    


    <!-- http://www.w3.org/2006/time#hasEnd -->


    <owl:ObjectProperty rdf:about="http://www.w3.org/2006/time#hasEnd">
        <rdfs:domain rdf:resource="http://www.w3.org/2006/time#Interval"/>
        <rdfs:range rdf:resource="http://www.w3.org/2006/time#Instant"/>
        <rdfs:isDefinedBy rdf:resource="http://www.w3.org/2006/time"/>
        <rdfs:label>has end</rdfs:label>
    </owl:ObjectProperty>
    


    <!-- https://www.theworldavatar.com/kg/ontobuiltenv/hasAddress -->


    <owl:ObjectProperty rdf:about="https://www.theworldavatar.com/kg/ontobuiltenv/hasAddress">
        <rdfs:domain rdf:resource="https://www.theworldavatar.com/kg/ontobuiltenv/Property"/>
        <rdfs:range rdf:resource="http://ontology.eil.utoronto.ca/icontact.owl#Address"/>
        <rdfs:comment>A relationship between a property and its address.</rdfs:comment>
        <rdfs:isDefinedBy rdf:resource="https://www.theworldavatar.com/kg/ontobuiltenv/"/>
        <rdfs:label>has address</rdfs:label>
    </owl:ObjectProperty>
    


    <!-- https://www.theworldavatar.com/kg/ontobuiltenv/hasAdministrativeDistrict -->


    <owl:ObjectProperty rdf:about="https://www.theworldavatar.com/kg/ontobuiltenv/hasAdministrativeDistrict">
        <rdfs:domain rdf:resource="http://ontology.eil.utoronto.ca/icontact.owl#Address"/>
        <rdfs:range rdf:resource="https://www.theworldavatar.com/kg/ontobuiltenv/AdministrativeDistrict"/>
        <rdfs:comment>A relationship between an address and an encompassing administrative district.</rdfs:comment>
        <rdfs:isDefinedBy rdf:resource="https://www.theworldavatar.com/kg/ontobuiltenv/"/>
        <rdfs:label>has administrative district</rdfs:label>
    </owl:ObjectProperty>
    


    <!-- https://www.theworldavatar.com/kg/ontobuiltenv/hasBuiltForm -->


    <owl:ObjectProperty rdf:about="https://www.theworldavatar.com/kg/ontobuiltenv/hasBuiltForm">
        <rdfs:domain rdf:resource="https://www.theworldavatar.com/kg/ontobuiltenv/Property"/>
        <rdfs:range rdf:resource="https://www.theworldavatar.com/kg/ontobuiltenv/BuiltForm"/>
        <rdfs:comment>A relationship between a property and its built form.</rdfs:comment>
        <rdfs:isDefinedBy rdf:resource="https://www.theworldavatar.com/kg/ontobuiltenv/"/>
        <rdfs:label>has built form</rdfs:label>
    </owl:ObjectProperty>
    


    <!-- https://www.theworldavatar.com/kg/ontobuiltenv/hasConstructionComponent -->


    <owl:ObjectProperty rdf:about="https://www.theworldavatar.com/kg/ontobuiltenv/hasConstructionComponent">
        <rdfs:domain rdf:resource="https://www.theworldavatar.com/kg/ontobuiltenv/Property"/>
        <rdfs:range rdf:resource="https://www.theworldavatar.com/kg/ontobuiltenv/ConstructionComponent"/>
        <rdfs:comment>A relationship between a property and one of its key construction components.</rdfs:comment>
        <rdfs:isDefinedBy rdf:resource="https://www.theworldavatar.com/kg/ontobuiltenv/"/>
        <rdfs:label>has construction component</rdfs:label>
    </owl:ObjectProperty>
    


    <!-- https://www.theworldavatar.com/kg/ontobuiltenv/hasConstructionDate -->


    <owl:ObjectProperty rdf:about="https://www.theworldavatar.com/kg/ontobuiltenv/hasConstructionDate">
        <rdfs:domain rdf:resource="https://www.theworldavatar.com/kg/ontobuiltenv/Property"/>
        <rdfs:range rdf:resource="http://www.w3.org/2006/time#Interval"/>
        <rdfs:comment>A relationship between a property and its construction dates.</rdfs:comment>
        <rdfs:isDefinedBy rdf:resource="https://www.theworldavatar.com/kg/ontobuiltenv/"/>
        <rdfs:label>has construction date</rdfs:label>
    </owl:ObjectProperty>
    


    <!-- https://www.theworldavatar.com/kg/ontobuiltenv/hasEstimatedConstructionCost -->


    <owl:ObjectProperty rdf:about="https://www.theworldavatar.com/kg/ontobuiltenv/hasEstimatedConstructionCost">
        <rdfs:domain rdf:resource="https://www.theworldavatar.com/kg/ontobuiltenv/Property"/>
        <rdfs:range rdf:resource="http://www.ontology-of-units-of-measure.org/resource/om-2/Cost"/>
        <rdfs:comment>A relationship between a building and its estimated construction cost.</rdfs:comment>
        <rdfs:isDefinedBy rdf:resource="https://www.theworldavatar.com/kg/ontobuiltenv/"/>
        <rdfs:label>has estimated construction cost</rdfs:label>
    </owl:ObjectProperty>
    


    <!-- https://www.theworldavatar.com/kg/ontobuiltenv/hasGroundElevation -->


    <owl:ObjectProperty rdf:about="https://www.theworldavatar.com/kg/ontobuiltenv/hasGroundElevation">
        <rdfs:domain rdf:resource="http://www.purl.org/oema/infrastructure/Building"/>
        <rdfs:range rdf:resource="http://www.ontology-of-units-of-measure.org/resource/om-2/Height"/>
        <rdfs:comment>A relationship between a building and its ground elevation.</rdfs:comment>
        <rdfs:isDefinedBy rdf:resource="https://www.theworldavatar.com/kg/ontobuiltenv/"/>
        <rdfs:label>has ground elevation</rdfs:label>
    </owl:ObjectProperty>
    


    <!-- https://www.theworldavatar.com/kg/ontobuiltenv/hasInstalledPVArea -->


    <owl:ObjectProperty rdf:about="https://www.theworldavatar.com/kg/ontobuiltenv/hasInstalledPVArea">
        <rdfs:domain rdf:resource="http://www.purl.org/oema/infrastructure/Building"/>
        <rdfs:range rdf:resource="http://www.ontology-of-units-of-measure.org/resource/om-2/Area"/>
        <rdfs:comment>A relationship between a building and its total installed photovoltaics area.</rdfs:comment>
        <rdfs:isDefinedBy rdf:resource="https://www.theworldavatar.com/kg/ontobuiltenv/"/>
        <rdfs:label>has installed PV area</rdfs:label>
    </owl:ObjectProperty>
    


    <!-- https://www.theworldavatar.com/kg/ontobuiltenv/hasLatestTransactionRecord -->


    <owl:ObjectProperty rdf:about="https://www.theworldavatar.com/kg/ontobuiltenv/hasLatestTransactionRecord">
        <rdfs:domain rdf:resource="https://www.theworldavatar.com/kg/ontobuiltenv/Property"/>
        <rdfs:range rdf:resource="http://landregistry.data.gov.uk/def/ppi/TransactionRecord"/>
        <rdfs:comment>A relationship between a property and its latest transaction record.</rdfs:comment>
        <rdfs:isDefinedBy rdf:resource="https://www.theworldavatar.com/kg/ontobuiltenv/"/>
        <rdfs:label>has latest transaction record</rdfs:label>
    </owl:ObjectProperty>
    


    <!-- https://www.theworldavatar.com/kg/ontobuiltenv/hasMarketValue -->


    <owl:ObjectProperty rdf:about="https://www.theworldavatar.com/kg/ontobuiltenv/hasMarketValue">
        <rdfs:domain rdf:resource="https://www.theworldavatar.com/kg/ontobuiltenv/Property"/>
        <rdfs:range rdf:resource="http://www.ontology-of-units-of-measure.org/resource/om-2/AmountOfMoney"/>
        <rdfs:comment>A relationship between a property and its (estimated) property value.</rdfs:comment>
        <rdfs:isDefinedBy rdf:resource="https://www.theworldavatar.com/kg/ontobuiltenv/"/>
        <rdfs:label>has market value</rdfs:label>
    </owl:ObjectProperty>
    


    <!-- https://www.theworldavatar.com/kg/ontobuiltenv/hasNumberOfFloors -->


    <owl:ObjectProperty rdf:about="https://www.theworldavatar.com/kg/ontobuiltenv/hasNumberOfFloors">
        <rdfs:domain rdf:resource="https://www.theworldavatar.com/kg/ontobuiltenv/Property"/>
        <rdfs:range rdf:resource="https://www.theworldavatar.com/kg/ontobuiltenv/NumberOfFloors"/>
        <rdfs:comment>A relationship between a property and its number of floors.</rdfs:comment>
        <rdfs:isDefinedBy rdf:resource="https://www.theworldavatar.com/kg/ontobuiltenv/"/>
        <rdfs:label>has number of floors</rdfs:label>
    </owl:ObjectProperty>
    


    <!-- https://www.theworldavatar.com/kg/ontobuiltenv/hasOntoCityGMLRepresentation -->


    <owl:ObjectProperty rdf:about="https://www.theworldavatar.com/kg/ontobuiltenv/hasOntoCityGMLRepresentation">
        <rdfs:domain rdf:resource="http://www.purl.org/oema/infrastructure/Building"/>
        <rdfs:range rdf:resource="http://www.w3.org/2002/07/owl#Thing"/>
        <rdfs:comment>A relationship between a building and its corresponding instance IRI in OntoCityGml.</rdfs:comment>
        <rdfs:isDefinedBy rdf:resource="https://www.theworldavatar.com/kg/ontobuiltenv/"/>
        <rdfs:label>has OntoCityGML representation</rdfs:label>
    </owl:ObjectProperty>
    


    <!-- https://www.theworldavatar.com/kg/ontobuiltenv/hasPVsuitableRoofArea -->


    <owl:ObjectProperty rdf:about="https://www.theworldavatar.com/kg/ontobuiltenv/hasPVsuitableRoofArea">
        <rdfs:domain rdf:resource="http://www.purl.org/oema/infrastructure/Building"/>
        <rdfs:range rdf:resource="http://www.ontology-of-units-of-measure.org/resource/om-2/Area"/>
        <rdfs:comment>A relationship between a building and its roof area suitable for photovoltaics installation.</rdfs:comment>
        <rdfs:isDefinedBy rdf:resource="https://www.theworldavatar.com/kg/ontobuiltenv/"/>
        <rdfs:label>has roof area suitable for PV</rdfs:label>
    </owl:ObjectProperty>
    


    <!-- https://www.theworldavatar.com/kg/ontobuiltenv/hasPostalCode -->


    <owl:ObjectProperty rdf:about="https://www.theworldavatar.com/kg/ontobuiltenv/hasPostalCode">
        <rdfs:domain rdf:resource="http://ontology.eil.utoronto.ca/icontact.owl#Address"/>
        <rdfs:range rdf:resource="https://www.theworldavatar.com/kg/ontobuiltenv/PostalCode"/>
        <rdfs:comment>A relationship between an address and the respective postal code.</rdfs:comment>
        <rdfs:isDefinedBy rdf:resource="https://www.theworldavatar.com/kg/ontobuiltenv/"/>
        <rdfs:label>has postal code</rdfs:label>
    </owl:ObjectProperty>
    


    <!-- https://www.theworldavatar.com/kg/ontobuiltenv/hasPropertyType -->


    <owl:ObjectProperty rdf:about="https://www.theworldavatar.com/kg/ontobuiltenv/hasPropertyType">
        <rdfs:domain rdf:resource="https://www.theworldavatar.com/kg/ontobuiltenv/Property"/>
        <rdfs:range rdf:resource="https://www.theworldavatar.com/kg/ontobuiltenv/PropertyType"/>
        <rdfs:comment>A relationship between a property and its property type.</rdfs:comment>
        <rdfs:isDefinedBy rdf:resource="https://www.theworldavatar.com/kg/ontobuiltenv/"/>
        <rdfs:label>has property type</rdfs:label>
    </owl:ObjectProperty>
    


    <!-- https://www.theworldavatar.com/kg/ontobuiltenv/hasPropertyUsage -->


    <owl:ObjectProperty rdf:about="https://www.theworldavatar.com/kg/ontobuiltenv/hasPropertyUsage">
        <rdfs:domain rdf:resource="https://www.theworldavatar.com/kg/ontobuiltenv/Property"/>
        <rdfs:range rdf:resource="https://www.theworldavatar.com/kg/ontobuiltenv/PropertyUsage"/>
        <rdfs:comment>A relationship between a property and its (intended) usage and/or function.</rdfs:comment>
        <rdfs:isDefinedBy rdf:resource="https://www.theworldavatar.com/kg/ontobuiltenv/"/>
        <rdfs:label>has property usage</rdfs:label>
    </owl:ObjectProperty>
    


    <!-- https://www.theworldavatar.com/kg/ontobuiltenv/hasTotalFloorArea -->


    <owl:ObjectProperty rdf:about="https://www.theworldavatar.com/kg/ontobuiltenv/hasTotalFloorArea">
        <rdfs:domain rdf:resource="https://www.theworldavatar.com/kg/ontobuiltenv/Property"/>
        <rdfs:range rdf:resource="http://www.ontology-of-units-of-measure.org/resource/om-2/Area"/>
        <rdfs:comment>A relationship between a property and its total floor area.</rdfs:comment>
        <rdfs:isDefinedBy rdf:resource="https://www.theworldavatar.com/kg/ontobuiltenv/"/>
        <rdfs:label>has total floor area</rdfs:label>
    </owl:ObjectProperty>
    


    <!-- https://www.theworldavatar.com/kg/ontobuiltenv/hasTotalRoofArea -->


    <owl:ObjectProperty rdf:about="https://www.theworldavatar.com/kg/ontobuiltenv/hasTotalRoofArea">
        <rdfs:domain rdf:resource="http://www.purl.org/oema/infrastructure/Building"/>
        <rdfs:range rdf:resource="http://www.ontology-of-units-of-measure.org/resource/om-2/Area"/>
        <rdfs:comment>A relationship between a building and its total roof area.</rdfs:comment>
        <rdfs:isDefinedBy rdf:resource="https://www.theworldavatar.com/kg/ontobuiltenv/"/>
        <rdfs:label>has total roof area</rdfs:label>
    </owl:ObjectProperty>
    


    <!-- https://www.theworldavatar.com/kg/ontobuiltenv/isIn -->


    <owl:ObjectProperty rdf:about="https://www.theworldavatar.com/kg/ontobuiltenv/isIn">
        <rdfs:domain rdf:resource="https://www.theworldavatar.com/kg/ontobuiltenv/Flat"/>
        <rdfs:range rdf:resource="http://www.purl.org/oema/infrastructure/Building"/>
        <rdfs:comment>A relationship between a flat/apartment and its parent building it is contained within.</rdfs:comment>
        <rdfs:isDefinedBy rdf:resource="https://www.theworldavatar.com/kg/ontobuiltenv/"/>
        <rdfs:label>is in</rdfs:label>
    </owl:ObjectProperty>
    


    <!-- https://www.theworldavatar.com/kg/ontobuiltenv/isPresumedMatchOf -->


    <owl:ObjectProperty rdf:about="https://www.theworldavatar.com/kg/ontobuiltenv/isPresumedMatchOf">
        <rdfs:domain rdf:resource="http://ontology.eil.utoronto.ca/icontact.owl#Address"/>
        <rdfs:range rdf:resource="http://www.w3.org/2002/07/owl#Thing"/>
        <rdfs:comment>A relationship between an address and a presumed match of the address in another knowledge base.</rdfs:comment>
        <rdfs:isDefinedBy rdf:resource="https://www.theworldavatar.com/kg/ontobuiltenv/"/>
        <rdfs:label>has presumed match</rdfs:label>
    </owl:ObjectProperty>
    


    <!-- https://www.theworldavatar.com/kg/ontobuiltenv/locatedIn -->


    <owl:ObjectProperty rdf:about="https://www.theworldavatar.com/kg/ontobuiltenv/locatedIn">
        <rdfs:domain rdf:resource="https://www.theworldavatar.com/kg/ontobuiltenv/Property"/>
        <rdfs:range rdf:resource="https://www.theworldavatar.com/kg/ontobuiltenv/AdministrativeDistrict"/>
        <rdfs:comment>A relationship between a property and an encompassing administrative district.</rdfs:comment>
        <rdfs:isDefinedBy rdf:resource="https://www.theworldavatar.com/kg/ontobuiltenv/"/>
        <rdfs:label>located in</rdfs:label>
    </owl:ObjectProperty>
    


    <!-- https://www.theworldavatar.com/kg/ontobuiltenv/representativeFor -->


    <owl:ObjectProperty rdf:about="https://www.theworldavatar.com/kg/ontobuiltenv/representativeFor">
        <rdfs:domain rdf:resource="https://www.theworldavatar.com/kg/ontobuiltenv/AveragePricePerSqm"/>
        <rdfs:domain rdf:resource="https://www.theworldavatar.com/kg/ontobuiltenv/PropertyPriceIndex"/>
        <rdfs:range rdf:resource="https://www.theworldavatar.com/kg/ontobuiltenv/AdministrativeDistrict"/>
        <rdfs:range rdf:resource="https://www.theworldavatar.com/kg/ontobuiltenv/PostalCode"/>
        <rdfs:comment>A relationship between a property price index and the area it refers to.</rdfs:comment>
        <rdfs:comment>A relationship between the average price per square metre and the area it refers to.</rdfs:comment>
        <rdfs:isDefinedBy rdf:resource="https://www.theworldavatar.com/kg/ontobuiltenv/"/>
        <rdfs:label>representative for</rdfs:label>
    </owl:ObjectProperty>
    


    <!-- https://www.theworldavatar.com/kg/ontotimeseries/hasTimeSeries -->


    <owl:ObjectProperty rdf:about="https://www.theworldavatar.com/kg/ontotimeseries/hasTimeSeries">
        <rdfs:domain rdf:resource="https://www.theworldavatar.com/kg/ontobuiltenv/PropertyPriceIndex"/>
        <rdfs:range rdf:resource="https://www.theworldavatar.com/kg/ontotimeseries/TimeSeries"/>
        <rdfs:comment>A relationship between the property price index and its actual time series history.</rdfs:comment>
        <rdfs:isDefinedBy rdf:resource="https://www.theworldavatar.com/kg/ontobuiltenv/"/>
        <rdfs:label>has time series</rdfs:label>
    </owl:ObjectProperty>
    


    <!-- 
    ///////////////////////////////////////////////////////////////////////////////////////
    //
    // Data properties
    //
    ///////////////////////////////////////////////////////////////////////////////////////
     -->


    


    <!-- http://landregistry.data.gov.uk/def/ppi/pricePaid -->


    <owl:DatatypeProperty rdf:about="http://landregistry.data.gov.uk/def/ppi/pricePaid">
        <rdfs:domain rdf:resource="http://landregistry.data.gov.uk/def/ppi/TransactionRecord"/>
        <rdfs:range rdf:resource="http://www.w3.org/2001/XMLSchema#integer"/>
        <rdfs:comment>A relationship between a transaction record and the associated transaction price.</rdfs:comment>
        <rdfs:isDefinedBy rdf:resource="https://www.theworldavatar.com/kg/ontobuiltenv/"/>
        <rdfs:label>Price paid</rdfs:label>
    </owl:DatatypeProperty>
    


    <!-- http://landregistry.data.gov.uk/def/ppi/transactionDate -->


    <owl:DatatypeProperty rdf:about="http://landregistry.data.gov.uk/def/ppi/transactionDate">
        <rdfs:domain rdf:resource="http://landregistry.data.gov.uk/def/ppi/TransactionRecord"/>
        <rdfs:range rdf:resource="http://www.w3.org/2001/XMLSchema#string"/>
        <rdfs:comment>A relationship between a transaction record and the associated transaction data.</rdfs:comment>
        <rdfs:isDefinedBy rdf:resource="https://www.theworldavatar.com/kg/ontobuiltenv/"/>
        <rdfs:label>Transaction date</rdfs:label>
    </owl:DatatypeProperty>
    


    <!-- http://ontology.eil.utoronto.ca/icontact.owl#hasBuilding -->


    <owl:DatatypeProperty rdf:about="http://ontology.eil.utoronto.ca/icontact.owl#hasBuilding">
        <rdfs:domain rdf:resource="http://ontology.eil.utoronto.ca/icontact.owl#Address"/>
        <rdfs:range rdf:resource="http://www.w3.org/2001/XMLSchema#string"/>
        <rdfs:comment>Name of the building where the address is located.  Often used in countries like England, India and Japan.</rdfs:comment>
        <rdfs:isDefinedBy rdf:resource="http://ontology.eil.utoronto.ca/icontact.owl"/>
        <rdfs:label>has building name</rdfs:label>
    </owl:DatatypeProperty>
    


    <!-- http://ontology.eil.utoronto.ca/icontact.owl#hasStreet -->


    <owl:DatatypeProperty rdf:about="http://ontology.eil.utoronto.ca/icontact.owl#hasStreet">
        <rdfs:domain rdf:resource="http://ontology.eil.utoronto.ca/icontact.owl#Address"/>
        <rdfs:range rdf:resource="http://www.w3.org/2001/XMLSchema#string"/>
        <rdfs:comment>A relationship between an address and the respective street name.</rdfs:comment>
        <rdfs:isDefinedBy rdf:resource="http://ontology.eil.utoronto.ca/icontact.owl"/>
        <rdfs:label>has street</rdfs:label>
    </owl:DatatypeProperty>
    


    <!-- http://ontology.eil.utoronto.ca/icontact.owl#hasStreetNumber -->


    <owl:DatatypeProperty rdf:about="http://ontology.eil.utoronto.ca/icontact.owl#hasStreetNumber">
        <rdfs:domain rdf:resource="http://ontology.eil.utoronto.ca/icontact.owl#Address"/>
        <rdfs:range rdf:resource="http://www.w3.org/2001/XMLSchema#string"/>
        <rdfs:comment>A relationship between an address and the respective street/house number.</rdfs:comment>
        <rdfs:isDefinedBy rdf:resource="http://ontology.eil.utoronto.ca/icontact.owl"/>
        <rdfs:label>has street number</rdfs:label>
    </owl:DatatypeProperty>
    


    <!-- http://www.ontology-of-units-of-measure.org/resource/om-2/hasNumericalValue -->


    <owl:DatatypeProperty rdf:about="http://www.ontology-of-units-of-measure.org/resource/om-2/hasNumericalValue">
        <rdfs:domain rdf:resource="http://www.ontology-of-units-of-measure.org/resource/om-2/Measure"/>
        <rdfs:range rdf:resource="http://www.w3.org/2001/XMLSchema#float"/>
        <rdfs:isDefinedBy rdf:resource="http://www.ontology-of-units-of-measure.org/resource/om-2/"/>
        <rdfs:label>has numerical value</rdfs:label>
    </owl:DatatypeProperty>
    


    <!-- http://www.ontology-of-units-of-measure.org/resource/om-2/symbol -->


    <owl:DatatypeProperty rdf:about="http://www.ontology-of-units-of-measure.org/resource/om-2/symbol">
        <rdfs:domain rdf:resource="http://www.ontology-of-units-of-measure.org/resource/om-2/Unit"/>
        <rdfs:range rdf:resource="http://www.w3.org/2001/XMLSchema#string"/>
        <rdfs:isDefinedBy rdf:resource="http://www.ontology-of-units-of-measure.org/resource/om-2/"/>
        <rdfs:label>symbol</rdfs:label>
    </owl:DatatypeProperty>
    


    <!-- http://www.w3.org/2000/01/rdf-schema#label -->


    <owl:DatatypeProperty rdf:about="http://www.w3.org/2000/01/rdf-schema#label">
        <rdfs:domain rdf:resource="https://www.theworldavatar.com/kg/ontobuiltenv/AdministrativeDistrict"/>
        <rdfs:domain rdf:resource="https://www.theworldavatar.com/kg/ontobuiltenv/PostalCode"/>
        <rdfs:domain rdf:resource="https://www.theworldavatar.com/kg/ontobuiltenv/PropertyUsage"/>
        <rdfs:range rdf:resource="http://www.w3.org/2001/XMLSchema#string"/>
    </owl:DatatypeProperty>
    


    <!-- http://www.w3.org/2006/time#inXSDDateTimeStamp -->


    <owl:DatatypeProperty rdf:about="http://www.w3.org/2006/time#inXSDDateTimeStamp">
        <rdfs:domain rdf:resource="http://www.w3.org/2006/time#Instant"/>
        <rdfs:range rdf:resource="http://www.w3.org/2001/XMLSchema#string"/>
        <rdfs:isDefinedBy rdf:resource="http://www.w3.org/2006/time"/>
        <rdfs:label>in XSD dateTimeStamp</rdfs:label>
    </owl:DatatypeProperty>
    


    <!-- https://www.theworldavatar.com/kg/ontobuiltenv/hasEnergyRating -->


    <owl:DatatypeProperty rdf:about="https://www.theworldavatar.com/kg/ontobuiltenv/hasEnergyRating">
        <rdfs:domain rdf:resource="https://www.theworldavatar.com/kg/ontobuiltenv/Property"/>
        <rdfs:range rdf:resource="http://www.w3.org/2001/XMLSchema#string"/>
        <rdfs:comment>A relationship between a property and its overall energy efficiency rating (e.g. linear &apos;A to G&apos; rating (where A is the most energy efficient and G is the least energy efficient))</rdfs:comment>
        <rdfs:isDefinedBy rdf:resource="https://www.theworldavatar.com/kg/ontobuiltenv/"/>
        <rdfs:label>has energy rating</rdfs:label>
    </owl:DatatypeProperty>
    


    <!-- https://www.theworldavatar.com/kg/ontobuiltenv/hasGFA -->


    <owl:DatatypeProperty rdf:about="https://www.theworldavatar.com/kg/ontobuiltenv/hasGFA">
        <rdfs:domain rdf:resource="https://www.theworldavatar.com/kg/ontobuiltenv/Property"/>
        <rdfs:range rdf:resource="http://www.w3.org/2001/XMLSchema#float"/>
        <rdfs:comment>A relationship between a building and its Gross Floor Area value.</rdfs:comment>
        <rdfs:isDefinedBy rdf:resource="https://www.theworldavatar.com/kg/ontobuiltenv/"/>
        <rdfs:label>has GFA</rdfs:label>
    </owl:DatatypeProperty>
    


    <!-- https://www.theworldavatar.com/kg/ontobuiltenv/hasIdentifier -->


    <owl:DatatypeProperty rdf:about="https://www.theworldavatar.com/kg/ontobuiltenv/hasIdentifier">
        <rdfs:domain rdf:resource="https://www.theworldavatar.com/kg/ontobuiltenv/Property"/>
        <rdfs:range rdf:resource="http://www.w3.org/2001/XMLSchema#string"/>
        <rdfs:comment>Unique identifier describing the property.</rdfs:comment>
        <rdfs:isDefinedBy rdf:resource="https://www.theworldavatar.com/kg/ontobuiltenv/"/>
        <rdfs:label>has identifier</rdfs:label>
    </owl:DatatypeProperty>
    


    <!-- https://www.theworldavatar.com/kg/ontobuiltenv/hasLatestEPC -->


    <owl:DatatypeProperty rdf:about="https://www.theworldavatar.com/kg/ontobuiltenv/hasLatestEPC">
        <rdfs:domain rdf:resource="https://www.theworldavatar.com/kg/ontobuiltenv/Property"/>
        <rdfs:range rdf:resource="http://www.w3.org/2001/XMLSchema#string"/>
        <rdfs:comment>A relationship between a property and its latest Energy Performance record (i.e. unique lodgement identifier).</rdfs:comment>
        <rdfs:isDefinedBy rdf:resource="https://www.theworldavatar.com/kg/ontobuiltenv/"/>
        <rdfs:label>latest EPC</rdfs:label>
    </owl:DatatypeProperty>
    


    <!-- https://www.theworldavatar.com/kg/ontobuiltenv/hasNumberOfHabitableRooms -->


    <owl:DatatypeProperty rdf:about="https://www.theworldavatar.com/kg/ontobuiltenv/hasNumberOfHabitableRooms">
        <rdfs:domain rdf:resource="https://www.theworldavatar.com/kg/ontobuiltenv/Property"/>
        <rdfs:range rdf:resource="http://www.w3.org/2001/XMLSchema#integer"/>
        <rdfs:comment>A relationship between a property and its total number of habitable rooms.</rdfs:comment>
        <rdfs:isDefinedBy rdf:resource="https://www.theworldavatar.com/kg/ontobuiltenv/"/>
        <rdfs:label>has number of habitable rooms</rdfs:label>
    </owl:DatatypeProperty>
    


    <!-- https://www.theworldavatar.com/kg/ontobuiltenv/hasUnitName -->


    <owl:DatatypeProperty rdf:about="https://www.theworldavatar.com/kg/ontobuiltenv/hasUnitName">
        <rdfs:domain rdf:resource="http://ontology.eil.utoronto.ca/icontact.owl#Address"/>
        <rdfs:range rdf:resource="http://www.w3.org/2001/XMLSchema#string"/>
        <rdfs:comment>A relationship between an address and the respective unit number, incl. potential description of the unit (e.g. &quot;Flat 1&quot;, &quot;Apartment A&quot;).</rdfs:comment>
        <rdfs:isDefinedBy rdf:resource="https://www.theworldavatar.com/kg/ontobuiltenv/"/>
        <rdfs:label>has unit name</rdfs:label>
    </owl:DatatypeProperty>
    


    <!-- https://www.theworldavatar.com/kg/ontobuiltenv/hasUsageShare -->


    <owl:DatatypeProperty rdf:about="https://www.theworldavatar.com/kg/ontobuiltenv/hasUsageShare">
        <rdfs:domain rdf:resource="https://www.theworldavatar.com/kg/ontobuiltenv/PropertyUsage"/>
        <rdfs:range rdf:resource="http://www.w3.org/2001/XMLSchema#float"/>
        <rdfs:comment>A relationship between a property usage and its relative share if property has multiple usages associated with it (between 0 and 1).</rdfs:comment>
        <rdfs:isDefinedBy rdf:resource="https://www.theworldavatar.com/kg/ontobuiltenv/"/>
        <rdfs:label>usage share</rdfs:label>
    </owl:DatatypeProperty>
    


    <!-- https://www.theworldavatar.com/kg/ontobuiltenv/hasValue -->


    <owl:DatatypeProperty rdf:about="https://www.theworldavatar.com/kg/ontobuiltenv/hasValue">
        <rdfs:domain rdf:resource="https://www.theworldavatar.com/kg/ontobuiltenv/NumberOfFloors"/>
        <rdfs:range rdf:resource="http://www.w3.org/2001/XMLSchema#integer"/>
        <rdfs:comment>A relationship between the number of floors and its numerical value.</rdfs:comment>
        <rdfs:isDefinedBy rdf:resource="https://www.theworldavatar.com/kg/ontobuiltenv/"/>
        <rdfs:label>has value</rdfs:label>
    </owl:DatatypeProperty>
    


    <!-- https://www.theworldavatar.com/kg/ontobuiltenv/hasWGS84LatitudeLongitude -->


    <owl:DatatypeProperty rdf:about="https://www.theworldavatar.com/kg/ontobuiltenv/hasWGS84LatitudeLongitude">
        <rdfs:domain rdf:resource="https://www.theworldavatar.com/kg/ontobuiltenv/Property"/>
        <rdfs:range rdf:resource="http://www.bigdata.com/rdf/geospatial/literals/v1#lat-lon"/>
        <rdfs:comment>Location of property footprint centroid in WGS84 coordinates.</rdfs:comment>
        <rdfs:isDefinedBy rdf:resource="https://www.theworldavatar.com/kg/ontobuiltenv/"/>
        <rdfs:label>has WGS84 coordinates</rdfs:label>
    </owl:DatatypeProperty>
    


    <!-- https://www.theworldavatar.com/kg/ontotimeseries/hasRDB -->


    <owl:DatatypeProperty rdf:about="https://www.theworldavatar.com/kg/ontotimeseries/hasRDB">
        <rdfs:domain rdf:resource="https://www.theworldavatar.com/kg/ontotimeseries/TimeSeries"/>
        <rdfs:range rdf:resource="http://www.w3.org/2001/XMLSchema#string"/>
        <rdfs:isDefinedBy rdf:resource="https://www.theworldavatar.com/kg/ontotimeseries/"/>
        <rdfs:label>has RDB link</rdfs:label>
    </owl:DatatypeProperty>
    


    <!-- https://www.theworldavatar.com/kg/ontotimeseries/hasTimeUnit -->


    <owl:DatatypeProperty rdf:about="https://www.theworldavatar.com/kg/ontotimeseries/hasTimeUnit">
        <rdfs:domain rdf:resource="https://www.theworldavatar.com/kg/ontotimeseries/TimeSeries"/>
        <rdfs:range rdf:resource="http://www.w3.org/2001/XMLSchema#string"/>
        <rdfs:isDefinedBy rdf:resource="https://www.theworldavatar.com/kg/ontotimeseries/"/>
        <rdfs:label>has time unit</rdfs:label>
    </owl:DatatypeProperty>
    


    <!-- 
    ///////////////////////////////////////////////////////////////////////////////////////
    //
    // Classes
    //
    ///////////////////////////////////////////////////////////////////////////////////////
     -->


    


    <!-- http://bimerr.iot.linkeddata.es/def/building#Building -->


    <owl:Class rdf:about="http://bimerr.iot.linkeddata.es/def/building#Building">
        <owl:equivalentClass rdf:resource="http://www.purl.org/oema/infrastructure/Building"/>
    </owl:Class>
    


    <!-- http://landregistry.data.gov.uk/def/ppi/TransactionRecord -->


    <owl:Class rdf:about="http://landregistry.data.gov.uk/def/ppi/TransactionRecord">
        <rdfs:comment>A transaction record describes a single previous transaction (i.e. sale) of a property.</rdfs:comment>
        <rdfs:isDefinedBy rdf:resource="http://landregistry.data.gov.uk/def/ppi/"/>
        <rdfs:label>Transaction record</rdfs:label>
    </owl:Class>
    


    <!-- http://ontology.eil.utoronto.ca/icity/Building/Building -->


    <owl:Class rdf:about="http://ontology.eil.utoronto.ca/icity/Building/Building">
        <owl:equivalentClass rdf:resource="http://www.purl.org/oema/infrastructure/Building"/>
    </owl:Class>
    


    <!-- http://ontology.eil.utoronto.ca/icontact.owl#Address -->


    <owl:Class rdf:about="http://ontology.eil.utoronto.ca/icontact.owl#Address">
        <rdfs:subClassOf>
            <owl:Restriction>
                <owl:onProperty rdf:resource="https://www.theworldavatar.com/kg/ontobuiltenv/hasPostalCode"/>
                <owl:qualifiedCardinality rdf:datatype="http://www.w3.org/2001/XMLSchema#nonNegativeInteger">1</owl:qualifiedCardinality>
                <owl:onClass rdf:resource="https://www.theworldavatar.com/kg/ontobuiltenv/PostalCode"/>
            </owl:Restriction>
        </rdfs:subClassOf>
    </owl:Class>
    


    <!-- http://www.google.com/digitalbuildings/0.0.1/facilities#Building -->


    <owl:Class rdf:about="http://www.google.com/digitalbuildings/0.0.1/facilities#Building">
        <owl:equivalentClass rdf:resource="http://www.purl.org/oema/infrastructure/Building"/>
    </owl:Class>
    


    <!-- http://www.ontology-of-units-of-measure.org/resource/om-2/AmountOfMoney -->


    <owl:Class rdf:about="http://www.ontology-of-units-of-measure.org/resource/om-2/AmountOfMoney"/>
    


    <!-- http://www.ontology-of-units-of-measure.org/resource/om-2/Area -->


    <owl:Class rdf:about="http://www.ontology-of-units-of-measure.org/resource/om-2/Area"/>
    


    <!-- http://www.ontology-of-units-of-measure.org/resource/om-2/Cost -->


    <owl:Class rdf:about="http://www.ontology-of-units-of-measure.org/resource/om-2/Cost"/>
    


    <!-- http://www.ontology-of-units-of-measure.org/resource/om-2/Height -->


    <owl:Class rdf:about="http://www.ontology-of-units-of-measure.org/resource/om-2/Height"/>
    


    <!-- http://www.ontology-of-units-of-measure.org/resource/om-2/Measure -->


    <owl:Class rdf:about="http://www.ontology-of-units-of-measure.org/resource/om-2/Measure"/>
    


    <!-- http://www.ontology-of-units-of-measure.org/resource/om-2/Unit -->


    <owl:Class rdf:about="http://www.ontology-of-units-of-measure.org/resource/om-2/Unit"/>
    


    <!-- http://www.opengis.net/ont/geosparql#Feature -->


    <owl:Class rdf:about="http://www.opengis.net/ont/geosparql#Feature"/>
    


    <!-- http://www.purl.org/oema/infrastructure/Building -->


    <owl:Class rdf:about="http://www.purl.org/oema/infrastructure/Building">
        <owl:equivalentClass rdf:resource="https://standards.buildingsmart.org/IFC/DEV/IFC4/ADD2_TC1/OWL#IfcBuilding"/>
        <owl:equivalentClass rdf:resource="https://w3id.org/bot#Building"/>
        <rdfs:subClassOf rdf:resource="http://www.opengis.net/ont/geosparql#Feature"/>
        <rdfs:subClassOf rdf:resource="https://www.theworldavatar.com/kg/ontobuiltenv/Property"/>
        <rdfs:subClassOf>
            <owl:Restriction>
                <owl:onProperty rdf:resource="https://www.theworldavatar.com/kg/ontobuiltenv/hasGroundElevation"/>
                <owl:qualifiedCardinality rdf:datatype="http://www.w3.org/2001/XMLSchema#nonNegativeInteger">1</owl:qualifiedCardinality>
                <owl:onClass rdf:resource="http://www.ontology-of-units-of-measure.org/resource/om-2/Height"/>
            </owl:Restriction>
        </rdfs:subClassOf>
        <rdfs:subClassOf>
            <owl:Restriction>
                <owl:onProperty rdf:resource="https://www.theworldavatar.com/kg/ontobuiltenv/hasInstalledPVArea"/>
                <owl:qualifiedCardinality rdf:datatype="http://www.w3.org/2001/XMLSchema#nonNegativeInteger">1</owl:qualifiedCardinality>
                <owl:onClass rdf:resource="http://www.ontology-of-units-of-measure.org/resource/om-2/Area"/>
            </owl:Restriction>
        </rdfs:subClassOf>
        <rdfs:subClassOf>
            <owl:Restriction>
                <owl:onProperty rdf:resource="https://www.theworldavatar.com/kg/ontobuiltenv/hasOntoCityGMLRepresentation"/>
                <owl:cardinality rdf:datatype="http://www.w3.org/2001/XMLSchema#nonNegativeInteger">1</owl:cardinality>
            </owl:Restriction>
        </rdfs:subClassOf>
        <rdfs:subClassOf>
            <owl:Restriction>
                <owl:onProperty rdf:resource="https://www.theworldavatar.com/kg/ontobuiltenv/hasPVsuitableRoofArea"/>
                <owl:qualifiedCardinality rdf:datatype="http://www.w3.org/2001/XMLSchema#nonNegativeInteger">1</owl:qualifiedCardinality>
                <owl:onClass rdf:resource="http://www.ontology-of-units-of-measure.org/resource/om-2/Area"/>
            </owl:Restriction>
        </rdfs:subClassOf>
        <rdfs:subClassOf>
            <owl:Restriction>
                <owl:onProperty rdf:resource="https://www.theworldavatar.com/kg/ontobuiltenv/hasTotalRoofArea"/>
                <owl:qualifiedCardinality rdf:datatype="http://www.w3.org/2001/XMLSchema#nonNegativeInteger">1</owl:qualifiedCardinality>
                <owl:onClass rdf:resource="http://www.ontology-of-units-of-measure.org/resource/om-2/Area"/>
            </owl:Restriction>
        </rdfs:subClassOf>
        <rdfs:comment>A built structure with ground, roof, and walls which stands more or less permanently in one place.</rdfs:comment>
        <rdfs:isDefinedBy rdf:resource="https://www.theworldavatar.com/kg/ontobuiltenv/"/>
        <rdfs:label>Building</rdfs:label>
    </owl:Class>
    


    <!-- http://www.w3.org/2006/time#Instant -->


    <owl:Class rdf:about="http://www.w3.org/2006/time#Instant"/>
    


    <!-- http://www.w3.org/2006/time#Interval -->


    <owl:Class rdf:about="http://www.w3.org/2006/time#Interval"/>
    


    <!-- https://standards.buildingsmart.org/IFC/DEV/IFC4/ADD2_TC1/OWL#IfcBuilding -->


    <owl:Class rdf:about="https://standards.buildingsmart.org/IFC/DEV/IFC4/ADD2_TC1/OWL#IfcBuilding"/>
    


    <!-- https://w3id.org/bot#Building -->


    <owl:Class rdf:about="https://w3id.org/bot#Building"/>
    


    <!-- https://www.theworldavatar.com/kg/ontobuiltenv/AdministrativeDistrict -->


    <owl:Class rdf:about="https://www.theworldavatar.com/kg/ontobuiltenv/AdministrativeDistrict">
        <rdfs:comment>An area defined for administrative purposes, e.g. a county or local authority district.</rdfs:comment>
        <rdfs:isDefinedBy rdf:resource="https://www.theworldavatar.com/kg/ontobuiltenv/"/>
        <rdfs:label>Administrative district</rdfs:label>
    </owl:Class>
    


    <!-- https://www.theworldavatar.com/kg/ontobuiltenv/AveragePricePerSqm -->


    <owl:Class rdf:about="https://www.theworldavatar.com/kg/ontobuiltenv/AveragePricePerSqm">
        <rdfs:subClassOf rdf:resource="https://www.theworldavatar.com/kg/ontouom/AmountOfMoneyPerArea"/>
        <rdfs:subClassOf>
            <owl:Restriction>
                <owl:onProperty rdf:resource="https://www.theworldavatar.com/kg/ontobuiltenv/representativeFor"/>
                <owl:qualifiedCardinality rdf:datatype="http://www.w3.org/2001/XMLSchema#nonNegativeInteger">1</owl:qualifiedCardinality>
                <owl:onClass rdf:resource="https://www.theworldavatar.com/kg/ontobuiltenv/PostalCode"/>
            </owl:Restriction>
        </rdfs:subClassOf>
        <rdfs:comment>The average property price per square metre in a particular area.</rdfs:comment>
        <rdfs:isDefinedBy rdf:resource="https://www.theworldavatar.com/kg/ontobuiltenv/"/>
        <rdfs:label>Average price per square metre</rdfs:label>
    </owl:Class>
    


    <!-- https://www.theworldavatar.com/kg/ontobuiltenv/Bank -->


    <owl:Class rdf:about="https://www.theworldavatar.com/kg/ontobuiltenv/Bank">
        <rdfs:subClassOf rdf:resource="https://www.theworldavatar.com/kg/ontobuiltenv/Non-Domestic"/>
        <rdfs:comment>A property where customers can deposit and withdraw money.</rdfs:comment>
        <rdfs:isDefinedBy rdf:resource="https://www.theworldavatar.com/kg/ontobuiltenv/"/>
        <rdfs:label>Bank</rdfs:label>
    </owl:Class>
    


    <!-- https://www.theworldavatar.com/kg/ontobuiltenv/BuiltForm -->


    <owl:Class rdf:about="https://www.theworldavatar.com/kg/ontobuiltenv/BuiltForm">
        <rdfs:comment>The built form of the property.</rdfs:comment>
        <rdfs:isDefinedBy rdf:resource="https://www.theworldavatar.com/kg/ontobuiltenv/"/>
        <rdfs:label>Built form</rdfs:label>
    </owl:Class>
    


    <!-- https://www.theworldavatar.com/kg/ontobuiltenv/Bungalow -->


    <owl:Class rdf:about="https://www.theworldavatar.com/kg/ontobuiltenv/Bungalow">
        <rdfs:subClassOf rdf:resource="https://www.theworldavatar.com/kg/ontobuiltenv/PropertyType"/>
        <rdfs:comment>A small house with a single story.</rdfs:comment>
        <rdfs:isDefinedBy rdf:resource="https://www.theworldavatar.com/kg/ontobuiltenv/"/>
        <rdfs:label>Bungalow</rdfs:label>
    </owl:Class>
    


    <!-- https://www.theworldavatar.com/kg/ontobuiltenv/Clinic -->


    <owl:Class rdf:about="https://www.theworldavatar.com/kg/ontobuiltenv/Clinic">
        <rdfs:subClassOf rdf:resource="https://www.theworldavatar.com/kg/ontobuiltenv/Medical"/>
        <rdfs:comment>A medical facility for outpatient primary level healthcare.</rdfs:comment>
        <rdfs:isDefinedBy rdf:resource="https://www.theworldavatar.com/kg/ontobuiltenv/"/>
        <rdfs:label>Clinic</rdfs:label>
    </owl:Class>
    


    <!-- https://www.theworldavatar.com/kg/ontobuiltenv/ConstructionComponent -->


    <owl:Class rdf:about="https://www.theworldavatar.com/kg/ontobuiltenv/ConstructionComponent">
        <rdfs:comment>Key construction component of a property (i.e. wall, floor, roof, window).</rdfs:comment>
        <rdfs:isDefinedBy rdf:resource="https://www.theworldavatar.com/kg/ontobuiltenv/"/>
        <rdfs:label>Construction component</rdfs:label>
    </owl:Class>
    


    <!-- https://www.theworldavatar.com/kg/ontobuiltenv/CulturalFacility -->


    <owl:Class rdf:about="https://www.theworldavatar.com/kg/ontobuiltenv/CulturalFacility">
        <rdfs:subClassOf rdf:resource="https://www.theworldavatar.com/kg/ontobuiltenv/Non-Domestic"/>
        <rdfs:comment>A feature that is deemed to be of particular interest to society.</rdfs:comment>
        <rdfs:isDefinedBy rdf:resource="https://www.theworldavatar.com/kg/ontobuiltenv/"/>
        <rdfs:label>Cultural facility</rdfs:label>
    </owl:Class>
    


    <!-- https://www.theworldavatar.com/kg/ontobuiltenv/Detached -->


    <owl:Class rdf:about="https://www.theworldavatar.com/kg/ontobuiltenv/Detached">
        <rdfs:subClassOf rdf:resource="https://www.theworldavatar.com/kg/ontobuiltenv/BuiltForm"/>
        <rdfs:comment>A property with a detached built form.</rdfs:comment>
        <rdfs:isDefinedBy rdf:resource="https://www.theworldavatar.com/kg/ontobuiltenv/"/>
        <rdfs:label>Detached</rdfs:label>
    </owl:Class>
    


    <!-- https://www.theworldavatar.com/kg/ontobuiltenv/Domestic -->


    <owl:Class rdf:about="https://www.theworldavatar.com/kg/ontobuiltenv/Domestic">
        <rdfs:subClassOf rdf:resource="https://www.theworldavatar.com/kg/ontobuiltenv/PropertyUsage"/>
        <rdfs:comment>A property that serves as living space for one or more parties.</rdfs:comment>
        <rdfs:isDefinedBy rdf:resource="https://www.theworldavatar.com/kg/ontobuiltenv/"/>
        <rdfs:label>Domestic</rdfs:label>
    </owl:Class>
    


    <!-- https://www.theworldavatar.com/kg/ontobuiltenv/DrinkingEstablishment -->


    <owl:Class rdf:about="https://www.theworldavatar.com/kg/ontobuiltenv/DrinkingEstablishment">
        <rdfs:subClassOf rdf:resource="https://www.theworldavatar.com/kg/ontobuiltenv/Non-Domestic"/>
        <rdfs:comment>A business whose primary function is the serving of alcoholic beverages for consumption on the premises.</rdfs:comment>
        <rdfs:isDefinedBy rdf:resource="https://www.theworldavatar.com/kg/ontobuiltenv/"/>
        <rdfs:label>Drinking establishment</rdfs:label>
    </owl:Class>
    


    <!-- https://www.theworldavatar.com/kg/ontobuiltenv/EatingEstablishment -->


    <owl:Class rdf:about="https://www.theworldavatar.com/kg/ontobuiltenv/EatingEstablishment">
        <rdfs:subClassOf rdf:resource="https://www.theworldavatar.com/kg/ontobuiltenv/Non-Domestic"/>
        <rdfs:comment>A business whose primary function is the serving of food for consumption on the premises.</rdfs:comment>
        <rdfs:isDefinedBy rdf:resource="https://www.theworldavatar.com/kg/ontobuiltenv/"/>
        <rdfs:label>Eating establishment</rdfs:label>
    </owl:Class>
    


    <!-- https://www.theworldavatar.com/kg/ontobuiltenv/Education -->


    <owl:Class rdf:about="https://www.theworldavatar.com/kg/ontobuiltenv/Education">
        <rdfs:subClassOf rdf:resource="https://www.theworldavatar.com/kg/ontobuiltenv/Non-Domestic"/>
        <rdfs:comment>Education includes a very broad group of sites with a common high level primary function of providing education (either state funded or by fees).</rdfs:comment>
        <rdfs:isDefinedBy rdf:resource="https://www.theworldavatar.com/kg/ontobuiltenv/"/>
        <rdfs:label>Education</rdfs:label>
    </owl:Class>
    


    <!-- https://www.theworldavatar.com/kg/ontobuiltenv/EmergencyService -->


    <owl:Class rdf:about="https://www.theworldavatar.com/kg/ontobuiltenv/EmergencyService">
        <rdfs:subClassOf rdf:resource="https://www.theworldavatar.com/kg/ontobuiltenv/Non-Domestic"/>
        <rdfs:comment>Emergency services are organizations which ensure public safety and health by addressing different emergencies.</rdfs:comment>
        <rdfs:isDefinedBy rdf:resource="https://www.theworldavatar.com/kg/ontobuiltenv/"/>
        <rdfs:label>Emergency service</rdfs:label>
    </owl:Class>
    


    <!-- https://www.theworldavatar.com/kg/ontobuiltenv/FireStation -->


    <owl:Class rdf:about="https://www.theworldavatar.com/kg/ontobuiltenv/FireStation">
        <rdfs:subClassOf rdf:resource="https://www.theworldavatar.com/kg/ontobuiltenv/EmergencyService"/>
        <rdfs:comment>A facility which may house fire fighters, and contains the equipment and vehicles.</rdfs:comment>
        <rdfs:isDefinedBy rdf:resource="https://www.theworldavatar.com/kg/ontobuiltenv/"/>
        <rdfs:label>Fire station</rdfs:label>
    </owl:Class>
    


    <!-- https://www.theworldavatar.com/kg/ontobuiltenv/Flat -->


    <owl:Class rdf:about="https://www.theworldavatar.com/kg/ontobuiltenv/Flat">
        <rdfs:subClassOf rdf:resource="https://www.theworldavatar.com/kg/ontobuiltenv/Property"/>
        <rdfs:comment>A self-contained suite of rooms which occupies part of a building.</rdfs:comment>
        <rdfs:isDefinedBy rdf:resource="https://www.theworldavatar.com/kg/ontobuiltenv/"/>
        <rdfs:label>Flat</rdfs:label>
    </owl:Class>
    


    <!-- https://www.theworldavatar.com/kg/ontobuiltenv/Floor -->


    <owl:Class rdf:about="https://www.theworldavatar.com/kg/ontobuiltenv/Floor">
        <rdfs:subClassOf rdf:resource="https://www.theworldavatar.com/kg/ontobuiltenv/ConstructionComponent"/>
        <rdfs:comment>Key construction characteristics of the property&apos;s floor.</rdfs:comment>
        <rdfs:isDefinedBy rdf:resource="https://www.theworldavatar.com/kg/ontobuiltenv/"/>
        <rdfs:label>Floor</rdfs:label>
    </owl:Class>
    


    <!-- https://www.theworldavatar.com/kg/ontobuiltenv/FloorsCatA -->


    <owl:Class rdf:about="https://www.theworldavatar.com/kg/ontobuiltenv/FloorsCatA">
        <rdfs:subClassOf rdf:resource="https://www.theworldavatar.com/kg/ontobuiltenv/NumberOfFloors"/>
        <rdfs:comment>Category A of floors: data from reliable departments (e.g. government agencies)</rdfs:comment>
        <rdfs:isDefinedBy rdf:resource="https://www.theworldavatar.com/kg/ontobuiltenv/"/>
        <rdfs:label>Floors category A</rdfs:label>
    </owl:Class>
    


    <!-- https://www.theworldavatar.com/kg/ontobuiltenv/FloorsCatB -->


    <owl:Class rdf:about="https://www.theworldavatar.com/kg/ontobuiltenv/FloorsCatB">
        <rdfs:subClassOf rdf:resource="https://www.theworldavatar.com/kg/ontobuiltenv/NumberOfFloors"/>
        <rdfs:comment>Category B of floors: open source data without any guarantees (e.g. OSM)</rdfs:comment>
        <rdfs:isDefinedBy rdf:resource="https://www.theworldavatar.com/kg/ontobuiltenv/"/>
        <rdfs:label>Floors category B</rdfs:label>
    </owl:Class>
    


    <!-- https://www.theworldavatar.com/kg/ontobuiltenv/FloorsCatC -->


    <owl:Class rdf:about="https://www.theworldavatar.com/kg/ontobuiltenv/FloorsCatC">
        <rdfs:subClassOf rdf:resource="https://www.theworldavatar.com/kg/ontobuiltenv/NumberOfFloors"/>
        <rdfs:comment>Category C of floors: estimate</rdfs:comment>
        <rdfs:isDefinedBy rdf:resource="https://www.theworldavatar.com/kg/ontobuiltenv/"/>
        <rdfs:label>Floors category C</rdfs:label>
    </owl:Class>
    


    <!-- https://www.theworldavatar.com/kg/ontobuiltenv/Hospital -->


    <owl:Class rdf:about="https://www.theworldavatar.com/kg/ontobuiltenv/Hospital">
        <rdfs:subClassOf rdf:resource="https://www.theworldavatar.com/kg/ontobuiltenv/Medical"/>
        <rdfs:comment>A medical facility that provides second level care.</rdfs:comment>
        <rdfs:isDefinedBy rdf:resource="https://www.theworldavatar.com/kg/ontobuiltenv/"/>
        <rdfs:label>Hospital</rdfs:label>
    </owl:Class>
    


    <!-- https://www.theworldavatar.com/kg/ontobuiltenv/Hotel -->


    <owl:Class rdf:about="https://www.theworldavatar.com/kg/ontobuiltenv/Hotel">
        <rdfs:subClassOf rdf:resource="https://www.theworldavatar.com/kg/ontobuiltenv/Non-Domestic"/>
        <rdfs:comment>A property where travelers can pay for lodging and meals and other services.</rdfs:comment>
        <rdfs:isDefinedBy rdf:resource="https://www.theworldavatar.com/kg/ontobuiltenv/"/>
        <rdfs:label>Hotel</rdfs:label>
    </owl:Class>
    


    <!-- https://www.theworldavatar.com/kg/ontobuiltenv/House -->


    <owl:Class rdf:about="https://www.theworldavatar.com/kg/ontobuiltenv/House">
        <rdfs:subClassOf rdf:resource="https://www.theworldavatar.com/kg/ontobuiltenv/PropertyType"/>
        <rdfs:comment>A dwelling that serves as living quarters for one or more families, with one or more storeys.</rdfs:comment>
        <rdfs:isDefinedBy rdf:resource="https://www.theworldavatar.com/kg/ontobuiltenv/"/>
        <rdfs:label>House</rdfs:label>
    </owl:Class>
    


    <!-- https://www.theworldavatar.com/kg/ontobuiltenv/IndustrialFacility -->


    <owl:Class rdf:about="https://www.theworldavatar.com/kg/ontobuiltenv/IndustrialFacility">
        <rdfs:subClassOf rdf:resource="https://www.theworldavatar.com/kg/ontobuiltenv/Non-Domestic"/>
        <rdfs:comment>A property used for industrial fabrication or processing of goods. </rdfs:comment>
        <rdfs:isDefinedBy rdf:resource="https://www.theworldavatar.com/kg/ontobuiltenv/"/>
        <rdfs:label>Industrial facility</rdfs:label>
    </owl:Class>
    


    <!-- https://www.theworldavatar.com/kg/ontobuiltenv/Maisonette -->


    <owl:Class rdf:about="https://www.theworldavatar.com/kg/ontobuiltenv/Maisonette">
        <rdfs:subClassOf rdf:resource="https://www.theworldavatar.com/kg/ontobuiltenv/PropertyType"/>
        <rdfs:comment>A self-contained apartment (usually on two floors) in a larger building and with its own entrance from the outside.</rdfs:comment>
        <rdfs:isDefinedBy rdf:resource="https://www.theworldavatar.com/kg/ontobuiltenv/"/>
        <rdfs:label>Maisonette</rdfs:label>
    </owl:Class>
    


    <!-- https://www.theworldavatar.com/kg/ontobuiltenv/Medical -->


    <owl:Class rdf:about="https://www.theworldavatar.com/kg/ontobuiltenv/Medical">
        <rdfs:subClassOf rdf:resource="https://www.theworldavatar.com/kg/ontobuiltenv/Non-Domestic"/>
        <rdfs:comment>Medical include buildings and sites focused on the provision of medical care services or the dispensing of medicinal drugs, or both.</rdfs:comment>
        <rdfs:isDefinedBy rdf:resource="https://www.theworldavatar.com/kg/ontobuiltenv/"/>
        <rdfs:label>Medical</rdfs:label>
    </owl:Class>
    


    <!-- https://www.theworldavatar.com/kg/ontobuiltenv/MultiResidential -->


    <owl:Class rdf:about="https://www.theworldavatar.com/kg/ontobuiltenv/MultiResidential">
        <rdfs:subClassOf rdf:resource="https://www.theworldavatar.com/kg/ontobuiltenv/Domestic"/>
        <rdfs:comment>A property that serves as living space for more than one party.</rdfs:comment>
        <rdfs:isDefinedBy rdf:resource="https://www.theworldavatar.com/kg/ontobuiltenv/"/>
        <rdfs:label>Multi residential</rdfs:label>
    </owl:Class>
    


    <!-- https://www.theworldavatar.com/kg/ontobuiltenv/Non-Domestic -->


    <owl:Class rdf:about="https://www.theworldavatar.com/kg/ontobuiltenv/Non-Domestic">
        <rdfs:subClassOf rdf:resource="https://www.theworldavatar.com/kg/ontobuiltenv/PropertyUsage"/>
        <rdfs:comment>A property that serves non-living purposes (i.e. commercial, industrial, public propertys).</rdfs:comment>
        <rdfs:isDefinedBy rdf:resource="https://www.theworldavatar.com/kg/ontobuiltenv/"/>
        <rdfs:label>Non-Domestic</rdfs:label>
    </owl:Class>
    


    <!-- https://www.theworldavatar.com/kg/ontobuiltenv/NumberOfFloors -->


    <owl:Class rdf:about="https://www.theworldavatar.com/kg/ontobuiltenv/NumberOfFloors">
        <rdfs:comment>A concept to describe the number of floors in a building.</rdfs:comment>
        <rdfs:isDefinedBy rdf:resource="https://www.theworldavatar.com/kg/ontobuiltenv/"/>
        <rdfs:label>Number of floors</rdfs:label>
    </owl:Class>
    


    <!-- https://www.theworldavatar.com/kg/ontobuiltenv/Office -->


    <owl:Class rdf:about="https://www.theworldavatar.com/kg/ontobuiltenv/Office">
        <rdfs:subClassOf rdf:resource="https://www.theworldavatar.com/kg/ontobuiltenv/Non-Domestic"/>
        <rdfs:comment>A place of business where professional or clerical duties are performed.</rdfs:comment>
        <rdfs:isDefinedBy rdf:resource="https://www.theworldavatar.com/kg/ontobuiltenv/"/>
        <rdfs:label>Office</rdfs:label>
    </owl:Class>
    


    <!-- https://www.theworldavatar.com/kg/ontobuiltenv/ParkHome -->


    <owl:Class rdf:about="https://www.theworldavatar.com/kg/ontobuiltenv/ParkHome">
        <rdfs:subClassOf rdf:resource="https://www.theworldavatar.com/kg/ontobuiltenv/PropertyType"/>
        <rdfs:comment>Typically offsite manufactured bungalow-style homes that are located within a private estate.</rdfs:comment>
        <rdfs:isDefinedBy rdf:resource="https://www.theworldavatar.com/kg/ontobuiltenv/"/>
        <rdfs:label>ParkHome</rdfs:label>
    </owl:Class>
    


    <!-- https://www.theworldavatar.com/kg/ontobuiltenv/Pharmacy -->


    <owl:Class rdf:about="https://www.theworldavatar.com/kg/ontobuiltenv/Pharmacy">
        <rdfs:subClassOf rdf:resource="https://www.theworldavatar.com/kg/ontobuiltenv/Medical"/>
        <rdfs:comment>A healthcare facility where medicinal drugs are prepared or sold.</rdfs:comment>
        <rdfs:isDefinedBy rdf:resource="https://www.theworldavatar.com/kg/ontobuiltenv/"/>
        <rdfs:label>Pharmacy</rdfs:label>
    </owl:Class>
    


    <!-- https://www.theworldavatar.com/kg/ontobuiltenv/PoliceStation -->


    <owl:Class rdf:about="https://www.theworldavatar.com/kg/ontobuiltenv/PoliceStation">
        <rdfs:subClassOf rdf:resource="https://www.theworldavatar.com/kg/ontobuiltenv/EmergencyService"/>
        <rdfs:comment>The local office of a police force in a particular area.</rdfs:comment>
        <rdfs:isDefinedBy rdf:resource="https://www.theworldavatar.com/kg/ontobuiltenv/"/>
        <rdfs:label>Police station</rdfs:label>
    </owl:Class>
    


    <!-- https://www.theworldavatar.com/kg/ontobuiltenv/PostalCode -->


    <owl:Class rdf:about="https://www.theworldavatar.com/kg/ontobuiltenv/PostalCode">
        <rdfs:comment>A code of letters and digits denoting a particular (mostly granular) geographic area used to aid in the sorting of mail.</rdfs:comment>
        <rdfs:isDefinedBy rdf:resource="https://www.theworldavatar.com/kg/ontobuiltenv/"/>
        <rdfs:label>Postal code</rdfs:label>
    </owl:Class>
    


    <!-- https://www.theworldavatar.com/kg/ontobuiltenv/Property -->


    <owl:Class rdf:about="https://www.theworldavatar.com/kg/ontobuiltenv/Property">
        <rdfs:subClassOf>
            <owl:Restriction>
                <owl:onProperty rdf:resource="https://www.theworldavatar.com/kg/ontobuiltenv/hasAddress"/>
                <owl:qualifiedCardinality rdf:datatype="http://www.w3.org/2001/XMLSchema#nonNegativeInteger">1</owl:qualifiedCardinality>
                <owl:onClass rdf:resource="http://ontology.eil.utoronto.ca/icontact.owl#Address"/>
            </owl:Restriction>
        </rdfs:subClassOf>
        <rdfs:subClassOf>
            <owl:Restriction>
                <owl:onProperty rdf:resource="https://www.theworldavatar.com/kg/ontobuiltenv/hasBuiltForm"/>
                <owl:qualifiedCardinality rdf:datatype="http://www.w3.org/2001/XMLSchema#nonNegativeInteger">1</owl:qualifiedCardinality>
                <owl:onClass rdf:resource="https://www.theworldavatar.com/kg/ontobuiltenv/BuiltForm"/>
            </owl:Restriction>
        </rdfs:subClassOf>
        <rdfs:subClassOf>
            <owl:Restriction>
                <owl:onProperty rdf:resource="https://www.theworldavatar.com/kg/ontobuiltenv/hasEstimatedConstructionCost"/>
                <owl:qualifiedCardinality rdf:datatype="http://www.w3.org/2001/XMLSchema#nonNegativeInteger">1</owl:qualifiedCardinality>
                <owl:onClass rdf:resource="http://www.ontology-of-units-of-measure.org/resource/om-2/Cost"/>
            </owl:Restriction>
        </rdfs:subClassOf>
        <rdfs:subClassOf>
            <owl:Restriction>
                <owl:onProperty rdf:resource="https://www.theworldavatar.com/kg/ontobuiltenv/hasLatestTransactionRecord"/>
                <owl:qualifiedCardinality rdf:datatype="http://www.w3.org/2001/XMLSchema#nonNegativeInteger">1</owl:qualifiedCardinality>
                <owl:onClass rdf:resource="http://landregistry.data.gov.uk/def/ppi/TransactionRecord"/>
            </owl:Restriction>
        </rdfs:subClassOf>
        <rdfs:subClassOf>
            <owl:Restriction>
                <owl:onProperty rdf:resource="https://www.theworldavatar.com/kg/ontobuiltenv/hasMarketValue"/>
                <owl:qualifiedCardinality rdf:datatype="http://www.w3.org/2001/XMLSchema#nonNegativeInteger">1</owl:qualifiedCardinality>
                <owl:onClass rdf:resource="http://www.ontology-of-units-of-measure.org/resource/om-2/AmountOfMoney"/>
            </owl:Restriction>
        </rdfs:subClassOf>
        <rdfs:subClassOf>
            <owl:Restriction>
                <owl:onProperty rdf:resource="https://www.theworldavatar.com/kg/ontobuiltenv/hasNumberOfFloors"/>
                <owl:qualifiedCardinality rdf:datatype="http://www.w3.org/2001/XMLSchema#nonNegativeInteger">1</owl:qualifiedCardinality>
                <owl:onClass rdf:resource="https://www.theworldavatar.com/kg/ontobuiltenv/NumberOfFloors"/>
            </owl:Restriction>
        </rdfs:subClassOf>
        <rdfs:subClassOf>
            <owl:Restriction>
                <owl:onProperty rdf:resource="https://www.theworldavatar.com/kg/ontobuiltenv/hasPropertyType"/>
                <owl:qualifiedCardinality rdf:datatype="http://www.w3.org/2001/XMLSchema#nonNegativeInteger">1</owl:qualifiedCardinality>
                <owl:onClass rdf:resource="https://www.theworldavatar.com/kg/ontobuiltenv/PropertyType"/>
            </owl:Restriction>
        </rdfs:subClassOf>
        <rdfs:subClassOf>
            <owl:Restriction>
                <owl:onProperty rdf:resource="https://www.theworldavatar.com/kg/ontobuiltenv/hasTotalFloorArea"/>
                <owl:qualifiedCardinality rdf:datatype="http://www.w3.org/2001/XMLSchema#nonNegativeInteger">1</owl:qualifiedCardinality>
                <owl:onClass rdf:resource="http://www.ontology-of-units-of-measure.org/resource/om-2/Area"/>
            </owl:Restriction>
        </rdfs:subClassOf>
        <rdfs:comment>A built structure which is available for occupation or business purposes.</rdfs:comment>
        <rdfs:isDefinedBy rdf:resource="https://www.theworldavatar.com/kg/ontobuiltenv/"/>
        <rdfs:label>Property</rdfs:label>
    </owl:Class>
    


    <!-- https://www.theworldavatar.com/kg/ontobuiltenv/PropertyPriceIndex -->


    <owl:Class rdf:about="https://www.theworldavatar.com/kg/ontobuiltenv/PropertyPriceIndex">
        <rdfs:subClassOf>
            <owl:Restriction>
                <owl:onProperty rdf:resource="https://www.theworldavatar.com/kg/ontotimeseries/hasTimeSeries"/>
                <owl:qualifiedCardinality rdf:datatype="http://www.w3.org/2001/XMLSchema#nonNegativeInteger">1</owl:qualifiedCardinality>
                <owl:onClass rdf:resource="https://www.theworldavatar.com/kg/ontotimeseries/TimeSeries"/>
            </owl:Restriction>
        </rdfs:subClassOf>
        <rdfs:comment>An index denoting the (average) property price evolution within a specific area over time.</rdfs:comment>
        <rdfs:isDefinedBy rdf:resource="https://www.theworldavatar.com/kg/ontobuiltenv/"/>
        <rdfs:label>Property price index</rdfs:label>
    </owl:Class>
    


    <!-- https://www.theworldavatar.com/kg/ontobuiltenv/PropertyType -->


    <owl:Class rdf:about="https://www.theworldavatar.com/kg/ontobuiltenv/PropertyType">
        <rdfs:comment>The general type of the property.</rdfs:comment>
        <rdfs:isDefinedBy rdf:resource="https://www.theworldavatar.com/kg/ontobuiltenv/"/>
        <rdfs:label>Property type</rdfs:label>
    </owl:Class>
    


    <!-- https://www.theworldavatar.com/kg/ontobuiltenv/PropertyUsage -->


    <owl:Class rdf:about="https://www.theworldavatar.com/kg/ontobuiltenv/PropertyUsage">
        <rdfs:comment>Description of the (intended) usage and/or function of a property. One property can have multiple usages. If multiple usages are assigned to one property, they have an usage share assigned to them (for single usage assignments this is assumed 1).</rdfs:comment>
        <rdfs:isDefinedBy rdf:resource="https://www.theworldavatar.com/kg/ontobuiltenv/"/>
        <rdfs:label>Property usage</rdfs:label>
    </owl:Class>
    


    <!-- https://www.theworldavatar.com/kg/ontobuiltenv/ReligiousFacility -->


    <owl:Class rdf:about="https://www.theworldavatar.com/kg/ontobuiltenv/ReligiousFacility">
        <rdfs:subClassOf rdf:resource="https://www.theworldavatar.com/kg/ontobuiltenv/Non-Domestic"/>
        <rdfs:comment>A place where members of a religious group congregate for worship.</rdfs:comment>
        <rdfs:isDefinedBy rdf:resource="https://www.theworldavatar.com/kg/ontobuiltenv/"/>
        <rdfs:label>Religious facility</rdfs:label>
    </owl:Class>
    


    <!-- https://www.theworldavatar.com/kg/ontobuiltenv/RetailEstablishment -->


    <owl:Class rdf:about="https://www.theworldavatar.com/kg/ontobuiltenv/RetailEstablishment">
        <rdfs:subClassOf rdf:resource="https://www.theworldavatar.com/kg/ontobuiltenv/Non-Domestic"/>
        <rdfs:comment>A feature that sells to the general public finished goods.</rdfs:comment>
        <rdfs:isDefinedBy rdf:resource="https://www.theworldavatar.com/kg/ontobuiltenv/"/>
        <rdfs:label>Retail establishment</rdfs:label>
    </owl:Class>
    


    <!-- https://www.theworldavatar.com/kg/ontobuiltenv/Roof -->


    <owl:Class rdf:about="https://www.theworldavatar.com/kg/ontobuiltenv/Roof">
        <rdfs:subClassOf rdf:resource="https://www.theworldavatar.com/kg/ontobuiltenv/ConstructionComponent"/>
        <rdfs:comment>Key construction characteristics of the property&apos;s roof.</rdfs:comment>
        <rdfs:isDefinedBy rdf:resource="https://www.theworldavatar.com/kg/ontobuiltenv/"/>
        <rdfs:label>Roof</rdfs:label>
    </owl:Class>
    


    <!-- https://www.theworldavatar.com/kg/ontobuiltenv/School -->


    <owl:Class rdf:about="https://www.theworldavatar.com/kg/ontobuiltenv/School">
        <rdfs:subClassOf rdf:resource="https://www.theworldavatar.com/kg/ontobuiltenv/Education"/>
        <rdfs:comment>A property where young people receive primary and secondary education.</rdfs:comment>
        <rdfs:isDefinedBy rdf:resource="https://www.theworldavatar.com/kg/ontobuiltenv/"/>
        <rdfs:label>School</rdfs:label>
    </owl:Class>
    


    <!-- https://www.theworldavatar.com/kg/ontobuiltenv/Semi-Detached -->


    <owl:Class rdf:about="https://www.theworldavatar.com/kg/ontobuiltenv/Semi-Detached">
        <rdfs:subClassOf rdf:resource="https://www.theworldavatar.com/kg/ontobuiltenv/BuiltForm"/>
        <rdfs:comment>A property with a semi-detached built form.</rdfs:comment>
        <rdfs:isDefinedBy rdf:resource="https://www.theworldavatar.com/kg/ontobuiltenv/"/>
        <rdfs:label>Semi-Detached</rdfs:label>
    </owl:Class>
    


    <!-- https://www.theworldavatar.com/kg/ontobuiltenv/SingleResidential -->


    <owl:Class rdf:about="https://www.theworldavatar.com/kg/ontobuiltenv/SingleResidential">
        <rdfs:subClassOf rdf:resource="https://www.theworldavatar.com/kg/ontobuiltenv/Domestic"/>
        <rdfs:comment>A property that serves as living space for one party.</rdfs:comment>
        <rdfs:isDefinedBy rdf:resource="https://www.theworldavatar.com/kg/ontobuiltenv/"/>
        <rdfs:label>Single residential</rdfs:label>
    </owl:Class>
    


    <!-- https://www.theworldavatar.com/kg/ontobuiltenv/SportsFacility -->


    <owl:Class rdf:about="https://www.theworldavatar.com/kg/ontobuiltenv/SportsFacility">
        <rdfs:subClassOf rdf:resource="https://www.theworldavatar.com/kg/ontobuiltenv/Non-Domestic"/>
        <rdfs:comment>A feature where one or many different sports can be played.</rdfs:comment>
        <rdfs:isDefinedBy rdf:resource="https://www.theworldavatar.com/kg/ontobuiltenv/"/>
        <rdfs:label>Sports facility</rdfs:label>
    </owl:Class>
    


    <!-- https://www.theworldavatar.com/kg/ontobuiltenv/Terraced -->


    <owl:Class rdf:about="https://www.theworldavatar.com/kg/ontobuiltenv/Terraced">
        <rdfs:subClassOf rdf:resource="https://www.theworldavatar.com/kg/ontobuiltenv/BuiltForm"/>
        <rdfs:comment>A property with a terraced built form.</rdfs:comment>
        <rdfs:isDefinedBy rdf:resource="https://www.theworldavatar.com/kg/ontobuiltenv/"/>
        <rdfs:label>Terraced</rdfs:label>
    </owl:Class>
    


    <!-- https://www.theworldavatar.com/kg/ontobuiltenv/TransportFacility -->


    <owl:Class rdf:about="https://www.theworldavatar.com/kg/ontobuiltenv/TransportFacility">
        <rdfs:subClassOf rdf:resource="https://www.theworldavatar.com/kg/ontobuiltenv/Non-Domestic"/>
        <rdfs:comment>A feature that is associated with the movement of passengers and goods.</rdfs:comment>
        <rdfs:isDefinedBy rdf:resource="https://www.theworldavatar.com/kg/ontobuiltenv/"/>
        <rdfs:label>Transport facility</rdfs:label>
    </owl:Class>
    


    <!-- https://www.theworldavatar.com/kg/ontobuiltenv/University -->


    <owl:Class rdf:about="https://www.theworldavatar.com/kg/ontobuiltenv/University">
        <rdfs:subClassOf rdf:resource="https://www.theworldavatar.com/kg/ontobuiltenv/Education"/>
        <rdfs:comment>A site providing higher/university education.</rdfs:comment>
        <rdfs:isDefinedBy rdf:resource="https://www.theworldavatar.com/kg/ontobuiltenv/"/>
        <rdfs:label>University</rdfs:label>
    </owl:Class>
    


    <!-- https://www.theworldavatar.com/kg/ontobuiltenv/Wall -->


    <owl:Class rdf:about="https://www.theworldavatar.com/kg/ontobuiltenv/Wall">
        <rdfs:subClassOf rdf:resource="https://www.theworldavatar.com/kg/ontobuiltenv/ConstructionComponent"/>
        <rdfs:comment>Key construction characteristics of the property&apos;s walls.</rdfs:comment>
        <rdfs:isDefinedBy rdf:resource="https://www.theworldavatar.com/kg/ontobuiltenv/"/>
        <rdfs:label>Wall</rdfs:label>
    </owl:Class>
    


    <!-- https://www.theworldavatar.com/kg/ontobuiltenv/Window -->


    <owl:Class rdf:about="https://www.theworldavatar.com/kg/ontobuiltenv/Window">
        <rdfs:subClassOf rdf:resource="https://www.theworldavatar.com/kg/ontobuiltenv/ConstructionComponent"/>
        <rdfs:comment>Key construction characteristics of the property&apos;s windows.</rdfs:comment>
        <rdfs:isDefinedBy rdf:resource="https://www.theworldavatar.com/kg/ontobuiltenv/"/>
        <rdfs:label>Window</rdfs:label>
    </owl:Class>
    


    <!-- https://www.theworldavatar.com/kg/ontotimeseries/TimeSeries -->


    <owl:Class rdf:about="https://www.theworldavatar.com/kg/ontotimeseries/TimeSeries"/>
    


    <!-- https://www.theworldavatar.com/kg/ontouom/AmountOfMoneyPerArea -->


    <owl:Class rdf:about="https://www.theworldavatar.com/kg/ontouom/AmountOfMoneyPerArea"/>
    


    <!-- https://www.theworldavatar.com/kg/ontouom/pound_sterling_per_sqm -->


    <owl:Class rdf:about="https://www.theworldavatar.com/kg/ontouom/pound_sterling_per_sqm">
        <rdfs:subClassOf rdf:resource="http://www.ontology-of-units-of-measure.org/resource/om-2/Unit"/>
        <rdfs:comment>Pound sterling per square metre.</rdfs:comment>
        <rdfs:isDefinedBy rdf:resource="http://www.ontology-of-units-of-measure.org/resource/om-2/"/>
        <rdfs:label>Pound sterling per sqm</rdfs:label>
    </owl:Class>
    


    <!-- 
    ///////////////////////////////////////////////////////////////////////////////////////
    //
    // Annotations
    //
    ///////////////////////////////////////////////////////////////////////////////////////
     -->


    <rdf:Description rdf:about="http://www.w3.org/2000/01/rdf-schema#label">
        <rdfs:comment>A relationship between a postal code and its actual code of letters and digits.</rdfs:comment>
        <rdfs:comment>A relationship between a property usage and a textual description of it (e.g. its name or (intended) usage classification).</rdfs:comment>
        <rdfs:comment>A relationship between an administrative district and its actual official name.</rdfs:comment>
        <rdfs:isDefinedBy rdf:resource="https://www.theworldavatar.com/kg/ontobuiltenv/"/>
        <rdfs:label>label</rdfs:label>
        <rdfs:label>usage label</rdfs:label>
    </rdf:Description>
</rdf:RDF>



<!-- Generated by the OWL API (version 5.5.0.2023-01-14T12:41:38Z) https://github.com/owlcs/owlapi/ -->


