<?xml version="1.0"?>
<rdf:RDF xmlns="http://www.theworldavatar.com/ontology/OntoFHRS/"
     xml:base="http://www.theworldavatar.com/ontology/OntoFHRS/"
     xmlns:dc="http://purl.org/dc/elements/1.1/"
     xmlns:owl="http://www.w3.org/2002/07/owl#"
     xmlns:rdf="http://www.w3.org/1999/02/22-rdf-syntax-ns#"
     xmlns:xml="http://www.w3.org/XML/1998/namespace"
     xmlns:xsd="http://www.w3.org/2001/XMLSchema#"
     xmlns:rdfs="http://www.w3.org/2000/01/rdf-schema#"
     xmlns:OntoFHRS="http://www.theworldavatar.com/ontology/OntoFHRS/">
    <owl:Ontology rdf:about="http://www.theworldavatar.com/ontology/OntoFHRS/">
        <dc:date>12 November 2024</dc:date>
        <gitCommitHash>c0599beca8df55873a1ab061dee64e52c510c6a0</gitCommitHash>
        <rdfs:comment>OntoFHRS is an ontology developed for representing food hygiene ratings of business establishments.</rdfs:comment>
        <owl:versionInfo>1</owl:versionInfo>
    </owl:Ontology>
    


    <!-- 
    ///////////////////////////////////////////////////////////////////////////////////////
    //
    // Annotation properties
    //
    ///////////////////////////////////////////////////////////////////////////////////////
     -->


    


    <!-- http://purl.org/dc/elements/1.1/date -->


    <owl:AnnotationProperty rdf:about="http://purl.org/dc/elements/1.1/date"/>
    


    <!-- http://www.theworldavatar.com/ontology/OntoFHRS/gitCommitHash -->


    <owl:AnnotationProperty rdf:about="http://www.theworldavatar.com/ontology/OntoFHRS/gitCommitHash"/>
    


    <!-- 
    ///////////////////////////////////////////////////////////////////////////////////////
    //
    // Datatypes
    //
    ///////////////////////////////////////////////////////////////////////////////////////
     -->


    


    <!-- http://www.opengis.net/ont/geosparql#wktLiteral -->


    <rdfs:Datatype rdf:about="http://www.opengis.net/ont/geosparql#wktLiteral"/>
    


    <!-- 
    ///////////////////////////////////////////////////////////////////////////////////////
    //
    // Object Properties
    //
    ///////////////////////////////////////////////////////////////////////////////////////
     -->


    


    <!-- http://ies.data.gov.uk/ontology/ies4#inPeriod -->


    <owl:ObjectProperty rdf:about="http://ies.data.gov.uk/ontology/ies4#inPeriod">
        <rdfs:domain>
            <owl:Class>
                <owl:unionOf rdf:parseType="Collection">
                    <rdf:Description rdf:about="http://www.theworldavatar.com/ontology/OntoFHRS/BusinessEstablishmentEnd"/>
                    <rdf:Description rdf:about="http://www.theworldavatar.com/ontology/OntoFHRS/BusinessEstablishmentStart"/>
                    <rdf:Description rdf:about="http://www.theworldavatar.com/ontology/OntoFHRS/RatingEnd"/>
                    <rdf:Description rdf:about="http://www.theworldavatar.com/ontology/OntoFHRS/RatingStart"/>
                </owl:unionOf>
            </owl:Class>
        </rdfs:domain>
        <rdfs:range rdf:resource="http://ies.data.gov.uk/ontology/ies4#ParticularPeriod"/>
        <rdfs:comment>An object property relating the start or end of an entity or event to a specific period.</rdfs:comment>
        <rdfs:isDefinedBy rdf:resource="http://ies.data.gov.uk/ontology/ies4"/>
        <rdfs:label>in period</rdfs:label>
    </owl:ObjectProperty>
    


    <!-- http://ies.data.gov.uk/ontology/ies4#isEndOf -->


    <owl:ObjectProperty rdf:about="http://ies.data.gov.uk/ontology/ies4#isEndOf">
        <rdfs:domain>
            <owl:Class>
                <owl:unionOf rdf:parseType="Collection">
                    <rdf:Description rdf:about="http://www.theworldavatar.com/ontology/OntoFHRS/BusinessEstablishmentEnd"/>
                    <rdf:Description rdf:about="http://www.theworldavatar.com/ontology/OntoFHRS/RatingEnd"/>
                </owl:unionOf>
            </owl:Class>
        </rdfs:domain>
        <rdfs:range rdf:resource="http://www.theworldavatar.com/ontology/OntoFHRS/BusinessEstablishment"/>
        <rdfs:comment>An object property representing the end date of a business establishment.</rdfs:comment>
        <rdfs:isDefinedBy rdf:resource="http://ies.data.gov.uk/ontology/ies4"/>
        <rdfs:label>is end of</rdfs:label>
    </owl:ObjectProperty>
    


    <!-- http://ies.data.gov.uk/ontology/ies4#isStartOf -->


    <owl:ObjectProperty rdf:about="http://ies.data.gov.uk/ontology/ies4#isStartOf">
        <rdfs:domain>
            <owl:Class>
                <owl:unionOf rdf:parseType="Collection">
                    <rdf:Description rdf:about="http://www.theworldavatar.com/ontology/OntoFHRS/BusinessEstablishmentStart"/>
                    <rdf:Description rdf:about="http://www.theworldavatar.com/ontology/OntoFHRS/RatingStart"/>
                </owl:unionOf>
            </owl:Class>
        </rdfs:domain>
        <rdfs:range rdf:resource="http://www.theworldavatar.com/ontology/OntoFHRS/BusinessEstablishment"/>
        <rdfs:comment>An object property representing the start date of a business establishment.</rdfs:comment>
        <rdfs:isDefinedBy rdf:resource="http://ies.data.gov.uk/ontology/ies4"/>
        <rdfs:label>is start of</rdfs:label>
    </owl:ObjectProperty>
    


    <!-- http://www.theworldavatar.com/ontology/OntoFHRS/hasAddress -->


    <owl:ObjectProperty rdf:about="http://www.theworldavatar.com/ontology/OntoFHRS/hasAddress">
        <rdfs:domain rdf:resource="http://www.theworldavatar.com/ontology/OntoFHRS/BusinessEstablishment"/>
        <rdfs:range rdf:resource="http://ies.data.gov.uk/ontology/ies4#Address"/>
        <rdfs:comment>An object property referring to the address of a business establishment.</rdfs:comment>
        <rdfs:isDefinedBy rdf:resource="http://www.theworldavatar.com/ontology/OntoFHRS/"/>
        <rdfs:label>has address</rdfs:label>
    </owl:ObjectProperty>
    


    <!-- http://www.theworldavatar.com/ontology/OntoFHRS/hasCity -->


    <owl:ObjectProperty rdf:about="http://www.theworldavatar.com/ontology/OntoFHRS/hasCity">
        <rdfs:domain rdf:resource="http://ies.data.gov.uk/ontology/ies4#Address"/>
        <rdfs:range rdf:resource="https://dbpedia.org/ontology/City"/>
        <rdfs:comment>An object property referring to the city provided in the address of a business establishment.</rdfs:comment>
        <rdfs:isDefinedBy rdf:resource="http://www.theworldavatar.com/ontology/OntoFHRS/"/>
        <rdfs:label>has city</rdfs:label>
    </owl:ObjectProperty>
    


    <!-- http://www.theworldavatar.com/ontology/OntoFHRS/hasConfidenceInManagementScore -->


    <owl:ObjectProperty rdf:about="http://www.theworldavatar.com/ontology/OntoFHRS/hasConfidenceInManagementScore">
        <rdfs:domain rdf:resource="http://www.theworldavatar.com/ontology/OntoFHRS/BusinessEstablishment"/>
        <rdfs:range rdf:resource="http://www.theworldavatar.com/ontology/OntoFHRS/ConfidenceInManagementScore"/>
        <rdfs:comment>An object property referring to the confidence in management score of a business establishment.</rdfs:comment>
        <rdfs:isDefinedBy rdf:resource="http://www.theworldavatar.com/ontology/OntoFHRS/"/>
        <rdfs:label>has confidence in management score</rdfs:label>
    </owl:ObjectProperty>
    


    <!-- http://www.theworldavatar.com/ontology/OntoFHRS/hasCountry -->


    <owl:ObjectProperty rdf:about="http://www.theworldavatar.com/ontology/OntoFHRS/hasCountry">
        <rdfs:domain rdf:resource="http://ies.data.gov.uk/ontology/ies4#Address"/>
        <rdfs:range rdf:resource="https://dbpedia.org/ontology/Country"/>
        <rdfs:comment>An object property referring to the country provided in the address of a business establishment.</rdfs:comment>
        <rdfs:isDefinedBy rdf:resource="http://www.theworldavatar.com/ontology/OntoFHRS/"/>
        <rdfs:label>has country</rdfs:label>
    </owl:ObjectProperty>
    


    <!-- http://www.theworldavatar.com/ontology/OntoFHRS/hasDistrictCouncil -->


    <owl:ObjectProperty rdf:about="http://www.theworldavatar.com/ontology/OntoFHRS/hasDistrictCouncil">
        <rdfs:domain rdf:resource="http://www.theworldavatar.com/ontology/OntoFHRS/BusinessEstablishment"/>
        <rdfs:range rdf:resource="http://www.theworldavatar.com/ontology/OntoFHRS/DistrictCouncil"/>
        <rdfs:comment>An object property referring to the district council a business establishment is located.</rdfs:comment>
        <rdfs:isDefinedBy rdf:resource="http://www.theworldavatar.com/ontology/OntoFHRS/"/>
        <rdfs:label>has district council</rdfs:label>
    </owl:ObjectProperty>
    


    <!-- http://www.theworldavatar.com/ontology/OntoFHRS/hasHygieneScore -->


    <owl:ObjectProperty rdf:about="http://www.theworldavatar.com/ontology/OntoFHRS/hasHygieneScore">
        <rdfs:domain rdf:resource="http://www.theworldavatar.com/ontology/OntoFHRS/BusinessEstablishment"/>
        <rdfs:range rdf:resource="http://www.theworldavatar.com/ontology/OntoFHRS/HygieneScore"/>
        <rdfs:comment>An object property referring to the hygiene score of a business establishment.</rdfs:comment>
        <rdfs:isDefinedBy rdf:resource="http://www.theworldavatar.com/ontology/OntoFHRS/"/>
        <rdfs:label>has hygiene score</rdfs:label>
    </owl:ObjectProperty>
    


    <!-- http://www.theworldavatar.com/ontology/OntoFHRS/hasLocalAuthority -->


    <owl:ObjectProperty rdf:about="http://www.theworldavatar.com/ontology/OntoFHRS/hasLocalAuthority">
        <rdfs:domain rdf:resource="http://www.theworldavatar.com/ontology/OntoFHRS/BusinessEstablishment"/>
        <rdfs:range rdf:resource="http://www.theworldavatar.com/ontology/OntoFHRS/LocalAuthority"/>
        <rdfs:comment>An object property referring to the local authority of a business establishment.</rdfs:comment>
        <rdfs:isDefinedBy rdf:resource="http://www.theworldavatar.com/ontology/OntoFHRS/"/>
        <rdfs:label>has local authority</rdfs:label>
    </owl:ObjectProperty>
    


    <!-- http://www.theworldavatar.com/ontology/OntoFHRS/hasRating -->


    <owl:ObjectProperty rdf:about="http://www.theworldavatar.com/ontology/OntoFHRS/hasRating">
        <rdfs:domain rdf:resource="http://www.theworldavatar.com/ontology/OntoFHRS/BusinessEstablishment"/>
        <rdfs:range rdf:resource="http://www.theworldavatar.com/ontology/OntoFHRS/Rating"/>
        <rdfs:comment>An object property referring to the rating of a business establishment.</rdfs:comment>
        <rdfs:isDefinedBy rdf:resource="http://www.theworldavatar.com/ontology/OntoFHRS/"/>
        <rdfs:label>has rating</rdfs:label>
    </owl:ObjectProperty>
    


    <!-- http://www.theworldavatar.com/ontology/OntoFHRS/hasRatingScheme -->


    <owl:ObjectProperty rdf:about="http://www.theworldavatar.com/ontology/OntoFHRS/hasRatingScheme">
        <rdfs:domain rdf:resource="http://www.theworldavatar.com/ontology/OntoFHRS/Rating"/>
        <rdfs:range rdf:resource="http://www.theworldavatar.com/ontology/OntoFHRS/RatingScheme"/>
        <rdfs:comment>An object property referring to the rating scheme used to calculate the rating of a business establishment.</rdfs:comment>
        <rdfs:isDefinedBy rdf:resource="http://www.theworldavatar.com/ontology/OntoFHRS/"/>
        <rdfs:label>has rating scheme</rdfs:label>
    </owl:ObjectProperty>
    


    <!-- http://www.theworldavatar.com/ontology/OntoFHRS/hasRegion -->


    <owl:ObjectProperty rdf:about="http://www.theworldavatar.com/ontology/OntoFHRS/hasRegion">
        <rdfs:domain rdf:resource="http://ies.data.gov.uk/ontology/ies4#Address"/>
        <rdfs:range rdf:resource="https://dbpedia.org/ontology/Region"/>
        <rdfs:comment>An object property referring to the region provided in the address of a business establishment.</rdfs:comment>
        <rdfs:isDefinedBy rdf:resource="http://www.theworldavatar.com/ontology/OntoFHRS/"/>
        <rdfs:label>has region</rdfs:label>
    </owl:ObjectProperty>
    


    <!-- http://www.theworldavatar.com/ontology/OntoFHRS/hasStructuralScore -->


    <owl:ObjectProperty rdf:about="http://www.theworldavatar.com/ontology/OntoFHRS/hasStructuralScore">
        <rdfs:domain rdf:resource="http://www.theworldavatar.com/ontology/OntoFHRS/BusinessEstablishment"/>
        <rdfs:range rdf:resource="http://www.theworldavatar.com/ontology/OntoFHRS/StructuralScore"/>
        <rdfs:comment>An object property referring to the structural score of a business establishment.</rdfs:comment>
        <rdfs:isDefinedBy rdf:resource="http://www.theworldavatar.com/ontology/OntoFHRS/"/>
        <rdfs:label>has structural score</rdfs:label>
    </owl:ObjectProperty>
    


    <!-- 
    ///////////////////////////////////////////////////////////////////////////////////////
    //
    // Data properties
    //
    ///////////////////////////////////////////////////////////////////////////////////////
     -->


    


    <!-- http://ies.data.gov.uk/ontology/ies4#iso8601PeriodRepresentation -->


    <owl:DatatypeProperty rdf:about="http://ies.data.gov.uk/ontology/ies4#iso8601PeriodRepresentation">
        <rdfs:domain rdf:resource="http://ies.data.gov.uk/ontology/ies4#ParticularPeriod"/>
        <rdfs:range rdf:resource="http://www.w3.org/2001/XMLSchema#anyURI"/>
        <rdfs:isDefinedBy rdf:resource="http://ies.data.gov.uk/ontology/ies4"/>
        <rdfs:label>iso 8601 period representation</rdfs:label>
    </owl:DatatypeProperty>
    


    <!-- http://ontology.eil.utoronto.ca/icontact.owl#hasStreet -->


    <owl:DatatypeProperty rdf:about="http://ontology.eil.utoronto.ca/icontact.owl#hasStreet">
        <rdfs:domain rdf:resource="http://ies.data.gov.uk/ontology/ies4#Address"/>
        <rdfs:range rdf:resource="http://www.w3.org/2001/XMLSchema#string"/>
        <rdfs:comment>A datatype property that represents the name of the street in the address of a business establishment.</rdfs:comment>
        <rdfs:isDefinedBy rdf:resource="http://www.theworldavatar.com/ontology/OntoFHRS/"/>
        <rdfs:label>has street</rdfs:label>
    </owl:DatatypeProperty>
    


    <!-- http://www.opengis.net/ont/geosparql#asWKT -->


    <owl:DatatypeProperty rdf:about="http://www.opengis.net/ont/geosparql#asWKT">
        <rdfs:domain rdf:resource="http://www.theworldavatar.com/ontology/OntoFHRS/BusinessEstablishment"/>
        <rdfs:range rdf:resource="http://www.opengis.net/ont/geosparql#wktLiteral"/>
        <rdfs:isDefinedBy rdf:resource="http://www.opengis.net/ont/geosparql"/>
        <rdfs:label>as WKT</rdfs:label>
    </owl:DatatypeProperty>
    


    <!-- http://www.theworldavatar.com/ontology/OntoFHRS/hasEmailAddress -->


    <owl:DatatypeProperty rdf:about="http://www.theworldavatar.com/ontology/OntoFHRS/hasEmailAddress">
        <rdfs:domain rdf:resource="http://www.theworldavatar.com/ontology/OntoFHRS/LocalAuthority"/>
        <rdfs:range rdf:resource="http://www.w3.org/2001/XMLSchema#string"/>
        <rdfs:comment>A datatype property that denotes the official email address of a local authority, facilitating electronic communication and inquiries.</rdfs:comment>
        <rdfs:isDefinedBy rdf:resource="http://www.theworldavatar.com/ontology/OntoFHRS/"/>
        <rdfs:label>has email address</rdfs:label>
    </owl:DatatypeProperty>
    


    <!-- http://www.theworldavatar.com/ontology/OntoFHRS/hasFHRSID -->


    <owl:DatatypeProperty rdf:about="http://www.theworldavatar.com/ontology/OntoFHRS/hasFHRSID">
        <rdfs:domain rdf:resource="http://www.theworldavatar.com/ontology/OntoFHRS/BusinessEstablishment"/>
        <rdfs:range rdf:resource="http://www.w3.org/2001/XMLSchema#string"/>
        <rdfs:comment>A datatype property that represents the FHRS identifier of a business establishment.</rdfs:comment>
        <rdfs:isDefinedBy rdf:resource="http://www.theworldavatar.com/ontology/OntoFHRS/"/>
        <rdfs:label>has fhrs id</rdfs:label>
    </owl:DatatypeProperty>
    


    <!-- http://www.theworldavatar.com/ontology/OntoFHRS/hasKey -->


    <owl:DatatypeProperty rdf:about="http://www.theworldavatar.com/ontology/OntoFHRS/hasKey">
        <rdfs:domain rdf:resource="http://www.theworldavatar.com/ontology/OntoFHRS/Rating"/>
        <rdfs:range rdf:resource="http://www.w3.org/2001/XMLSchema#string"/>
        <rdfs:comment>A datatype property that represents the key of the rating of a business establishment.</rdfs:comment>
        <rdfs:isDefinedBy rdf:resource="http://www.theworldavatar.com/ontology/OntoFHRS/"/>
        <rdfs:label>has key</rdfs:label>
    </owl:DatatypeProperty>
    


    <!-- http://www.theworldavatar.com/ontology/OntoFHRS/hasLocalAuthorityBusinessID -->


    <owl:DatatypeProperty rdf:about="http://www.theworldavatar.com/ontology/OntoFHRS/hasLocalAuthorityBusinessID">
        <rdfs:domain rdf:resource="http://www.theworldavatar.com/ontology/OntoFHRS/BusinessEstablishment"/>
        <rdfs:range rdf:resource="http://www.w3.org/2001/XMLSchema#string"/>
        <rdfs:comment>A datatype property that represents the business identifier assigned by a local authority to a business establishment.</rdfs:comment>
        <rdfs:isDefinedBy rdf:resource="http://www.theworldavatar.com/ontology/OntoFHRS/"/>
        <rdfs:label>has local authority business id</rdfs:label>
    </owl:DatatypeProperty>
    


    <!-- http://www.theworldavatar.com/ontology/OntoFHRS/hasLocalAuthorityCode -->


    <owl:DatatypeProperty rdf:about="http://www.theworldavatar.com/ontology/OntoFHRS/hasLocalAuthorityCode">
        <rdfs:domain rdf:resource="http://www.theworldavatar.com/ontology/OntoFHRS/LocalAuthority"/>
        <rdfs:range rdf:resource="http://www.w3.org/2001/XMLSchema#string"/>
        <rdfs:comment>A datatype property that represents the unique identifier code assigned to a local authority.</rdfs:comment>
        <rdfs:isDefinedBy rdf:resource="http://www.theworldavatar.com/ontology/OntoFHRS/"/>
        <rdfs:label>has local authority code</rdfs:label>
    </owl:DatatypeProperty>
    


    <!-- http://www.theworldavatar.com/ontology/OntoFHRS/hasName -->


    <owl:DatatypeProperty rdf:about="http://www.theworldavatar.com/ontology/OntoFHRS/hasName">
        <rdfs:domain>
            <owl:Class>
                <owl:unionOf rdf:parseType="Collection">
                    <rdf:Description rdf:about="http://www.theworldavatar.com/ontology/OntoFHRS/BusinessEstablishment"/>
                    <rdf:Description rdf:about="http://www.theworldavatar.com/ontology/OntoFHRS/DistrictCouncil"/>
                    <rdf:Description rdf:about="http://www.theworldavatar.com/ontology/OntoFHRS/LocalAuthority"/>
                </owl:unionOf>
            </owl:Class>
        </rdfs:domain>
        <rdfs:range rdf:resource="http://www.w3.org/2001/XMLSchema#string"/>
        <rdfs:comment>A datatype property that represents the human-readable identifier or name of an entity, such as a business establishment, local authority, and district council.</rdfs:comment>
        <rdfs:isDefinedBy rdf:resource="http://www.theworldavatar.com/ontology/OntoFHRS/"/>
        <rdfs:label>has name</rdfs:label>
    </owl:DatatypeProperty>
    


    <!-- http://www.theworldavatar.com/ontology/OntoFHRS/hasPostcode -->


    <owl:DatatypeProperty rdf:about="http://www.theworldavatar.com/ontology/OntoFHRS/hasPostcode">
        <rdfs:domain rdf:resource="http://ies.data.gov.uk/ontology/ies4#Address"/>
        <rdfs:range rdf:resource="http://www.w3.org/2001/XMLSchema#string"/>
        <rdfs:comment>A datatype property that represents the postcode in the address of a business establishment.</rdfs:comment>
        <rdfs:isDefinedBy rdf:resource="http://www.theworldavatar.com/ontology/OntoFHRS/"/>
        <rdfs:label>has postcode</rdfs:label>
    </owl:DatatypeProperty>
    


    <!-- http://www.theworldavatar.com/ontology/OntoFHRS/hasStreetNumber -->


    <owl:DatatypeProperty rdf:about="http://www.theworldavatar.com/ontology/OntoFHRS/hasStreetNumber">
        <rdfs:domain rdf:resource="http://ies.data.gov.uk/ontology/ies4#Address"/>
        <rdfs:range rdf:resource="http://www.w3.org/2001/XMLSchema#string"/>
        <rdfs:comment>A datatype property that denotes the street number component in the address of a business establishment.</rdfs:comment>
        <rdfs:isDefinedBy rdf:resource="http://www.theworldavatar.com/ontology/OntoFHRS/"/>
        <rdfs:label>has street number</rdfs:label>
    </owl:DatatypeProperty>
    


    <!-- http://www.theworldavatar.com/ontology/OntoFHRS/hasValue -->


    <owl:DatatypeProperty rdf:about="http://www.theworldavatar.com/ontology/OntoFHRS/hasValue">
        <rdfs:domain>
            <owl:Class>
                <owl:unionOf rdf:parseType="Collection">
                    <rdf:Description rdf:about="http://www.theworldavatar.com/ontology/OntoFHRS/Rating"/>
                    <rdf:Description rdf:about="http://www.theworldavatar.com/ontology/OntoFHRS/Score"/>
                </owl:unionOf>
            </owl:Class>
        </rdfs:domain>
        <rdfs:range rdf:resource="http://www.w3.org/2001/XMLSchema#string"/>
        <rdfs:comment>A datatype property that represents the value of the rating or hygiene score of a business establishment.</rdfs:comment>
        <rdfs:isDefinedBy rdf:resource="http://www.theworldavatar.com/ontology/OntoFHRS/"/>
        <rdfs:label>has value</rdfs:label>
    </owl:DatatypeProperty>
    


    <!-- http://www.theworldavatar.com/ontology/OntoFHRS/hasWebsite -->


    <owl:DatatypeProperty rdf:about="http://www.theworldavatar.com/ontology/OntoFHRS/hasWebsite">
        <rdfs:domain rdf:resource="http://www.theworldavatar.com/ontology/OntoFHRS/LocalAuthority"/>
        <rdfs:range rdf:resource="http://www.w3.org/2001/XMLSchema#anyURI"/>
        <rdfs:comment>A datatype property that denotes the official web address (URL) of a local authority, providing access to its online resources and services.</rdfs:comment>
        <rdfs:isDefinedBy rdf:resource="http://www.theworldavatar.com/ontology/OntoFHRS/"/>
        <rdfs:label>has website</rdfs:label>
    </owl:DatatypeProperty>
    


    <!-- http://www.theworldavatar.com/ontology/OntoFHRS/indicatesQuality -->


    <owl:DatatypeProperty rdf:about="http://www.theworldavatar.com/ontology/OntoFHRS/indicatesQuality">
        <rdfs:domain rdf:resource="http://www.theworldavatar.com/ontology/OntoFHRS/Rating"/>
        <rdfs:range rdf:resource="http://www.w3.org/2001/XMLSchema#string"/>
        <rdfs:comment>A datatype property that represents the quality of the rating of a business establishment. The quality can be very good, good, generally satisfactory, improvement necessary, major improvement necessary or urgent improvement necessary.</rdfs:comment>
        <rdfs:isDefinedBy rdf:resource="http://www.theworldavatar.com/ontology/OntoFHRS/"/>
        <rdfs:label>indicates quality</rdfs:label>
    </owl:DatatypeProperty>
    


    <!-- http://www.theworldavatar.com/ontology/OntoFHRS/isNewRatingPending -->


    <owl:DatatypeProperty rdf:about="http://www.theworldavatar.com/ontology/OntoFHRS/isNewRatingPending">
        <rdfs:domain rdf:resource="http://www.theworldavatar.com/ontology/OntoFHRS/BusinessEstablishment"/>
        <rdfs:range rdf:resource="http://www.w3.org/2001/XMLSchema#boolean"/>
        <rdfs:comment>A datatype property that indicates whether a business establishment is awaiting the assignment of a new rating.</rdfs:comment>
        <rdfs:isDefinedBy rdf:resource="http://www.theworldavatar.com/ontology/OntoFHRS/"/>
        <rdfs:label>is new rating pending</rdfs:label>
    </owl:DatatypeProperty>
    


    <!-- 
    ///////////////////////////////////////////////////////////////////////////////////////
    //
    // Classes
    //
    ///////////////////////////////////////////////////////////////////////////////////////
     -->


    


    <!-- http://ies.data.gov.uk/ontology/ies4#Address -->


    <owl:Class rdf:about="http://ies.data.gov.uk/ontology/ies4#Address">
        <rdfs:comment>A collection of information required to identify the exact place or location of a business establishment.</rdfs:comment>
        <rdfs:isDefinedBy rdf:resource="http://ies.data.gov.uk/ontology/ies4"/>
        <rdfs:label>Address</rdfs:label>
    </owl:Class>
    


    <!-- http://ies.data.gov.uk/ontology/ies4#BoundingState -->


    <owl:Class rdf:about="http://ies.data.gov.uk/ontology/ies4#BoundingState">
        <rdfs:isDefinedBy rdf:resource="http://ies.data.gov.uk/ontology/ies4"/>
        <rdfs:label>Bounding State</rdfs:label>
    </owl:Class>
    


    <!-- http://ies.data.gov.uk/ontology/ies4#ParticularPeriod -->


    <owl:Class rdf:about="http://ies.data.gov.uk/ontology/ies4#ParticularPeriod">
        <rdfs:isDefinedBy rdf:resource="http://ies.data.gov.uk/ontology/ies4"/>
        <rdfs:label>Particular Period</rdfs:label>
    </owl:Class>
    


    <!-- http://www.theworldavatar.com/ontology/OntoFHRS/Bar -->


    <owl:Class rdf:about="http://www.theworldavatar.com/ontology/OntoFHRS/Bar">
        <rdfs:subClassOf rdf:resource="http://www.theworldavatar.com/ontology/OntoFHRS/BusinessEstablishment"/>
        <rdfs:comment>A business establishment that serves alcoholic drinks.</rdfs:comment>
        <rdfs:isDefinedBy rdf:resource="http://www.theworldavatar.com/ontology/OntoFHRS/"/>
        <rdfs:label>Bar</rdfs:label>
    </owl:Class>
    


    <!-- http://www.theworldavatar.com/ontology/OntoFHRS/BedandBreakfast -->


    <owl:Class rdf:about="http://www.theworldavatar.com/ontology/OntoFHRS/BedandBreakfast">
        <rdfs:subClassOf rdf:resource="http://www.theworldavatar.com/ontology/OntoFHRS/BusinessEstablishment"/>
        <rdfs:comment>A small-scale lodging establishment, typically in a private home, that provides overnight stay and breakfast to travellers.</rdfs:comment>
        <rdfs:isDefinedBy rdf:resource="http://www.theworldavatar.com/ontology/OntoFHRS/"/>
        <rdfs:label>Bed and Breakfast</rdfs:label>
    </owl:Class>
    


    <!-- http://www.theworldavatar.com/ontology/OntoFHRS/BusinessEstablishment -->


    <owl:Class rdf:about="http://www.theworldavatar.com/ontology/OntoFHRS/BusinessEstablishment">
        <rdfs:comment>An establishment dedicated to commercial activities, goods production, processing, storage, or offering services.</rdfs:comment>
        <rdfs:isDefinedBy rdf:resource="http://www.theworldavatar.com/ontology/OntoFHRS/"/>
        <rdfs:label>Business Establishment</rdfs:label>
    </owl:Class>
    


    <!-- http://www.theworldavatar.com/ontology/OntoFHRS/BusinessEstablishmentEnd -->


    <owl:Class rdf:about="http://www.theworldavatar.com/ontology/OntoFHRS/BusinessEstablishmentEnd">
        <rdfs:subClassOf rdf:resource="http://ies.data.gov.uk/ontology/ies4#BoundingState"/>
        <rdfs:subClassOf>
            <owl:Restriction>
                <owl:onProperty rdf:resource="http://ies.data.gov.uk/ontology/ies4#isEndOf"/>
                <owl:allValuesFrom rdf:resource="http://www.theworldavatar.com/ontology/OntoFHRS/BusinessEstablishment"/>
            </owl:Restriction>
        </rdfs:subClassOf>
        <rdfs:comment>The date of decommissioning or closure of a business establishment.</rdfs:comment>
        <rdfs:isDefinedBy rdf:resource="http://www.theworldavatar.com/ontology/OntoFHRS/"/>
        <rdfs:label>Business Establishment End</rdfs:label>
    </owl:Class>
    


    <!-- http://www.theworldavatar.com/ontology/OntoFHRS/BusinessEstablishmentStart -->


    <owl:Class rdf:about="http://www.theworldavatar.com/ontology/OntoFHRS/BusinessEstablishmentStart">
        <rdfs:subClassOf rdf:resource="http://ies.data.gov.uk/ontology/ies4#BoundingState"/>
        <rdfs:subClassOf>
            <owl:Restriction>
                <owl:onProperty rdf:resource="http://ies.data.gov.uk/ontology/ies4#isStartOf"/>
                <owl:allValuesFrom rdf:resource="http://www.theworldavatar.com/ontology/OntoFHRS/BusinessEstablishment"/>
            </owl:Restriction>
        </rdfs:subClassOf>
        <rdfs:comment>Tthe official date when the business began operations or was inaugurated.</rdfs:comment>
        <rdfs:isDefinedBy rdf:resource="http://www.theworldavatar.com/ontology/OntoFHRS/"/>
        <rdfs:label>Business Establishment Start</rdfs:label>
    </owl:Class>
    


    <!-- http://www.theworldavatar.com/ontology/OntoFHRS/Cafe -->


    <owl:Class rdf:about="http://www.theworldavatar.com/ontology/OntoFHRS/Cafe">
        <rdfs:subClassOf rdf:resource="http://www.theworldavatar.com/ontology/OntoFHRS/BusinessEstablishment"/>
        <rdfs:comment>A business establishment where people can drink coffee, tea, and other beverages and eat light meals and snacks.</rdfs:comment>
        <rdfs:isDefinedBy rdf:resource="http://www.theworldavatar.com/ontology/OntoFHRS/"/>
        <rdfs:label>Cafe</rdfs:label>
    </owl:Class>
    


    <!-- http://www.theworldavatar.com/ontology/OntoFHRS/Canteen -->


    <owl:Class rdf:about="http://www.theworldavatar.com/ontology/OntoFHRS/Canteen">
        <rdfs:subClassOf rdf:resource="http://www.theworldavatar.com/ontology/OntoFHRS/BusinessEstablishment"/>
        <rdfs:comment>A business establishment that serves food and drinks in educational institutions, workplaces, or other organisations.</rdfs:comment>
        <rdfs:isDefinedBy rdf:resource="http://www.theworldavatar.com/ontology/OntoFHRS/"/>
        <rdfs:label>Canteen</rdfs:label>
    </owl:Class>
    


    <!-- http://www.theworldavatar.com/ontology/OntoFHRS/CaringPremiseFoodFacility -->


    <owl:Class rdf:about="http://www.theworldavatar.com/ontology/OntoFHRS/CaringPremiseFoodFacility">
        <rdfs:subClassOf rdf:resource="http://www.theworldavatar.com/ontology/OntoFHRS/BusinessEstablishment"/>
        <rdfs:comment>A food facility within a caring premise that provides meals and snacks tailored to the dietary needs of residents.</rdfs:comment>
        <rdfs:isDefinedBy rdf:resource="http://www.theworldavatar.com/ontology/OntoFHRS/"/>
        <rdfs:label>Caring Premise Food Facility</rdfs:label>
    </owl:Class>
    


    <!-- http://www.theworldavatar.com/ontology/OntoFHRS/CateringPremise -->


    <owl:Class rdf:about="http://www.theworldavatar.com/ontology/OntoFHRS/CateringPremise">
        <rdfs:subClassOf rdf:resource="http://www.theworldavatar.com/ontology/OntoFHRS/BusinessEstablishment"/>
        <rdfs:comment>A food establishment that generally serves food to be consumed on its premises.</rdfs:comment>
        <rdfs:isDefinedBy rdf:resource="http://www.theworldavatar.com/ontology/OntoFHRS/"/>
        <rdfs:label>Catering Premise</rdfs:label>
    </owl:Class>
    


    <!-- http://www.theworldavatar.com/ontology/OntoFHRS/ChildcarePremiseFoodFacility -->


    <owl:Class rdf:about="http://www.theworldavatar.com/ontology/OntoFHRS/ChildcarePremiseFoodFacility">
        <rdfs:subClassOf rdf:resource="http://www.theworldavatar.com/ontology/OntoFHRS/BusinessEstablishment"/>
        <rdfs:comment>A food facility within a childcare centre serving meals and snacks to children.</rdfs:comment>
        <rdfs:isDefinedBy rdf:resource="http://www.theworldavatar.com/ontology/OntoFHRS/"/>
        <rdfs:label>Childcare Premise Food Facility</rdfs:label>
    </owl:Class>
    


    <!-- http://www.theworldavatar.com/ontology/OntoFHRS/CollegeCanteen -->


    <owl:Class rdf:about="http://www.theworldavatar.com/ontology/OntoFHRS/CollegeCanteen">
        <rdfs:subClassOf rdf:resource="http://www.theworldavatar.com/ontology/OntoFHRS/Canteen"/>
        <rdfs:comment>A canteen that offers food and drinks to students, faculty and staff on a college campus.</rdfs:comment>
        <rdfs:isDefinedBy rdf:resource="http://www.theworldavatar.com/ontology/OntoFHRS/"/>
        <rdfs:label>College Canteen</rdfs:label>
    </owl:Class>
    


    <!-- http://www.theworldavatar.com/ontology/OntoFHRS/ConfidenceInManagementScore -->


    <owl:Class rdf:about="http://www.theworldavatar.com/ontology/OntoFHRS/ConfidenceInManagementScore">
        <rdfs:subClassOf rdf:resource="http://www.theworldavatar.com/ontology/OntoFHRS/Score"/>
        <rdfs:comment>A score indicating the adequacy of implementing food safety management procedures, staff training, and awareness of potential hazards in a business establishment that serves or sells food and drinks. The score can be 0, 5, 10, 20 or 30. The lower the score, the better. The following document provides a detailed description of the confidence in management score: https://www.ncass.org.uk/wp-content/uploads/2023/01/Food-Hygiene-Rating-Scheme-Guide.pdf.</rdfs:comment>
        <rdfs:isDefinedBy rdf:resource="http://www.theworldavatar.com/ontology/OntoFHRS/"/>
        <rdfs:label>Confidence In Management Score</rdfs:label>
    </owl:Class>
    


    <!-- http://www.theworldavatar.com/ontology/OntoFHRS/DistrictCouncil -->


    <owl:Class rdf:about="http://www.theworldavatar.com/ontology/OntoFHRS/DistrictCouncil">
        <rdfs:comment>An administrative unit with responsibilities for providing rubbish collection, recreational, environmental, and other services within the associated geographical boundary.</rdfs:comment>
        <rdfs:isDefinedBy rdf:resource="http://www.theworldavatar.com/ontology/OntoFHRS/"/>
        <rdfs:label>District council</rdfs:label>
    </owl:Class>
    


    <!-- http://www.theworldavatar.com/ontology/OntoFHRS/FarmerFoodFacility -->


    <owl:Class rdf:about="http://www.theworldavatar.com/ontology/OntoFHRS/FarmerFoodFacility">
        <rdfs:subClassOf rdf:resource="http://www.theworldavatar.com/ontology/OntoFHRS/BusinessEstablishment"/>
        <rdfs:comment>A business establishment where farmers process, package and sell locally produced food or drink.</rdfs:comment>
        <rdfs:isDefinedBy rdf:resource="http://www.theworldavatar.com/ontology/OntoFHRS/"/>
        <rdfs:label>Farmer Food Facility</rdfs:label>
    </owl:Class>
    


    <!-- http://www.theworldavatar.com/ontology/OntoFHRS/FoodDistributor -->


    <owl:Class rdf:about="http://www.theworldavatar.com/ontology/OntoFHRS/FoodDistributor">
        <rdfs:subClassOf rdf:resource="http://www.theworldavatar.com/ontology/OntoFHRS/BusinessEstablishment"/>
        <rdfs:comment>A business establishment that distributes food products from manufacturers and producers to retailers, restaurants and other outlets.</rdfs:comment>
        <rdfs:isDefinedBy rdf:resource="http://www.theworldavatar.com/ontology/OntoFHRS/"/>
        <rdfs:label>Food Distributor</rdfs:label>
    </owl:Class>
    


    <!-- http://www.theworldavatar.com/ontology/OntoFHRS/FoodManufacturer -->


    <owl:Class rdf:about="http://www.theworldavatar.com/ontology/OntoFHRS/FoodManufacturer">
        <rdfs:subClassOf rdf:resource="http://www.theworldavatar.com/ontology/OntoFHRS/BusinessEstablishment"/>
        <rdfs:comment>A business establishment that processes raw ingredients into consumable food products.</rdfs:comment>
        <rdfs:isDefinedBy rdf:resource="http://www.theworldavatar.com/ontology/OntoFHRS/"/>
        <rdfs:label>Food Manufacturer</rdfs:label>
    </owl:Class>
    


    <!-- http://www.theworldavatar.com/ontology/OntoFHRS/FoodPacker -->


    <owl:Class rdf:about="http://www.theworldavatar.com/ontology/OntoFHRS/FoodPacker">
        <rdfs:subClassOf rdf:resource="http://www.theworldavatar.com/ontology/OntoFHRS/BusinessEstablishment"/>
        <rdfs:comment>A business establishment that packages food products for shipment, distribution, delivery and consumption.</rdfs:comment>
        <rdfs:isDefinedBy rdf:resource="http://www.theworldavatar.com/ontology/OntoFHRS/"/>
        <rdfs:label>Food Packer</rdfs:label>
    </owl:Class>
    


    <!-- http://www.theworldavatar.com/ontology/OntoFHRS/FoodRetailer -->


    <owl:Class rdf:about="http://www.theworldavatar.com/ontology/OntoFHRS/FoodRetailer">
        <rdfs:subClassOf rdf:resource="http://www.theworldavatar.com/ontology/OntoFHRS/BusinessEstablishment"/>
        <rdfs:comment>A business establishment that sells food products directly to the public, end users or consumers.</rdfs:comment>
        <rdfs:isDefinedBy rdf:resource="http://www.theworldavatar.com/ontology/OntoFHRS/"/>
        <rdfs:label>Food Retailer</rdfs:label>
    </owl:Class>
    


    <!-- http://www.theworldavatar.com/ontology/OntoFHRS/FoodTransporter -->


    <owl:Class rdf:about="http://www.theworldavatar.com/ontology/OntoFHRS/FoodTransporter">
        <rdfs:subClassOf rdf:resource="http://www.theworldavatar.com/ontology/OntoFHRS/BusinessEstablishment"/>
        <rdfs:comment>A business establishment that transports food products from manufacturers and producers to retailers, restaurants and other outlets.</rdfs:comment>
        <rdfs:isDefinedBy rdf:resource="http://www.theworldavatar.com/ontology/OntoFHRS/"/>
        <rdfs:label>Food Transporter</rdfs:label>
    </owl:Class>
    


    <!-- http://www.theworldavatar.com/ontology/OntoFHRS/GrowerFoodFacility -->


    <owl:Class rdf:about="http://www.theworldavatar.com/ontology/OntoFHRS/GrowerFoodFacility">
        <rdfs:subClassOf rdf:resource="http://www.theworldavatar.com/ontology/OntoFHRS/BusinessEstablishment"/>
        <rdfs:comment>A business establishment where growers sell locally produced food products or drink.</rdfs:comment>
        <rdfs:isDefinedBy rdf:resource="http://www.theworldavatar.com/ontology/OntoFHRS/"/>
        <rdfs:label>Grower Food Facility</rdfs:label>
    </owl:Class>
    


    <!-- http://www.theworldavatar.com/ontology/OntoFHRS/GuestHouse -->


    <owl:Class rdf:about="http://www.theworldavatar.com/ontology/OntoFHRS/GuestHouse">
        <rdfs:subClassOf rdf:resource="http://www.theworldavatar.com/ontology/OntoFHRS/BusinessEstablishment"/>
        <rdfs:comment>A lodging establishment in a private house, usually smaller than a hotel, that offers travellers overnight stays and occasionally meals.</rdfs:comment>
        <rdfs:isDefinedBy rdf:resource="http://www.theworldavatar.com/ontology/OntoFHRS/"/>
        <rdfs:label>Guest House</rdfs:label>
    </owl:Class>
    


    <!-- http://www.theworldavatar.com/ontology/OntoFHRS/HospitalPremiseFoodFacility -->


    <owl:Class rdf:about="http://www.theworldavatar.com/ontology/OntoFHRS/HospitalPremiseFoodFacility">
        <rdfs:subClassOf rdf:resource="http://www.theworldavatar.com/ontology/OntoFHRS/BusinessEstablishment"/>
        <rdfs:comment>A business establishment within a hospital that serves food and beverages to patients, staff, and visitors.</rdfs:comment>
        <rdfs:isDefinedBy rdf:resource="http://www.theworldavatar.com/ontology/OntoFHRS/"/>
        <rdfs:label>Hospital Premise Food Facility</rdfs:label>
    </owl:Class>
    


    <!-- http://www.theworldavatar.com/ontology/OntoFHRS/Hotel -->


    <owl:Class rdf:about="http://www.theworldavatar.com/ontology/OntoFHRS/Hotel">
        <rdfs:subClassOf rdf:resource="http://www.theworldavatar.com/ontology/OntoFHRS/BusinessEstablishment"/>
        <rdfs:comment>A business establishment that provides travellers lodging, meals and other services.</rdfs:comment>
        <rdfs:isDefinedBy rdf:resource="http://www.theworldavatar.com/ontology/OntoFHRS/"/>
        <rdfs:label>Hotel</rdfs:label>
    </owl:Class>
    


    <!-- http://www.theworldavatar.com/ontology/OntoFHRS/HygieneScore -->


    <owl:Class rdf:about="http://www.theworldavatar.com/ontology/OntoFHRS/HygieneScore">
        <rdfs:subClassOf rdf:resource="http://www.theworldavatar.com/ontology/OntoFHRS/Score"/>
        <rdfs:comment>A score indicating the food safety and hygiene of a business establishment that serves or sells food and drinks. The score can be 0, 5, 10, 15, 20 or 25. The lower the score, the better. The following document provides a detailed description of the hygiene score: https://www.ncass.org.uk/wp-content/uploads/2023/01/Food-Hygiene-Rating-Scheme-Guide.pdf.</rdfs:comment>
        <rdfs:isDefinedBy rdf:resource="http://www.theworldavatar.com/ontology/OntoFHRS/"/>
        <rdfs:label>Hygiene Score</rdfs:label>
    </owl:Class>
    


    <!-- http://www.theworldavatar.com/ontology/OntoFHRS/Hypermarket -->


    <owl:Class rdf:about="http://www.theworldavatar.com/ontology/OntoFHRS/Hypermarket">
        <rdfs:subClassOf rdf:resource="http://www.theworldavatar.com/ontology/OntoFHRS/BusinessEstablishment"/>
        <rdfs:comment>A large-scale supermarket often located on the outskirts of a city, offering a vast array of goods including groceries, clothes, furniture, and household items.</rdfs:comment>
        <rdfs:isDefinedBy rdf:resource="http://www.theworldavatar.com/ontology/OntoFHRS/"/>
        <rdfs:label>Hypermarket</rdfs:label>
    </owl:Class>
    


    <!-- http://www.theworldavatar.com/ontology/OntoFHRS/LocalAuthority -->


    <owl:Class rdf:about="http://www.theworldavatar.com/ontology/OntoFHRS/LocalAuthority">
        <rdfs:comment>An organisation that is officially responsible for overseeing all public services and amenities within a specific region, guided by the local government.</rdfs:comment>
        <rdfs:isDefinedBy rdf:resource="http://www.theworldavatar.com/ontology/OntoFHRS/"/>
        <rdfs:label>Local Authority</rdfs:label>
    </owl:Class>
    


    <!-- http://www.theworldavatar.com/ontology/OntoFHRS/MobileCaterer -->


    <owl:Class rdf:about="http://www.theworldavatar.com/ontology/OntoFHRS/MobileCaterer">
        <rdfs:subClassOf rdf:resource="http://www.theworldavatar.com/ontology/OntoFHRS/BusinessEstablishment"/>
        <rdfs:comment>A business establishment that serves food and drinks from a vehicle that can move from one location to another.</rdfs:comment>
        <rdfs:isDefinedBy rdf:resource="http://www.theworldavatar.com/ontology/OntoFHRS/"/>
        <rdfs:label>Mobile Caterer</rdfs:label>
    </owl:Class>
    


    <!-- http://www.theworldavatar.com/ontology/OntoFHRS/NightClub -->


    <owl:Class rdf:about="http://www.theworldavatar.com/ontology/OntoFHRS/NightClub">
        <rdfs:subClassOf rdf:resource="http://www.theworldavatar.com/ontology/OntoFHRS/BusinessEstablishment"/>
        <rdfs:comment>A business establishment that remains open until late at night, offering food and drink alongside entertainment such as live music, dance performances, and dancing opportunities.</rdfs:comment>
        <rdfs:isDefinedBy rdf:resource="http://www.theworldavatar.com/ontology/OntoFHRS/"/>
        <rdfs:label>Night Club</rdfs:label>
    </owl:Class>
    


    <!-- http://www.theworldavatar.com/ontology/OntoFHRS/Pub -->


    <owl:Class rdf:about="http://www.theworldavatar.com/ontology/OntoFHRS/Pub">
        <rdfs:subClassOf rdf:resource="http://www.theworldavatar.com/ontology/OntoFHRS/BusinessEstablishment"/>
        <rdfs:comment>A business establishment that serves alcoholic drinks, especially beer, as well as other beverages, and often offers light meals.</rdfs:comment>
        <rdfs:isDefinedBy rdf:resource="http://www.theworldavatar.com/ontology/OntoFHRS/"/>
        <rdfs:label>Pub</rdfs:label>
    </owl:Class>
    


    <!-- http://www.theworldavatar.com/ontology/OntoFHRS/Rating -->


    <owl:Class rdf:about="http://www.theworldavatar.com/ontology/OntoFHRS/Rating">
        <rdfs:comment>The level of standard maintained by a business establishment for food safety and preparation,  on a scale from 5, indicating very good, to 0 indicating urgent improvement required. The following document provides a detailed description of the Food Hygiene Rating Scheme: https://www.ncass.org.uk/wp-content/uploads/2023/01/Food-Hygiene-Rating-Scheme-Guide.pdf.</rdfs:comment>
        <rdfs:isDefinedBy rdf:resource="http://www.theworldavatar.com/ontology/OntoFHRS/"/>
        <rdfs:label>Rating</rdfs:label>
    </owl:Class>
    


    <!-- http://www.theworldavatar.com/ontology/OntoFHRS/RatingEnd -->


    <owl:Class rdf:about="http://www.theworldavatar.com/ontology/OntoFHRS/RatingEnd">
        <rdfs:subClassOf rdf:resource="http://ies.data.gov.uk/ontology/ies4#BoundingState"/>
        <rdfs:subClassOf>
            <owl:Restriction>
                <owl:onProperty rdf:resource="http://ies.data.gov.uk/ontology/ies4#isEndOf"/>
                <owl:allValuesFrom rdf:resource="http://www.theworldavatar.com/ontology/OntoFHRS/BusinessEstablishment"/>
            </owl:Restriction>
        </rdfs:subClassOf>
        <rdfs:comment>The date on which a rating of a business establishment expired.</rdfs:comment>
        <rdfs:isDefinedBy rdf:resource="http://www.theworldavatar.com/ontology/OntoFHRS/"/>
        <rdfs:label>Rating End</rdfs:label>
    </owl:Class>
    


    <!-- http://www.theworldavatar.com/ontology/OntoFHRS/RatingScheme -->


    <owl:Class rdf:about="http://www.theworldavatar.com/ontology/OntoFHRS/RatingScheme">
        <rdfs:comment>A scheme to assess hygiene practices, food handling, structural conditions, and management procedures of business establishments serving or selling food and drinks.</rdfs:comment>
        <rdfs:isDefinedBy rdf:resource="http://www.theworldavatar.com/ontology/OntoFHRS/"/>
        <rdfs:label>Rating Scheme</rdfs:label>
    </owl:Class>
    


    <!-- http://www.theworldavatar.com/ontology/OntoFHRS/RatingStart -->


    <owl:Class rdf:about="http://www.theworldavatar.com/ontology/OntoFHRS/RatingStart">
        <rdfs:subClassOf rdf:resource="http://ies.data.gov.uk/ontology/ies4#BoundingState"/>
        <rdfs:subClassOf>
            <owl:Restriction>
                <owl:onProperty rdf:resource="http://ies.data.gov.uk/ontology/ies4#isStartOf"/>
                <owl:allValuesFrom rdf:resource="http://www.theworldavatar.com/ontology/OntoFHRS/BusinessEstablishment"/>
            </owl:Restriction>
        </rdfs:subClassOf>
        <rdfs:comment>The initial date when a rating became effective for a business establishment.</rdfs:comment>
        <rdfs:isDefinedBy rdf:resource="http://www.theworldavatar.com/ontology/OntoFHRS/"/>
        <rdfs:label>Rating Start</rdfs:label>
    </owl:Class>
    


    <!-- http://www.theworldavatar.com/ontology/OntoFHRS/Restaurant -->


    <owl:Class rdf:about="http://www.theworldavatar.com/ontology/OntoFHRS/Restaurant">
        <rdfs:subClassOf rdf:resource="http://www.theworldavatar.com/ontology/OntoFHRS/BusinessEstablishment"/>
        <rdfs:comment>A business establishment where people can consume food and drinks.</rdfs:comment>
        <rdfs:isDefinedBy rdf:resource="http://www.theworldavatar.com/ontology/OntoFHRS/"/>
        <rdfs:label>Restaurant</rdfs:label>
    </owl:Class>
    


    <!-- http://www.theworldavatar.com/ontology/OntoFHRS/SandwichShop -->


    <owl:Class rdf:about="http://www.theworldavatar.com/ontology/OntoFHRS/SandwichShop">
        <rdfs:subClassOf rdf:resource="http://www.theworldavatar.com/ontology/OntoFHRS/BusinessEstablishment"/>
        <rdfs:comment>A food establishment that generally sells a variety of sandwiches, often prepared on the premises.</rdfs:comment>
        <rdfs:isDefinedBy rdf:resource="http://www.theworldavatar.com/ontology/OntoFHRS/"/>
        <rdfs:label>Sandwich Shop</rdfs:label>
    </owl:Class>
    


    <!-- http://www.theworldavatar.com/ontology/OntoFHRS/SchoolCanteen -->


    <owl:Class rdf:about="http://www.theworldavatar.com/ontology/OntoFHRS/SchoolCanteen">
        <rdfs:subClassOf rdf:resource="http://www.theworldavatar.com/ontology/OntoFHRS/Canteen"/>
        <rdfs:comment>A canteen that offers food and drinks to students and staff in a school.</rdfs:comment>
        <rdfs:isDefinedBy rdf:resource="http://www.theworldavatar.com/ontology/OntoFHRS/"/>
        <rdfs:label>School Canteen</rdfs:label>
    </owl:Class>
    


    <!-- http://www.theworldavatar.com/ontology/OntoFHRS/Score -->


    <owl:Class rdf:about="http://www.theworldavatar.com/ontology/OntoFHRS/Score">
        <rdfs:comment>A quantitative measure indicating the overall quality, including food safety and hygiene, structural adequacy, and food safety management procedure of a business establishment that serves or sells food and drinks.</rdfs:comment>
        <rdfs:isDefinedBy rdf:resource="http://www.theworldavatar.com/ontology/OntoFHRS/"/>
        <rdfs:label>Score</rdfs:label>
    </owl:Class>
    


    <!-- http://www.theworldavatar.com/ontology/OntoFHRS/StructuralScore -->


    <owl:Class rdf:about="http://www.theworldavatar.com/ontology/OntoFHRS/StructuralScore">
        <rdfs:subClassOf rdf:resource="http://www.theworldavatar.com/ontology/OntoFHRS/Score"/>
        <rdfs:comment>A score indicating the level of structural adequacy required to operate safely and the design layout that prevents cross-contamination in a business establishment that serves or sells food and drinks. The score can be 0, 5, 10, 15, 20 or 25. The lower the score, the better. The following document provides a detailed description of the structural score: https://www.ncass.org.uk/wp-content/uploads/2023/01/Food-Hygiene-Rating-Scheme-Guide.pdf.</rdfs:comment>
        <rdfs:isDefinedBy rdf:resource="http://www.theworldavatar.com/ontology/OntoFHRS/"/>
        <rdfs:label>Structural Score</rdfs:label>
    </owl:Class>
    


    <!-- http://www.theworldavatar.com/ontology/OntoFHRS/Supermarket -->


    <owl:Class rdf:about="http://www.theworldavatar.com/ontology/OntoFHRS/Supermarket">
        <rdfs:subClassOf rdf:resource="http://www.theworldavatar.com/ontology/OntoFHRS/BusinessEstablishment"/>
        <rdfs:comment>A business establishment that sells groceries, food, dairy products and household items.</rdfs:comment>
        <rdfs:isDefinedBy rdf:resource="http://www.theworldavatar.com/ontology/OntoFHRS/"/>
        <rdfs:label>Supermarket</rdfs:label>
    </owl:Class>
    


    <!-- http://www.theworldavatar.com/ontology/OntoFHRS/Takeaway -->


    <owl:Class rdf:about="http://www.theworldavatar.com/ontology/OntoFHRS/Takeaway">
        <rdfs:subClassOf rdf:resource="http://www.theworldavatar.com/ontology/OntoFHRS/BusinessEstablishment"/>
        <rdfs:comment>A food establishment that sells cooked food to be eaten elsewhere, away from its premises.</rdfs:comment>
        <rdfs:isDefinedBy rdf:resource="http://www.theworldavatar.com/ontology/OntoFHRS/"/>
        <rdfs:label>Takeaway</rdfs:label>
    </owl:Class>
    


    <!-- http://www.theworldavatar.com/ontology/OntoFHRS/UniversityCanteen -->


    <owl:Class rdf:about="http://www.theworldavatar.com/ontology/OntoFHRS/UniversityCanteen">
        <rdfs:subClassOf rdf:resource="http://www.theworldavatar.com/ontology/OntoFHRS/Canteen"/>
        <rdfs:comment>A canteen located on a university campus that offers food and beverages to students, faculty, staff, and sometimes visitors.</rdfs:comment>
        <rdfs:isDefinedBy rdf:resource="http://www.theworldavatar.com/ontology/OntoFHRS/"/>
        <rdfs:label>University Canteen</rdfs:label>
    </owl:Class>
    


    <!-- https://dbpedia.org/ontology/City -->


    <owl:Class rdf:about="https://dbpedia.org/ontology/City">
        <rdfs:isDefinedBy rdf:resource="https://dbpedia.org/ontology"/>
        <rdfs:label>City</rdfs:label>
    </owl:Class>
    


    <!-- https://dbpedia.org/ontology/Country -->


    <owl:Class rdf:about="https://dbpedia.org/ontology/Country">
        <rdfs:isDefinedBy rdf:resource="https://dbpedia.org/ontology"/>
        <rdfs:label>Country</rdfs:label>
    </owl:Class>
    


    <!-- https://dbpedia.org/ontology/Region -->


    <owl:Class rdf:about="https://dbpedia.org/ontology/Region">
        <rdfs:isDefinedBy rdf:resource="https://dbpedia.org/ontology"/>
        <rdfs:label>Region</rdfs:label>
    </owl:Class>
</rdf:RDF>



<!-- Generated by the OWL API (version 5.5.0.2023-01-14T12:41:38Z) https://github.com/owlcs/owlapi/ -->


