<?xml version="1.0"?>
<rdf:RDF xmlns="https://www.theworldavatar.com/kg/ontobuildingstructure/"
     xml:base="https://www.theworldavatar.com/kg/ontobuildingstructure/"
     xmlns:dc="http://purl.org/dc/elements/1.1/"
     xmlns:owl="http://www.w3.org/2002/07/owl#"
     xmlns:rdf="http://www.w3.org/1999/02/22-rdf-syntax-ns#"
     xmlns:xml="http://www.w3.org/XML/1998/namespace"
     xmlns:xsd="http://www.w3.org/2001/XMLSchema#"
     xmlns:rdfs="http://www.w3.org/2000/01/rdf-schema#"
     xmlns:ontobuildingstructure="https://www.theworldavatar.com/kg/ontobuildingstructure/">
    <owl:Ontology rdf:about="https://www.theworldavatar.com/kg/ontobuildingstructure/">
        <dc:date>02 January 2024</dc:date>
        <rdfs:comment>The Building Structure ontology (OntoBuildingStructure) is an ontology developed to represent the building structural components (walls, doors, slabs, roofs, stairs) and their individual characteristics such as dimensions and qualities.</rdfs:comment>
        <owl:versionInfo>1</owl:versionInfo>
        <gitCommitHash>c0599beca8df55873a1ab061dee64e52c510c6a0</gitCommitHash>
    </owl:Ontology>
    


    <!-- 
    ///////////////////////////////////////////////////////////////////////////////////////
    //
    // Annotation properties
    //
    ///////////////////////////////////////////////////////////////////////////////////////
     -->


    


    <!-- http://purl.org/dc/elements/1.1/date -->


    <owl:AnnotationProperty rdf:about="http://purl.org/dc/elements/1.1/date"/>
    


    <!-- https://www.theworldavatar.com/kg/ontobuildingstructure/gitCommitHash -->


    <owl:AnnotationProperty rdf:about="https://www.theworldavatar.com/kg/ontobuildingstructure/gitCommitHash"/>
    


    <!-- 
    ///////////////////////////////////////////////////////////////////////////////////////
    //
    // Object Properties
    //
    ///////////////////////////////////////////////////////////////////////////////////////
     -->


    


    <!-- https://www.theworldavatar.com/kg/ontobuildingstructure/comprisesOf -->


    <owl:ObjectProperty rdf:about="https://www.theworldavatar.com/kg/ontobuildingstructure/comprisesOf">
        <rdfs:domain>
            <owl:Class>
                <owl:unionOf rdf:parseType="Collection">
                    <rdf:Description rdf:about="https://www.theworldavatar.com/kg/ontobuildingstructure/RoofFacade"/>
                    <rdf:Description rdf:about="https://www.theworldavatar.com/kg/ontobuildingstructure/WallFacade"/>
                </owl:unionOf>
            </owl:Class>
        </rdfs:domain>
        <rdfs:range>
            <owl:Class>
                <owl:unionOf rdf:parseType="Collection">
                    <rdf:Description rdf:about="https://www.theworldavatar.com/kg/ontobuildingstructure/Roof"/>
                    <rdf:Description rdf:about="https://www.theworldavatar.com/kg/ontobuildingstructure/Wall"/>
                </owl:unionOf>
            </owl:Class>
        </rdfs:range>
        <rdfs:comment>A relation between a facade and its comprising components. Each facade comprises of one or more instances of their coresponding component type, such as a roof or a wall.</rdfs:comment>
        <rdfs:comment>A relation between a facade and its comprising components. Each facade comprises of one or more instances of their corresponding component type, such as a roof or a wall.</rdfs:comment>
        <rdfs:isDefinedBy rdf:resource="https://www.theworldavatar.com/kg/ontobuildingstructure/"/>
        <rdfs:label>comprises of</rdfs:label>
    </owl:ObjectProperty>
    


    <!-- https://www.theworldavatar.com/kg/ontobuildingstructure/consistsOf -->


    <owl:ObjectProperty rdf:about="https://www.theworldavatar.com/kg/ontobuildingstructure/consistsOf">
        <rdf:type rdf:resource="http://www.w3.org/2002/07/owl#AsymmetricProperty"/>
        <rdfs:domain>
            <owl:Class>
                <owl:unionOf rdf:parseType="Collection">
                    <rdf:Description rdf:about="https://www.theworldavatar.com/kg/ontobuildingstructure/Stair"/>
                    <rdf:Description rdf:about="https://www.theworldavatar.com/kg/ontobuildingstructure/Wall"/>
                </owl:unionOf>
            </owl:Class>
        </rdfs:domain>
        <rdfs:range>
            <owl:Class>
                <owl:unionOf rdf:parseType="Collection">
                    <rdf:Description rdf:about="https://www.theworldavatar.com/kg/ontobuildingstructure/Door"/>
                    <rdf:Description rdf:about="https://www.theworldavatar.com/kg/ontobuildingstructure/Landing"/>
                    <rdf:Description rdf:about="https://www.theworldavatar.com/kg/ontobuildingstructure/Railing"/>
                    <rdf:Description rdf:about="https://www.theworldavatar.com/kg/ontobuildingstructure/StairFlight"/>
                    <rdf:Description rdf:about="https://www.theworldavatar.com/kg/ontobuildingstructure/StairStructuralComponent"/>
                    <rdf:Description rdf:about="https://www.theworldavatar.com/kg/ontobuildingstructure/Window"/>
                </owl:unionOf>
            </owl:Class>
        </rdfs:range>
        <rdfs:comment>A relation between a facade and its comprising components. Each facade comprises of one or more instances of their corresponding component type, such as a roof or a wall.</rdfs:comment>
        <rdfs:comment>A relationship that denotes the subcomposition of an assembly with their individual components. An example is that stairs consists of railing, landing, stair flights, and stair structural components.</rdfs:comment>
        <rdfs:isDefinedBy rdf:resource="https://www.theworldavatar.com/kg/ontobuildingstructure/"/>
        <rdfs:label>consists of</rdfs:label>
    </owl:ObjectProperty>
    


    <!-- https://www.theworldavatar.com/kg/ontobuildingstructure/hasArea -->


    <owl:ObjectProperty rdf:about="https://www.theworldavatar.com/kg/ontobuildingstructure/hasArea">
        <rdfs:subPropertyOf rdf:resource="https://www.theworldavatar.com/kg/ontobuildingstructure/hasQuantity"/>
        <rdf:type rdf:resource="http://www.w3.org/2002/07/owl#AsymmetricProperty"/>
        <rdfs:domain rdf:resource="https://www.theworldavatar.com/kg/ontobuildingstructure/Roof"/>
        <rdfs:range rdf:resource="https://www.theworldavatar.com/kg/ontobuildingstructure/RoofArea"/>
        <rdfs:comment>A relationship between the roof of a building and the area it covers.</rdfs:comment>
        <rdfs:isDefinedBy rdf:resource="https://www.theworldavatar.com/kg/ontobuildingstructure/"/>
        <rdfs:label>has area of</rdfs:label>
    </owl:ObjectProperty>
    


    <!-- https://www.theworldavatar.com/kg/ontobuildingstructure/hasFacade -->


    <owl:ObjectProperty rdf:about="https://www.theworldavatar.com/kg/ontobuildingstructure/hasFacade">
        <rdfs:domain rdf:resource="https://w3id.org/bot#Building"/>
        <rdfs:range>
            <owl:Class>
                <owl:unionOf rdf:parseType="Collection">
                    <rdf:Description rdf:about="https://www.theworldavatar.com/kg/ontobuildingstructure/RoofFacade"/>
                    <rdf:Description rdf:about="https://www.theworldavatar.com/kg/ontobuildingstructure/WallFacade"/>
                </owl:unionOf>
            </owl:Class>
        </rdfs:range>
        <rdfs:comment>A relation that links a building to their roof and wall facades.</rdfs:comment>
        <rdfs:isDefinedBy rdf:resource="https://www.theworldavatar.com/kg/ontobuildingstructure/"/>
        <rdfs:label>has facade</rdfs:label>
    </owl:ObjectProperty>
    


    <!-- https://www.theworldavatar.com/kg/ontobuildingstructure/hasOrientation -->


    <owl:ObjectProperty rdf:about="https://www.theworldavatar.com/kg/ontobuildingstructure/hasOrientation">
        <rdfs:subPropertyOf rdf:resource="https://www.theworldavatar.com/kg/ontobuildingstructure/hasQuantity"/>
        <rdf:type rdf:resource="http://www.w3.org/2002/07/owl#AsymmetricProperty"/>
        <rdfs:domain rdf:resource="https://www.theworldavatar.com/kg/ontobuildingstructure/InclinedRoof"/>
        <rdfs:range rdf:resource="http://www.ontology-of-units-of-measure.org/resource/om-2/Angle"/>
        <rdfs:comment>A relationship between a roof and its angle/position relative to the Sun.</rdfs:comment>
        <rdfs:isDefinedBy rdf:resource="https://www.theworldavatar.com/kg/ontobuildingstructure/"/>
        <rdfs:label>has orientation</rdfs:label>
    </owl:ObjectProperty>
    


    <!-- https://www.theworldavatar.com/kg/ontobuildingstructure/hasQuantity -->


    <owl:ObjectProperty rdf:about="https://www.theworldavatar.com/kg/ontobuildingstructure/hasQuantity">
        <rdf:type rdf:resource="http://www.w3.org/2002/07/owl#AsymmetricProperty"/>
        <rdfs:domain rdf:resource="http://www.w3.org/2002/07/owl#Thing"/>
        <rdfs:range rdf:resource="http://www.ontology-of-units-of-measure.org/resource/om-2/Quantity"/>
        <rdfs:comment>Links any entity to a specific quantity defined in the OM ontology. This relationship is not intended to be stated explicitly, but inferred from its sub-properties. For application, only the sub-properties are used.</rdfs:comment>
        <rdfs:isDefinedBy rdf:resource="https://www.theworldavatar.com/kg/ontobuildingstructure/"/>
        <rdfs:label>has quantity</rdfs:label>
    </owl:ObjectProperty>
    


    <!-- https://www.theworldavatar.com/kg/ontobuildingstructure/hasSlope -->


    <owl:ObjectProperty rdf:about="https://www.theworldavatar.com/kg/ontobuildingstructure/hasSlope">
        <rdfs:subPropertyOf rdf:resource="https://www.theworldavatar.com/kg/ontobuildingstructure/hasQuantity"/>
        <rdf:type rdf:resource="http://www.w3.org/2002/07/owl#AsymmetricProperty"/>
        <rdfs:domain rdf:resource="https://www.theworldavatar.com/kg/ontobuildingstructure/InclinedRoof"/>
        <rdfs:range rdf:resource="http://www.ontology-of-units-of-measure.org/resource/om-2/Angle"/>
        <rdfs:comment>A relationship between a roof and its slope angle.</rdfs:comment>
        <rdfs:isDefinedBy rdf:resource="https://www.theworldavatar.com/kg/ontobuildingstructure/"/>
        <rdfs:label>has slope</rdfs:label>
    </owl:ObjectProperty>
    


    <!-- 
    ///////////////////////////////////////////////////////////////////////////////////////
    //
    // Data properties
    //
    ///////////////////////////////////////////////////////////////////////////////////////
     -->


    


    <!-- https://www.theworldavatar.com/kg/ontobuildingstructure/hasNumOfRise -->


    <owl:DatatypeProperty rdf:about="https://www.theworldavatar.com/kg/ontobuildingstructure/hasNumOfRise">
        <rdfs:domain rdf:resource="https://www.theworldavatar.com/kg/ontobuildingstructure/StairFlight"/>
        <rdfs:range rdf:resource="http://www.w3.org/2001/XMLSchema#integer"/>
        <rdfs:comment>Defines the number of risers on a stair flight.</rdfs:comment>
        <rdfs:isDefinedBy rdf:resource="https://www.theworldavatar.com/kg/ontobuildingstructure/"/>
        <rdfs:label>has number of risers</rdfs:label>
    </owl:DatatypeProperty>
    


    <!-- https://www.theworldavatar.com/kg/ontobuildingstructure/hasNumOfTread -->


    <owl:DatatypeProperty rdf:about="https://www.theworldavatar.com/kg/ontobuildingstructure/hasNumOfTread">
        <rdfs:domain rdf:resource="https://www.theworldavatar.com/kg/ontobuildingstructure/StairFlight"/>
        <rdfs:range rdf:resource="http://www.w3.org/2001/XMLSchema#integer"/>
        <rdfs:comment>Defines the number of treads on a stair flight.</rdfs:comment>
        <rdfs:isDefinedBy rdf:resource="https://www.theworldavatar.com/kg/ontobuildingstructure/"/>
        <rdfs:label>has number of treads</rdfs:label>
    </owl:DatatypeProperty>
    


    <!-- https://www.theworldavatar.com/kg/ontobuildingstructure/hasRiserHeight -->


    <owl:DatatypeProperty rdf:about="https://www.theworldavatar.com/kg/ontobuildingstructure/hasRiserHeight">
        <rdfs:domain rdf:resource="https://www.theworldavatar.com/kg/ontobuildingstructure/StairFlight"/>
        <rdfs:range rdf:resource="http://www.w3.org/2001/XMLSchema#double"/>
        <rdfs:comment>Defines the height of each riser on a stair flight.</rdfs:comment>
        <rdfs:isDefinedBy rdf:resource="https://www.theworldavatar.com/kg/ontobuildingstructure/"/>
        <rdfs:label>has riser height</rdfs:label>
    </owl:DatatypeProperty>
    


    <!-- https://www.theworldavatar.com/kg/ontobuildingstructure/hasTreadLength -->


    <owl:DatatypeProperty rdf:about="https://www.theworldavatar.com/kg/ontobuildingstructure/hasTreadLength">
        <rdfs:domain rdf:resource="https://www.theworldavatar.com/kg/ontobuildingstructure/StairFlight"/>
        <rdfs:range rdf:resource="http://www.w3.org/2001/XMLSchema#double"/>
        <rdfs:comment>Defines the length of each tread on a stair flight.</rdfs:comment>
        <rdfs:isDefinedBy rdf:resource="https://www.theworldavatar.com/kg/ontobuildingstructure/"/>
        <rdfs:label>has tread length</rdfs:label>
    </owl:DatatypeProperty>
    


    <!-- https://www.theworldavatar.com/kg/ontobuildingstructure/isHeatSupportSuitable -->


    <owl:DatatypeProperty rdf:about="https://www.theworldavatar.com/kg/ontobuildingstructure/isHeatSupportSuitable">
        <rdfs:domain rdf:resource="https://www.theworldavatar.com/kg/ontobuildingstructure/Roof"/>
        <rdfs:range rdf:resource="http://www.w3.org/2001/XMLSchema#boolean"/>
        <rdfs:comment>A Boolean indicator that is true when the roof is suitable for installation of heat support, and is false, otherwise.</rdfs:comment>
        <rdfs:isDefinedBy rdf:resource="https://www.theworldavatar.com/kg/ontobuildingstructure/"/>
        <rdfs:label>is heat support suitable</rdfs:label>
    </owl:DatatypeProperty>
    


    <!-- https://www.theworldavatar.com/kg/ontobuildingstructure/isPVPanelSuitable -->


    <owl:DatatypeProperty rdf:about="https://www.theworldavatar.com/kg/ontobuildingstructure/isPVPanelSuitable">
        <rdfs:domain rdf:resource="https://www.theworldavatar.com/kg/ontobuildingstructure/Roof"/>
        <rdfs:range rdf:resource="http://www.w3.org/2001/XMLSchema#boolean"/>
        <rdfs:comment>A Boolean indicator that is true when the roof is suitable for installation of photovoltaic panels, and is false, otherwise.</rdfs:comment>
        <rdfs:isDefinedBy rdf:resource="https://www.theworldavatar.com/kg/ontobuildingstructure/"/>
        <rdfs:label>is pv panel suitable</rdfs:label>
    </owl:DatatypeProperty>
    


    <!-- https://www.theworldavatar.com/kg/ontobuildingstructure/isSolarCollectorSuitable -->


    <owl:DatatypeProperty rdf:about="https://www.theworldavatar.com/kg/ontobuildingstructure/isSolarCollectorSuitable">
        <rdfs:domain rdf:resource="https://www.theworldavatar.com/kg/ontobuildingstructure/Roof"/>
        <rdfs:range rdf:resource="http://www.w3.org/2001/XMLSchema#boolean"/>
        <rdfs:comment>A Boolean indicator that is true when the roof is suitable for installation of solar collectors, and is false, otherwise.</rdfs:comment>
        <rdfs:isDefinedBy rdf:resource="https://www.theworldavatar.com/kg/ontobuildingstructure/"/>
        <rdfs:label>is solar collector suitable</rdfs:label>
    </owl:DatatypeProperty>
    


    <!-- 
    ///////////////////////////////////////////////////////////////////////////////////////
    //
    // Classes
    //
    ///////////////////////////////////////////////////////////////////////////////////////
     -->


    


    <!-- http://www.ontology-of-units-of-measure.org/resource/om-2/Angle -->


    <owl:Class rdf:about="http://www.ontology-of-units-of-measure.org/resource/om-2/Angle"/>
    


    <!-- http://www.ontology-of-units-of-measure.org/resource/om-2/Area -->


    <owl:Class rdf:about="http://www.ontology-of-units-of-measure.org/resource/om-2/Area"/>
    


    <!-- http://www.ontology-of-units-of-measure.org/resource/om-2/Quantity -->


    <owl:Class rdf:about="http://www.ontology-of-units-of-measure.org/resource/om-2/Quantity"/>
    


    <!-- https://w3id.org/bot#Building -->


    <owl:Class rdf:about="https://w3id.org/bot#Building"/>
    


    <!-- https://w3id.org/bot#Element -->


    <owl:Class rdf:about="https://w3id.org/bot#Element"/>
    


    <!-- https://www.theworldavatar.com/kg/ontobuildingstructure/Assembly -->


    <owl:Class rdf:about="https://www.theworldavatar.com/kg/ontobuildingstructure/Assembly">
        <rdfs:subClassOf rdf:resource="https://www.theworldavatar.com/kg/ontobuildingstructure/BuildingStructureComponent"/>
        <rdfs:comment>A building structure component that is composed of at least two other components, including assemblies. For example, a wall is an assembly that can consist of a door or window.</rdfs:comment>
        <rdfs:isDefinedBy rdf:resource="https://www.theworldavatar.com/kg/ontobuildingstructure/"/>
        <rdfs:label>Assembly</rdfs:label>
    </owl:Class>
    


    <!-- https://www.theworldavatar.com/kg/ontobuildingstructure/BuildingStructureComponent -->


    <owl:Class rdf:about="https://www.theworldavatar.com/kg/ontobuildingstructure/BuildingStructureComponent">
        <rdfs:subClassOf rdf:resource="https://w3id.org/bot#Element"/>
        <rdfs:comment>An abstract class defining the attached construction parts of a building that constitute the building, such as walls, built-in partitions, roofs, doors, and columns. Generally, the building and all of its structural components are treated as a whole when the building is acquired, constructed, reconstructed, or erected and first placed in service.</rdfs:comment>
        <rdfs:isDefinedBy rdf:resource="https://www.theworldavatar.com/kg/ontobuildingstructure/"/>
        <rdfs:label>Building Structure Component </rdfs:label>
    </owl:Class>
    


    <!-- https://www.theworldavatar.com/kg/ontobuildingstructure/Ceiling -->


    <owl:Class rdf:about="https://www.theworldavatar.com/kg/ontobuildingstructure/Ceiling">
        <rdfs:subClassOf rdf:resource="https://www.theworldavatar.com/kg/ontobuildingstructure/BuildingStructureComponent"/>
        <rdfs:comment>Upper interior surface component of any space in a construction, building, or infrastructure.</rdfs:comment>
        <rdfs:isDefinedBy rdf:resource="https://www.theworldavatar.com/kg/ontobuildingstructure/"/>
        <rdfs:label>Ceiling</rdfs:label>
    </owl:Class>
    


    <!-- https://www.theworldavatar.com/kg/ontobuildingstructure/Column -->


    <owl:Class rdf:about="https://www.theworldavatar.com/kg/ontobuildingstructure/Column">
        <rdfs:subClassOf rdf:resource="https://www.theworldavatar.com/kg/ontobuildingstructure/BuildingStructureComponent"/>
        <rdfs:comment>A vertical load-bearing structural member that is designed to support and transmit the load of the slab on the higher floors to the foundation through compression.</rdfs:comment>
        <rdfs:isDefinedBy rdf:resource="https://www.theworldavatar.com/kg/ontobuildingstructure/"/>
        <rdfs:label>Column</rdfs:label>
    </owl:Class>
    


    <!-- https://www.theworldavatar.com/kg/ontobuildingstructure/Door -->


    <owl:Class rdf:about="https://www.theworldavatar.com/kg/ontobuildingstructure/Door">
        <rdfs:subClassOf rdf:resource="https://www.theworldavatar.com/kg/ontobuildingstructure/BuildingStructureComponent"/>
        <rdfs:comment>Construction for closing an opening, intended primarily for access with hinged, pivoted or sliding operation.</rdfs:comment>
        <rdfs:isDefinedBy rdf:resource="https://www.theworldavatar.com/kg/ontobuildingstructure/"/>
        <rdfs:label>Door</rdfs:label>
    </owl:Class>
    


    <!-- https://www.theworldavatar.com/kg/ontobuildingstructure/EastWallFacade -->


    <owl:Class rdf:about="https://www.theworldavatar.com/kg/ontobuildingstructure/EastWallFacade">
        <rdfs:subClassOf rdf:resource="https://www.theworldavatar.com/kg/ontobuildingstructure/WallFacade"/>
        <rdfs:comment>The easthern frontage  of a building. It can comprise of several walls.</rdfs:comment>
        <rdfs:isDefinedBy rdf:resource="https://www.theworldavatar.com/kg/ontobuildingstructure/"/>
        <rdfs:label>East Wall Facade</rdfs:label>
    </owl:Class>
    


    <!-- https://www.theworldavatar.com/kg/ontobuildingstructure/FlatRoof -->


    <owl:Class rdf:about="https://www.theworldavatar.com/kg/ontobuildingstructure/FlatRoof">
        <rdfs:subClassOf rdf:resource="https://www.theworldavatar.com/kg/ontobuildingstructure/Roof"/>
        <rdfs:comment>Roof with a slope angle that is less than 9.46 degree.</rdfs:comment>
        <rdfs:isDefinedBy rdf:resource="https://www.theworldavatar.com/kg/ontobuildingstructure/"/>
        <rdfs:label>Flat Roof</rdfs:label>
    </owl:Class>
    


    <!-- https://www.theworldavatar.com/kg/ontobuildingstructure/Floor -->


    <owl:Class rdf:about="https://www.theworldavatar.com/kg/ontobuildingstructure/Floor">
        <rdfs:subClassOf rdf:resource="https://www.theworldavatar.com/kg/ontobuildingstructure/BuildingStructureComponent"/>
        <rdfs:comment>Lower support component of any space in a construction, building, or infrastructure. It include a slab and flooring finish.</rdfs:comment>
        <rdfs:isDefinedBy rdf:resource="https://www.theworldavatar.com/kg/ontobuildingstructure/"/>
        <rdfs:label>Floor</rdfs:label>
    </owl:Class>
    


    <!-- https://www.theworldavatar.com/kg/ontobuildingstructure/InclinedRoof -->


    <owl:Class rdf:about="https://www.theworldavatar.com/kg/ontobuildingstructure/InclinedRoof">
        <rdfs:subClassOf rdf:resource="https://www.theworldavatar.com/kg/ontobuildingstructure/Roof"/>
        <rdfs:comment>Roof with a slope angle that is greater than or equal to 9.46 degree.</rdfs:comment>
        <rdfs:isDefinedBy rdf:resource="https://www.theworldavatar.com/kg/ontobuildingstructure/"/>
        <rdfs:label>Inclined Roof</rdfs:label>
    </owl:Class>
    


    <!-- https://www.theworldavatar.com/kg/ontobuildingstructure/Landing -->


    <owl:Class rdf:about="https://www.theworldavatar.com/kg/ontobuildingstructure/Landing">
        <rdfs:subClassOf rdf:resource="https://www.theworldavatar.com/kg/ontobuildingstructure/BuildingStructureComponent"/>
        <rdfs:comment>A floor section that is connected to one or more stair flights or ramp flights.</rdfs:comment>
        <rdfs:isDefinedBy rdf:resource="https://www.theworldavatar.com/kg/ontobuildingstructure/"/>
        <rdfs:label>Landing</rdfs:label>
    </owl:Class>
    


    <!-- https://www.theworldavatar.com/kg/ontobuildingstructure/NorthWallFacade -->


    <owl:Class rdf:about="https://www.theworldavatar.com/kg/ontobuildingstructure/NorthWallFacade">
        <rdfs:subClassOf rdf:resource="https://www.theworldavatar.com/kg/ontobuildingstructure/WallFacade"/>
        <rdfs:comment>The northern frontage  of a building. It can comprise of several walls.</rdfs:comment>
        <rdfs:isDefinedBy rdf:resource="https://www.theworldavatar.com/kg/ontobuildingstructure/"/>
        <rdfs:label>North Wall Facade</rdfs:label>
    </owl:Class>
    


    <!-- https://www.theworldavatar.com/kg/ontobuildingstructure/Railing -->


    <owl:Class rdf:about="https://www.theworldavatar.com/kg/ontobuildingstructure/Railing">
        <rdfs:subClassOf rdf:resource="https://www.theworldavatar.com/kg/ontobuildingstructure/BuildingStructureComponent"/>
        <rdfs:comment>A frame assembly that is adjacent to human circulation spaces and at some space boundaries, in which it is used in lieu of walls or to complement walls. It is usually designed to aid humans, either as an optional physical support, or to prevent injury by falling.</rdfs:comment>
        <rdfs:isDefinedBy rdf:resource="https://www.theworldavatar.com/kg/ontobuildingstructure/"/>
        <rdfs:label>Railing</rdfs:label>
    </owl:Class>
    


    <!-- https://www.theworldavatar.com/kg/ontobuildingstructure/Roof -->


    <owl:Class rdf:about="https://www.theworldavatar.com/kg/ontobuildingstructure/Roof">
        <rdfs:subClassOf rdf:resource="https://www.theworldavatar.com/kg/ontobuildingstructure/BuildingStructureComponent"/>
        <rdfs:comment>Construction enclosing the building from above.</rdfs:comment>
        <rdfs:isDefinedBy rdf:resource="https://www.theworldavatar.com/kg/ontobuildingstructure/"/>
        <rdfs:label>Roof</rdfs:label>
    </owl:Class>
    


    <!-- https://www.theworldavatar.com/kg/ontobuildingstructure/RoofArea -->


    <owl:Class rdf:about="https://www.theworldavatar.com/kg/ontobuildingstructure/RoofArea">
        <rdfs:subClassOf rdf:resource="http://www.ontology-of-units-of-measure.org/resource/om-2/Area"/>
        <rdfs:comment>The size of the roof on a building</rdfs:comment>
        <rdfs:isDefinedBy rdf:resource="https://www.theworldavatar.com/kg/ontobuildingstructure/"/>
        <rdfs:label>Roof Area</rdfs:label>
    </owl:Class>
    


    <!-- https://www.theworldavatar.com/kg/ontobuildingstructure/RoofFacade -->


    <owl:Class rdf:about="https://www.theworldavatar.com/kg/ontobuildingstructure/RoofFacade">
        <rdfs:subClassOf>
            <owl:Restriction>
                <owl:onProperty rdf:resource="https://www.theworldavatar.com/kg/ontobuildingstructure/comprisesOf"/>
                <owl:allValuesFrom rdf:resource="https://www.theworldavatar.com/kg/ontobuildingstructure/Roof"/>
            </owl:Restriction>
        </rdfs:subClassOf>
        <rdfs:comment>The visible surface of a building&apos;s roof at aerial view. It can comprise of several roofs.</rdfs:comment>
        <rdfs:isDefinedBy rdf:resource="https://www.theworldavatar.com/kg/ontobuildingstructure/"/>
        <rdfs:label>Roof Facade</rdfs:label>
    </owl:Class>
    


    <!-- https://www.theworldavatar.com/kg/ontobuildingstructure/SolarSuitableRoofArea -->


    <owl:Class rdf:about="https://www.theworldavatar.com/kg/ontobuildingstructure/SolarSuitableRoofArea">
        <rdfs:subClassOf rdf:resource="https://www.theworldavatar.com/kg/ontobuildingstructure/RoofArea"/>
        <rdfs:comment>The size of the roof area of a building that is suitable for solar use.</rdfs:comment>
        <rdfs:isDefinedBy rdf:resource="https://www.theworldavatar.com/kg/ontobuildingstructure/"/>
        <rdfs:label>Solar Suitable Roof Area</rdfs:label>
    </owl:Class>
    


    <!-- https://www.theworldavatar.com/kg/ontobuildingstructure/SouthWallFacade -->


    <owl:Class rdf:about="https://www.theworldavatar.com/kg/ontobuildingstructure/SouthWallFacade">
        <rdfs:subClassOf rdf:resource="https://www.theworldavatar.com/kg/ontobuildingstructure/WallFacade"/>
        <rdfs:comment>The southern frontage  of a building. It can comprise of several walls.</rdfs:comment>
        <rdfs:isDefinedBy rdf:resource="https://www.theworldavatar.com/kg/ontobuildingstructure/"/>
        <rdfs:label>South Wall Facade</rdfs:label>
    </owl:Class>
    


    <!-- https://www.theworldavatar.com/kg/ontobuildingstructure/Stair -->


    <owl:Class rdf:about="https://www.theworldavatar.com/kg/ontobuildingstructure/Stair">
        <rdfs:subClassOf rdf:resource="https://www.theworldavatar.com/kg/ontobuildingstructure/Assembly"/>
        <rdfs:subClassOf>
            <owl:Restriction>
                <owl:onProperty rdf:resource="https://www.theworldavatar.com/kg/ontobuildingstructure/consistsOf"/>
                <owl:allValuesFrom>
                    <owl:Class>
                        <owl:unionOf rdf:parseType="Collection">
                            <rdf:Description rdf:about="https://www.theworldavatar.com/kg/ontobuildingstructure/Landing"/>
                            <rdf:Description rdf:about="https://www.theworldavatar.com/kg/ontobuildingstructure/Railing"/>
                            <rdf:Description rdf:about="https://www.theworldavatar.com/kg/ontobuildingstructure/StairFlight"/>
                            <rdf:Description rdf:about="https://www.theworldavatar.com/kg/ontobuildingstructure/StairStructuralComponent"/>
                        </owl:unionOf>
                    </owl:Class>
                </owl:allValuesFrom>
            </owl:Restriction>
        </rdfs:subClassOf>
        <rdfs:comment>Construction comprising a succession of horizontal stages (steps or landings) that make it possible to pass on foot to other levels. It can be treater as an assembly consisting of the following types: stair flights, railings, landings, and stair structural components.</rdfs:comment>
        <rdfs:isDefinedBy rdf:resource="https://www.theworldavatar.com/kg/ontobuildingstructure/"/>
        <rdfs:label>Stair</rdfs:label>
    </owl:Class>
    


    <!-- https://www.theworldavatar.com/kg/ontobuildingstructure/StairFlight -->


    <owl:Class rdf:about="https://www.theworldavatar.com/kg/ontobuildingstructure/StairFlight">
        <rdfs:subClassOf rdf:resource="https://www.theworldavatar.com/kg/ontobuildingstructure/BuildingStructureComponent"/>
        <rdfs:comment>An assembly of building components in a single &amp;quot;run&amp;quot; of stair steps that are not interrupted by a landing.</rdfs:comment>
        <rdfs:isDefinedBy rdf:resource="https://www.theworldavatar.com/kg/ontobuildingstructure/"/>
        <rdfs:label>Stair Flight</rdfs:label>
    </owl:Class>
    


    <!-- https://www.theworldavatar.com/kg/ontobuildingstructure/StairStructuralComponent -->


    <owl:Class rdf:about="https://www.theworldavatar.com/kg/ontobuildingstructure/StairStructuralComponent">
        <rdfs:subClassOf rdf:resource="https://www.theworldavatar.com/kg/ontobuildingstructure/BuildingStructureComponent"/>
        <rdfs:comment>A structural member designed to carry loads between or beyond points of support for a staircase.</rdfs:comment>
        <rdfs:isDefinedBy rdf:resource="https://www.theworldavatar.com/kg/ontobuildingstructure/"/>
        <rdfs:label>Stair Structural Component </rdfs:label>
    </owl:Class>
    


    <!-- https://www.theworldavatar.com/kg/ontobuildingstructure/TotalRoofArea -->


    <owl:Class rdf:about="https://www.theworldavatar.com/kg/ontobuildingstructure/TotalRoofArea">
        <rdfs:subClassOf rdf:resource="https://www.theworldavatar.com/kg/ontobuildingstructure/RoofArea"/>
        <rdfs:comment>The total size of the roof of a building.</rdfs:comment>
        <rdfs:isDefinedBy rdf:resource="https://www.theworldavatar.com/kg/ontobuildingstructure/"/>
        <rdfs:label>Total Roof Area </rdfs:label>
    </owl:Class>
    


    <!-- https://www.theworldavatar.com/kg/ontobuildingstructure/Wall -->


    <owl:Class rdf:about="https://www.theworldavatar.com/kg/ontobuildingstructure/Wall">
        <rdfs:subClassOf rdf:resource="https://www.theworldavatar.com/kg/ontobuildingstructure/Assembly"/>
        <rdfs:subClassOf>
            <owl:Restriction>
                <owl:onProperty rdf:resource="https://www.theworldavatar.com/kg/ontobuildingstructure/consistsOf"/>
                <owl:allValuesFrom>
                    <owl:Class>
                        <owl:unionOf rdf:parseType="Collection">
                            <rdf:Description rdf:about="https://www.theworldavatar.com/kg/ontobuildingstructure/Door"/>
                            <rdf:Description rdf:about="https://www.theworldavatar.com/kg/ontobuildingstructure/Window"/>
                        </owl:unionOf>
                    </owl:Class>
                </owl:allValuesFrom>
            </owl:Restriction>
        </rdfs:subClassOf>
        <rdfs:comment>Vertical construction usually in masonry or in concrete which bounds or subdivides a construction works and fulfills a load bearing or retaining function. It is also an assembly that can host doors and windows.</rdfs:comment>
        <rdfs:isDefinedBy rdf:resource="https://www.theworldavatar.com/kg/ontobuildingstructure/"/>
        <rdfs:label>Wall</rdfs:label>
    </owl:Class>
    


    <!-- https://www.theworldavatar.com/kg/ontobuildingstructure/WallFacade -->


    <owl:Class rdf:about="https://www.theworldavatar.com/kg/ontobuildingstructure/WallFacade">
        <rdfs:subClassOf>
            <owl:Restriction>
                <owl:onProperty rdf:resource="https://www.theworldavatar.com/kg/ontobuildingstructure/comprisesOf"/>
                <owl:allValuesFrom rdf:resource="https://www.theworldavatar.com/kg/ontobuildingstructure/Wall"/>
            </owl:Restriction>
        </rdfs:subClassOf>
        <rdfs:comment>The frontage  of a building. It can comprise of several walls.</rdfs:comment>
        <rdfs:isDefinedBy rdf:resource="https://www.theworldavatar.com/kg/ontobuildingstructure/"/>
        <rdfs:label>Wall Facade</rdfs:label>
    </owl:Class>
    


    <!-- https://www.theworldavatar.com/kg/ontobuildingstructure/WestWallFacade -->


    <owl:Class rdf:about="https://www.theworldavatar.com/kg/ontobuildingstructure/WestWallFacade">
        <rdfs:subClassOf rdf:resource="https://www.theworldavatar.com/kg/ontobuildingstructure/WallFacade"/>
        <rdfs:comment>The westhern frontage  of a building. It can comprise of several walls.</rdfs:comment>
        <rdfs:isDefinedBy rdf:resource="https://www.theworldavatar.com/kg/ontobuildingstructure/"/>
        <rdfs:label>West Wall Facade</rdfs:label>
    </owl:Class>
    


    <!-- https://www.theworldavatar.com/kg/ontobuildingstructure/Window -->


    <owl:Class rdf:about="https://www.theworldavatar.com/kg/ontobuildingstructure/Window">
        <rdfs:subClassOf rdf:resource="https://www.theworldavatar.com/kg/ontobuildingstructure/BuildingStructureComponent"/>
        <rdfs:comment>Construction for closing a vertical or near vertical opening in a wall or pitched roof that will admit light and may admit fresh air.</rdfs:comment>
        <rdfs:isDefinedBy rdf:resource="https://www.theworldavatar.com/kg/ontobuildingstructure/"/>
        <rdfs:label>Window</rdfs:label>
    </owl:Class>
</rdf:RDF>



<!-- Generated by the OWL API (version 5.5.0.2023-01-14T12:41:38Z) https://github.com/owlcs/owlapi/ -->


