<?xml version="1.0"?>
<rdf:RDF xmlns="https://www.theworldavatar.com/kg/ontobms/"
     xml:base="https://www.theworldavatar.com/kg/ontobms/"
     xmlns:dc="http://purl.org/dc/elements/1.1/"
     xmlns:owl="http://www.w3.org/2002/07/owl#"
     xmlns:rdf="http://www.w3.org/1999/02/22-rdf-syntax-ns#"
     xmlns:xml="http://www.w3.org/XML/1998/namespace"
     xmlns:xsd="http://www.w3.org/2001/XMLSchema#"
     xmlns:rdfs="http://www.w3.org/2000/01/rdf-schema#"
     xmlns:ontobms="https://www.theworldavatar.com/kg/ontobms/">
    <owl:Ontology rdf:about="https://www.theworldavatar.com/kg/ontobms/">
        <owl:imports rdf:resource="https://saref.etsi.org/saref4bldg/v1.1.2/saref4bldg.rdf"/>
        <dc:date>28 May 2024</dc:date>
        <rdfs:comment>OntoBMS is an ontology for Building Management Systems.</rdfs:comment>
        <owl:versionInfo>1.5</owl:versionInfo>
        <gitCommitHash>c0599beca8df55873a1ab061dee64e52c510c6a0</gitCommitHash>
    </owl:Ontology>
    


    <!-- 
    ///////////////////////////////////////////////////////////////////////////////////////
    //
    // Annotation properties
    //
    ///////////////////////////////////////////////////////////////////////////////////////
     -->


    


    <!-- http://purl.org/dc/elements/1.1/date -->


    <owl:AnnotationProperty rdf:about="http://purl.org/dc/elements/1.1/date"/>
    


    <!-- https://www.theworldavatar.com/kg/ontobms/gitCommitHash -->


    <owl:AnnotationProperty rdf:about="https://www.theworldavatar.com/kg/ontobms/gitCommitHash"/>
    


    <!-- 
    ///////////////////////////////////////////////////////////////////////////////////////
    //
    // Object Properties
    //
    ///////////////////////////////////////////////////////////////////////////////////////
     -->


    


    <!-- https://www.theworldavatar.com/kg/ontobms/conveys -->


    <owl:ObjectProperty rdf:about="https://www.theworldavatar.com/kg/ontobms/conveys">
        <rdfs:domain rdf:resource="https://saref.etsi.org/saref4bldg/FlowMovingDevice"/>
        <rdfs:range rdf:resource="http://www.theworldavatar.com/ontology/ontocape/material/substance/substance.owl#Substance"/>
        <rdfs:comment>A relationship that describes the sustance being conveyed by a flow moving device (e.g. duct).</rdfs:comment>
        <rdfs:isDefinedBy rdf:resource="https://www.theworldavatar.com/kg/ontobms/"/>
        <rdfs:label>conveys</rdfs:label>
    </owl:ObjectProperty>
    


    <!-- https://www.theworldavatar.com/kg/ontobms/extractsAirFrom -->


    <owl:ObjectProperty rdf:about="https://www.theworldavatar.com/kg/ontobms/extractsAirFrom">
        <rdfs:domain rdf:resource="https://saref.etsi.org/core/HVAC"/>
        <rdfs:range>
            <owl:Class>
                <owl:unionOf rdf:parseType="Collection">
                    <rdf:Description rdf:about="https://saref.etsi.org/saref4bldg/FlowMovingDevice"/>
                    <rdf:Description rdf:about="https://saref.etsi.org/saref4bldg/FlowTreatmentDevice"/>
                </owl:unionOf>
            </owl:Class>
        </rdfs:range>
        <rdfs:comment>A relationship that describes a HVAC device removing air from a flow moving device or a flow treatment device.</rdfs:comment>
        <rdfs:isDefinedBy rdf:resource="https://www.theworldavatar.com/kg/ontobms/"/>
        <rdfs:label>extracts air from</rdfs:label>
    </owl:ObjectProperty>
    


    <!-- https://www.theworldavatar.com/kg/ontobms/hasAirExchangeRate -->


    <owl:ObjectProperty rdf:about="https://www.theworldavatar.com/kg/ontobms/hasAirExchangeRate">
        <rdfs:subPropertyOf rdf:resource="https://www.theworldavatar.com/kg/ontodevice/hasQuantity"/>
        <rdfs:domain rdf:resource="https://w3id.org/bot#Zone"/>
        <rdfs:range rdf:resource="https://www.theworldavatar.com/kg/ontobms/AirChangePerHour"/>
        <rdfs:comment>A relationship that describes how many times the air within a defined space (usually a room or building) is replaced with fresh air in one hour.</rdfs:comment>
        <rdfs:isDefinedBy rdf:resource="https://www.theworldavatar.com/kg/ontobms/"/>
        <rdfs:label>has air exchange rate</rdfs:label>
    </owl:ObjectProperty>
    


    <!-- https://www.theworldavatar.com/kg/ontobms/hasAirFlowRate -->


    <owl:ObjectProperty rdf:about="https://www.theworldavatar.com/kg/ontobms/hasAirFlowRate">
        <rdfs:subPropertyOf rdf:resource="https://www.theworldavatar.com/kg/ontobms/hasFlowRate"/>
        <rdfs:domain>
            <owl:Class>
                <owl:unionOf rdf:parseType="Collection">
                    <rdf:Description rdf:about="http://www.theworldavatar.com/ontology/ontocape/chemical_process_system/CPS_behavior/behavior.owl#ConvectiveTransportRate"/>
                    <rdf:Description rdf:about="https://saref.etsi.org/core/HVAC"/>
                    <rdf:Description rdf:about="https://saref.etsi.org/saref4bldg/FlowMovingDevice"/>
                </owl:unionOf>
            </owl:Class>
        </rdfs:domain>
        <rdfs:range rdf:resource="http://www.ontology-of-units-of-measure.org/resource/om-2/VolumetricFlowRate"/>
        <rdfs:comment>A relationship that describes the flow rate of air being conveyed or processed by a HVAC or Flow Moving Device (Duct etc) or it can be used to describe the volumetric air flow rate of a convective transport rate.</rdfs:comment>
        <rdfs:isDefinedBy rdf:resource="https://www.theworldavatar.com/kg/ontobms/"/>
        <rdfs:label>has air flow rate</rdfs:label>
    </owl:ObjectProperty>
    


    <!-- https://www.theworldavatar.com/kg/ontobms/hasFlowRate -->


    <owl:ObjectProperty rdf:about="https://www.theworldavatar.com/kg/ontobms/hasFlowRate">
        <rdfs:subPropertyOf rdf:resource="https://www.theworldavatar.com/kg/ontodevice/hasQuantity"/>
        <rdfs:domain>
            <owl:Class>
                <owl:unionOf rdf:parseType="Collection">
                    <rdf:Description rdf:about="http://www.theworldavatar.com/ontology/ontocape/chemical_process_system/CPS_behavior/behavior.owl#ConvectiveTransportRate"/>
                    <rdf:Description rdf:about="https://saref.etsi.org/core/HVAC"/>
                    <rdf:Description rdf:about="https://saref.etsi.org/saref4bldg/FlowMovingDevice"/>
                </owl:unionOf>
            </owl:Class>
        </rdfs:domain>
        <rdfs:range rdf:resource="http://www.ontology-of-units-of-measure.org/resource/om-2/VolumetricFlowRate"/>
        <rdfs:comment>A relationship that describes the flow rate of a substance being conveyed or processed by a HVAC or Flow Moving Device (Duct etc) or it can be used to describe the volumetric flow rate of a convective transport rate.</rdfs:comment>
        <rdfs:isDefinedBy rdf:resource="https://www.theworldavatar.com/kg/ontobms/"/>
        <rdfs:label>has flow rate</rdfs:label>
    </owl:ObjectProperty>
    


    <!-- https://www.theworldavatar.com/kg/ontobms/hasHeatDuty -->


    <owl:ObjectProperty rdf:about="https://www.theworldavatar.com/kg/ontobms/hasHeatDuty">
        <rdfs:subPropertyOf rdf:resource="https://www.theworldavatar.com/kg/ontodevice/hasQuantity"/>
        <rdfs:domain rdf:resource="http://www.theworldavatar.com/ontology/ontocape/chemical_process_system/CPS_function/process.owl#TemperatureChange"/>
        <rdfs:range rdf:resource="https://www.theworldavatar.com/kg/ontobms/HeatDuty"/>
        <rdfs:comment>A relationship that describes the heat duty involved in a temperature change process.</rdfs:comment>
        <rdfs:isDefinedBy rdf:resource="https://www.theworldavatar.com/kg/ontobms/"/>
        <rdfs:label>has heat duty</rdfs:label>
    </owl:ObjectProperty>
    


    <!-- https://www.theworldavatar.com/kg/ontobms/hasHighLevelState -->


    <owl:ObjectProperty rdf:about="https://www.theworldavatar.com/kg/ontobms/hasHighLevelState">
        <rdfs:domain rdf:resource="https://saref.etsi.org/core/MultiLevelState"/>
        <rdfs:range rdf:resource="https://www.theworldavatar.com/kg/ontobms/HighLevelState"/>
        <rdfs:comment>A relationship that describes a high level state of a multi-level state.</rdfs:comment>
        <rdfs:isDefinedBy rdf:resource="https://www.theworldavatar.com/kg/ontobms/"/>
        <rdfs:label>has high level state</rdfs:label>
    </owl:ObjectProperty>
    


    <!-- https://www.theworldavatar.com/kg/ontobms/hasInput -->


    <owl:ObjectProperty rdf:about="https://www.theworldavatar.com/kg/ontobms/hasInput">
        <rdfs:domain rdf:resource="https://saref.etsi.org/saref4bldg/FlowMovingDevice"/>
        <rdfs:range rdf:resource="http://www.theworldavatar.com/ontology/ontocape/upper_level/network_system.owl#DirectedConnection"/>
        <rdfs:comment>A relationship describing a flow moving device (e.g. duct) having a directed connection (e.g. streamline) as an input.</rdfs:comment>
        <rdfs:isDefinedBy rdf:resource="https://www.theworldavatar.com/kg/ontobms/"/>
        <rdfs:label>has input</rdfs:label>
    </owl:ObjectProperty>
    


    <!-- https://www.theworldavatar.com/kg/ontobms/hasLowLevelState -->


    <owl:ObjectProperty rdf:about="https://www.theworldavatar.com/kg/ontobms/hasLowLevelState">
        <rdfs:domain rdf:resource="https://saref.etsi.org/core/MultiLevelState"/>
        <rdfs:range rdf:resource="https://www.theworldavatar.com/kg/ontobms/LowLevelState"/>
        <rdfs:comment>A relationship that describes a low level state of a multi-level state.</rdfs:comment>
        <rdfs:isDefinedBy rdf:resource="https://www.theworldavatar.com/kg/ontobms/"/>
        <rdfs:label>has low level state</rdfs:label>
    </owl:ObjectProperty>
    


    <!-- https://www.theworldavatar.com/kg/ontobms/hasMediumLevelState -->


    <owl:ObjectProperty rdf:about="https://www.theworldavatar.com/kg/ontobms/hasMediumLevelState">
        <rdfs:domain rdf:resource="https://saref.etsi.org/core/MultiLevelState"/>
        <rdfs:range rdf:resource="https://www.theworldavatar.com/kg/ontobms/MediumLevelState"/>
        <rdfs:comment>A relationship that describes a medium level state of a multi-level state.</rdfs:comment>
        <rdfs:isDefinedBy rdf:resource="https://www.theworldavatar.com/kg/ontobms/"/>
        <rdfs:label>has medium level state</rdfs:label>
    </owl:ObjectProperty>
    


    <!-- https://www.theworldavatar.com/kg/ontobms/hasOpening -->


    <owl:ObjectProperty rdf:about="https://www.theworldavatar.com/kg/ontobms/hasOpening">
        <rdfs:domain rdf:resource="https://www.theworldavatar.com/kg/ontobms/ExtractionArm"/>
        <rdfs:range rdf:resource="http://www.ontology-of-units-of-measure.org/resource/om-2/Percentage"/>
        <rdfs:comment>A relationship that describes the opening of an extraction arm in percentage.</rdfs:comment>
        <rdfs:isDefinedBy rdf:resource="https://www.theworldavatar.com/kg/ontobms/"/>
        <rdfs:label>has opening</rdfs:label>
    </owl:ObjectProperty>
    


    <!-- https://www.theworldavatar.com/kg/ontobms/hasOutput -->


    <owl:ObjectProperty rdf:about="https://www.theworldavatar.com/kg/ontobms/hasOutput">
        <rdfs:domain rdf:resource="https://saref.etsi.org/saref4bldg/FlowMovingDevice"/>
        <rdfs:range rdf:resource="http://www.theworldavatar.com/ontology/ontocape/upper_level/network_system.owl#DirectedConnection"/>
        <rdfs:comment>A relationship describing a flow moving device (e.g. duct) having a directed connection (e.g. streamline) as an output.</rdfs:comment>
        <rdfs:isDefinedBy rdf:resource="https://www.theworldavatar.com/kg/ontobms/"/>
        <rdfs:label>has output</rdfs:label>
    </owl:ObjectProperty>
    


    <!-- https://www.theworldavatar.com/kg/ontobms/hasSashOpenPercentage -->


    <owl:ObjectProperty rdf:about="https://www.theworldavatar.com/kg/ontobms/hasSashOpenPercentage">
        <rdfs:subPropertyOf rdf:resource="https://www.theworldavatar.com/kg/ontodevice/hasQuantity"/>
        <rdfs:domain rdf:resource="https://www.theworldavatar.com/kg/ontobms/FumeHood"/>
        <rdfs:range rdf:resource="http://www.ontology-of-units-of-measure.org/resource/om-2/Percentage"/>
        <rdfs:comment>A relationship to describe the sash opening of a fumehood as a percentage.</rdfs:comment>
        <rdfs:isDefinedBy rdf:resource="https://www.theworldavatar.com/kg/ontobms/"/>
        <rdfs:label>has sash open percentage</rdfs:label>
    </owl:ObjectProperty>
    


    <!-- https://www.theworldavatar.com/kg/ontobms/hasWaterFlowRate -->


    <owl:ObjectProperty rdf:about="https://www.theworldavatar.com/kg/ontobms/hasWaterFlowRate">
        <rdfs:subPropertyOf rdf:resource="https://www.theworldavatar.com/kg/ontobms/hasFlowRate"/>
        <rdfs:domain>
            <owl:Class>
                <owl:unionOf rdf:parseType="Collection">
                    <rdf:Description rdf:about="http://www.theworldavatar.com/ontology/ontocape/chemical_process_system/CPS_behavior/behavior.owl#ConvectiveTransportRate"/>
                    <rdf:Description rdf:about="https://saref.etsi.org/core/HVAC"/>
                    <rdf:Description rdf:about="https://saref.etsi.org/saref4bldg/FlowMovingDevice"/>
                </owl:unionOf>
            </owl:Class>
        </rdfs:domain>
        <rdfs:range rdf:resource="http://www.ontology-of-units-of-measure.org/resource/om-2/VolumetricFlowRate"/>
        <rdfs:comment>A relationship that describes the flow rate of water being conveyed or processed by a HVAC or Flow Moving Device (Pipe etc) or it can be used to describe the volumetric water flow rate of a convective transport rate.</rdfs:comment>
        <rdfs:isDefinedBy rdf:resource="https://www.theworldavatar.com/kg/ontobms/"/>
        <rdfs:label>has water flow rate</rdfs:label>
    </owl:ObjectProperty>
    


    <!-- https://www.theworldavatar.com/kg/ontobms/isComposedOf -->


    <owl:ObjectProperty rdf:about="https://www.theworldavatar.com/kg/ontobms/isComposedOf">
        <rdfs:domain rdf:resource="https://www.theworldavatar.com/kg/ontobms/HeatDuty"/>
        <rdfs:range rdf:resource="https://www.theworldavatar.com/kg/ontobms/HeatDuty"/>
        <rdfs:comment>A relationship that describes a heat duty being comprised of other heat duties.</rdfs:comment>
        <rdfs:isDefinedBy rdf:resource="https://www.theworldavatar.com/kg/ontobms/"/>
        <rdfs:label>is composed of</rdfs:label>
    </owl:ObjectProperty>
    


    <!-- https://www.theworldavatar.com/kg/ontobms/realizes -->


    <owl:ObjectProperty rdf:about="https://www.theworldavatar.com/kg/ontobms/realizes">
        <rdfs:domain rdf:resource="https://www.theworldavatar.com/kg/ontodevice/Device"/>
        <rdfs:range rdf:resource="http://www.theworldavatar.com/ontology/ontocape/chemical_process_system/CPS_function/process.owl#UnitOperation"/>
        <rdfs:comment>A relationship that describes a device fulfilling an unit operation (Mixing, Separation etc).</rdfs:comment>
        <rdfs:isDefinedBy rdf:resource="https://www.theworldavatar.com/kg/ontobms/"/>
        <rdfs:label>realizes</rdfs:label>
    </owl:ObjectProperty>
    


    <!-- https://www.theworldavatar.com/kg/ontobms/suppliesAirTo -->


    <owl:ObjectProperty rdf:about="https://www.theworldavatar.com/kg/ontobms/suppliesAirTo">
        <rdfs:domain rdf:resource="https://saref.etsi.org/core/HVAC"/>
        <rdfs:range rdf:resource="https://saref.etsi.org/saref4bldg/FlowMovingDevice"/>
        <rdfs:comment>A relationship that describes a HVAC device supplying air to a flow moving device.</rdfs:comment>
        <rdfs:isDefinedBy rdf:resource="https://www.theworldavatar.com/kg/ontobms/"/>
        <rdfs:label>supplies air to</rdfs:label>
    </owl:ObjectProperty>
    


    <!-- https://www.theworldavatar.com/kg/ontodevice/hasQuantity -->


    <owl:ObjectProperty rdf:about="https://www.theworldavatar.com/kg/ontodevice/hasQuantity"/>
    


    <!-- 
    ///////////////////////////////////////////////////////////////////////////////////////
    //
    // Data properties
    //
    ///////////////////////////////////////////////////////////////////////////////////////
     -->


    


    <!-- https://www.theworldavatar.com/kg/ontobms/hasBacnetDeviceID -->


    <owl:DatatypeProperty rdf:about="https://www.theworldavatar.com/kg/ontobms/hasBacnetDeviceID">
        <rdfs:domain>
            <owl:Class>
                <owl:unionOf rdf:parseType="Collection">
                    <rdf:Description rdf:about="http://www.ontology-of-units-of-measure.org/resource/om-2/Measure"/>
                    <rdf:Description rdf:about="https://saref.etsi.org/core/State"/>
                    <rdf:Description rdf:about="https://www.theworldavatar.com/kg/ontodevice/Mode"/>
                </owl:unionOf>
            </owl:Class>
        </rdfs:domain>
        <rdfs:range rdf:resource="http://www.w3.org/2001/XMLSchema#string"/>
        <rdfs:comment>A relationship that describes the Bacnet Device ID assigned to an entity.</rdfs:comment>
        <rdfs:isDefinedBy rdf:resource="https://www.theworldavatar.com/kg/ontobms/"/>
        <rdfs:label>has bacnet device ID</rdfs:label>
    </owl:DatatypeProperty>
    


    <!-- https://www.theworldavatar.com/kg/ontobms/hasBacnetObjectID -->


    <owl:DatatypeProperty rdf:about="https://www.theworldavatar.com/kg/ontobms/hasBacnetObjectID">
        <rdfs:domain>
            <owl:Class>
                <owl:unionOf rdf:parseType="Collection">
                    <rdf:Description rdf:about="http://www.ontology-of-units-of-measure.org/resource/om-2/Measure"/>
                    <rdf:Description rdf:about="https://saref.etsi.org/core/State"/>
                    <rdf:Description rdf:about="https://www.theworldavatar.com/kg/ontodevice/Mode"/>
                </owl:unionOf>
            </owl:Class>
        </rdfs:domain>
        <rdfs:range rdf:resource="http://www.w3.org/2001/XMLSchema#string"/>
        <rdfs:comment>A relationship that describes the Bacnet Object ID assigned to an entity.</rdfs:comment>
        <rdfs:isDefinedBy rdf:resource="https://www.theworldavatar.com/kg/ontobms/"/>
        <rdfs:label>has bacnet object ID</rdfs:label>
    </owl:DatatypeProperty>
    


    <!-- 
    ///////////////////////////////////////////////////////////////////////////////////////
    //
    // Classes
    //
    ///////////////////////////////////////////////////////////////////////////////////////
     -->


    


    <!-- http://www.ontology-of-units-of-measure.org/resource/om-2/Frequency -->


    <owl:Class rdf:about="http://www.ontology-of-units-of-measure.org/resource/om-2/Frequency"/>
    


    <!-- http://www.ontology-of-units-of-measure.org/resource/om-2/HeatFlowRate -->


    <owl:Class rdf:about="http://www.ontology-of-units-of-measure.org/resource/om-2/HeatFlowRate"/>
    


    <!-- http://www.ontology-of-units-of-measure.org/resource/om-2/Measure -->


    <owl:Class rdf:about="http://www.ontology-of-units-of-measure.org/resource/om-2/Measure"/>
    


    <!-- http://www.ontology-of-units-of-measure.org/resource/om-2/Percentage -->


    <owl:Class rdf:about="http://www.ontology-of-units-of-measure.org/resource/om-2/Percentage"/>
    


    <!-- http://www.ontology-of-units-of-measure.org/resource/om-2/Pressure -->


    <owl:Class rdf:about="http://www.ontology-of-units-of-measure.org/resource/om-2/Pressure"/>
    


    <!-- http://www.ontology-of-units-of-measure.org/resource/om-2/VolumetricFlowRate -->


    <owl:Class rdf:about="http://www.ontology-of-units-of-measure.org/resource/om-2/VolumetricFlowRate"/>
    


    <!-- http://www.theworldavatar.com/ontology/ontocape/chemical_process_system/CPS_behavior/behavior.owl#ConvectiveTransportRate -->


    <owl:Class rdf:about="http://www.theworldavatar.com/ontology/ontocape/chemical_process_system/CPS_behavior/behavior.owl#ConvectiveTransportRate"/>
    


    <!-- http://www.theworldavatar.com/ontology/ontocape/chemical_process_system/CPS_function/process.owl#TemperatureChange -->


    <owl:Class rdf:about="http://www.theworldavatar.com/ontology/ontocape/chemical_process_system/CPS_function/process.owl#TemperatureChange"/>
    


    <!-- http://www.theworldavatar.com/ontology/ontocape/chemical_process_system/CPS_function/process.owl#UnitOperation -->


    <owl:Class rdf:about="http://www.theworldavatar.com/ontology/ontocape/chemical_process_system/CPS_function/process.owl#UnitOperation"/>
    


    <!-- http://www.theworldavatar.com/ontology/ontocape/material/substance/substance.owl#Substance -->


    <owl:Class rdf:about="http://www.theworldavatar.com/ontology/ontocape/material/substance/substance.owl#Substance"/>
    


    <!-- http://www.theworldavatar.com/ontology/ontocape/upper_level/network_system.owl#DirectedConnection -->


    <owl:Class rdf:about="http://www.theworldavatar.com/ontology/ontocape/upper_level/network_system.owl#DirectedConnection"/>
    


    <!-- https://saref.etsi.org/core/HVAC -->


    <owl:Class rdf:about="https://saref.etsi.org/core/HVAC"/>
    


    <!-- https://saref.etsi.org/core/MultiLevelState -->


    <owl:Class rdf:about="https://saref.etsi.org/core/MultiLevelState"/>
    


    <!-- https://saref.etsi.org/core/State -->


    <owl:Class rdf:about="https://saref.etsi.org/core/State"/>
    


    <!-- https://saref.etsi.org/saref4bldg/Coil -->


    <owl:Class rdf:about="https://saref.etsi.org/saref4bldg/Coil"/>
    


    <!-- https://saref.etsi.org/saref4bldg/Fan -->


    <owl:Class rdf:about="https://saref.etsi.org/saref4bldg/Fan"/>
    


    <!-- https://saref.etsi.org/saref4bldg/FlowMovingDevice -->


    <owl:Class rdf:about="https://saref.etsi.org/saref4bldg/FlowMovingDevice"/>
    


    <!-- https://saref.etsi.org/saref4bldg/FlowTreatmentDevice -->


    <owl:Class rdf:about="https://saref.etsi.org/saref4bldg/FlowTreatmentDevice"/>
    


    <!-- https://w3id.org/bot#Zone -->


    <owl:Class rdf:about="https://w3id.org/bot#Zone"/>
    


    <!-- https://www.theworldavatar.com/kg/ontobms/AirChangePerHour -->


    <owl:Class rdf:about="https://www.theworldavatar.com/kg/ontobms/AirChangePerHour">
        <rdfs:subClassOf rdf:resource="http://www.ontology-of-units-of-measure.org/resource/om-2/Frequency"/>
        <rdfs:comment>A measure of how many times the air within a defined space (usually a room or building) is replaced with fresh air in one hour. </rdfs:comment>
        <rdfs:isDefinedBy rdf:resource="https://www.theworldavatar.com/kg/ontobms/"/>
        <rdfs:label>Air change per hour</rdfs:label>
    </owl:Class>
    


    <!-- https://www.theworldavatar.com/kg/ontobms/AirHandlingUnit -->


    <owl:Class rdf:about="https://www.theworldavatar.com/kg/ontobms/AirHandlingUnit">
        <rdfs:subClassOf rdf:resource="https://saref.etsi.org/core/HVAC"/>
        <rdfs:comment>A device that condition and distribute air within a building. </rdfs:comment>
        <rdfs:isDefinedBy rdf:resource="https://www.theworldavatar.com/kg/ontobms/"/>
        <rdfs:label>Air handling unit</rdfs:label>
    </owl:Class>
    


    <!-- https://www.theworldavatar.com/kg/ontobms/CAVSystem -->


    <owl:Class rdf:about="https://www.theworldavatar.com/kg/ontobms/CAVSystem">
        <rdfs:subClassOf rdf:resource="https://saref.etsi.org/core/HVAC"/>
        <rdfs:comment>A Constant Air Volume System that supply a constant airflow at a variable temperature.</rdfs:comment>
        <rdfs:isDefinedBy rdf:resource="https://www.theworldavatar.com/kg/ontobms/"/>
        <rdfs:label>CAV system</rdfs:label>
    </owl:Class>
    


    <!-- https://www.theworldavatar.com/kg/ontobms/CanopyHood -->


    <owl:Class rdf:about="https://www.theworldavatar.com/kg/ontobms/CanopyHood">
        <rdfs:subClassOf rdf:resource="https://saref.etsi.org/saref4bldg/FlowTreatmentDevice"/>
        <rdfs:comment>A device designed to vent non-toxic vapors like steam, heat and odors.</rdfs:comment>
        <rdfs:isDefinedBy rdf:resource="https://www.theworldavatar.com/kg/ontobms/"/>
        <rdfs:label>Canopy hood</rdfs:label>
    </owl:Class>
    


    <!-- https://www.theworldavatar.com/kg/ontobms/DamperControl -->


    <owl:Class rdf:about="https://www.theworldavatar.com/kg/ontobms/DamperControl">
        <rdfs:subClassOf rdf:resource="http://www.ontology-of-units-of-measure.org/resource/om-2/Pressure"/>
        <rdfs:comment>A pressure based measurement used to control the volume of air that flows through your HVAC system by providing measurements to control the damper position.</rdfs:comment>
        <rdfs:isDefinedBy rdf:resource="https://www.theworldavatar.com/kg/ontobms/"/>
        <rdfs:label>Damper control</rdfs:label>
    </owl:Class>
    


    <!-- https://www.theworldavatar.com/kg/ontobms/DamperFeedback -->


    <owl:Class rdf:about="https://www.theworldavatar.com/kg/ontobms/DamperFeedback">
        <rdfs:subClassOf rdf:resource="http://www.ontology-of-units-of-measure.org/resource/om-2/Pressure"/>
        <rdfs:comment>A signal (pressure based) that that can be used to determine the exact position of a damper.</rdfs:comment>
        <rdfs:isDefinedBy rdf:resource="https://www.theworldavatar.com/kg/ontobms/"/>
        <rdfs:label>Damper feedback</rdfs:label>
    </owl:Class>
    


    <!-- https://www.theworldavatar.com/kg/ontobms/DamperState -->


    <owl:Class rdf:about="https://www.theworldavatar.com/kg/ontobms/DamperState">
        <rdfs:subClassOf rdf:resource="https://saref.etsi.org/core/MultiLevelState"/>
        <rdfs:comment>The current state of a damper.</rdfs:comment>
        <rdfs:isDefinedBy rdf:resource="https://www.theworldavatar.com/kg/ontobms/"/>
        <rdfs:label>Damper state</rdfs:label>
    </owl:Class>
    


    <!-- https://www.theworldavatar.com/kg/ontobms/Duct -->


    <owl:Class rdf:about="https://www.theworldavatar.com/kg/ontobms/Duct">
        <rdfs:subClassOf rdf:resource="https://saref.etsi.org/saref4bldg/FlowMovingDevice"/>
        <rdfs:comment>A duct is a conduit or passage used in heating, ventilation, and air conditioning to deliver and remove air.</rdfs:comment>
        <rdfs:isDefinedBy rdf:resource="https://www.theworldavatar.com/kg/ontobms/"/>
        <rdfs:label>Duct</rdfs:label>
    </owl:Class>
    


    <!-- https://www.theworldavatar.com/kg/ontobms/ElectricalCoil -->


    <owl:Class rdf:about="https://www.theworldavatar.com/kg/ontobms/ElectricalCoil">
        <rdfs:subClassOf rdf:resource="https://saref.etsi.org/saref4bldg/Coil"/>
        <rdfs:comment>A coil that uses electricity to generate heat for heat transfer purposes.</rdfs:comment>
        <rdfs:isDefinedBy rdf:resource="https://www.theworldavatar.com/kg/ontobms/"/>
        <rdfs:label>Electrical coil</rdfs:label>
    </owl:Class>
    


    <!-- https://www.theworldavatar.com/kg/ontobms/ExhaustFan -->


    <owl:Class rdf:about="https://www.theworldavatar.com/kg/ontobms/ExhaustFan">
        <rdfs:subClassOf rdf:resource="https://saref.etsi.org/saref4bldg/Fan"/>
        <rdfs:comment>An exhaust fan pull odors, fumes, and moisture from an area and vent them outdoors for removal.</rdfs:comment>
        <rdfs:isDefinedBy rdf:resource="https://www.theworldavatar.com/kg/ontobms/"/>
        <rdfs:label>Exhaust fan</rdfs:label>
    </owl:Class>
    


    <!-- https://www.theworldavatar.com/kg/ontobms/ExhaustVAV -->


    <owl:Class rdf:about="https://www.theworldavatar.com/kg/ontobms/ExhaustVAV">
        <rdfs:subClassOf rdf:resource="https://www.theworldavatar.com/kg/ontobms/VAVSystem"/>
        <rdfs:comment>A Variable Air Volume System that extracts airflow at a constant or varying temperature.</rdfs:comment>
        <rdfs:isDefinedBy rdf:resource="https://www.theworldavatar.com/kg/ontobms/"/>
        <rdfs:label>Exhaust VAV</rdfs:label>
    </owl:Class>
    


    <!-- https://www.theworldavatar.com/kg/ontobms/ExtractionArm -->


    <owl:Class rdf:about="https://www.theworldavatar.com/kg/ontobms/ExtractionArm">
        <rdfs:subClassOf rdf:resource="https://saref.etsi.org/saref4bldg/FlowTreatmentDevice"/>
        <rdfs:comment>A device that captures welding and soldering fumes, gases, vapours and dusts directly at source and can be connected to a central extraction unit via fans or a pipeline.</rdfs:comment>
        <rdfs:isDefinedBy rdf:resource="https://www.theworldavatar.com/kg/ontobms/"/>
        <rdfs:label>Extraction arm</rdfs:label>
    </owl:Class>
    


    <!-- https://www.theworldavatar.com/kg/ontobms/FanCoilUnit -->


    <owl:Class rdf:about="https://www.theworldavatar.com/kg/ontobms/FanCoilUnit">
        <rdfs:subClassOf rdf:resource="https://saref.etsi.org/core/HVAC"/>
        <rdfs:comment>A device that consists of a fan, a coil, and other components, that are used to cool or heat the air recirculating within a room.</rdfs:comment>
        <rdfs:isDefinedBy rdf:resource="https://www.theworldavatar.com/kg/ontobms/"/>
        <rdfs:label>Fan coil unit</rdfs:label>
    </owl:Class>
    


    <!-- https://www.theworldavatar.com/kg/ontobms/FumeHood -->


    <owl:Class rdf:about="https://www.theworldavatar.com/kg/ontobms/FumeHood">
        <rdfs:subClassOf rdf:resource="https://saref.etsi.org/saref4bldg/FlowTreatmentDevice"/>
        <rdfs:comment>A device that uses venting and air flow to protect users from hazardous substances such as vapors, gases, and particulates.</rdfs:comment>
        <rdfs:isDefinedBy rdf:resource="https://www.theworldavatar.com/kg/ontobms/"/>
        <rdfs:label>Fume hood</rdfs:label>
    </owl:Class>
    


    <!-- https://www.theworldavatar.com/kg/ontobms/HeatDuty -->


    <owl:Class rdf:about="https://www.theworldavatar.com/kg/ontobms/HeatDuty">
        <rdfs:subClassOf rdf:resource="http://www.ontology-of-units-of-measure.org/resource/om-2/HeatFlowRate"/>
        <rdfs:comment>The amount of heat that needs to be added or removed to create the required change in temperature.</rdfs:comment>
        <rdfs:isDefinedBy rdf:resource="https://www.theworldavatar.com/kg/ontobms/"/>
        <rdfs:label>Heat duty</rdfs:label>
    </owl:Class>
    


    <!-- https://www.theworldavatar.com/kg/ontobms/HighLevelState -->


    <owl:Class rdf:about="https://www.theworldavatar.com/kg/ontobms/HighLevelState">
        <rdfs:subClassOf rdf:resource="https://saref.etsi.org/core/State"/>
        <rdfs:comment>The current state of a device at a high level.</rdfs:comment>
        <rdfs:isDefinedBy rdf:resource="https://www.theworldavatar.com/kg/ontobms/"/>
        <rdfs:label>High level state</rdfs:label>
    </owl:Class>
    


    <!-- https://www.theworldavatar.com/kg/ontobms/HighPlumeFan -->


    <owl:Class rdf:about="https://www.theworldavatar.com/kg/ontobms/HighPlumeFan">
        <rdfs:subClassOf rdf:resource="https://www.theworldavatar.com/kg/ontobms/ExhaustFan"/>
        <rdfs:comment>A type of exhaust fan that dilute and disperse potentially hazardous exhaust or fumes quickly and safely.</rdfs:comment>
        <rdfs:isDefinedBy rdf:resource="https://www.theworldavatar.com/kg/ontobms/"/>
        <rdfs:label>High plume fan</rdfs:label>
    </owl:Class>
    


    <!-- https://www.theworldavatar.com/kg/ontobms/LowLevelState -->


    <owl:Class rdf:about="https://www.theworldavatar.com/kg/ontobms/LowLevelState">
        <rdfs:subClassOf rdf:resource="https://saref.etsi.org/core/State"/>
        <rdfs:comment>The current state of a device at a low level.</rdfs:comment>
        <rdfs:isDefinedBy rdf:resource="https://www.theworldavatar.com/kg/ontobms/"/>
        <rdfs:label>Low level state</rdfs:label>
    </owl:Class>
    


    <!-- https://www.theworldavatar.com/kg/ontobms/MakeupAirUnit -->


    <owl:Class rdf:about="https://www.theworldavatar.com/kg/ontobms/MakeupAirUnit">
        <rdfs:subClassOf rdf:resource="https://saref.etsi.org/core/HVAC"/>
        <rdfs:comment>A device that provide a consistent and controlled solution to replacing the air within a space.</rdfs:comment>
        <rdfs:isDefinedBy rdf:resource="https://www.theworldavatar.com/kg/ontobms/"/>
        <rdfs:label>Makeup air unit</rdfs:label>
    </owl:Class>
    


    <!-- https://www.theworldavatar.com/kg/ontobms/MediumLevelState -->


    <owl:Class rdf:about="https://www.theworldavatar.com/kg/ontobms/MediumLevelState">
        <rdfs:subClassOf rdf:resource="https://saref.etsi.org/core/State"/>
        <rdfs:comment>The current state of a device at a medium level.</rdfs:comment>
        <rdfs:isDefinedBy rdf:resource="https://www.theworldavatar.com/kg/ontobms/"/>
        <rdfs:label>Medium level state</rdfs:label>
    </owl:Class>
    


    <!-- https://www.theworldavatar.com/kg/ontobms/Pipe -->


    <owl:Class rdf:about="https://www.theworldavatar.com/kg/ontobms/Pipe">
        <rdfs:subClassOf rdf:resource="https://saref.etsi.org/saref4bldg/FlowMovingDevice"/>
        <rdfs:comment>A pipe is a tubular section or hollow cylinder, usually but not necessarily of circular cross-section, used mainly to convey fluids.</rdfs:comment>
        <rdfs:isDefinedBy rdf:resource="https://www.theworldavatar.com/kg/ontobms/"/>
        <rdfs:label>Pipe</rdfs:label>
    </owl:Class>
    


    <!-- https://www.theworldavatar.com/kg/ontobms/PipeManifold -->


    <owl:Class rdf:about="https://www.theworldavatar.com/kg/ontobms/PipeManifold">
        <rdfs:subClassOf rdf:resource="https://saref.etsi.org/saref4bldg/FlowMovingDevice"/>
        <rdfs:comment>A device that channels multiple fluid streams into a single pipe, or vice versa.</rdfs:comment>
        <rdfs:isDefinedBy rdf:resource="https://www.theworldavatar.com/kg/ontobms/"/>
        <rdfs:label>Pipe manifold</rdfs:label>
    </owl:Class>
    


    <!-- https://www.theworldavatar.com/kg/ontobms/Plenum -->


    <owl:Class rdf:about="https://www.theworldavatar.com/kg/ontobms/Plenum">
        <rdfs:subClassOf rdf:resource="https://saref.etsi.org/core/HVAC"/>
        <rdfs:comment>A separate space provided for air circulation for heating, ventilation, and air-conditioning.</rdfs:comment>
        <rdfs:isDefinedBy rdf:resource="https://www.theworldavatar.com/kg/ontobms/"/>
        <rdfs:label>Plenum</rdfs:label>
    </owl:Class>
    


    <!-- https://www.theworldavatar.com/kg/ontobms/SupplyVAV -->


    <owl:Class rdf:about="https://www.theworldavatar.com/kg/ontobms/SupplyVAV">
        <rdfs:subClassOf rdf:resource="https://www.theworldavatar.com/kg/ontobms/VAVSystem"/>
        <rdfs:comment>A Variable Air Volume System that supplies airflow at a constant or varying temperature.</rdfs:comment>
        <rdfs:isDefinedBy rdf:resource="https://www.theworldavatar.com/kg/ontobms/"/>
        <rdfs:label>Supply VAV</rdfs:label>
    </owl:Class>
    


    <!-- https://www.theworldavatar.com/kg/ontobms/Tee -->


    <owl:Class rdf:about="https://www.theworldavatar.com/kg/ontobms/Tee">
        <rdfs:subClassOf rdf:resource="https://saref.etsi.org/saref4bldg/FlowMovingDevice"/>
        <rdfs:comment>A Tee is a connector between pipes to separate or combine some streams.</rdfs:comment>
        <rdfs:isDefinedBy rdf:resource="https://www.theworldavatar.com/kg/ontobms/"/>
        <rdfs:label>Tee</rdfs:label>
    </owl:Class>
    


    <!-- https://www.theworldavatar.com/kg/ontobms/VAVSystem -->


    <owl:Class rdf:about="https://www.theworldavatar.com/kg/ontobms/VAVSystem">
        <rdfs:subClassOf rdf:resource="https://saref.etsi.org/core/HVAC"/>
        <rdfs:comment>A Variable Air Volume System that vary the airflow at a constant or varying temperature.</rdfs:comment>
        <rdfs:isDefinedBy rdf:resource="https://www.theworldavatar.com/kg/ontobms/"/>
        <rdfs:label>VAV system</rdfs:label>
    </owl:Class>
    


    <!-- https://www.theworldavatar.com/kg/ontobms/VSDControl -->


    <owl:Class rdf:about="https://www.theworldavatar.com/kg/ontobms/VSDControl">
        <rdfs:subClassOf rdf:resource="http://www.ontology-of-units-of-measure.org/resource/om-2/Frequency"/>
        <rdfs:comment>A frequency based measurement used to control an AC motor's speed and torque.</rdfs:comment>
        <rdfs:isDefinedBy rdf:resource="https://www.theworldavatar.com/kg/ontobms/"/>
        <rdfs:label>VSD control</rdfs:label>
    </owl:Class>
    


    <!-- https://www.theworldavatar.com/kg/ontobms/VSDFeedback -->


    <owl:Class rdf:about="https://www.theworldavatar.com/kg/ontobms/VSDFeedback">
        <rdfs:subClassOf rdf:resource="http://www.ontology-of-units-of-measure.org/resource/om-2/Frequency"/>
        <rdfs:comment>A signal (frequency based) that that can be used to determine the current state of a VSD device (fan etc).</rdfs:comment>
        <rdfs:isDefinedBy rdf:resource="https://www.theworldavatar.com/kg/ontobms/"/>
        <rdfs:label>VSD feedback</rdfs:label>
    </owl:Class>
    


    <!-- https://www.theworldavatar.com/kg/ontobms/WalkInFumeHood -->


    <owl:Class rdf:about="https://www.theworldavatar.com/kg/ontobms/WalkInFumeHood">
        <rdfs:subClassOf rdf:resource="https://www.theworldavatar.com/kg/ontobms/FumeHood"/>
        <rdfs:comment>A larger fume hood designed to be able to house large laboratory instruments and equipment. </rdfs:comment>
        <rdfs:isDefinedBy rdf:resource="https://www.theworldavatar.com/kg/ontobms/"/>
        <rdfs:label>Walk-in fume hood</rdfs:label>
    </owl:Class>
    


    <!-- https://www.theworldavatar.com/kg/ontobms/WaterCoil -->


    <owl:Class rdf:about="https://www.theworldavatar.com/kg/ontobms/WaterCoil">
        <rdfs:subClassOf rdf:resource="https://saref.etsi.org/saref4bldg/Coil"/>
        <rdfs:comment>A coil that uses water as a heat transfer medium.</rdfs:comment>
        <rdfs:isDefinedBy rdf:resource="https://www.theworldavatar.com/kg/ontobms/"/>
        <rdfs:label>Water coil</rdfs:label>
    </owl:Class>
    


    <!-- https://www.theworldavatar.com/kg/ontodevice/Device -->


    <owl:Class rdf:about="https://www.theworldavatar.com/kg/ontodevice/Device"/>
    


    <!-- https://www.theworldavatar.com/kg/ontodevice/Mode -->


    <owl:Class rdf:about="https://www.theworldavatar.com/kg/ontodevice/Mode"/>
</rdf:RDF>



<!-- Generated by the OWL API (version 5.5.0.2023-01-14T12:41:38Z) https://github.com/owlcs/owlapi/ -->


