<?xml version="1.0"?>
<rdf:RDF xmlns="https://www.theworldavatar.com/kg/ontopoi/"
     xml:base="https://www.theworldavatar.com/kg/ontopoi/"
     xmlns:dc="http://purl.org/dc/elements/1.1/"
     xmlns:owl="http://www.w3.org/2002/07/owl#"
     xmlns:rdf="http://www.w3.org/1999/02/22-rdf-syntax-ns#"
     xmlns:xml="http://www.w3.org/XML/1998/namespace"
     xmlns:xsd="http://www.w3.org/2001/XMLSchema#"
     xmlns:rdfs="http://www.w3.org/2000/01/rdf-schema#"
     xmlns:ontopoi="https://www.theworldavatar.com/kg/ontopoi/">
    <owl:Ontology rdf:about="https://www.theworldavatar.com/kg/ontopoi/">
        <dc:date>25 October 2024</dc:date>
        <rdfs:comment>OntoPOI is an ontology developed for representing points of interest.</rdfs:comment>
        <owl:versionInfo>1</owl:versionInfo>
        <gitCommitHash>c0599beca8df55873a1ab061dee64e52c510c6a0</gitCommitHash>
    </owl:Ontology>
    


    <!-- 
    ///////////////////////////////////////////////////////////////////////////////////////
    //
    // Annotation properties
    //
    ///////////////////////////////////////////////////////////////////////////////////////
     -->


    


    <!-- http://purl.org/dc/elements/1.1/date -->


    <owl:AnnotationProperty rdf:about="http://purl.org/dc/elements/1.1/date"/>
    


    <!-- https://www.theworldavatar.com/kg/ontopoi/gitCommitHash -->


    <owl:AnnotationProperty rdf:about="https://www.theworldavatar.com/kg/ontopoi/gitCommitHash"/>
    


    <!-- 
    ///////////////////////////////////////////////////////////////////////////////////////
    //
    // Classes
    //
    ///////////////////////////////////////////////////////////////////////////////////////
     -->


    


    <!-- https://www.theworldavatar.com/kg/ontopoi/Abrasiveproductsandgrindingequipment -->


    <owl:Class rdf:about="https://www.theworldavatar.com/kg/ontopoi/Abrasiveproductsandgrindingequipment">
        <rdfs:subClassOf rdf:resource="https://www.theworldavatar.com/kg/ontopoi/Industrialproducts"/>
        <rdfs:comment>Abrasive products and grinding equipment is a subcategory of industrial products</rdfs:comment>
        <rdfs:isDefinedBy rdf:resource="https://www.theworldavatar.com/kg/ontopoi"/>
        <rdfs:label>Abrasive products and grinding equipment</rdfs:label>
    </owl:Class>
    


    <!-- https://www.theworldavatar.com/kg/ontopoi/Accessequipment -->


    <owl:Class rdf:about="https://www.theworldavatar.com/kg/ontopoi/Accessequipment">
        <rdfs:subClassOf rdf:resource="https://www.theworldavatar.com/kg/ontopoi/Industrialproducts"/>
        <rdfs:comment>Access equipment is a subcategory of industrial products</rdfs:comment>
        <rdfs:isDefinedBy rdf:resource="https://www.theworldavatar.com/kg/ontopoi"/>
        <rdfs:label>Access equipment</rdfs:label>
    </owl:Class>
    


    <!-- https://www.theworldavatar.com/kg/ontopoi/Accidentandemergencyhospitals -->


    <owl:Class rdf:about="https://www.theworldavatar.com/kg/ontopoi/Accidentandemergencyhospitals">
        <rdfs:subClassOf rdf:resource="https://www.theworldavatar.com/kg/ontopoi/Healthpractitionersandestablishments"/>
        <rdfs:comment>Accident and emergency hospitals is a subcategory of health practitioners and establishments</rdfs:comment>
        <rdfs:isDefinedBy rdf:resource="https://www.theworldavatar.com/kg/ontopoi"/>
        <rdfs:label>Accident and emergency hospitals</rdfs:label>
    </owl:Class>
    


    <!-- https://www.theworldavatar.com/kg/ontopoi/Accommodation -->


    <owl:Class rdf:about="https://www.theworldavatar.com/kg/ontopoi/Accommodation">
        <rdfs:subClassOf rdf:resource="https://www.theworldavatar.com/kg/ontopoi/Accommodationandeatinganddrinking"/>
        <rdfs:comment>Accommodation is a subcategory of accommodation, eating and drinking</rdfs:comment>
        <rdfs:isDefinedBy rdf:resource="https://www.theworldavatar.com/kg/ontopoi"/>
        <rdfs:label>Accommodation</rdfs:label>
    </owl:Class>
    


    <!-- https://www.theworldavatar.com/kg/ontopoi/Accommodationandeatinganddrinking -->


    <owl:Class rdf:about="https://www.theworldavatar.com/kg/ontopoi/Accommodationandeatinganddrinking"/>
    


    <!-- https://www.theworldavatar.com/kg/ontopoi/Accountantsandauditors -->


    <owl:Class rdf:about="https://www.theworldavatar.com/kg/ontopoi/Accountantsandauditors">
        <rdfs:subClassOf rdf:resource="https://www.theworldavatar.com/kg/ontopoi/Legalandfinancial"/>
        <rdfs:comment>Accountants and auditors is a subcategory of legal and financial</rdfs:comment>
        <rdfs:isDefinedBy rdf:resource="https://www.theworldavatar.com/kg/ontopoi"/>
        <rdfs:label>Accountants and auditors</rdfs:label>
    </owl:Class>
    


    <!-- https://www.theworldavatar.com/kg/ontopoi/Adhesivesandsealants -->


    <owl:Class rdf:about="https://www.theworldavatar.com/kg/ontopoi/Adhesivesandsealants">
        <rdfs:subClassOf rdf:resource="https://www.theworldavatar.com/kg/ontopoi/Industrialproducts"/>
        <rdfs:comment>Adhesives and sealants is a subcategory of industrial products</rdfs:comment>
        <rdfs:isDefinedBy rdf:resource="https://www.theworldavatar.com/kg/ontopoi"/>
        <rdfs:label>Adhesives and sealants</rdfs:label>
    </owl:Class>
    


    <!-- https://www.theworldavatar.com/kg/ontopoi/Adultservices -->


    <owl:Class rdf:about="https://www.theworldavatar.com/kg/ontopoi/Adultservices">
        <rdfs:subClassOf rdf:resource="https://www.theworldavatar.com/kg/ontopoi/Personalandconsumerandotherservices"/>
        <rdfs:comment>Adult services is a subcategory of personal, consumer and other services</rdfs:comment>
        <rdfs:isDefinedBy rdf:resource="https://www.theworldavatar.com/kg/ontopoi"/>
        <rdfs:label>Adult services</rdfs:label>
    </owl:Class>
    


    <!-- https://www.theworldavatar.com/kg/ontopoi/Adultshops -->


    <owl:Class rdf:about="https://www.theworldavatar.com/kg/ontopoi/Adultshops">
        <rdfs:subClassOf rdf:resource="https://www.theworldavatar.com/kg/ontopoi/Householdandofficeandleisureandgarden"/>
        <rdfs:comment>Adult shops is a subcategory of household, office, leisure and garden</rdfs:comment>
        <rdfs:isDefinedBy rdf:resource="https://www.theworldavatar.com/kg/ontopoi"/>
        <rdfs:label>Adult shops</rdfs:label>
    </owl:Class>
    


    <!-- https://www.theworldavatar.com/kg/ontopoi/Adultvenues -->


    <owl:Class rdf:about="https://www.theworldavatar.com/kg/ontopoi/Adultvenues">
        <rdfs:subClassOf rdf:resource="https://www.theworldavatar.com/kg/ontopoi/Venuesandstageandscreen"/>
        <rdfs:comment>Adult venues is a subcategory of venues, stage and screen</rdfs:comment>
        <rdfs:isDefinedBy rdf:resource="https://www.theworldavatar.com/kg/ontopoi"/>
        <rdfs:label>Adult venues</rdfs:label>
    </owl:Class>
    


    <!-- https://www.theworldavatar.com/kg/ontopoi/Advertisingservices -->


    <owl:Class rdf:about="https://www.theworldavatar.com/kg/ontopoi/Advertisingservices">
        <rdfs:subClassOf rdf:resource="https://www.theworldavatar.com/kg/ontopoi/ITandadvertisingandmarketingandmediaservices"/>
        <rdfs:comment>Advertising services is a subcategory of it, advertising, marketing and media service s</rdfs:comment>
        <rdfs:isDefinedBy rdf:resource="https://www.theworldavatar.com/kg/ontopoi"/>
        <rdfs:label>Advertising services</rdfs:label>
    </owl:Class>
    


    <!-- https://www.theworldavatar.com/kg/ontopoi/Aeroplanes -->


    <owl:Class rdf:about="https://www.theworldavatar.com/kg/ontopoi/Aeroplanes">
        <rdfs:subClassOf rdf:resource="https://www.theworldavatar.com/kg/ontopoi/Industrialproducts"/>
        <rdfs:comment>Aeroplanes is a subcategory of industrial products</rdfs:comment>
        <rdfs:isDefinedBy rdf:resource="https://www.theworldavatar.com/kg/ontopoi"/>
        <rdfs:label>Aeroplanes</rdfs:label>
    </owl:Class>
    


    <!-- https://www.theworldavatar.com/kg/ontopoi/Agriculturalcontractors -->


    <owl:Class rdf:about="https://www.theworldavatar.com/kg/ontopoi/Agriculturalcontractors">
        <rdfs:subClassOf rdf:resource="https://www.theworldavatar.com/kg/ontopoi/Contractservices"/>
        <rdfs:comment>Agricultural contractors is a subcategory of contract services</rdfs:comment>
        <rdfs:isDefinedBy rdf:resource="https://www.theworldavatar.com/kg/ontopoi"/>
        <rdfs:label>Agricultural contractors</rdfs:label>
    </owl:Class>
    


    <!-- https://www.theworldavatar.com/kg/ontopoi/Agriculturalmachineryandgoods -->


    <owl:Class rdf:about="https://www.theworldavatar.com/kg/ontopoi/Agriculturalmachineryandgoods">
        <rdfs:subClassOf rdf:resource="https://www.theworldavatar.com/kg/ontopoi/Industrialproducts"/>
        <rdfs:comment>Agricultural machinery and goods is a subcategory of industrial products</rdfs:comment>
        <rdfs:isDefinedBy rdf:resource="https://www.theworldavatar.com/kg/ontopoi"/>
        <rdfs:label>Agricultural machinery and goods</rdfs:label>
    </owl:Class>
    


    <!-- https://www.theworldavatar.com/kg/ontopoi/Air -->


    <owl:Class rdf:about="https://www.theworldavatar.com/kg/ontopoi/Air">
        <rdfs:subClassOf rdf:resource="https://www.theworldavatar.com/kg/ontopoi/Transport"/>
        <rdfs:comment>Air is a subcategory of transport</rdfs:comment>
        <rdfs:isDefinedBy rdf:resource="https://www.theworldavatar.com/kg/ontopoi"/>
        <rdfs:label>Air</rdfs:label>
    </owl:Class>
    


    <!-- https://www.theworldavatar.com/kg/ontopoi/Airandwaterfiltration -->


    <owl:Class rdf:about="https://www.theworldavatar.com/kg/ontopoi/Airandwaterfiltration">
        <rdfs:subClassOf rdf:resource="https://www.theworldavatar.com/kg/ontopoi/Industrialproducts"/>
        <rdfs:comment>Air and water filtration is a subcategory of industrial products</rdfs:comment>
        <rdfs:isDefinedBy rdf:resource="https://www.theworldavatar.com/kg/ontopoi"/>
        <rdfs:label>Air and water filtration</rdfs:label>
    </owl:Class>
    


    <!-- https://www.theworldavatar.com/kg/ontopoi/Aircraftcharters -->


    <owl:Class rdf:about="https://www.theworldavatar.com/kg/ontopoi/Aircraftcharters">
        <rdfs:subClassOf rdf:resource="https://www.theworldavatar.com/kg/ontopoi/Contractservices"/>
        <rdfs:comment>Aircraft charters is a subcategory of contract services</rdfs:comment>
        <rdfs:isDefinedBy rdf:resource="https://www.theworldavatar.com/kg/ontopoi"/>
        <rdfs:label>Aircraft charters</rdfs:label>
    </owl:Class>
    


    <!-- https://www.theworldavatar.com/kg/ontopoi/Airlinesandairlineservices -->


    <owl:Class rdf:about="https://www.theworldavatar.com/kg/ontopoi/Airlinesandairlineservices">
        <rdfs:subClassOf rdf:resource="https://www.theworldavatar.com/kg/ontopoi/Transportandstorageanddelivery"/>
        <rdfs:comment>Airlines and airline services is a subcategory of transport, storage and delivery</rdfs:comment>
        <rdfs:isDefinedBy rdf:resource="https://www.theworldavatar.com/kg/ontopoi"/>
        <rdfs:label>Airlines and airline services</rdfs:label>
    </owl:Class>
    


    <!-- https://www.theworldavatar.com/kg/ontopoi/Airportsandlandingstrips -->


    <owl:Class rdf:about="https://www.theworldavatar.com/kg/ontopoi/Airportsandlandingstrips">
        <rdfs:subClassOf rdf:resource="https://www.theworldavatar.com/kg/ontopoi/Air"/>
        <rdfs:comment>Airports and landing strips is a subcategory of air</rdfs:comment>
        <rdfs:isDefinedBy rdf:resource="https://www.theworldavatar.com/kg/ontopoi"/>
        <rdfs:label>Airports and landing strips</rdfs:label>
    </owl:Class>
    


    <!-- https://www.theworldavatar.com/kg/ontopoi/Alcoholicdrinks -->


    <owl:Class rdf:about="https://www.theworldavatar.com/kg/ontopoi/Alcoholicdrinks">
        <rdfs:subClassOf rdf:resource="https://www.theworldavatar.com/kg/ontopoi/Foodstuffs"/>
        <rdfs:comment>Alcoholic drinks is a subcategory of foodstuffs</rdfs:comment>
        <rdfs:isDefinedBy rdf:resource="https://www.theworldavatar.com/kg/ontopoi"/>
        <rdfs:label>Alcoholic drinks</rdfs:label>
    </owl:Class>
    


    <!-- https://www.theworldavatar.com/kg/ontopoi/Alcoholicdrinksincludingoff-licencesandwholesalers -->


    <owl:Class rdf:about="https://www.theworldavatar.com/kg/ontopoi/Alcoholicdrinksincludingoff-licencesandwholesalers">
        <rdfs:subClassOf rdf:resource="https://www.theworldavatar.com/kg/ontopoi/Foodanddrinkandmultiitemretail"/>
        <rdfs:comment>Alcoholic drinks including off-licences and wholesalers is a subcategory of food, drink and multi item retail</rdfs:comment>
        <rdfs:isDefinedBy rdf:resource="https://www.theworldavatar.com/kg/ontopoi"/>
        <rdfs:label>Alcoholic drinks including off-licences and wholesalers</rdfs:label>
    </owl:Class>
    


    <!-- https://www.theworldavatar.com/kg/ontopoi/Allotments -->


    <owl:Class rdf:about="https://www.theworldavatar.com/kg/ontopoi/Allotments">
        <rdfs:subClassOf rdf:resource="https://www.theworldavatar.com/kg/ontopoi/Infrastructureandfacilities"/>
        <rdfs:comment>Allotments is a subcategory of infrastructure and facilities</rdfs:comment>
        <rdfs:isDefinedBy rdf:resource="https://www.theworldavatar.com/kg/ontopoi"/>
        <rdfs:label>Allotments</rdfs:label>
    </owl:Class>
    


    <!-- https://www.theworldavatar.com/kg/ontopoi/Alternativeandnaturalandcomplementary -->


    <owl:Class rdf:about="https://www.theworldavatar.com/kg/ontopoi/Alternativeandnaturalandcomplementary">
        <rdfs:subClassOf rdf:resource="https://www.theworldavatar.com/kg/ontopoi/Healthpractitionersandestablishments"/>
        <rdfs:comment>Alternative, natural and complementary is a subcategory of health practitioners and establishments</rdfs:comment>
        <rdfs:isDefinedBy rdf:resource="https://www.theworldavatar.com/kg/ontopoi"/>
        <rdfs:label>Alternative, natural and complementary</rdfs:label>
    </owl:Class>
    


    <!-- https://www.theworldavatar.com/kg/ontopoi/Ambulanceandmedicaltransportationservices -->


    <owl:Class rdf:about="https://www.theworldavatar.com/kg/ontopoi/Ambulanceandmedicaltransportationservices">
        <rdfs:subClassOf rdf:resource="https://www.theworldavatar.com/kg/ontopoi/Healthsupportservices"/>
        <rdfs:comment>Ambulance and medical transportation services is a subcategory of health support services</rdfs:comment>
        <rdfs:isDefinedBy rdf:resource="https://www.theworldavatar.com/kg/ontopoi"/>
        <rdfs:label>Ambulance and medical transportation services</rdfs:label>
    </owl:Class>
    


    <!-- https://www.theworldavatar.com/kg/ontopoi/Amusementparksandarcades -->


    <owl:Class rdf:about="https://www.theworldavatar.com/kg/ontopoi/Amusementparksandarcades">
        <rdfs:subClassOf rdf:resource="https://www.theworldavatar.com/kg/ontopoi/Gambling"/>
        <rdfs:comment>Amusement parks and arcades is a subcategory of gambling</rdfs:comment>
        <rdfs:isDefinedBy rdf:resource="https://www.theworldavatar.com/kg/ontopoi"/>
        <rdfs:label>Amusement parks and arcades</rdfs:label>
    </owl:Class>
    


    <!-- https://www.theworldavatar.com/kg/ontopoi/Anglingandsportsfishing -->


    <owl:Class rdf:about="https://www.theworldavatar.com/kg/ontopoi/Anglingandsportsfishing">
        <rdfs:subClassOf rdf:resource="https://www.theworldavatar.com/kg/ontopoi/Outdoorpursuits"/>
        <rdfs:comment>Angling and sports fishing is a subcategory of outdoor pursuits</rdfs:comment>
        <rdfs:isDefinedBy rdf:resource="https://www.theworldavatar.com/kg/ontopoi"/>
        <rdfs:label>Angling and sports fishing</rdfs:label>
    </owl:Class>
    


    <!-- https://www.theworldavatar.com/kg/ontopoi/Animalclippingandgrooming -->


    <owl:Class rdf:about="https://www.theworldavatar.com/kg/ontopoi/Animalclippingandgrooming">
        <rdfs:subClassOf rdf:resource="https://www.theworldavatar.com/kg/ontopoi/Animalwelfare"/>
        <rdfs:comment>Animal clipping and grooming is a subcategory of animal welfare</rdfs:comment>
        <rdfs:isDefinedBy rdf:resource="https://www.theworldavatar.com/kg/ontopoi"/>
        <rdfs:label>Animal clipping and grooming</rdfs:label>
    </owl:Class>
    


    <!-- https://www.theworldavatar.com/kg/ontopoi/Animalfeedsandpetfoodsandhayandstraw -->


    <owl:Class rdf:about="https://www.theworldavatar.com/kg/ontopoi/Animalfeedsandpetfoodsandhayandstraw">
        <rdfs:subClassOf rdf:resource="https://www.theworldavatar.com/kg/ontopoi/Foodstuffs"/>
        <rdfs:comment>Animal feeds, pet foods, hay and straw is a subcategory of foodstuffs</rdfs:comment>
        <rdfs:isDefinedBy rdf:resource="https://www.theworldavatar.com/kg/ontopoi"/>
        <rdfs:label>Animal feeds, pet foods, hay and straw</rdfs:label>
    </owl:Class>
    


    <!-- https://www.theworldavatar.com/kg/ontopoi/Animaltransportation -->


    <owl:Class rdf:about="https://www.theworldavatar.com/kg/ontopoi/Animaltransportation">
        <rdfs:subClassOf rdf:resource="https://www.theworldavatar.com/kg/ontopoi/Transportandstorageanddelivery"/>
        <rdfs:comment>Animal transportation is a subcategory of transport, storage and delivery</rdfs:comment>
        <rdfs:isDefinedBy rdf:resource="https://www.theworldavatar.com/kg/ontopoi"/>
        <rdfs:label>Animal transportation</rdfs:label>
    </owl:Class>
    


    <!-- https://www.theworldavatar.com/kg/ontopoi/Animalwelfare -->


    <owl:Class rdf:about="https://www.theworldavatar.com/kg/ontopoi/Animalwelfare">
        <rdfs:subClassOf rdf:resource="https://www.theworldavatar.com/kg/ontopoi/Educationandhealth"/>
        <rdfs:comment>Animal welfare is a subcategory of education and health</rdfs:comment>
        <rdfs:isDefinedBy rdf:resource="https://www.theworldavatar.com/kg/ontopoi"/>
        <rdfs:label>Animal welfare</rdfs:label>
    </owl:Class>
    


    <!-- https://www.theworldavatar.com/kg/ontopoi/Animalwelfareorganisations -->


    <owl:Class rdf:about="https://www.theworldavatar.com/kg/ontopoi/Animalwelfareorganisations">
        <rdfs:subClassOf rdf:resource="https://www.theworldavatar.com/kg/ontopoi/Organisations"/>
        <rdfs:comment>Animal welfare organisations is a subcategory of organisations</rdfs:comment>
        <rdfs:isDefinedBy rdf:resource="https://www.theworldavatar.com/kg/ontopoi"/>
        <rdfs:label>Animal welfare organisations</rdfs:label>
    </owl:Class>
    


    <!-- https://www.theworldavatar.com/kg/ontopoi/Aquariaandsealifecentres -->


    <owl:Class rdf:about="https://www.theworldavatar.com/kg/ontopoi/Aquariaandsealifecentres">
        <rdfs:subClassOf rdf:resource="https://www.theworldavatar.com/kg/ontopoi/Botanicalandzoological"/>
        <rdfs:comment>Aquaria and sea life centres is a subcategory of botanical and zoological</rdfs:comment>
        <rdfs:isDefinedBy rdf:resource="https://www.theworldavatar.com/kg/ontopoi"/>
        <rdfs:label>Aquaria and sea life centres</rdfs:label>
    </owl:Class>
    


    <!-- https://www.theworldavatar.com/kg/ontopoi/Aqueducts -->


    <owl:Class rdf:about="https://www.theworldavatar.com/kg/ontopoi/Aqueducts">
        <rdfs:subClassOf rdf:resource="https://www.theworldavatar.com/kg/ontopoi/Water"/>
        <rdfs:comment>Aqueducts is a subcategory of water</rdfs:comment>
        <rdfs:isDefinedBy rdf:resource="https://www.theworldavatar.com/kg/ontopoi"/>
        <rdfs:label>Aqueducts</rdfs:label>
    </owl:Class>
    


    <!-- https://www.theworldavatar.com/kg/ontopoi/Arablefarming -->


    <owl:Class rdf:about="https://www.theworldavatar.com/kg/ontopoi/Arablefarming">
        <rdfs:subClassOf rdf:resource="https://www.theworldavatar.com/kg/ontopoi/Farming"/>
        <rdfs:comment>Arable farming is a subcategory of farming</rdfs:comment>
        <rdfs:isDefinedBy rdf:resource="https://www.theworldavatar.com/kg/ontopoi"/>
        <rdfs:label>Arable farming</rdfs:label>
    </owl:Class>
    


    <!-- https://www.theworldavatar.com/kg/ontopoi/Archaeologicalsites -->


    <owl:Class rdf:about="https://www.theworldavatar.com/kg/ontopoi/Archaeologicalsites">
        <rdfs:subClassOf rdf:resource="https://www.theworldavatar.com/kg/ontopoi/Historicalandcultural"/>
        <rdfs:comment>Archaeological sites is a subcategory of historical and cultural</rdfs:comment>
        <rdfs:isDefinedBy rdf:resource="https://www.theworldavatar.com/kg/ontopoi"/>
        <rdfs:label>Archaeological sites</rdfs:label>
    </owl:Class>
    


    <!-- https://www.theworldavatar.com/kg/ontopoi/Architecturalandbuilding-relatedconsultants -->


    <owl:Class rdf:about="https://www.theworldavatar.com/kg/ontopoi/Architecturalandbuilding-relatedconsultants">
        <rdfs:subClassOf rdf:resource="https://www.theworldavatar.com/kg/ontopoi/Consultancies"/>
        <rdfs:comment>Architectural and building-related consultants is a subcategory of consultancies</rdfs:comment>
        <rdfs:isDefinedBy rdf:resource="https://www.theworldavatar.com/kg/ontopoi"/>
        <rdfs:label>Architectural and building-related consultants</rdfs:label>
    </owl:Class>
    


    <!-- https://www.theworldavatar.com/kg/ontopoi/Armedservices -->


    <owl:Class rdf:about="https://www.theworldavatar.com/kg/ontopoi/Armedservices">
        <rdfs:subClassOf rdf:resource="https://www.theworldavatar.com/kg/ontopoi/Centralandlocalgovernment"/>
        <rdfs:comment>Armed services is a subcategory of central and local government</rdfs:comment>
        <rdfs:isDefinedBy rdf:resource="https://www.theworldavatar.com/kg/ontopoi"/>
        <rdfs:label>Armed services</rdfs:label>
    </owl:Class>
    


    <!-- https://www.theworldavatar.com/kg/ontopoi/Armsandammunition -->


    <owl:Class rdf:about="https://www.theworldavatar.com/kg/ontopoi/Armsandammunition">
        <rdfs:subClassOf rdf:resource="https://www.theworldavatar.com/kg/ontopoi/Industrialproducts"/>
        <rdfs:comment>Arms and ammunition is a subcategory of industrial products</rdfs:comment>
        <rdfs:isDefinedBy rdf:resource="https://www.theworldavatar.com/kg/ontopoi"/>
        <rdfs:label>Arms and ammunition</rdfs:label>
    </owl:Class>
    


    <!-- https://www.theworldavatar.com/kg/ontopoi/Artandantiques -->


    <owl:Class rdf:about="https://www.theworldavatar.com/kg/ontopoi/Artandantiques">
        <rdfs:subClassOf rdf:resource="https://www.theworldavatar.com/kg/ontopoi/Householdandofficeandleisureandgarden"/>
        <rdfs:comment>Art and antiques is a subcategory of household, office, leisure and garden</rdfs:comment>
        <rdfs:isDefinedBy rdf:resource="https://www.theworldavatar.com/kg/ontopoi"/>
        <rdfs:label>Art and antiques</rdfs:label>
    </owl:Class>
    


    <!-- https://www.theworldavatar.com/kg/ontopoi/Artgalleries -->


    <owl:Class rdf:about="https://www.theworldavatar.com/kg/ontopoi/Artgalleries">
        <rdfs:subClassOf rdf:resource="https://www.theworldavatar.com/kg/ontopoi/Historicalandcultural"/>
        <rdfs:comment>Art galleries is a subcategory of historical and cultural</rdfs:comment>
        <rdfs:isDefinedBy rdf:resource="https://www.theworldavatar.com/kg/ontopoi"/>
        <rdfs:label>Art galleries</rdfs:label>
    </owl:Class>
    


    <!-- https://www.theworldavatar.com/kg/ontopoi/Artistsandillustratorsandcalligraphers -->


    <owl:Class rdf:about="https://www.theworldavatar.com/kg/ontopoi/Artistsandillustratorsandcalligraphers">
        <rdfs:subClassOf rdf:resource="https://www.theworldavatar.com/kg/ontopoi/ITandadvertisingandmarketingandmediaservices"/>
        <rdfs:comment>Artists, illustrators and calligraphers is a subcategory of it, advertising, marketing and media service s</rdfs:comment>
        <rdfs:isDefinedBy rdf:resource="https://www.theworldavatar.com/kg/ontopoi"/>
        <rdfs:label>Artists, illustrators and calligraphers</rdfs:label>
    </owl:Class>
    


    <!-- https://www.theworldavatar.com/kg/ontopoi/Astrologersandclairvoyantsandpalmists -->


    <owl:Class rdf:about="https://www.theworldavatar.com/kg/ontopoi/Astrologersandclairvoyantsandpalmists">
        <rdfs:subClassOf rdf:resource="https://www.theworldavatar.com/kg/ontopoi/Personalandconsumerandotherservices"/>
        <rdfs:comment>Astrologers, clairvoyants and palmists is a subcategory of personal, consumer and other services</rdfs:comment>
        <rdfs:isDefinedBy rdf:resource="https://www.theworldavatar.com/kg/ontopoi"/>
        <rdfs:label>Astrologers, clairvoyants and palmists</rdfs:label>
    </owl:Class>
    


    <!-- https://www.theworldavatar.com/kg/ontopoi/Athleticsfacilities -->


    <owl:Class rdf:about="https://www.theworldavatar.com/kg/ontopoi/Athleticsfacilities">
        <rdfs:subClassOf rdf:resource="https://www.theworldavatar.com/kg/ontopoi/Sportscomplex"/>
        <rdfs:comment>Athletics facilities is a subcategory of sports complex</rdfs:comment>
        <rdfs:isDefinedBy rdf:resource="https://www.theworldavatar.com/kg/ontopoi"/>
        <rdfs:label>Athletics facilities</rdfs:label>
    </owl:Class>
    


    <!-- https://www.theworldavatar.com/kg/ontopoi/Attractions -->


    <owl:Class rdf:about="https://www.theworldavatar.com/kg/ontopoi/Attractions"/>
    


    <!-- https://www.theworldavatar.com/kg/ontopoi/Auctioneersandauctionroomsandvaluers -->


    <owl:Class rdf:about="https://www.theworldavatar.com/kg/ontopoi/Auctioneersandauctionroomsandvaluers">
        <rdfs:subClassOf rdf:resource="https://www.theworldavatar.com/kg/ontopoi/Legalandfinancial"/>
        <rdfs:comment>Auctioneers, auction rooms and valuers is a subcategory of legal and financial</rdfs:comment>
        <rdfs:isDefinedBy rdf:resource="https://www.theworldavatar.com/kg/ontopoi"/>
        <rdfs:label>Auctioneers, auction rooms and valuers</rdfs:label>
    </owl:Class>
    


    <!-- https://www.theworldavatar.com/kg/ontopoi/Aviationengineers -->


    <owl:Class rdf:about="https://www.theworldavatar.com/kg/ontopoi/Aviationengineers">
        <rdfs:subClassOf rdf:resource="https://www.theworldavatar.com/kg/ontopoi/Engineeringservices"/>
        <rdfs:comment>Aviation engineers is a subcategory of engineering services</rdfs:comment>
        <rdfs:isDefinedBy rdf:resource="https://www.theworldavatar.com/kg/ontopoi"/>
        <rdfs:label>Aviation engineers</rdfs:label>
    </owl:Class>
    


    <!-- https://www.theworldavatar.com/kg/ontopoi/Babyandnurseryandplaygroundequipment -->


    <owl:Class rdf:about="https://www.theworldavatar.com/kg/ontopoi/Babyandnurseryandplaygroundequipment">
        <rdfs:subClassOf rdf:resource="https://www.theworldavatar.com/kg/ontopoi/Consumerproducts"/>
        <rdfs:comment>Baby, nursery and playground equipment is a subcategory of consumer products</rdfs:comment>
        <rdfs:isDefinedBy rdf:resource="https://www.theworldavatar.com/kg/ontopoi"/>
        <rdfs:label>Baby, nursery and playground equipment</rdfs:label>
    </owl:Class>
    


    <!-- https://www.theworldavatar.com/kg/ontopoi/Babyandnurseryequipmentandchildrenclothes -->


    <owl:Class rdf:about="https://www.theworldavatar.com/kg/ontopoi/Babyandnurseryequipmentandchildrenclothes">
        <rdfs:subClassOf rdf:resource="https://www.theworldavatar.com/kg/ontopoi/Clothingandaccessories"/>
        <rdfs:comment>Baby and nursery equipment and children&apos;s clothes is a subcategory of clothing and accessories</rdfs:comment>
        <rdfs:isDefinedBy rdf:resource="https://www.theworldavatar.com/kg/ontopoi"/>
        <rdfs:label>Baby and nursery equipment and children&apos;s clothes</rdfs:label>
    </owl:Class>
    


    <!-- https://www.theworldavatar.com/kg/ontopoi/Bakeries -->


    <owl:Class rdf:about="https://www.theworldavatar.com/kg/ontopoi/Bakeries">
        <rdfs:subClassOf rdf:resource="https://www.theworldavatar.com/kg/ontopoi/Foodanddrinkandmultiitemretail"/>
        <rdfs:comment>Bakeries is a subcategory of food, drink and multi item retail</rdfs:comment>
        <rdfs:isDefinedBy rdf:resource="https://www.theworldavatar.com/kg/ontopoi"/>
        <rdfs:label>Bakeries</rdfs:label>
    </owl:Class>
    


    <!-- https://www.theworldavatar.com/kg/ontopoi/Bakingandconfectionery -->


    <owl:Class rdf:about="https://www.theworldavatar.com/kg/ontopoi/Bakingandconfectionery">
        <rdfs:subClassOf rdf:resource="https://www.theworldavatar.com/kg/ontopoi/Foodstuffs"/>
        <rdfs:comment>Baking and confectionery is a subcategory of foodstuffs</rdfs:comment>
        <rdfs:isDefinedBy rdf:resource="https://www.theworldavatar.com/kg/ontopoi"/>
        <rdfs:label>Baking and confectionery</rdfs:label>
    </owl:Class>
    


    <!-- https://www.theworldavatar.com/kg/ontopoi/Balletanddanceschools -->


    <owl:Class rdf:about="https://www.theworldavatar.com/kg/ontopoi/Balletanddanceschools">
        <rdfs:subClassOf rdf:resource="https://www.theworldavatar.com/kg/ontopoi/Recreationalandvocationaleducation"/>
        <rdfs:comment>Ballet and dance schools is a subcategory of recreational and vocational education</rdfs:comment>
        <rdfs:isDefinedBy rdf:resource="https://www.theworldavatar.com/kg/ontopoi"/>
        <rdfs:label>Ballet and dance schools</rdfs:label>
    </owl:Class>
    


    <!-- https://www.theworldavatar.com/kg/ontopoi/Banksandbuildingsocieties -->


    <owl:Class rdf:about="https://www.theworldavatar.com/kg/ontopoi/Banksandbuildingsocieties">
        <rdfs:subClassOf rdf:resource="https://www.theworldavatar.com/kg/ontopoi/Legalandfinancial"/>
        <rdfs:comment>Banks and building societies is a subcategory of legal and financial</rdfs:comment>
        <rdfs:isDefinedBy rdf:resource="https://www.theworldavatar.com/kg/ontopoi"/>
        <rdfs:label>Banks and building societies</rdfs:label>
    </owl:Class>
    


    <!-- https://www.theworldavatar.com/kg/ontopoi/Banquetingandfunctionrooms -->


    <owl:Class rdf:about="https://www.theworldavatar.com/kg/ontopoi/Banquetingandfunctionrooms">
        <rdfs:subClassOf rdf:resource="https://www.theworldavatar.com/kg/ontopoi/Eatinganddrinking"/>
        <rdfs:comment>Banqueting and function rooms is a subcategory of eating and drinking</rdfs:comment>
        <rdfs:isDefinedBy rdf:resource="https://www.theworldavatar.com/kg/ontopoi"/>
        <rdfs:label>Banqueting and function rooms</rdfs:label>
    </owl:Class>
    


    <!-- https://www.theworldavatar.com/kg/ontopoi/Bathroomfixturesandfittingsandsanitaryequipment -->


    <owl:Class rdf:about="https://www.theworldavatar.com/kg/ontopoi/Bathroomfixturesandfittingsandsanitaryequipment">
        <rdfs:subClassOf rdf:resource="https://www.theworldavatar.com/kg/ontopoi/Consumerproducts"/>
        <rdfs:comment>Bathroom fixtures, fittings and sanitary equipment is a subcategory of consumer products</rdfs:comment>
        <rdfs:isDefinedBy rdf:resource="https://www.theworldavatar.com/kg/ontopoi"/>
        <rdfs:label>Bathroom fixtures, fittings and sanitary equipment</rdfs:label>
    </owl:Class>
    


    <!-- https://www.theworldavatar.com/kg/ontopoi/Battlefields -->


    <owl:Class rdf:about="https://www.theworldavatar.com/kg/ontopoi/Battlefields">
        <rdfs:subClassOf rdf:resource="https://www.theworldavatar.com/kg/ontopoi/Historicalandcultural"/>
        <rdfs:comment>Battlefields is a subcategory of historical and cultural</rdfs:comment>
        <rdfs:isDefinedBy rdf:resource="https://www.theworldavatar.com/kg/ontopoi"/>
        <rdfs:label>Battlefields</rdfs:label>
    </owl:Class>
    


    <!-- https://www.theworldavatar.com/kg/ontopoi/Bearingandgearanddriveelements -->


    <owl:Class rdf:about="https://www.theworldavatar.com/kg/ontopoi/Bearingandgearanddriveelements">
        <rdfs:subClassOf rdf:resource="https://www.theworldavatar.com/kg/ontopoi/Industrialproducts"/>
        <rdfs:comment>Bearing, gear and drive elements is a subcategory of industrial products</rdfs:comment>
        <rdfs:isDefinedBy rdf:resource="https://www.theworldavatar.com/kg/ontopoi"/>
        <rdfs:label>Bearing, gear and drive elements</rdfs:label>
    </owl:Class>
    


    <!-- https://www.theworldavatar.com/kg/ontopoi/Beautyandhairdressingschools -->


    <owl:Class rdf:about="https://www.theworldavatar.com/kg/ontopoi/Beautyandhairdressingschools">
        <rdfs:subClassOf rdf:resource="https://www.theworldavatar.com/kg/ontopoi/Recreationalandvocationaleducation"/>
        <rdfs:comment>Beauty and hairdressing schools is a subcategory of recreational and vocational education</rdfs:comment>
        <rdfs:isDefinedBy rdf:resource="https://www.theworldavatar.com/kg/ontopoi"/>
        <rdfs:label>Beauty and hairdressing schools</rdfs:label>
    </owl:Class>
    


    <!-- https://www.theworldavatar.com/kg/ontopoi/Bedandbreakfastandbackpackeraccommodation -->


    <owl:Class rdf:about="https://www.theworldavatar.com/kg/ontopoi/Bedandbreakfastandbackpackeraccommodation">
        <rdfs:subClassOf rdf:resource="https://www.theworldavatar.com/kg/ontopoi/Accommodation"/>
        <rdfs:comment>Bed and breakfast and backpacker accommodation is a subcategory of accommodation</rdfs:comment>
        <rdfs:isDefinedBy rdf:resource="https://www.theworldavatar.com/kg/ontopoi"/>
        <rdfs:label>Bed and breakfast and backpacker accommodation</rdfs:label>
    </owl:Class>
    


    <!-- https://www.theworldavatar.com/kg/ontopoi/Bedsandbedding -->


    <owl:Class rdf:about="https://www.theworldavatar.com/kg/ontopoi/Bedsandbedding">
        <rdfs:subClassOf rdf:resource="https://www.theworldavatar.com/kg/ontopoi/Consumerproducts"/>
        <rdfs:comment>Beds and bedding is a subcategory of consumer products</rdfs:comment>
        <rdfs:isDefinedBy rdf:resource="https://www.theworldavatar.com/kg/ontopoi"/>
        <rdfs:label>Beds and bedding</rdfs:label>
    </owl:Class>
    


    <!-- https://www.theworldavatar.com/kg/ontopoi/Bee-keepers -->


    <owl:Class rdf:about="https://www.theworldavatar.com/kg/ontopoi/Bee-keepers">
        <rdfs:subClassOf rdf:resource="https://www.theworldavatar.com/kg/ontopoi/Farming"/>
        <rdfs:comment>Bee-keepers is a subcategory of farming</rdfs:comment>
        <rdfs:isDefinedBy rdf:resource="https://www.theworldavatar.com/kg/ontopoi"/>
        <rdfs:label>Bee-keepers</rdfs:label>
    </owl:Class>
    


    <!-- https://www.theworldavatar.com/kg/ontopoi/Bee-keepingsupplies -->


    <owl:Class rdf:about="https://www.theworldavatar.com/kg/ontopoi/Bee-keepingsupplies">
        <rdfs:subClassOf rdf:resource="https://www.theworldavatar.com/kg/ontopoi/Industrialproducts"/>
        <rdfs:comment>Bee-keeping supplies is a subcategory of industrial products</rdfs:comment>
        <rdfs:isDefinedBy rdf:resource="https://www.theworldavatar.com/kg/ontopoi"/>
        <rdfs:label>Bee-keeping supplies</rdfs:label>
    </owl:Class>
    


    <!-- https://www.theworldavatar.com/kg/ontopoi/Bingohalls -->


    <owl:Class rdf:about="https://www.theworldavatar.com/kg/ontopoi/Bingohalls">
        <rdfs:subClassOf rdf:resource="https://www.theworldavatar.com/kg/ontopoi/Gambling"/>
        <rdfs:comment>Bingo halls is a subcategory of gambling</rdfs:comment>
        <rdfs:isDefinedBy rdf:resource="https://www.theworldavatar.com/kg/ontopoi"/>
        <rdfs:label>Bingo halls</rdfs:label>
    </owl:Class>
    


    <!-- https://www.theworldavatar.com/kg/ontopoi/Birdreservesandcollectionsandsanctuaries -->


    <owl:Class rdf:about="https://www.theworldavatar.com/kg/ontopoi/Birdreservesandcollectionsandsanctuaries">
        <rdfs:subClassOf rdf:resource="https://www.theworldavatar.com/kg/ontopoi/Botanicalandzoological"/>
        <rdfs:comment>Bird reserves, collections and sanctuaries is a subcategory of botanical and zoological</rdfs:comment>
        <rdfs:isDefinedBy rdf:resource="https://www.theworldavatar.com/kg/ontopoi"/>
        <rdfs:label>Bird reserves, collections and sanctuaries</rdfs:label>
    </owl:Class>
    


    <!-- https://www.theworldavatar.com/kg/ontopoi/Bloodtransfusionservice -->


    <owl:Class rdf:about="https://www.theworldavatar.com/kg/ontopoi/Bloodtransfusionservice">
        <rdfs:subClassOf rdf:resource="https://www.theworldavatar.com/kg/ontopoi/Healthsupportservices"/>
        <rdfs:comment>Blood transfusion service is a subcategory of health support services</rdfs:comment>
        <rdfs:isDefinedBy rdf:resource="https://www.theworldavatar.com/kg/ontopoi"/>
        <rdfs:label>Blood transfusion service</rdfs:label>
    </owl:Class>
    


    <!-- https://www.theworldavatar.com/kg/ontopoi/Boathiringservices -->


    <owl:Class rdf:about="https://www.theworldavatar.com/kg/ontopoi/Boathiringservices">
        <rdfs:subClassOf rdf:resource="https://www.theworldavatar.com/kg/ontopoi/Hireservices"/>
        <rdfs:comment>Boat hiring services is a subcategory of hire services</rdfs:comment>
        <rdfs:isDefinedBy rdf:resource="https://www.theworldavatar.com/kg/ontopoi"/>
        <rdfs:label>Boat hiring services</rdfs:label>
    </owl:Class>
    


    <!-- https://www.theworldavatar.com/kg/ontopoi/Bodiesofwater -->


    <owl:Class rdf:about="https://www.theworldavatar.com/kg/ontopoi/Bodiesofwater">
        <rdfs:subClassOf rdf:resource="https://www.theworldavatar.com/kg/ontopoi/Attractions"/>
        <rdfs:comment>Bodies of water is a subcategory of attractions</rdfs:comment>
        <rdfs:isDefinedBy rdf:resource="https://www.theworldavatar.com/kg/ontopoi"/>
        <rdfs:label>Bodies of water</rdfs:label>
    </owl:Class>
    


    <!-- https://www.theworldavatar.com/kg/ontopoi/Bookmakers -->


    <owl:Class rdf:about="https://www.theworldavatar.com/kg/ontopoi/Bookmakers">
        <rdfs:subClassOf rdf:resource="https://www.theworldavatar.com/kg/ontopoi/Gambling"/>
        <rdfs:comment>Bookmakers is a subcategory of gambling</rdfs:comment>
        <rdfs:isDefinedBy rdf:resource="https://www.theworldavatar.com/kg/ontopoi"/>
        <rdfs:label>Bookmakers</rdfs:label>
    </owl:Class>
    


    <!-- https://www.theworldavatar.com/kg/ontopoi/Booksandmaps -->


    <owl:Class rdf:about="https://www.theworldavatar.com/kg/ontopoi/Booksandmaps">
        <rdfs:subClassOf rdf:resource="https://www.theworldavatar.com/kg/ontopoi/Householdandofficeandleisureandgarden"/>
        <rdfs:comment>Books and maps is a subcategory of household, office, leisure and garden</rdfs:comment>
        <rdfs:isDefinedBy rdf:resource="https://www.theworldavatar.com/kg/ontopoi"/>
        <rdfs:label>Books and maps</rdfs:label>
    </owl:Class>
    


    <!-- https://www.theworldavatar.com/kg/ontopoi/Botanicalandzoological -->


    <owl:Class rdf:about="https://www.theworldavatar.com/kg/ontopoi/Botanicalandzoological">
        <rdfs:subClassOf rdf:resource="https://www.theworldavatar.com/kg/ontopoi/Attractions"/>
        <rdfs:comment>Botanical and zoological is a subcategory of attractions</rdfs:comment>
        <rdfs:isDefinedBy rdf:resource="https://www.theworldavatar.com/kg/ontopoi"/>
        <rdfs:label>Botanical and zoological</rdfs:label>
    </owl:Class>
    


    <!-- https://www.theworldavatar.com/kg/ontopoi/Bouncycastlesandinflatableshire -->


    <owl:Class rdf:about="https://www.theworldavatar.com/kg/ontopoi/Bouncycastlesandinflatableshire">
        <rdfs:subClassOf rdf:resource="https://www.theworldavatar.com/kg/ontopoi/Hireservices"/>
        <rdfs:comment>Bouncy castles and inflatables hire is a subcategory of hire services</rdfs:comment>
        <rdfs:isDefinedBy rdf:resource="https://www.theworldavatar.com/kg/ontopoi"/>
        <rdfs:label>Bouncy castles and inflatables hire</rdfs:label>
    </owl:Class>
    


    <!-- https://www.theworldavatar.com/kg/ontopoi/Bowlingfacilities -->


    <owl:Class rdf:about="https://www.theworldavatar.com/kg/ontopoi/Bowlingfacilities">
        <rdfs:subClassOf rdf:resource="https://www.theworldavatar.com/kg/ontopoi/Sportscomplex"/>
        <rdfs:comment>Bowling facilities is a subcategory of sports complex</rdfs:comment>
        <rdfs:isDefinedBy rdf:resource="https://www.theworldavatar.com/kg/ontopoi"/>
        <rdfs:label>Bowling facilities</rdfs:label>
    </owl:Class>
    


    <!-- https://www.theworldavatar.com/kg/ontopoi/Bricksandtilesandclayandceramicproducts -->


    <owl:Class rdf:about="https://www.theworldavatar.com/kg/ontopoi/Bricksandtilesandclayandceramicproducts">
        <rdfs:subClassOf rdf:resource="https://www.theworldavatar.com/kg/ontopoi/Industrialproducts"/>
        <rdfs:comment>Bricks, tiles, clay and ceramic products is a subcategory of industrial products</rdfs:comment>
        <rdfs:isDefinedBy rdf:resource="https://www.theworldavatar.com/kg/ontopoi"/>
        <rdfs:label>Bricks, tiles, clay and ceramic products</rdfs:label>
    </owl:Class>
    


    <!-- https://www.theworldavatar.com/kg/ontopoi/Bridges -->


    <owl:Class rdf:about="https://www.theworldavatar.com/kg/ontopoi/Bridges">
        <rdfs:subClassOf rdf:resource="https://www.theworldavatar.com/kg/ontopoi/Roadandrail"/>
        <rdfs:comment>Bridges is a subcategory of road and rail</rdfs:comment>
        <rdfs:isDefinedBy rdf:resource="https://www.theworldavatar.com/kg/ontopoi"/>
        <rdfs:label>Bridges</rdfs:label>
    </owl:Class>
    


    <!-- https://www.theworldavatar.com/kg/ontopoi/Broadagerangeandsecondarystateschools -->


    <owl:Class rdf:about="https://www.theworldavatar.com/kg/ontopoi/Broadagerangeandsecondarystateschools">
        <rdfs:subClassOf rdf:resource="https://www.theworldavatar.com/kg/ontopoi/Primaryandsecondaryandtertiaryeducation"/>
        <rdfs:comment>Broad age range and secondary state schools is a subcategory of primary, secondary and tertiary education</rdfs:comment>
        <rdfs:isDefinedBy rdf:resource="https://www.theworldavatar.com/kg/ontopoi"/>
        <rdfs:label>Broad age range and secondary state schools</rdfs:label>
    </owl:Class>
    


    <!-- https://www.theworldavatar.com/kg/ontopoi/Brushes -->


    <owl:Class rdf:about="https://www.theworldavatar.com/kg/ontopoi/Brushes">
        <rdfs:subClassOf rdf:resource="https://www.theworldavatar.com/kg/ontopoi/Consumerproducts"/>
        <rdfs:comment>Brushes is a subcategory of consumer products</rdfs:comment>
        <rdfs:isDefinedBy rdf:resource="https://www.theworldavatar.com/kg/ontopoi"/>
        <rdfs:label>Brushes</rdfs:label>
    </owl:Class>
    


    <!-- https://www.theworldavatar.com/kg/ontopoi/Buildingandcomponentsuppliers -->


    <owl:Class rdf:about="https://www.theworldavatar.com/kg/ontopoi/Buildingandcomponentsuppliers">
        <rdfs:subClassOf rdf:resource="https://www.theworldavatar.com/kg/ontopoi/Constructionservices"/>
        <rdfs:comment>Building and component suppliers is a subcategory of construction services</rdfs:comment>
        <rdfs:isDefinedBy rdf:resource="https://www.theworldavatar.com/kg/ontopoi"/>
        <rdfs:label>Building and component suppliers</rdfs:label>
    </owl:Class>
    


    <!-- https://www.theworldavatar.com/kg/ontopoi/Buildingcontractors -->


    <owl:Class rdf:about="https://www.theworldavatar.com/kg/ontopoi/Buildingcontractors">
        <rdfs:subClassOf rdf:resource="https://www.theworldavatar.com/kg/ontopoi/Constructionservices"/>
        <rdfs:comment>Building contractors is a subcategory of construction services</rdfs:comment>
        <rdfs:isDefinedBy rdf:resource="https://www.theworldavatar.com/kg/ontopoi"/>
        <rdfs:label>Building contractors</rdfs:label>
    </owl:Class>
    


    <!-- https://www.theworldavatar.com/kg/ontopoi/Buildingrepairs -->


    <owl:Class rdf:about="https://www.theworldavatar.com/kg/ontopoi/Buildingrepairs">
        <rdfs:subClassOf rdf:resource="https://www.theworldavatar.com/kg/ontopoi/Repairandservicing"/>
        <rdfs:comment>Building repairs is a subcategory of repair and servicing</rdfs:comment>
        <rdfs:isDefinedBy rdf:resource="https://www.theworldavatar.com/kg/ontopoi"/>
        <rdfs:label>Building repairs</rdfs:label>
    </owl:Class>
    


    <!-- https://www.theworldavatar.com/kg/ontopoi/Busandcoachstationsanddepotsandcompanies -->


    <owl:Class rdf:about="https://www.theworldavatar.com/kg/ontopoi/Busandcoachstationsanddepotsandcompanies">
        <rdfs:subClassOf rdf:resource="https://www.theworldavatar.com/kg/ontopoi/Publictransportandstationsandinfrastructure"/>
        <rdfs:comment>Bus and coach stations, depots and companies is a subcategory of public transport, stations and infrastructure</rdfs:comment>
        <rdfs:isDefinedBy rdf:resource="https://www.theworldavatar.com/kg/ontopoi"/>
        <rdfs:label>Bus and coach stations, depots and companies</rdfs:label>
    </owl:Class>
    


    <!-- https://www.theworldavatar.com/kg/ontopoi/Business-relatedconsultants -->


    <owl:Class rdf:about="https://www.theworldavatar.com/kg/ontopoi/Business-relatedconsultants">
        <rdfs:subClassOf rdf:resource="https://www.theworldavatar.com/kg/ontopoi/Consultancies"/>
        <rdfs:comment>Business-related consultants is a subcategory of consultancies</rdfs:comment>
        <rdfs:isDefinedBy rdf:resource="https://www.theworldavatar.com/kg/ontopoi"/>
        <rdfs:label>Business-related consultants</rdfs:label>
    </owl:Class>
    


    <!-- https://www.theworldavatar.com/kg/ontopoi/Businessparksandindustrialestates -->


    <owl:Class rdf:about="https://www.theworldavatar.com/kg/ontopoi/Businessparksandindustrialestates">
        <rdfs:subClassOf rdf:resource="https://www.theworldavatar.com/kg/ontopoi/Industrialfeatures"/>
        <rdfs:comment>Business parks and industrial estates is a subcategory of industrial features</rdfs:comment>
        <rdfs:isDefinedBy rdf:resource="https://www.theworldavatar.com/kg/ontopoi"/>
        <rdfs:label>Business parks and industrial estates</rdfs:label>
    </owl:Class>
    


    <!-- https://www.theworldavatar.com/kg/ontopoi/Busstops -->


    <owl:Class rdf:about="https://www.theworldavatar.com/kg/ontopoi/Busstops">
        <rdfs:subClassOf rdf:resource="https://www.theworldavatar.com/kg/ontopoi/Bustransport"/>
        <rdfs:comment>Bus stops is a subcategory of bus transport</rdfs:comment>
        <rdfs:isDefinedBy rdf:resource="https://www.theworldavatar.com/kg/ontopoi"/>
        <rdfs:label>Bus stops</rdfs:label>
    </owl:Class>
    


    <!-- https://www.theworldavatar.com/kg/ontopoi/Bustransport -->


    <owl:Class rdf:about="https://www.theworldavatar.com/kg/ontopoi/Bustransport">
        <rdfs:subClassOf rdf:resource="https://www.theworldavatar.com/kg/ontopoi/Transport"/>
        <rdfs:comment>Bus transport is a subcategory of transport</rdfs:comment>
        <rdfs:isDefinedBy rdf:resource="https://www.theworldavatar.com/kg/ontopoi"/>
        <rdfs:label>Bus transport</rdfs:label>
    </owl:Class>
    


    <!-- https://www.theworldavatar.com/kg/ontopoi/Butchers -->


    <owl:Class rdf:about="https://www.theworldavatar.com/kg/ontopoi/Butchers">
        <rdfs:subClassOf rdf:resource="https://www.theworldavatar.com/kg/ontopoi/Foodanddrinkandmultiitemretail"/>
        <rdfs:comment>Butchers is a subcategory of food, drink and multi item retail</rdfs:comment>
        <rdfs:isDefinedBy rdf:resource="https://www.theworldavatar.com/kg/ontopoi"/>
        <rdfs:label>Butchers</rdfs:label>
    </owl:Class>
    


    <!-- https://www.theworldavatar.com/kg/ontopoi/Butterflyfarms -->


    <owl:Class rdf:about="https://www.theworldavatar.com/kg/ontopoi/Butterflyfarms">
        <rdfs:subClassOf rdf:resource="https://www.theworldavatar.com/kg/ontopoi/Botanicalandzoological"/>
        <rdfs:comment>Butterfly farms is a subcategory of botanical and zoological</rdfs:comment>
        <rdfs:isDefinedBy rdf:resource="https://www.theworldavatar.com/kg/ontopoi"/>
        <rdfs:label>Butterfly farms</rdfs:label>
    </owl:Class>
    


    <!-- https://www.theworldavatar.com/kg/ontopoi/CVwriters -->


    <owl:Class rdf:about="https://www.theworldavatar.com/kg/ontopoi/CVwriters">
        <rdfs:subClassOf rdf:resource="https://www.theworldavatar.com/kg/ontopoi/Personalandconsumerandotherservices"/>
        <rdfs:comment>Cv writers is a subcategory of personal, consumer and other services</rdfs:comment>
        <rdfs:isDefinedBy rdf:resource="https://www.theworldavatar.com/kg/ontopoi"/>
        <rdfs:label>CV writers</rdfs:label>
    </owl:Class>
    


    <!-- https://www.theworldavatar.com/kg/ontopoi/Cableandwireandfibreoptics -->


    <owl:Class rdf:about="https://www.theworldavatar.com/kg/ontopoi/Cableandwireandfibreoptics">
        <rdfs:subClassOf rdf:resource="https://www.theworldavatar.com/kg/ontopoi/Industrialproducts"/>
        <rdfs:comment>Cable, wire and fibre optics is a subcategory of industrial products</rdfs:comment>
        <rdfs:isDefinedBy rdf:resource="https://www.theworldavatar.com/kg/ontopoi"/>
        <rdfs:label>Cable, wire and fibre optics</rdfs:label>
    </owl:Class>
    


    <!-- https://www.theworldavatar.com/kg/ontopoi/Cafesandsnackbarsandtearooms -->


    <owl:Class rdf:about="https://www.theworldavatar.com/kg/ontopoi/Cafesandsnackbarsandtearooms">
        <rdfs:subClassOf rdf:resource="https://www.theworldavatar.com/kg/ontopoi/Eatinganddrinking"/>
        <rdfs:comment>Cafes, snack bars and tea rooms is a subcategory of eating and drinking</rdfs:comment>
        <rdfs:isDefinedBy rdf:resource="https://www.theworldavatar.com/kg/ontopoi"/>
        <rdfs:label>Cafes, snack bars and tea rooms</rdfs:label>
    </owl:Class>
    


    <!-- https://www.theworldavatar.com/kg/ontopoi/Campingandcaravanning -->


    <owl:Class rdf:about="https://www.theworldavatar.com/kg/ontopoi/Campingandcaravanning">
        <rdfs:subClassOf rdf:resource="https://www.theworldavatar.com/kg/ontopoi/Householdandofficeandleisureandgarden"/>
        <rdfs:comment>Camping and caravanning is a subcategory of household, office, leisure and garden</rdfs:comment>
        <rdfs:isDefinedBy rdf:resource="https://www.theworldavatar.com/kg/ontopoi"/>
        <rdfs:label>Camping and caravanning</rdfs:label>
    </owl:Class>
    


    <!-- https://www.theworldavatar.com/kg/ontopoi/Campingandcaravanningandmobilehomesandholidayparksandcentres -->


    <owl:Class rdf:about="https://www.theworldavatar.com/kg/ontopoi/Campingandcaravanningandmobilehomesandholidayparksandcentres">
        <rdfs:subClassOf rdf:resource="https://www.theworldavatar.com/kg/ontopoi/Accommodation"/>
        <rdfs:comment>Camping, caravanning, mobile homes, holiday parks and centres is a subcategory of accommodation</rdfs:comment>
        <rdfs:isDefinedBy rdf:resource="https://www.theworldavatar.com/kg/ontopoi"/>
        <rdfs:label>Camping, caravanning, mobile homes, holiday parks and centres</rdfs:label>
    </owl:Class>
    


    <!-- https://www.theworldavatar.com/kg/ontopoi/Candles -->


    <owl:Class rdf:about="https://www.theworldavatar.com/kg/ontopoi/Candles">
        <rdfs:subClassOf rdf:resource="https://www.theworldavatar.com/kg/ontopoi/Consumerproducts"/>
        <rdfs:comment>Candles is a subcategory of consumer products</rdfs:comment>
        <rdfs:isDefinedBy rdf:resource="https://www.theworldavatar.com/kg/ontopoi"/>
        <rdfs:label>Candles</rdfs:label>
    </owl:Class>
    


    <!-- https://www.theworldavatar.com/kg/ontopoi/Canvasgoods -->


    <owl:Class rdf:about="https://www.theworldavatar.com/kg/ontopoi/Canvasgoods">
        <rdfs:subClassOf rdf:resource="https://www.theworldavatar.com/kg/ontopoi/Consumerproducts"/>
        <rdfs:comment>Canvas goods is a subcategory of consumer products</rdfs:comment>
        <rdfs:isDefinedBy rdf:resource="https://www.theworldavatar.com/kg/ontopoi"/>
        <rdfs:label>Canvas goods</rdfs:label>
    </owl:Class>
    


    <!-- https://www.theworldavatar.com/kg/ontopoi/Careersofficesandarmedforcesrecruitment -->


    <owl:Class rdf:about="https://www.theworldavatar.com/kg/ontopoi/Careersofficesandarmedforcesrecruitment">
        <rdfs:subClassOf rdf:resource="https://www.theworldavatar.com/kg/ontopoi/Employmentandcareeragencies"/>
        <rdfs:comment>Careers offices and armed forces recruitment is a subcategory of employment and career agencies</rdfs:comment>
        <rdfs:isDefinedBy rdf:resource="https://www.theworldavatar.com/kg/ontopoi"/>
        <rdfs:label>Careers offices and armed forces recruitment</rdfs:label>
    </owl:Class>
    


    <!-- https://www.theworldavatar.com/kg/ontopoi/Carpetsandflooringandrugsandsoftfurnishings -->


    <owl:Class rdf:about="https://www.theworldavatar.com/kg/ontopoi/Carpetsandflooringandrugsandsoftfurnishings">
        <rdfs:subClassOf rdf:resource="https://www.theworldavatar.com/kg/ontopoi/Consumerproducts"/>
        <rdfs:comment>Carpets, flooring, rugs and soft furnishings is a subcategory of consumer products</rdfs:comment>
        <rdfs:isDefinedBy rdf:resource="https://www.theworldavatar.com/kg/ontopoi"/>
        <rdfs:label>Carpets, flooring, rugs and soft furnishings</rdfs:label>
    </owl:Class>
    


    <!-- https://www.theworldavatar.com/kg/ontopoi/Carpetsandrugsandsoftfurnishingsandneedlecraft -->


    <owl:Class rdf:about="https://www.theworldavatar.com/kg/ontopoi/Carpetsandrugsandsoftfurnishingsandneedlecraft">
        <rdfs:subClassOf rdf:resource="https://www.theworldavatar.com/kg/ontopoi/Householdandofficeandleisureandgarden"/>
        <rdfs:comment>Carpets, rugs, soft furnishings and needlecraft is a subcategory of household, office, leisure and garden</rdfs:comment>
        <rdfs:isDefinedBy rdf:resource="https://www.theworldavatar.com/kg/ontopoi"/>
        <rdfs:label>Carpets, rugs, soft furnishings and needlecraft</rdfs:label>
    </owl:Class>
    


    <!-- https://www.theworldavatar.com/kg/ontopoi/Carportsandsteelbuildings -->


    <owl:Class rdf:about="https://www.theworldavatar.com/kg/ontopoi/Carportsandsteelbuildings">
        <rdfs:subClassOf rdf:resource="https://www.theworldavatar.com/kg/ontopoi/Industrialproducts"/>
        <rdfs:comment>Car ports and steel buildings is a subcategory of industrial products</rdfs:comment>
        <rdfs:isDefinedBy rdf:resource="https://www.theworldavatar.com/kg/ontopoi"/>
        <rdfs:label>Car ports and steel buildings</rdfs:label>
    </owl:Class>
    


    <!-- https://www.theworldavatar.com/kg/ontopoi/Cashandcarry -->


    <owl:Class rdf:about="https://www.theworldavatar.com/kg/ontopoi/Cashandcarry">
        <rdfs:subClassOf rdf:resource="https://www.theworldavatar.com/kg/ontopoi/Foodanddrinkandmultiitemretail"/>
        <rdfs:comment>Cash and carry is a subcategory of food, drink and multi item retail</rdfs:comment>
        <rdfs:isDefinedBy rdf:resource="https://www.theworldavatar.com/kg/ontopoi"/>
        <rdfs:label>Cash and carry</rdfs:label>
    </owl:Class>
    


    <!-- https://www.theworldavatar.com/kg/ontopoi/Cashmachines -->


    <owl:Class rdf:about="https://www.theworldavatar.com/kg/ontopoi/Cashmachines">
        <rdfs:subClassOf rdf:resource="https://www.theworldavatar.com/kg/ontopoi/Legalandfinancial"/>
        <rdfs:comment>Cash machines is a subcategory of legal and financial</rdfs:comment>
        <rdfs:isDefinedBy rdf:resource="https://www.theworldavatar.com/kg/ontopoi"/>
        <rdfs:label>Cash machines</rdfs:label>
    </owl:Class>
    


    <!-- https://www.theworldavatar.com/kg/ontopoi/Casinos -->


    <owl:Class rdf:about="https://www.theworldavatar.com/kg/ontopoi/Casinos">
        <rdfs:subClassOf rdf:resource="https://www.theworldavatar.com/kg/ontopoi/Gambling"/>
        <rdfs:comment>Casinos is a subcategory of gambling</rdfs:comment>
        <rdfs:isDefinedBy rdf:resource="https://www.theworldavatar.com/kg/ontopoi"/>
        <rdfs:label>Casinos</rdfs:label>
    </owl:Class>
    


    <!-- https://www.theworldavatar.com/kg/ontopoi/Cateringandnon-specificfoodproducts -->


    <owl:Class rdf:about="https://www.theworldavatar.com/kg/ontopoi/Cateringandnon-specificfoodproducts">
        <rdfs:subClassOf rdf:resource="https://www.theworldavatar.com/kg/ontopoi/Foodstuffs"/>
        <rdfs:comment>Catering and non-specific food products is a subcategory of foodstuffs</rdfs:comment>
        <rdfs:isDefinedBy rdf:resource="https://www.theworldavatar.com/kg/ontopoi"/>
        <rdfs:label>Catering and non-specific food products</rdfs:label>
    </owl:Class>
    


    <!-- https://www.theworldavatar.com/kg/ontopoi/Cateringservices -->


    <owl:Class rdf:about="https://www.theworldavatar.com/kg/ontopoi/Cateringservices">
        <rdfs:subClassOf rdf:resource="https://www.theworldavatar.com/kg/ontopoi/Contractservices"/>
        <rdfs:comment>Catering services is a subcategory of contract services</rdfs:comment>
        <rdfs:isDefinedBy rdf:resource="https://www.theworldavatar.com/kg/ontopoi"/>
        <rdfs:label>Catering services</rdfs:label>
    </owl:Class>
    


    <!-- https://www.theworldavatar.com/kg/ontopoi/Cattlegrids -->


    <owl:Class rdf:about="https://www.theworldavatar.com/kg/ontopoi/Cattlegrids">
        <rdfs:subClassOf rdf:resource="https://www.theworldavatar.com/kg/ontopoi/Roadandrail"/>
        <rdfs:comment>Cattle grids is a subcategory of road and rail</rdfs:comment>
        <rdfs:isDefinedBy rdf:resource="https://www.theworldavatar.com/kg/ontopoi"/>
        <rdfs:label>Cattle grids</rdfs:label>
    </owl:Class>
    


    <!-- https://www.theworldavatar.com/kg/ontopoi/Cemeteriesandcrematoria -->


    <owl:Class rdf:about="https://www.theworldavatar.com/kg/ontopoi/Cemeteriesandcrematoria">
        <rdfs:subClassOf rdf:resource="https://www.theworldavatar.com/kg/ontopoi/Infrastructureandfacilities"/>
        <rdfs:comment>Cemeteries and crematoria is a subcategory of infrastructure and facilities</rdfs:comment>
        <rdfs:isDefinedBy rdf:resource="https://www.theworldavatar.com/kg/ontopoi"/>
        <rdfs:label>Cemeteries and crematoria</rdfs:label>
    </owl:Class>
    


    <!-- https://www.theworldavatar.com/kg/ontopoi/Centralandlocalgovernment -->


    <owl:Class rdf:about="https://www.theworldavatar.com/kg/ontopoi/Centralandlocalgovernment">
        <rdfs:subClassOf rdf:resource="https://www.theworldavatar.com/kg/ontopoi/Publicinfrastructure"/>
        <rdfs:comment>Central and local government is a subcategory of public infrastructure</rdfs:comment>
        <rdfs:isDefinedBy rdf:resource="https://www.theworldavatar.com/kg/ontopoi"/>
        <rdfs:label>Central and local government</rdfs:label>
    </owl:Class>
    


    <!-- https://www.theworldavatar.com/kg/ontopoi/Centralgovernment -->


    <owl:Class rdf:about="https://www.theworldavatar.com/kg/ontopoi/Centralgovernment">
        <rdfs:subClassOf rdf:resource="https://www.theworldavatar.com/kg/ontopoi/Centralandlocalgovernment"/>
        <rdfs:comment>Central government is a subcategory of central and local government</rdfs:comment>
        <rdfs:isDefinedBy rdf:resource="https://www.theworldavatar.com/kg/ontopoi"/>
        <rdfs:label>Central government</rdfs:label>
    </owl:Class>
    


    <!-- https://www.theworldavatar.com/kg/ontopoi/Charitableorganisations -->


    <owl:Class rdf:about="https://www.theworldavatar.com/kg/ontopoi/Charitableorganisations">
        <rdfs:subClassOf rdf:resource="https://www.theworldavatar.com/kg/ontopoi/Organisations"/>
        <rdfs:comment>Charitable organisations is a subcategory of organisations</rdfs:comment>
        <rdfs:isDefinedBy rdf:resource="https://www.theworldavatar.com/kg/ontopoi"/>
        <rdfs:label>Charitable organisations</rdfs:label>
    </owl:Class>
    


    <!-- https://www.theworldavatar.com/kg/ontopoi/Charityshops -->


    <owl:Class rdf:about="https://www.theworldavatar.com/kg/ontopoi/Charityshops">
        <rdfs:subClassOf rdf:resource="https://www.theworldavatar.com/kg/ontopoi/Householdandofficeandleisureandgarden"/>
        <rdfs:comment>Charity shops is a subcategory of household, office, leisure and garden</rdfs:comment>
        <rdfs:isDefinedBy rdf:resource="https://www.theworldavatar.com/kg/ontopoi"/>
        <rdfs:label>Charity shops</rdfs:label>
    </owl:Class>
    


    <!-- https://www.theworldavatar.com/kg/ontopoi/Chemicalengineers -->


    <owl:Class rdf:about="https://www.theworldavatar.com/kg/ontopoi/Chemicalengineers">
        <rdfs:subClassOf rdf:resource="https://www.theworldavatar.com/kg/ontopoi/Engineeringservices"/>
        <rdfs:comment>Chemical engineers is a subcategory of engineering services</rdfs:comment>
        <rdfs:isDefinedBy rdf:resource="https://www.theworldavatar.com/kg/ontopoi"/>
        <rdfs:label>Chemical engineers</rdfs:label>
    </owl:Class>
    


    <!-- https://www.theworldavatar.com/kg/ontopoi/Chemistsandpharmacies -->


    <owl:Class rdf:about="https://www.theworldavatar.com/kg/ontopoi/Chemistsandpharmacies">
        <rdfs:subClassOf rdf:resource="https://www.theworldavatar.com/kg/ontopoi/Healthpractitionersandestablishments"/>
        <rdfs:comment>Chemists and pharmacies is a subcategory of health practitioners and establishments</rdfs:comment>
        <rdfs:isDefinedBy rdf:resource="https://www.theworldavatar.com/kg/ontopoi"/>
        <rdfs:label>Chemists and pharmacies</rdfs:label>
    </owl:Class>
    


    <!-- https://www.theworldavatar.com/kg/ontopoi/Chequecashing -->


    <owl:Class rdf:about="https://www.theworldavatar.com/kg/ontopoi/Chequecashing">
        <rdfs:subClassOf rdf:resource="https://www.theworldavatar.com/kg/ontopoi/Legalandfinancial"/>
        <rdfs:comment>Cheque cashing is a subcategory of legal and financial</rdfs:comment>
        <rdfs:isDefinedBy rdf:resource="https://www.theworldavatar.com/kg/ontopoi"/>
        <rdfs:label>Cheque cashing</rdfs:label>
    </owl:Class>
    


    <!-- https://www.theworldavatar.com/kg/ontopoi/Childrenactivitycentres -->


    <owl:Class rdf:about="https://www.theworldavatar.com/kg/ontopoi/Childrenactivitycentres">
        <rdfs:subClassOf rdf:resource="https://www.theworldavatar.com/kg/ontopoi/Sportandentertainmentsupportservices"/>
        <rdfs:comment>Children&apos;s activity centres is a subcategory of sport and entertainment support services</rdfs:comment>
        <rdfs:isDefinedBy rdf:resource="https://www.theworldavatar.com/kg/ontopoi"/>
        <rdfs:label>Children&apos;s activity centres</rdfs:label>
    </owl:Class>
    


    <!-- https://www.theworldavatar.com/kg/ontopoi/Chinaandglassware -->


    <owl:Class rdf:about="https://www.theworldavatar.com/kg/ontopoi/Chinaandglassware">
        <rdfs:subClassOf rdf:resource="https://www.theworldavatar.com/kg/ontopoi/Consumerproducts"/>
        <rdfs:subClassOf rdf:resource="https://www.theworldavatar.com/kg/ontopoi/Householdandofficeandleisureandgarden"/>
        <rdfs:comment>China and glassware is a subcategory of consumer products</rdfs:comment>
        <rdfs:comment>China and glassware is a subcategory of household, office, leisure and garden</rdfs:comment>
        <rdfs:isDefinedBy rdf:resource="https://www.theworldavatar.com/kg/ontopoi"/>
        <rdfs:label>China and glassware</rdfs:label>
    </owl:Class>
    


    <!-- https://www.theworldavatar.com/kg/ontopoi/Cinemas -->


    <owl:Class rdf:about="https://www.theworldavatar.com/kg/ontopoi/Cinemas">
        <rdfs:subClassOf rdf:resource="https://www.theworldavatar.com/kg/ontopoi/Venuesandstageandscreen"/>
        <rdfs:comment>Cinemas is a subcategory of venues, stage and screen</rdfs:comment>
        <rdfs:isDefinedBy rdf:resource="https://www.theworldavatar.com/kg/ontopoi"/>
        <rdfs:label>Cinemas</rdfs:label>
    </owl:Class>
    


    <!-- https://www.theworldavatar.com/kg/ontopoi/Civilengineers -->


    <owl:Class rdf:about="https://www.theworldavatar.com/kg/ontopoi/Civilengineers">
        <rdfs:subClassOf rdf:resource="https://www.theworldavatar.com/kg/ontopoi/Engineeringservices"/>
        <rdfs:comment>Civil engineers is a subcategory of engineering services</rdfs:comment>
        <rdfs:isDefinedBy rdf:resource="https://www.theworldavatar.com/kg/ontopoi"/>
        <rdfs:label>Civil engineers</rdfs:label>
    </owl:Class>
    


    <!-- https://www.theworldavatar.com/kg/ontopoi/Cleaningequipmentandsupplies -->


    <owl:Class rdf:about="https://www.theworldavatar.com/kg/ontopoi/Cleaningequipmentandsupplies">
        <rdfs:subClassOf rdf:resource="https://www.theworldavatar.com/kg/ontopoi/Industrialproducts"/>
        <rdfs:comment>Cleaning equipment and supplies is a subcategory of industrial products</rdfs:comment>
        <rdfs:isDefinedBy rdf:resource="https://www.theworldavatar.com/kg/ontopoi"/>
        <rdfs:label>Cleaning equipment and supplies</rdfs:label>
    </owl:Class>
    


    <!-- https://www.theworldavatar.com/kg/ontopoi/Cleaningservices -->


    <owl:Class rdf:about="https://www.theworldavatar.com/kg/ontopoi/Cleaningservices">
        <rdfs:subClassOf rdf:resource="https://www.theworldavatar.com/kg/ontopoi/Personalandconsumerandotherservices"/>
        <rdfs:comment>Cleaning services is a subcategory of personal, consumer and other services</rdfs:comment>
        <rdfs:isDefinedBy rdf:resource="https://www.theworldavatar.com/kg/ontopoi"/>
        <rdfs:label>Cleaning services</rdfs:label>
    </owl:Class>
    


    <!-- https://www.theworldavatar.com/kg/ontopoi/Clearanceandsalvagedealers -->


    <owl:Class rdf:about="https://www.theworldavatar.com/kg/ontopoi/Clearanceandsalvagedealers">
        <rdfs:subClassOf rdf:resource="https://www.theworldavatar.com/kg/ontopoi/Recyclingservices"/>
        <rdfs:comment>Clearance and salvage dealers is a subcategory of recycling services</rdfs:comment>
        <rdfs:isDefinedBy rdf:resource="https://www.theworldavatar.com/kg/ontopoi"/>
        <rdfs:label>Clearance and salvage dealers</rdfs:label>
    </owl:Class>
    


    <!-- https://www.theworldavatar.com/kg/ontopoi/Climbingfacilities -->


    <owl:Class rdf:about="https://www.theworldavatar.com/kg/ontopoi/Climbingfacilities">
        <rdfs:subClassOf rdf:resource="https://www.theworldavatar.com/kg/ontopoi/Sportscomplex"/>
        <rdfs:comment>Climbing facilities is a subcategory of sports complex</rdfs:comment>
        <rdfs:isDefinedBy rdf:resource="https://www.theworldavatar.com/kg/ontopoi"/>
        <rdfs:label>Climbing facilities</rdfs:label>
    </owl:Class>
    


    <!-- https://www.theworldavatar.com/kg/ontopoi/Clinicsandhealthcentres -->


    <owl:Class rdf:about="https://www.theworldavatar.com/kg/ontopoi/Clinicsandhealthcentres">
        <rdfs:subClassOf rdf:resource="https://www.theworldavatar.com/kg/ontopoi/Healthpractitionersandestablishments"/>
        <rdfs:comment>Clinics and health centres is a subcategory of health practitioners and establishments</rdfs:comment>
        <rdfs:isDefinedBy rdf:resource="https://www.theworldavatar.com/kg/ontopoi"/>
        <rdfs:label>Clinics and health centres</rdfs:label>
    </owl:Class>
    


    <!-- https://www.theworldavatar.com/kg/ontopoi/Clothing -->


    <owl:Class rdf:about="https://www.theworldavatar.com/kg/ontopoi/Clothing">
        <rdfs:subClassOf rdf:resource="https://www.theworldavatar.com/kg/ontopoi/Clothingandaccessories"/>
        <rdfs:comment>Clothing is a subcategory of clothing and accessories</rdfs:comment>
        <rdfs:isDefinedBy rdf:resource="https://www.theworldavatar.com/kg/ontopoi"/>
        <rdfs:label>Clothing</rdfs:label>
    </owl:Class>
    


    <!-- https://www.theworldavatar.com/kg/ontopoi/Clothingandaccessories -->


    <owl:Class rdf:about="https://www.theworldavatar.com/kg/ontopoi/Clothingandaccessories">
        <rdfs:subClassOf rdf:resource="https://www.theworldavatar.com/kg/ontopoi/Retail"/>
        <rdfs:comment>Clothing and accessories is a subcategory of retail</rdfs:comment>
        <rdfs:isDefinedBy rdf:resource="https://www.theworldavatar.com/kg/ontopoi"/>
        <rdfs:label>Clothing and accessories</rdfs:label>
    </owl:Class>
    


    <!-- https://www.theworldavatar.com/kg/ontopoi/Clothingandcomponentsandaccessories -->


    <owl:Class rdf:about="https://www.theworldavatar.com/kg/ontopoi/Clothingandcomponentsandaccessories">
        <rdfs:subClassOf rdf:resource="https://www.theworldavatar.com/kg/ontopoi/Consumerproducts"/>
        <rdfs:comment>Clothing, components and accessories is a subcategory of consumer products</rdfs:comment>
        <rdfs:isDefinedBy rdf:resource="https://www.theworldavatar.com/kg/ontopoi"/>
        <rdfs:label>Clothing, components and accessories</rdfs:label>
    </owl:Class>
    


    <!-- https://www.theworldavatar.com/kg/ontopoi/Clothinghire -->


    <owl:Class rdf:about="https://www.theworldavatar.com/kg/ontopoi/Clothinghire">
        <rdfs:subClassOf rdf:resource="https://www.theworldavatar.com/kg/ontopoi/Hireservices"/>
        <rdfs:comment>Clothing hire is a subcategory of hire services</rdfs:comment>
        <rdfs:isDefinedBy rdf:resource="https://www.theworldavatar.com/kg/ontopoi"/>
        <rdfs:label>Clothing hire</rdfs:label>
    </owl:Class>
    


    <!-- https://www.theworldavatar.com/kg/ontopoi/Coalmining -->


    <owl:Class rdf:about="https://www.theworldavatar.com/kg/ontopoi/Coalmining">
        <rdfs:subClassOf rdf:resource="https://www.theworldavatar.com/kg/ontopoi/Extractiveindustries"/>
        <rdfs:comment>Coal mining is a subcategory of extractive industries</rdfs:comment>
        <rdfs:isDefinedBy rdf:resource="https://www.theworldavatar.com/kg/ontopoi"/>
        <rdfs:label>Coal mining</rdfs:label>
    </owl:Class>
    


    <!-- https://www.theworldavatar.com/kg/ontopoi/CoastalSafety -->


    <owl:Class rdf:about="https://www.theworldavatar.com/kg/ontopoi/CoastalSafety">
        <rdfs:subClassOf rdf:resource="https://www.theworldavatar.com/kg/ontopoi/Centralandlocalgovernment"/>
        <rdfs:comment>Coastal safety is a subcategory of central and local government</rdfs:comment>
        <rdfs:isDefinedBy rdf:resource="https://www.theworldavatar.com/kg/ontopoi"/>
        <rdfs:label>Coastal Safety</rdfs:label>
    </owl:Class>
    


    <!-- https://www.theworldavatar.com/kg/ontopoi/Coloursandchemicalsandwatersoftenersandsupplies -->


    <owl:Class rdf:about="https://www.theworldavatar.com/kg/ontopoi/Coloursandchemicalsandwatersoftenersandsupplies">
        <rdfs:subClassOf rdf:resource="https://www.theworldavatar.com/kg/ontopoi/Industrialproducts"/>
        <rdfs:comment>Colours, chemicals and water softeners and supplies is a subcategory of industrial products</rdfs:comment>
        <rdfs:isDefinedBy rdf:resource="https://www.theworldavatar.com/kg/ontopoi"/>
        <rdfs:label>Colours, chemicals and water softeners and supplies</rdfs:label>
    </owl:Class>
    


    <!-- https://www.theworldavatar.com/kg/ontopoi/Combatandlaserandpaintballgames -->


    <owl:Class rdf:about="https://www.theworldavatar.com/kg/ontopoi/Combatandlaserandpaintballgames">
        <rdfs:subClassOf rdf:resource="https://www.theworldavatar.com/kg/ontopoi/Outdoorpursuits"/>
        <rdfs:comment>Combat, laser and paintball games is a subcategory of outdoor pursuits</rdfs:comment>
        <rdfs:isDefinedBy rdf:resource="https://www.theworldavatar.com/kg/ontopoi"/>
        <rdfs:label>Combat, laser and paintball games</rdfs:label>
    </owl:Class>
    


    <!-- https://www.theworldavatar.com/kg/ontopoi/Comicbooks -->


    <owl:Class rdf:about="https://www.theworldavatar.com/kg/ontopoi/Comicbooks">
        <rdfs:subClassOf rdf:resource="https://www.theworldavatar.com/kg/ontopoi/Householdandofficeandleisureandgarden"/>
        <rdfs:comment>Comic books is a subcategory of household, office, leisure and garden</rdfs:comment>
        <rdfs:isDefinedBy rdf:resource="https://www.theworldavatar.com/kg/ontopoi"/>
        <rdfs:label>Comic books</rdfs:label>
    </owl:Class>
    


    <!-- https://www.theworldavatar.com/kg/ontopoi/Commercialpropertyletting -->


    <owl:Class rdf:about="https://www.theworldavatar.com/kg/ontopoi/Commercialpropertyletting">
        <rdfs:subClassOf rdf:resource="https://www.theworldavatar.com/kg/ontopoi/Propertyanddevelopmentservices"/>
        <rdfs:comment>Commercial property letting is a subcategory of property and development services</rdfs:comment>
        <rdfs:isDefinedBy rdf:resource="https://www.theworldavatar.com/kg/ontopoi"/>
        <rdfs:label>Commercial property letting</rdfs:label>
    </owl:Class>
    


    <!-- https://www.theworldavatar.com/kg/ontopoi/Commercialservices -->


    <owl:Class rdf:about="https://www.theworldavatar.com/kg/ontopoi/Commercialservices"/>
    


    <!-- https://www.theworldavatar.com/kg/ontopoi/Commoditydealers -->


    <owl:Class rdf:about="https://www.theworldavatar.com/kg/ontopoi/Commoditydealers">
        <rdfs:subClassOf rdf:resource="https://www.theworldavatar.com/kg/ontopoi/Legalandfinancial"/>
        <rdfs:comment>Commodity dealers is a subcategory of legal and financial</rdfs:comment>
        <rdfs:isDefinedBy rdf:resource="https://www.theworldavatar.com/kg/ontopoi"/>
        <rdfs:label>Commodity dealers</rdfs:label>
    </owl:Class>
    


    <!-- https://www.theworldavatar.com/kg/ontopoi/Commons -->


    <owl:Class rdf:about="https://www.theworldavatar.com/kg/ontopoi/Commons">
        <rdfs:subClassOf rdf:resource="https://www.theworldavatar.com/kg/ontopoi/Recreational"/>
        <rdfs:comment>Commons is a subcategory of recreational</rdfs:comment>
        <rdfs:isDefinedBy rdf:resource="https://www.theworldavatar.com/kg/ontopoi"/>
        <rdfs:label>Commons</rdfs:label>
    </owl:Class>
    


    <!-- https://www.theworldavatar.com/kg/ontopoi/Communitynetworksandprojects -->


    <owl:Class rdf:about="https://www.theworldavatar.com/kg/ontopoi/Communitynetworksandprojects">
        <rdfs:subClassOf rdf:resource="https://www.theworldavatar.com/kg/ontopoi/Organisations"/>
        <rdfs:comment>Community networks and projects is a subcategory of organisations</rdfs:comment>
        <rdfs:isDefinedBy rdf:resource="https://www.theworldavatar.com/kg/ontopoi"/>
        <rdfs:label>Community networks and projects</rdfs:label>
    </owl:Class>
    


    <!-- https://www.theworldavatar.com/kg/ontopoi/Companyregistrationandtrademarks -->


    <owl:Class rdf:about="https://www.theworldavatar.com/kg/ontopoi/Companyregistrationandtrademarks">
        <rdfs:subClassOf rdf:resource="https://www.theworldavatar.com/kg/ontopoi/Legalandfinancial"/>
        <rdfs:comment>Company registration and trademarks is a subcategory of legal and financial</rdfs:comment>
        <rdfs:isDefinedBy rdf:resource="https://www.theworldavatar.com/kg/ontopoi"/>
        <rdfs:label>Company registration and trademarks</rdfs:label>
    </owl:Class>
    


    <!-- https://www.theworldavatar.com/kg/ontopoi/Computerconsultants -->


    <owl:Class rdf:about="https://www.theworldavatar.com/kg/ontopoi/Computerconsultants">
        <rdfs:subClassOf rdf:resource="https://www.theworldavatar.com/kg/ontopoi/Consultancies"/>
        <rdfs:comment>Computer consultants is a subcategory of consultancies</rdfs:comment>
        <rdfs:isDefinedBy rdf:resource="https://www.theworldavatar.com/kg/ontopoi"/>
        <rdfs:label>Computer consultants</rdfs:label>
    </owl:Class>
    


    <!-- https://www.theworldavatar.com/kg/ontopoi/Computersecurity -->


    <owl:Class rdf:about="https://www.theworldavatar.com/kg/ontopoi/Computersecurity">
        <rdfs:subClassOf rdf:resource="https://www.theworldavatar.com/kg/ontopoi/ITandadvertisingandmarketingandmediaservices"/>
        <rdfs:comment>Computer security is a subcategory of it, advertising, marketing and media service s</rdfs:comment>
        <rdfs:isDefinedBy rdf:resource="https://www.theworldavatar.com/kg/ontopoi"/>
        <rdfs:label>Computer security</rdfs:label>
    </owl:Class>
    


    <!-- https://www.theworldavatar.com/kg/ontopoi/Computershops -->


    <owl:Class rdf:about="https://www.theworldavatar.com/kg/ontopoi/Computershops">
        <rdfs:subClassOf rdf:resource="https://www.theworldavatar.com/kg/ontopoi/Householdandofficeandleisureandgarden"/>
        <rdfs:comment>Computer shops is a subcategory of household, office, leisure and garden</rdfs:comment>
        <rdfs:isDefinedBy rdf:resource="https://www.theworldavatar.com/kg/ontopoi"/>
        <rdfs:label>Computer shops</rdfs:label>
    </owl:Class>
    


    <!-- https://www.theworldavatar.com/kg/ontopoi/Computersupplies -->


    <owl:Class rdf:about="https://www.theworldavatar.com/kg/ontopoi/Computersupplies">
        <rdfs:subClassOf rdf:resource="https://www.theworldavatar.com/kg/ontopoi/Householdandofficeandleisureandgarden"/>
        <rdfs:comment>Computer supplies is a subcategory of household, office, leisure and garden</rdfs:comment>
        <rdfs:isDefinedBy rdf:resource="https://www.theworldavatar.com/kg/ontopoi"/>
        <rdfs:label>Computer supplies</rdfs:label>
    </owl:Class>
    


    <!-- https://www.theworldavatar.com/kg/ontopoi/Computersystemsservices -->


    <owl:Class rdf:about="https://www.theworldavatar.com/kg/ontopoi/Computersystemsservices">
        <rdfs:subClassOf rdf:resource="https://www.theworldavatar.com/kg/ontopoi/ITandadvertisingandmarketingandmediaservices"/>
        <rdfs:comment>Computer systems services is a subcategory of it, advertising, marketing and media service s</rdfs:comment>
        <rdfs:isDefinedBy rdf:resource="https://www.theworldavatar.com/kg/ontopoi"/>
        <rdfs:label>Computer systems services</rdfs:label>
    </owl:Class>
    


    <!-- https://www.theworldavatar.com/kg/ontopoi/Concertorexhibitionorganisersandservices -->


    <owl:Class rdf:about="https://www.theworldavatar.com/kg/ontopoi/Concertorexhibitionorganisersandservices">
        <rdfs:subClassOf rdf:resource="https://www.theworldavatar.com/kg/ontopoi/ITandadvertisingandmarketingandmediaservices"/>
        <rdfs:comment>Concert or exhibition organisers and services is a subcategory of it, advertising, marketing and media service s</rdfs:comment>
        <rdfs:isDefinedBy rdf:resource="https://www.theworldavatar.com/kg/ontopoi"/>
        <rdfs:label>Concert or exhibition organisers and services</rdfs:label>
    </owl:Class>
    


    <!-- https://www.theworldavatar.com/kg/ontopoi/Concreteproducts -->


    <owl:Class rdf:about="https://www.theworldavatar.com/kg/ontopoi/Concreteproducts">
        <rdfs:subClassOf rdf:resource="https://www.theworldavatar.com/kg/ontopoi/Industrialproducts"/>
        <rdfs:comment>Concrete products is a subcategory of industrial products</rdfs:comment>
        <rdfs:isDefinedBy rdf:resource="https://www.theworldavatar.com/kg/ontopoi"/>
        <rdfs:label>Concrete products</rdfs:label>
    </owl:Class>
    


    <!-- https://www.theworldavatar.com/kg/ontopoi/Confectioners -->


    <owl:Class rdf:about="https://www.theworldavatar.com/kg/ontopoi/Confectioners">
        <rdfs:subClassOf rdf:resource="https://www.theworldavatar.com/kg/ontopoi/Foodanddrinkandmultiitemretail"/>
        <rdfs:comment>Confectioners is a subcategory of food, drink and multi item retail</rdfs:comment>
        <rdfs:isDefinedBy rdf:resource="https://www.theworldavatar.com/kg/ontopoi"/>
        <rdfs:label>Confectioners</rdfs:label>
    </owl:Class>
    


    <!-- https://www.theworldavatar.com/kg/ontopoi/Conferenceandexhibitioncentres -->


    <owl:Class rdf:about="https://www.theworldavatar.com/kg/ontopoi/Conferenceandexhibitioncentres">
        <rdfs:subClassOf rdf:resource="https://www.theworldavatar.com/kg/ontopoi/Venuesandstageandscreen"/>
        <rdfs:comment>Conference and exhibition centres is a subcategory of venues, stage and screen</rdfs:comment>
        <rdfs:isDefinedBy rdf:resource="https://www.theworldavatar.com/kg/ontopoi"/>
        <rdfs:label>Conference and exhibition centres</rdfs:label>
    </owl:Class>
    


    <!-- https://www.theworldavatar.com/kg/ontopoi/ConservationOrganisations -->


    <owl:Class rdf:about="https://www.theworldavatar.com/kg/ontopoi/ConservationOrganisations">
        <rdfs:subClassOf rdf:resource="https://www.theworldavatar.com/kg/ontopoi/Organisations"/>
        <rdfs:comment>Conservation organisations is a subcategory of organisations</rdfs:comment>
        <rdfs:isDefinedBy rdf:resource="https://www.theworldavatar.com/kg/ontopoi"/>
        <rdfs:label>Conservation Organisations</rdfs:label>
    </owl:Class>
    


    <!-- https://www.theworldavatar.com/kg/ontopoi/Conservatories -->


    <owl:Class rdf:about="https://www.theworldavatar.com/kg/ontopoi/Conservatories">
        <rdfs:subClassOf rdf:resource="https://www.theworldavatar.com/kg/ontopoi/Consumerproducts"/>
        <rdfs:comment>Conservatories is a subcategory of consumer products</rdfs:comment>
        <rdfs:isDefinedBy rdf:resource="https://www.theworldavatar.com/kg/ontopoi"/>
        <rdfs:label>Conservatories</rdfs:label>
    </owl:Class>
    


    <!-- https://www.theworldavatar.com/kg/ontopoi/Constructionandtoolhire -->


    <owl:Class rdf:about="https://www.theworldavatar.com/kg/ontopoi/Constructionandtoolhire">
        <rdfs:subClassOf rdf:resource="https://www.theworldavatar.com/kg/ontopoi/Hireservices"/>
        <rdfs:comment>Construction and tool hire is a subcategory of hire services</rdfs:comment>
        <rdfs:isDefinedBy rdf:resource="https://www.theworldavatar.com/kg/ontopoi"/>
        <rdfs:label>Construction and tool hire</rdfs:label>
    </owl:Class>
    


    <!-- https://www.theworldavatar.com/kg/ontopoi/Constructioncompletionservices -->


    <owl:Class rdf:about="https://www.theworldavatar.com/kg/ontopoi/Constructioncompletionservices">
        <rdfs:subClassOf rdf:resource="https://www.theworldavatar.com/kg/ontopoi/Constructionservices"/>
        <rdfs:comment>Construction completion services is a subcategory of construction services</rdfs:comment>
        <rdfs:isDefinedBy rdf:resource="https://www.theworldavatar.com/kg/ontopoi"/>
        <rdfs:label>Construction completion services</rdfs:label>
    </owl:Class>
    


    <!-- https://www.theworldavatar.com/kg/ontopoi/Constructionplant -->


    <owl:Class rdf:about="https://www.theworldavatar.com/kg/ontopoi/Constructionplant">
        <rdfs:subClassOf rdf:resource="https://www.theworldavatar.com/kg/ontopoi/Constructionservices"/>
        <rdfs:comment>Construction plant is a subcategory of construction services</rdfs:comment>
        <rdfs:isDefinedBy rdf:resource="https://www.theworldavatar.com/kg/ontopoi"/>
        <rdfs:label>Construction plant</rdfs:label>
    </owl:Class>
    


    <!-- https://www.theworldavatar.com/kg/ontopoi/Constructionserviceconsultants -->


    <owl:Class rdf:about="https://www.theworldavatar.com/kg/ontopoi/Constructionserviceconsultants">
        <rdfs:subClassOf rdf:resource="https://www.theworldavatar.com/kg/ontopoi/Consultancies"/>
        <rdfs:comment>Construction service consultants is a subcategory of consultancies</rdfs:comment>
        <rdfs:isDefinedBy rdf:resource="https://www.theworldavatar.com/kg/ontopoi"/>
        <rdfs:label>Construction service consultants</rdfs:label>
    </owl:Class>
    


    <!-- https://www.theworldavatar.com/kg/ontopoi/Constructionservices -->


    <owl:Class rdf:about="https://www.theworldavatar.com/kg/ontopoi/Constructionservices">
        <rdfs:subClassOf rdf:resource="https://www.theworldavatar.com/kg/ontopoi/Commercialservices"/>
        <rdfs:comment>Construction services is a subcategory of commercial services</rdfs:comment>
        <rdfs:isDefinedBy rdf:resource="https://www.theworldavatar.com/kg/ontopoi"/>
        <rdfs:label>Construction services</rdfs:label>
    </owl:Class>
    


    <!-- https://www.theworldavatar.com/kg/ontopoi/Consularservices -->


    <owl:Class rdf:about="https://www.theworldavatar.com/kg/ontopoi/Consularservices">
        <rdfs:subClassOf rdf:resource="https://www.theworldavatar.com/kg/ontopoi/Centralandlocalgovernment"/>
        <rdfs:comment>Consular services is a subcategory of central and local government</rdfs:comment>
        <rdfs:isDefinedBy rdf:resource="https://www.theworldavatar.com/kg/ontopoi"/>
        <rdfs:label>Consular services</rdfs:label>
    </owl:Class>
    


    <!-- https://www.theworldavatar.com/kg/ontopoi/Consultancies -->


    <owl:Class rdf:about="https://www.theworldavatar.com/kg/ontopoi/Consultancies">
        <rdfs:subClassOf rdf:resource="https://www.theworldavatar.com/kg/ontopoi/Commercialservices"/>
        <rdfs:comment>Consultancies is a subcategory of commercial services</rdfs:comment>
        <rdfs:isDefinedBy rdf:resource="https://www.theworldavatar.com/kg/ontopoi"/>
        <rdfs:label>Consultancies</rdfs:label>
    </owl:Class>
    


    <!-- https://www.theworldavatar.com/kg/ontopoi/Consumerproducts -->


    <owl:Class rdf:about="https://www.theworldavatar.com/kg/ontopoi/Consumerproducts">
        <rdfs:subClassOf rdf:resource="https://www.theworldavatar.com/kg/ontopoi/Manufacturingandproduction"/>
        <rdfs:comment>Consumer products is a subcategory of manufacturing and production</rdfs:comment>
        <rdfs:isDefinedBy rdf:resource="https://www.theworldavatar.com/kg/ontopoi"/>
        <rdfs:label>Consumer products</rdfs:label>
    </owl:Class>
    


    <!-- https://www.theworldavatar.com/kg/ontopoi/Containerandstorage -->


    <owl:Class rdf:about="https://www.theworldavatar.com/kg/ontopoi/Containerandstorage">
        <rdfs:subClassOf rdf:resource="https://www.theworldavatar.com/kg/ontopoi/Transportandstorageanddelivery"/>
        <rdfs:comment>Container and storage is a subcategory of transport, storage and delivery</rdfs:comment>
        <rdfs:isDefinedBy rdf:resource="https://www.theworldavatar.com/kg/ontopoi"/>
        <rdfs:label>Container and storage</rdfs:label>
    </owl:Class>
    


    <!-- https://www.theworldavatar.com/kg/ontopoi/Contractcleaningservices -->


    <owl:Class rdf:about="https://www.theworldavatar.com/kg/ontopoi/Contractcleaningservices">
        <rdfs:subClassOf rdf:resource="https://www.theworldavatar.com/kg/ontopoi/Contractservices"/>
        <rdfs:comment>Contract cleaning services is a subcategory of contract services</rdfs:comment>
        <rdfs:isDefinedBy rdf:resource="https://www.theworldavatar.com/kg/ontopoi"/>
        <rdfs:label>Contract cleaning services</rdfs:label>
    </owl:Class>
    


    <!-- https://www.theworldavatar.com/kg/ontopoi/Contractservices -->


    <owl:Class rdf:about="https://www.theworldavatar.com/kg/ontopoi/Contractservices">
        <rdfs:subClassOf rdf:resource="https://www.theworldavatar.com/kg/ontopoi/Commercialservices"/>
        <rdfs:comment>Contract services is a subcategory of commercial services</rdfs:comment>
        <rdfs:isDefinedBy rdf:resource="https://www.theworldavatar.com/kg/ontopoi"/>
        <rdfs:label>Contract services</rdfs:label>
    </owl:Class>
    


    <!-- https://www.theworldavatar.com/kg/ontopoi/Conveniencestoresandindependentsupermarkets -->


    <owl:Class rdf:about="https://www.theworldavatar.com/kg/ontopoi/Conveniencestoresandindependentsupermarkets">
        <rdfs:subClassOf rdf:resource="https://www.theworldavatar.com/kg/ontopoi/Foodanddrinkandmultiitemretail"/>
        <rdfs:comment>Convenience stores and independent supermarkets is a subcategory of food, drink and multi item retail</rdfs:comment>
        <rdfs:isDefinedBy rdf:resource="https://www.theworldavatar.com/kg/ontopoi"/>
        <rdfs:label>Convenience stores and independent supermarkets</rdfs:label>
    </owl:Class>
    


    <!-- https://www.theworldavatar.com/kg/ontopoi/Coolingandrefrigeration -->


    <owl:Class rdf:about="https://www.theworldavatar.com/kg/ontopoi/Coolingandrefrigeration">
        <rdfs:subClassOf rdf:resource="https://www.theworldavatar.com/kg/ontopoi/Industrialproducts"/>
        <rdfs:comment>Cooling and refrigeration is a subcategory of industrial products</rdfs:comment>
        <rdfs:isDefinedBy rdf:resource="https://www.theworldavatar.com/kg/ontopoi"/>
        <rdfs:label>Cooling and refrigeration</rdfs:label>
    </owl:Class>
    


    <!-- https://www.theworldavatar.com/kg/ontopoi/Copyrightandpatent -->


    <owl:Class rdf:about="https://www.theworldavatar.com/kg/ontopoi/Copyrightandpatent">
        <rdfs:subClassOf rdf:resource="https://www.theworldavatar.com/kg/ontopoi/Legalandfinancial"/>
        <rdfs:comment>Copyright and patent is a subcategory of legal and financial</rdfs:comment>
        <rdfs:isDefinedBy rdf:resource="https://www.theworldavatar.com/kg/ontopoi"/>
        <rdfs:label>Copyright and patent</rdfs:label>
    </owl:Class>
    


    <!-- https://www.theworldavatar.com/kg/ontopoi/Cosmeticsandtoiletriesandperfumes -->


    <owl:Class rdf:about="https://www.theworldavatar.com/kg/ontopoi/Cosmeticsandtoiletriesandperfumes">
        <rdfs:subClassOf rdf:resource="https://www.theworldavatar.com/kg/ontopoi/Consumerproducts"/>
        <rdfs:comment>Cosmetics, toiletries and perfumes is a subcategory of consumer products</rdfs:comment>
        <rdfs:isDefinedBy rdf:resource="https://www.theworldavatar.com/kg/ontopoi"/>
        <rdfs:label>Cosmetics, toiletries and perfumes</rdfs:label>
    </owl:Class>
    


    <!-- https://www.theworldavatar.com/kg/ontopoi/Cosmeticsandtoiletriesandperfumesandhairdressingsupplies -->


    <owl:Class rdf:about="https://www.theworldavatar.com/kg/ontopoi/Cosmeticsandtoiletriesandperfumesandhairdressingsupplies">
        <rdfs:subClassOf rdf:resource="https://www.theworldavatar.com/kg/ontopoi/Householdandofficeandleisureandgarden"/>
        <rdfs:comment>Cosmetics, toiletries, perfumes and hairdressing supplies is a subcategory of household, office, leisure and garden</rdfs:comment>
        <rdfs:isDefinedBy rdf:resource="https://www.theworldavatar.com/kg/ontopoi"/>
        <rdfs:label>Cosmetics, toiletries, perfumes and hairdressing supplies</rdfs:label>
    </owl:Class>
    


    <!-- https://www.theworldavatar.com/kg/ontopoi/Counsellingandadviceservices -->


    <owl:Class rdf:about="https://www.theworldavatar.com/kg/ontopoi/Counsellingandadviceservices">
        <rdfs:subClassOf rdf:resource="https://www.theworldavatar.com/kg/ontopoi/Healthsupportservices"/>
        <rdfs:comment>Counselling and advice services is a subcategory of health support services</rdfs:comment>
        <rdfs:isDefinedBy rdf:resource="https://www.theworldavatar.com/kg/ontopoi"/>
        <rdfs:label>Counselling and advice services</rdfs:label>
    </owl:Class>
    


    <!-- https://www.theworldavatar.com/kg/ontopoi/Countryandnationalparks -->


    <owl:Class rdf:about="https://www.theworldavatar.com/kg/ontopoi/Countryandnationalparks">
        <rdfs:subClassOf rdf:resource="https://www.theworldavatar.com/kg/ontopoi/Recreational"/>
        <rdfs:comment>Country and national parks is a subcategory of recreational</rdfs:comment>
        <rdfs:isDefinedBy rdf:resource="https://www.theworldavatar.com/kg/ontopoi"/>
        <rdfs:label>Country and national parks</rdfs:label>
    </owl:Class>
    


    <!-- https://www.theworldavatar.com/kg/ontopoi/Courieranddeliveryandmessenger -->


    <owl:Class rdf:about="https://www.theworldavatar.com/kg/ontopoi/Courieranddeliveryandmessenger">
        <rdfs:subClassOf rdf:resource="https://www.theworldavatar.com/kg/ontopoi/Transportandstorageanddelivery"/>
        <rdfs:comment>Courier, delivery and messenger is a subcategory of transport, storage and delivery</rdfs:comment>
        <rdfs:isDefinedBy rdf:resource="https://www.theworldavatar.com/kg/ontopoi"/>
        <rdfs:label>Courier, delivery and messenger</rdfs:label>
    </owl:Class>
    


    <!-- https://www.theworldavatar.com/kg/ontopoi/Courtsandcourtservicesandtribunals -->


    <owl:Class rdf:about="https://www.theworldavatar.com/kg/ontopoi/Courtsandcourtservicesandtribunals">
        <rdfs:subClassOf rdf:resource="https://www.theworldavatar.com/kg/ontopoi/Centralandlocalgovernment"/>
        <rdfs:comment>Courts, court services and tribunals is a subcategory of central and local government</rdfs:comment>
        <rdfs:isDefinedBy rdf:resource="https://www.theworldavatar.com/kg/ontopoi"/>
        <rdfs:label>Courts, court services and tribunals</rdfs:label>
    </owl:Class>
    


    <!-- https://www.theworldavatar.com/kg/ontopoi/Craftsupplies -->


    <owl:Class rdf:about="https://www.theworldavatar.com/kg/ontopoi/Craftsupplies">
        <rdfs:subClassOf rdf:resource="https://www.theworldavatar.com/kg/ontopoi/Householdandofficeandleisureandgarden"/>
        <rdfs:comment>Craft supplies is a subcategory of household, office, leisure and garden</rdfs:comment>
        <rdfs:isDefinedBy rdf:resource="https://www.theworldavatar.com/kg/ontopoi"/>
        <rdfs:label>Craft supplies</rdfs:label>
    </owl:Class>
    


    <!-- https://www.theworldavatar.com/kg/ontopoi/Creditreferenceagencies -->


    <owl:Class rdf:about="https://www.theworldavatar.com/kg/ontopoi/Creditreferenceagencies">
        <rdfs:subClassOf rdf:resource="https://www.theworldavatar.com/kg/ontopoi/Legalandfinancial"/>
        <rdfs:comment>Credit reference agencies is a subcategory of legal and financial</rdfs:comment>
        <rdfs:isDefinedBy rdf:resource="https://www.theworldavatar.com/kg/ontopoi"/>
        <rdfs:label>Credit reference agencies</rdfs:label>
    </owl:Class>
    


    <!-- https://www.theworldavatar.com/kg/ontopoi/Currencyconversionandmoneytransfers -->


    <owl:Class rdf:about="https://www.theworldavatar.com/kg/ontopoi/Currencyconversionandmoneytransfers">
        <rdfs:subClassOf rdf:resource="https://www.theworldavatar.com/kg/ontopoi/Legalandfinancial"/>
        <rdfs:comment>Currency conversion and money transfers is a subcategory of legal and financial</rdfs:comment>
        <rdfs:isDefinedBy rdf:resource="https://www.theworldavatar.com/kg/ontopoi"/>
        <rdfs:label>Currency conversion and money transfers</rdfs:label>
    </owl:Class>
    


    <!-- https://www.theworldavatar.com/kg/ontopoi/Curtainsandblinds -->


    <owl:Class rdf:about="https://www.theworldavatar.com/kg/ontopoi/Curtainsandblinds">
        <rdfs:subClassOf rdf:resource="https://www.theworldavatar.com/kg/ontopoi/Consumerproducts"/>
        <rdfs:comment>Curtains and blinds is a subcategory of consumer products</rdfs:comment>
        <rdfs:isDefinedBy rdf:resource="https://www.theworldavatar.com/kg/ontopoi"/>
        <rdfs:label>Curtains and blinds</rdfs:label>
    </owl:Class>
    


    <!-- https://www.theworldavatar.com/kg/ontopoi/Customerservicecentres -->


    <owl:Class rdf:about="https://www.theworldavatar.com/kg/ontopoi/Customerservicecentres">
        <rdfs:subClassOf rdf:resource="https://www.theworldavatar.com/kg/ontopoi/Personalandconsumerandotherservices"/>
        <rdfs:comment>Customer service centres is a subcategory of personal, consumer and other services</rdfs:comment>
        <rdfs:isDefinedBy rdf:resource="https://www.theworldavatar.com/kg/ontopoi"/>
        <rdfs:label>Customer service centres</rdfs:label>
    </owl:Class>
    


    <!-- https://www.theworldavatar.com/kg/ontopoi/Cutleryandtableware -->


    <owl:Class rdf:about="https://www.theworldavatar.com/kg/ontopoi/Cutleryandtableware">
        <rdfs:subClassOf rdf:resource="https://www.theworldavatar.com/kg/ontopoi/Consumerproducts"/>
        <rdfs:comment>Cutlery and tableware is a subcategory of consumer products</rdfs:comment>
        <rdfs:isDefinedBy rdf:resource="https://www.theworldavatar.com/kg/ontopoi"/>
        <rdfs:label>Cutlery and tableware</rdfs:label>
    </owl:Class>
    


    <!-- https://www.theworldavatar.com/kg/ontopoi/Cuttinganddrillingandweldingservices -->


    <owl:Class rdf:about="https://www.theworldavatar.com/kg/ontopoi/Cuttinganddrillingandweldingservices">
        <rdfs:subClassOf rdf:resource="https://www.theworldavatar.com/kg/ontopoi/Constructionservices"/>
        <rdfs:comment>Cutting, drilling and welding services is a subcategory of construction services</rdfs:comment>
        <rdfs:isDefinedBy rdf:resource="https://www.theworldavatar.com/kg/ontopoi"/>
        <rdfs:label>Cutting, drilling and welding services</rdfs:label>
    </owl:Class>
    


    <!-- https://www.theworldavatar.com/kg/ontopoi/Cyclesandaccessories -->


    <owl:Class rdf:about="https://www.theworldavatar.com/kg/ontopoi/Cyclesandaccessories">
        <rdfs:subClassOf rdf:resource="https://www.theworldavatar.com/kg/ontopoi/Householdandofficeandleisureandgarden"/>
        <rdfs:comment>Cycles and accessories is a subcategory of household, office, leisure and garden</rdfs:comment>
        <rdfs:isDefinedBy rdf:resource="https://www.theworldavatar.com/kg/ontopoi"/>
        <rdfs:label>Cycles and accessories</rdfs:label>
    </owl:Class>
    


    <!-- https://www.theworldavatar.com/kg/ontopoi/DIYandhomeimprovement -->


    <owl:Class rdf:about="https://www.theworldavatar.com/kg/ontopoi/DIYandhomeimprovement">
        <rdfs:subClassOf rdf:resource="https://www.theworldavatar.com/kg/ontopoi/Householdandofficeandleisureandgarden"/>
        <rdfs:comment>Diy and home improvement is a subcategory of household, office, leisure and garden</rdfs:comment>
        <rdfs:isDefinedBy rdf:resource="https://www.theworldavatar.com/kg/ontopoi"/>
        <rdfs:label>DIY and home improvement</rdfs:label>
    </owl:Class>
    


    <!-- https://www.theworldavatar.com/kg/ontopoi/Dairyfarming -->


    <owl:Class rdf:about="https://www.theworldavatar.com/kg/ontopoi/Dairyfarming">
        <rdfs:subClassOf rdf:resource="https://www.theworldavatar.com/kg/ontopoi/Farming"/>
        <rdfs:comment>Dairy farming is a subcategory of farming</rdfs:comment>
        <rdfs:isDefinedBy rdf:resource="https://www.theworldavatar.com/kg/ontopoi"/>
        <rdfs:label>Dairy farming</rdfs:label>
    </owl:Class>
    


    <!-- https://www.theworldavatar.com/kg/ontopoi/Dairyproducts -->


    <owl:Class rdf:about="https://www.theworldavatar.com/kg/ontopoi/Dairyproducts">
        <rdfs:subClassOf rdf:resource="https://www.theworldavatar.com/kg/ontopoi/Foodstuffs"/>
        <rdfs:comment>Dairy products is a subcategory of foodstuffs</rdfs:comment>
        <rdfs:isDefinedBy rdf:resource="https://www.theworldavatar.com/kg/ontopoi"/>
        <rdfs:label>Dairy products</rdfs:label>
    </owl:Class>
    


    <!-- https://www.theworldavatar.com/kg/ontopoi/Databaseservices -->


    <owl:Class rdf:about="https://www.theworldavatar.com/kg/ontopoi/Databaseservices">
        <rdfs:subClassOf rdf:resource="https://www.theworldavatar.com/kg/ontopoi/ITandadvertisingandmarketingandmediaservices"/>
        <rdfs:comment>Database services is a subcategory of it, advertising, marketing and media service s</rdfs:comment>
        <rdfs:isDefinedBy rdf:resource="https://www.theworldavatar.com/kg/ontopoi"/>
        <rdfs:label>Database services</rdfs:label>
    </owl:Class>
    


    <!-- https://www.theworldavatar.com/kg/ontopoi/DayandCareCentres -->


    <owl:Class rdf:about="https://www.theworldavatar.com/kg/ontopoi/DayandCareCentres">
        <rdfs:subClassOf rdf:resource="https://www.theworldavatar.com/kg/ontopoi/Healthpractitionersandestablishments"/>
        <rdfs:comment>Day and care centres is a subcategory of health practitioners and establishments</rdfs:comment>
        <rdfs:isDefinedBy rdf:resource="https://www.theworldavatar.com/kg/ontopoi"/>
        <rdfs:label>Day and Care Centres</rdfs:label>
    </owl:Class>
    


    <!-- https://www.theworldavatar.com/kg/ontopoi/Debtcollectingagencies -->


    <owl:Class rdf:about="https://www.theworldavatar.com/kg/ontopoi/Debtcollectingagencies">
        <rdfs:subClassOf rdf:resource="https://www.theworldavatar.com/kg/ontopoi/Legalandfinancial"/>
        <rdfs:comment>Debt collecting agencies is a subcategory of legal and financial</rdfs:comment>
        <rdfs:isDefinedBy rdf:resource="https://www.theworldavatar.com/kg/ontopoi"/>
        <rdfs:label>Debt collecting agencies</rdfs:label>
    </owl:Class>
    


    <!-- https://www.theworldavatar.com/kg/ontopoi/Delicatessens -->


    <owl:Class rdf:about="https://www.theworldavatar.com/kg/ontopoi/Delicatessens">
        <rdfs:subClassOf rdf:resource="https://www.theworldavatar.com/kg/ontopoi/Foodanddrinkandmultiitemretail"/>
        <rdfs:comment>Delicatessens is a subcategory of food, drink and multi item retail</rdfs:comment>
        <rdfs:isDefinedBy rdf:resource="https://www.theworldavatar.com/kg/ontopoi"/>
        <rdfs:label>Delicatessens</rdfs:label>
    </owl:Class>
    


    <!-- https://www.theworldavatar.com/kg/ontopoi/Demolitionservices -->


    <owl:Class rdf:about="https://www.theworldavatar.com/kg/ontopoi/Demolitionservices">
        <rdfs:subClassOf rdf:resource="https://www.theworldavatar.com/kg/ontopoi/Constructionservices"/>
        <rdfs:comment>Demolition services is a subcategory of construction services</rdfs:comment>
        <rdfs:isDefinedBy rdf:resource="https://www.theworldavatar.com/kg/ontopoi"/>
        <rdfs:label>Demolition services</rdfs:label>
    </owl:Class>
    


    <!-- https://www.theworldavatar.com/kg/ontopoi/Dentalandmedicallaboratories -->


    <owl:Class rdf:about="https://www.theworldavatar.com/kg/ontopoi/Dentalandmedicallaboratories">
        <rdfs:subClassOf rdf:resource="https://www.theworldavatar.com/kg/ontopoi/Healthpractitionersandestablishments"/>
        <rdfs:comment>Dental and medical laboratories is a subcategory of health practitioners and establishments</rdfs:comment>
        <rdfs:isDefinedBy rdf:resource="https://www.theworldavatar.com/kg/ontopoi"/>
        <rdfs:label>Dental and medical laboratories</rdfs:label>
    </owl:Class>
    


    <!-- https://www.theworldavatar.com/kg/ontopoi/Dentalsurgeries -->


    <owl:Class rdf:about="https://www.theworldavatar.com/kg/ontopoi/Dentalsurgeries">
        <rdfs:subClassOf rdf:resource="https://www.theworldavatar.com/kg/ontopoi/Healthpractitionersandestablishments"/>
        <rdfs:comment>Dental surgeries is a subcategory of health practitioners and establishments</rdfs:comment>
        <rdfs:isDefinedBy rdf:resource="https://www.theworldavatar.com/kg/ontopoi"/>
        <rdfs:label>Dental surgeries</rdfs:label>
    </owl:Class>
    


    <!-- https://www.theworldavatar.com/kg/ontopoi/Dentaltechnicians -->


    <owl:Class rdf:about="https://www.theworldavatar.com/kg/ontopoi/Dentaltechnicians">
        <rdfs:subClassOf rdf:resource="https://www.theworldavatar.com/kg/ontopoi/Healthpractitionersandestablishments"/>
        <rdfs:comment>Dental technicians is a subcategory of health practitioners and establishments</rdfs:comment>
        <rdfs:isDefinedBy rdf:resource="https://www.theworldavatar.com/kg/ontopoi"/>
        <rdfs:label>Dental technicians</rdfs:label>
    </owl:Class>
    


    <!-- https://www.theworldavatar.com/kg/ontopoi/Departmentstores -->


    <owl:Class rdf:about="https://www.theworldavatar.com/kg/ontopoi/Departmentstores">
        <rdfs:subClassOf rdf:resource="https://www.theworldavatar.com/kg/ontopoi/Householdandofficeandleisureandgarden"/>
        <rdfs:comment>Department stores is a subcategory of household, office, leisure and garden</rdfs:comment>
        <rdfs:isDefinedBy rdf:resource="https://www.theworldavatar.com/kg/ontopoi"/>
        <rdfs:label>Department stores</rdfs:label>
    </owl:Class>
    


    <!-- https://www.theworldavatar.com/kg/ontopoi/Designatedscenicfeatures -->


    <owl:Class rdf:about="https://www.theworldavatar.com/kg/ontopoi/Designatedscenicfeatures">
        <rdfs:subClassOf rdf:resource="https://www.theworldavatar.com/kg/ontopoi/Landscapefeatures"/>
        <rdfs:comment>Designated scenic features is a subcategory of landscape features</rdfs:comment>
        <rdfs:isDefinedBy rdf:resource="https://www.theworldavatar.com/kg/ontopoi"/>
        <rdfs:label>Designated scenic features</rdfs:label>
    </owl:Class>
    


    <!-- https://www.theworldavatar.com/kg/ontopoi/Designservices -->


    <owl:Class rdf:about="https://www.theworldavatar.com/kg/ontopoi/Designservices">
        <rdfs:subClassOf rdf:resource="https://www.theworldavatar.com/kg/ontopoi/Researchanddesign"/>
        <rdfs:comment>Design services is a subcategory of research and design</rdfs:comment>
        <rdfs:isDefinedBy rdf:resource="https://www.theworldavatar.com/kg/ontopoi"/>
        <rdfs:label>Design services</rdfs:label>
    </owl:Class>
    


    <!-- https://www.theworldavatar.com/kg/ontopoi/Desktoppublishingservices -->


    <owl:Class rdf:about="https://www.theworldavatar.com/kg/ontopoi/Desktoppublishingservices">
        <rdfs:subClassOf rdf:resource="https://www.theworldavatar.com/kg/ontopoi/ITandadvertisingandmarketingandmediaservices"/>
        <rdfs:comment>Desktop publishing services is a subcategory of it, advertising, marketing and media service s</rdfs:comment>
        <rdfs:isDefinedBy rdf:resource="https://www.theworldavatar.com/kg/ontopoi"/>
        <rdfs:label>Desktop publishing services</rdfs:label>
    </owl:Class>
    


    <!-- https://www.theworldavatar.com/kg/ontopoi/Detectiveandinvestigationagencies -->


    <owl:Class rdf:about="https://www.theworldavatar.com/kg/ontopoi/Detectiveandinvestigationagencies">
        <rdfs:subClassOf rdf:resource="https://www.theworldavatar.com/kg/ontopoi/Personalandconsumerandotherservices"/>
        <rdfs:comment>Detective and investigation agencies is a subcategory of personal, consumer and other services</rdfs:comment>
        <rdfs:isDefinedBy rdf:resource="https://www.theworldavatar.com/kg/ontopoi"/>
        <rdfs:label>Detective and investigation agencies</rdfs:label>
    </owl:Class>
    


    <!-- https://www.theworldavatar.com/kg/ontopoi/Dieticiansandnutritionists -->


    <owl:Class rdf:about="https://www.theworldavatar.com/kg/ontopoi/Dieticiansandnutritionists">
        <rdfs:subClassOf rdf:resource="https://www.theworldavatar.com/kg/ontopoi/Healthpractitionersandestablishments"/>
        <rdfs:comment>Dieticians and nutritionists is a subcategory of health practitioners and establishments</rdfs:comment>
        <rdfs:isDefinedBy rdf:resource="https://www.theworldavatar.com/kg/ontopoi"/>
        <rdfs:label>Dieticians and nutritionists</rdfs:label>
    </owl:Class>
    


    <!-- https://www.theworldavatar.com/kg/ontopoi/Disabilityandmobilityequipment -->


    <owl:Class rdf:about="https://www.theworldavatar.com/kg/ontopoi/Disabilityandmobilityequipment">
        <rdfs:subClassOf rdf:resource="https://www.theworldavatar.com/kg/ontopoi/Consumerproducts"/>
        <rdfs:comment>Disability and mobility equipment is a subcategory of consumer products</rdfs:comment>
        <rdfs:isDefinedBy rdf:resource="https://www.theworldavatar.com/kg/ontopoi"/>
        <rdfs:label>Disability and mobility equipment</rdfs:label>
    </owl:Class>
    


    <!-- https://www.theworldavatar.com/kg/ontopoi/Discountstores -->


    <owl:Class rdf:about="https://www.theworldavatar.com/kg/ontopoi/Discountstores">
        <rdfs:subClassOf rdf:resource="https://www.theworldavatar.com/kg/ontopoi/Householdandofficeandleisureandgarden"/>
        <rdfs:comment>Discount stores is a subcategory of household, office, leisure and garden</rdfs:comment>
        <rdfs:isDefinedBy rdf:resource="https://www.theworldavatar.com/kg/ontopoi"/>
        <rdfs:label>Discount stores</rdfs:label>
    </owl:Class>
    


    <!-- https://www.theworldavatar.com/kg/ontopoi/Displayandwindowdressers -->


    <owl:Class rdf:about="https://www.theworldavatar.com/kg/ontopoi/Displayandwindowdressers">
        <rdfs:subClassOf rdf:resource="https://www.theworldavatar.com/kg/ontopoi/Contractservices"/>
        <rdfs:comment>Display and window dressers is a subcategory of contract services</rdfs:comment>
        <rdfs:isDefinedBy rdf:resource="https://www.theworldavatar.com/kg/ontopoi"/>
        <rdfs:label>Display and window dressers</rdfs:label>
    </owl:Class>
    


    <!-- https://www.theworldavatar.com/kg/ontopoi/Disposableproducts -->


    <owl:Class rdf:about="https://www.theworldavatar.com/kg/ontopoi/Disposableproducts">
        <rdfs:subClassOf rdf:resource="https://www.theworldavatar.com/kg/ontopoi/Consumerproducts"/>
        <rdfs:comment>Disposable products is a subcategory of consumer products</rdfs:comment>
        <rdfs:isDefinedBy rdf:resource="https://www.theworldavatar.com/kg/ontopoi"/>
        <rdfs:label>Disposable products</rdfs:label>
    </owl:Class>
    


    <!-- https://www.theworldavatar.com/kg/ontopoi/Distributionandhaulage -->


    <owl:Class rdf:about="https://www.theworldavatar.com/kg/ontopoi/Distributionandhaulage">
        <rdfs:subClassOf rdf:resource="https://www.theworldavatar.com/kg/ontopoi/Transportandstorageanddelivery"/>
        <rdfs:comment>Distribution and haulage is a subcategory of transport, storage and delivery</rdfs:comment>
        <rdfs:isDefinedBy rdf:resource="https://www.theworldavatar.com/kg/ontopoi"/>
        <rdfs:label>Distribution and haulage</rdfs:label>
    </owl:Class>
    


    <!-- https://www.theworldavatar.com/kg/ontopoi/Divingschools -->


    <owl:Class rdf:about="https://www.theworldavatar.com/kg/ontopoi/Divingschools">
        <rdfs:subClassOf rdf:resource="https://www.theworldavatar.com/kg/ontopoi/Recreationalandvocationaleducation"/>
        <rdfs:comment>Diving schools is a subcategory of recreational and vocational education</rdfs:comment>
        <rdfs:isDefinedBy rdf:resource="https://www.theworldavatar.com/kg/ontopoi"/>
        <rdfs:label>Diving schools</rdfs:label>
    </owl:Class>
    


    <!-- https://www.theworldavatar.com/kg/ontopoi/Divingservices -->


    <owl:Class rdf:about="https://www.theworldavatar.com/kg/ontopoi/Divingservices">
        <rdfs:subClassOf rdf:resource="https://www.theworldavatar.com/kg/ontopoi/Constructionservices"/>
        <rdfs:comment>Diving services is a subcategory of construction services</rdfs:comment>
        <rdfs:isDefinedBy rdf:resource="https://www.theworldavatar.com/kg/ontopoi"/>
        <rdfs:label>Diving services</rdfs:label>
    </owl:Class>
    


    <!-- https://www.theworldavatar.com/kg/ontopoi/Doctorssurgeries -->


    <owl:Class rdf:about="https://www.theworldavatar.com/kg/ontopoi/Doctorssurgeries">
        <rdfs:subClassOf rdf:resource="https://www.theworldavatar.com/kg/ontopoi/Healthpractitionersandestablishments"/>
        <rdfs:comment>Doctors surgeries is a subcategory of health practitioners and establishments</rdfs:comment>
        <rdfs:isDefinedBy rdf:resource="https://www.theworldavatar.com/kg/ontopoi"/>
        <rdfs:label>Doctors surgeries</rdfs:label>
    </owl:Class>
    


    <!-- https://www.theworldavatar.com/kg/ontopoi/Dogtraining -->


    <owl:Class rdf:about="https://www.theworldavatar.com/kg/ontopoi/Dogtraining">
        <rdfs:subClassOf rdf:resource="https://www.theworldavatar.com/kg/ontopoi/Animalwelfare"/>
        <rdfs:comment>Dog training is a subcategory of animal welfare</rdfs:comment>
        <rdfs:isDefinedBy rdf:resource="https://www.theworldavatar.com/kg/ontopoi"/>
        <rdfs:label>Dog training</rdfs:label>
    </owl:Class>
    


    <!-- https://www.theworldavatar.com/kg/ontopoi/Domesticappliances -->


    <owl:Class rdf:about="https://www.theworldavatar.com/kg/ontopoi/Domesticappliances">
        <rdfs:subClassOf rdf:resource="https://www.theworldavatar.com/kg/ontopoi/Householdandofficeandleisureandgarden"/>
        <rdfs:comment>Domestic appliances is a subcategory of household, office, leisure and garden</rdfs:comment>
        <rdfs:isDefinedBy rdf:resource="https://www.theworldavatar.com/kg/ontopoi"/>
        <rdfs:label>Domestic appliances</rdfs:label>
    </owl:Class>
    


    <!-- https://www.theworldavatar.com/kg/ontopoi/Domesticstaffandhomehelp -->


    <owl:Class rdf:about="https://www.theworldavatar.com/kg/ontopoi/Domesticstaffandhomehelp">
        <rdfs:subClassOf rdf:resource="https://www.theworldavatar.com/kg/ontopoi/Employmentandcareeragencies"/>
        <rdfs:comment>Domestic staff and home help is a subcategory of employment and career agencies</rdfs:comment>
        <rdfs:isDefinedBy rdf:resource="https://www.theworldavatar.com/kg/ontopoi"/>
        <rdfs:label>Domestic staff and home help</rdfs:label>
    </owl:Class>
    


    <!-- https://www.theworldavatar.com/kg/ontopoi/Drainandsewageclearance -->


    <owl:Class rdf:about="https://www.theworldavatar.com/kg/ontopoi/Drainandsewageclearance">
        <rdfs:subClassOf rdf:resource="https://www.theworldavatar.com/kg/ontopoi/Contractservices"/>
        <rdfs:comment>Drain and sewage clearance is a subcategory of contract services</rdfs:comment>
        <rdfs:isDefinedBy rdf:resource="https://www.theworldavatar.com/kg/ontopoi"/>
        <rdfs:label>Drain and sewage clearance</rdfs:label>
    </owl:Class>
    


    <!-- https://www.theworldavatar.com/kg/ontopoi/Dramaschools -->


    <owl:Class rdf:about="https://www.theworldavatar.com/kg/ontopoi/Dramaschools">
        <rdfs:subClassOf rdf:resource="https://www.theworldavatar.com/kg/ontopoi/Recreationalandvocationaleducation"/>
        <rdfs:comment>Drama schools is a subcategory of recreational and vocational education</rdfs:comment>
        <rdfs:isDefinedBy rdf:resource="https://www.theworldavatar.com/kg/ontopoi"/>
        <rdfs:label>Drama schools</rdfs:label>
    </owl:Class>
    


    <!-- https://www.theworldavatar.com/kg/ontopoi/Drinkingfountainsandwaterpoints -->


    <owl:Class rdf:about="https://www.theworldavatar.com/kg/ontopoi/Drinkingfountainsandwaterpoints">
        <rdfs:subClassOf rdf:resource="https://www.theworldavatar.com/kg/ontopoi/Infrastructureandfacilities"/>
        <rdfs:comment>Drinking fountains and water points is a subcategory of infrastructure and facilities</rdfs:comment>
        <rdfs:isDefinedBy rdf:resource="https://www.theworldavatar.com/kg/ontopoi"/>
        <rdfs:label>Drinking fountains and water points</rdfs:label>
    </owl:Class>
    


    <!-- https://www.theworldavatar.com/kg/ontopoi/Driveragencies -->


    <owl:Class rdf:about="https://www.theworldavatar.com/kg/ontopoi/Driveragencies">
        <rdfs:subClassOf rdf:resource="https://www.theworldavatar.com/kg/ontopoi/Employmentandcareeragencies"/>
        <rdfs:comment>Driver agencies is a subcategory of employment and career agencies</rdfs:comment>
        <rdfs:isDefinedBy rdf:resource="https://www.theworldavatar.com/kg/ontopoi"/>
        <rdfs:label>Driver agencies</rdfs:label>
    </owl:Class>
    


    <!-- https://www.theworldavatar.com/kg/ontopoi/Drivingandmotorcycleschools -->


    <owl:Class rdf:about="https://www.theworldavatar.com/kg/ontopoi/Drivingandmotorcycleschools">
        <rdfs:subClassOf rdf:resource="https://www.theworldavatar.com/kg/ontopoi/Recreationalandvocationaleducation"/>
        <rdfs:comment>Driving and motorcycle schools is a subcategory of recreational and vocational education</rdfs:comment>
        <rdfs:isDefinedBy rdf:resource="https://www.theworldavatar.com/kg/ontopoi"/>
        <rdfs:label>Driving and motorcycle schools</rdfs:label>
    </owl:Class>
    


    <!-- https://www.theworldavatar.com/kg/ontopoi/Drivingtestcentres -->


    <owl:Class rdf:about="https://www.theworldavatar.com/kg/ontopoi/Drivingtestcentres">
        <rdfs:subClassOf rdf:resource="https://www.theworldavatar.com/kg/ontopoi/Centralandlocalgovernment"/>
        <rdfs:comment>Driving test centres is a subcategory of central and local government</rdfs:comment>
        <rdfs:isDefinedBy rdf:resource="https://www.theworldavatar.com/kg/ontopoi"/>
        <rdfs:label>Driving test centres</rdfs:label>
    </owl:Class>
    


    <!-- https://www.theworldavatar.com/kg/ontopoi/Eatinganddrinking -->


    <owl:Class rdf:about="https://www.theworldavatar.com/kg/ontopoi/Eatinganddrinking">
        <rdfs:subClassOf rdf:resource="https://www.theworldavatar.com/kg/ontopoi/Accommodationandeatinganddrinking"/>
        <rdfs:comment>Eating and drinking is a subcategory of accommodation, eating and drinking</rdfs:comment>
        <rdfs:isDefinedBy rdf:resource="https://www.theworldavatar.com/kg/ontopoi"/>
        <rdfs:label>Eating and drinking</rdfs:label>
    </owl:Class>
    


    <!-- https://www.theworldavatar.com/kg/ontopoi/Educationalequipmentandsupplies -->


    <owl:Class rdf:about="https://www.theworldavatar.com/kg/ontopoi/Educationalequipmentandsupplies">
        <rdfs:subClassOf rdf:resource="https://www.theworldavatar.com/kg/ontopoi/Industrialproducts"/>
        <rdfs:comment>Educational equipment and supplies is a subcategory of industrial products</rdfs:comment>
        <rdfs:isDefinedBy rdf:resource="https://www.theworldavatar.com/kg/ontopoi"/>
        <rdfs:label>Educational equipment and supplies</rdfs:label>
    </owl:Class>
    


    <!-- https://www.theworldavatar.com/kg/ontopoi/Educationandhealth -->


    <owl:Class rdf:about="https://www.theworldavatar.com/kg/ontopoi/Educationandhealth"/>
    


    <!-- https://www.theworldavatar.com/kg/ontopoi/Educationauthorities -->


    <owl:Class rdf:about="https://www.theworldavatar.com/kg/ontopoi/Educationauthorities">
        <rdfs:subClassOf rdf:resource="https://www.theworldavatar.com/kg/ontopoi/Educationsupportservices"/>
        <rdfs:comment>Education authorities is a subcategory of education support services</rdfs:comment>
        <rdfs:isDefinedBy rdf:resource="https://www.theworldavatar.com/kg/ontopoi"/>
        <rdfs:label>Education authorities</rdfs:label>
    </owl:Class>
    


    <!-- https://www.theworldavatar.com/kg/ontopoi/Educationservices -->


    <owl:Class rdf:about="https://www.theworldavatar.com/kg/ontopoi/Educationservices">
        <rdfs:subClassOf rdf:resource="https://www.theworldavatar.com/kg/ontopoi/Educationsupportservices"/>
        <rdfs:comment>Education services is a subcategory of education support services</rdfs:comment>
        <rdfs:isDefinedBy rdf:resource="https://www.theworldavatar.com/kg/ontopoi"/>
        <rdfs:label>Education services</rdfs:label>
    </owl:Class>
    


    <!-- https://www.theworldavatar.com/kg/ontopoi/Educationsupportservices -->


    <owl:Class rdf:about="https://www.theworldavatar.com/kg/ontopoi/Educationsupportservices">
        <rdfs:subClassOf rdf:resource="https://www.theworldavatar.com/kg/ontopoi/Educationandhealth"/>
        <rdfs:comment>Education support services is a subcategory of education and health</rdfs:comment>
        <rdfs:isDefinedBy rdf:resource="https://www.theworldavatar.com/kg/ontopoi"/>
        <rdfs:label>Education support services</rdfs:label>
    </owl:Class>
    


    <!-- https://www.theworldavatar.com/kg/ontopoi/Electricalandelectronicengineers -->


    <owl:Class rdf:about="https://www.theworldavatar.com/kg/ontopoi/Electricalandelectronicengineers">
        <rdfs:subClassOf rdf:resource="https://www.theworldavatar.com/kg/ontopoi/Engineeringservices"/>
        <rdfs:comment>Electrical and electronic engineers is a subcategory of engineering services</rdfs:comment>
        <rdfs:isDefinedBy rdf:resource="https://www.theworldavatar.com/kg/ontopoi"/>
        <rdfs:label>Electrical and electronic engineers</rdfs:label>
    </owl:Class>
    


    <!-- https://www.theworldavatar.com/kg/ontopoi/Electricalcomponents -->


    <owl:Class rdf:about="https://www.theworldavatar.com/kg/ontopoi/Electricalcomponents">
        <rdfs:subClassOf rdf:resource="https://www.theworldavatar.com/kg/ontopoi/Industrialproducts"/>
        <rdfs:comment>Electrical components is a subcategory of industrial products</rdfs:comment>
        <rdfs:isDefinedBy rdf:resource="https://www.theworldavatar.com/kg/ontopoi"/>
        <rdfs:label>Electrical components</rdfs:label>
    </owl:Class>
    


    <!-- https://www.theworldavatar.com/kg/ontopoi/Electricalcontractors -->


    <owl:Class rdf:about="https://www.theworldavatar.com/kg/ontopoi/Electricalcontractors">
        <rdfs:subClassOf rdf:resource="https://www.theworldavatar.com/kg/ontopoi/Constructionservices"/>
        <rdfs:comment>Electrical contractors is a subcategory of construction services</rdfs:comment>
        <rdfs:isDefinedBy rdf:resource="https://www.theworldavatar.com/kg/ontopoi"/>
        <rdfs:label>Electrical contractors</rdfs:label>
    </owl:Class>
    


    <!-- https://www.theworldavatar.com/kg/ontopoi/Electricalequipmentrepairandservicing -->


    <owl:Class rdf:about="https://www.theworldavatar.com/kg/ontopoi/Electricalequipmentrepairandservicing">
        <rdfs:subClassOf rdf:resource="https://www.theworldavatar.com/kg/ontopoi/Repairandservicing"/>
        <rdfs:comment>Electrical equipment repair and servicing is a subcategory of repair and servicing</rdfs:comment>
        <rdfs:isDefinedBy rdf:resource="https://www.theworldavatar.com/kg/ontopoi"/>
        <rdfs:label>Electrical equipment repair and servicing</rdfs:label>
    </owl:Class>
    


    <!-- https://www.theworldavatar.com/kg/ontopoi/Electricalfeatures -->


    <owl:Class rdf:about="https://www.theworldavatar.com/kg/ontopoi/Electricalfeatures">
        <rdfs:subClassOf rdf:resource="https://www.theworldavatar.com/kg/ontopoi/Infrastructureandfacilities"/>
        <rdfs:comment>Electrical features is a subcategory of infrastructure and facilities</rdfs:comment>
        <rdfs:isDefinedBy rdf:resource="https://www.theworldavatar.com/kg/ontopoi"/>
        <rdfs:label>Electrical features</rdfs:label>
    </owl:Class>
    


    <!-- https://www.theworldavatar.com/kg/ontopoi/Electricalgoodsandcomponents -->


    <owl:Class rdf:about="https://www.theworldavatar.com/kg/ontopoi/Electricalgoodsandcomponents">
        <rdfs:subClassOf rdf:resource="https://www.theworldavatar.com/kg/ontopoi/Householdandofficeandleisureandgarden"/>
        <rdfs:comment>Electrical goods and components is a subcategory of household, office, leisure and garden</rdfs:comment>
        <rdfs:isDefinedBy rdf:resource="https://www.theworldavatar.com/kg/ontopoi"/>
        <rdfs:label>Electrical goods and components</rdfs:label>
    </owl:Class>
    


    <!-- https://www.theworldavatar.com/kg/ontopoi/Electricalmotorsandgenerators -->


    <owl:Class rdf:about="https://www.theworldavatar.com/kg/ontopoi/Electricalmotorsandgenerators">
        <rdfs:subClassOf rdf:resource="https://www.theworldavatar.com/kg/ontopoi/Industrialproducts"/>
        <rdfs:comment>Electrical motors and generators is a subcategory of industrial products</rdfs:comment>
        <rdfs:isDefinedBy rdf:resource="https://www.theworldavatar.com/kg/ontopoi"/>
        <rdfs:label>Electrical motors and generators</rdfs:label>
    </owl:Class>
    


    <!-- https://www.theworldavatar.com/kg/ontopoi/Electricalproductionandmanipulationequipment -->


    <owl:Class rdf:about="https://www.theworldavatar.com/kg/ontopoi/Electricalproductionandmanipulationequipment">
        <rdfs:subClassOf rdf:resource="https://www.theworldavatar.com/kg/ontopoi/Industrialproducts"/>
        <rdfs:comment>Electrical production and manipulation equipment is a subcategory of industrial products</rdfs:comment>
        <rdfs:isDefinedBy rdf:resource="https://www.theworldavatar.com/kg/ontopoi"/>
        <rdfs:label>Electrical production and manipulation equipment</rdfs:label>
    </owl:Class>
    


    <!-- https://www.theworldavatar.com/kg/ontopoi/ElectronicandInternetpublishers -->


    <owl:Class rdf:about="https://www.theworldavatar.com/kg/ontopoi/ElectronicandInternetpublishers">
        <rdfs:subClassOf rdf:resource="https://www.theworldavatar.com/kg/ontopoi/ITandadvertisingandmarketingandmediaservices"/>
        <rdfs:comment>Electronic and internet publishers is a subcategory of it, advertising, marketing and media service s</rdfs:comment>
        <rdfs:isDefinedBy rdf:resource="https://www.theworldavatar.com/kg/ontopoi"/>
        <rdfs:label>Electronic and Internet publishers</rdfs:label>
    </owl:Class>
    


    <!-- https://www.theworldavatar.com/kg/ontopoi/Electronicequipment -->


    <owl:Class rdf:about="https://www.theworldavatar.com/kg/ontopoi/Electronicequipment">
        <rdfs:subClassOf rdf:resource="https://www.theworldavatar.com/kg/ontopoi/Industrialproducts"/>
        <rdfs:comment>Electronic equipment is a subcategory of industrial products</rdfs:comment>
        <rdfs:isDefinedBy rdf:resource="https://www.theworldavatar.com/kg/ontopoi"/>
        <rdfs:label>Electronic equipment</rdfs:label>
    </owl:Class>
    


    <!-- https://www.theworldavatar.com/kg/ontopoi/Electronicmedia -->


    <owl:Class rdf:about="https://www.theworldavatar.com/kg/ontopoi/Electronicmedia">
        <rdfs:subClassOf rdf:resource="https://www.theworldavatar.com/kg/ontopoi/Industrialproducts"/>
        <rdfs:comment>Electronic media is a subcategory of industrial products</rdfs:comment>
        <rdfs:isDefinedBy rdf:resource="https://www.theworldavatar.com/kg/ontopoi"/>
        <rdfs:label>Electronic media</rdfs:label>
    </owl:Class>
    


    <!-- https://www.theworldavatar.com/kg/ontopoi/Embassiesandconsulates -->


    <owl:Class rdf:about="https://www.theworldavatar.com/kg/ontopoi/Embassiesandconsulates">
        <rdfs:subClassOf rdf:resource="https://www.theworldavatar.com/kg/ontopoi/Centralandlocalgovernment"/>
        <rdfs:comment>Embassies and consulates is a subcategory of central and local government</rdfs:comment>
        <rdfs:isDefinedBy rdf:resource="https://www.theworldavatar.com/kg/ontopoi"/>
        <rdfs:label>Embassies and consulates</rdfs:label>
    </owl:Class>
    


    <!-- https://www.theworldavatar.com/kg/ontopoi/Employmentagencies -->


    <owl:Class rdf:about="https://www.theworldavatar.com/kg/ontopoi/Employmentagencies">
        <rdfs:subClassOf rdf:resource="https://www.theworldavatar.com/kg/ontopoi/Employmentandcareeragencies"/>
        <rdfs:comment>Employment agencies is a subcategory of employment and career agencies</rdfs:comment>
        <rdfs:isDefinedBy rdf:resource="https://www.theworldavatar.com/kg/ontopoi"/>
        <rdfs:label>Employment agencies</rdfs:label>
    </owl:Class>
    


    <!-- https://www.theworldavatar.com/kg/ontopoi/Employmentandcareeragencies -->


    <owl:Class rdf:about="https://www.theworldavatar.com/kg/ontopoi/Employmentandcareeragencies">
        <rdfs:subClassOf rdf:resource="https://www.theworldavatar.com/kg/ontopoi/Commercialservices"/>
        <rdfs:comment>Employment and career agencies is a subcategory of commercial services</rdfs:comment>
        <rdfs:isDefinedBy rdf:resource="https://www.theworldavatar.com/kg/ontopoi"/>
        <rdfs:label>Employment and career agencies</rdfs:label>
    </owl:Class>
    


    <!-- https://www.theworldavatar.com/kg/ontopoi/Energyproduction -->


    <owl:Class rdf:about="https://www.theworldavatar.com/kg/ontopoi/Energyproduction">
        <rdfs:subClassOf rdf:resource="https://www.theworldavatar.com/kg/ontopoi/Industrialfeatures"/>
        <rdfs:comment>Energy production is a subcategory of industrial features</rdfs:comment>
        <rdfs:isDefinedBy rdf:resource="https://www.theworldavatar.com/kg/ontopoi"/>
        <rdfs:label>Energy production</rdfs:label>
    </owl:Class>
    


    <!-- https://www.theworldavatar.com/kg/ontopoi/Engineeringservices -->


    <owl:Class rdf:about="https://www.theworldavatar.com/kg/ontopoi/Engineeringservices">
        <rdfs:subClassOf rdf:resource="https://www.theworldavatar.com/kg/ontopoi/Commercialservices"/>
        <rdfs:comment>Engineering services is a subcategory of commercial services</rdfs:comment>
        <rdfs:isDefinedBy rdf:resource="https://www.theworldavatar.com/kg/ontopoi"/>
        <rdfs:label>Engineering services</rdfs:label>
    </owl:Class>
    


    <!-- https://www.theworldavatar.com/kg/ontopoi/Engines -->


    <owl:Class rdf:about="https://www.theworldavatar.com/kg/ontopoi/Engines">
        <rdfs:subClassOf rdf:resource="https://www.theworldavatar.com/kg/ontopoi/Industrialproducts"/>
        <rdfs:comment>Engines is a subcategory of industrial products</rdfs:comment>
        <rdfs:isDefinedBy rdf:resource="https://www.theworldavatar.com/kg/ontopoi"/>
        <rdfs:label>Engines</rdfs:label>
    </owl:Class>
    


    <!-- https://www.theworldavatar.com/kg/ontopoi/Entertainmentservices -->


    <owl:Class rdf:about="https://www.theworldavatar.com/kg/ontopoi/Entertainmentservices">
        <rdfs:subClassOf rdf:resource="https://www.theworldavatar.com/kg/ontopoi/Sportandentertainmentsupportservices"/>
        <rdfs:comment>Entertainment services is a subcategory of sport and entertainment support services</rdfs:comment>
        <rdfs:isDefinedBy rdf:resource="https://www.theworldavatar.com/kg/ontopoi"/>
        <rdfs:label>Entertainment services</rdfs:label>
    </owl:Class>
    


    <!-- https://www.theworldavatar.com/kg/ontopoi/Estateandpropertymanagement -->


    <owl:Class rdf:about="https://www.theworldavatar.com/kg/ontopoi/Estateandpropertymanagement">
        <rdfs:subClassOf rdf:resource="https://www.theworldavatar.com/kg/ontopoi/Propertyanddevelopmentservices"/>
        <rdfs:comment>Estate and property management is a subcategory of property and development services</rdfs:comment>
        <rdfs:isDefinedBy rdf:resource="https://www.theworldavatar.com/kg/ontopoi"/>
        <rdfs:label>Estate and property management</rdfs:label>
    </owl:Class>
    


    <!-- https://www.theworldavatar.com/kg/ontopoi/EventTicketAgentsandBoxOffice -->


    <owl:Class rdf:about="https://www.theworldavatar.com/kg/ontopoi/EventTicketAgentsandBoxOffice">
        <rdfs:subClassOf rdf:resource="https://www.theworldavatar.com/kg/ontopoi/Personalandconsumerandotherservices"/>
        <rdfs:comment>Event ticket agents and box office is a subcategory of personal, consumer and other services</rdfs:comment>
        <rdfs:isDefinedBy rdf:resource="https://www.theworldavatar.com/kg/ontopoi"/>
        <rdfs:label>Event Ticket Agents and Box Office</rdfs:label>
    </owl:Class>
    


    <!-- https://www.theworldavatar.com/kg/ontopoi/Examinationboards -->


    <owl:Class rdf:about="https://www.theworldavatar.com/kg/ontopoi/Examinationboards">
        <rdfs:subClassOf rdf:resource="https://www.theworldavatar.com/kg/ontopoi/Educationsupportservices"/>
        <rdfs:comment>Examination boards is a subcategory of education support services</rdfs:comment>
        <rdfs:isDefinedBy rdf:resource="https://www.theworldavatar.com/kg/ontopoi"/>
        <rdfs:label>Examination boards</rdfs:label>
    </owl:Class>
    


    <!-- https://www.theworldavatar.com/kg/ontopoi/Extractiveindustries -->


    <owl:Class rdf:about="https://www.theworldavatar.com/kg/ontopoi/Extractiveindustries">
        <rdfs:subClassOf rdf:resource="https://www.theworldavatar.com/kg/ontopoi/Manufacturingandproduction"/>
        <rdfs:comment>Extractive industries is a subcategory of manufacturing and production</rdfs:comment>
        <rdfs:isDefinedBy rdf:resource="https://www.theworldavatar.com/kg/ontopoi"/>
        <rdfs:label>Extractive industries</rdfs:label>
    </owl:Class>
    


    <!-- https://www.theworldavatar.com/kg/ontopoi/Fanclubsandassociations -->


    <owl:Class rdf:about="https://www.theworldavatar.com/kg/ontopoi/Fanclubsandassociations">
        <rdfs:subClassOf rdf:resource="https://www.theworldavatar.com/kg/ontopoi/Organisations"/>
        <rdfs:comment>Fan clubs and associations is a subcategory of organisations</rdfs:comment>
        <rdfs:isDefinedBy rdf:resource="https://www.theworldavatar.com/kg/ontopoi"/>
        <rdfs:label>Fan clubs and associations</rdfs:label>
    </owl:Class>
    


    <!-- https://www.theworldavatar.com/kg/ontopoi/Farm-basedattractions -->


    <owl:Class rdf:about="https://www.theworldavatar.com/kg/ontopoi/Farm-basedattractions">
        <rdfs:subClassOf rdf:resource="https://www.theworldavatar.com/kg/ontopoi/Botanicalandzoological"/>
        <rdfs:comment>Farm-based attractions is a subcategory of botanical and zoological</rdfs:comment>
        <rdfs:isDefinedBy rdf:resource="https://www.theworldavatar.com/kg/ontopoi"/>
        <rdfs:label>Farm-based attractions</rdfs:label>
    </owl:Class>
    


    <!-- https://www.theworldavatar.com/kg/ontopoi/Farming -->


    <owl:Class rdf:about="https://www.theworldavatar.com/kg/ontopoi/Farming">
        <rdfs:subClassOf rdf:resource="https://www.theworldavatar.com/kg/ontopoi/Manufacturingandproduction"/>
        <rdfs:comment>Farming is a subcategory of manufacturing and production</rdfs:comment>
        <rdfs:isDefinedBy rdf:resource="https://www.theworldavatar.com/kg/ontopoi"/>
        <rdfs:label>Farming</rdfs:label>
    </owl:Class>
    


    <!-- https://www.theworldavatar.com/kg/ontopoi/Fastfoodandtakeawayoutlets -->


    <owl:Class rdf:about="https://www.theworldavatar.com/kg/ontopoi/Fastfoodandtakeawayoutlets">
        <rdfs:subClassOf rdf:resource="https://www.theworldavatar.com/kg/ontopoi/Eatinganddrinking"/>
        <rdfs:comment>Fast food and takeaway outlets is a subcategory of eating and drinking</rdfs:comment>
        <rdfs:isDefinedBy rdf:resource="https://www.theworldavatar.com/kg/ontopoi"/>
        <rdfs:label>Fast food and takeaway outlets</rdfs:label>
    </owl:Class>
    


    <!-- https://www.theworldavatar.com/kg/ontopoi/Fastfooddeliveryservices -->


    <owl:Class rdf:about="https://www.theworldavatar.com/kg/ontopoi/Fastfooddeliveryservices">
        <rdfs:subClassOf rdf:resource="https://www.theworldavatar.com/kg/ontopoi/Eatinganddrinking"/>
        <rdfs:comment>Fast food delivery services is a subcategory of eating and drinking</rdfs:comment>
        <rdfs:isDefinedBy rdf:resource="https://www.theworldavatar.com/kg/ontopoi"/>
        <rdfs:label>Fast food delivery services</rdfs:label>
    </owl:Class>
    


    <!-- https://www.theworldavatar.com/kg/ontopoi/Fencesandgatesandrailings -->


    <owl:Class rdf:about="https://www.theworldavatar.com/kg/ontopoi/Fencesandgatesandrailings">
        <rdfs:subClassOf rdf:resource="https://www.theworldavatar.com/kg/ontopoi/Industrialproducts"/>
        <rdfs:comment>Fences, gates and railings is a subcategory of industrial products</rdfs:comment>
        <rdfs:isDefinedBy rdf:resource="https://www.theworldavatar.com/kg/ontopoi"/>
        <rdfs:label>Fences, gates and railings</rdfs:label>
    </owl:Class>
    


    <!-- https://www.theworldavatar.com/kg/ontopoi/Fencinganddrystonewallingservices -->


    <owl:Class rdf:about="https://www.theworldavatar.com/kg/ontopoi/Fencinganddrystonewallingservices">
        <rdfs:subClassOf rdf:resource="https://www.theworldavatar.com/kg/ontopoi/Constructionservices"/>
        <rdfs:comment>Fencing and drystone walling services is a subcategory of construction services</rdfs:comment>
        <rdfs:isDefinedBy rdf:resource="https://www.theworldavatar.com/kg/ontopoi"/>
        <rdfs:label>Fencing and drystone walling services</rdfs:label>
    </owl:Class>
    


    <!-- https://www.theworldavatar.com/kg/ontopoi/Fengshuiconsultantsandfurnishersandshopfitters -->


    <owl:Class rdf:about="https://www.theworldavatar.com/kg/ontopoi/Fengshuiconsultantsandfurnishersandshopfitters">
        <rdfs:subClassOf rdf:resource="https://www.theworldavatar.com/kg/ontopoi/Consultancies"/>
        <rdfs:comment>Feng shui consultants, furnishers and shop fitters is a subcategory of consultancies</rdfs:comment>
        <rdfs:isDefinedBy rdf:resource="https://www.theworldavatar.com/kg/ontopoi"/>
        <rdfs:label>Feng shui consultants, furnishers and shop fitters</rdfs:label>
    </owl:Class>
    


    <!-- https://www.theworldavatar.com/kg/ontopoi/Ferriesandferryterminals -->


    <owl:Class rdf:about="https://www.theworldavatar.com/kg/ontopoi/Ferriesandferryterminals">
        <rdfs:subClassOf rdf:resource="https://www.theworldavatar.com/kg/ontopoi/Water"/>
        <rdfs:comment>Ferries and ferry terminals is a subcategory of water</rdfs:comment>
        <rdfs:isDefinedBy rdf:resource="https://www.theworldavatar.com/kg/ontopoi"/>
        <rdfs:label>Ferries and ferry terminals</rdfs:label>
    </owl:Class>
    


    <!-- https://www.theworldavatar.com/kg/ontopoi/Ferryandcruisecompanies -->


    <owl:Class rdf:about="https://www.theworldavatar.com/kg/ontopoi/Ferryandcruisecompanies">
        <rdfs:subClassOf rdf:resource="https://www.theworldavatar.com/kg/ontopoi/Transportandstorageanddelivery"/>
        <rdfs:comment>Ferry and cruise companies is a subcategory of transport, storage and delivery</rdfs:comment>
        <rdfs:isDefinedBy rdf:resource="https://www.theworldavatar.com/kg/ontopoi"/>
        <rdfs:label>Ferry and cruise companies</rdfs:label>
    </owl:Class>
    


    <!-- https://www.theworldavatar.com/kg/ontopoi/Fertilisers -->


    <owl:Class rdf:about="https://www.theworldavatar.com/kg/ontopoi/Fertilisers">
        <rdfs:subClassOf rdf:resource="https://www.theworldavatar.com/kg/ontopoi/Industrialproducts"/>
        <rdfs:comment>Fertilisers is a subcategory of industrial products</rdfs:comment>
        <rdfs:isDefinedBy rdf:resource="https://www.theworldavatar.com/kg/ontopoi"/>
        <rdfs:label>Fertilisers</rdfs:label>
    </owl:Class>
    


    <!-- https://www.theworldavatar.com/kg/ontopoi/Filmandvideoservices -->


    <owl:Class rdf:about="https://www.theworldavatar.com/kg/ontopoi/Filmandvideoservices">
        <rdfs:subClassOf rdf:resource="https://www.theworldavatar.com/kg/ontopoi/ITandadvertisingandmarketingandmediaservices"/>
        <rdfs:comment>Film and video services is a subcategory of it, advertising, marketing and media service s</rdfs:comment>
        <rdfs:isDefinedBy rdf:resource="https://www.theworldavatar.com/kg/ontopoi"/>
        <rdfs:label>Film and video services</rdfs:label>
    </owl:Class>
    


    <!-- https://www.theworldavatar.com/kg/ontopoi/Financialadviceservices -->


    <owl:Class rdf:about="https://www.theworldavatar.com/kg/ontopoi/Financialadviceservices">
        <rdfs:subClassOf rdf:resource="https://www.theworldavatar.com/kg/ontopoi/Legalandfinancial"/>
        <rdfs:comment>Financial advice services is a subcategory of legal and financial</rdfs:comment>
        <rdfs:isDefinedBy rdf:resource="https://www.theworldavatar.com/kg/ontopoi"/>
        <rdfs:label>Financial advice services</rdfs:label>
    </owl:Class>
    


    <!-- https://www.theworldavatar.com/kg/ontopoi/Firebrigadestations -->


    <owl:Class rdf:about="https://www.theworldavatar.com/kg/ontopoi/Firebrigadestations">
        <rdfs:subClassOf rdf:resource="https://www.theworldavatar.com/kg/ontopoi/Centralandlocalgovernment"/>
        <rdfs:comment>Fire brigade stations is a subcategory of central and local government</rdfs:comment>
        <rdfs:isDefinedBy rdf:resource="https://www.theworldavatar.com/kg/ontopoi"/>
        <rdfs:label>Fire brigade stations</rdfs:label>
    </owl:Class>
    


    <!-- https://www.theworldavatar.com/kg/ontopoi/Fireplacesandmantelpieces -->


    <owl:Class rdf:about="https://www.theworldavatar.com/kg/ontopoi/Fireplacesandmantelpieces">
        <rdfs:subClassOf rdf:resource="https://www.theworldavatar.com/kg/ontopoi/Consumerproducts"/>
        <rdfs:comment>Fireplaces and mantelpieces is a subcategory of consumer products</rdfs:comment>
        <rdfs:isDefinedBy rdf:resource="https://www.theworldavatar.com/kg/ontopoi"/>
        <rdfs:label>Fireplaces and mantelpieces</rdfs:label>
    </owl:Class>
    


    <!-- https://www.theworldavatar.com/kg/ontopoi/Fireworkrelatedservices -->


    <owl:Class rdf:about="https://www.theworldavatar.com/kg/ontopoi/Fireworkrelatedservices">
        <rdfs:subClassOf rdf:resource="https://www.theworldavatar.com/kg/ontopoi/Sportandentertainmentsupportservices"/>
        <rdfs:comment>Firework related services is a subcategory of sport and entertainment support services</rdfs:comment>
        <rdfs:isDefinedBy rdf:resource="https://www.theworldavatar.com/kg/ontopoi"/>
        <rdfs:label>Firework related services</rdfs:label>
    </owl:Class>
    


    <!-- https://www.theworldavatar.com/kg/ontopoi/Firstaidtraining -->


    <owl:Class rdf:about="https://www.theworldavatar.com/kg/ontopoi/Firstaidtraining">
        <rdfs:subClassOf rdf:resource="https://www.theworldavatar.com/kg/ontopoi/Recreationalandvocationaleducation"/>
        <rdfs:comment>First aid training is a subcategory of recreational and vocational education</rdfs:comment>
        <rdfs:isDefinedBy rdf:resource="https://www.theworldavatar.com/kg/ontopoi"/>
        <rdfs:label>First aid training</rdfs:label>
    </owl:Class>
    


    <!-- https://www.theworldavatar.com/kg/ontopoi/Firstandprimaryandinfantschools -->


    <owl:Class rdf:about="https://www.theworldavatar.com/kg/ontopoi/Firstandprimaryandinfantschools">
        <rdfs:subClassOf rdf:resource="https://www.theworldavatar.com/kg/ontopoi/Primaryandsecondaryandtertiaryeducation"/>
        <rdfs:comment>First, primary and infant schools is a subcategory of primary, secondary and tertiary education</rdfs:comment>
        <rdfs:isDefinedBy rdf:resource="https://www.theworldavatar.com/kg/ontopoi"/>
        <rdfs:label>First, primary and infant schools</rdfs:label>
    </owl:Class>
    


    <!-- https://www.theworldavatar.com/kg/ontopoi/Fishandchipshops -->


    <owl:Class rdf:about="https://www.theworldavatar.com/kg/ontopoi/Fishandchipshops">
        <rdfs:subClassOf rdf:resource="https://www.theworldavatar.com/kg/ontopoi/Eatinganddrinking"/>
        <rdfs:comment>Fish and chip shops is a subcategory of eating and drinking</rdfs:comment>
        <rdfs:isDefinedBy rdf:resource="https://www.theworldavatar.com/kg/ontopoi"/>
        <rdfs:label>Fish and chip shops</rdfs:label>
    </owl:Class>
    


    <!-- https://www.theworldavatar.com/kg/ontopoi/Fishandmeatandpoultryproducts -->


    <owl:Class rdf:about="https://www.theworldavatar.com/kg/ontopoi/Fishandmeatandpoultryproducts">
        <rdfs:subClassOf rdf:resource="https://www.theworldavatar.com/kg/ontopoi/Foodstuffs"/>
        <rdfs:comment>Fish, meat and poultry products is a subcategory of foodstuffs</rdfs:comment>
        <rdfs:isDefinedBy rdf:resource="https://www.theworldavatar.com/kg/ontopoi"/>
        <rdfs:label>Fish, meat and poultry products</rdfs:label>
    </owl:Class>
    


    <!-- https://www.theworldavatar.com/kg/ontopoi/Fishandshellfish -->


    <owl:Class rdf:about="https://www.theworldavatar.com/kg/ontopoi/Fishandshellfish">
        <rdfs:subClassOf rdf:resource="https://www.theworldavatar.com/kg/ontopoi/Farming"/>
        <rdfs:comment>Fish and shellfish is a subcategory of farming</rdfs:comment>
        <rdfs:isDefinedBy rdf:resource="https://www.theworldavatar.com/kg/ontopoi"/>
        <rdfs:label>Fish and shellfish</rdfs:label>
    </owl:Class>
    


    <!-- https://www.theworldavatar.com/kg/ontopoi/Fishmongers -->


    <owl:Class rdf:about="https://www.theworldavatar.com/kg/ontopoi/Fishmongers">
        <rdfs:subClassOf rdf:resource="https://www.theworldavatar.com/kg/ontopoi/Foodanddrinkandmultiitemretail"/>
        <rdfs:comment>Fishmongers is a subcategory of food, drink and multi item retail</rdfs:comment>
        <rdfs:isDefinedBy rdf:resource="https://www.theworldavatar.com/kg/ontopoi"/>
        <rdfs:label>Fishmongers</rdfs:label>
    </owl:Class>
    


    <!-- https://www.theworldavatar.com/kg/ontopoi/Florists -->


    <owl:Class rdf:about="https://www.theworldavatar.com/kg/ontopoi/Florists">
        <rdfs:subClassOf rdf:resource="https://www.theworldavatar.com/kg/ontopoi/Householdandofficeandleisureandgarden"/>
        <rdfs:comment>Florists is a subcategory of household, office, leisure and garden</rdfs:comment>
        <rdfs:isDefinedBy rdf:resource="https://www.theworldavatar.com/kg/ontopoi"/>
        <rdfs:label>Florists</rdfs:label>
    </owl:Class>
    


    <!-- https://www.theworldavatar.com/kg/ontopoi/Flyingschools -->


    <owl:Class rdf:about="https://www.theworldavatar.com/kg/ontopoi/Flyingschools">
        <rdfs:subClassOf rdf:resource="https://www.theworldavatar.com/kg/ontopoi/Recreationalandvocationaleducation"/>
        <rdfs:comment>Flying schools is a subcategory of recreational and vocational education</rdfs:comment>
        <rdfs:isDefinedBy rdf:resource="https://www.theworldavatar.com/kg/ontopoi"/>
        <rdfs:label>Flying schools</rdfs:label>
    </owl:Class>
    


    <!-- https://www.theworldavatar.com/kg/ontopoi/Foodandbeverageindustrymachinery -->


    <owl:Class rdf:about="https://www.theworldavatar.com/kg/ontopoi/Foodandbeverageindustrymachinery">
        <rdfs:subClassOf rdf:resource="https://www.theworldavatar.com/kg/ontopoi/Industrialproducts"/>
        <rdfs:comment>Food and beverage industry machinery is a subcategory of industrial products</rdfs:comment>
        <rdfs:isDefinedBy rdf:resource="https://www.theworldavatar.com/kg/ontopoi"/>
        <rdfs:label>Food and beverage industry machinery</rdfs:label>
    </owl:Class>
    


    <!-- https://www.theworldavatar.com/kg/ontopoi/Foodanddrinkandmultiitemretail -->


    <owl:Class rdf:about="https://www.theworldavatar.com/kg/ontopoi/Foodanddrinkandmultiitemretail">
        <rdfs:subClassOf rdf:resource="https://www.theworldavatar.com/kg/ontopoi/Retail"/>
        <rdfs:comment>Food, drink and multi item retail is a subcategory of retail</rdfs:comment>
        <rdfs:isDefinedBy rdf:resource="https://www.theworldavatar.com/kg/ontopoi"/>
        <rdfs:label>Food, drink and multi item retail</rdfs:label>
    </owl:Class>
    


    <!-- https://www.theworldavatar.com/kg/ontopoi/Foodconsultants -->


    <owl:Class rdf:about="https://www.theworldavatar.com/kg/ontopoi/Foodconsultants">
        <rdfs:subClassOf rdf:resource="https://www.theworldavatar.com/kg/ontopoi/Consultancies"/>
        <rdfs:comment>Food consultants is a subcategory of consultancies</rdfs:comment>
        <rdfs:isDefinedBy rdf:resource="https://www.theworldavatar.com/kg/ontopoi"/>
        <rdfs:label>Food consultants</rdfs:label>
    </owl:Class>
    


    <!-- https://www.theworldavatar.com/kg/ontopoi/Foodstuffs -->


    <owl:Class rdf:about="https://www.theworldavatar.com/kg/ontopoi/Foodstuffs">
        <rdfs:subClassOf rdf:resource="https://www.theworldavatar.com/kg/ontopoi/Manufacturingandproduction"/>
        <rdfs:comment>Foodstuffs is a subcategory of manufacturing and production</rdfs:comment>
        <rdfs:isDefinedBy rdf:resource="https://www.theworldavatar.com/kg/ontopoi"/>
        <rdfs:label>Foodstuffs</rdfs:label>
    </owl:Class>
    


    <!-- https://www.theworldavatar.com/kg/ontopoi/Footbridges -->


    <owl:Class rdf:about="https://www.theworldavatar.com/kg/ontopoi/Footbridges">
        <rdfs:subClassOf rdf:resource="https://www.theworldavatar.com/kg/ontopoi/Walking"/>
        <rdfs:comment>Footbridges is a subcategory of walking</rdfs:comment>
        <rdfs:isDefinedBy rdf:resource="https://www.theworldavatar.com/kg/ontopoi"/>
        <rdfs:label>Footbridges</rdfs:label>
    </owl:Class>
    


    <!-- https://www.theworldavatar.com/kg/ontopoi/Footrelatedservices -->


    <owl:Class rdf:about="https://www.theworldavatar.com/kg/ontopoi/Footrelatedservices">
        <rdfs:subClassOf rdf:resource="https://www.theworldavatar.com/kg/ontopoi/Healthpractitionersandestablishments"/>
        <rdfs:comment>Foot related services is a subcategory of health practitioners and establishments</rdfs:comment>
        <rdfs:isDefinedBy rdf:resource="https://www.theworldavatar.com/kg/ontopoi"/>
        <rdfs:label>Foot related services</rdfs:label>
    </owl:Class>
    


    <!-- https://www.theworldavatar.com/kg/ontopoi/Footwear -->


    <owl:Class rdf:about="https://www.theworldavatar.com/kg/ontopoi/Footwear">
        <rdfs:subClassOf rdf:resource="https://www.theworldavatar.com/kg/ontopoi/Clothingandaccessories"/>
        <rdfs:subClassOf rdf:resource="https://www.theworldavatar.com/kg/ontopoi/Consumerproducts"/>
        <rdfs:comment>Footwear is a subcategory of clothing and accessories</rdfs:comment>
        <rdfs:comment>Footwear is a subcategory of consumer products</rdfs:comment>
        <rdfs:isDefinedBy rdf:resource="https://www.theworldavatar.com/kg/ontopoi"/>
        <rdfs:label>Footwear</rdfs:label>
    </owl:Class>
    


    <!-- https://www.theworldavatar.com/kg/ontopoi/Fordsandlevelcrossings -->


    <owl:Class rdf:about="https://www.theworldavatar.com/kg/ontopoi/Fordsandlevelcrossings">
        <rdfs:subClassOf rdf:resource="https://www.theworldavatar.com/kg/ontopoi/Roadandrail"/>
        <rdfs:comment>Fords and level crossings is a subcategory of road and rail</rdfs:comment>
        <rdfs:isDefinedBy rdf:resource="https://www.theworldavatar.com/kg/ontopoi"/>
        <rdfs:label>Fords and level crossings</rdfs:label>
    </owl:Class>
    


    <!-- https://www.theworldavatar.com/kg/ontopoi/Foreigncountrysupportactivities -->


    <owl:Class rdf:about="https://www.theworldavatar.com/kg/ontopoi/Foreigncountrysupportactivities">
        <rdfs:subClassOf rdf:resource="https://www.theworldavatar.com/kg/ontopoi/Centralandlocalgovernment"/>
        <rdfs:comment>Foreign country support activities is a subcategory of central and local government</rdfs:comment>
        <rdfs:isDefinedBy rdf:resource="https://www.theworldavatar.com/kg/ontopoi"/>
        <rdfs:label>Foreign country support activities</rdfs:label>
    </owl:Class>
    


    <!-- https://www.theworldavatar.com/kg/ontopoi/Forestry -->


    <owl:Class rdf:about="https://www.theworldavatar.com/kg/ontopoi/Forestry">
        <rdfs:subClassOf rdf:resource="https://www.theworldavatar.com/kg/ontopoi/Farming"/>
        <rdfs:comment>Forestry is a subcategory of farming</rdfs:comment>
        <rdfs:isDefinedBy rdf:resource="https://www.theworldavatar.com/kg/ontopoi"/>
        <rdfs:label>Forestry</rdfs:label>
    </owl:Class>
    


    <!-- https://www.theworldavatar.com/kg/ontopoi/Franchiseandholdingcompanyservices -->


    <owl:Class rdf:about="https://www.theworldavatar.com/kg/ontopoi/Franchiseandholdingcompanyservices">
        <rdfs:subClassOf rdf:resource="https://www.theworldavatar.com/kg/ontopoi/Legalandfinancial"/>
        <rdfs:comment>Franchise and holding company services is a subcategory of legal and financial</rdfs:comment>
        <rdfs:isDefinedBy rdf:resource="https://www.theworldavatar.com/kg/ontopoi"/>
        <rdfs:label>Franchise and holding company services</rdfs:label>
    </owl:Class>
    


    <!-- https://www.theworldavatar.com/kg/ontopoi/Frozenfoods -->


    <owl:Class rdf:about="https://www.theworldavatar.com/kg/ontopoi/Frozenfoods">
        <rdfs:subClassOf rdf:resource="https://www.theworldavatar.com/kg/ontopoi/Foodanddrinkandmultiitemretail"/>
        <rdfs:comment>Frozen foods is a subcategory of food, drink and multi item retail</rdfs:comment>
        <rdfs:isDefinedBy rdf:resource="https://www.theworldavatar.com/kg/ontopoi"/>
        <rdfs:label>Frozen foods</rdfs:label>
    </owl:Class>
    


    <!-- https://www.theworldavatar.com/kg/ontopoi/Fruitandflowerandvegetablegrowers -->


    <owl:Class rdf:about="https://www.theworldavatar.com/kg/ontopoi/Fruitandflowerandvegetablegrowers">
        <rdfs:subClassOf rdf:resource="https://www.theworldavatar.com/kg/ontopoi/Farming"/>
        <rdfs:comment>Fruit, flower and vegetable growers is a subcategory of farming</rdfs:comment>
        <rdfs:isDefinedBy rdf:resource="https://www.theworldavatar.com/kg/ontopoi"/>
        <rdfs:label>Fruit, flower and vegetable growers</rdfs:label>
    </owl:Class>
    


    <!-- https://www.theworldavatar.com/kg/ontopoi/Fueldistributorsandsuppliers -->


    <owl:Class rdf:about="https://www.theworldavatar.com/kg/ontopoi/Fueldistributorsandsuppliers">
        <rdfs:subClassOf rdf:resource="https://www.theworldavatar.com/kg/ontopoi/Householdandofficeandleisureandgarden"/>
        <rdfs:comment>Fuel distributors and suppliers is a subcategory of household, office, leisure and garden</rdfs:comment>
        <rdfs:isDefinedBy rdf:resource="https://www.theworldavatar.com/kg/ontopoi"/>
        <rdfs:label>Fuel distributors and suppliers</rdfs:label>
    </owl:Class>
    


    <!-- https://www.theworldavatar.com/kg/ontopoi/Fundraisingservices -->


    <owl:Class rdf:about="https://www.theworldavatar.com/kg/ontopoi/Fundraisingservices">
        <rdfs:subClassOf rdf:resource="https://www.theworldavatar.com/kg/ontopoi/Legalandfinancial"/>
        <rdfs:comment>Fundraising services is a subcategory of legal and financial</rdfs:comment>
        <rdfs:isDefinedBy rdf:resource="https://www.theworldavatar.com/kg/ontopoi"/>
        <rdfs:label>Fundraising services</rdfs:label>
    </owl:Class>
    


    <!-- https://www.theworldavatar.com/kg/ontopoi/Funeralandassociatedservices -->


    <owl:Class rdf:about="https://www.theworldavatar.com/kg/ontopoi/Funeralandassociatedservices">
        <rdfs:subClassOf rdf:resource="https://www.theworldavatar.com/kg/ontopoi/Personalandconsumerandotherservices"/>
        <rdfs:comment>Funeral and associated services is a subcategory of personal, consumer and other services</rdfs:comment>
        <rdfs:isDefinedBy rdf:resource="https://www.theworldavatar.com/kg/ontopoi"/>
        <rdfs:label>Funeral and associated services</rdfs:label>
    </owl:Class>
    


    <!-- https://www.theworldavatar.com/kg/ontopoi/Funfairservices -->


    <owl:Class rdf:about="https://www.theworldavatar.com/kg/ontopoi/Funfairservices">
        <rdfs:subClassOf rdf:resource="https://www.theworldavatar.com/kg/ontopoi/Sportandentertainmentsupportservices"/>
        <rdfs:comment>Funfair services is a subcategory of sport and entertainment support services</rdfs:comment>
        <rdfs:isDefinedBy rdf:resource="https://www.theworldavatar.com/kg/ontopoi"/>
        <rdfs:label>Funfair services</rdfs:label>
    </owl:Class>
    


    <!-- https://www.theworldavatar.com/kg/ontopoi/Furniture -->


    <owl:Class rdf:about="https://www.theworldavatar.com/kg/ontopoi/Furniture">
        <rdfs:subClassOf rdf:resource="https://www.theworldavatar.com/kg/ontopoi/Consumerproducts"/>
        <rdfs:subClassOf rdf:resource="https://www.theworldavatar.com/kg/ontopoi/Householdandofficeandleisureandgarden"/>
        <rdfs:comment>Furniture is a subcategory of consumer products</rdfs:comment>
        <rdfs:comment>Furniture is a subcategory of household, office, leisure and garden</rdfs:comment>
        <rdfs:isDefinedBy rdf:resource="https://www.theworldavatar.com/kg/ontopoi"/>
        <rdfs:label>Furniture</rdfs:label>
    </owl:Class>
    


    <!-- https://www.theworldavatar.com/kg/ontopoi/Furthereducationestablishments -->


    <owl:Class rdf:about="https://www.theworldavatar.com/kg/ontopoi/Furthereducationestablishments">
        <rdfs:subClassOf rdf:resource="https://www.theworldavatar.com/kg/ontopoi/Primaryandsecondaryandtertiaryeducation"/>
        <rdfs:comment>Further education establishments is a subcategory of primary, secondary and tertiary education</rdfs:comment>
        <rdfs:isDefinedBy rdf:resource="https://www.theworldavatar.com/kg/ontopoi"/>
        <rdfs:label>Further education establishments</rdfs:label>
    </owl:Class>
    


    <!-- https://www.theworldavatar.com/kg/ontopoi/Gambling -->


    <owl:Class rdf:about="https://www.theworldavatar.com/kg/ontopoi/Gambling">
        <rdfs:subClassOf rdf:resource="https://www.theworldavatar.com/kg/ontopoi/Sportandentertainment"/>
        <rdfs:comment>Gambling is a subcategory of sport and entertainment</rdfs:comment>
        <rdfs:isDefinedBy rdf:resource="https://www.theworldavatar.com/kg/ontopoi"/>
        <rdfs:label>Gambling</rdfs:label>
    </owl:Class>
    


    <!-- https://www.theworldavatar.com/kg/ontopoi/Garagesandgardenandportablebuildings -->


    <owl:Class rdf:about="https://www.theworldavatar.com/kg/ontopoi/Garagesandgardenandportablebuildings">
        <rdfs:subClassOf rdf:resource="https://www.theworldavatar.com/kg/ontopoi/Householdandofficeandleisureandgarden"/>
        <rdfs:comment>Garages, garden and portable buildings is a subcategory of household, office, leisure and garden</rdfs:comment>
        <rdfs:isDefinedBy rdf:resource="https://www.theworldavatar.com/kg/ontopoi"/>
        <rdfs:label>Garages, garden and portable buildings</rdfs:label>
    </owl:Class>
    


    <!-- https://www.theworldavatar.com/kg/ontopoi/Gardencentresandnurseries -->


    <owl:Class rdf:about="https://www.theworldavatar.com/kg/ontopoi/Gardencentresandnurseries">
        <rdfs:subClassOf rdf:resource="https://www.theworldavatar.com/kg/ontopoi/Householdandofficeandleisureandgarden"/>
        <rdfs:comment>Garden centres and nurseries is a subcategory of household, office, leisure and garden</rdfs:comment>
        <rdfs:isDefinedBy rdf:resource="https://www.theworldavatar.com/kg/ontopoi"/>
        <rdfs:label>Garden centres and nurseries</rdfs:label>
    </owl:Class>
    


    <!-- https://www.theworldavatar.com/kg/ontopoi/Gardengoods -->


    <owl:Class rdf:about="https://www.theworldavatar.com/kg/ontopoi/Gardengoods">
        <rdfs:subClassOf rdf:resource="https://www.theworldavatar.com/kg/ontopoi/Consumerproducts"/>
        <rdfs:comment>Garden goods is a subcategory of consumer products</rdfs:comment>
        <rdfs:isDefinedBy rdf:resource="https://www.theworldavatar.com/kg/ontopoi"/>
        <rdfs:label>Garden goods</rdfs:label>
    </owl:Class>
    


    <!-- https://www.theworldavatar.com/kg/ontopoi/Gardeningandlandscapingandtreesurgeryservices -->


    <owl:Class rdf:about="https://www.theworldavatar.com/kg/ontopoi/Gardeningandlandscapingandtreesurgeryservices">
        <rdfs:subClassOf rdf:resource="https://www.theworldavatar.com/kg/ontopoi/Constructionservices"/>
        <rdfs:comment>Gardening, landscaping and tree surgery services is a subcategory of construction services</rdfs:comment>
        <rdfs:isDefinedBy rdf:resource="https://www.theworldavatar.com/kg/ontopoi"/>
        <rdfs:label>Gardening, landscaping and tree surgery services</rdfs:label>
    </owl:Class>
    


    <!-- https://www.theworldavatar.com/kg/ontopoi/Gardenmachineryandfurniture -->


    <owl:Class rdf:about="https://www.theworldavatar.com/kg/ontopoi/Gardenmachineryandfurniture">
        <rdfs:subClassOf rdf:resource="https://www.theworldavatar.com/kg/ontopoi/Householdandofficeandleisureandgarden"/>
        <rdfs:comment>Garden machinery and furniture is a subcategory of household, office, leisure and garden</rdfs:comment>
        <rdfs:isDefinedBy rdf:resource="https://www.theworldavatar.com/kg/ontopoi"/>
        <rdfs:label>Garden machinery and furniture</rdfs:label>
    </owl:Class>
    


    <!-- https://www.theworldavatar.com/kg/ontopoi/Gasfeatures -->


    <owl:Class rdf:about="https://www.theworldavatar.com/kg/ontopoi/Gasfeatures">
        <rdfs:subClassOf rdf:resource="https://www.theworldavatar.com/kg/ontopoi/Infrastructureandfacilities"/>
        <rdfs:comment>Gas features is a subcategory of infrastructure and facilities</rdfs:comment>
        <rdfs:isDefinedBy rdf:resource="https://www.theworldavatar.com/kg/ontopoi"/>
        <rdfs:label>Gas features</rdfs:label>
    </owl:Class>
    


    <!-- https://www.theworldavatar.com/kg/ontopoi/General-purposemachinery -->


    <owl:Class rdf:about="https://www.theworldavatar.com/kg/ontopoi/General-purposemachinery">
        <rdfs:subClassOf rdf:resource="https://www.theworldavatar.com/kg/ontopoi/Industrialproducts"/>
        <rdfs:comment>General-purpose machinery is a subcategory of industrial products</rdfs:comment>
        <rdfs:isDefinedBy rdf:resource="https://www.theworldavatar.com/kg/ontopoi"/>
        <rdfs:label>General-purpose machinery</rdfs:label>
    </owl:Class>
    


    <!-- https://www.theworldavatar.com/kg/ontopoi/Generalcomputerservices -->


    <owl:Class rdf:about="https://www.theworldavatar.com/kg/ontopoi/Generalcomputerservices">
        <rdfs:subClassOf rdf:resource="https://www.theworldavatar.com/kg/ontopoi/ITandadvertisingandmarketingandmediaservices"/>
        <rdfs:comment>General computer services is a subcategory of it, advertising, marketing and media service s</rdfs:comment>
        <rdfs:isDefinedBy rdf:resource="https://www.theworldavatar.com/kg/ontopoi"/>
        <rdfs:label>General computer services</rdfs:label>
    </owl:Class>
    


    <!-- https://www.theworldavatar.com/kg/ontopoi/Generalconstructionsupplies -->


    <owl:Class rdf:about="https://www.theworldavatar.com/kg/ontopoi/Generalconstructionsupplies">
        <rdfs:subClassOf rdf:resource="https://www.theworldavatar.com/kg/ontopoi/Industrialproducts"/>
        <rdfs:comment>General construction supplies is a subcategory of industrial products</rdfs:comment>
        <rdfs:isDefinedBy rdf:resource="https://www.theworldavatar.com/kg/ontopoi"/>
        <rdfs:label>General construction supplies</rdfs:label>
    </owl:Class>
    


    <!-- https://www.theworldavatar.com/kg/ontopoi/Generalhouseholdgoods -->


    <owl:Class rdf:about="https://www.theworldavatar.com/kg/ontopoi/Generalhouseholdgoods">
        <rdfs:subClassOf rdf:resource="https://www.theworldavatar.com/kg/ontopoi/Householdandofficeandleisureandgarden"/>
        <rdfs:comment>General household goods is a subcategory of household, office, leisure and garden</rdfs:comment>
        <rdfs:isDefinedBy rdf:resource="https://www.theworldavatar.com/kg/ontopoi"/>
        <rdfs:label>General household goods</rdfs:label>
    </owl:Class>
    


    <!-- https://www.theworldavatar.com/kg/ontopoi/Generalmanufacturing -->


    <owl:Class rdf:about="https://www.theworldavatar.com/kg/ontopoi/Generalmanufacturing">
        <rdfs:subClassOf rdf:resource="https://www.theworldavatar.com/kg/ontopoi/Industrialproducts"/>
        <rdfs:comment>General manufacturing is a subcategory of industrial products</rdfs:comment>
        <rdfs:isDefinedBy rdf:resource="https://www.theworldavatar.com/kg/ontopoi"/>
        <rdfs:label>General manufacturing</rdfs:label>
    </owl:Class>
    


    <!-- https://www.theworldavatar.com/kg/ontopoi/Giftsandcards -->


    <owl:Class rdf:about="https://www.theworldavatar.com/kg/ontopoi/Giftsandcards">
        <rdfs:subClassOf rdf:resource="https://www.theworldavatar.com/kg/ontopoi/Householdandofficeandleisureandgarden"/>
        <rdfs:comment>Gifts and cards is a subcategory of household, office, leisure and garden</rdfs:comment>
        <rdfs:isDefinedBy rdf:resource="https://www.theworldavatar.com/kg/ontopoi"/>
        <rdfs:label>Gifts and cards</rdfs:label>
    </owl:Class>
    


    <!-- https://www.theworldavatar.com/kg/ontopoi/Giftware -->


    <owl:Class rdf:about="https://www.theworldavatar.com/kg/ontopoi/Giftware">
        <rdfs:subClassOf rdf:resource="https://www.theworldavatar.com/kg/ontopoi/Consumerproducts"/>
        <rdfs:comment>Giftware is a subcategory of consumer products</rdfs:comment>
        <rdfs:isDefinedBy rdf:resource="https://www.theworldavatar.com/kg/ontopoi"/>
        <rdfs:label>Giftware</rdfs:label>
    </owl:Class>
    


    <!-- https://www.theworldavatar.com/kg/ontopoi/Glass -->


    <owl:Class rdf:about="https://www.theworldavatar.com/kg/ontopoi/Glass">
        <rdfs:subClassOf rdf:resource="https://www.theworldavatar.com/kg/ontopoi/Industrialproducts"/>
        <rdfs:comment>Glass is a subcategory of industrial products</rdfs:comment>
        <rdfs:isDefinedBy rdf:resource="https://www.theworldavatar.com/kg/ontopoi"/>
        <rdfs:label>Glass</rdfs:label>
    </owl:Class>
    


    <!-- https://www.theworldavatar.com/kg/ontopoi/Glassfibreservices -->


    <owl:Class rdf:about="https://www.theworldavatar.com/kg/ontopoi/Glassfibreservices">
        <rdfs:subClassOf rdf:resource="https://www.theworldavatar.com/kg/ontopoi/Industrialproducts"/>
        <rdfs:comment>Glass fibre services is a subcategory of industrial products</rdfs:comment>
        <rdfs:isDefinedBy rdf:resource="https://www.theworldavatar.com/kg/ontopoi"/>
        <rdfs:label>Glass fibre services</rdfs:label>
    </owl:Class>
    


    <!-- https://www.theworldavatar.com/kg/ontopoi/Glaziers -->


    <owl:Class rdf:about="https://www.theworldavatar.com/kg/ontopoi/Glaziers">
        <rdfs:subClassOf rdf:resource="https://www.theworldavatar.com/kg/ontopoi/Constructionservices"/>
        <rdfs:comment>Glaziers is a subcategory of construction services</rdfs:comment>
        <rdfs:isDefinedBy rdf:resource="https://www.theworldavatar.com/kg/ontopoi"/>
        <rdfs:label>Glaziers</rdfs:label>
    </owl:Class>
    


    <!-- https://www.theworldavatar.com/kg/ontopoi/Golfrangesandcoursesandclubsandprofessionals -->


    <owl:Class rdf:about="https://www.theworldavatar.com/kg/ontopoi/Golfrangesandcoursesandclubsandprofessionals">
        <rdfs:subClassOf rdf:resource="https://www.theworldavatar.com/kg/ontopoi/Sportscomplex"/>
        <rdfs:comment>Golf ranges, courses, clubs and professionals is a subcategory of sports complex</rdfs:comment>
        <rdfs:isDefinedBy rdf:resource="https://www.theworldavatar.com/kg/ontopoi"/>
        <rdfs:label>Golf ranges, courses, clubs and professionals</rdfs:label>
    </owl:Class>
    


    <!-- https://www.theworldavatar.com/kg/ontopoi/Greenandnewagegoods -->


    <owl:Class rdf:about="https://www.theworldavatar.com/kg/ontopoi/Greenandnewagegoods">
        <rdfs:subClassOf rdf:resource="https://www.theworldavatar.com/kg/ontopoi/Foodanddrinkandmultiitemretail"/>
        <rdfs:comment>Green and new age goods is a subcategory of food, drink and multi item retail</rdfs:comment>
        <rdfs:isDefinedBy rdf:resource="https://www.theworldavatar.com/kg/ontopoi"/>
        <rdfs:label>Green and new age goods</rdfs:label>
    </owl:Class>
    


    <!-- https://www.theworldavatar.com/kg/ontopoi/Grocersandfarmshopsandpickyourown -->


    <owl:Class rdf:about="https://www.theworldavatar.com/kg/ontopoi/Grocersandfarmshopsandpickyourown">
        <rdfs:subClassOf rdf:resource="https://www.theworldavatar.com/kg/ontopoi/Foodanddrinkandmultiitemretail"/>
        <rdfs:comment>Grocers, farm shops and pick your own is a subcategory of food, drink and multi item retail</rdfs:comment>
        <rdfs:isDefinedBy rdf:resource="https://www.theworldavatar.com/kg/ontopoi"/>
        <rdfs:label>Grocers, farm shops and pick your own</rdfs:label>
    </owl:Class>
    


    <!-- https://www.theworldavatar.com/kg/ontopoi/Gymnasiumsandsportshallsandleisurecentres -->


    <owl:Class rdf:about="https://www.theworldavatar.com/kg/ontopoi/Gymnasiumsandsportshallsandleisurecentres">
        <rdfs:subClassOf rdf:resource="https://www.theworldavatar.com/kg/ontopoi/Sportscomplex"/>
        <rdfs:comment>Gymnasiums, sports halls and leisure centres is a subcategory of sports complex</rdfs:comment>
        <rdfs:isDefinedBy rdf:resource="https://www.theworldavatar.com/kg/ontopoi"/>
        <rdfs:label>Gymnasiums, sports halls and leisure centres</rdfs:label>
    </owl:Class>
    


    <!-- https://www.theworldavatar.com/kg/ontopoi/Hailandridezones -->


    <owl:Class rdf:about="https://www.theworldavatar.com/kg/ontopoi/Hailandridezones">
        <rdfs:subClassOf rdf:resource="https://www.theworldavatar.com/kg/ontopoi/Bustransport"/>
        <rdfs:comment>Hail and ride zones is a subcategory of bus transport</rdfs:comment>
        <rdfs:isDefinedBy rdf:resource="https://www.theworldavatar.com/kg/ontopoi"/>
        <rdfs:label>Hail and ride zones</rdfs:label>
    </owl:Class>
    


    <!-- https://www.theworldavatar.com/kg/ontopoi/Hairandbeautyservices -->


    <owl:Class rdf:about="https://www.theworldavatar.com/kg/ontopoi/Hairandbeautyservices">
        <rdfs:subClassOf rdf:resource="https://www.theworldavatar.com/kg/ontopoi/Personalandconsumerandotherservices"/>
        <rdfs:comment>Hair and beauty services is a subcategory of personal, consumer and other services</rdfs:comment>
        <rdfs:isDefinedBy rdf:resource="https://www.theworldavatar.com/kg/ontopoi"/>
        <rdfs:label>Hair and beauty services</rdfs:label>
    </owl:Class>
    


    <!-- https://www.theworldavatar.com/kg/ontopoi/Hallsandcommunitycentres -->


    <owl:Class rdf:about="https://www.theworldavatar.com/kg/ontopoi/Hallsandcommunitycentres">
        <rdfs:subClassOf rdf:resource="https://www.theworldavatar.com/kg/ontopoi/Infrastructureandfacilities"/>
        <rdfs:comment>Halls and community centres is a subcategory of infrastructure and facilities</rdfs:comment>
        <rdfs:isDefinedBy rdf:resource="https://www.theworldavatar.com/kg/ontopoi"/>
        <rdfs:label>Halls and community centres</rdfs:label>
    </owl:Class>
    


    <!-- https://www.theworldavatar.com/kg/ontopoi/Headquartersandadministrationandcentraloffices -->


    <owl:Class rdf:about="https://www.theworldavatar.com/kg/ontopoi/Headquartersandadministrationandcentraloffices">
        <rdfs:subClassOf rdf:resource="https://www.theworldavatar.com/kg/ontopoi/Personalandconsumerandotherservices"/>
        <rdfs:comment>Headquarters, administration and central offices is a subcategory of personal, consumer and other services</rdfs:comment>
        <rdfs:isDefinedBy rdf:resource="https://www.theworldavatar.com/kg/ontopoi"/>
        <rdfs:label>Headquarters, administration and central offices</rdfs:label>
    </owl:Class>
    


    <!-- https://www.theworldavatar.com/kg/ontopoi/Healthauthorities -->


    <owl:Class rdf:about="https://www.theworldavatar.com/kg/ontopoi/Healthauthorities">
        <rdfs:subClassOf rdf:resource="https://www.theworldavatar.com/kg/ontopoi/Healthsupportservices"/>
        <rdfs:comment>Health authorities is a subcategory of health support services</rdfs:comment>
        <rdfs:isDefinedBy rdf:resource="https://www.theworldavatar.com/kg/ontopoi"/>
        <rdfs:label>Health authorities</rdfs:label>
    </owl:Class>
    


    <!-- https://www.theworldavatar.com/kg/ontopoi/Healthpractitionersandestablishments -->


    <owl:Class rdf:about="https://www.theworldavatar.com/kg/ontopoi/Healthpractitionersandestablishments">
        <rdfs:subClassOf rdf:resource="https://www.theworldavatar.com/kg/ontopoi/Educationandhealth"/>
        <rdfs:comment>Health practitioners and establishments is a subcategory of education and health</rdfs:comment>
        <rdfs:isDefinedBy rdf:resource="https://www.theworldavatar.com/kg/ontopoi"/>
        <rdfs:label>Health practitioners and establishments</rdfs:label>
    </owl:Class>
    


    <!-- https://www.theworldavatar.com/kg/ontopoi/Healthsupportservices -->


    <owl:Class rdf:about="https://www.theworldavatar.com/kg/ontopoi/Healthsupportservices">
        <rdfs:subClassOf rdf:resource="https://www.theworldavatar.com/kg/ontopoi/Educationandhealth"/>
        <rdfs:comment>Health support services is a subcategory of education and health</rdfs:comment>
        <rdfs:isDefinedBy rdf:resource="https://www.theworldavatar.com/kg/ontopoi"/>
        <rdfs:label>Health support services</rdfs:label>
    </owl:Class>
    


    <!-- https://www.theworldavatar.com/kg/ontopoi/Helipads -->


    <owl:Class rdf:about="https://www.theworldavatar.com/kg/ontopoi/Helipads">
        <rdfs:subClassOf rdf:resource="https://www.theworldavatar.com/kg/ontopoi/Air"/>
        <rdfs:comment>Helipads is a subcategory of air</rdfs:comment>
        <rdfs:isDefinedBy rdf:resource="https://www.theworldavatar.com/kg/ontopoi"/>
        <rdfs:label>Helipads</rdfs:label>
    </owl:Class>
    


    <!-- https://www.theworldavatar.com/kg/ontopoi/Herbsandspices -->


    <owl:Class rdf:about="https://www.theworldavatar.com/kg/ontopoi/Herbsandspices">
        <rdfs:subClassOf rdf:resource="https://www.theworldavatar.com/kg/ontopoi/Foodanddrinkandmultiitemretail"/>
        <rdfs:comment>Herbs and spices is a subcategory of food, drink and multi item retail</rdfs:comment>
        <rdfs:isDefinedBy rdf:resource="https://www.theworldavatar.com/kg/ontopoi"/>
        <rdfs:label>Herbs and spices</rdfs:label>
    </owl:Class>
    


    <!-- https://www.theworldavatar.com/kg/ontopoi/Highereducationestablishments -->


    <owl:Class rdf:about="https://www.theworldavatar.com/kg/ontopoi/Highereducationestablishments">
        <rdfs:subClassOf rdf:resource="https://www.theworldavatar.com/kg/ontopoi/Primaryandsecondaryandtertiaryeducation"/>
        <rdfs:comment>Higher education establishments is a subcategory of primary, secondary and tertiary education</rdfs:comment>
        <rdfs:isDefinedBy rdf:resource="https://www.theworldavatar.com/kg/ontopoi"/>
        <rdfs:label>Higher education establishments</rdfs:label>
    </owl:Class>
    


    <!-- https://www.theworldavatar.com/kg/ontopoi/Hireservices -->


    <owl:Class rdf:about="https://www.theworldavatar.com/kg/ontopoi/Hireservices">
        <rdfs:subClassOf rdf:resource="https://www.theworldavatar.com/kg/ontopoi/Commercialservices"/>
        <rdfs:comment>Hire services is a subcategory of commercial services</rdfs:comment>
        <rdfs:isDefinedBy rdf:resource="https://www.theworldavatar.com/kg/ontopoi"/>
        <rdfs:label>Hire services</rdfs:label>
    </owl:Class>
    


    <!-- https://www.theworldavatar.com/kg/ontopoi/Historicalandcultural -->


    <owl:Class rdf:about="https://www.theworldavatar.com/kg/ontopoi/Historicalandcultural">
        <rdfs:subClassOf rdf:resource="https://www.theworldavatar.com/kg/ontopoi/Attractions"/>
        <rdfs:comment>Historical and cultural is a subcategory of attractions</rdfs:comment>
        <rdfs:isDefinedBy rdf:resource="https://www.theworldavatar.com/kg/ontopoi"/>
        <rdfs:label>Historical and cultural</rdfs:label>
    </owl:Class>
    


    <!-- https://www.theworldavatar.com/kg/ontopoi/Historicalresearch -->


    <owl:Class rdf:about="https://www.theworldavatar.com/kg/ontopoi/Historicalresearch">
        <rdfs:subClassOf rdf:resource="https://www.theworldavatar.com/kg/ontopoi/Personalandconsumerandotherservices"/>
        <rdfs:comment>Historical research is a subcategory of personal, consumer and other services</rdfs:comment>
        <rdfs:isDefinedBy rdf:resource="https://www.theworldavatar.com/kg/ontopoi"/>
        <rdfs:label>Historical research</rdfs:label>
    </owl:Class>
    


    <!-- https://www.theworldavatar.com/kg/ontopoi/Historicalships -->


    <owl:Class rdf:about="https://www.theworldavatar.com/kg/ontopoi/Historicalships">
        <rdfs:subClassOf rdf:resource="https://www.theworldavatar.com/kg/ontopoi/Historicalandcultural"/>
        <rdfs:comment>Historical ships is a subcategory of historical and cultural</rdfs:comment>
        <rdfs:isDefinedBy rdf:resource="https://www.theworldavatar.com/kg/ontopoi"/>
        <rdfs:label>Historical ships</rdfs:label>
    </owl:Class>
    


    <!-- https://www.theworldavatar.com/kg/ontopoi/Historicandceremonialstructures -->


    <owl:Class rdf:about="https://www.theworldavatar.com/kg/ontopoi/Historicandceremonialstructures">
        <rdfs:subClassOf rdf:resource="https://www.theworldavatar.com/kg/ontopoi/Historicalandcultural"/>
        <rdfs:comment>Historic and ceremonial structures is a subcategory of historical and cultural</rdfs:comment>
        <rdfs:isDefinedBy rdf:resource="https://www.theworldavatar.com/kg/ontopoi"/>
        <rdfs:label>Historic and ceremonial structures</rdfs:label>
    </owl:Class>
    


    <!-- https://www.theworldavatar.com/kg/ontopoi/Historicbuildingsincludingcastlesandfortsandabbeys -->


    <owl:Class rdf:about="https://www.theworldavatar.com/kg/ontopoi/Historicbuildingsincludingcastlesandfortsandabbeys">
        <rdfs:subClassOf rdf:resource="https://www.theworldavatar.com/kg/ontopoi/Historicalandcultural"/>
        <rdfs:comment>Historic buildings including castles, forts and abbeys is a subcategory of historical and cultural</rdfs:comment>
        <rdfs:isDefinedBy rdf:resource="https://www.theworldavatar.com/kg/ontopoi"/>
        <rdfs:label>Historic buildings including castles, forts and abbeys</rdfs:label>
    </owl:Class>
    


    <!-- https://www.theworldavatar.com/kg/ontopoi/Hobbyandsportsandpastimeproducts -->


    <owl:Class rdf:about="https://www.theworldavatar.com/kg/ontopoi/Hobbyandsportsandpastimeproducts">
        <rdfs:subClassOf rdf:resource="https://www.theworldavatar.com/kg/ontopoi/Consumerproducts"/>
        <rdfs:subClassOf rdf:resource="https://www.theworldavatar.com/kg/ontopoi/Householdandofficeandleisureandgarden"/>
        <rdfs:comment>Hobby, sports and pastime products is a subcategory of consumer products</rdfs:comment>
        <rdfs:comment>Hobby, sports and pastime products is a subcategory of household, office, leisure and garden</rdfs:comment>
        <rdfs:isDefinedBy rdf:resource="https://www.theworldavatar.com/kg/ontopoi"/>
        <rdfs:label>Hobby, sports and pastime products</rdfs:label>
    </owl:Class>
    


    <!-- https://www.theworldavatar.com/kg/ontopoi/Homeopaths -->


    <owl:Class rdf:about="https://www.theworldavatar.com/kg/ontopoi/Homeopaths">
        <rdfs:subClassOf rdf:resource="https://www.theworldavatar.com/kg/ontopoi/Healthpractitionersandestablishments"/>
        <rdfs:comment>Homeopaths is a subcategory of health practitioners and establishments</rdfs:comment>
        <rdfs:isDefinedBy rdf:resource="https://www.theworldavatar.com/kg/ontopoi"/>
        <rdfs:label>Homeopaths</rdfs:label>
    </owl:Class>
    


    <!-- https://www.theworldavatar.com/kg/ontopoi/Horsebreedersanddealers -->


    <owl:Class rdf:about="https://www.theworldavatar.com/kg/ontopoi/Horsebreedersanddealers">
        <rdfs:subClassOf rdf:resource="https://www.theworldavatar.com/kg/ontopoi/Farming"/>
        <rdfs:comment>Horse breeders and dealers is a subcategory of farming</rdfs:comment>
        <rdfs:isDefinedBy rdf:resource="https://www.theworldavatar.com/kg/ontopoi"/>
        <rdfs:label>Horse breeders and dealers</rdfs:label>
    </owl:Class>
    


    <!-- https://www.theworldavatar.com/kg/ontopoi/Horsetraining -->


    <owl:Class rdf:about="https://www.theworldavatar.com/kg/ontopoi/Horsetraining">
        <rdfs:subClassOf rdf:resource="https://www.theworldavatar.com/kg/ontopoi/Animalwelfare"/>
        <rdfs:comment>Horse training is a subcategory of animal welfare</rdfs:comment>
        <rdfs:isDefinedBy rdf:resource="https://www.theworldavatar.com/kg/ontopoi"/>
        <rdfs:label>Horse training</rdfs:label>
    </owl:Class>
    


    <!-- https://www.theworldavatar.com/kg/ontopoi/Horticulturalattractions -->


    <owl:Class rdf:about="https://www.theworldavatar.com/kg/ontopoi/Horticulturalattractions">
        <rdfs:subClassOf rdf:resource="https://www.theworldavatar.com/kg/ontopoi/Botanicalandzoological"/>
        <rdfs:comment>Horticultural attractions is a subcategory of botanical and zoological</rdfs:comment>
        <rdfs:isDefinedBy rdf:resource="https://www.theworldavatar.com/kg/ontopoi"/>
        <rdfs:label>Horticultural attractions</rdfs:label>
    </owl:Class>
    


    <!-- https://www.theworldavatar.com/kg/ontopoi/Horticulturalequipment -->


    <owl:Class rdf:about="https://www.theworldavatar.com/kg/ontopoi/Horticulturalequipment">
        <rdfs:subClassOf rdf:resource="https://www.theworldavatar.com/kg/ontopoi/Industrialproducts"/>
        <rdfs:comment>Horticultural equipment is a subcategory of industrial products</rdfs:comment>
        <rdfs:isDefinedBy rdf:resource="https://www.theworldavatar.com/kg/ontopoi"/>
        <rdfs:label>Horticultural equipment</rdfs:label>
    </owl:Class>
    


    <!-- https://www.theworldavatar.com/kg/ontopoi/Hospices -->


    <owl:Class rdf:about="https://www.theworldavatar.com/kg/ontopoi/Hospices">
        <rdfs:subClassOf rdf:resource="https://www.theworldavatar.com/kg/ontopoi/Healthpractitionersandestablishments"/>
        <rdfs:comment>Hospices is a subcategory of health practitioners and establishments</rdfs:comment>
        <rdfs:isDefinedBy rdf:resource="https://www.theworldavatar.com/kg/ontopoi"/>
        <rdfs:label>Hospices</rdfs:label>
    </owl:Class>
    


    <!-- https://www.theworldavatar.com/kg/ontopoi/Hospitals -->


    <owl:Class rdf:about="https://www.theworldavatar.com/kg/ontopoi/Hospitals">
        <rdfs:subClassOf rdf:resource="https://www.theworldavatar.com/kg/ontopoi/Healthpractitionersandestablishments"/>
        <rdfs:comment>Hospitals is a subcategory of health practitioners and establishments</rdfs:comment>
        <rdfs:isDefinedBy rdf:resource="https://www.theworldavatar.com/kg/ontopoi"/>
        <rdfs:label>Hospitals</rdfs:label>
    </owl:Class>
    


    <!-- https://www.theworldavatar.com/kg/ontopoi/Hostelsandrefugesforthehomeless -->


    <owl:Class rdf:about="https://www.theworldavatar.com/kg/ontopoi/Hostelsandrefugesforthehomeless">
        <rdfs:subClassOf rdf:resource="https://www.theworldavatar.com/kg/ontopoi/Accommodation"/>
        <rdfs:comment>Hostels and refuges for the homeless is a subcategory of accommodation</rdfs:comment>
        <rdfs:isDefinedBy rdf:resource="https://www.theworldavatar.com/kg/ontopoi"/>
        <rdfs:label>Hostels and refuges for the homeless</rdfs:label>
    </owl:Class>
    


    <!-- https://www.theworldavatar.com/kg/ontopoi/Hotairballooning -->


    <owl:Class rdf:about="https://www.theworldavatar.com/kg/ontopoi/Hotairballooning">
        <rdfs:subClassOf rdf:resource="https://www.theworldavatar.com/kg/ontopoi/Outdoorpursuits"/>
        <rdfs:comment>Hot air ballooning is a subcategory of outdoor pursuits</rdfs:comment>
        <rdfs:isDefinedBy rdf:resource="https://www.theworldavatar.com/kg/ontopoi"/>
        <rdfs:label>Hot air ballooning</rdfs:label>
    </owl:Class>
    


    <!-- https://www.theworldavatar.com/kg/ontopoi/HotelBookingAgencies -->


    <owl:Class rdf:about="https://www.theworldavatar.com/kg/ontopoi/HotelBookingAgencies">
        <rdfs:subClassOf rdf:resource="https://www.theworldavatar.com/kg/ontopoi/Personalandconsumerandotherservices"/>
        <rdfs:comment>Hotel booking agencies is a subcategory of personal, consumer and other services</rdfs:comment>
        <rdfs:isDefinedBy rdf:resource="https://www.theworldavatar.com/kg/ontopoi"/>
        <rdfs:label>Hotel Booking Agencies</rdfs:label>
    </owl:Class>
    


    <!-- https://www.theworldavatar.com/kg/ontopoi/Hotelsandmotelsandcountryhousesandinns -->


    <owl:Class rdf:about="https://www.theworldavatar.com/kg/ontopoi/Hotelsandmotelsandcountryhousesandinns">
        <rdfs:subClassOf rdf:resource="https://www.theworldavatar.com/kg/ontopoi/Accommodation"/>
        <rdfs:comment>Hotels, motels, country houses and inns is a subcategory of accommodation</rdfs:comment>
        <rdfs:isDefinedBy rdf:resource="https://www.theworldavatar.com/kg/ontopoi"/>
        <rdfs:label>Hotels, motels, country houses and inns</rdfs:label>
    </owl:Class>
    


    <!-- https://www.theworldavatar.com/kg/ontopoi/Householdandofficeandleisureandgarden -->


    <owl:Class rdf:about="https://www.theworldavatar.com/kg/ontopoi/Householdandofficeandleisureandgarden">
        <rdfs:subClassOf rdf:resource="https://www.theworldavatar.com/kg/ontopoi/Retail"/>
        <rdfs:comment>Household, office, leisure and garden is a subcategory of retail</rdfs:comment>
        <rdfs:isDefinedBy rdf:resource="https://www.theworldavatar.com/kg/ontopoi"/>
        <rdfs:label>Household, office, leisure and garden</rdfs:label>
    </owl:Class>
    


    <!-- https://www.theworldavatar.com/kg/ontopoi/Householdrepairsandrestoration -->


    <owl:Class rdf:about="https://www.theworldavatar.com/kg/ontopoi/Householdrepairsandrestoration">
        <rdfs:subClassOf rdf:resource="https://www.theworldavatar.com/kg/ontopoi/Repairandservicing"/>
        <rdfs:comment>Household repairs and restoration is a subcategory of repair and servicing</rdfs:comment>
        <rdfs:isDefinedBy rdf:resource="https://www.theworldavatar.com/kg/ontopoi"/>
        <rdfs:label>Household repairs and restoration</rdfs:label>
    </owl:Class>
    


    <!-- https://www.theworldavatar.com/kg/ontopoi/Hydraulicengineers -->


    <owl:Class rdf:about="https://www.theworldavatar.com/kg/ontopoi/Hydraulicengineers">
        <rdfs:subClassOf rdf:resource="https://www.theworldavatar.com/kg/ontopoi/Engineeringservices"/>
        <rdfs:comment>Hydraulic engineers is a subcategory of engineering services</rdfs:comment>
        <rdfs:isDefinedBy rdf:resource="https://www.theworldavatar.com/kg/ontopoi"/>
        <rdfs:label>Hydraulic engineers</rdfs:label>
    </owl:Class>
    


    <!-- https://www.theworldavatar.com/kg/ontopoi/ITandadvertisingandmarketingandmediaservices -->


    <owl:Class rdf:about="https://www.theworldavatar.com/kg/ontopoi/ITandadvertisingandmarketingandmediaservices">
        <rdfs:subClassOf rdf:resource="https://www.theworldavatar.com/kg/ontopoi/Commercialservices"/>
        <rdfs:comment>It, advertising, marketing and media service s is a subcategory of commercial services</rdfs:comment>
        <rdfs:isDefinedBy rdf:resource="https://www.theworldavatar.com/kg/ontopoi"/>
        <rdfs:label>IT, advertising, marketing and media service s</rdfs:label>
    </owl:Class>
    


    <!-- https://www.theworldavatar.com/kg/ontopoi/Ice -->


    <owl:Class rdf:about="https://www.theworldavatar.com/kg/ontopoi/Ice">
        <rdfs:subClassOf rdf:resource="https://www.theworldavatar.com/kg/ontopoi/Industrialproducts"/>
        <rdfs:comment>Ice is a subcategory of industrial products</rdfs:comment>
        <rdfs:isDefinedBy rdf:resource="https://www.theworldavatar.com/kg/ontopoi"/>
        <rdfs:label>Ice</rdfs:label>
    </owl:Class>
    


    <!-- https://www.theworldavatar.com/kg/ontopoi/Icerinks -->


    <owl:Class rdf:about="https://www.theworldavatar.com/kg/ontopoi/Icerinks">
        <rdfs:subClassOf rdf:resource="https://www.theworldavatar.com/kg/ontopoi/Sportscomplex"/>
        <rdfs:comment>Ice rinks is a subcategory of sports complex</rdfs:comment>
        <rdfs:isDefinedBy rdf:resource="https://www.theworldavatar.com/kg/ontopoi"/>
        <rdfs:label>Ice rinks</rdfs:label>
    </owl:Class>
    


    <!-- https://www.theworldavatar.com/kg/ontopoi/Imageconsultants -->


    <owl:Class rdf:about="https://www.theworldavatar.com/kg/ontopoi/Imageconsultants">
        <rdfs:subClassOf rdf:resource="https://www.theworldavatar.com/kg/ontopoi/Consultancies"/>
        <rdfs:comment>Image consultants is a subcategory of consultancies</rdfs:comment>
        <rdfs:isDefinedBy rdf:resource="https://www.theworldavatar.com/kg/ontopoi"/>
        <rdfs:label>Image consultants</rdfs:label>
    </owl:Class>
    


    <!-- https://www.theworldavatar.com/kg/ontopoi/Importandexportservices -->


    <owl:Class rdf:about="https://www.theworldavatar.com/kg/ontopoi/Importandexportservices">
        <rdfs:subClassOf rdf:resource="https://www.theworldavatar.com/kg/ontopoi/Transportandstorageanddelivery"/>
        <rdfs:comment>Import and export services is a subcategory of transport, storage and delivery</rdfs:comment>
        <rdfs:isDefinedBy rdf:resource="https://www.theworldavatar.com/kg/ontopoi"/>
        <rdfs:label>Import and export services</rdfs:label>
    </owl:Class>
    


    <!-- https://www.theworldavatar.com/kg/ontopoi/Independentandpreparatoryschools -->


    <owl:Class rdf:about="https://www.theworldavatar.com/kg/ontopoi/Independentandpreparatoryschools">
        <rdfs:subClassOf rdf:resource="https://www.theworldavatar.com/kg/ontopoi/Primaryandsecondaryandtertiaryeducation"/>
        <rdfs:comment>Independent and preparatory schools is a subcategory of primary, secondary and tertiary education</rdfs:comment>
        <rdfs:isDefinedBy rdf:resource="https://www.theworldavatar.com/kg/ontopoi"/>
        <rdfs:label>Independent and preparatory schools</rdfs:label>
    </owl:Class>
    


    <!-- https://www.theworldavatar.com/kg/ontopoi/Industrialcoatingsandfinishings -->


    <owl:Class rdf:about="https://www.theworldavatar.com/kg/ontopoi/Industrialcoatingsandfinishings">
        <rdfs:subClassOf rdf:resource="https://www.theworldavatar.com/kg/ontopoi/Industrialproducts"/>
        <rdfs:comment>Industrial coatings and finishings is a subcategory of industrial products</rdfs:comment>
        <rdfs:isDefinedBy rdf:resource="https://www.theworldavatar.com/kg/ontopoi"/>
        <rdfs:label>Industrial coatings and finishings</rdfs:label>
    </owl:Class>
    


    <!-- https://www.theworldavatar.com/kg/ontopoi/Industrialengineers -->


    <owl:Class rdf:about="https://www.theworldavatar.com/kg/ontopoi/Industrialengineers">
        <rdfs:subClassOf rdf:resource="https://www.theworldavatar.com/kg/ontopoi/Engineeringservices"/>
        <rdfs:comment>Industrial engineers is a subcategory of engineering services</rdfs:comment>
        <rdfs:isDefinedBy rdf:resource="https://www.theworldavatar.com/kg/ontopoi"/>
        <rdfs:label>Industrial engineers</rdfs:label>
    </owl:Class>
    


    <!-- https://www.theworldavatar.com/kg/ontopoi/Industrialfeatures -->


    <owl:Class rdf:about="https://www.theworldavatar.com/kg/ontopoi/Industrialfeatures">
        <rdfs:subClassOf rdf:resource="https://www.theworldavatar.com/kg/ontopoi/Manufacturingandproduction"/>
        <rdfs:comment>Industrial features is a subcategory of manufacturing and production</rdfs:comment>
        <rdfs:isDefinedBy rdf:resource="https://www.theworldavatar.com/kg/ontopoi"/>
        <rdfs:label>Industrial features</rdfs:label>
    </owl:Class>
    


    <!-- https://www.theworldavatar.com/kg/ontopoi/Industrialproducts -->


    <owl:Class rdf:about="https://www.theworldavatar.com/kg/ontopoi/Industrialproducts">
        <rdfs:subClassOf rdf:resource="https://www.theworldavatar.com/kg/ontopoi/Manufacturingandproduction"/>
        <rdfs:comment>Industrial products is a subcategory of manufacturing and production</rdfs:comment>
        <rdfs:isDefinedBy rdf:resource="https://www.theworldavatar.com/kg/ontopoi"/>
        <rdfs:label>Industrial products</rdfs:label>
    </owl:Class>
    


    <!-- https://www.theworldavatar.com/kg/ontopoi/Industrialrepairsandservicing -->


    <owl:Class rdf:about="https://www.theworldavatar.com/kg/ontopoi/Industrialrepairsandservicing">
        <rdfs:subClassOf rdf:resource="https://www.theworldavatar.com/kg/ontopoi/Repairandservicing"/>
        <rdfs:comment>Industrial repairs and servicing is a subcategory of repair and servicing</rdfs:comment>
        <rdfs:isDefinedBy rdf:resource="https://www.theworldavatar.com/kg/ontopoi"/>
        <rdfs:label>Industrial repairs and servicing</rdfs:label>
    </owl:Class>
    


    <!-- https://www.theworldavatar.com/kg/ontopoi/Informationcentres -->


    <owl:Class rdf:about="https://www.theworldavatar.com/kg/ontopoi/Informationcentres">
        <rdfs:subClassOf rdf:resource="https://www.theworldavatar.com/kg/ontopoi/Tourism"/>
        <rdfs:comment>Information centres is a subcategory of tourism</rdfs:comment>
        <rdfs:isDefinedBy rdf:resource="https://www.theworldavatar.com/kg/ontopoi"/>
        <rdfs:label>Information centres</rdfs:label>
    </owl:Class>
    


    <!-- https://www.theworldavatar.com/kg/ontopoi/Infrastructureandfacilities -->


    <owl:Class rdf:about="https://www.theworldavatar.com/kg/ontopoi/Infrastructureandfacilities">
        <rdfs:subClassOf rdf:resource="https://www.theworldavatar.com/kg/ontopoi/Publicinfrastructure"/>
        <rdfs:comment>Infrastructure and facilities is a subcategory of public infrastructure</rdfs:comment>
        <rdfs:isDefinedBy rdf:resource="https://www.theworldavatar.com/kg/ontopoi"/>
        <rdfs:label>Infrastructure and facilities</rdfs:label>
    </owl:Class>
    


    <!-- https://www.theworldavatar.com/kg/ontopoi/Institutesandprofessionalorganisations -->


    <owl:Class rdf:about="https://www.theworldavatar.com/kg/ontopoi/Institutesandprofessionalorganisations">
        <rdfs:subClassOf rdf:resource="https://www.theworldavatar.com/kg/ontopoi/Organisations"/>
        <rdfs:comment>Institutes and professional organisations is a subcategory of organisations</rdfs:comment>
        <rdfs:isDefinedBy rdf:resource="https://www.theworldavatar.com/kg/ontopoi"/>
        <rdfs:label>Institutes and professional organisations</rdfs:label>
    </owl:Class>
    


    <!-- https://www.theworldavatar.com/kg/ontopoi/Instrumentationengineers -->


    <owl:Class rdf:about="https://www.theworldavatar.com/kg/ontopoi/Instrumentationengineers">
        <rdfs:subClassOf rdf:resource="https://www.theworldavatar.com/kg/ontopoi/Engineeringservices"/>
        <rdfs:comment>Instrumentation engineers is a subcategory of engineering services</rdfs:comment>
        <rdfs:isDefinedBy rdf:resource="https://www.theworldavatar.com/kg/ontopoi"/>
        <rdfs:label>Instrumentation engineers</rdfs:label>
    </owl:Class>
    


    <!-- https://www.theworldavatar.com/kg/ontopoi/Insurersandsupportactivities -->


    <owl:Class rdf:about="https://www.theworldavatar.com/kg/ontopoi/Insurersandsupportactivities">
        <rdfs:subClassOf rdf:resource="https://www.theworldavatar.com/kg/ontopoi/Legalandfinancial"/>
        <rdfs:comment>Insurers and support activities is a subcategory of legal and financial</rdfs:comment>
        <rdfs:isDefinedBy rdf:resource="https://www.theworldavatar.com/kg/ontopoi"/>
        <rdfs:label>Insurers and support activities</rdfs:label>
    </owl:Class>
    


    <!-- https://www.theworldavatar.com/kg/ontopoi/InternetCafes -->


    <owl:Class rdf:about="https://www.theworldavatar.com/kg/ontopoi/InternetCafes">
        <rdfs:subClassOf rdf:resource="https://www.theworldavatar.com/kg/ontopoi/Eatinganddrinking"/>
        <rdfs:comment>Internet cafes is a subcategory of eating and drinking</rdfs:comment>
        <rdfs:isDefinedBy rdf:resource="https://www.theworldavatar.com/kg/ontopoi"/>
        <rdfs:label>Internet Cafes</rdfs:label>
    </owl:Class>
    


    <!-- https://www.theworldavatar.com/kg/ontopoi/Internetservices -->


    <owl:Class rdf:about="https://www.theworldavatar.com/kg/ontopoi/Internetservices">
        <rdfs:subClassOf rdf:resource="https://www.theworldavatar.com/kg/ontopoi/ITandadvertisingandmarketingandmediaservices"/>
        <rdfs:comment>Internet services is a subcategory of it, advertising, marketing and media service s</rdfs:comment>
        <rdfs:isDefinedBy rdf:resource="https://www.theworldavatar.com/kg/ontopoi"/>
        <rdfs:label>Internet services</rdfs:label>
    </owl:Class>
    


    <!-- https://www.theworldavatar.com/kg/ontopoi/Interpretationandtranslationconsultants -->


    <owl:Class rdf:about="https://www.theworldavatar.com/kg/ontopoi/Interpretationandtranslationconsultants">
        <rdfs:subClassOf rdf:resource="https://www.theworldavatar.com/kg/ontopoi/Consultancies"/>
        <rdfs:comment>Interpretation and translation consultants is a subcategory of consultancies</rdfs:comment>
        <rdfs:isDefinedBy rdf:resource="https://www.theworldavatar.com/kg/ontopoi"/>
        <rdfs:label>Interpretation and translation consultants</rdfs:label>
    </owl:Class>
    


    <!-- https://www.theworldavatar.com/kg/ontopoi/Introductionanddatingagencies -->


    <owl:Class rdf:about="https://www.theworldavatar.com/kg/ontopoi/Introductionanddatingagencies">
        <rdfs:subClassOf rdf:resource="https://www.theworldavatar.com/kg/ontopoi/Personalandconsumerandotherservices"/>
        <rdfs:comment>Introduction and dating agencies is a subcategory of personal, consumer and other services</rdfs:comment>
        <rdfs:isDefinedBy rdf:resource="https://www.theworldavatar.com/kg/ontopoi"/>
        <rdfs:label>Introduction and dating agencies</rdfs:label>
    </owl:Class>
    


    <!-- https://www.theworldavatar.com/kg/ontopoi/Jewelleryandfashionaccessories -->


    <owl:Class rdf:about="https://www.theworldavatar.com/kg/ontopoi/Jewelleryandfashionaccessories">
        <rdfs:subClassOf rdf:resource="https://www.theworldavatar.com/kg/ontopoi/Clothingandaccessories"/>
        <rdfs:comment>Jewellery and fashion accessories is a subcategory of clothing and accessories</rdfs:comment>
        <rdfs:isDefinedBy rdf:resource="https://www.theworldavatar.com/kg/ontopoi"/>
        <rdfs:label>Jewellery and fashion accessories</rdfs:label>
    </owl:Class>
    


    <!-- https://www.theworldavatar.com/kg/ontopoi/Jewelleryandgemsandclocksandwatches -->


    <owl:Class rdf:about="https://www.theworldavatar.com/kg/ontopoi/Jewelleryandgemsandclocksandwatches">
        <rdfs:subClassOf rdf:resource="https://www.theworldavatar.com/kg/ontopoi/Consumerproducts"/>
        <rdfs:comment>Jewellery, gems, clocks and watches is a subcategory of consumer products</rdfs:comment>
        <rdfs:isDefinedBy rdf:resource="https://www.theworldavatar.com/kg/ontopoi"/>
        <rdfs:label>Jewellery, gems, clocks and watches</rdfs:label>
    </owl:Class>
    


    <!-- https://www.theworldavatar.com/kg/ontopoi/Jobcentres -->


    <owl:Class rdf:about="https://www.theworldavatar.com/kg/ontopoi/Jobcentres">
        <rdfs:subClassOf rdf:resource="https://www.theworldavatar.com/kg/ontopoi/Centralandlocalgovernment"/>
        <rdfs:comment>Job centres is a subcategory of central and local government</rdfs:comment>
        <rdfs:isDefinedBy rdf:resource="https://www.theworldavatar.com/kg/ontopoi"/>
        <rdfs:label>Job centres</rdfs:label>
    </owl:Class>
    


    <!-- https://www.theworldavatar.com/kg/ontopoi/Kennelsandcatteries -->


    <owl:Class rdf:about="https://www.theworldavatar.com/kg/ontopoi/Kennelsandcatteries">
        <rdfs:subClassOf rdf:resource="https://www.theworldavatar.com/kg/ontopoi/Animalwelfare"/>
        <rdfs:comment>Kennels and catteries is a subcategory of animal welfare</rdfs:comment>
        <rdfs:isDefinedBy rdf:resource="https://www.theworldavatar.com/kg/ontopoi"/>
        <rdfs:label>Kennels and catteries</rdfs:label>
    </owl:Class>
    


    <!-- https://www.theworldavatar.com/kg/ontopoi/Lakesandwaters -->


    <owl:Class rdf:about="https://www.theworldavatar.com/kg/ontopoi/Lakesandwaters">
        <rdfs:subClassOf rdf:resource="https://www.theworldavatar.com/kg/ontopoi/Bodiesofwater"/>
        <rdfs:comment>Lakes and waters is a subcategory of bodies of water</rdfs:comment>
        <rdfs:isDefinedBy rdf:resource="https://www.theworldavatar.com/kg/ontopoi"/>
        <rdfs:label>Lakes and waters</rdfs:label>
    </owl:Class>
    


    <!-- https://www.theworldavatar.com/kg/ontopoi/Lampshadesandlighting -->


    <owl:Class rdf:about="https://www.theworldavatar.com/kg/ontopoi/Lampshadesandlighting">
        <rdfs:subClassOf rdf:resource="https://www.theworldavatar.com/kg/ontopoi/Consumerproducts"/>
        <rdfs:comment>Lampshades and lighting is a subcategory of consumer products</rdfs:comment>
        <rdfs:isDefinedBy rdf:resource="https://www.theworldavatar.com/kg/ontopoi"/>
        <rdfs:label>Lampshades and lighting</rdfs:label>
    </owl:Class>
    


    <!-- https://www.theworldavatar.com/kg/ontopoi/Landscapefeatures -->


    <owl:Class rdf:about="https://www.theworldavatar.com/kg/ontopoi/Landscapefeatures">
        <rdfs:subClassOf rdf:resource="https://www.theworldavatar.com/kg/ontopoi/Attractions"/>
        <rdfs:comment>Landscape features is a subcategory of attractions</rdfs:comment>
        <rdfs:isDefinedBy rdf:resource="https://www.theworldavatar.com/kg/ontopoi"/>
        <rdfs:label>Landscape features</rdfs:label>
    </owl:Class>
    


    <!-- https://www.theworldavatar.com/kg/ontopoi/Languageschools -->


    <owl:Class rdf:about="https://www.theworldavatar.com/kg/ontopoi/Languageschools">
        <rdfs:subClassOf rdf:resource="https://www.theworldavatar.com/kg/ontopoi/Recreationalandvocationaleducation"/>
        <rdfs:comment>Language schools is a subcategory of recreational and vocational education</rdfs:comment>
        <rdfs:isDefinedBy rdf:resource="https://www.theworldavatar.com/kg/ontopoi"/>
        <rdfs:label>Language schools</rdfs:label>
    </owl:Class>
    


    <!-- https://www.theworldavatar.com/kg/ontopoi/Laseriaandobservatoriesandplanetaria -->


    <owl:Class rdf:about="https://www.theworldavatar.com/kg/ontopoi/Laseriaandobservatoriesandplanetaria">
        <rdfs:subClassOf rdf:resource="https://www.theworldavatar.com/kg/ontopoi/Tourism"/>
        <rdfs:comment>Laseria, observatories and planetaria is a subcategory of tourism</rdfs:comment>
        <rdfs:isDefinedBy rdf:resource="https://www.theworldavatar.com/kg/ontopoi"/>
        <rdfs:label>Laseria, observatories and planetaria</rdfs:label>
    </owl:Class>
    


    <!-- https://www.theworldavatar.com/kg/ontopoi/Leathergoodsandluggageandtravelaccessoriesincludinghandbags -->


    <owl:Class rdf:about="https://www.theworldavatar.com/kg/ontopoi/Leathergoodsandluggageandtravelaccessoriesincludinghandbags">
        <rdfs:subClassOf rdf:resource="https://www.theworldavatar.com/kg/ontopoi/Householdandofficeandleisureandgarden"/>
        <rdfs:comment>Leather goods, luggage and travel accessories including handbags is a subcategory of household, office, leisure and garden</rdfs:comment>
        <rdfs:isDefinedBy rdf:resource="https://www.theworldavatar.com/kg/ontopoi"/>
        <rdfs:label>Leather goods, luggage and travel accessories including handbags</rdfs:label>
    </owl:Class>
    


    <!-- https://www.theworldavatar.com/kg/ontopoi/Leatherproducts -->


    <owl:Class rdf:about="https://www.theworldavatar.com/kg/ontopoi/Leatherproducts">
        <rdfs:subClassOf rdf:resource="https://www.theworldavatar.com/kg/ontopoi/Consumerproducts"/>
        <rdfs:comment>Leather products is a subcategory of consumer products</rdfs:comment>
        <rdfs:isDefinedBy rdf:resource="https://www.theworldavatar.com/kg/ontopoi"/>
        <rdfs:label>Leather products</rdfs:label>
    </owl:Class>
    


    <!-- https://www.theworldavatar.com/kg/ontopoi/Legalandfinancial -->


    <owl:Class rdf:about="https://www.theworldavatar.com/kg/ontopoi/Legalandfinancial">
        <rdfs:subClassOf rdf:resource="https://www.theworldavatar.com/kg/ontopoi/Commercialservices"/>
        <rdfs:comment>Legal and financial is a subcategory of commercial services</rdfs:comment>
        <rdfs:isDefinedBy rdf:resource="https://www.theworldavatar.com/kg/ontopoi"/>
        <rdfs:label>Legal and financial</rdfs:label>
    </owl:Class>
    


    <!-- https://www.theworldavatar.com/kg/ontopoi/Leisureequipmenthirings -->


    <owl:Class rdf:about="https://www.theworldavatar.com/kg/ontopoi/Leisureequipmenthirings">
        <rdfs:subClassOf rdf:resource="https://www.theworldavatar.com/kg/ontopoi/Hireservices"/>
        <rdfs:comment>Leisure equipment hirings is a subcategory of hire services</rdfs:comment>
        <rdfs:isDefinedBy rdf:resource="https://www.theworldavatar.com/kg/ontopoi"/>
        <rdfs:label>Leisure equipment hirings</rdfs:label>
    </owl:Class>
    


    <!-- https://www.theworldavatar.com/kg/ontopoi/Letterboxes -->


    <owl:Class rdf:about="https://www.theworldavatar.com/kg/ontopoi/Letterboxes">
        <rdfs:subClassOf rdf:resource="https://www.theworldavatar.com/kg/ontopoi/Infrastructureandfacilities"/>
        <rdfs:comment>Letter boxes is a subcategory of infrastructure and facilities</rdfs:comment>
        <rdfs:isDefinedBy rdf:resource="https://www.theworldavatar.com/kg/ontopoi"/>
        <rdfs:label>Letter boxes</rdfs:label>
    </owl:Class>
    


    <!-- https://www.theworldavatar.com/kg/ontopoi/Libraries -->


    <owl:Class rdf:about="https://www.theworldavatar.com/kg/ontopoi/Libraries">
        <rdfs:subClassOf rdf:resource="https://www.theworldavatar.com/kg/ontopoi/Infrastructureandfacilities"/>
        <rdfs:comment>Libraries is a subcategory of infrastructure and facilities</rdfs:comment>
        <rdfs:isDefinedBy rdf:resource="https://www.theworldavatar.com/kg/ontopoi"/>
        <rdfs:label>Libraries</rdfs:label>
    </owl:Class>
    


    <!-- https://www.theworldavatar.com/kg/ontopoi/Liftingandhandlingequipment -->


    <owl:Class rdf:about="https://www.theworldavatar.com/kg/ontopoi/Liftingandhandlingequipment">
        <rdfs:subClassOf rdf:resource="https://www.theworldavatar.com/kg/ontopoi/Industrialproducts"/>
        <rdfs:comment>Lifting and handling equipment is a subcategory of industrial products</rdfs:comment>
        <rdfs:isDefinedBy rdf:resource="https://www.theworldavatar.com/kg/ontopoi"/>
        <rdfs:label>Lifting and handling equipment</rdfs:label>
    </owl:Class>
    


    <!-- https://www.theworldavatar.com/kg/ontopoi/Lighting -->


    <owl:Class rdf:about="https://www.theworldavatar.com/kg/ontopoi/Lighting">
        <rdfs:subClassOf rdf:resource="https://www.theworldavatar.com/kg/ontopoi/Householdandofficeandleisureandgarden"/>
        <rdfs:comment>Lighting is a subcategory of household, office, leisure and garden</rdfs:comment>
        <rdfs:isDefinedBy rdf:resource="https://www.theworldavatar.com/kg/ontopoi"/>
        <rdfs:label>Lighting</rdfs:label>
    </owl:Class>
    


    <!-- https://www.theworldavatar.com/kg/ontopoi/Limekilns -->


    <owl:Class rdf:about="https://www.theworldavatar.com/kg/ontopoi/Limekilns">
        <rdfs:subClassOf rdf:resource="https://www.theworldavatar.com/kg/ontopoi/Industrialfeatures"/>
        <rdfs:comment>Lime kilns is a subcategory of industrial features</rdfs:comment>
        <rdfs:isDefinedBy rdf:resource="https://www.theworldavatar.com/kg/ontopoi"/>
        <rdfs:label>Lime kilns</rdfs:label>
    </owl:Class>
    


    <!-- https://www.theworldavatar.com/kg/ontopoi/Linenhireandwashroomservices -->


    <owl:Class rdf:about="https://www.theworldavatar.com/kg/ontopoi/Linenhireandwashroomservices">
        <rdfs:subClassOf rdf:resource="https://www.theworldavatar.com/kg/ontopoi/Contractservices"/>
        <rdfs:comment>Linen hire and washroom services is a subcategory of contract services</rdfs:comment>
        <rdfs:isDefinedBy rdf:resource="https://www.theworldavatar.com/kg/ontopoi"/>
        <rdfs:label>Linen hire and washroom services</rdfs:label>
    </owl:Class>
    


    <!-- https://www.theworldavatar.com/kg/ontopoi/Lingerieandhosiery -->


    <owl:Class rdf:about="https://www.theworldavatar.com/kg/ontopoi/Lingerieandhosiery">
        <rdfs:subClassOf rdf:resource="https://www.theworldavatar.com/kg/ontopoi/Clothingandaccessories"/>
        <rdfs:subClassOf rdf:resource="https://www.theworldavatar.com/kg/ontopoi/Consumerproducts"/>
        <rdfs:comment>Lingerie and hosiery is a subcategory of clothing and accessories</rdfs:comment>
        <rdfs:comment>Lingerie and hosiery is a subcategory of consumer products</rdfs:comment>
        <rdfs:isDefinedBy rdf:resource="https://www.theworldavatar.com/kg/ontopoi"/>
        <rdfs:label>Lingerie and hosiery</rdfs:label>
    </owl:Class>
    


    <!-- https://www.theworldavatar.com/kg/ontopoi/Literaryservices -->


    <owl:Class rdf:about="https://www.theworldavatar.com/kg/ontopoi/Literaryservices">
        <rdfs:subClassOf rdf:resource="https://www.theworldavatar.com/kg/ontopoi/ITandadvertisingandmarketingandmediaservices"/>
        <rdfs:comment>Literary services is a subcategory of it, advertising, marketing and media service s</rdfs:comment>
        <rdfs:isDefinedBy rdf:resource="https://www.theworldavatar.com/kg/ontopoi"/>
        <rdfs:label>Literary services</rdfs:label>
    </owl:Class>
    


    <!-- https://www.theworldavatar.com/kg/ontopoi/Livestockfarming -->


    <owl:Class rdf:about="https://www.theworldavatar.com/kg/ontopoi/Livestockfarming">
        <rdfs:subClassOf rdf:resource="https://www.theworldavatar.com/kg/ontopoi/Farming"/>
        <rdfs:comment>Livestock farming is a subcategory of farming</rdfs:comment>
        <rdfs:isDefinedBy rdf:resource="https://www.theworldavatar.com/kg/ontopoi"/>
        <rdfs:label>Livestock farming</rdfs:label>
    </owl:Class>
    


    <!-- https://www.theworldavatar.com/kg/ontopoi/Livestockmarkets -->


    <owl:Class rdf:about="https://www.theworldavatar.com/kg/ontopoi/Livestockmarkets">
        <rdfs:subClassOf rdf:resource="https://www.theworldavatar.com/kg/ontopoi/Foodanddrinkandmultiitemretail"/>
        <rdfs:comment>Livestock markets is a subcategory of food, drink and multi item retail</rdfs:comment>
        <rdfs:isDefinedBy rdf:resource="https://www.theworldavatar.com/kg/ontopoi"/>
        <rdfs:label>Livestock markets</rdfs:label>
    </owl:Class>
    


    <!-- https://www.theworldavatar.com/kg/ontopoi/Localgovernment -->


    <owl:Class rdf:about="https://www.theworldavatar.com/kg/ontopoi/Localgovernment">
        <rdfs:subClassOf rdf:resource="https://www.theworldavatar.com/kg/ontopoi/Centralandlocalgovernment"/>
        <rdfs:comment>Local government is a subcategory of central and local government</rdfs:comment>
        <rdfs:isDefinedBy rdf:resource="https://www.theworldavatar.com/kg/ontopoi"/>
        <rdfs:label>Local government</rdfs:label>
    </owl:Class>
    


    <!-- https://www.theworldavatar.com/kg/ontopoi/Lochsandlochans -->


    <owl:Class rdf:about="https://www.theworldavatar.com/kg/ontopoi/Lochsandlochans">
        <rdfs:subClassOf rdf:resource="https://www.theworldavatar.com/kg/ontopoi/Bodiesofwater"/>
        <rdfs:comment>Lochs and lochans is a subcategory of bodies of water</rdfs:comment>
        <rdfs:isDefinedBy rdf:resource="https://www.theworldavatar.com/kg/ontopoi"/>
        <rdfs:label>Lochs and lochans</rdfs:label>
    </owl:Class>
    


    <!-- https://www.theworldavatar.com/kg/ontopoi/Lockandkeyandsecurityservices -->


    <owl:Class rdf:about="https://www.theworldavatar.com/kg/ontopoi/Lockandkeyandsecurityservices">
        <rdfs:subClassOf rdf:resource="https://www.theworldavatar.com/kg/ontopoi/Personalandconsumerandotherservices"/>
        <rdfs:comment>Lock, key and security services is a subcategory of personal, consumer and other services</rdfs:comment>
        <rdfs:isDefinedBy rdf:resource="https://www.theworldavatar.com/kg/ontopoi"/>
        <rdfs:label>Lock, key and security services</rdfs:label>
    </owl:Class>
    


    <!-- https://www.theworldavatar.com/kg/ontopoi/Locks -->


    <owl:Class rdf:about="https://www.theworldavatar.com/kg/ontopoi/Locks">
        <rdfs:subClassOf rdf:resource="https://www.theworldavatar.com/kg/ontopoi/Water"/>
        <rdfs:comment>Locks is a subcategory of water</rdfs:comment>
        <rdfs:isDefinedBy rdf:resource="https://www.theworldavatar.com/kg/ontopoi"/>
        <rdfs:label>Locks</rdfs:label>
    </owl:Class>
    


    <!-- https://www.theworldavatar.com/kg/ontopoi/LondonUndergroundentrances -->


    <owl:Class rdf:about="https://www.theworldavatar.com/kg/ontopoi/LondonUndergroundentrances">
        <rdfs:subClassOf rdf:resource="https://www.theworldavatar.com/kg/ontopoi/Publictransportandstationsandinfrastructure"/>
        <rdfs:comment>London underground entrances is a subcategory of public transport, stations and infrastructure</rdfs:comment>
        <rdfs:isDefinedBy rdf:resource="https://www.theworldavatar.com/kg/ontopoi"/>
        <rdfs:label>London Underground entrances</rdfs:label>
    </owl:Class>
    


    <!-- https://www.theworldavatar.com/kg/ontopoi/Lubricantsandlubricatingequipment -->


    <owl:Class rdf:about="https://www.theworldavatar.com/kg/ontopoi/Lubricantsandlubricatingequipment">
        <rdfs:subClassOf rdf:resource="https://www.theworldavatar.com/kg/ontopoi/Industrialproducts"/>
        <rdfs:comment>Lubricants and lubricating equipment is a subcategory of industrial products</rdfs:comment>
        <rdfs:isDefinedBy rdf:resource="https://www.theworldavatar.com/kg/ontopoi"/>
        <rdfs:label>Lubricants and lubricating equipment</rdfs:label>
    </owl:Class>
    


    <!-- https://www.theworldavatar.com/kg/ontopoi/Luggageandbagsandumbrellasandtravelaccessories -->


    <owl:Class rdf:about="https://www.theworldavatar.com/kg/ontopoi/Luggageandbagsandumbrellasandtravelaccessories">
        <rdfs:subClassOf rdf:resource="https://www.theworldavatar.com/kg/ontopoi/Consumerproducts"/>
        <rdfs:comment>Luggage, bags, umbrellas and travel accessories is a subcategory of consumer products</rdfs:comment>
        <rdfs:isDefinedBy rdf:resource="https://www.theworldavatar.com/kg/ontopoi"/>
        <rdfs:label>Luggage, bags, umbrellas and travel accessories</rdfs:label>
    </owl:Class>
    


    <!-- https://www.theworldavatar.com/kg/ontopoi/Mailingandotherinformationservices -->


    <owl:Class rdf:about="https://www.theworldavatar.com/kg/ontopoi/Mailingandotherinformationservices">
        <rdfs:subClassOf rdf:resource="https://www.theworldavatar.com/kg/ontopoi/ITandadvertisingandmarketingandmediaservices"/>
        <rdfs:comment>Mailing and other information services is a subcategory of it, advertising, marketing and media service s</rdfs:comment>
        <rdfs:isDefinedBy rdf:resource="https://www.theworldavatar.com/kg/ontopoi"/>
        <rdfs:label>Mailing and other information services</rdfs:label>
    </owl:Class>
    


    <!-- https://www.theworldavatar.com/kg/ontopoi/Mailorderandcataloguestores -->


    <owl:Class rdf:about="https://www.theworldavatar.com/kg/ontopoi/Mailorderandcataloguestores">
        <rdfs:subClassOf rdf:resource="https://www.theworldavatar.com/kg/ontopoi/Householdandofficeandleisureandgarden"/>
        <rdfs:comment>Mail order and catalogue stores is a subcategory of household, office, leisure and garden</rdfs:comment>
        <rdfs:isDefinedBy rdf:resource="https://www.theworldavatar.com/kg/ontopoi"/>
        <rdfs:label>Mail order and catalogue stores</rdfs:label>
    </owl:Class>
    


    <!-- https://www.theworldavatar.com/kg/ontopoi/Manufacturingandproduction -->


    <owl:Class rdf:about="https://www.theworldavatar.com/kg/ontopoi/Manufacturingandproduction"/>
    


    <!-- https://www.theworldavatar.com/kg/ontopoi/Marineengineersandservices -->


    <owl:Class rdf:about="https://www.theworldavatar.com/kg/ontopoi/Marineengineersandservices">
        <rdfs:subClassOf rdf:resource="https://www.theworldavatar.com/kg/ontopoi/Engineeringservices"/>
        <rdfs:comment>Marine engineers and services is a subcategory of engineering services</rdfs:comment>
        <rdfs:isDefinedBy rdf:resource="https://www.theworldavatar.com/kg/ontopoi"/>
        <rdfs:label>Marine engineers and services</rdfs:label>
    </owl:Class>
    


    <!-- https://www.theworldavatar.com/kg/ontopoi/Marineequipmentincludingboatsandships -->


    <owl:Class rdf:about="https://www.theworldavatar.com/kg/ontopoi/Marineequipmentincludingboatsandships">
        <rdfs:subClassOf rdf:resource="https://www.theworldavatar.com/kg/ontopoi/Industrialproducts"/>
        <rdfs:comment>Marine equipment including boats and ships is a subcategory of industrial products</rdfs:comment>
        <rdfs:isDefinedBy rdf:resource="https://www.theworldavatar.com/kg/ontopoi"/>
        <rdfs:label>Marine equipment including boats and ships</rdfs:label>
    </owl:Class>
    


    <!-- https://www.theworldavatar.com/kg/ontopoi/Marketingservices -->


    <owl:Class rdf:about="https://www.theworldavatar.com/kg/ontopoi/Marketingservices">
        <rdfs:subClassOf rdf:resource="https://www.theworldavatar.com/kg/ontopoi/ITandadvertisingandmarketingandmediaservices"/>
        <rdfs:comment>Marketing services is a subcategory of it, advertising, marketing and media service s</rdfs:comment>
        <rdfs:isDefinedBy rdf:resource="https://www.theworldavatar.com/kg/ontopoi"/>
        <rdfs:label>Marketing services</rdfs:label>
    </owl:Class>
    


    <!-- https://www.theworldavatar.com/kg/ontopoi/Markets -->


    <owl:Class rdf:about="https://www.theworldavatar.com/kg/ontopoi/Markets">
        <rdfs:subClassOf rdf:resource="https://www.theworldavatar.com/kg/ontopoi/Foodanddrinkandmultiitemretail"/>
        <rdfs:comment>Markets is a subcategory of food, drink and multi item retail</rdfs:comment>
        <rdfs:isDefinedBy rdf:resource="https://www.theworldavatar.com/kg/ontopoi"/>
        <rdfs:label>Markets</rdfs:label>
    </owl:Class>
    


    <!-- https://www.theworldavatar.com/kg/ontopoi/Martialartsinstruction -->


    <owl:Class rdf:about="https://www.theworldavatar.com/kg/ontopoi/Martialartsinstruction">
        <rdfs:subClassOf rdf:resource="https://www.theworldavatar.com/kg/ontopoi/Recreationalandvocationaleducation"/>
        <rdfs:comment>Martial arts instruction is a subcategory of recreational and vocational education</rdfs:comment>
        <rdfs:isDefinedBy rdf:resource="https://www.theworldavatar.com/kg/ontopoi"/>
        <rdfs:label>Martial arts instruction</rdfs:label>
    </owl:Class>
    


    <!-- https://www.theworldavatar.com/kg/ontopoi/Measurementandinspectionequipment -->


    <owl:Class rdf:about="https://www.theworldavatar.com/kg/ontopoi/Measurementandinspectionequipment">
        <rdfs:subClassOf rdf:resource="https://www.theworldavatar.com/kg/ontopoi/Industrialproducts"/>
        <rdfs:comment>Measurement and inspection equipment is a subcategory of industrial products</rdfs:comment>
        <rdfs:isDefinedBy rdf:resource="https://www.theworldavatar.com/kg/ontopoi"/>
        <rdfs:label>Measurement and inspection equipment</rdfs:label>
    </owl:Class>
    


    <!-- https://www.theworldavatar.com/kg/ontopoi/Mechanicalengineers -->


    <owl:Class rdf:about="https://www.theworldavatar.com/kg/ontopoi/Mechanicalengineers">
        <rdfs:subClassOf rdf:resource="https://www.theworldavatar.com/kg/ontopoi/Engineeringservices"/>
        <rdfs:comment>Mechanical engineers is a subcategory of engineering services</rdfs:comment>
        <rdfs:isDefinedBy rdf:resource="https://www.theworldavatar.com/kg/ontopoi"/>
        <rdfs:label>Mechanical engineers</rdfs:label>
    </owl:Class>
    


    <!-- https://www.theworldavatar.com/kg/ontopoi/Medalsandtrophiesandceremonialandreligiousgoods -->


    <owl:Class rdf:about="https://www.theworldavatar.com/kg/ontopoi/Medalsandtrophiesandceremonialandreligiousgoods">
        <rdfs:subClassOf rdf:resource="https://www.theworldavatar.com/kg/ontopoi/Consumerproducts"/>
        <rdfs:comment>Medals, trophies, ceremonial and religious goods is a subcategory of consumer products</rdfs:comment>
        <rdfs:isDefinedBy rdf:resource="https://www.theworldavatar.com/kg/ontopoi"/>
        <rdfs:label>Medals, trophies, ceremonial and religious goods</rdfs:label>
    </owl:Class>
    


    <!-- https://www.theworldavatar.com/kg/ontopoi/Medicalequipmentandsuppliesandpharmaceuticals -->


    <owl:Class rdf:about="https://www.theworldavatar.com/kg/ontopoi/Medicalequipmentandsuppliesandpharmaceuticals">
        <rdfs:subClassOf rdf:resource="https://www.theworldavatar.com/kg/ontopoi/Industrialproducts"/>
        <rdfs:comment>Medical equipment, supplies and pharm aceuticals is a subcategory of industrial products</rdfs:comment>
        <rdfs:isDefinedBy rdf:resource="https://www.theworldavatar.com/kg/ontopoi"/>
        <rdfs:label>Medical equipment, supplies and pharm aceuticals</rdfs:label>
    </owl:Class>
    


    <!-- https://www.theworldavatar.com/kg/ontopoi/Medicalequipmentrentalandleasing -->


    <owl:Class rdf:about="https://www.theworldavatar.com/kg/ontopoi/Medicalequipmentrentalandleasing">
        <rdfs:subClassOf rdf:resource="https://www.theworldavatar.com/kg/ontopoi/Healthsupportservices"/>
        <rdfs:comment>Medical equipment rental and leasing is a subcategory of health support services</rdfs:comment>
        <rdfs:isDefinedBy rdf:resource="https://www.theworldavatar.com/kg/ontopoi"/>
        <rdfs:label>Medical equipment rental and leasing</rdfs:label>
    </owl:Class>
    


    <!-- https://www.theworldavatar.com/kg/ontopoi/Medicalwastedisposalservices -->


    <owl:Class rdf:about="https://www.theworldavatar.com/kg/ontopoi/Medicalwastedisposalservices">
        <rdfs:subClassOf rdf:resource="https://www.theworldavatar.com/kg/ontopoi/Healthsupportservices"/>
        <rdfs:comment>Medical waste disposal services is a subcategory of health support services</rdfs:comment>
        <rdfs:isDefinedBy rdf:resource="https://www.theworldavatar.com/kg/ontopoi"/>
        <rdfs:label>Medical waste disposal services</rdfs:label>
    </owl:Class>
    


    <!-- https://www.theworldavatar.com/kg/ontopoi/MembersofparliamentandmembersofEuropeanparliament -->


    <owl:Class rdf:about="https://www.theworldavatar.com/kg/ontopoi/MembersofparliamentandmembersofEuropeanparliament">
        <rdfs:subClassOf rdf:resource="https://www.theworldavatar.com/kg/ontopoi/Centralandlocalgovernment"/>
        <rdfs:comment>Members of parliament and members of european parliament is a subcategory of central and local government</rdfs:comment>
        <rdfs:isDefinedBy rdf:resource="https://www.theworldavatar.com/kg/ontopoi"/>
        <rdfs:label>Members of parliament and members of European parliament</rdfs:label>
    </owl:Class>
    


    <!-- https://www.theworldavatar.com/kg/ontopoi/Mentalhealthcentresandpractitioners -->


    <owl:Class rdf:about="https://www.theworldavatar.com/kg/ontopoi/Mentalhealthcentresandpractitioners">
        <rdfs:subClassOf rdf:resource="https://www.theworldavatar.com/kg/ontopoi/Healthpractitionersandestablishments"/>
        <rdfs:comment>Mental health centres and practitioners is a subcategory of health practitioners and establishments</rdfs:comment>
        <rdfs:isDefinedBy rdf:resource="https://www.theworldavatar.com/kg/ontopoi"/>
        <rdfs:label>Mental health centres and practitioners</rdfs:label>
    </owl:Class>
    


    <!-- https://www.theworldavatar.com/kg/ontopoi/Messageandgreetingservices -->


    <owl:Class rdf:about="https://www.theworldavatar.com/kg/ontopoi/Messageandgreetingservices">
        <rdfs:subClassOf rdf:resource="https://www.theworldavatar.com/kg/ontopoi/Personalandconsumerandotherservices"/>
        <rdfs:comment>Message and greeting services is a subcategory of personal, consumer and other services</rdfs:comment>
        <rdfs:isDefinedBy rdf:resource="https://www.theworldavatar.com/kg/ontopoi"/>
        <rdfs:label>Message and greeting services</rdfs:label>
    </owl:Class>
    


    <!-- https://www.theworldavatar.com/kg/ontopoi/Metalsmanufacturersandfabricatorsandstockholders -->


    <owl:Class rdf:about="https://www.theworldavatar.com/kg/ontopoi/Metalsmanufacturersandfabricatorsandstockholders">
        <rdfs:subClassOf rdf:resource="https://www.theworldavatar.com/kg/ontopoi/Industrialproducts"/>
        <rdfs:comment>Metals manufacturers, fabricators and stockholders is a subcategory of industrial products</rdfs:comment>
        <rdfs:isDefinedBy rdf:resource="https://www.theworldavatar.com/kg/ontopoi"/>
        <rdfs:label>Metals manufacturers, fabricators and stockholders</rdfs:label>
    </owl:Class>
    


    <!-- https://www.theworldavatar.com/kg/ontopoi/Metalworkersincludingblacksmiths -->


    <owl:Class rdf:about="https://www.theworldavatar.com/kg/ontopoi/Metalworkersincludingblacksmiths">
        <rdfs:subClassOf rdf:resource="https://www.theworldavatar.com/kg/ontopoi/Constructionservices"/>
        <rdfs:comment>Metalworkers including blacksmiths is a subcategory of construction services</rdfs:comment>
        <rdfs:isDefinedBy rdf:resource="https://www.theworldavatar.com/kg/ontopoi"/>
        <rdfs:label>Metalworkers including blacksmiths</rdfs:label>
    </owl:Class>
    


    <!-- https://www.theworldavatar.com/kg/ontopoi/Meteorologicalfeatures -->


    <owl:Class rdf:about="https://www.theworldavatar.com/kg/ontopoi/Meteorologicalfeatures">
        <rdfs:subClassOf rdf:resource="https://www.theworldavatar.com/kg/ontopoi/Infrastructureandfacilities"/>
        <rdfs:comment>Meteorological features is a subcategory of infrastructure and facilities</rdfs:comment>
        <rdfs:isDefinedBy rdf:resource="https://www.theworldavatar.com/kg/ontopoi"/>
        <rdfs:label>Meteorological features</rdfs:label>
    </owl:Class>
    


    <!-- https://www.theworldavatar.com/kg/ontopoi/Midwifery -->


    <owl:Class rdf:about="https://www.theworldavatar.com/kg/ontopoi/Midwifery">
        <rdfs:subClassOf rdf:resource="https://www.theworldavatar.com/kg/ontopoi/Healthpractitionersandestablishments"/>
        <rdfs:comment>Midwifery is a subcategory of health practitioners and establishments</rdfs:comment>
        <rdfs:isDefinedBy rdf:resource="https://www.theworldavatar.com/kg/ontopoi"/>
        <rdfs:label>Midwifery</rdfs:label>
    </owl:Class>
    


    <!-- https://www.theworldavatar.com/kg/ontopoi/Millingandrefiningandfoodadditives -->


    <owl:Class rdf:about="https://www.theworldavatar.com/kg/ontopoi/Millingandrefiningandfoodadditives">
        <rdfs:subClassOf rdf:resource="https://www.theworldavatar.com/kg/ontopoi/Foodstuffs"/>
        <rdfs:comment>Milling, refining and food additives is a subcategory of foodstuffs</rdfs:comment>
        <rdfs:isDefinedBy rdf:resource="https://www.theworldavatar.com/kg/ontopoi"/>
        <rdfs:label>Milling, refining and food additives</rdfs:label>
    </owl:Class>
    


    <!-- https://www.theworldavatar.com/kg/ontopoi/Mixedorunspecifiedfarming -->


    <owl:Class rdf:about="https://www.theworldavatar.com/kg/ontopoi/Mixedorunspecifiedfarming">
        <rdfs:subClassOf rdf:resource="https://www.theworldavatar.com/kg/ontopoi/Farming"/>
        <rdfs:comment>Mixed or unspecified farming is a subcategory of farming</rdfs:comment>
        <rdfs:isDefinedBy rdf:resource="https://www.theworldavatar.com/kg/ontopoi"/>
        <rdfs:label>Mixed or unspecified farming</rdfs:label>
    </owl:Class>
    


    <!-- https://www.theworldavatar.com/kg/ontopoi/Mobilediscos -->


    <owl:Class rdf:about="https://www.theworldavatar.com/kg/ontopoi/Mobilediscos">
        <rdfs:subClassOf rdf:resource="https://www.theworldavatar.com/kg/ontopoi/Sportandentertainmentsupportservices"/>
        <rdfs:comment>Mobile discos is a subcategory of sport and entertainment support services</rdfs:comment>
        <rdfs:isDefinedBy rdf:resource="https://www.theworldavatar.com/kg/ontopoi"/>
        <rdfs:label>Mobile discos</rdfs:label>
    </owl:Class>
    


    <!-- https://www.theworldavatar.com/kg/ontopoi/Modellingandtheatricalagencies -->


    <owl:Class rdf:about="https://www.theworldavatar.com/kg/ontopoi/Modellingandtheatricalagencies">
        <rdfs:subClassOf rdf:resource="https://www.theworldavatar.com/kg/ontopoi/Employmentandcareeragencies"/>
        <rdfs:comment>Modelling and theatrical agencies is a subcategory of employment and career agencies</rdfs:comment>
        <rdfs:isDefinedBy rdf:resource="https://www.theworldavatar.com/kg/ontopoi"/>
        <rdfs:label>Modelling and theatrical agencies</rdfs:label>
    </owl:Class>
    


    <!-- https://www.theworldavatar.com/kg/ontopoi/Modelvillages -->


    <owl:Class rdf:about="https://www.theworldavatar.com/kg/ontopoi/Modelvillages">
        <rdfs:subClassOf rdf:resource="https://www.theworldavatar.com/kg/ontopoi/Tourism"/>
        <rdfs:comment>Model villages is a subcategory of tourism</rdfs:comment>
        <rdfs:isDefinedBy rdf:resource="https://www.theworldavatar.com/kg/ontopoi"/>
        <rdfs:label>Model villages</rdfs:label>
    </owl:Class>
    


    <!-- https://www.theworldavatar.com/kg/ontopoi/Mooringsandunloadingfacilities -->


    <owl:Class rdf:about="https://www.theworldavatar.com/kg/ontopoi/Mooringsandunloadingfacilities">
        <rdfs:subClassOf rdf:resource="https://www.theworldavatar.com/kg/ontopoi/Water"/>
        <rdfs:comment>Moorings and unloading facilities is a subcategory of water</rdfs:comment>
        <rdfs:isDefinedBy rdf:resource="https://www.theworldavatar.com/kg/ontopoi"/>
        <rdfs:label>Moorings and unloading facilities</rdfs:label>
    </owl:Class>
    


    <!-- https://www.theworldavatar.com/kg/ontopoi/Mortgageandfinanciallenders -->


    <owl:Class rdf:about="https://www.theworldavatar.com/kg/ontopoi/Mortgageandfinanciallenders">
        <rdfs:subClassOf rdf:resource="https://www.theworldavatar.com/kg/ontopoi/Legalandfinancial"/>
        <rdfs:comment>Mortgage and financial lenders is a subcategory of legal and financial</rdfs:comment>
        <rdfs:isDefinedBy rdf:resource="https://www.theworldavatar.com/kg/ontopoi"/>
        <rdfs:label>Mortgage and financial lenders</rdfs:label>
    </owl:Class>
    


    <!-- https://www.theworldavatar.com/kg/ontopoi/Motoring -->


    <owl:Class rdf:about="https://www.theworldavatar.com/kg/ontopoi/Motoring">
        <rdfs:subClassOf rdf:resource="https://www.theworldavatar.com/kg/ontopoi/Retail"/>
        <rdfs:comment>Motoring is a subcategory of retail</rdfs:comment>
        <rdfs:isDefinedBy rdf:resource="https://www.theworldavatar.com/kg/ontopoi"/>
        <rdfs:label>Motoring</rdfs:label>
    </owl:Class>
    


    <!-- https://www.theworldavatar.com/kg/ontopoi/Motoringorganisations -->


    <owl:Class rdf:about="https://www.theworldavatar.com/kg/ontopoi/Motoringorganisations">
        <rdfs:subClassOf rdf:resource="https://www.theworldavatar.com/kg/ontopoi/Personalandconsumerandotherservices"/>
        <rdfs:comment>Motoring organisations is a subcategory of personal, consumer and other services</rdfs:comment>
        <rdfs:isDefinedBy rdf:resource="https://www.theworldavatar.com/kg/ontopoi"/>
        <rdfs:label>Motoring organisations</rdfs:label>
    </owl:Class>
    


    <!-- https://www.theworldavatar.com/kg/ontopoi/Motorsportservices -->


    <owl:Class rdf:about="https://www.theworldavatar.com/kg/ontopoi/Motorsportservices">
        <rdfs:subClassOf rdf:resource="https://www.theworldavatar.com/kg/ontopoi/Sportandentertainmentsupportservices"/>
        <rdfs:comment>Motorsport services is a subcategory of sport and entertainment support services</rdfs:comment>
        <rdfs:isDefinedBy rdf:resource="https://www.theworldavatar.com/kg/ontopoi"/>
        <rdfs:label>Motorsport services</rdfs:label>
    </owl:Class>
    


    <!-- https://www.theworldavatar.com/kg/ontopoi/Motorsportvenues -->


    <owl:Class rdf:about="https://www.theworldavatar.com/kg/ontopoi/Motorsportvenues">
        <rdfs:subClassOf rdf:resource="https://www.theworldavatar.com/kg/ontopoi/Sportscomplex"/>
        <rdfs:comment>Motorsport venues is a subcategory of sports complex</rdfs:comment>
        <rdfs:isDefinedBy rdf:resource="https://www.theworldavatar.com/kg/ontopoi"/>
        <rdfs:label>Motorsport venues</rdfs:label>
    </owl:Class>
    


    <!-- https://www.theworldavatar.com/kg/ontopoi/Motorwayservicestations -->


    <owl:Class rdf:about="https://www.theworldavatar.com/kg/ontopoi/Motorwayservicestations">
        <rdfs:subClassOf rdf:resource="https://www.theworldavatar.com/kg/ontopoi/Roadandrail"/>
        <rdfs:comment>Motorway service stations is a subcategory of road and rail</rdfs:comment>
        <rdfs:isDefinedBy rdf:resource="https://www.theworldavatar.com/kg/ontopoi"/>
        <rdfs:label>Motorway service stations</rdfs:label>
    </owl:Class>
    


    <!-- https://www.theworldavatar.com/kg/ontopoi/Mouldsanddiesandcastings -->


    <owl:Class rdf:about="https://www.theworldavatar.com/kg/ontopoi/Mouldsanddiesandcastings">
        <rdfs:subClassOf rdf:resource="https://www.theworldavatar.com/kg/ontopoi/Industrialproducts"/>
        <rdfs:comment>Moulds, dies and castings is a subcategory of industrial products</rdfs:comment>
        <rdfs:isDefinedBy rdf:resource="https://www.theworldavatar.com/kg/ontopoi"/>
        <rdfs:label>Moulds, dies and castings</rdfs:label>
    </owl:Class>
    


    <!-- https://www.theworldavatar.com/kg/ontopoi/MunicipalParksandGardens -->


    <owl:Class rdf:about="https://www.theworldavatar.com/kg/ontopoi/MunicipalParksandGardens">
        <rdfs:subClassOf rdf:resource="https://www.theworldavatar.com/kg/ontopoi/Recreational"/>
        <rdfs:comment>Municipal parks and gardens is a subcategory of recreational</rdfs:comment>
        <rdfs:isDefinedBy rdf:resource="https://www.theworldavatar.com/kg/ontopoi"/>
        <rdfs:label>Municipal Parks and Gardens</rdfs:label>
    </owl:Class>
    


    <!-- https://www.theworldavatar.com/kg/ontopoi/Museums -->


    <owl:Class rdf:about="https://www.theworldavatar.com/kg/ontopoi/Museums">
        <rdfs:subClassOf rdf:resource="https://www.theworldavatar.com/kg/ontopoi/Historicalandcultural"/>
        <rdfs:comment>Museums is a subcategory of historical and cultural</rdfs:comment>
        <rdfs:isDefinedBy rdf:resource="https://www.theworldavatar.com/kg/ontopoi"/>
        <rdfs:label>Museums</rdfs:label>
    </owl:Class>
    


    <!-- https://www.theworldavatar.com/kg/ontopoi/Musicalinstruments -->


    <owl:Class rdf:about="https://www.theworldavatar.com/kg/ontopoi/Musicalinstruments">
        <rdfs:subClassOf rdf:resource="https://www.theworldavatar.com/kg/ontopoi/Consumerproducts"/>
        <rdfs:subClassOf rdf:resource="https://www.theworldavatar.com/kg/ontopoi/Householdandofficeandleisureandgarden"/>
        <rdfs:comment>Musical instruments is a subcategory of consumer products</rdfs:comment>
        <rdfs:comment>Musical instruments is a subcategory of household, office, leisure and garden</rdfs:comment>
        <rdfs:isDefinedBy rdf:resource="https://www.theworldavatar.com/kg/ontopoi"/>
        <rdfs:label>Musical instruments</rdfs:label>
    </owl:Class>
    


    <!-- https://www.theworldavatar.com/kg/ontopoi/Musicandvideo -->


    <owl:Class rdf:about="https://www.theworldavatar.com/kg/ontopoi/Musicandvideo">
        <rdfs:subClassOf rdf:resource="https://www.theworldavatar.com/kg/ontopoi/Householdandofficeandleisureandgarden"/>
        <rdfs:comment>Music and video is a subcategory of household, office, leisure and garden</rdfs:comment>
        <rdfs:isDefinedBy rdf:resource="https://www.theworldavatar.com/kg/ontopoi"/>
        <rdfs:label>Music and video</rdfs:label>
    </owl:Class>
    


    <!-- https://www.theworldavatar.com/kg/ontopoi/Musiciansandorchestrasandcomposers -->


    <owl:Class rdf:about="https://www.theworldavatar.com/kg/ontopoi/Musiciansandorchestrasandcomposers">
        <rdfs:subClassOf rdf:resource="https://www.theworldavatar.com/kg/ontopoi/Personalandconsumerandotherservices"/>
        <rdfs:comment>Musicians, orchestras and composers is a subcategory of personal, consumer and other services</rdfs:comment>
        <rdfs:isDefinedBy rdf:resource="https://www.theworldavatar.com/kg/ontopoi"/>
        <rdfs:label>Musicians, orchestras and composers</rdfs:label>
    </owl:Class>
    


    <!-- https://www.theworldavatar.com/kg/ontopoi/Musicteachersandschools -->


    <owl:Class rdf:about="https://www.theworldavatar.com/kg/ontopoi/Musicteachersandschools">
        <rdfs:subClassOf rdf:resource="https://www.theworldavatar.com/kg/ontopoi/Recreationalandvocationaleducation"/>
        <rdfs:comment>Music teachers and schools is a subcategory of recreational and vocational education</rdfs:comment>
        <rdfs:isDefinedBy rdf:resource="https://www.theworldavatar.com/kg/ontopoi"/>
        <rdfs:label>Music teachers and schools</rdfs:label>
    </owl:Class>
    


    <!-- https://www.theworldavatar.com/kg/ontopoi/Newvehicles -->


    <owl:Class rdf:about="https://www.theworldavatar.com/kg/ontopoi/Newvehicles">
        <rdfs:subClassOf rdf:resource="https://www.theworldavatar.com/kg/ontopoi/Motoring"/>
        <rdfs:comment>New vehicles is a subcategory of motoring</rdfs:comment>
        <rdfs:isDefinedBy rdf:resource="https://www.theworldavatar.com/kg/ontopoi"/>
        <rdfs:label>New vehicles</rdfs:label>
    </owl:Class>
    


    <!-- https://www.theworldavatar.com/kg/ontopoi/Nightclubs -->


    <owl:Class rdf:about="https://www.theworldavatar.com/kg/ontopoi/Nightclubs">
        <rdfs:subClassOf rdf:resource="https://www.theworldavatar.com/kg/ontopoi/Venuesandstageandscreen"/>
        <rdfs:comment>Nightclubs is a subcategory of venues, stage and screen</rdfs:comment>
        <rdfs:isDefinedBy rdf:resource="https://www.theworldavatar.com/kg/ontopoi"/>
        <rdfs:label>Nightclubs</rdfs:label>
    </owl:Class>
    


    <!-- https://www.theworldavatar.com/kg/ontopoi/Non-alcoholicdrinks -->


    <owl:Class rdf:about="https://www.theworldavatar.com/kg/ontopoi/Non-alcoholicdrinks">
        <rdfs:subClassOf rdf:resource="https://www.theworldavatar.com/kg/ontopoi/Foodstuffs"/>
        <rdfs:comment>Non-alcoholic drinks is a subcategory of foodstuffs</rdfs:comment>
        <rdfs:isDefinedBy rdf:resource="https://www.theworldavatar.com/kg/ontopoi"/>
        <rdfs:label>Non-alcoholic drinks</rdfs:label>
    </owl:Class>
    


    <!-- https://www.theworldavatar.com/kg/ontopoi/Nurseryschoolsandpre-andafter-schoolcare -->


    <owl:Class rdf:about="https://www.theworldavatar.com/kg/ontopoi/Nurseryschoolsandpre-andafter-schoolcare">
        <rdfs:subClassOf rdf:resource="https://www.theworldavatar.com/kg/ontopoi/Recreationalandvocationaleducation"/>
        <rdfs:comment>Nursery schools and pre- and after-school care is a subcategory of recreational and vocational education</rdfs:comment>
        <rdfs:isDefinedBy rdf:resource="https://www.theworldavatar.com/kg/ontopoi"/>
        <rdfs:label>Nursery schools and pre- and after-school care</rdfs:label>
    </owl:Class>
    


    <!-- https://www.theworldavatar.com/kg/ontopoi/Nursingagencies -->


    <owl:Class rdf:about="https://www.theworldavatar.com/kg/ontopoi/Nursingagencies">
        <rdfs:subClassOf rdf:resource="https://www.theworldavatar.com/kg/ontopoi/Employmentandcareeragencies"/>
        <rdfs:comment>Nursing agencies is a subcategory of employment and career agencies</rdfs:comment>
        <rdfs:isDefinedBy rdf:resource="https://www.theworldavatar.com/kg/ontopoi"/>
        <rdfs:label>Nursing agencies</rdfs:label>
    </owl:Class>
    


    <!-- https://www.theworldavatar.com/kg/ontopoi/Nursingandresidentialcarehomes -->


    <owl:Class rdf:about="https://www.theworldavatar.com/kg/ontopoi/Nursingandresidentialcarehomes">
        <rdfs:subClassOf rdf:resource="https://www.theworldavatar.com/kg/ontopoi/Healthpractitionersandestablishments"/>
        <rdfs:comment>Nursing and residential care homes is a subcategory of health practitioners and establishments</rdfs:comment>
        <rdfs:isDefinedBy rdf:resource="https://www.theworldavatar.com/kg/ontopoi"/>
        <rdfs:label>Nursing and residential care homes</rdfs:label>
    </owl:Class>
    


    <!-- https://www.theworldavatar.com/kg/ontopoi/Oasthouses -->


    <owl:Class rdf:about="https://www.theworldavatar.com/kg/ontopoi/Oasthouses">
        <rdfs:subClassOf rdf:resource="https://www.theworldavatar.com/kg/ontopoi/Industrialfeatures"/>
        <rdfs:comment>Oast houses is a subcategory of industrial features</rdfs:comment>
        <rdfs:isDefinedBy rdf:resource="https://www.theworldavatar.com/kg/ontopoi"/>
        <rdfs:label>Oast houses</rdfs:label>
    </owl:Class>
    


    <!-- https://www.theworldavatar.com/kg/ontopoi/Officeandshopequipment -->


    <owl:Class rdf:about="https://www.theworldavatar.com/kg/ontopoi/Officeandshopequipment">
        <rdfs:subClassOf rdf:resource="https://www.theworldavatar.com/kg/ontopoi/Industrialproducts"/>
        <rdfs:comment>Office and shop equipment is a subcategory of industrial products</rdfs:comment>
        <rdfs:isDefinedBy rdf:resource="https://www.theworldavatar.com/kg/ontopoi"/>
        <rdfs:label>Office and shop equipment</rdfs:label>
    </owl:Class>
    


    <!-- https://www.theworldavatar.com/kg/ontopoi/Officeservices -->


    <owl:Class rdf:about="https://www.theworldavatar.com/kg/ontopoi/Officeservices">
        <rdfs:subClassOf rdf:resource="https://www.theworldavatar.com/kg/ontopoi/Contractservices"/>
        <rdfs:comment>Office services is a subcategory of contract services</rdfs:comment>
        <rdfs:isDefinedBy rdf:resource="https://www.theworldavatar.com/kg/ontopoi"/>
        <rdfs:label>Office services</rdfs:label>
    </owl:Class>
    


    <!-- https://www.theworldavatar.com/kg/ontopoi/Oilandgasextractionandrefineryandproductmanufacture -->


    <owl:Class rdf:about="https://www.theworldavatar.com/kg/ontopoi/Oilandgasextractionandrefineryandproductmanufacture">
        <rdfs:subClassOf rdf:resource="https://www.theworldavatar.com/kg/ontopoi/Extractiveindustries"/>
        <rdfs:comment>Oil and gas extraction, refinery and product manufacture is a subcategory of extractive industries</rdfs:comment>
        <rdfs:isDefinedBy rdf:resource="https://www.theworldavatar.com/kg/ontopoi"/>
        <rdfs:label>Oil and gas extraction, refinery and product manufacture</rdfs:label>
    </owl:Class>
    


    <!-- https://www.theworldavatar.com/kg/ontopoi/Optometristsandopticians -->


    <owl:Class rdf:about="https://www.theworldavatar.com/kg/ontopoi/Optometristsandopticians">
        <rdfs:subClassOf rdf:resource="https://www.theworldavatar.com/kg/ontopoi/Healthpractitionersandestablishments"/>
        <rdfs:comment>Optometrists and opticians is a subcategory of health practitioners and establishments</rdfs:comment>
        <rdfs:isDefinedBy rdf:resource="https://www.theworldavatar.com/kg/ontopoi"/>
        <rdfs:label>Optometrists and opticians</rdfs:label>
    </owl:Class>
    


    <!-- https://www.theworldavatar.com/kg/ontopoi/Oremining -->


    <owl:Class rdf:about="https://www.theworldavatar.com/kg/ontopoi/Oremining">
        <rdfs:subClassOf rdf:resource="https://www.theworldavatar.com/kg/ontopoi/Extractiveindustries"/>
        <rdfs:comment>Ore mining is a subcategory of extractive industries</rdfs:comment>
        <rdfs:isDefinedBy rdf:resource="https://www.theworldavatar.com/kg/ontopoi"/>
        <rdfs:label>Ore mining</rdfs:label>
    </owl:Class>
    


    <!-- https://www.theworldavatar.com/kg/ontopoi/Organicandhealthandgourmetandkosherfoods -->


    <owl:Class rdf:about="https://www.theworldavatar.com/kg/ontopoi/Organicandhealthandgourmetandkosherfoods">
        <rdfs:subClassOf rdf:resource="https://www.theworldavatar.com/kg/ontopoi/Foodanddrinkandmultiitemretail"/>
        <rdfs:comment>Organic, health, gourmet and kosher foods is a subcategory of food, drink and multi item retail</rdfs:comment>
        <rdfs:isDefinedBy rdf:resource="https://www.theworldavatar.com/kg/ontopoi"/>
        <rdfs:label>Organic, health, gourmet and kosher foods</rdfs:label>
    </owl:Class>
    


    <!-- https://www.theworldavatar.com/kg/ontopoi/Organisations -->


    <owl:Class rdf:about="https://www.theworldavatar.com/kg/ontopoi/Organisations">
        <rdfs:subClassOf rdf:resource="https://www.theworldavatar.com/kg/ontopoi/Publicinfrastructure"/>
        <rdfs:comment>Organisations is a subcategory of public infrastructure</rdfs:comment>
        <rdfs:isDefinedBy rdf:resource="https://www.theworldavatar.com/kg/ontopoi"/>
        <rdfs:label>Organisations</rdfs:label>
    </owl:Class>
    


    <!-- https://www.theworldavatar.com/kg/ontopoi/Outdoorpursuitorganisersandequipment -->


    <owl:Class rdf:about="https://www.theworldavatar.com/kg/ontopoi/Outdoorpursuitorganisersandequipment">
        <rdfs:subClassOf rdf:resource="https://www.theworldavatar.com/kg/ontopoi/Outdoorpursuits"/>
        <rdfs:comment>Outdoor pursuit organisers and equipment is a subcategory of outdoor pursuits</rdfs:comment>
        <rdfs:isDefinedBy rdf:resource="https://www.theworldavatar.com/kg/ontopoi"/>
        <rdfs:label>Outdoor pursuit organisers and equipment</rdfs:label>
    </owl:Class>
    


    <!-- https://www.theworldavatar.com/kg/ontopoi/Outdoorpursuits -->


    <owl:Class rdf:about="https://www.theworldavatar.com/kg/ontopoi/Outdoorpursuits">
        <rdfs:subClassOf rdf:resource="https://www.theworldavatar.com/kg/ontopoi/Sportandentertainment"/>
        <rdfs:comment>Outdoor pursuits is a subcategory of sport and entertainment</rdfs:comment>
        <rdfs:isDefinedBy rdf:resource="https://www.theworldavatar.com/kg/ontopoi"/>
        <rdfs:label>Outdoor pursuits</rdfs:label>
    </owl:Class>
    


    <!-- https://www.theworldavatar.com/kg/ontopoi/Ovensandfurnaces -->


    <owl:Class rdf:about="https://www.theworldavatar.com/kg/ontopoi/Ovensandfurnaces">
        <rdfs:subClassOf rdf:resource="https://www.theworldavatar.com/kg/ontopoi/Industrialproducts"/>
        <rdfs:comment>Ovens and furnaces is a subcategory of industrial products</rdfs:comment>
        <rdfs:isDefinedBy rdf:resource="https://www.theworldavatar.com/kg/ontopoi"/>
        <rdfs:label>Ovens and furnaces</rdfs:label>
    </owl:Class>
    


    <!-- https://www.theworldavatar.com/kg/ontopoi/Packaging -->


    <owl:Class rdf:about="https://www.theworldavatar.com/kg/ontopoi/Packaging">
        <rdfs:subClassOf rdf:resource="https://www.theworldavatar.com/kg/ontopoi/Industrialproducts"/>
        <rdfs:comment>Packaging is a subcategory of industrial products</rdfs:comment>
        <rdfs:isDefinedBy rdf:resource="https://www.theworldavatar.com/kg/ontopoi"/>
        <rdfs:label>Packaging</rdfs:label>
    </owl:Class>
    


    <!-- https://www.theworldavatar.com/kg/ontopoi/Packers -->


    <owl:Class rdf:about="https://www.theworldavatar.com/kg/ontopoi/Packers">
        <rdfs:subClassOf rdf:resource="https://www.theworldavatar.com/kg/ontopoi/Contractservices"/>
        <rdfs:comment>Packers is a subcategory of contract services</rdfs:comment>
        <rdfs:isDefinedBy rdf:resource="https://www.theworldavatar.com/kg/ontopoi"/>
        <rdfs:label>Packers</rdfs:label>
    </owl:Class>
    


    <!-- https://www.theworldavatar.com/kg/ontopoi/Paintinganddecoratingservices -->


    <owl:Class rdf:about="https://www.theworldavatar.com/kg/ontopoi/Paintinganddecoratingservices">
        <rdfs:subClassOf rdf:resource="https://www.theworldavatar.com/kg/ontopoi/Constructionservices"/>
        <rdfs:comment>Painting and decorating services is a subcategory of construction services</rdfs:comment>
        <rdfs:isDefinedBy rdf:resource="https://www.theworldavatar.com/kg/ontopoi"/>
        <rdfs:label>Painting and decorating services</rdfs:label>
    </owl:Class>
    


    <!-- https://www.theworldavatar.com/kg/ontopoi/Paintsandvarnishesandlacquers -->


    <owl:Class rdf:about="https://www.theworldavatar.com/kg/ontopoi/Paintsandvarnishesandlacquers">
        <rdfs:subClassOf rdf:resource="https://www.theworldavatar.com/kg/ontopoi/Industrialproducts"/>
        <rdfs:comment>Paints, varnishes and lacquers is a subcategory of industrial products</rdfs:comment>
        <rdfs:isDefinedBy rdf:resource="https://www.theworldavatar.com/kg/ontopoi"/>
        <rdfs:label>Paints, varnishes and lacquers</rdfs:label>
    </owl:Class>
    


    <!-- https://www.theworldavatar.com/kg/ontopoi/Parachutingandbungeejumping -->


    <owl:Class rdf:about="https://www.theworldavatar.com/kg/ontopoi/Parachutingandbungeejumping">
        <rdfs:subClassOf rdf:resource="https://www.theworldavatar.com/kg/ontopoi/Outdoorpursuits"/>
        <rdfs:comment>Parachuting and bungee jumping is a subcategory of outdoor pursuits</rdfs:comment>
        <rdfs:isDefinedBy rdf:resource="https://www.theworldavatar.com/kg/ontopoi"/>
        <rdfs:label>Parachuting and bungee jumping</rdfs:label>
    </owl:Class>
    


    <!-- https://www.theworldavatar.com/kg/ontopoi/Paraglidingandhang-gliding -->


    <owl:Class rdf:about="https://www.theworldavatar.com/kg/ontopoi/Paraglidingandhang-gliding">
        <rdfs:subClassOf rdf:resource="https://www.theworldavatar.com/kg/ontopoi/Outdoorpursuits"/>
        <rdfs:comment>Paragliding and hang-gliding is a subcategory of outdoor pursuits</rdfs:comment>
        <rdfs:isDefinedBy rdf:resource="https://www.theworldavatar.com/kg/ontopoi"/>
        <rdfs:label>Paragliding and hang-gliding</rdfs:label>
    </owl:Class>
    


    <!-- https://www.theworldavatar.com/kg/ontopoi/Parentingandchildcareservices -->


    <owl:Class rdf:about="https://www.theworldavatar.com/kg/ontopoi/Parentingandchildcareservices">
        <rdfs:subClassOf rdf:resource="https://www.theworldavatar.com/kg/ontopoi/Healthpractitionersandestablishments"/>
        <rdfs:comment>Parenting and childcare services is a subcategory of health practitioners and establishments</rdfs:comment>
        <rdfs:isDefinedBy rdf:resource="https://www.theworldavatar.com/kg/ontopoi"/>
        <rdfs:label>Parenting and childcare services</rdfs:label>
    </owl:Class>
    


    <!-- https://www.theworldavatar.com/kg/ontopoi/Parking -->


    <owl:Class rdf:about="https://www.theworldavatar.com/kg/ontopoi/Parking">
        <rdfs:subClassOf rdf:resource="https://www.theworldavatar.com/kg/ontopoi/Roadandrail"/>
        <rdfs:comment>Parking is a subcategory of road and rail</rdfs:comment>
        <rdfs:isDefinedBy rdf:resource="https://www.theworldavatar.com/kg/ontopoi"/>
        <rdfs:label>Parking</rdfs:label>
    </owl:Class>
    


    <!-- https://www.theworldavatar.com/kg/ontopoi/Partygoodsandnovelties -->


    <owl:Class rdf:about="https://www.theworldavatar.com/kg/ontopoi/Partygoodsandnovelties">
        <rdfs:subClassOf rdf:resource="https://www.theworldavatar.com/kg/ontopoi/Householdandofficeandleisureandgarden"/>
        <rdfs:comment>Party goods and novelties is a subcategory of household, office, leisure and garden</rdfs:comment>
        <rdfs:isDefinedBy rdf:resource="https://www.theworldavatar.com/kg/ontopoi"/>
        <rdfs:label>Party goods and novelties</rdfs:label>
    </owl:Class>
    


    <!-- https://www.theworldavatar.com/kg/ontopoi/Partyorganisers -->


    <owl:Class rdf:about="https://www.theworldavatar.com/kg/ontopoi/Partyorganisers">
        <rdfs:subClassOf rdf:resource="https://www.theworldavatar.com/kg/ontopoi/Personalandconsumerandotherservices"/>
        <rdfs:comment>Party organisers is a subcategory of personal, consumer and other services</rdfs:comment>
        <rdfs:isDefinedBy rdf:resource="https://www.theworldavatar.com/kg/ontopoi"/>
        <rdfs:label>Party organisers</rdfs:label>
    </owl:Class>
    


    <!-- https://www.theworldavatar.com/kg/ontopoi/Pawnbrokers -->


    <owl:Class rdf:about="https://www.theworldavatar.com/kg/ontopoi/Pawnbrokers">
        <rdfs:subClassOf rdf:resource="https://www.theworldavatar.com/kg/ontopoi/Legalandfinancial"/>
        <rdfs:comment>Pawnbrokers is a subcategory of legal and financial</rdfs:comment>
        <rdfs:isDefinedBy rdf:resource="https://www.theworldavatar.com/kg/ontopoi"/>
        <rdfs:label>Pawnbrokers</rdfs:label>
    </owl:Class>
    


    <!-- https://www.theworldavatar.com/kg/ontopoi/Pensionandfundmanagement -->


    <owl:Class rdf:about="https://www.theworldavatar.com/kg/ontopoi/Pensionandfundmanagement">
        <rdfs:subClassOf rdf:resource="https://www.theworldavatar.com/kg/ontopoi/Legalandfinancial"/>
        <rdfs:comment>Pension and fund management is a subcategory of legal and financial</rdfs:comment>
        <rdfs:isDefinedBy rdf:resource="https://www.theworldavatar.com/kg/ontopoi"/>
        <rdfs:label>Pension and fund management</rdfs:label>
    </owl:Class>
    


    <!-- https://www.theworldavatar.com/kg/ontopoi/Personalandconsumerandotherservices -->


    <owl:Class rdf:about="https://www.theworldavatar.com/kg/ontopoi/Personalandconsumerandotherservices">
        <rdfs:subClassOf rdf:resource="https://www.theworldavatar.com/kg/ontopoi/Commercialservices"/>
        <rdfs:comment>Personal, consumer and other services is a subcategory of commercial services</rdfs:comment>
        <rdfs:isDefinedBy rdf:resource="https://www.theworldavatar.com/kg/ontopoi"/>
        <rdfs:label>Personal, consumer and other services</rdfs:label>
    </owl:Class>
    


    <!-- https://www.theworldavatar.com/kg/ontopoi/Personalisation -->


    <owl:Class rdf:about="https://www.theworldavatar.com/kg/ontopoi/Personalisation">
        <rdfs:subClassOf rdf:resource="https://www.theworldavatar.com/kg/ontopoi/Personalandconsumerandotherservices"/>
        <rdfs:comment>Personalisation is a subcategory of personal, consumer and other services</rdfs:comment>
        <rdfs:isDefinedBy rdf:resource="https://www.theworldavatar.com/kg/ontopoi"/>
        <rdfs:label>Personalisation</rdfs:label>
    </owl:Class>
    


    <!-- https://www.theworldavatar.com/kg/ontopoi/Pestandvermincontrol -->


    <owl:Class rdf:about="https://www.theworldavatar.com/kg/ontopoi/Pestandvermincontrol">
        <rdfs:subClassOf rdf:resource="https://www.theworldavatar.com/kg/ontopoi/Contractservices"/>
        <rdfs:comment>Pest and vermin control is a subcategory of contract services</rdfs:comment>
        <rdfs:isDefinedBy rdf:resource="https://www.theworldavatar.com/kg/ontopoi"/>
        <rdfs:label>Pest and vermin control</rdfs:label>
    </owl:Class>
    


    <!-- https://www.theworldavatar.com/kg/ontopoi/Pesticides -->


    <owl:Class rdf:about="https://www.theworldavatar.com/kg/ontopoi/Pesticides">
        <rdfs:subClassOf rdf:resource="https://www.theworldavatar.com/kg/ontopoi/Industrialproducts"/>
        <rdfs:comment>Pesticides is a subcategory of industrial products</rdfs:comment>
        <rdfs:isDefinedBy rdf:resource="https://www.theworldavatar.com/kg/ontopoi"/>
        <rdfs:label>Pesticides</rdfs:label>
    </owl:Class>
    


    <!-- https://www.theworldavatar.com/kg/ontopoi/Petcemeteriesandcrematoria -->


    <owl:Class rdf:about="https://www.theworldavatar.com/kg/ontopoi/Petcemeteriesandcrematoria">
        <rdfs:subClassOf rdf:resource="https://www.theworldavatar.com/kg/ontopoi/Animalwelfare"/>
        <rdfs:comment>Pet cemeteries and crematoria is a subcategory of animal welfare</rdfs:comment>
        <rdfs:isDefinedBy rdf:resource="https://www.theworldavatar.com/kg/ontopoi"/>
        <rdfs:label>Pet cemeteries and crematoria</rdfs:label>
    </owl:Class>
    


    <!-- https://www.theworldavatar.com/kg/ontopoi/Petrolandfuelstations -->


    <owl:Class rdf:about="https://www.theworldavatar.com/kg/ontopoi/Petrolandfuelstations">
        <rdfs:subClassOf rdf:resource="https://www.theworldavatar.com/kg/ontopoi/Roadandrail"/>
        <rdfs:comment>Petrol and fuel stations is a subcategory of road and rail</rdfs:comment>
        <rdfs:isDefinedBy rdf:resource="https://www.theworldavatar.com/kg/ontopoi"/>
        <rdfs:label>Petrol and fuel stations</rdfs:label>
    </owl:Class>
    


    <!-- https://www.theworldavatar.com/kg/ontopoi/Petsandsuppliesandservices -->


    <owl:Class rdf:about="https://www.theworldavatar.com/kg/ontopoi/Petsandsuppliesandservices">
        <rdfs:subClassOf rdf:resource="https://www.theworldavatar.com/kg/ontopoi/Householdandofficeandleisureandgarden"/>
        <rdfs:comment>Pets, supplies and services is a subcategory of household, office, leisure and garden</rdfs:comment>
        <rdfs:isDefinedBy rdf:resource="https://www.theworldavatar.com/kg/ontopoi"/>
        <rdfs:label>Pets, supplies and services</rdfs:label>
    </owl:Class>
    


    <!-- https://www.theworldavatar.com/kg/ontopoi/Photographicandopticalequipment -->


    <owl:Class rdf:about="https://www.theworldavatar.com/kg/ontopoi/Photographicandopticalequipment">
        <rdfs:subClassOf rdf:resource="https://www.theworldavatar.com/kg/ontopoi/Consumerproducts"/>
        <rdfs:subClassOf rdf:resource="https://www.theworldavatar.com/kg/ontopoi/Householdandofficeandleisureandgarden"/>
        <rdfs:comment>Photographic and optical equipment is a subcategory of consumer products</rdfs:comment>
        <rdfs:comment>Photographic and optical equipment is a subcategory of household, office, leisure and garden</rdfs:comment>
        <rdfs:isDefinedBy rdf:resource="https://www.theworldavatar.com/kg/ontopoi"/>
        <rdfs:label>Photographic and optical equipment</rdfs:label>
    </owl:Class>
    


    <!-- https://www.theworldavatar.com/kg/ontopoi/Photographicservices -->


    <owl:Class rdf:about="https://www.theworldavatar.com/kg/ontopoi/Photographicservices">
        <rdfs:subClassOf rdf:resource="https://www.theworldavatar.com/kg/ontopoi/Personalandconsumerandotherservices"/>
        <rdfs:comment>Photographic services is a subcategory of personal, consumer and other services</rdfs:comment>
        <rdfs:isDefinedBy rdf:resource="https://www.theworldavatar.com/kg/ontopoi"/>
        <rdfs:label>Photographic services</rdfs:label>
    </owl:Class>
    


    <!-- https://www.theworldavatar.com/kg/ontopoi/Physicaltherapy -->


    <owl:Class rdf:about="https://www.theworldavatar.com/kg/ontopoi/Physicaltherapy">
        <rdfs:subClassOf rdf:resource="https://www.theworldavatar.com/kg/ontopoi/Healthpractitionersandestablishments"/>
        <rdfs:comment>Physical therapy is a subcategory of health practitioners and establishments</rdfs:comment>
        <rdfs:isDefinedBy rdf:resource="https://www.theworldavatar.com/kg/ontopoi"/>
        <rdfs:label>Physical therapy</rdfs:label>
    </owl:Class>
    


    <!-- https://www.theworldavatar.com/kg/ontopoi/Picnicareas -->


    <owl:Class rdf:about="https://www.theworldavatar.com/kg/ontopoi/Picnicareas">
        <rdfs:subClassOf rdf:resource="https://www.theworldavatar.com/kg/ontopoi/Recreational"/>
        <rdfs:comment>Picnic areas is a subcategory of recreational</rdfs:comment>
        <rdfs:isDefinedBy rdf:resource="https://www.theworldavatar.com/kg/ontopoi"/>
        <rdfs:label>Picnic areas</rdfs:label>
    </owl:Class>
    


    <!-- https://www.theworldavatar.com/kg/ontopoi/Pipelines -->


    <owl:Class rdf:about="https://www.theworldavatar.com/kg/ontopoi/Pipelines">
        <rdfs:subClassOf rdf:resource="https://www.theworldavatar.com/kg/ontopoi/Industrialfeatures"/>
        <rdfs:comment>Pipelines is a subcategory of industrial features</rdfs:comment>
        <rdfs:isDefinedBy rdf:resource="https://www.theworldavatar.com/kg/ontopoi"/>
        <rdfs:label>Pipelines</rdfs:label>
    </owl:Class>
    


    <!-- https://www.theworldavatar.com/kg/ontopoi/Placesofworship -->


    <owl:Class rdf:about="https://www.theworldavatar.com/kg/ontopoi/Placesofworship">
        <rdfs:subClassOf rdf:resource="https://www.theworldavatar.com/kg/ontopoi/Infrastructureandfacilities"/>
        <rdfs:comment>Places of worship is a subcategory of infrastructure and facilities</rdfs:comment>
        <rdfs:isDefinedBy rdf:resource="https://www.theworldavatar.com/kg/ontopoi"/>
        <rdfs:label>Places of worship</rdfs:label>
    </owl:Class>
    


    <!-- https://www.theworldavatar.com/kg/ontopoi/Plasterers -->


    <owl:Class rdf:about="https://www.theworldavatar.com/kg/ontopoi/Plasterers">
        <rdfs:subClassOf rdf:resource="https://www.theworldavatar.com/kg/ontopoi/Constructionservices"/>
        <rdfs:comment>Plasterers is a subcategory of construction services</rdfs:comment>
        <rdfs:isDefinedBy rdf:resource="https://www.theworldavatar.com/kg/ontopoi"/>
        <rdfs:label>Plasterers</rdfs:label>
    </owl:Class>
    


    <!-- https://www.theworldavatar.com/kg/ontopoi/Platemakersandprintfinishersandtypesetters -->


    <owl:Class rdf:about="https://www.theworldavatar.com/kg/ontopoi/Platemakersandprintfinishersandtypesetters">
        <rdfs:subClassOf rdf:resource="https://www.theworldavatar.com/kg/ontopoi/ITandadvertisingandmarketingandmediaservices"/>
        <rdfs:comment>Plate makers, print finishers and typesetters is a subcategory of it, advertising, marketing and media service s</rdfs:comment>
        <rdfs:isDefinedBy rdf:resource="https://www.theworldavatar.com/kg/ontopoi"/>
        <rdfs:label>Plate makers, print finishers and typesetters</rdfs:label>
    </owl:Class>
    


    <!-- https://www.theworldavatar.com/kg/ontopoi/Playgrounds -->


    <owl:Class rdf:about="https://www.theworldavatar.com/kg/ontopoi/Playgrounds">
        <rdfs:subClassOf rdf:resource="https://www.theworldavatar.com/kg/ontopoi/Recreational"/>
        <rdfs:comment>Playgrounds is a subcategory of recreational</rdfs:comment>
        <rdfs:isDefinedBy rdf:resource="https://www.theworldavatar.com/kg/ontopoi"/>
        <rdfs:label>Playgrounds</rdfs:label>
    </owl:Class>
    


    <!-- https://www.theworldavatar.com/kg/ontopoi/Plumbingandheatingservices -->


    <owl:Class rdf:about="https://www.theworldavatar.com/kg/ontopoi/Plumbingandheatingservices">
        <rdfs:subClassOf rdf:resource="https://www.theworldavatar.com/kg/ontopoi/Constructionservices"/>
        <rdfs:comment>Plumbing and heating services is a subcategory of construction services</rdfs:comment>
        <rdfs:isDefinedBy rdf:resource="https://www.theworldavatar.com/kg/ontopoi"/>
        <rdfs:label>Plumbing and heating services</rdfs:label>
    </owl:Class>
    


    <!-- https://www.theworldavatar.com/kg/ontopoi/Pneumaticengineers -->


    <owl:Class rdf:about="https://www.theworldavatar.com/kg/ontopoi/Pneumaticengineers">
        <rdfs:subClassOf rdf:resource="https://www.theworldavatar.com/kg/ontopoi/Engineeringservices"/>
        <rdfs:comment>Pneumatic engineers is a subcategory of engineering services</rdfs:comment>
        <rdfs:isDefinedBy rdf:resource="https://www.theworldavatar.com/kg/ontopoi"/>
        <rdfs:label>Pneumatic engineers</rdfs:label>
    </owl:Class>
    


    <!-- https://www.theworldavatar.com/kg/ontopoi/Policestations -->


    <owl:Class rdf:about="https://www.theworldavatar.com/kg/ontopoi/Policestations">
        <rdfs:subClassOf rdf:resource="https://www.theworldavatar.com/kg/ontopoi/Centralandlocalgovernment"/>
        <rdfs:comment>Police stations is a subcategory of central and local government</rdfs:comment>
        <rdfs:isDefinedBy rdf:resource="https://www.theworldavatar.com/kg/ontopoi"/>
        <rdfs:label>Police stations</rdfs:label>
    </owl:Class>
    


    <!-- https://www.theworldavatar.com/kg/ontopoi/Politicalpartiesandrelatedorganisations -->


    <owl:Class rdf:about="https://www.theworldavatar.com/kg/ontopoi/Politicalpartiesandrelatedorganisations">
        <rdfs:subClassOf rdf:resource="https://www.theworldavatar.com/kg/ontopoi/Organisations"/>
        <rdfs:comment>Political parties and related organisations is a subcategory of organisations</rdfs:comment>
        <rdfs:isDefinedBy rdf:resource="https://www.theworldavatar.com/kg/ontopoi"/>
        <rdfs:label>Political parties and related organisations</rdfs:label>
    </owl:Class>
    


    <!-- https://www.theworldavatar.com/kg/ontopoi/Poolandcourtconstruction -->


    <owl:Class rdf:about="https://www.theworldavatar.com/kg/ontopoi/Poolandcourtconstruction">
        <rdfs:subClassOf rdf:resource="https://www.theworldavatar.com/kg/ontopoi/Constructionservices"/>
        <rdfs:comment>Pool and court construction is a subcategory of construction services</rdfs:comment>
        <rdfs:isDefinedBy rdf:resource="https://www.theworldavatar.com/kg/ontopoi"/>
        <rdfs:label>Pool and court construction</rdfs:label>
    </owl:Class>
    


    <!-- https://www.theworldavatar.com/kg/ontopoi/Postoffices -->


    <owl:Class rdf:about="https://www.theworldavatar.com/kg/ontopoi/Postoffices">
        <rdfs:subClassOf rdf:resource="https://www.theworldavatar.com/kg/ontopoi/Householdandofficeandleisureandgarden"/>
        <rdfs:comment>Post offices is a subcategory of household, office, leisure and garden</rdfs:comment>
        <rdfs:isDefinedBy rdf:resource="https://www.theworldavatar.com/kg/ontopoi"/>
        <rdfs:label>Post offices</rdfs:label>
    </owl:Class>
    


    <!-- https://www.theworldavatar.com/kg/ontopoi/Potteries -->


    <owl:Class rdf:about="https://www.theworldavatar.com/kg/ontopoi/Potteries">
        <rdfs:subClassOf rdf:resource="https://www.theworldavatar.com/kg/ontopoi/Householdandofficeandleisureandgarden"/>
        <rdfs:comment>Potteries is a subcategory of household, office, leisure and garden</rdfs:comment>
        <rdfs:isDefinedBy rdf:resource="https://www.theworldavatar.com/kg/ontopoi"/>
        <rdfs:label>Potteries</rdfs:label>
    </owl:Class>
    


    <!-- https://www.theworldavatar.com/kg/ontopoi/Poultryfarmingandequipmentandsupplies -->


    <owl:Class rdf:about="https://www.theworldavatar.com/kg/ontopoi/Poultryfarmingandequipmentandsupplies">
        <rdfs:subClassOf rdf:resource="https://www.theworldavatar.com/kg/ontopoi/Farming"/>
        <rdfs:comment>Poultry farming, equipment and supplies is a subcategory of farming</rdfs:comment>
        <rdfs:isDefinedBy rdf:resource="https://www.theworldavatar.com/kg/ontopoi"/>
        <rdfs:label>Poultry farming, equipment and supplies</rdfs:label>
    </owl:Class>
    


    <!-- https://www.theworldavatar.com/kg/ontopoi/Precisionengineers -->


    <owl:Class rdf:about="https://www.theworldavatar.com/kg/ontopoi/Precisionengineers">
        <rdfs:subClassOf rdf:resource="https://www.theworldavatar.com/kg/ontopoi/Engineeringservices"/>
        <rdfs:comment>Precision engineers is a subcategory of engineering services</rdfs:comment>
        <rdfs:isDefinedBy rdf:resource="https://www.theworldavatar.com/kg/ontopoi"/>
        <rdfs:label>Precision engineers</rdfs:label>
    </owl:Class>
    


    <!-- https://www.theworldavatar.com/kg/ontopoi/Pregnancyrelatedservicesandhelpcentres -->


    <owl:Class rdf:about="https://www.theworldavatar.com/kg/ontopoi/Pregnancyrelatedservicesandhelpcentres">
        <rdfs:subClassOf rdf:resource="https://www.theworldavatar.com/kg/ontopoi/Healthsupportservices"/>
        <rdfs:comment>Pregnancy related services and help centres is a subcategory of health support services</rdfs:comment>
        <rdfs:isDefinedBy rdf:resource="https://www.theworldavatar.com/kg/ontopoi"/>
        <rdfs:label>Pregnancy related services and help centres</rdfs:label>
    </owl:Class>
    


    <!-- https://www.theworldavatar.com/kg/ontopoi/Pressandjournalismservices -->


    <owl:Class rdf:about="https://www.theworldavatar.com/kg/ontopoi/Pressandjournalismservices">
        <rdfs:subClassOf rdf:resource="https://www.theworldavatar.com/kg/ontopoi/ITandadvertisingandmarketingandmediaservices"/>
        <rdfs:comment>Press and journalism services is a subcategory of it, advertising, marketing and media service s</rdfs:comment>
        <rdfs:isDefinedBy rdf:resource="https://www.theworldavatar.com/kg/ontopoi"/>
        <rdfs:label>Press and journalism services</rdfs:label>
    </owl:Class>
    


    <!-- https://www.theworldavatar.com/kg/ontopoi/Primaryandsecondaryandtertiaryeducation -->


    <owl:Class rdf:about="https://www.theworldavatar.com/kg/ontopoi/Primaryandsecondaryandtertiaryeducation">
        <rdfs:subClassOf rdf:resource="https://www.theworldavatar.com/kg/ontopoi/Educationandhealth"/>
        <rdfs:comment>Primary, secondary and tertiary education is a subcategory of education and health</rdfs:comment>
        <rdfs:isDefinedBy rdf:resource="https://www.theworldavatar.com/kg/ontopoi"/>
        <rdfs:label>Primary, secondary and tertiary education</rdfs:label>
    </owl:Class>
    


    <!-- https://www.theworldavatar.com/kg/ontopoi/Printing-relatedmachinery -->


    <owl:Class rdf:about="https://www.theworldavatar.com/kg/ontopoi/Printing-relatedmachinery">
        <rdfs:subClassOf rdf:resource="https://www.theworldavatar.com/kg/ontopoi/Industrialproducts"/>
        <rdfs:comment>Printing-related machinery is a subcategory of industrial products</rdfs:comment>
        <rdfs:isDefinedBy rdf:resource="https://www.theworldavatar.com/kg/ontopoi"/>
        <rdfs:label>Printing-related machinery</rdfs:label>
    </owl:Class>
    


    <!-- https://www.theworldavatar.com/kg/ontopoi/Printingandphotocopyingservices -->


    <owl:Class rdf:about="https://www.theworldavatar.com/kg/ontopoi/Printingandphotocopyingservices">
        <rdfs:subClassOf rdf:resource="https://www.theworldavatar.com/kg/ontopoi/ITandadvertisingandmarketingandmediaservices"/>
        <rdfs:comment>Printing and photocopying services is a subcategory of it, advertising, marketing and media service s</rdfs:comment>
        <rdfs:isDefinedBy rdf:resource="https://www.theworldavatar.com/kg/ontopoi"/>
        <rdfs:label>Printing and photocopying services</rdfs:label>
    </owl:Class>
    


    <!-- https://www.theworldavatar.com/kg/ontopoi/Printingongarments -->


    <owl:Class rdf:about="https://www.theworldavatar.com/kg/ontopoi/Printingongarments">
        <rdfs:subClassOf rdf:resource="https://www.theworldavatar.com/kg/ontopoi/Personalandconsumerandotherservices"/>
        <rdfs:comment>Printing on garments is a subcategory of personal, consumer and other services</rdfs:comment>
        <rdfs:isDefinedBy rdf:resource="https://www.theworldavatar.com/kg/ontopoi"/>
        <rdfs:label>Printing on garments</rdfs:label>
    </owl:Class>
    


    <!-- https://www.theworldavatar.com/kg/ontopoi/Prisons -->


    <owl:Class rdf:about="https://www.theworldavatar.com/kg/ontopoi/Prisons">
        <rdfs:subClassOf rdf:resource="https://www.theworldavatar.com/kg/ontopoi/Centralandlocalgovernment"/>
        <rdfs:comment>Prisons is a subcategory of central and local government</rdfs:comment>
        <rdfs:isDefinedBy rdf:resource="https://www.theworldavatar.com/kg/ontopoi"/>
        <rdfs:label>Prisons</rdfs:label>
    </owl:Class>
    


    <!-- https://www.theworldavatar.com/kg/ontopoi/Probationofficesandpolicesupportservices -->


    <owl:Class rdf:about="https://www.theworldavatar.com/kg/ontopoi/Probationofficesandpolicesupportservices">
        <rdfs:subClassOf rdf:resource="https://www.theworldavatar.com/kg/ontopoi/Centralandlocalgovernment"/>
        <rdfs:comment>Probation offices and police support services is a subcategory of central and local government</rdfs:comment>
        <rdfs:isDefinedBy rdf:resource="https://www.theworldavatar.com/kg/ontopoi"/>
        <rdfs:label>Probation offices and police support services</rdfs:label>
    </owl:Class>
    


    <!-- https://www.theworldavatar.com/kg/ontopoi/Propertyanddevelopmentservices -->


    <owl:Class rdf:about="https://www.theworldavatar.com/kg/ontopoi/Propertyanddevelopmentservices">
        <rdfs:subClassOf rdf:resource="https://www.theworldavatar.com/kg/ontopoi/Commercialservices"/>
        <rdfs:comment>Property and development services is a subcategory of commercial services</rdfs:comment>
        <rdfs:isDefinedBy rdf:resource="https://www.theworldavatar.com/kg/ontopoi"/>
        <rdfs:label>Property and development services</rdfs:label>
    </owl:Class>
    


    <!-- https://www.theworldavatar.com/kg/ontopoi/Propertydevelopmentservices -->


    <owl:Class rdf:about="https://www.theworldavatar.com/kg/ontopoi/Propertydevelopmentservices">
        <rdfs:subClassOf rdf:resource="https://www.theworldavatar.com/kg/ontopoi/Propertyanddevelopmentservices"/>
        <rdfs:comment>Property development services is a subcategory of property and development services</rdfs:comment>
        <rdfs:isDefinedBy rdf:resource="https://www.theworldavatar.com/kg/ontopoi"/>
        <rdfs:label>Property development services</rdfs:label>
    </owl:Class>
    


    <!-- https://www.theworldavatar.com/kg/ontopoi/Propertyinformationservices -->


    <owl:Class rdf:about="https://www.theworldavatar.com/kg/ontopoi/Propertyinformationservices">
        <rdfs:subClassOf rdf:resource="https://www.theworldavatar.com/kg/ontopoi/Propertyanddevelopmentservices"/>
        <rdfs:comment>Property information services is a subcategory of property and development services</rdfs:comment>
        <rdfs:isDefinedBy rdf:resource="https://www.theworldavatar.com/kg/ontopoi"/>
        <rdfs:label>Property information services</rdfs:label>
    </owl:Class>
    


    <!-- https://www.theworldavatar.com/kg/ontopoi/Propertyletting -->


    <owl:Class rdf:about="https://www.theworldavatar.com/kg/ontopoi/Propertyletting">
        <rdfs:subClassOf rdf:resource="https://www.theworldavatar.com/kg/ontopoi/Propertyanddevelopmentservices"/>
        <rdfs:comment>Property letting is a subcategory of property and development services</rdfs:comment>
        <rdfs:isDefinedBy rdf:resource="https://www.theworldavatar.com/kg/ontopoi"/>
        <rdfs:label>Property letting</rdfs:label>
    </owl:Class>
    


    <!-- https://www.theworldavatar.com/kg/ontopoi/Propertysales -->


    <owl:Class rdf:about="https://www.theworldavatar.com/kg/ontopoi/Propertysales">
        <rdfs:subClassOf rdf:resource="https://www.theworldavatar.com/kg/ontopoi/Propertyanddevelopmentservices"/>
        <rdfs:comment>Property sales is a subcategory of property and development services</rdfs:comment>
        <rdfs:isDefinedBy rdf:resource="https://www.theworldavatar.com/kg/ontopoi"/>
        <rdfs:label>Property sales</rdfs:label>
    </owl:Class>
    


    <!-- https://www.theworldavatar.com/kg/ontopoi/Publicinfrastructure -->


    <owl:Class rdf:about="https://www.theworldavatar.com/kg/ontopoi/Publicinfrastructure"/>
    


    <!-- https://www.theworldavatar.com/kg/ontopoi/Publictoilets -->


    <owl:Class rdf:about="https://www.theworldavatar.com/kg/ontopoi/Publictoilets">
        <rdfs:subClassOf rdf:resource="https://www.theworldavatar.com/kg/ontopoi/Infrastructureandfacilities"/>
        <rdfs:comment>Public toilets is a subcategory of infrastructure and facilities</rdfs:comment>
        <rdfs:isDefinedBy rdf:resource="https://www.theworldavatar.com/kg/ontopoi"/>
        <rdfs:label>Public toilets</rdfs:label>
    </owl:Class>
    


    <!-- https://www.theworldavatar.com/kg/ontopoi/Publictransportandstationsandinfrastructure -->


    <owl:Class rdf:about="https://www.theworldavatar.com/kg/ontopoi/Publictransportandstationsandinfrastructure">
        <rdfs:subClassOf rdf:resource="https://www.theworldavatar.com/kg/ontopoi/Transport"/>
        <rdfs:comment>Public transport, stations and infrastructure is a subcategory of transport</rdfs:comment>
        <rdfs:isDefinedBy rdf:resource="https://www.theworldavatar.com/kg/ontopoi"/>
        <rdfs:label>Public transport, stations and infrastructure</rdfs:label>
    </owl:Class>
    


    <!-- https://www.theworldavatar.com/kg/ontopoi/Publishedgoods -->


    <owl:Class rdf:about="https://www.theworldavatar.com/kg/ontopoi/Publishedgoods">
        <rdfs:subClassOf rdf:resource="https://www.theworldavatar.com/kg/ontopoi/Industrialproducts"/>
        <rdfs:comment>Published goods is a subcategory of industrial products</rdfs:comment>
        <rdfs:isDefinedBy rdf:resource="https://www.theworldavatar.com/kg/ontopoi"/>
        <rdfs:label>Published goods</rdfs:label>
    </owl:Class>
    


    <!-- https://www.theworldavatar.com/kg/ontopoi/Pubsandbarsandinns -->


    <owl:Class rdf:about="https://www.theworldavatar.com/kg/ontopoi/Pubsandbarsandinns">
        <rdfs:subClassOf rdf:resource="https://www.theworldavatar.com/kg/ontopoi/Eatinganddrinking"/>
        <rdfs:comment>Pubs, bars and inns is a subcategory of eating and drinking</rdfs:comment>
        <rdfs:isDefinedBy rdf:resource="https://www.theworldavatar.com/kg/ontopoi"/>
        <rdfs:label>Pubs, bars and inns</rdfs:label>
    </owl:Class>
    


    <!-- https://www.theworldavatar.com/kg/ontopoi/Pumpsandcompressors -->


    <owl:Class rdf:about="https://www.theworldavatar.com/kg/ontopoi/Pumpsandcompressors">
        <rdfs:subClassOf rdf:resource="https://www.theworldavatar.com/kg/ontopoi/Industrialproducts"/>
        <rdfs:comment>Pumps and compressors is a subcategory of industrial products</rdfs:comment>
        <rdfs:isDefinedBy rdf:resource="https://www.theworldavatar.com/kg/ontopoi"/>
        <rdfs:label>Pumps and compressors</rdfs:label>
    </owl:Class>
    


    <!-- https://www.theworldavatar.com/kg/ontopoi/Pupilreferralunits -->


    <owl:Class rdf:about="https://www.theworldavatar.com/kg/ontopoi/Pupilreferralunits">
        <rdfs:subClassOf rdf:resource="https://www.theworldavatar.com/kg/ontopoi/Primaryandsecondaryandtertiaryeducation"/>
        <rdfs:comment>Pupil referral units is a subcategory of primary, secondary and tertiary education</rdfs:comment>
        <rdfs:isDefinedBy rdf:resource="https://www.theworldavatar.com/kg/ontopoi"/>
        <rdfs:label>Pupil referral units</rdfs:label>
    </owl:Class>
    


    <!-- https://www.theworldavatar.com/kg/ontopoi/Racecoursesandgreyhoundtracks -->


    <owl:Class rdf:about="https://www.theworldavatar.com/kg/ontopoi/Racecoursesandgreyhoundtracks">
        <rdfs:subClassOf rdf:resource="https://www.theworldavatar.com/kg/ontopoi/Sportscomplex"/>
        <rdfs:comment>Racecourses and greyhound tracks is a subcategory of sports complex</rdfs:comment>
        <rdfs:isDefinedBy rdf:resource="https://www.theworldavatar.com/kg/ontopoi"/>
        <rdfs:label>Racecourses and greyhound tracks</rdfs:label>
    </owl:Class>
    


    <!-- https://www.theworldavatar.com/kg/ontopoi/Radarandtelecommunicationsequipment -->


    <owl:Class rdf:about="https://www.theworldavatar.com/kg/ontopoi/Radarandtelecommunicationsequipment">
        <rdfs:subClassOf rdf:resource="https://www.theworldavatar.com/kg/ontopoi/Industrialproducts"/>
        <rdfs:comment>Radar and telecommunications equipment is a subcategory of industrial products</rdfs:comment>
        <rdfs:isDefinedBy rdf:resource="https://www.theworldavatar.com/kg/ontopoi"/>
        <rdfs:label>Radar and telecommunications equipment</rdfs:label>
    </owl:Class>
    


    <!-- https://www.theworldavatar.com/kg/ontopoi/Ragmerchants -->


    <owl:Class rdf:about="https://www.theworldavatar.com/kg/ontopoi/Ragmerchants">
        <rdfs:subClassOf rdf:resource="https://www.theworldavatar.com/kg/ontopoi/Recyclingservices"/>
        <rdfs:comment>Rag merchants is a subcategory of recycling services</rdfs:comment>
        <rdfs:isDefinedBy rdf:resource="https://www.theworldavatar.com/kg/ontopoi"/>
        <rdfs:label>Rag merchants</rdfs:label>
    </owl:Class>
    


    <!-- https://www.theworldavatar.com/kg/ontopoi/Railwayrelatedservices -->


    <owl:Class rdf:about="https://www.theworldavatar.com/kg/ontopoi/Railwayrelatedservices">
        <rdfs:subClassOf rdf:resource="https://www.theworldavatar.com/kg/ontopoi/Transportandstorageanddelivery"/>
        <rdfs:comment>Railway related services is a subcategory of transport, storage and delivery</rdfs:comment>
        <rdfs:isDefinedBy rdf:resource="https://www.theworldavatar.com/kg/ontopoi"/>
        <rdfs:label>Railway related services</rdfs:label>
    </owl:Class>
    


    <!-- https://www.theworldavatar.com/kg/ontopoi/Railwaystationsandjunctionsandhalts -->


    <owl:Class rdf:about="https://www.theworldavatar.com/kg/ontopoi/Railwaystationsandjunctionsandhalts">
        <rdfs:subClassOf rdf:resource="https://www.theworldavatar.com/kg/ontopoi/Publictransportandstationsandinfrastructure"/>
        <rdfs:comment>Railway stations, junctions and halts is a subcategory of public transport, stations and infrastructure</rdfs:comment>
        <rdfs:isDefinedBy rdf:resource="https://www.theworldavatar.com/kg/ontopoi"/>
        <rdfs:label>Railway stations, junctions and halts</rdfs:label>
    </owl:Class>
    


    <!-- https://www.theworldavatar.com/kg/ontopoi/Recordingstudiosandrecordcompanies -->


    <owl:Class rdf:about="https://www.theworldavatar.com/kg/ontopoi/Recordingstudiosandrecordcompanies">
        <rdfs:subClassOf rdf:resource="https://www.theworldavatar.com/kg/ontopoi/ITandadvertisingandmarketingandmediaservices"/>
        <rdfs:comment>Recording studios and record companies is a subcategory of it, advertising, marketing and media service s</rdfs:comment>
        <rdfs:isDefinedBy rdf:resource="https://www.theworldavatar.com/kg/ontopoi"/>
        <rdfs:label>Recording studios and record companies</rdfs:label>
    </owl:Class>
    


    <!-- https://www.theworldavatar.com/kg/ontopoi/Recreational -->


    <owl:Class rdf:about="https://www.theworldavatar.com/kg/ontopoi/Recreational">
        <rdfs:subClassOf rdf:resource="https://www.theworldavatar.com/kg/ontopoi/Attractions"/>
        <rdfs:comment>Recreational is a subcategory of attractions</rdfs:comment>
        <rdfs:isDefinedBy rdf:resource="https://www.theworldavatar.com/kg/ontopoi"/>
        <rdfs:label>Recreational</rdfs:label>
    </owl:Class>
    


    <!-- https://www.theworldavatar.com/kg/ontopoi/Recreationalandvocationaleducation -->


    <owl:Class rdf:about="https://www.theworldavatar.com/kg/ontopoi/Recreationalandvocationaleducation">
        <rdfs:subClassOf rdf:resource="https://www.theworldavatar.com/kg/ontopoi/Educationandhealth"/>
        <rdfs:comment>Recreational and vocational education is a subcategory of education and health</rdfs:comment>
        <rdfs:isDefinedBy rdf:resource="https://www.theworldavatar.com/kg/ontopoi"/>
        <rdfs:label>Recreational and vocational education</rdfs:label>
    </owl:Class>
    


    <!-- https://www.theworldavatar.com/kg/ontopoi/Recyclingandreclamationanddisposal -->


    <owl:Class rdf:about="https://www.theworldavatar.com/kg/ontopoi/Recyclingandreclamationanddisposal">
        <rdfs:subClassOf rdf:resource="https://www.theworldavatar.com/kg/ontopoi/Recyclingservices"/>
        <rdfs:comment>Recycling, reclamation and disposal is a subcategory of recycling services</rdfs:comment>
        <rdfs:isDefinedBy rdf:resource="https://www.theworldavatar.com/kg/ontopoi"/>
        <rdfs:label>Recycling, reclamation and disposal</rdfs:label>
    </owl:Class>
    


    <!-- https://www.theworldavatar.com/kg/ontopoi/Recyclingcentres -->


    <owl:Class rdf:about="https://www.theworldavatar.com/kg/ontopoi/Recyclingcentres">
        <rdfs:subClassOf rdf:resource="https://www.theworldavatar.com/kg/ontopoi/Infrastructureandfacilities"/>
        <rdfs:comment>Recycling centres is a subcategory of infrastructure and facilities</rdfs:comment>
        <rdfs:isDefinedBy rdf:resource="https://www.theworldavatar.com/kg/ontopoi"/>
        <rdfs:label>Recycling centres</rdfs:label>
    </owl:Class>
    


    <!-- https://www.theworldavatar.com/kg/ontopoi/Recyclingservices -->


    <owl:Class rdf:about="https://www.theworldavatar.com/kg/ontopoi/Recyclingservices">
        <rdfs:subClassOf rdf:resource="https://www.theworldavatar.com/kg/ontopoi/Commercialservices"/>
        <rdfs:comment>Recycling services is a subcategory of commercial services</rdfs:comment>
        <rdfs:isDefinedBy rdf:resource="https://www.theworldavatar.com/kg/ontopoi"/>
        <rdfs:label>Recycling services</rdfs:label>
    </owl:Class>
    


    <!-- https://www.theworldavatar.com/kg/ontopoi/Refrigerationandfreezingappliances -->


    <owl:Class rdf:about="https://www.theworldavatar.com/kg/ontopoi/Refrigerationandfreezingappliances">
        <rdfs:subClassOf rdf:resource="https://www.theworldavatar.com/kg/ontopoi/Consumerproducts"/>
        <rdfs:comment>Refrigeration and freezing appliances is a subcategory of consumer products</rdfs:comment>
        <rdfs:isDefinedBy rdf:resource="https://www.theworldavatar.com/kg/ontopoi"/>
        <rdfs:label>Refrigeration and freezing appliances</rdfs:label>
    </owl:Class>
    


    <!-- https://www.theworldavatar.com/kg/ontopoi/Refusedisposalfacilities -->


    <owl:Class rdf:about="https://www.theworldavatar.com/kg/ontopoi/Refusedisposalfacilities">
        <rdfs:subClassOf rdf:resource="https://www.theworldavatar.com/kg/ontopoi/Infrastructureandfacilities"/>
        <rdfs:comment>Refuse disposal facilities is a subcategory of infrastructure and facilities</rdfs:comment>
        <rdfs:isDefinedBy rdf:resource="https://www.theworldavatar.com/kg/ontopoi"/>
        <rdfs:label>Refuse disposal facilities</rdfs:label>
    </owl:Class>
    


    <!-- https://www.theworldavatar.com/kg/ontopoi/Registrarsoffices -->


    <owl:Class rdf:about="https://www.theworldavatar.com/kg/ontopoi/Registrarsoffices">
        <rdfs:subClassOf rdf:resource="https://www.theworldavatar.com/kg/ontopoi/Centralandlocalgovernment"/>
        <rdfs:comment>Registrars offices is a subcategory of central and local government</rdfs:comment>
        <rdfs:isDefinedBy rdf:resource="https://www.theworldavatar.com/kg/ontopoi"/>
        <rdfs:label>Registrars offices</rdfs:label>
    </owl:Class>
    


    <!-- https://www.theworldavatar.com/kg/ontopoi/Religiousorganisations -->


    <owl:Class rdf:about="https://www.theworldavatar.com/kg/ontopoi/Religiousorganisations">
        <rdfs:subClassOf rdf:resource="https://www.theworldavatar.com/kg/ontopoi/Organisations"/>
        <rdfs:comment>Religious organisations is a subcategory of organisations</rdfs:comment>
        <rdfs:isDefinedBy rdf:resource="https://www.theworldavatar.com/kg/ontopoi"/>
        <rdfs:label>Religious organisations</rdfs:label>
    </owl:Class>
    


    <!-- https://www.theworldavatar.com/kg/ontopoi/Removalsandshippingagents -->


    <owl:Class rdf:about="https://www.theworldavatar.com/kg/ontopoi/Removalsandshippingagents">
        <rdfs:subClassOf rdf:resource="https://www.theworldavatar.com/kg/ontopoi/Transportandstorageanddelivery"/>
        <rdfs:comment>Removals and shipping agents is a subcategory of transport, storage and delivery</rdfs:comment>
        <rdfs:isDefinedBy rdf:resource="https://www.theworldavatar.com/kg/ontopoi"/>
        <rdfs:label>Removals and shipping agents</rdfs:label>
    </owl:Class>
    


    <!-- https://www.theworldavatar.com/kg/ontopoi/Rentingandleasingofpersonalandhouseholdgoods -->


    <owl:Class rdf:about="https://www.theworldavatar.com/kg/ontopoi/Rentingandleasingofpersonalandhouseholdgoods">
        <rdfs:subClassOf rdf:resource="https://www.theworldavatar.com/kg/ontopoi/Hireservices"/>
        <rdfs:comment>Renting and leasing of personal and household goods is a subcategory of hire services</rdfs:comment>
        <rdfs:isDefinedBy rdf:resource="https://www.theworldavatar.com/kg/ontopoi"/>
        <rdfs:label>Renting and leasing of personal and household goods</rdfs:label>
    </owl:Class>
    


    <!-- https://www.theworldavatar.com/kg/ontopoi/Repairandservicing -->


    <owl:Class rdf:about="https://www.theworldavatar.com/kg/ontopoi/Repairandservicing">
        <rdfs:subClassOf rdf:resource="https://www.theworldavatar.com/kg/ontopoi/Commercialservices"/>
        <rdfs:comment>Repair and servicing is a subcategory of commercial services</rdfs:comment>
        <rdfs:isDefinedBy rdf:resource="https://www.theworldavatar.com/kg/ontopoi"/>
        <rdfs:label>Repair and servicing</rdfs:label>
    </owl:Class>
    


    <!-- https://www.theworldavatar.com/kg/ontopoi/Researchanddesign -->


    <owl:Class rdf:about="https://www.theworldavatar.com/kg/ontopoi/Researchanddesign">
        <rdfs:subClassOf rdf:resource="https://www.theworldavatar.com/kg/ontopoi/Commercialservices"/>
        <rdfs:comment>Research and design is a subcategory of commercial services</rdfs:comment>
        <rdfs:isDefinedBy rdf:resource="https://www.theworldavatar.com/kg/ontopoi"/>
        <rdfs:label>Research and design</rdfs:label>
    </owl:Class>
    


    <!-- https://www.theworldavatar.com/kg/ontopoi/Researchservices -->


    <owl:Class rdf:about="https://www.theworldavatar.com/kg/ontopoi/Researchservices">
        <rdfs:subClassOf rdf:resource="https://www.theworldavatar.com/kg/ontopoi/Researchanddesign"/>
        <rdfs:comment>Research services is a subcategory of research and design</rdfs:comment>
        <rdfs:isDefinedBy rdf:resource="https://www.theworldavatar.com/kg/ontopoi"/>
        <rdfs:label>Research services</rdfs:label>
    </owl:Class>
    


    <!-- https://www.theworldavatar.com/kg/ontopoi/Reservoirs -->


    <owl:Class rdf:about="https://www.theworldavatar.com/kg/ontopoi/Reservoirs">
        <rdfs:subClassOf rdf:resource="https://www.theworldavatar.com/kg/ontopoi/Bodiesofwater"/>
        <rdfs:comment>Reservoirs is a subcategory of bodies of water</rdfs:comment>
        <rdfs:isDefinedBy rdf:resource="https://www.theworldavatar.com/kg/ontopoi"/>
        <rdfs:label>Reservoirs</rdfs:label>
    </owl:Class>
    


    <!-- https://www.theworldavatar.com/kg/ontopoi/Restaurants -->


    <owl:Class rdf:about="https://www.theworldavatar.com/kg/ontopoi/Restaurants">
        <rdfs:subClassOf rdf:resource="https://www.theworldavatar.com/kg/ontopoi/Eatinganddrinking"/>
        <rdfs:comment>Restaurants is a subcategory of eating and drinking</rdfs:comment>
        <rdfs:isDefinedBy rdf:resource="https://www.theworldavatar.com/kg/ontopoi"/>
        <rdfs:label>Restaurants</rdfs:label>
    </owl:Class>
    


    <!-- https://www.theworldavatar.com/kg/ontopoi/Restorationandpreservationservices -->


    <owl:Class rdf:about="https://www.theworldavatar.com/kg/ontopoi/Restorationandpreservationservices">
        <rdfs:subClassOf rdf:resource="https://www.theworldavatar.com/kg/ontopoi/Constructionservices"/>
        <rdfs:comment>Restoration and preservation services is a subcategory of construction services</rdfs:comment>
        <rdfs:isDefinedBy rdf:resource="https://www.theworldavatar.com/kg/ontopoi"/>
        <rdfs:label>Restoration and preservation services</rdfs:label>
    </owl:Class>
    


    <!-- https://www.theworldavatar.com/kg/ontopoi/Retail -->


    <owl:Class rdf:about="https://www.theworldavatar.com/kg/ontopoi/Retail"/>
    


    <!-- https://www.theworldavatar.com/kg/ontopoi/Revenueandcustomsoffices -->


    <owl:Class rdf:about="https://www.theworldavatar.com/kg/ontopoi/Revenueandcustomsoffices">
        <rdfs:subClassOf rdf:resource="https://www.theworldavatar.com/kg/ontopoi/Centralandlocalgovernment"/>
        <rdfs:comment>Revenue and customs offices is a subcategory of central and local government</rdfs:comment>
        <rdfs:isDefinedBy rdf:resource="https://www.theworldavatar.com/kg/ontopoi"/>
        <rdfs:label>Revenue and customs offices</rdfs:label>
    </owl:Class>
    


    <!-- https://www.theworldavatar.com/kg/ontopoi/Ridingschoolsandliverystablesandequestriancentres -->


    <owl:Class rdf:about="https://www.theworldavatar.com/kg/ontopoi/Ridingschoolsandliverystablesandequestriancentres">
        <rdfs:subClassOf rdf:resource="https://www.theworldavatar.com/kg/ontopoi/Outdoorpursuits"/>
        <rdfs:comment>Riding schools, livery stables and equestrian centres is a subcategory of outdoor pursuits</rdfs:comment>
        <rdfs:isDefinedBy rdf:resource="https://www.theworldavatar.com/kg/ontopoi"/>
        <rdfs:label>Riding schools, livery stables and equestrian centres</rdfs:label>
    </owl:Class>
    


    <!-- https://www.theworldavatar.com/kg/ontopoi/Riversandcanalorganisationsandinfrastructure -->


    <owl:Class rdf:about="https://www.theworldavatar.com/kg/ontopoi/Riversandcanalorganisationsandinfrastructure">
        <rdfs:subClassOf rdf:resource="https://www.theworldavatar.com/kg/ontopoi/Water"/>
        <rdfs:comment>Rivers and canal organisations and infrastructure is a subcategory of water</rdfs:comment>
        <rdfs:isDefinedBy rdf:resource="https://www.theworldavatar.com/kg/ontopoi"/>
        <rdfs:label>Rivers and canal organisations and infrastructure</rdfs:label>
    </owl:Class>
    


    <!-- https://www.theworldavatar.com/kg/ontopoi/Roadandrail -->


    <owl:Class rdf:about="https://www.theworldavatar.com/kg/ontopoi/Roadandrail">
        <rdfs:subClassOf rdf:resource="https://www.theworldavatar.com/kg/ontopoi/Transport"/>
        <rdfs:comment>Road and rail is a subcategory of transport</rdfs:comment>
        <rdfs:isDefinedBy rdf:resource="https://www.theworldavatar.com/kg/ontopoi"/>
        <rdfs:label>Road and rail</rdfs:label>
    </owl:Class>
    


    <!-- https://www.theworldavatar.com/kg/ontopoi/Roadconstructionservices -->


    <owl:Class rdf:about="https://www.theworldavatar.com/kg/ontopoi/Roadconstructionservices">
        <rdfs:subClassOf rdf:resource="https://www.theworldavatar.com/kg/ontopoi/Constructionservices"/>
        <rdfs:comment>Road construction services is a subcategory of construction services</rdfs:comment>
        <rdfs:isDefinedBy rdf:resource="https://www.theworldavatar.com/kg/ontopoi"/>
        <rdfs:label>Road construction services</rdfs:label>
    </owl:Class>
    


    <!-- https://www.theworldavatar.com/kg/ontopoi/Roadmaintenanceequipment -->


    <owl:Class rdf:about="https://www.theworldavatar.com/kg/ontopoi/Roadmaintenanceequipment">
        <rdfs:subClassOf rdf:resource="https://www.theworldavatar.com/kg/ontopoi/Industrialproducts"/>
        <rdfs:comment>Road maintenance equipment is a subcategory of industrial products</rdfs:comment>
        <rdfs:isDefinedBy rdf:resource="https://www.theworldavatar.com/kg/ontopoi"/>
        <rdfs:label>Road maintenance equipment</rdfs:label>
    </owl:Class>
    


    <!-- https://www.theworldavatar.com/kg/ontopoi/Roofingandchimneyservices -->


    <owl:Class rdf:about="https://www.theworldavatar.com/kg/ontopoi/Roofingandchimneyservices">
        <rdfs:subClassOf rdf:resource="https://www.theworldavatar.com/kg/ontopoi/Constructionservices"/>
        <rdfs:comment>Roofing and chimney services is a subcategory of construction services</rdfs:comment>
        <rdfs:isDefinedBy rdf:resource="https://www.theworldavatar.com/kg/ontopoi"/>
        <rdfs:label>Roofing and chimney services</rdfs:label>
    </owl:Class>
    


    <!-- https://www.theworldavatar.com/kg/ontopoi/Ropesandnetsandcordage -->


    <owl:Class rdf:about="https://www.theworldavatar.com/kg/ontopoi/Ropesandnetsandcordage">
        <rdfs:subClassOf rdf:resource="https://www.theworldavatar.com/kg/ontopoi/Industrialproducts"/>
        <rdfs:comment>Ropes, nets and cordage is a subcategory of industrial products</rdfs:comment>
        <rdfs:isDefinedBy rdf:resource="https://www.theworldavatar.com/kg/ontopoi"/>
        <rdfs:label>Ropes, nets and cordage</rdfs:label>
    </owl:Class>
    


    <!-- https://www.theworldavatar.com/kg/ontopoi/Rubberandsiliconesandplastics -->


    <owl:Class rdf:about="https://www.theworldavatar.com/kg/ontopoi/Rubberandsiliconesandplastics">
        <rdfs:subClassOf rdf:resource="https://www.theworldavatar.com/kg/ontopoi/Industrialproducts"/>
        <rdfs:comment>Rubber, silicones and plastics is a subcategory of industrial products</rdfs:comment>
        <rdfs:isDefinedBy rdf:resource="https://www.theworldavatar.com/kg/ontopoi"/>
        <rdfs:label>Rubber, silicones and plastics</rdfs:label>
    </owl:Class>
    


    <!-- https://www.theworldavatar.com/kg/ontopoi/Sailingschools -->


    <owl:Class rdf:about="https://www.theworldavatar.com/kg/ontopoi/Sailingschools">
        <rdfs:subClassOf rdf:resource="https://www.theworldavatar.com/kg/ontopoi/Recreationalandvocationaleducation"/>
        <rdfs:comment>Sailing schools is a subcategory of recreational and vocational education</rdfs:comment>
        <rdfs:isDefinedBy rdf:resource="https://www.theworldavatar.com/kg/ontopoi"/>
        <rdfs:label>Sailing schools</rdfs:label>
    </owl:Class>
    


    <!-- https://www.theworldavatar.com/kg/ontopoi/Salmonladders -->


    <owl:Class rdf:about="https://www.theworldavatar.com/kg/ontopoi/Salmonladders">
        <rdfs:subClassOf rdf:resource="https://www.theworldavatar.com/kg/ontopoi/Botanicalandzoological"/>
        <rdfs:comment>Salmon ladders is a subcategory of botanical and zoological</rdfs:comment>
        <rdfs:isDefinedBy rdf:resource="https://www.theworldavatar.com/kg/ontopoi"/>
        <rdfs:label>Salmon ladders</rdfs:label>
    </owl:Class>
    


    <!-- https://www.theworldavatar.com/kg/ontopoi/Sandandgravelandclayextractionandmerchants -->


    <owl:Class rdf:about="https://www.theworldavatar.com/kg/ontopoi/Sandandgravelandclayextractionandmerchants">
        <rdfs:subClassOf rdf:resource="https://www.theworldavatar.com/kg/ontopoi/Extractiveindustries"/>
        <rdfs:comment>Sand, gravel and clay extraction and merchants is a subcategory of extractive industries</rdfs:comment>
        <rdfs:isDefinedBy rdf:resource="https://www.theworldavatar.com/kg/ontopoi"/>
        <rdfs:label>Sand, gravel and clay extraction and merchants</rdfs:label>
    </owl:Class>
    


    <!-- https://www.theworldavatar.com/kg/ontopoi/Saunasandsunbeds -->


    <owl:Class rdf:about="https://www.theworldavatar.com/kg/ontopoi/Saunasandsunbeds">
        <rdfs:subClassOf rdf:resource="https://www.theworldavatar.com/kg/ontopoi/Consumerproducts"/>
        <rdfs:comment>Saunas and sunbeds is a subcategory of consumer products</rdfs:comment>
        <rdfs:isDefinedBy rdf:resource="https://www.theworldavatar.com/kg/ontopoi"/>
        <rdfs:label>Saunas and sunbeds</rdfs:label>
    </owl:Class>
    


    <!-- https://www.theworldavatar.com/kg/ontopoi/Scrapmetaldealersandbreakersyards -->


    <owl:Class rdf:about="https://www.theworldavatar.com/kg/ontopoi/Scrapmetaldealersandbreakersyards">
        <rdfs:subClassOf rdf:resource="https://www.theworldavatar.com/kg/ontopoi/Recyclingservices"/>
        <rdfs:comment>Scrap meta ldealers and breakers yards is a subcategory of recycling services</rdfs:comment>
        <rdfs:isDefinedBy rdf:resource="https://www.theworldavatar.com/kg/ontopoi"/>
        <rdfs:label>Scrap meta ldealers and breakers yards</rdfs:label>
    </owl:Class>
    


    <!-- https://www.theworldavatar.com/kg/ontopoi/Sculptorsandwoodworkersandstonemasons -->


    <owl:Class rdf:about="https://www.theworldavatar.com/kg/ontopoi/Sculptorsandwoodworkersandstonemasons">
        <rdfs:subClassOf rdf:resource="https://www.theworldavatar.com/kg/ontopoi/Personalandconsumerandotherservices"/>
        <rdfs:comment>Sculptors, woodworkers and stonemasons is a subcategory of personal, consumer and other services</rdfs:comment>
        <rdfs:isDefinedBy rdf:resource="https://www.theworldavatar.com/kg/ontopoi"/>
        <rdfs:label>Sculptors, woodworkers and stonemasons</rdfs:label>
    </owl:Class>
    


    <!-- https://www.theworldavatar.com/kg/ontopoi/Sealsandtapesandtapsandvalves -->


    <owl:Class rdf:about="https://www.theworldavatar.com/kg/ontopoi/Sealsandtapesandtapsandvalves">
        <rdfs:subClassOf rdf:resource="https://www.theworldavatar.com/kg/ontopoi/Industrialproducts"/>
        <rdfs:comment>Seals, tapes, taps and valves is a subcategory of industrial products</rdfs:comment>
        <rdfs:isDefinedBy rdf:resource="https://www.theworldavatar.com/kg/ontopoi"/>
        <rdfs:label>Seals, tapes, taps and valves</rdfs:label>
    </owl:Class>
    


    <!-- https://www.theworldavatar.com/kg/ontopoi/Second-handgoods -->


    <owl:Class rdf:about="https://www.theworldavatar.com/kg/ontopoi/Second-handgoods">
        <rdfs:subClassOf rdf:resource="https://www.theworldavatar.com/kg/ontopoi/Householdandofficeandleisureandgarden"/>
        <rdfs:comment>Second-hand goods is a subcategory of household, office, leisure and garden</rdfs:comment>
        <rdfs:isDefinedBy rdf:resource="https://www.theworldavatar.com/kg/ontopoi"/>
        <rdfs:label>Second-hand goods</rdfs:label>
    </owl:Class>
    


    <!-- https://www.theworldavatar.com/kg/ontopoi/Second-handvehicles -->


    <owl:Class rdf:about="https://www.theworldavatar.com/kg/ontopoi/Second-handvehicles">
        <rdfs:subClassOf rdf:resource="https://www.theworldavatar.com/kg/ontopoi/Motoring"/>
        <rdfs:comment>Second-hand vehicles is a subcategory of motoring</rdfs:comment>
        <rdfs:isDefinedBy rdf:resource="https://www.theworldavatar.com/kg/ontopoi"/>
        <rdfs:label>Second-hand vehicles</rdfs:label>
    </owl:Class>
    


    <!-- https://www.theworldavatar.com/kg/ontopoi/Secureunits -->


    <owl:Class rdf:about="https://www.theworldavatar.com/kg/ontopoi/Secureunits">
        <rdfs:subClassOf rdf:resource="https://www.theworldavatar.com/kg/ontopoi/Educationsupportservices"/>
        <rdfs:comment>Secure units is a subcategory of education support services</rdfs:comment>
        <rdfs:isDefinedBy rdf:resource="https://www.theworldavatar.com/kg/ontopoi"/>
        <rdfs:label>Secure units</rdfs:label>
    </owl:Class>
    


    <!-- https://www.theworldavatar.com/kg/ontopoi/Securityconsultants -->


    <owl:Class rdf:about="https://www.theworldavatar.com/kg/ontopoi/Securityconsultants">
        <rdfs:subClassOf rdf:resource="https://www.theworldavatar.com/kg/ontopoi/Consultancies"/>
        <rdfs:comment>Security consultants is a subcategory of consultancies</rdfs:comment>
        <rdfs:isDefinedBy rdf:resource="https://www.theworldavatar.com/kg/ontopoi"/>
        <rdfs:label>Security consultants</rdfs:label>
    </owl:Class>
    


    <!-- https://www.theworldavatar.com/kg/ontopoi/Selfcatering -->


    <owl:Class rdf:about="https://www.theworldavatar.com/kg/ontopoi/Selfcatering">
        <rdfs:subClassOf rdf:resource="https://www.theworldavatar.com/kg/ontopoi/Accommodation"/>
        <rdfs:comment>Self catering is a subcategory of accommodation</rdfs:comment>
        <rdfs:isDefinedBy rdf:resource="https://www.theworldavatar.com/kg/ontopoi"/>
        <rdfs:label>Self catering</rdfs:label>
    </owl:Class>
    


    <!-- https://www.theworldavatar.com/kg/ontopoi/Serviceindustryequipmentrepairs -->


    <owl:Class rdf:about="https://www.theworldavatar.com/kg/ontopoi/Serviceindustryequipmentrepairs">
        <rdfs:subClassOf rdf:resource="https://www.theworldavatar.com/kg/ontopoi/Repairandservicing"/>
        <rdfs:comment>Service industry equipment repairs is a subcategory of repair and servicing</rdfs:comment>
        <rdfs:isDefinedBy rdf:resource="https://www.theworldavatar.com/kg/ontopoi"/>
        <rdfs:label>Service industry equipment repairs</rdfs:label>
    </owl:Class>
    


    <!-- https://www.theworldavatar.com/kg/ontopoi/SewageServices -->


    <owl:Class rdf:about="https://www.theworldavatar.com/kg/ontopoi/SewageServices">
        <rdfs:subClassOf rdf:resource="https://www.theworldavatar.com/kg/ontopoi/Personalandconsumerandotherservices"/>
        <rdfs:comment>Sewage services is a subcategory of personal, consumer and other services</rdfs:comment>
        <rdfs:isDefinedBy rdf:resource="https://www.theworldavatar.com/kg/ontopoi"/>
        <rdfs:label>Sewage Services</rdfs:label>
    </owl:Class>
    


    <!-- https://www.theworldavatar.com/kg/ontopoi/Shelvingandstorageandsafesandvaults -->


    <owl:Class rdf:about="https://www.theworldavatar.com/kg/ontopoi/Shelvingandstorageandsafesandvaults">
        <rdfs:subClassOf rdf:resource="https://www.theworldavatar.com/kg/ontopoi/Industrialproducts"/>
        <rdfs:comment>Shelving, storage, safes and vaults is a subcategory of industrial products</rdfs:comment>
        <rdfs:isDefinedBy rdf:resource="https://www.theworldavatar.com/kg/ontopoi"/>
        <rdfs:label>Shelving, storage, safes and vaults</rdfs:label>
    </owl:Class>
    


    <!-- https://www.theworldavatar.com/kg/ontopoi/Shoerepairs -->


    <owl:Class rdf:about="https://www.theworldavatar.com/kg/ontopoi/Shoerepairs">
        <rdfs:subClassOf rdf:resource="https://www.theworldavatar.com/kg/ontopoi/Repairandservicing"/>
        <rdfs:comment>Shoe repairs is a subcategory of repair and servicing</rdfs:comment>
        <rdfs:isDefinedBy rdf:resource="https://www.theworldavatar.com/kg/ontopoi"/>
        <rdfs:label>Shoe repairs</rdfs:label>
    </owl:Class>
    


    <!-- https://www.theworldavatar.com/kg/ontopoi/Shootingfacilities -->


    <owl:Class rdf:about="https://www.theworldavatar.com/kg/ontopoi/Shootingfacilities">
        <rdfs:subClassOf rdf:resource="https://www.theworldavatar.com/kg/ontopoi/Sportscomplex"/>
        <rdfs:comment>Shooting facilities is a subcategory of sports complex</rdfs:comment>
        <rdfs:isDefinedBy rdf:resource="https://www.theworldavatar.com/kg/ontopoi"/>
        <rdfs:label>Shooting facilities</rdfs:label>
    </owl:Class>
    


    <!-- https://www.theworldavatar.com/kg/ontopoi/Shoppingcentresandretailparks -->


    <owl:Class rdf:about="https://www.theworldavatar.com/kg/ontopoi/Shoppingcentresandretailparks">
        <rdfs:subClassOf rdf:resource="https://www.theworldavatar.com/kg/ontopoi/Householdandofficeandleisureandgarden"/>
        <rdfs:comment>Shopping centres and retail parks is a subcategory of household, office, leisure and garden</rdfs:comment>
        <rdfs:isDefinedBy rdf:resource="https://www.theworldavatar.com/kg/ontopoi"/>
        <rdfs:label>Shopping centres and retail parks</rdfs:label>
    </owl:Class>
    


    <!-- https://www.theworldavatar.com/kg/ontopoi/Sightseeingandtoursandviewingandvisitorcentres -->


    <owl:Class rdf:about="https://www.theworldavatar.com/kg/ontopoi/Sightseeingandtoursandviewingandvisitorcentres">
        <rdfs:subClassOf rdf:resource="https://www.theworldavatar.com/kg/ontopoi/Tourism"/>
        <rdfs:comment>Sightseeing, tours, viewing and visitor centres is a subcategory of tourism</rdfs:comment>
        <rdfs:isDefinedBy rdf:resource="https://www.theworldavatar.com/kg/ontopoi"/>
        <rdfs:label>Sightseeing, tours, viewing and visitor centres</rdfs:label>
    </owl:Class>
    


    <!-- https://www.theworldavatar.com/kg/ontopoi/Signallingfacilities -->


    <owl:Class rdf:about="https://www.theworldavatar.com/kg/ontopoi/Signallingfacilities">
        <rdfs:subClassOf rdf:resource="https://www.theworldavatar.com/kg/ontopoi/Roadandrail"/>
        <rdfs:comment>Signalling facilities is a subcategory of road and rail</rdfs:comment>
        <rdfs:isDefinedBy rdf:resource="https://www.theworldavatar.com/kg/ontopoi"/>
        <rdfs:label>Signalling facilities</rdfs:label>
    </owl:Class>
    


    <!-- https://www.theworldavatar.com/kg/ontopoi/Signs -->


    <owl:Class rdf:about="https://www.theworldavatar.com/kg/ontopoi/Signs">
        <rdfs:subClassOf rdf:resource="https://www.theworldavatar.com/kg/ontopoi/Industrialproducts"/>
        <rdfs:comment>Signs is a subcategory of industrial products</rdfs:comment>
        <rdfs:isDefinedBy rdf:resource="https://www.theworldavatar.com/kg/ontopoi"/>
        <rdfs:label>Signs</rdfs:label>
    </owl:Class>
    


    <!-- https://www.theworldavatar.com/kg/ontopoi/Skiinfrastructureandaerialcableways -->


    <owl:Class rdf:about="https://www.theworldavatar.com/kg/ontopoi/Skiinfrastructureandaerialcableways">
        <rdfs:subClassOf rdf:resource="https://www.theworldavatar.com/kg/ontopoi/Sportscomplex"/>
        <rdfs:comment>Ski infrastructure and aerial cableways is a subcategory of sports complex</rdfs:comment>
        <rdfs:isDefinedBy rdf:resource="https://www.theworldavatar.com/kg/ontopoi"/>
        <rdfs:label>Ski infrastructure and aerial cableways</rdfs:label>
    </owl:Class>
    


    <!-- https://www.theworldavatar.com/kg/ontopoi/Slimmingclubsandservices -->


    <owl:Class rdf:about="https://www.theworldavatar.com/kg/ontopoi/Slimmingclubsandservices">
        <rdfs:subClassOf rdf:resource="https://www.theworldavatar.com/kg/ontopoi/Personalandconsumerandotherservices"/>
        <rdfs:comment>Slimming clubs and services is a subcategory of personal, consumer and other services</rdfs:comment>
        <rdfs:isDefinedBy rdf:resource="https://www.theworldavatar.com/kg/ontopoi"/>
        <rdfs:label>Slimming clubs and services</rdfs:label>
    </owl:Class>
    


    <!-- https://www.theworldavatar.com/kg/ontopoi/Snookerandpoolhalls -->


    <owl:Class rdf:about="https://www.theworldavatar.com/kg/ontopoi/Snookerandpoolhalls">
        <rdfs:subClassOf rdf:resource="https://www.theworldavatar.com/kg/ontopoi/Sportscomplex"/>
        <rdfs:comment>Snooker and pool halls is a subcategory of sports complex</rdfs:comment>
        <rdfs:isDefinedBy rdf:resource="https://www.theworldavatar.com/kg/ontopoi"/>
        <rdfs:label>Snooker and pool halls</rdfs:label>
    </owl:Class>
    


    <!-- https://www.theworldavatar.com/kg/ontopoi/Socialclubs -->


    <owl:Class rdf:about="https://www.theworldavatar.com/kg/ontopoi/Socialclubs">
        <rdfs:subClassOf rdf:resource="https://www.theworldavatar.com/kg/ontopoi/Venuesandstageandscreen"/>
        <rdfs:comment>Social clubs is a subcategory of venues, stage and screen</rdfs:comment>
        <rdfs:isDefinedBy rdf:resource="https://www.theworldavatar.com/kg/ontopoi"/>
        <rdfs:label>Social clubs</rdfs:label>
    </owl:Class>
    


    <!-- https://www.theworldavatar.com/kg/ontopoi/Socialserviceactivities -->


    <owl:Class rdf:about="https://www.theworldavatar.com/kg/ontopoi/Socialserviceactivities">
        <rdfs:subClassOf rdf:resource="https://www.theworldavatar.com/kg/ontopoi/Centralandlocalgovernment"/>
        <rdfs:comment>Social service activities is a subcategory of central and local government</rdfs:comment>
        <rdfs:isDefinedBy rdf:resource="https://www.theworldavatar.com/kg/ontopoi"/>
        <rdfs:label>Social service activities</rdfs:label>
    </owl:Class>
    


    <!-- https://www.theworldavatar.com/kg/ontopoi/Solicitorsandadvocatesandnotariespublic -->


    <owl:Class rdf:about="https://www.theworldavatar.com/kg/ontopoi/Solicitorsandadvocatesandnotariespublic">
        <rdfs:subClassOf rdf:resource="https://www.theworldavatar.com/kg/ontopoi/Legalandfinancial"/>
        <rdfs:comment>Solicitors, advocates and notaries public is a subcategory of legal and financial</rdfs:comment>
        <rdfs:isDefinedBy rdf:resource="https://www.theworldavatar.com/kg/ontopoi"/>
        <rdfs:label>Solicitors, advocates and notaries public</rdfs:label>
    </owl:Class>
    


    <!-- https://www.theworldavatar.com/kg/ontopoi/Soundandlightandvisionserviceandequipmenthire -->


    <owl:Class rdf:about="https://www.theworldavatar.com/kg/ontopoi/Soundandlightandvisionserviceandequipmenthire">
        <rdfs:subClassOf rdf:resource="https://www.theworldavatar.com/kg/ontopoi/Hireservices"/>
        <rdfs:comment>Sound, light and vision service and equipment hire is a subcategory of hire services</rdfs:comment>
        <rdfs:isDefinedBy rdf:resource="https://www.theworldavatar.com/kg/ontopoi"/>
        <rdfs:label>Sound, light and vision service and equipment hire</rdfs:label>
    </owl:Class>
    


    <!-- https://www.theworldavatar.com/kg/ontopoi/Spas -->


    <owl:Class rdf:about="https://www.theworldavatar.com/kg/ontopoi/Spas">
        <rdfs:subClassOf rdf:resource="https://www.theworldavatar.com/kg/ontopoi/Personalandconsumerandotherservices"/>
        <rdfs:comment>Spas is a subcategory of personal, consumer and other services</rdfs:comment>
        <rdfs:isDefinedBy rdf:resource="https://www.theworldavatar.com/kg/ontopoi"/>
        <rdfs:label>Spas</rdfs:label>
    </owl:Class>
    


    <!-- https://www.theworldavatar.com/kg/ontopoi/Specialpurposemachineryandequipment -->


    <owl:Class rdf:about="https://www.theworldavatar.com/kg/ontopoi/Specialpurposemachineryandequipment">
        <rdfs:subClassOf rdf:resource="https://www.theworldavatar.com/kg/ontopoi/Industrialproducts"/>
        <rdfs:comment>Special purpose machinery and equipment is a subcategory of industrial products</rdfs:comment>
        <rdfs:isDefinedBy rdf:resource="https://www.theworldavatar.com/kg/ontopoi"/>
        <rdfs:label>Special purpose machinery and equipment</rdfs:label>
    </owl:Class>
    


    <!-- https://www.theworldavatar.com/kg/ontopoi/Specialschoolsandcolleges -->


    <owl:Class rdf:about="https://www.theworldavatar.com/kg/ontopoi/Specialschoolsandcolleges">
        <rdfs:subClassOf rdf:resource="https://www.theworldavatar.com/kg/ontopoi/Primaryandsecondaryandtertiaryeducation"/>
        <rdfs:comment>Special schools and colleges is a subcategory of primary, secondary and tertiary education</rdfs:comment>
        <rdfs:isDefinedBy rdf:resource="https://www.theworldavatar.com/kg/ontopoi"/>
        <rdfs:label>Special schools and colleges</rdfs:label>
    </owl:Class>
    


    <!-- https://www.theworldavatar.com/kg/ontopoi/Speechtherapists -->


    <owl:Class rdf:about="https://www.theworldavatar.com/kg/ontopoi/Speechtherapists">
        <rdfs:subClassOf rdf:resource="https://www.theworldavatar.com/kg/ontopoi/Healthpractitionersandestablishments"/>
        <rdfs:comment>Speech therapists is a subcategory of health practitioners and establishments</rdfs:comment>
        <rdfs:isDefinedBy rdf:resource="https://www.theworldavatar.com/kg/ontopoi"/>
        <rdfs:label>Speech therapists</rdfs:label>
    </owl:Class>
    


    <!-- https://www.theworldavatar.com/kg/ontopoi/Sportandentertainment -->


    <owl:Class rdf:about="https://www.theworldavatar.com/kg/ontopoi/Sportandentertainment"/>
    


    <!-- https://www.theworldavatar.com/kg/ontopoi/Sportandentertainmentsupportservices -->


    <owl:Class rdf:about="https://www.theworldavatar.com/kg/ontopoi/Sportandentertainmentsupportservices">
        <rdfs:subClassOf rdf:resource="https://www.theworldavatar.com/kg/ontopoi/Sportandentertainment"/>
        <rdfs:comment>Sport and entertainment support services is a subcategory of sport and entertainment</rdfs:comment>
        <rdfs:isDefinedBy rdf:resource="https://www.theworldavatar.com/kg/ontopoi"/>
        <rdfs:label>Sport and entertainment support services</rdfs:label>
    </owl:Class>
    


    <!-- https://www.theworldavatar.com/kg/ontopoi/Sportsandfitnesscoaching -->


    <owl:Class rdf:about="https://www.theworldavatar.com/kg/ontopoi/Sportsandfitnesscoaching">
        <rdfs:subClassOf rdf:resource="https://www.theworldavatar.com/kg/ontopoi/Recreationalandvocationaleducation"/>
        <rdfs:comment>Sports and fitness coaching is a subcategory of recreational and vocational education</rdfs:comment>
        <rdfs:isDefinedBy rdf:resource="https://www.theworldavatar.com/kg/ontopoi"/>
        <rdfs:label>Sports and fitness coaching</rdfs:label>
    </owl:Class>
    


    <!-- https://www.theworldavatar.com/kg/ontopoi/Sportsandleisureequipmentrepair -->


    <owl:Class rdf:about="https://www.theworldavatar.com/kg/ontopoi/Sportsandleisureequipmentrepair">
        <rdfs:subClassOf rdf:resource="https://www.theworldavatar.com/kg/ontopoi/Repairandservicing"/>
        <rdfs:comment>Sports and leisure equipment repair is a subcategory of repair and servicing</rdfs:comment>
        <rdfs:isDefinedBy rdf:resource="https://www.theworldavatar.com/kg/ontopoi"/>
        <rdfs:label>Sports and leisure equipment repair</rdfs:label>
    </owl:Class>
    


    <!-- https://www.theworldavatar.com/kg/ontopoi/Sportsclubsandassociations -->


    <owl:Class rdf:about="https://www.theworldavatar.com/kg/ontopoi/Sportsclubsandassociations">
        <rdfs:subClassOf rdf:resource="https://www.theworldavatar.com/kg/ontopoi/Organisations"/>
        <rdfs:comment>Sports clubs and associations is a subcategory of organisations</rdfs:comment>
        <rdfs:isDefinedBy rdf:resource="https://www.theworldavatar.com/kg/ontopoi"/>
        <rdfs:label>Sports clubs and associations</rdfs:label>
    </owl:Class>
    


    <!-- https://www.theworldavatar.com/kg/ontopoi/Sportscomplex -->


    <owl:Class rdf:about="https://www.theworldavatar.com/kg/ontopoi/Sportscomplex">
        <rdfs:subClassOf rdf:resource="https://www.theworldavatar.com/kg/ontopoi/Sportandentertainment"/>
        <rdfs:comment>Sports complex is a subcategory of sport and entertainment</rdfs:comment>
        <rdfs:isDefinedBy rdf:resource="https://www.theworldavatar.com/kg/ontopoi"/>
        <rdfs:label>Sports complex</rdfs:label>
    </owl:Class>
    


    <!-- https://www.theworldavatar.com/kg/ontopoi/Sportsgroundsandstadiaandpitches -->


    <owl:Class rdf:about="https://www.theworldavatar.com/kg/ontopoi/Sportsgroundsandstadiaandpitches">
        <rdfs:subClassOf rdf:resource="https://www.theworldavatar.com/kg/ontopoi/Sportscomplex"/>
        <rdfs:comment>Sports grounds, stadia and pitches is a subcategory of sports complex</rdfs:comment>
        <rdfs:isDefinedBy rdf:resource="https://www.theworldavatar.com/kg/ontopoi"/>
        <rdfs:label>Sports grounds, stadia and pitches</rdfs:label>
    </owl:Class>
    


    <!-- https://www.theworldavatar.com/kg/ontopoi/Sportsservices -->


    <owl:Class rdf:about="https://www.theworldavatar.com/kg/ontopoi/Sportsservices">
        <rdfs:subClassOf rdf:resource="https://www.theworldavatar.com/kg/ontopoi/Personalandconsumerandotherservices"/>
        <rdfs:comment>Sports services is a subcategory of personal, consumer and other services</rdfs:comment>
        <rdfs:isDefinedBy rdf:resource="https://www.theworldavatar.com/kg/ontopoi"/>
        <rdfs:label>Sports services</rdfs:label>
    </owl:Class>
    


    <!-- https://www.theworldavatar.com/kg/ontopoi/Squashcourts -->


    <owl:Class rdf:about="https://www.theworldavatar.com/kg/ontopoi/Squashcourts">
        <rdfs:subClassOf rdf:resource="https://www.theworldavatar.com/kg/ontopoi/Sportscomplex"/>
        <rdfs:comment>Squash courts is a subcategory of sports complex</rdfs:comment>
        <rdfs:isDefinedBy rdf:resource="https://www.theworldavatar.com/kg/ontopoi"/>
        <rdfs:label>Squash courts</rdfs:label>
    </owl:Class>
    


    <!-- https://www.theworldavatar.com/kg/ontopoi/Stationeryandofficesupplies -->


    <owl:Class rdf:about="https://www.theworldavatar.com/kg/ontopoi/Stationeryandofficesupplies">
        <rdfs:subClassOf rdf:resource="https://www.theworldavatar.com/kg/ontopoi/Householdandofficeandleisureandgarden"/>
        <rdfs:comment>Stationery and office supplies is a subcategory of household, office, leisure and garden</rdfs:comment>
        <rdfs:isDefinedBy rdf:resource="https://www.theworldavatar.com/kg/ontopoi"/>
        <rdfs:label>Stationery and office supplies</rdfs:label>
    </owl:Class>
    


    <!-- https://www.theworldavatar.com/kg/ontopoi/Stationeryandstampsandtagsandlabels -->


    <owl:Class rdf:about="https://www.theworldavatar.com/kg/ontopoi/Stationeryandstampsandtagsandlabels">
        <rdfs:subClassOf rdf:resource="https://www.theworldavatar.com/kg/ontopoi/Industrialproducts"/>
        <rdfs:comment>Stationery, stamps, tags and labels is a subcategory of industrial products</rdfs:comment>
        <rdfs:isDefinedBy rdf:resource="https://www.theworldavatar.com/kg/ontopoi"/>
        <rdfs:label>Stationery, stamps, tags and labels</rdfs:label>
    </owl:Class>
    


    <!-- https://www.theworldavatar.com/kg/ontopoi/Stocksandsharesandunittrusts -->


    <owl:Class rdf:about="https://www.theworldavatar.com/kg/ontopoi/Stocksandsharesandunittrusts">
        <rdfs:subClassOf rdf:resource="https://www.theworldavatar.com/kg/ontopoi/Legalandfinancial"/>
        <rdfs:comment>Stocks, shares and unit trusts is a subcategory of legal and financial</rdfs:comment>
        <rdfs:isDefinedBy rdf:resource="https://www.theworldavatar.com/kg/ontopoi"/>
        <rdfs:label>Stocks, shares and unit trusts</rdfs:label>
    </owl:Class>
    


    <!-- https://www.theworldavatar.com/kg/ontopoi/Stonequarryingandpreparation -->


    <owl:Class rdf:about="https://www.theworldavatar.com/kg/ontopoi/Stonequarryingandpreparation">
        <rdfs:subClassOf rdf:resource="https://www.theworldavatar.com/kg/ontopoi/Extractiveindustries"/>
        <rdfs:comment>Stone quarrying and preparation is a subcategory of extractive industries</rdfs:comment>
        <rdfs:isDefinedBy rdf:resource="https://www.theworldavatar.com/kg/ontopoi"/>
        <rdfs:label>Stone quarrying and preparation</rdfs:label>
    </owl:Class>
    


    <!-- https://www.theworldavatar.com/kg/ontopoi/Structuralengineers -->


    <owl:Class rdf:about="https://www.theworldavatar.com/kg/ontopoi/Structuralengineers">
        <rdfs:subClassOf rdf:resource="https://www.theworldavatar.com/kg/ontopoi/Engineeringservices"/>
        <rdfs:comment>Structural engineers is a subcategory of engineering services</rdfs:comment>
        <rdfs:isDefinedBy rdf:resource="https://www.theworldavatar.com/kg/ontopoi"/>
        <rdfs:label>Structural engineers</rdfs:label>
    </owl:Class>
    


    <!-- https://www.theworldavatar.com/kg/ontopoi/Supermarketchains -->


    <owl:Class rdf:about="https://www.theworldavatar.com/kg/ontopoi/Supermarketchains">
        <rdfs:subClassOf rdf:resource="https://www.theworldavatar.com/kg/ontopoi/Foodanddrinkandmultiitemretail"/>
        <rdfs:comment>Supermarket chains is a subcategory of food, drink and multi item retail</rdfs:comment>
        <rdfs:isDefinedBy rdf:resource="https://www.theworldavatar.com/kg/ontopoi"/>
        <rdfs:label>Supermarket chains</rdfs:label>
    </owl:Class>
    


    <!-- https://www.theworldavatar.com/kg/ontopoi/Surgeonsandcosmeticsurgeries -->


    <owl:Class rdf:about="https://www.theworldavatar.com/kg/ontopoi/Surgeonsandcosmeticsurgeries">
        <rdfs:subClassOf rdf:resource="https://www.theworldavatar.com/kg/ontopoi/Healthpractitionersandestablishments"/>
        <rdfs:comment>Surgeons and cosmetic surgeries is a subcategory of health practitioners and establishments</rdfs:comment>
        <rdfs:isDefinedBy rdf:resource="https://www.theworldavatar.com/kg/ontopoi"/>
        <rdfs:label>Surgeons and cosmetic surgeries</rdfs:label>
    </owl:Class>
    


    <!-- https://www.theworldavatar.com/kg/ontopoi/Surplusgoods -->


    <owl:Class rdf:about="https://www.theworldavatar.com/kg/ontopoi/Surplusgoods">
        <rdfs:subClassOf rdf:resource="https://www.theworldavatar.com/kg/ontopoi/Householdandofficeandleisureandgarden"/>
        <rdfs:comment>Surplus goods is a subcategory of household, office, leisure and garden</rdfs:comment>
        <rdfs:isDefinedBy rdf:resource="https://www.theworldavatar.com/kg/ontopoi"/>
        <rdfs:label>Surplus goods</rdfs:label>
    </owl:Class>
    


    <!-- https://www.theworldavatar.com/kg/ontopoi/Swimmingpools -->


    <owl:Class rdf:about="https://www.theworldavatar.com/kg/ontopoi/Swimmingpools">
        <rdfs:subClassOf rdf:resource="https://www.theworldavatar.com/kg/ontopoi/Sportscomplex"/>
        <rdfs:comment>Swimming pools is a subcategory of sports complex</rdfs:comment>
        <rdfs:isDefinedBy rdf:resource="https://www.theworldavatar.com/kg/ontopoi"/>
        <rdfs:label>Swimming pools</rdfs:label>
    </owl:Class>
    


    <!-- https://www.theworldavatar.com/kg/ontopoi/Tailoringandclothingalteration -->


    <owl:Class rdf:about="https://www.theworldavatar.com/kg/ontopoi/Tailoringandclothingalteration">
        <rdfs:subClassOf rdf:resource="https://www.theworldavatar.com/kg/ontopoi/Personalandconsumerandotherservices"/>
        <rdfs:comment>Tailoring and clothing alteration is a subcategory of personal, consumer and other services</rdfs:comment>
        <rdfs:isDefinedBy rdf:resource="https://www.theworldavatar.com/kg/ontopoi"/>
        <rdfs:label>Tailoring and clothing alteration</rdfs:label>
    </owl:Class>
    


    <!-- https://www.theworldavatar.com/kg/ontopoi/Tarnsandpoolsandmeres -->


    <owl:Class rdf:about="https://www.theworldavatar.com/kg/ontopoi/Tarnsandpoolsandmeres">
        <rdfs:subClassOf rdf:resource="https://www.theworldavatar.com/kg/ontopoi/Bodiesofwater"/>
        <rdfs:comment>Tarns, pools and meres is a subcategory of bodies of water</rdfs:comment>
        <rdfs:isDefinedBy rdf:resource="https://www.theworldavatar.com/kg/ontopoi"/>
        <rdfs:label>Tarns, pools and meres</rdfs:label>
    </owl:Class>
    


    <!-- https://www.theworldavatar.com/kg/ontopoi/Tattooingandpiercingservices -->


    <owl:Class rdf:about="https://www.theworldavatar.com/kg/ontopoi/Tattooingandpiercingservices">
        <rdfs:subClassOf rdf:resource="https://www.theworldavatar.com/kg/ontopoi/Personalandconsumerandotherservices"/>
        <rdfs:comment>Tattooing and piercing services is a subcategory of personal, consumer and other services</rdfs:comment>
        <rdfs:isDefinedBy rdf:resource="https://www.theworldavatar.com/kg/ontopoi"/>
        <rdfs:label>Tattooing and piercing services</rdfs:label>
    </owl:Class>
    


    <!-- https://www.theworldavatar.com/kg/ontopoi/Taxiranks -->


    <owl:Class rdf:about="https://www.theworldavatar.com/kg/ontopoi/Taxiranks">
        <rdfs:subClassOf rdf:resource="https://www.theworldavatar.com/kg/ontopoi/Publictransportandstationsandinfrastructure"/>
        <rdfs:comment>Taxi ranks is a subcategory of public transport, stations and infrastructure</rdfs:comment>
        <rdfs:isDefinedBy rdf:resource="https://www.theworldavatar.com/kg/ontopoi"/>
        <rdfs:label>Taxi ranks</rdfs:label>
    </owl:Class>
    


    <!-- https://www.theworldavatar.com/kg/ontopoi/Taxiservices -->


    <owl:Class rdf:about="https://www.theworldavatar.com/kg/ontopoi/Taxiservices">
        <rdfs:subClassOf rdf:resource="https://www.theworldavatar.com/kg/ontopoi/Transportandstorageanddelivery"/>
        <rdfs:comment>Taxi services is a subcategory of transport, storage and delivery</rdfs:comment>
        <rdfs:isDefinedBy rdf:resource="https://www.theworldavatar.com/kg/ontopoi"/>
        <rdfs:label>Taxi services</rdfs:label>
    </owl:Class>
    


    <!-- https://www.theworldavatar.com/kg/ontopoi/Teaandcoffeemerchants -->


    <owl:Class rdf:about="https://www.theworldavatar.com/kg/ontopoi/Teaandcoffeemerchants">
        <rdfs:subClassOf rdf:resource="https://www.theworldavatar.com/kg/ontopoi/Foodanddrinkandmultiitemretail"/>
        <rdfs:comment>Tea and coffee merchants is a subcategory of food, drink and multi item retail</rdfs:comment>
        <rdfs:isDefinedBy rdf:resource="https://www.theworldavatar.com/kg/ontopoi"/>
        <rdfs:label>Tea and coffee merchants</rdfs:label>
    </owl:Class>
    


    <!-- https://www.theworldavatar.com/kg/ontopoi/Telecommunicationscompanies -->


    <owl:Class rdf:about="https://www.theworldavatar.com/kg/ontopoi/Telecommunicationscompanies">
        <rdfs:subClassOf rdf:resource="https://www.theworldavatar.com/kg/ontopoi/Infrastructureandfacilities"/>
        <rdfs:comment>Telecommunications companies is a subcategory of infrastructure and facilities</rdfs:comment>
        <rdfs:isDefinedBy rdf:resource="https://www.theworldavatar.com/kg/ontopoi"/>
        <rdfs:label>Telecommunications companies</rdfs:label>
    </owl:Class>
    


    <!-- https://www.theworldavatar.com/kg/ontopoi/Telecommunicationsconsultants -->


    <owl:Class rdf:about="https://www.theworldavatar.com/kg/ontopoi/Telecommunicationsconsultants">
        <rdfs:subClassOf rdf:resource="https://www.theworldavatar.com/kg/ontopoi/Consultancies"/>
        <rdfs:comment>Telecommunications consultants is a subcategory of consultancies</rdfs:comment>
        <rdfs:isDefinedBy rdf:resource="https://www.theworldavatar.com/kg/ontopoi"/>
        <rdfs:label>Telecommunications consultants</rdfs:label>
    </owl:Class>
    


    <!-- https://www.theworldavatar.com/kg/ontopoi/Telecommunicationsfeatures -->


    <owl:Class rdf:about="https://www.theworldavatar.com/kg/ontopoi/Telecommunicationsfeatures">
        <rdfs:subClassOf rdf:resource="https://www.theworldavatar.com/kg/ontopoi/Infrastructureandfacilities"/>
        <rdfs:comment>Telecommunications features is a subcategory of infrastructure and facilities</rdfs:comment>
        <rdfs:isDefinedBy rdf:resource="https://www.theworldavatar.com/kg/ontopoi"/>
        <rdfs:label>Telecommunications features</rdfs:label>
    </owl:Class>
    


    <!-- https://www.theworldavatar.com/kg/ontopoi/Telephoneandtelexandfaxservices -->


    <owl:Class rdf:about="https://www.theworldavatar.com/kg/ontopoi/Telephoneandtelexandfaxservices">
        <rdfs:subClassOf rdf:resource="https://www.theworldavatar.com/kg/ontopoi/ITandadvertisingandmarketingandmediaservices"/>
        <rdfs:comment>Telephone, telex and fax services is a subcategory of it, advertising, marketing and media service s</rdfs:comment>
        <rdfs:isDefinedBy rdf:resource="https://www.theworldavatar.com/kg/ontopoi"/>
        <rdfs:label>Telephone, telex and fax services</rdfs:label>
    </owl:Class>
    


    <!-- https://www.theworldavatar.com/kg/ontopoi/Telephonesandtelephonecards -->


    <owl:Class rdf:about="https://www.theworldavatar.com/kg/ontopoi/Telephonesandtelephonecards">
        <rdfs:subClassOf rdf:resource="https://www.theworldavatar.com/kg/ontopoi/Householdandofficeandleisureandgarden"/>
        <rdfs:comment>Telephones and telephone cards is a subcategory of household, office, leisure and garden</rdfs:comment>
        <rdfs:isDefinedBy rdf:resource="https://www.theworldavatar.com/kg/ontopoi"/>
        <rdfs:label>Telephones and telephone cards</rdfs:label>
    </owl:Class>
    


    <!-- https://www.theworldavatar.com/kg/ontopoi/Televisionandradioservices -->


    <owl:Class rdf:about="https://www.theworldavatar.com/kg/ontopoi/Televisionandradioservices">
        <rdfs:subClassOf rdf:resource="https://www.theworldavatar.com/kg/ontopoi/ITandadvertisingandmarketingandmediaservices"/>
        <rdfs:comment>Television and radio services is a subcategory of it, advertising, marketing and media service s</rdfs:comment>
        <rdfs:isDefinedBy rdf:resource="https://www.theworldavatar.com/kg/ontopoi"/>
        <rdfs:label>Television and radio services</rdfs:label>
    </owl:Class>
    


    <!-- https://www.theworldavatar.com/kg/ontopoi/Tennisfacilities -->


    <owl:Class rdf:about="https://www.theworldavatar.com/kg/ontopoi/Tennisfacilities">
        <rdfs:subClassOf rdf:resource="https://www.theworldavatar.com/kg/ontopoi/Sportscomplex"/>
        <rdfs:comment>Tennis facilities is a subcategory of sports complex</rdfs:comment>
        <rdfs:isDefinedBy rdf:resource="https://www.theworldavatar.com/kg/ontopoi"/>
        <rdfs:label>Tennis facilities</rdfs:label>
    </owl:Class>
    


    <!-- https://www.theworldavatar.com/kg/ontopoi/Tentsandmarqueesandcampingequipment -->


    <owl:Class rdf:about="https://www.theworldavatar.com/kg/ontopoi/Tentsandmarqueesandcampingequipment">
        <rdfs:subClassOf rdf:resource="https://www.theworldavatar.com/kg/ontopoi/Consumerproducts"/>
        <rdfs:comment>Tents, marquees and camping equipment is a subcategory of consumer products</rdfs:comment>
        <rdfs:isDefinedBy rdf:resource="https://www.theworldavatar.com/kg/ontopoi"/>
        <rdfs:label>Tents, marquees and camping equipment</rdfs:label>
    </owl:Class>
    


    <!-- https://www.theworldavatar.com/kg/ontopoi/Testingandanalysisservices -->


    <owl:Class rdf:about="https://www.theworldavatar.com/kg/ontopoi/Testingandanalysisservices">
        <rdfs:subClassOf rdf:resource="https://www.theworldavatar.com/kg/ontopoi/Researchanddesign"/>
        <rdfs:comment>Testing and analysis services is a subcategory of research and design</rdfs:comment>
        <rdfs:isDefinedBy rdf:resource="https://www.theworldavatar.com/kg/ontopoi"/>
        <rdfs:label>Testing and analysis services</rdfs:label>
    </owl:Class>
    


    <!-- https://www.theworldavatar.com/kg/ontopoi/Textilesandfabricsandsilkandmachinery -->


    <owl:Class rdf:about="https://www.theworldavatar.com/kg/ontopoi/Textilesandfabricsandsilkandmachinery">
        <rdfs:subClassOf rdf:resource="https://www.theworldavatar.com/kg/ontopoi/Industrialproducts"/>
        <rdfs:comment>Textiles, fabrics, silk and machinery is a subcategory of industrial products</rdfs:comment>
        <rdfs:isDefinedBy rdf:resource="https://www.theworldavatar.com/kg/ontopoi"/>
        <rdfs:label>Textiles, fabrics, silk and machinery</rdfs:label>
    </owl:Class>
    


    <!-- https://www.theworldavatar.com/kg/ontopoi/Theatresandconcerthalls -->


    <owl:Class rdf:about="https://www.theworldavatar.com/kg/ontopoi/Theatresandconcerthalls">
        <rdfs:subClassOf rdf:resource="https://www.theworldavatar.com/kg/ontopoi/Venuesandstageandscreen"/>
        <rdfs:comment>Theatres and concert halls is a subcategory of venues, stage and screen</rdfs:comment>
        <rdfs:isDefinedBy rdf:resource="https://www.theworldavatar.com/kg/ontopoi"/>
        <rdfs:label>Theatres and concert halls</rdfs:label>
    </owl:Class>
    


    <!-- https://www.theworldavatar.com/kg/ontopoi/Themeandadventureparks -->


    <owl:Class rdf:about="https://www.theworldavatar.com/kg/ontopoi/Themeandadventureparks">
        <rdfs:subClassOf rdf:resource="https://www.theworldavatar.com/kg/ontopoi/Tourism"/>
        <rdfs:comment>Theme and adventure parks is a subcategory of tourism</rdfs:comment>
        <rdfs:isDefinedBy rdf:resource="https://www.theworldavatar.com/kg/ontopoi"/>
        <rdfs:label>Theme and adventure parks</rdfs:label>
    </owl:Class>
    


    <!-- https://www.theworldavatar.com/kg/ontopoi/Timeshare -->


    <owl:Class rdf:about="https://www.theworldavatar.com/kg/ontopoi/Timeshare">
        <rdfs:subClassOf rdf:resource="https://www.theworldavatar.com/kg/ontopoi/Accommodation"/>
        <rdfs:comment>Timeshare is a subcategory of accommodation</rdfs:comment>
        <rdfs:isDefinedBy rdf:resource="https://www.theworldavatar.com/kg/ontopoi"/>
        <rdfs:label>Timeshare</rdfs:label>
    </owl:Class>
    


    <!-- https://www.theworldavatar.com/kg/ontopoi/Tobaccoproducts -->


    <owl:Class rdf:about="https://www.theworldavatar.com/kg/ontopoi/Tobaccoproducts">
        <rdfs:subClassOf rdf:resource="https://www.theworldavatar.com/kg/ontopoi/Consumerproducts"/>
        <rdfs:comment>Tobacco products is a subcategory of consumer products</rdfs:comment>
        <rdfs:isDefinedBy rdf:resource="https://www.theworldavatar.com/kg/ontopoi"/>
        <rdfs:label>Tobacco products</rdfs:label>
    </owl:Class>
    


    <!-- https://www.theworldavatar.com/kg/ontopoi/Toolrepairs -->


    <owl:Class rdf:about="https://www.theworldavatar.com/kg/ontopoi/Toolrepairs">
        <rdfs:subClassOf rdf:resource="https://www.theworldavatar.com/kg/ontopoi/Repairandservicing"/>
        <rdfs:comment>Tool repairs is a subcategory of repair and servicing</rdfs:comment>
        <rdfs:isDefinedBy rdf:resource="https://www.theworldavatar.com/kg/ontopoi"/>
        <rdfs:label>Tool repairs</rdfs:label>
    </owl:Class>
    


    <!-- https://www.theworldavatar.com/kg/ontopoi/Toolsincludingmachineshops -->


    <owl:Class rdf:about="https://www.theworldavatar.com/kg/ontopoi/Toolsincludingmachineshops">
        <rdfs:subClassOf rdf:resource="https://www.theworldavatar.com/kg/ontopoi/Industrialproducts"/>
        <rdfs:comment>Tools including machine shops is a subcategory of industrial products</rdfs:comment>
        <rdfs:isDefinedBy rdf:resource="https://www.theworldavatar.com/kg/ontopoi"/>
        <rdfs:label>Tools including machine shops</rdfs:label>
    </owl:Class>
    


    <!-- https://www.theworldavatar.com/kg/ontopoi/Tourism -->


    <owl:Class rdf:about="https://www.theworldavatar.com/kg/ontopoi/Tourism">
        <rdfs:subClassOf rdf:resource="https://www.theworldavatar.com/kg/ontopoi/Attractions"/>
        <rdfs:comment>Tourism is a subcategory of attractions</rdfs:comment>
        <rdfs:isDefinedBy rdf:resource="https://www.theworldavatar.com/kg/ontopoi"/>
        <rdfs:label>Tourism</rdfs:label>
    </owl:Class>
    


    <!-- https://www.theworldavatar.com/kg/ontopoi/Trafficmanagementandtransport-relatedconsultants -->


    <owl:Class rdf:about="https://www.theworldavatar.com/kg/ontopoi/Trafficmanagementandtransport-relatedconsultants">
        <rdfs:subClassOf rdf:resource="https://www.theworldavatar.com/kg/ontopoi/Consultancies"/>
        <rdfs:comment>Traffic management and transport-related consultants is a subcategory of consultancies</rdfs:comment>
        <rdfs:isDefinedBy rdf:resource="https://www.theworldavatar.com/kg/ontopoi"/>
        <rdfs:label>Traffic management and transport-related consultants</rdfs:label>
    </owl:Class>
    


    <!-- https://www.theworldavatar.com/kg/ontopoi/Trainingprovidersandcentres -->


    <owl:Class rdf:about="https://www.theworldavatar.com/kg/ontopoi/Trainingprovidersandcentres">
        <rdfs:subClassOf rdf:resource="https://www.theworldavatar.com/kg/ontopoi/Recreationalandvocationaleducation"/>
        <rdfs:comment>Training providers and centres is a subcategory of recreational and vocational education</rdfs:comment>
        <rdfs:isDefinedBy rdf:resource="https://www.theworldavatar.com/kg/ontopoi"/>
        <rdfs:label>Training providers and centres</rdfs:label>
    </owl:Class>
    


    <!-- https://www.theworldavatar.com/kg/ontopoi/Tramandmetroandlightrailwaystationsandstops -->


    <owl:Class rdf:about="https://www.theworldavatar.com/kg/ontopoi/Tramandmetroandlightrailwaystationsandstops">
        <rdfs:subClassOf rdf:resource="https://www.theworldavatar.com/kg/ontopoi/Publictransportandstationsandinfrastructure"/>
        <rdfs:comment>Tram, metro and light railway stations and stops is a subcategory of public transport, stations and infrastructure</rdfs:comment>
        <rdfs:isDefinedBy rdf:resource="https://www.theworldavatar.com/kg/ontopoi"/>
        <rdfs:label>Tram, metro and light railway stations and stops</rdfs:label>
    </owl:Class>
    


    <!-- https://www.theworldavatar.com/kg/ontopoi/Transport -->


    <owl:Class rdf:about="https://www.theworldavatar.com/kg/ontopoi/Transport"/>
    


    <!-- https://www.theworldavatar.com/kg/ontopoi/Transportandstorageanddelivery -->


    <owl:Class rdf:about="https://www.theworldavatar.com/kg/ontopoi/Transportandstorageanddelivery">
        <rdfs:subClassOf rdf:resource="https://www.theworldavatar.com/kg/ontopoi/Commercialservices"/>
        <rdfs:comment>Transport, storage and delivery is a subcategory of commercial services</rdfs:comment>
        <rdfs:isDefinedBy rdf:resource="https://www.theworldavatar.com/kg/ontopoi"/>
        <rdfs:label>Transport, storage and delivery</rdfs:label>
    </owl:Class>
    


    <!-- https://www.theworldavatar.com/kg/ontopoi/Travelagencies -->


    <owl:Class rdf:about="https://www.theworldavatar.com/kg/ontopoi/Travelagencies">
        <rdfs:subClassOf rdf:resource="https://www.theworldavatar.com/kg/ontopoi/Householdandofficeandleisureandgarden"/>
        <rdfs:comment>Travel agencies is a subcategory of household, office, leisure and garden</rdfs:comment>
        <rdfs:isDefinedBy rdf:resource="https://www.theworldavatar.com/kg/ontopoi"/>
        <rdfs:label>Travel agencies</rdfs:label>
    </owl:Class>
    


    <!-- https://www.theworldavatar.com/kg/ontopoi/Tribunals -->


    <owl:Class rdf:about="https://www.theworldavatar.com/kg/ontopoi/Tribunals">
        <rdfs:subClassOf rdf:resource="https://www.theworldavatar.com/kg/ontopoi/Centralandlocalgovernment"/>
        <rdfs:comment>Tribunals is a subcategory of central and local government</rdfs:comment>
        <rdfs:isDefinedBy rdf:resource="https://www.theworldavatar.com/kg/ontopoi"/>
        <rdfs:label>Tribunals</rdfs:label>
    </owl:Class>
    


    <!-- https://www.theworldavatar.com/kg/ontopoi/Trigonometricpoints -->


    <owl:Class rdf:about="https://www.theworldavatar.com/kg/ontopoi/Trigonometricpoints">
        <rdfs:subClassOf rdf:resource="https://www.theworldavatar.com/kg/ontopoi/Landscapefeatures"/>
        <rdfs:comment>Trigonometric points is a subcategory of landscape features</rdfs:comment>
        <rdfs:isDefinedBy rdf:resource="https://www.theworldavatar.com/kg/ontopoi"/>
        <rdfs:label>Trigonometric points</rdfs:label>
    </owl:Class>
    


    <!-- https://www.theworldavatar.com/kg/ontopoi/Trophiesandengravingservices -->


    <owl:Class rdf:about="https://www.theworldavatar.com/kg/ontopoi/Trophiesandengravingservices">
        <rdfs:subClassOf rdf:resource="https://www.theworldavatar.com/kg/ontopoi/Personalandconsumerandotherservices"/>
        <rdfs:comment>Trophies and engraving services is a subcategory of personal, consumer and other services</rdfs:comment>
        <rdfs:isDefinedBy rdf:resource="https://www.theworldavatar.com/kg/ontopoi"/>
        <rdfs:label>Trophies and engraving services</rdfs:label>
    </owl:Class>
    


    <!-- https://www.theworldavatar.com/kg/ontopoi/Undergroundnetworkstations -->


    <owl:Class rdf:about="https://www.theworldavatar.com/kg/ontopoi/Undergroundnetworkstations">
        <rdfs:subClassOf rdf:resource="https://www.theworldavatar.com/kg/ontopoi/Publictransportandstationsandinfrastructure"/>
        <rdfs:comment>Underground network stations is a subcategory of public transport, stations and infrastructure</rdfs:comment>
        <rdfs:isDefinedBy rdf:resource="https://www.theworldavatar.com/kg/ontopoi"/>
        <rdfs:label>Underground network stations</rdfs:label>
    </owl:Class>
    


    <!-- https://www.theworldavatar.com/kg/ontopoi/Unspecifiedandotherattractions -->


    <owl:Class rdf:about="https://www.theworldavatar.com/kg/ontopoi/Unspecifiedandotherattractions">
        <rdfs:subClassOf rdf:resource="https://www.theworldavatar.com/kg/ontopoi/Tourism"/>
        <rdfs:comment>Unspecified and other attractions is a subcategory of tourism</rdfs:comment>
        <rdfs:isDefinedBy rdf:resource="https://www.theworldavatar.com/kg/ontopoi"/>
        <rdfs:label>Unspecified and other attractions</rdfs:label>
    </owl:Class>
    


    <!-- https://www.theworldavatar.com/kg/ontopoi/Unspecifiedandotherschools -->


    <owl:Class rdf:about="https://www.theworldavatar.com/kg/ontopoi/Unspecifiedandotherschools">
        <rdfs:subClassOf rdf:resource="https://www.theworldavatar.com/kg/ontopoi/Primaryandsecondaryandtertiaryeducation"/>
        <rdfs:comment>Unspecified and other schools is a subcategory of primary, secondary and tertiary education</rdfs:comment>
        <rdfs:isDefinedBy rdf:resource="https://www.theworldavatar.com/kg/ontopoi"/>
        <rdfs:label>Unspecified and other schools</rdfs:label>
    </owl:Class>
    


    <!-- https://www.theworldavatar.com/kg/ontopoi/Unspecifiedquarriesormines -->


    <owl:Class rdf:about="https://www.theworldavatar.com/kg/ontopoi/Unspecifiedquarriesormines">
        <rdfs:subClassOf rdf:resource="https://www.theworldavatar.com/kg/ontopoi/Extractiveindustries"/>
        <rdfs:comment>Unspecified quarries or mines is a subcategory of extractive industries</rdfs:comment>
        <rdfs:isDefinedBy rdf:resource="https://www.theworldavatar.com/kg/ontopoi"/>
        <rdfs:label>Unspecified quarries or mines</rdfs:label>
    </owl:Class>
    


    <!-- https://www.theworldavatar.com/kg/ontopoi/Unspecifiedworksorfactories -->


    <owl:Class rdf:about="https://www.theworldavatar.com/kg/ontopoi/Unspecifiedworksorfactories">
        <rdfs:subClassOf rdf:resource="https://www.theworldavatar.com/kg/ontopoi/Industrialfeatures"/>
        <rdfs:comment>Unspecified works or factories is a subcategory of industrial features</rdfs:comment>
        <rdfs:isDefinedBy rdf:resource="https://www.theworldavatar.com/kg/ontopoi"/>
        <rdfs:label>Unspecified works or factories</rdfs:label>
    </owl:Class>
    


    <!-- https://www.theworldavatar.com/kg/ontopoi/Utilitycompaniesandbrokers -->


    <owl:Class rdf:about="https://www.theworldavatar.com/kg/ontopoi/Utilitycompaniesandbrokers">
        <rdfs:subClassOf rdf:resource="https://www.theworldavatar.com/kg/ontopoi/Infrastructureandfacilities"/>
        <rdfs:comment>Utility companies and brokers is a subcategory of infrastructure and facilities</rdfs:comment>
        <rdfs:isDefinedBy rdf:resource="https://www.theworldavatar.com/kg/ontopoi"/>
        <rdfs:label>Utility companies and brokers</rdfs:label>
    </owl:Class>
    


    <!-- https://www.theworldavatar.com/kg/ontopoi/Vehicleauctions -->


    <owl:Class rdf:about="https://www.theworldavatar.com/kg/ontopoi/Vehicleauctions">
        <rdfs:subClassOf rdf:resource="https://www.theworldavatar.com/kg/ontopoi/Motoring"/>
        <rdfs:comment>Vehicle auctions is a subcategory of motoring</rdfs:comment>
        <rdfs:isDefinedBy rdf:resource="https://www.theworldavatar.com/kg/ontopoi"/>
        <rdfs:label>Vehicle auctions</rdfs:label>
    </owl:Class>
    


    <!-- https://www.theworldavatar.com/kg/ontopoi/Vehiclebodybuilders -->


    <owl:Class rdf:about="https://www.theworldavatar.com/kg/ontopoi/Vehiclebodybuilders">
        <rdfs:subClassOf rdf:resource="https://www.theworldavatar.com/kg/ontopoi/Industrialproducts"/>
        <rdfs:comment>Vehicle bodybuilders is a subcategory of industrial products</rdfs:comment>
        <rdfs:isDefinedBy rdf:resource="https://www.theworldavatar.com/kg/ontopoi"/>
        <rdfs:label>Vehicle bodybuilders</rdfs:label>
    </owl:Class>
    


    <!-- https://www.theworldavatar.com/kg/ontopoi/Vehiclebreakdownandrecoveryservices -->


    <owl:Class rdf:about="https://www.theworldavatar.com/kg/ontopoi/Vehiclebreakdownandrecoveryservices">
        <rdfs:subClassOf rdf:resource="https://www.theworldavatar.com/kg/ontopoi/Personalandconsumerandotherservices"/>
        <rdfs:comment>Vehicle breakdown and recovery services is a subcategory of personal, consumer and other services</rdfs:comment>
        <rdfs:isDefinedBy rdf:resource="https://www.theworldavatar.com/kg/ontopoi"/>
        <rdfs:label>Vehicle breakdown and recovery services</rdfs:label>
    </owl:Class>
    


    <!-- https://www.theworldavatar.com/kg/ontopoi/Vehiclecleaningservices -->


    <owl:Class rdf:about="https://www.theworldavatar.com/kg/ontopoi/Vehiclecleaningservices">
        <rdfs:subClassOf rdf:resource="https://www.theworldavatar.com/kg/ontopoi/Personalandconsumerandotherservices"/>
        <rdfs:comment>Vehicle cleaning services is a subcategory of personal, consumer and other services</rdfs:comment>
        <rdfs:isDefinedBy rdf:resource="https://www.theworldavatar.com/kg/ontopoi"/>
        <rdfs:label>Vehicle cleaning services</rdfs:label>
    </owl:Class>
    


    <!-- https://www.theworldavatar.com/kg/ontopoi/Vehiclecomponents -->


    <owl:Class rdf:about="https://www.theworldavatar.com/kg/ontopoi/Vehiclecomponents">
        <rdfs:subClassOf rdf:resource="https://www.theworldavatar.com/kg/ontopoi/Industrialproducts"/>
        <rdfs:comment>Vehicle components is a subcategory of industrial products</rdfs:comment>
        <rdfs:isDefinedBy rdf:resource="https://www.theworldavatar.com/kg/ontopoi"/>
        <rdfs:label>Vehicle components</rdfs:label>
    </owl:Class>
    


    <!-- https://www.theworldavatar.com/kg/ontopoi/Vehiclehireandrental -->


    <owl:Class rdf:about="https://www.theworldavatar.com/kg/ontopoi/Vehiclehireandrental">
        <rdfs:subClassOf rdf:resource="https://www.theworldavatar.com/kg/ontopoi/Hireservices"/>
        <rdfs:comment>Vehicle hire and rental is a subcategory of hire services</rdfs:comment>
        <rdfs:isDefinedBy rdf:resource="https://www.theworldavatar.com/kg/ontopoi"/>
        <rdfs:label>Vehicle hire and rental</rdfs:label>
    </owl:Class>
    


    <!-- https://www.theworldavatar.com/kg/ontopoi/Vehiclepartsandaccessories -->


    <owl:Class rdf:about="https://www.theworldavatar.com/kg/ontopoi/Vehiclepartsandaccessories">
        <rdfs:subClassOf rdf:resource="https://www.theworldavatar.com/kg/ontopoi/Motoring"/>
        <rdfs:comment>Vehicle parts and accessories is a subcategory of motoring</rdfs:comment>
        <rdfs:isDefinedBy rdf:resource="https://www.theworldavatar.com/kg/ontopoi"/>
        <rdfs:label>Vehicle parts and accessories</rdfs:label>
    </owl:Class>
    


    <!-- https://www.theworldavatar.com/kg/ontopoi/Vehiclerepairandtestingandservicing -->


    <owl:Class rdf:about="https://www.theworldavatar.com/kg/ontopoi/Vehiclerepairandtestingandservicing">
        <rdfs:subClassOf rdf:resource="https://www.theworldavatar.com/kg/ontopoi/Repairandservicing"/>
        <rdfs:comment>Vehicle repair, testing and servicing is a subcategory of repair and servicing</rdfs:comment>
        <rdfs:isDefinedBy rdf:resource="https://www.theworldavatar.com/kg/ontopoi"/>
        <rdfs:label>Vehicle repair, testing and servicing</rdfs:label>
    </owl:Class>
    


    <!-- https://www.theworldavatar.com/kg/ontopoi/Vehicles -->


    <owl:Class rdf:about="https://www.theworldavatar.com/kg/ontopoi/Vehicles">
        <rdfs:subClassOf rdf:resource="https://www.theworldavatar.com/kg/ontopoi/Industrialproducts"/>
        <rdfs:comment>Vehicles is a subcategory of industrial products</rdfs:comment>
        <rdfs:isDefinedBy rdf:resource="https://www.theworldavatar.com/kg/ontopoi"/>
        <rdfs:label>Vehicles</rdfs:label>
    </owl:Class>
    


    <!-- https://www.theworldavatar.com/kg/ontopoi/Velodromes -->


    <owl:Class rdf:about="https://www.theworldavatar.com/kg/ontopoi/Velodromes">
        <rdfs:subClassOf rdf:resource="https://www.theworldavatar.com/kg/ontopoi/Sportscomplex"/>
        <rdfs:comment>Velodromes is a subcategory of sports complex</rdfs:comment>
        <rdfs:isDefinedBy rdf:resource="https://www.theworldavatar.com/kg/ontopoi"/>
        <rdfs:label>Velodromes</rdfs:label>
    </owl:Class>
    


    <!-- https://www.theworldavatar.com/kg/ontopoi/Venuesandstageandscreen -->


    <owl:Class rdf:about="https://www.theworldavatar.com/kg/ontopoi/Venuesandstageandscreen">
        <rdfs:subClassOf rdf:resource="https://www.theworldavatar.com/kg/ontopoi/Sportandentertainment"/>
        <rdfs:comment>Venues, stage and screen is a subcategory of sport and entertainment</rdfs:comment>
        <rdfs:isDefinedBy rdf:resource="https://www.theworldavatar.com/kg/ontopoi"/>
        <rdfs:label>Venues, stage and screen</rdfs:label>
    </owl:Class>
    


    <!-- https://www.theworldavatar.com/kg/ontopoi/Veterinariansandanimalhospitals -->


    <owl:Class rdf:about="https://www.theworldavatar.com/kg/ontopoi/Veterinariansandanimalhospitals">
        <rdfs:subClassOf rdf:resource="https://www.theworldavatar.com/kg/ontopoi/Animalwelfare"/>
        <rdfs:comment>Veterinarians and animal hospitals is a subcategory of animal welfare</rdfs:comment>
        <rdfs:isDefinedBy rdf:resource="https://www.theworldavatar.com/kg/ontopoi"/>
        <rdfs:label>Veterinarians and animal hospitals</rdfs:label>
    </owl:Class>
    


    <!-- https://www.theworldavatar.com/kg/ontopoi/Veterinarypharmacies -->


    <owl:Class rdf:about="https://www.theworldavatar.com/kg/ontopoi/Veterinarypharmacies">
        <rdfs:subClassOf rdf:resource="https://www.theworldavatar.com/kg/ontopoi/Animalwelfare"/>
        <rdfs:comment>Veterinary pharmacies is a subcategory of animal welfare</rdfs:comment>
        <rdfs:isDefinedBy rdf:resource="https://www.theworldavatar.com/kg/ontopoi"/>
        <rdfs:label>Veterinary pharmacies</rdfs:label>
    </owl:Class>
    


    <!-- https://www.theworldavatar.com/kg/ontopoi/Viaducts -->


    <owl:Class rdf:about="https://www.theworldavatar.com/kg/ontopoi/Viaducts">
        <rdfs:subClassOf rdf:resource="https://www.theworldavatar.com/kg/ontopoi/Roadandrail"/>
        <rdfs:comment>Viaducts is a subcategory of road and rail</rdfs:comment>
        <rdfs:isDefinedBy rdf:resource="https://www.theworldavatar.com/kg/ontopoi"/>
        <rdfs:label>Viaducts</rdfs:label>
    </owl:Class>
    


    <!-- https://www.theworldavatar.com/kg/ontopoi/Walk-incentres -->


    <owl:Class rdf:about="https://www.theworldavatar.com/kg/ontopoi/Walk-incentres">
        <rdfs:subClassOf rdf:resource="https://www.theworldavatar.com/kg/ontopoi/Healthpractitionersandestablishments"/>
        <rdfs:comment>Walk-in centres is a subcategory of health practitioners and establishments</rdfs:comment>
        <rdfs:isDefinedBy rdf:resource="https://www.theworldavatar.com/kg/ontopoi"/>
        <rdfs:label>Walk-in centres</rdfs:label>
    </owl:Class>
    


    <!-- https://www.theworldavatar.com/kg/ontopoi/Walking -->


    <owl:Class rdf:about="https://www.theworldavatar.com/kg/ontopoi/Walking">
        <rdfs:subClassOf rdf:resource="https://www.theworldavatar.com/kg/ontopoi/Transport"/>
        <rdfs:comment>Walking is a subcategory of transport</rdfs:comment>
        <rdfs:isDefinedBy rdf:resource="https://www.theworldavatar.com/kg/ontopoi"/>
        <rdfs:label>Walking</rdfs:label>
    </owl:Class>
    


    <!-- https://www.theworldavatar.com/kg/ontopoi/Wastecollectionandprocessinganddisposalequipment -->


    <owl:Class rdf:about="https://www.theworldavatar.com/kg/ontopoi/Wastecollectionandprocessinganddisposalequipment">
        <rdfs:subClassOf rdf:resource="https://www.theworldavatar.com/kg/ontopoi/Industrialproducts"/>
        <rdfs:comment>Waste collection, processing and disposal equipment is a subcategory of industrial products</rdfs:comment>
        <rdfs:isDefinedBy rdf:resource="https://www.theworldavatar.com/kg/ontopoi"/>
        <rdfs:label>Waste collection, processing and disposal equipment</rdfs:label>
    </owl:Class>
    


    <!-- https://www.theworldavatar.com/kg/ontopoi/Wastepapermerchants -->


    <owl:Class rdf:about="https://www.theworldavatar.com/kg/ontopoi/Wastepapermerchants">
        <rdfs:subClassOf rdf:resource="https://www.theworldavatar.com/kg/ontopoi/Recyclingservices"/>
        <rdfs:comment>Waste paper merchants is a subcategory of recycling services</rdfs:comment>
        <rdfs:isDefinedBy rdf:resource="https://www.theworldavatar.com/kg/ontopoi"/>
        <rdfs:label>Waste paper merchants</rdfs:label>
    </owl:Class>
    


    <!-- https://www.theworldavatar.com/kg/ontopoi/Wastestorageandprocessinganddisposal -->


    <owl:Class rdf:about="https://www.theworldavatar.com/kg/ontopoi/Wastestorageandprocessinganddisposal">
        <rdfs:subClassOf rdf:resource="https://www.theworldavatar.com/kg/ontopoi/Infrastructureandfacilities"/>
        <rdfs:comment>Waste storage, processing and disposal is a subcategory of infrastructure and facilities</rdfs:comment>
        <rdfs:isDefinedBy rdf:resource="https://www.theworldavatar.com/kg/ontopoi"/>
        <rdfs:label>Waste storage, processing and disposal</rdfs:label>
    </owl:Class>
    


    <!-- https://www.theworldavatar.com/kg/ontopoi/Water -->


    <owl:Class rdf:about="https://www.theworldavatar.com/kg/ontopoi/Water">
        <rdfs:subClassOf rdf:resource="https://www.theworldavatar.com/kg/ontopoi/Transport"/>
        <rdfs:comment>Water is a subcategory of transport</rdfs:comment>
        <rdfs:isDefinedBy rdf:resource="https://www.theworldavatar.com/kg/ontopoi"/>
        <rdfs:label>Water</rdfs:label>
    </owl:Class>
    


    <!-- https://www.theworldavatar.com/kg/ontopoi/Waterpumpingstations -->


    <owl:Class rdf:about="https://www.theworldavatar.com/kg/ontopoi/Waterpumpingstations">
        <rdfs:subClassOf rdf:resource="https://www.theworldavatar.com/kg/ontopoi/Industrialfeatures"/>
        <rdfs:comment>Water pumping stations is a subcategory of industrial features</rdfs:comment>
        <rdfs:isDefinedBy rdf:resource="https://www.theworldavatar.com/kg/ontopoi"/>
        <rdfs:label>Water pumping stations</rdfs:label>
    </owl:Class>
    


    <!-- https://www.theworldavatar.com/kg/ontopoi/Watersports -->


    <owl:Class rdf:about="https://www.theworldavatar.com/kg/ontopoi/Watersports">
        <rdfs:subClassOf rdf:resource="https://www.theworldavatar.com/kg/ontopoi/Outdoorpursuits"/>
        <rdfs:comment>Water sports is a subcategory of outdoor pursuits</rdfs:comment>
        <rdfs:isDefinedBy rdf:resource="https://www.theworldavatar.com/kg/ontopoi"/>
        <rdfs:label>Water sports</rdfs:label>
    </owl:Class>
    


    <!-- https://www.theworldavatar.com/kg/ontopoi/Weatherservices -->


    <owl:Class rdf:about="https://www.theworldavatar.com/kg/ontopoi/Weatherservices">
        <rdfs:subClassOf rdf:resource="https://www.theworldavatar.com/kg/ontopoi/Personalandconsumerandotherservices"/>
        <rdfs:comment>Weather services is a subcategory of personal, consumer and other services</rdfs:comment>
        <rdfs:isDefinedBy rdf:resource="https://www.theworldavatar.com/kg/ontopoi"/>
        <rdfs:label>Weather services</rdfs:label>
    </owl:Class>
    


    <!-- https://www.theworldavatar.com/kg/ontopoi/Weddingservices -->


    <owl:Class rdf:about="https://www.theworldavatar.com/kg/ontopoi/Weddingservices">
        <rdfs:subClassOf rdf:resource="https://www.theworldavatar.com/kg/ontopoi/Personalandconsumerandotherservices"/>
        <rdfs:comment>Wedding services is a subcategory of personal, consumer and other services</rdfs:comment>
        <rdfs:isDefinedBy rdf:resource="https://www.theworldavatar.com/kg/ontopoi"/>
        <rdfs:label>Wedding services</rdfs:label>
    </owl:Class>
    


    <!-- https://www.theworldavatar.com/kg/ontopoi/Weighbridges -->


    <owl:Class rdf:about="https://www.theworldavatar.com/kg/ontopoi/Weighbridges">
        <rdfs:subClassOf rdf:resource="https://www.theworldavatar.com/kg/ontopoi/Roadandrail"/>
        <rdfs:comment>Weighbridges is a subcategory of road and rail</rdfs:comment>
        <rdfs:isDefinedBy rdf:resource="https://www.theworldavatar.com/kg/ontopoi"/>
        <rdfs:label>Weighbridges</rdfs:label>
    </owl:Class>
    


    <!-- https://www.theworldavatar.com/kg/ontopoi/Weirsandsluicesanddams -->


    <owl:Class rdf:about="https://www.theworldavatar.com/kg/ontopoi/Weirsandsluicesanddams">
        <rdfs:subClassOf rdf:resource="https://www.theworldavatar.com/kg/ontopoi/Water"/>
        <rdfs:comment>Weirs, sluices and dams is a subcategory of water</rdfs:comment>
        <rdfs:isDefinedBy rdf:resource="https://www.theworldavatar.com/kg/ontopoi"/>
        <rdfs:label>Weirs, sluices and dams</rdfs:label>
    </owl:Class>
    


    <!-- https://www.theworldavatar.com/kg/ontopoi/Wi-Fihotspots -->


    <owl:Class rdf:about="https://www.theworldavatar.com/kg/ontopoi/Wi-Fihotspots">
        <rdfs:subClassOf rdf:resource="https://www.theworldavatar.com/kg/ontopoi/Infrastructureandfacilities"/>
        <rdfs:comment>Wi-fi hotspots is a subcategory of infrastructure and facilities</rdfs:comment>
        <rdfs:isDefinedBy rdf:resource="https://www.theworldavatar.com/kg/ontopoi"/>
        <rdfs:label>Wi-Fi hotspots</rdfs:label>
    </owl:Class>
    


    <!-- https://www.theworldavatar.com/kg/ontopoi/Windowcleaners -->


    <owl:Class rdf:about="https://www.theworldavatar.com/kg/ontopoi/Windowcleaners">
        <rdfs:subClassOf rdf:resource="https://www.theworldavatar.com/kg/ontopoi/Personalandconsumerandotherservices"/>
        <rdfs:comment>Window cleaners is a subcategory of personal, consumer and other services</rdfs:comment>
        <rdfs:isDefinedBy rdf:resource="https://www.theworldavatar.com/kg/ontopoi"/>
        <rdfs:label>Window cleaners</rdfs:label>
    </owl:Class>
    


    <!-- https://www.theworldavatar.com/kg/ontopoi/Woodproductsincludingcharcoalandpaperandcardandboard -->


    <owl:Class rdf:about="https://www.theworldavatar.com/kg/ontopoi/Woodproductsincludingcharcoalandpaperandcardandboard">
        <rdfs:subClassOf rdf:resource="https://www.theworldavatar.com/kg/ontopoi/Industrialproducts"/>
        <rdfs:comment>Wood products including charcoal, paper, card and board is a subcategory of industrial products</rdfs:comment>
        <rdfs:isDefinedBy rdf:resource="https://www.theworldavatar.com/kg/ontopoi"/>
        <rdfs:label>Wood products including charcoal, paper, card and board</rdfs:label>
    </owl:Class>
    


    <!-- https://www.theworldavatar.com/kg/ontopoi/Workwear -->


    <owl:Class rdf:about="https://www.theworldavatar.com/kg/ontopoi/Workwear">
        <rdfs:subClassOf rdf:resource="https://www.theworldavatar.com/kg/ontopoi/Industrialproducts"/>
        <rdfs:comment>Workwear is a subcategory of industrial products</rdfs:comment>
        <rdfs:isDefinedBy rdf:resource="https://www.theworldavatar.com/kg/ontopoi"/>
        <rdfs:label>Workwear</rdfs:label>
    </owl:Class>
    


    <!-- https://www.theworldavatar.com/kg/ontopoi/X-rayservices -->


    <owl:Class rdf:about="https://www.theworldavatar.com/kg/ontopoi/X-rayservices">
        <rdfs:subClassOf rdf:resource="https://www.theworldavatar.com/kg/ontopoi/Healthsupportservices"/>
        <rdfs:comment>X-ray services is a subcategory of health support services</rdfs:comment>
        <rdfs:isDefinedBy rdf:resource="https://www.theworldavatar.com/kg/ontopoi"/>
        <rdfs:label>X-ray services</rdfs:label>
    </owl:Class>
    


    <!-- https://www.theworldavatar.com/kg/ontopoi/Youthaccommodation -->


    <owl:Class rdf:about="https://www.theworldavatar.com/kg/ontopoi/Youthaccommodation">
        <rdfs:subClassOf rdf:resource="https://www.theworldavatar.com/kg/ontopoi/Accommodation"/>
        <rdfs:comment>Youth accommodation is a subcategory of accommodation</rdfs:comment>
        <rdfs:isDefinedBy rdf:resource="https://www.theworldavatar.com/kg/ontopoi"/>
        <rdfs:label>Youth accommodation</rdfs:label>
    </owl:Class>
    


    <!-- https://www.theworldavatar.com/kg/ontopoi/Youthorganisations -->


    <owl:Class rdf:about="https://www.theworldavatar.com/kg/ontopoi/Youthorganisations">
        <rdfs:subClassOf rdf:resource="https://www.theworldavatar.com/kg/ontopoi/Organisations"/>
        <rdfs:comment>Youth organisations is a subcategory of organisations</rdfs:comment>
        <rdfs:isDefinedBy rdf:resource="https://www.theworldavatar.com/kg/ontopoi"/>
        <rdfs:label>Youth organisations</rdfs:label>
    </owl:Class>
    


    <!-- https://www.theworldavatar.com/kg/ontopoi/Zoosandanimalcollections -->


    <owl:Class rdf:about="https://www.theworldavatar.com/kg/ontopoi/Zoosandanimalcollections">
        <rdfs:subClassOf rdf:resource="https://www.theworldavatar.com/kg/ontopoi/Botanicalandzoological"/>
        <rdfs:comment>Zoos and animal collections is a subcategory of botanical and zoological</rdfs:comment>
        <rdfs:isDefinedBy rdf:resource="https://www.theworldavatar.com/kg/ontopoi"/>
        <rdfs:label>Zoos and animal collections</rdfs:label>
    </owl:Class>
    


    <!-- https://www.theworldavatar.com/kg/ontopoi/Animalbreeders(nothorses) -->


    <owl:Class rdf:about="https://www.theworldavatar.com/kg/ontopoi/Animalbreeders(nothorses)">
        <rdfs:subClassOf rdf:resource="https://www.theworldavatar.com/kg/ontopoi/Farming"/>
        <rdfs:comment>Animal breeders (not horses) is a subcategory of farming</rdfs:comment>
        <rdfs:isDefinedBy rdf:resource="https://www.theworldavatar.com/kg/ontopoi"/>
        <rdfs:label>Animal breeders (not horses)</rdfs:label>
    </owl:Class>
    


    <!-- https://www.theworldavatar.com/kg/ontopoi/Cookersandstovesnon-electrical -->


    <owl:Class rdf:about="https://www.theworldavatar.com/kg/ontopoi/Cookersandstovesnon-electrical">
        <rdfs:subClassOf rdf:resource="https://www.theworldavatar.com/kg/ontopoi/Consumerproducts"/>
        <rdfs:comment>Cookers and stoves  non-electrical is a subcategory of consumer products</rdfs:comment>
        <rdfs:isDefinedBy rdf:resource="https://www.theworldavatar.com/kg/ontopoi"/>
        <rdfs:label>Cookers and stoves  non-electrical</rdfs:label>
    </owl:Class>
    


    <!-- https://www.theworldavatar.com/kg/ontopoi/PayPointlocations -->


    <owl:Class rdf:about="https://www.theworldavatar.com/kg/ontopoi/PayPointlocations">
        <rdfs:subClassOf rdf:resource="https://www.theworldavatar.com/kg/ontopoi/Legalandfinancial"/>
        <rdfs:comment>Paypoint locations is a subcategory of legal and financial</rdfs:comment>
        <rdfs:isDefinedBy rdf:resource="https://www.theworldavatar.com/kg/ontopoi"/>
        <rdfs:label>PayPoint locations</rdfs:label>
    </owl:Class>
    


    <!-- https://www.theworldavatar.com/kg/ontopoi/Railways(heritageandsteamandminiature) -->


    <owl:Class rdf:about="https://www.theworldavatar.com/kg/ontopoi/Railways(heritageandsteamandminiature)">
        <rdfs:subClassOf rdf:resource="https://www.theworldavatar.com/kg/ontopoi/Tourism"/>
        <rdfs:comment>Railways (heritage, steam and miniature) is a subcategory of tourism</rdfs:comment>
        <rdfs:isDefinedBy rdf:resource="https://www.theworldavatar.com/kg/ontopoi"/>
        <rdfs:label>Railways (heritage, steam and miniature)</rdfs:label>
    </owl:Class>
</rdf:RDF>



<!-- Generated by the OWL API (version 5.5.0.2023-01-14T12:41:38Z) https://github.com/owlcs/owlapi/ -->


