<?xml version="1.0"?>
<rdf:RDF xmlns="https://www.theworldavatar.com/kg/ontopoi/"
     xml:base="https://www.theworldavatar.com/kg/ontopoi/"
     xmlns:dc="http://purl.org/dc/elements/1.1/"
     xmlns:owl="http://www.w3.org/2002/07/owl#"
     xmlns:rdf="http://www.w3.org/1999/02/22-rdf-syntax-ns#"
     xmlns:xml="http://www.w3.org/XML/1998/namespace"
     xmlns:xsd="http://www.w3.org/2001/XMLSchema#"
     xmlns:rdfs="http://www.w3.org/2000/01/rdf-schema#"
     xmlns:ontopoi="https://www.theworldavatar.com/kg/ontopoi/">
    <owl:Ontology rdf:about="https://www.theworldavatar.com/kg/ontopoi/">
        <dc:date>11 November 2024</dc:date>
        <rdfs:comment>OntoPOI is an ontology developed for representing points of interest.</rdfs:comment>
        <owl:versionInfo>1</owl:versionInfo>
        <gitCommitHash>c0599beca8df55873a1ab061dee64e52c510c6a0</gitCommitHash>
    </owl:Ontology>
    


    <!-- 
    ///////////////////////////////////////////////////////////////////////////////////////
    //
    // Annotation properties
    //
    ///////////////////////////////////////////////////////////////////////////////////////
     -->


    


    <!-- http://purl.org/dc/elements/1.1/date -->


    <owl:AnnotationProperty rdf:about="http://purl.org/dc/elements/1.1/date"/>
    


    <!-- https://www.theworldavatar.com/kg/ontopoi/gitCommitHash -->


    <owl:AnnotationProperty rdf:about="https://www.theworldavatar.com/kg/ontopoi/gitCommitHash"/>
    


    <!-- 
    ///////////////////////////////////////////////////////////////////////////////////////
    //
    // Datatypes
    //
    ///////////////////////////////////////////////////////////////////////////////////////
     -->


    


    <!-- http://www.opengis.net/ont/geosparql#wktLiteral -->


    <rdfs:Datatype rdf:about="http://www.opengis.net/ont/geosparql#wktLiteral"/>
    


    <!-- 
    ///////////////////////////////////////////////////////////////////////////////////////
    //
    // Object Properties
    //
    ///////////////////////////////////////////////////////////////////////////////////////
     -->


    


    <!-- http://ies.data.gov.uk/ontology/ies4#branding -->


    <owl:ObjectProperty rdf:about="http://ies.data.gov.uk/ontology/ies4#branding">
        <rdfs:domain rdf:resource="https://www.theworldavatar.com/kg/ontopoi/PointOfInterest"/>
        <rdfs:range rdf:resource="http://ies.data.gov.uk/ontology/ies4#Organisation"/>
        <rdfs:comment>The brand associated with the POI</rdfs:comment>
        <rdfs:isDefinedBy rdf:resource="http://ies.data.gov.uk/ontology/ies4"/>
        <rdfs:label>has Brand</rdfs:label>
    </owl:ObjectProperty>
    


    <!-- http://ies.data.gov.uk/ontology/ies4#hasSourceReference -->


    <owl:ObjectProperty rdf:about="http://ies.data.gov.uk/ontology/ies4#hasSourceReference">
        <rdfs:domain rdf:resource="https://www.theworldavatar.com/kg/ontopoi/PointOfInterest"/>
        <rdfs:range rdf:resource="https://www.theworldavatar.com/kg/ontopoi/SourceReference"/>
        <rdfs:comment>The source of the data, e.g., Ordnance Survey</rdfs:comment>
        <rdfs:isDefinedBy rdf:resource="http://ies.data.gov.uk/ontology/ies4"/>
        <rdfs:label>has Source Reference</rdfs:label>
    </owl:ObjectProperty>
    


    <!-- http://ies.data.gov.uk/ontology/ies4#inPeriod -->


    <owl:ObjectProperty rdf:about="http://ies.data.gov.uk/ontology/ies4#inPeriod">
        <rdfs:domain>
            <owl:Class>
                <owl:unionOf rdf:parseType="Collection">
                    <rdf:Description rdf:about="https://www.theworldavatar.com/kg/ontopoi/PointOfInterestEnd"/>
                    <rdf:Description rdf:about="https://www.theworldavatar.com/kg/ontopoi/PointOfInterestStart"/>
                </owl:unionOf>
            </owl:Class>
        </rdfs:domain>
        <rdfs:range rdf:resource="http://ies.data.gov.uk/ontology/ies4#ParticularPeriod"/>
        <rdfs:comment>An object property relating the start or end of a point-of-interest entity to a specific period.</rdfs:comment>
        <rdfs:isDefinedBy rdf:resource="http://ies.data.gov.uk/ontology/ies4"/>
        <rdfs:label>in Period</rdfs:label>
    </owl:ObjectProperty>
    


    <!-- http://ies.data.gov.uk/ontology/ies4#isEndOf -->


    <owl:ObjectProperty rdf:about="http://ies.data.gov.uk/ontology/ies4#isEndOf">
        <rdfs:domain rdf:resource="https://www.theworldavatar.com/kg/ontopoi/PointOfInterestEnd"/>
        <rdfs:range rdf:resource="https://www.theworldavatar.com/kg/ontopoi/PointOfInterest"/>
        <rdfs:comment>An object property representing the end date of a point-of-interest entity.</rdfs:comment>
        <rdfs:isDefinedBy rdf:resource="http://ies.data.gov.uk/ontology/ies4"/>
        <rdfs:label>is End Of</rdfs:label>
    </owl:ObjectProperty>
    


    <!-- http://ies.data.gov.uk/ontology/ies4#isStartOf -->


    <owl:ObjectProperty rdf:about="http://ies.data.gov.uk/ontology/ies4#isStartOf">
        <rdfs:domain rdf:resource="https://www.theworldavatar.com/kg/ontopoi/PointOfInterestStart"/>
        <rdfs:range rdf:resource="https://www.theworldavatar.com/kg/ontopoi/PointOfInterest"/>
        <rdfs:comment>An object property representing the start date of a point-of-interest entity.</rdfs:comment>
        <rdfs:isDefinedBy rdf:resource="http://ies.data.gov.uk/ontology/ies4"/>
        <rdfs:label>is Start Of</rdfs:label>
    </owl:ObjectProperty>
    


    <!-- http://www.ontology-of-units-of-measure.org/resource/om-2/hasUnit -->


    <owl:ObjectProperty rdf:about="http://www.ontology-of-units-of-measure.org/resource/om-2/hasUnit">
        <rdfs:domain rdf:resource="http://www.ontology-of-units-of-measure.org/resource/om-2/Measure"/>
        <rdfs:range rdf:resource="http://www.ontology-of-units-of-measure.org/resource/om-2/Unit"/>
        <rdfs:isDefinedBy rdf:resource="http://www.ontology-of-units-of-measure.org/resource/om-2"/>
        <rdfs:label>has Unit</rdfs:label>
    </owl:ObjectProperty>
    


    <!-- http://www.ontology-of-units-of-measure.org/resource/om-2/hasValue -->


    <owl:ObjectProperty rdf:about="http://www.ontology-of-units-of-measure.org/resource/om-2/hasValue">
        <rdfs:domain rdf:resource="https://www.theworldavatar.com/kg/ontopoi/Distance"/>
        <rdfs:range rdf:resource="http://www.ontology-of-units-of-measure.org/resource/om-2/Measure"/>
        <rdfs:isDefinedBy rdf:resource="http://www.ontology-of-units-of-measure.org/resource/om-2"/>
        <rdfs:label>has Value</rdfs:label>
    </owl:ObjectProperty>
    


    <!-- http://www.theworldavatar.com/kg/OntoFHRS/hasAddress -->


    <owl:ObjectProperty rdf:about="http://www.theworldavatar.com/kg/OntoFHRS/hasAddress">
        <rdfs:domain rdf:resource="https://www.theworldavatar.com/kg/ontopoi/PointOfInterest"/>
        <rdfs:range rdf:resource="http://ies.data.gov.uk/ontology/ies4#Address"/>
        <rdfs:comment>The address of the POI, including the street address and building number</rdfs:comment>
        <rdfs:isDefinedBy rdf:resource="https://www.theworldavatar.com/kg/ontopoi"/>
        <rdfs:label>has Address</rdfs:label>
    </owl:ObjectProperty>
    


    <!-- http://www.w3.org/2006/vcard/ns#hasLocality -->


    <owl:ObjectProperty rdf:about="http://www.w3.org/2006/vcard/ns#hasLocality">
        <rdfs:domain rdf:resource="http://ies.data.gov.uk/ontology/ies4#Address"/>
        <rdfs:range rdf:resource="https://www.theworldavatar.com/kg/ontopoi/Locality"/>
        <rdfs:comment>The local area or town where the POI is situated</rdfs:comment>
        <rdfs:isDefinedBy rdf:resource="http://www.w3.org/2006/vcard/ns"/>
        <rdfs:label>has Locality</rdfs:label>
    </owl:ObjectProperty>
    


    <!-- https://www.theworldavatar.com/kg/ontopoi/hasAdministrativeBoundary -->


    <owl:ObjectProperty rdf:about="https://www.theworldavatar.com/kg/ontopoi/hasAdministrativeBoundary">
        <rdfs:domain rdf:resource="https://www.theworldavatar.com/kg/ontopoi/PointOfInterest"/>
        <rdfs:range rdf:resource="https://www.theworldavatar.com/kg/ontobuiltenv/AdministrativeDistrict"/>
        <rdfs:comment>The administrative boundary in which the POI falls (e.g., a local government or district boundary)</rdfs:comment>
        <rdfs:isDefinedBy rdf:resource="https://www.theworldavatar.com/kg/ontopoi"/>
        <rdfs:label>has Administrative Boundary</rdfs:label>
    </owl:ObjectProperty>
    


    <!-- https://www.theworldavatar.com/kg/ontopoi/hasDistance -->


    <owl:ObjectProperty rdf:about="https://www.theworldavatar.com/kg/ontopoi/hasDistance">
        <rdfs:domain rdf:resource="https://www.theworldavatar.com/kg/ontopoi/PointOfInterest"/>
        <rdfs:range rdf:resource="https://www.theworldavatar.com/kg/ontopoi/Distance"/>
        <rdfs:comment>An object property indicating the distance from the POI to its nearest ITN</rdfs:comment>
        <rdfs:isDefinedBy rdf:resource="https://www.theworldavatar.com/kg/ontopoi"/>
        <rdfs:label>has Distance</rdfs:label>
    </owl:ObjectProperty>
    


    <!-- https://www.theworldavatar.com/kg/ontopoi/hasGeographicCounty -->


    <owl:ObjectProperty rdf:about="https://www.theworldavatar.com/kg/ontopoi/hasGeographicCounty">
        <rdfs:domain rdf:resource="http://ies.data.gov.uk/ontology/ies4#Address"/>
        <rdfs:range rdf:resource="https://www.theworldavatar.com/kg/ontopoi/GeographicCounty"/>
        <rdfs:comment>The geographic county where the POI is located</rdfs:comment>
        <rdfs:isDefinedBy rdf:resource="https://www.theworldavatar.com/kg/ontopoi"/>
        <rdfs:label>has Geographic County</rdfs:label>
    </owl:ObjectProperty>
    


    <!-- https://www.theworldavatar.com/kg/ontopoi/hasNearestITN -->


    <owl:ObjectProperty rdf:about="https://www.theworldavatar.com/kg/ontopoi/hasNearestITN">
        <rdfs:domain rdf:resource="https://www.theworldavatar.com/kg/ontopoi/PointOfInterest"/>
        <rdfs:range rdf:resource="https://www.theworldavatar.com/kg/ontopoi/ITN"/>
        <rdfs:isDefinedBy rdf:resource="https://www.theworldavatar.com/kg/ontopoi"/>
        <rdfs:label>has nearest ITN</rdfs:label>
    </owl:ObjectProperty>
    


    <!-- 
    ///////////////////////////////////////////////////////////////////////////////////////
    //
    // Data properties
    //
    ///////////////////////////////////////////////////////////////////////////////////////
     -->


    


    <!-- http://ies.data.gov.uk/ontology/ies4#iso8601PeriodRepresentation -->


    <owl:DatatypeProperty rdf:about="http://ies.data.gov.uk/ontology/ies4#iso8601PeriodRepresentation">
        <rdfs:domain rdf:resource="http://ies.data.gov.uk/ontology/ies4#ParticularPeriod"/>
        <rdfs:range rdf:resource="http://www.w3.org/2001/XMLSchema#anyURI"/>
        <rdfs:isDefinedBy rdf:resource="http://ies.data.gov.uk/ontology/ies4"/>
        <rdfs:label>iso 8601 Period Representation</rdfs:label>
    </owl:DatatypeProperty>
    


    <!-- http://ontology.eil.utoronto.ca/icontact.owl#hasStreet -->


    <owl:DatatypeProperty rdf:about="http://ontology.eil.utoronto.ca/icontact.owl#hasStreet">
        <rdfs:domain rdf:resource="http://ies.data.gov.uk/ontology/ies4#Address"/>
        <rdfs:range rdf:resource="http://www.w3.org/2001/XMLSchema#string"/>
        <rdfs:comment>Name of the street where the POI is located</rdfs:comment>
        <rdfs:isDefinedBy rdf:resource="http://ontology.eil.utoronto.ca/icontact.owl"/>
        <rdfs:label>has Street</rdfs:label>
    </owl:DatatypeProperty>
    


    <!-- http://www.ontology-of-units-of-measure.org/resource/om-2/hasNumericalValue -->


    <owl:DatatypeProperty rdf:about="http://www.ontology-of-units-of-measure.org/resource/om-2/hasNumericalValue">
        <rdfs:domain rdf:resource="http://www.ontology-of-units-of-measure.org/resource/om-2/Measure"/>
        <rdfs:range rdf:resource="http://www.w3.org/2001/XMLSchema#double"/>
        <rdfs:isDefinedBy rdf:resource="http://www.ontology-of-units-of-measure.org/resource/om-2"/>
        <rdfs:label>has Numerical Value</rdfs:label>
    </owl:DatatypeProperty>
    


    <!-- http://www.opengis.net/ont/geosparql#asWKT -->


    <owl:DatatypeProperty rdf:about="http://www.opengis.net/ont/geosparql#asWKT">
        <rdfs:domain>
            <owl:Class>
                <owl:unionOf rdf:parseType="Collection">
                    <rdf:Description rdf:about="https://www.theworldavatar.com/kg/ontopoi/ITN"/>
                    <rdf:Description rdf:about="https://www.theworldavatar.com/kg/ontopoi/PointOfInterest"/>
                </owl:unionOf>
            </owl:Class>
        </rdfs:domain>
        <rdfs:range rdf:resource="http://www.opengis.net/ont/geosparql#wktLiteral"/>
        <rdfs:comment>The spatial geometry of a Point of Interest (POI), represented in Well-Known Text (WKT) format, detailing its shape and boundaries</rdfs:comment>
        <rdfs:isDefinedBy rdf:resource="http://www.opengis.net/ont/geosparql"/>
        <rdfs:label>as WKT</rdfs:label>
    </owl:DatatypeProperty>
    


    <!-- http://www.w3.org/2006/vcard/ns#postal-code -->


    <owl:DatatypeProperty rdf:about="http://www.w3.org/2006/vcard/ns#postal-code">
        <rdfs:domain rdf:resource="http://ies.data.gov.uk/ontology/ies4#Address"/>
        <rdfs:range rdf:resource="http://www.w3.org/2001/XMLSchema#string"/>
        <rdfs:comment>Postal code associated with the POI</rdfs:comment>
        <rdfs:isDefinedBy rdf:resource="http://www.w3.org/2006/vcard/ns"/>
        <rdfs:label>has Postal Code</rdfs:label>
    </owl:DatatypeProperty>
    


    <!-- https://www.theworldavatar.com/kg/ontopoi/hasMeasureOfImportance -->


    <owl:DatatypeProperty rdf:about="https://www.theworldavatar.com/kg/ontopoi/hasMeasureOfImportance">
        <rdfs:domain rdf:resource="http://rdfs.co/juso/Street"/>
        <rdfs:range rdf:resource="http://www.w3.org/2001/XMLSchema#integer"/>
        <rdfs:comment>The Measure of Importance (MI) reflects how significant or large a street is</rdfs:comment>
        <rdfs:label>has Measure Of Importance (MI)</rdfs:label>
    </owl:DatatypeProperty>
    


    <!-- https://www.theworldavatar.com/kg/ontopoi/hasName -->


    <owl:DatatypeProperty rdf:about="https://www.theworldavatar.com/kg/ontopoi/hasName">
        <rdfs:domain rdf:resource="https://www.theworldavatar.com/kg/ontopoi/PointOfInterest"/>
        <rdfs:range rdf:resource="http://www.w3.org/2001/XMLSchema#string"/>
        <rdfs:comment>The name of the point of interest (e.g., business, landmark, or facility)</rdfs:comment>
        <rdfs:isDefinedBy rdf:resource="https://www.theworldavatar.com/kg/ontopoi"/>
        <rdfs:label>has Name</rdfs:label>
    </owl:DatatypeProperty>
    


    <!-- https://www.theworldavatar.com/kg/ontopoi/hasPointXClassificationCode -->


    <owl:DatatypeProperty rdf:about="https://www.theworldavatar.com/kg/ontopoi/hasPointXClassificationCode">
        <rdfs:domain rdf:resource="https://www.theworldavatar.com/kg/ontopoi/PointOfInterest"/>
        <rdfs:range rdf:resource="http://www.w3.org/2001/XMLSchema#string"/>
        <rdfs:comment>The classification code indicating the type of POI, represented by concatenating the top-level category ID, mid-level category ID, and the POI own unique ID, in that order</rdfs:comment>
        <rdfs:isDefinedBy rdf:resource="https://www.theworldavatar.com/kg/ontopoi"/>
        <rdfs:label>has PointX Classification Code</rdfs:label>
    </owl:DatatypeProperty>
    


    <!-- https://www.theworldavatar.com/kg/ontopoi/hasPositionalAccuracy -->


    <owl:DatatypeProperty rdf:about="https://www.theworldavatar.com/kg/ontopoi/hasPositionalAccuracy">
        <rdfs:domain rdf:resource="https://www.theworldavatar.com/kg/ontopoi/PointOfInterest"/>
        <rdfs:range rdf:resource="http://www.w3.org/2001/XMLSchema#integer"/>
        <rdfs:comment>An indication of how precisely the Point of Interest (POI) location has been mapped. The positional accuracy value can be an integer between 1 and 4, where 1 means positioned at the exact address or location, usually within the building footprint; 2 means positioned near the address or location for non-addressable features; 3 means placed at the road associated with the address or location; and 4 means positioned within the general geographical locality.</rdfs:comment>
        <rdfs:isDefinedBy rdf:resource="https://www.theworldavatar.com/kg/ontopoi"/>
        <rdfs:label>has Positional Accuracy</rdfs:label>
    </owl:DatatypeProperty>
    


    <!-- https://www.theworldavatar.com/kg/ontopoi/hasQualifier -->


    <owl:DatatypeProperty rdf:about="https://www.theworldavatar.com/kg/ontopoi/hasQualifier">
        <rdfs:domain rdf:resource="https://www.theworldavatar.com/kg/ontopoi/PointOfInterest"/>
        <rdfs:range rdf:resource="http://www.w3.org/2001/XMLSchema#string"/>
        <rdfs:comment>Specifies the class of qualifier associated with the POI, e.g., Food Bank</rdfs:comment>
        <rdfs:isDefinedBy rdf:resource="https://www.theworldavatar.com/kg/ontopoi"/>
        <rdfs:label>has Qualifier</rdfs:label>
    </owl:DatatypeProperty>
    


    <!-- https://www.theworldavatar.com/kg/ontopoi/hasQualifierType -->


    <owl:DatatypeProperty rdf:about="https://www.theworldavatar.com/kg/ontopoi/hasQualifierType">
        <rdfs:domain rdf:resource="https://www.theworldavatar.com/kg/ontopoi/PointOfInterest"/>
        <rdfs:range rdf:resource="http://www.w3.org/2001/XMLSchema#string"/>
        <rdfs:comment>Specifies the type of qualifier associated with the POI, which could provide further context or detail about the point, e.g., Charity</rdfs:comment>
        <rdfs:isDefinedBy rdf:resource="https://www.theworldavatar.com/kg/ontopoi"/>
        <rdfs:label>has Qualifier Type</rdfs:label>
    </owl:DatatypeProperty>
    


    <!-- https://www.theworldavatar.com/kg/ontopoi/hasReferenceNumber -->


    <owl:DatatypeProperty rdf:about="https://www.theworldavatar.com/kg/ontopoi/hasReferenceNumber">
        <rdfs:domain rdf:resource="https://www.theworldavatar.com/kg/ontopoi/PointOfInterest"/>
        <rdfs:range rdf:resource="http://www.w3.org/2001/XMLSchema#string"/>
        <rdfs:comment>The unique reference number for the POI entity</rdfs:comment>
        <rdfs:isDefinedBy rdf:resource="https://www.theworldavatar.com/kg/ontopoi"/>
        <rdfs:label>has Reference Number</rdfs:label>
    </owl:DatatypeProperty>
    


    <!-- https://www.theworldavatar.com/kg/ontopoi/hasSupplyDate -->


    <owl:DatatypeProperty rdf:about="https://www.theworldavatar.com/kg/ontopoi/hasSupplyDate">
        <rdfs:domain rdf:resource="https://www.theworldavatar.com/kg/ontopoi/PointOfInterest"/>
        <rdfs:range rdf:resource="http://www.w3.org/2001/XMLSchema#dateTime"/>
        <rdfs:comment>The date when the POI data was supplied or last updated</rdfs:comment>
        <rdfs:isDefinedBy rdf:resource="https://www.theworldavatar.com/kg/ontopoi"/>
        <rdfs:label>has Supply Date</rdfs:label>
    </owl:DatatypeProperty>
    


    <!-- https://www.theworldavatar.com/kg/ontopoi/hasTOID -->


    <owl:DatatypeProperty rdf:about="https://www.theworldavatar.com/kg/ontopoi/hasTOID">
        <rdfs:domain>
            <owl:Class>
                <owl:unionOf rdf:parseType="Collection">
                    <rdf:Description rdf:about="https://www.theworldavatar.com/kg/ontopoi/ITN"/>
                    <rdf:Description rdf:about="https://www.theworldavatar.com/kg/ontopoi/PointOfInterest"/>
                </owl:unionOf>
            </owl:Class>
        </rdfs:domain>
        <rdfs:range rdf:resource="http://www.w3.org/2001/XMLSchema#string"/>
        <rdfs:comment>The Topographic Object Identifier (TOID) of the POI or ITN, a unique ID used by Ordnance Survey to identify topographic features in the UK</rdfs:comment>
        <rdfs:isDefinedBy rdf:resource="https://www.theworldavatar.com/kg/ontopoi"/>
        <rdfs:label>has TOID</rdfs:label>
    </owl:DatatypeProperty>
    


    <!-- https://www.theworldavatar.com/kg/ontopoi/hasTOIDVersion -->


    <owl:DatatypeProperty rdf:about="https://www.theworldavatar.com/kg/ontopoi/hasTOIDVersion">
        <rdfs:domain>
            <owl:Class>
                <owl:unionOf rdf:parseType="Collection">
                    <rdf:Description rdf:about="https://www.theworldavatar.com/kg/ontopoi/ITN"/>
                    <rdf:Description rdf:about="https://www.theworldavatar.com/kg/ontopoi/PointOfInterest"/>
                </owl:unionOf>
            </owl:Class>
        </rdfs:domain>
        <rdfs:range rdf:resource="http://www.w3.org/2001/XMLSchema#string"/>
        <rdfs:comment>The version of the Topographic Object Identifier (TOID) of the POI or ITN</rdfs:comment>
        <rdfs:isDefinedBy rdf:resource="https://www.theworldavatar.com/kg/ontopoi"/>
        <rdfs:label>has TOID Version</rdfs:label>
    </owl:DatatypeProperty>
    


    <!-- https://www.theworldavatar.com/kg/ontopoi/hasTelephoneNumber -->


    <owl:DatatypeProperty rdf:about="https://www.theworldavatar.com/kg/ontopoi/hasTelephoneNumber">
        <rdfs:domain rdf:resource="https://www.theworldavatar.com/kg/ontopoi/PointOfInterest"/>
        <rdfs:range rdf:resource="http://www.w3.org/2001/XMLSchema#string"/>
        <rdfs:comment>Contact telephone number for the POI</rdfs:comment>
        <rdfs:isDefinedBy rdf:resource="https://www.theworldavatar.com/kg/ontopoi"/>
        <rdfs:label>has Telephone Number</rdfs:label>
    </owl:DatatypeProperty>
    


    <!-- https://www.theworldavatar.com/kg/ontopoi/hasUPRN -->


    <owl:DatatypeProperty rdf:about="https://www.theworldavatar.com/kg/ontopoi/hasUPRN">
        <rdfs:domain rdf:resource="https://www.theworldavatar.com/kg/ontopoi/PointOfInterest"/>
        <rdfs:range rdf:resource="http://www.w3.org/2001/XMLSchema#string"/>
        <rdfs:comment>It indicates the Unique Property Reference Number (UPRN) of the POI, which serves as the identifier for the corresponding land or property unit in the AddressBase of Ordnance Survey</rdfs:comment>
        <rdfs:isDefinedBy rdf:resource="https://www.theworldavatar.com/kg/ontopoi"/>
        <rdfs:label>has UPRN</rdfs:label>
    </owl:DatatypeProperty>
    


    <!-- https://www.theworldavatar.com/kg/ontopoi/hasURL -->


    <owl:DatatypeProperty rdf:about="https://www.theworldavatar.com/kg/ontopoi/hasURL">
        <rdfs:domain rdf:resource="https://www.theworldavatar.com/kg/ontopoi/PointOfInterest"/>
        <rdfs:range rdf:resource="http://www.w3.org/2001/XMLSchema#anyURI"/>
        <rdfs:comment>The web address (URL) of the POI</rdfs:comment>
        <rdfs:isDefinedBy rdf:resource="https://www.theworldavatar.com/kg/ontopoi"/>
        <rdfs:label>has URL</rdfs:label>
    </owl:DatatypeProperty>
    


    <!-- https://www.theworldavatar.com/kg/ontopoi/hasUSRN -->


    <owl:DatatypeProperty rdf:about="https://www.theworldavatar.com/kg/ontopoi/hasUSRN">
        <rdfs:domain rdf:resource="http://rdfs.co/juso/Street"/>
        <rdfs:range rdf:resource="http://www.w3.org/2001/XMLSchema#string"/>
        <rdfs:comment>The Unique Street Reference Number (USRN) is an 8-digit identifier that uniquely identifies every street in Great Britain</rdfs:comment>
        <rdfs:isDefinedBy rdf:resource="https://www.theworldavatar.com/kg/ontopoi"/>
        <rdfs:label>has USRN</rdfs:label>
    </owl:DatatypeProperty>
    


    <!-- https://www.theworldavatar.com/kg/ontopoi/isAddressVerified -->


    <owl:DatatypeProperty rdf:about="https://www.theworldavatar.com/kg/ontopoi/isAddressVerified">
        <rdfs:domain rdf:resource="https://www.theworldavatar.com/kg/ontopoi/PointOfInterest"/>
        <rdfs:range rdf:resource="http://www.w3.org/2001/XMLSchema#boolean"/>
        <rdfs:comment>Indicates whether the address has been verified</rdfs:comment>
        <rdfs:isDefinedBy rdf:resource="https://www.theworldavatar.com/kg/ontopoi"/>
        <rdfs:label>is Address Verified</rdfs:label>
    </owl:DatatypeProperty>
    


    <!-- 
    ///////////////////////////////////////////////////////////////////////////////////////
    //
    // Classes
    //
    ///////////////////////////////////////////////////////////////////////////////////////
     -->


    


    <!-- http://ies.data.gov.uk/ontology/ies4#Address -->


    <owl:Class rdf:about="http://ies.data.gov.uk/ontology/ies4#Address">
        <rdfs:subClassOf>
            <owl:Restriction>
                <owl:onProperty rdf:resource="http://www.w3.org/2006/vcard/ns#hasLocality"/>
                <owl:qualifiedCardinality rdf:datatype="http://www.w3.org/2001/XMLSchema#nonNegativeInteger">1</owl:qualifiedCardinality>
                <owl:onClass rdf:resource="https://www.theworldavatar.com/kg/ontopoi/Locality"/>
            </owl:Restriction>
        </rdfs:subClassOf>
        <rdfs:subClassOf>
            <owl:Restriction>
                <owl:onProperty rdf:resource="https://www.theworldavatar.com/kg/ontopoi/hasGeographicCounty"/>
                <owl:qualifiedCardinality rdf:datatype="http://www.w3.org/2001/XMLSchema#nonNegativeInteger">1</owl:qualifiedCardinality>
                <owl:onClass rdf:resource="https://www.theworldavatar.com/kg/ontopoi/GeographicCounty"/>
            </owl:Restriction>
        </rdfs:subClassOf>
    </owl:Class>
    


    <!-- http://ies.data.gov.uk/ontology/ies4#BoundingState -->


    <owl:Class rdf:about="http://ies.data.gov.uk/ontology/ies4#BoundingState">
        <rdfs:isDefinedBy rdf:resource="http://ies.data.gov.uk/ontology/ies4"/>
        <rdfs:label>Bounding State</rdfs:label>
    </owl:Class>
    


    <!-- http://ies.data.gov.uk/ontology/ies4#Organisation -->


    <owl:Class rdf:about="http://ies.data.gov.uk/ontology/ies4#Organisation"/>
    


    <!-- http://ies.data.gov.uk/ontology/ies4#ParticularPeriod -->


    <owl:Class rdf:about="http://ies.data.gov.uk/ontology/ies4#ParticularPeriod"/>
    


    <!-- http://rdfs.co/juso/Street -->


    <owl:Class rdf:about="http://rdfs.co/juso/Street"/>
    


    <!-- http://www.ontology-of-units-of-measure.org/resource/om-2/Measure -->


    <owl:Class rdf:about="http://www.ontology-of-units-of-measure.org/resource/om-2/Measure"/>
    


    <!-- http://www.ontology-of-units-of-measure.org/resource/om-2/Quantity -->


    <owl:Class rdf:about="http://www.ontology-of-units-of-measure.org/resource/om-2/Quantity"/>
    


    <!-- http://www.ontology-of-units-of-measure.org/resource/om-2/Unit -->


    <owl:Class rdf:about="http://www.ontology-of-units-of-measure.org/resource/om-2/Unit"/>
    


    <!-- https://dbpedia.org/ontology/Locality -->


    <owl:Class rdf:about="https://dbpedia.org/ontology/Locality">
        <rdfs:comment>A geographic area or neighborhood within a larger city, town, or administrative region</rdfs:comment>
        <rdfs:isDefinedBy rdf:resource="https://dbpedia.org/ontology"/>
        <rdfs:label>Locality</rdfs:label>
    </owl:Class>
    


    <!-- https://dbpedia.org/ontology/Street -->


    <owl:Class rdf:about="https://dbpedia.org/ontology/Street">
        <rdfs:isDefinedBy rdf:resource="https://www.theworldavatar.com/kg/ontopoi"/>
        <rdfs:label>Street</rdfs:label>
    </owl:Class>
    


    <!-- https://www.theworldavatar.com/kg/ontobuiltenv/AdministrativeDistrict -->


    <owl:Class rdf:about="https://www.theworldavatar.com/kg/ontobuiltenv/AdministrativeDistrict"/>
    


    <!-- https://www.theworldavatar.com/kg/ontopoi/AbrasiveProductsAndGrindingEquipment -->


    <owl:Class rdf:about="https://www.theworldavatar.com/kg/ontopoi/AbrasiveProductsAndGrindingEquipment">
        <rdfs:subClassOf rdf:resource="https://www.theworldavatar.com/kg/ontopoi/IndustrialProducts"/>
        <rdfs:comment>Abrasive products and grinding equipment is a subcategory of industrial products</rdfs:comment>
        <rdfs:isDefinedBy rdf:resource="https://www.theworldavatar.com/kg/ontopoi"/>
        <rdfs:label>Abrasive products and grinding equipment</rdfs:label>
    </owl:Class>
    


    <!-- https://www.theworldavatar.com/kg/ontopoi/AccessEquipment -->


    <owl:Class rdf:about="https://www.theworldavatar.com/kg/ontopoi/AccessEquipment">
        <rdfs:subClassOf rdf:resource="https://www.theworldavatar.com/kg/ontopoi/IndustrialProducts"/>
        <rdfs:comment>Access equipment is a subcategory of industrial products</rdfs:comment>
        <rdfs:isDefinedBy rdf:resource="https://www.theworldavatar.com/kg/ontopoi"/>
        <rdfs:label>Access equipment</rdfs:label>
    </owl:Class>
    


    <!-- https://www.theworldavatar.com/kg/ontopoi/AccidentAndEmergencyHospitals -->


    <owl:Class rdf:about="https://www.theworldavatar.com/kg/ontopoi/AccidentAndEmergencyHospitals">
        <rdfs:subClassOf rdf:resource="https://www.theworldavatar.com/kg/ontopoi/HealthPractitionersAndEstablishments"/>
        <rdfs:comment>Accident and emergency hospitals is a subcategory of health practitioners and establishments</rdfs:comment>
        <rdfs:isDefinedBy rdf:resource="https://www.theworldavatar.com/kg/ontopoi"/>
        <rdfs:label>Accident and emergency hospitals</rdfs:label>
    </owl:Class>
    


    <!-- https://www.theworldavatar.com/kg/ontopoi/Accommodation -->


    <owl:Class rdf:about="https://www.theworldavatar.com/kg/ontopoi/Accommodation">
        <rdfs:subClassOf rdf:resource="https://www.theworldavatar.com/kg/ontopoi/AccommodationAndEatingAndDrinking"/>
        <rdfs:comment>Accommodation is a subcategory of accommodation, eating and drinking</rdfs:comment>
        <rdfs:isDefinedBy rdf:resource="https://www.theworldavatar.com/kg/ontopoi"/>
        <rdfs:label>Accommodation</rdfs:label>
    </owl:Class>
    


    <!-- https://www.theworldavatar.com/kg/ontopoi/AccommodationAndEatingAndDrinking -->


    <owl:Class rdf:about="https://www.theworldavatar.com/kg/ontopoi/AccommodationAndEatingAndDrinking"/>
    


    <!-- https://www.theworldavatar.com/kg/ontopoi/AccommodationEatingAndDrinking -->


    <owl:Class rdf:about="https://www.theworldavatar.com/kg/ontopoi/AccommodationEatingAndDrinking">
        <rdfs:subClassOf rdf:resource="https://www.theworldavatar.com/kg/ontopoi/PointOfInterest"/>
        <rdfs:comment>Any facility or place where individuals can stay temporarily and/or consume food and drinks, typically while traveling</rdfs:comment>
        <rdfs:isDefinedBy rdf:resource="https://www.theworldavatar.com/kg/ontopoi"/>
        <rdfs:label>Accommodation, eating and drinking</rdfs:label>
    </owl:Class>
    


    <!-- https://www.theworldavatar.com/kg/ontopoi/AccountantsAndAuditors -->


    <owl:Class rdf:about="https://www.theworldavatar.com/kg/ontopoi/AccountantsAndAuditors">
        <rdfs:subClassOf rdf:resource="https://www.theworldavatar.com/kg/ontopoi/LegalAndFinancial"/>
        <rdfs:comment>Accountants and auditors is a subcategory of legal and financial</rdfs:comment>
        <rdfs:isDefinedBy rdf:resource="https://www.theworldavatar.com/kg/ontopoi"/>
        <rdfs:label>Accountants and auditors</rdfs:label>
    </owl:Class>
    


    <!-- https://www.theworldavatar.com/kg/ontopoi/AdhesivesAndSealants -->


    <owl:Class rdf:about="https://www.theworldavatar.com/kg/ontopoi/AdhesivesAndSealants">
        <rdfs:subClassOf rdf:resource="https://www.theworldavatar.com/kg/ontopoi/IndustrialProducts"/>
        <rdfs:comment>Adhesives and sealants is a subcategory of industrial products</rdfs:comment>
        <rdfs:isDefinedBy rdf:resource="https://www.theworldavatar.com/kg/ontopoi"/>
        <rdfs:label>Adhesives and sealants</rdfs:label>
    </owl:Class>
    


    <!-- https://www.theworldavatar.com/kg/ontopoi/AdultServices -->


    <owl:Class rdf:about="https://www.theworldavatar.com/kg/ontopoi/AdultServices">
        <rdfs:subClassOf rdf:resource="https://www.theworldavatar.com/kg/ontopoi/PersonalAndConsumerAndOtherServices"/>
        <rdfs:comment>Adult services is a subcategory of personal, consumer and other services</rdfs:comment>
        <rdfs:isDefinedBy rdf:resource="https://www.theworldavatar.com/kg/ontopoi"/>
        <rdfs:label>Adult services</rdfs:label>
    </owl:Class>
    


    <!-- https://www.theworldavatar.com/kg/ontopoi/AdultShops -->


    <owl:Class rdf:about="https://www.theworldavatar.com/kg/ontopoi/AdultShops">
        <rdfs:subClassOf rdf:resource="https://www.theworldavatar.com/kg/ontopoi/HouseholdAndOfficeAndLeisureAndGarden"/>
        <rdfs:comment>Adult shops is a subcategory of household, office, leisure and garden</rdfs:comment>
        <rdfs:isDefinedBy rdf:resource="https://www.theworldavatar.com/kg/ontopoi"/>
        <rdfs:label>Adult shops</rdfs:label>
    </owl:Class>
    


    <!-- https://www.theworldavatar.com/kg/ontopoi/AdultVenues -->


    <owl:Class rdf:about="https://www.theworldavatar.com/kg/ontopoi/AdultVenues">
        <rdfs:subClassOf rdf:resource="https://www.theworldavatar.com/kg/ontopoi/VenuesAndStageAndScreen"/>
        <rdfs:comment>Adult venues is a subcategory of venues, stage and screen</rdfs:comment>
        <rdfs:isDefinedBy rdf:resource="https://www.theworldavatar.com/kg/ontopoi"/>
        <rdfs:label>Adult venues</rdfs:label>
    </owl:Class>
    


    <!-- https://www.theworldavatar.com/kg/ontopoi/AdvertisingServices -->


    <owl:Class rdf:about="https://www.theworldavatar.com/kg/ontopoi/AdvertisingServices">
        <rdfs:subClassOf rdf:resource="https://www.theworldavatar.com/kg/ontopoi/ItAndAdvertisingAndMarketingAndMediaServiceS"/>
        <rdfs:comment>Advertising services is a subcategory of it, advertising, marketing and media service s</rdfs:comment>
        <rdfs:isDefinedBy rdf:resource="https://www.theworldavatar.com/kg/ontopoi"/>
        <rdfs:label>Advertising services</rdfs:label>
    </owl:Class>
    


    <!-- https://www.theworldavatar.com/kg/ontopoi/Aeroplanes -->


    <owl:Class rdf:about="https://www.theworldavatar.com/kg/ontopoi/Aeroplanes">
        <rdfs:subClassOf rdf:resource="https://www.theworldavatar.com/kg/ontopoi/IndustrialProducts"/>
        <rdfs:comment>Aeroplanes is a subcategory of industrial products</rdfs:comment>
        <rdfs:isDefinedBy rdf:resource="https://www.theworldavatar.com/kg/ontopoi"/>
        <rdfs:label>Aeroplanes</rdfs:label>
    </owl:Class>
    


    <!-- https://www.theworldavatar.com/kg/ontopoi/AgriculturalContractors -->


    <owl:Class rdf:about="https://www.theworldavatar.com/kg/ontopoi/AgriculturalContractors">
        <rdfs:subClassOf rdf:resource="https://www.theworldavatar.com/kg/ontopoi/ContractServices"/>
        <rdfs:comment>Agricultural contractors is a subcategory of contract services</rdfs:comment>
        <rdfs:isDefinedBy rdf:resource="https://www.theworldavatar.com/kg/ontopoi"/>
        <rdfs:label>Agricultural contractors</rdfs:label>
    </owl:Class>
    


    <!-- https://www.theworldavatar.com/kg/ontopoi/AgriculturalMachineryAndGoods -->


    <owl:Class rdf:about="https://www.theworldavatar.com/kg/ontopoi/AgriculturalMachineryAndGoods">
        <rdfs:subClassOf rdf:resource="https://www.theworldavatar.com/kg/ontopoi/IndustrialProducts"/>
        <rdfs:comment>Agricultural machinery and goods is a subcategory of industrial products</rdfs:comment>
        <rdfs:isDefinedBy rdf:resource="https://www.theworldavatar.com/kg/ontopoi"/>
        <rdfs:label>Agricultural machinery and goods</rdfs:label>
    </owl:Class>
    


    <!-- https://www.theworldavatar.com/kg/ontopoi/Air -->


    <owl:Class rdf:about="https://www.theworldavatar.com/kg/ontopoi/Air">
        <rdfs:subClassOf rdf:resource="https://www.theworldavatar.com/kg/ontopoi/Transport"/>
        <rdfs:comment>Air is a subcategory of transport</rdfs:comment>
        <rdfs:isDefinedBy rdf:resource="https://www.theworldavatar.com/kg/ontopoi"/>
        <rdfs:label>Air</rdfs:label>
    </owl:Class>
    


    <!-- https://www.theworldavatar.com/kg/ontopoi/AirAndWaterFiltration -->


    <owl:Class rdf:about="https://www.theworldavatar.com/kg/ontopoi/AirAndWaterFiltration">
        <rdfs:subClassOf rdf:resource="https://www.theworldavatar.com/kg/ontopoi/IndustrialProducts"/>
        <rdfs:comment>Air and water filtration is a subcategory of industrial products</rdfs:comment>
        <rdfs:isDefinedBy rdf:resource="https://www.theworldavatar.com/kg/ontopoi"/>
        <rdfs:label>Air and water filtration</rdfs:label>
    </owl:Class>
    


    <!-- https://www.theworldavatar.com/kg/ontopoi/AircraftCharters -->


    <owl:Class rdf:about="https://www.theworldavatar.com/kg/ontopoi/AircraftCharters">
        <rdfs:subClassOf rdf:resource="https://www.theworldavatar.com/kg/ontopoi/ContractServices"/>
        <rdfs:comment>Aircraft charters is a subcategory of contract services</rdfs:comment>
        <rdfs:isDefinedBy rdf:resource="https://www.theworldavatar.com/kg/ontopoi"/>
        <rdfs:label>Aircraft charters</rdfs:label>
    </owl:Class>
    


    <!-- https://www.theworldavatar.com/kg/ontopoi/AirlinesAndAirlineServices -->


    <owl:Class rdf:about="https://www.theworldavatar.com/kg/ontopoi/AirlinesAndAirlineServices">
        <rdfs:subClassOf rdf:resource="https://www.theworldavatar.com/kg/ontopoi/TransportAndStorageAndDelivery"/>
        <rdfs:comment>Airlines and airline services is a subcategory of transport, storage and delivery</rdfs:comment>
        <rdfs:isDefinedBy rdf:resource="https://www.theworldavatar.com/kg/ontopoi"/>
        <rdfs:label>Airlines and airline services</rdfs:label>
    </owl:Class>
    


    <!-- https://www.theworldavatar.com/kg/ontopoi/AirportsAndLandingStrips -->


    <owl:Class rdf:about="https://www.theworldavatar.com/kg/ontopoi/AirportsAndLandingStrips">
        <rdfs:subClassOf rdf:resource="https://www.theworldavatar.com/kg/ontopoi/Air"/>
        <rdfs:comment>Airports and landing strips is a subcategory of air</rdfs:comment>
        <rdfs:isDefinedBy rdf:resource="https://www.theworldavatar.com/kg/ontopoi"/>
        <rdfs:label>Airports and landing strips</rdfs:label>
    </owl:Class>
    


    <!-- https://www.theworldavatar.com/kg/ontopoi/AlcoholicDrinks -->


    <owl:Class rdf:about="https://www.theworldavatar.com/kg/ontopoi/AlcoholicDrinks">
        <rdfs:subClassOf rdf:resource="https://www.theworldavatar.com/kg/ontopoi/Foodstuffs"/>
        <rdfs:comment>Alcoholic drinks is a subcategory of foodstuffs</rdfs:comment>
        <rdfs:isDefinedBy rdf:resource="https://www.theworldavatar.com/kg/ontopoi"/>
        <rdfs:label>Alcoholic drinks</rdfs:label>
    </owl:Class>
    


    <!-- https://www.theworldavatar.com/kg/ontopoi/AlcoholicDrinksIncludingOff-LicencesAndWholesalers -->


    <owl:Class rdf:about="https://www.theworldavatar.com/kg/ontopoi/AlcoholicDrinksIncludingOff-LicencesAndWholesalers">
        <rdfs:subClassOf rdf:resource="https://www.theworldavatar.com/kg/ontopoi/FoodAndDrinkAndMultiItemRetail"/>
        <rdfs:comment>Alcoholic drinks including off-licences and wholesalers is a subcategory of food, drink and multi item retail</rdfs:comment>
        <rdfs:isDefinedBy rdf:resource="https://www.theworldavatar.com/kg/ontopoi"/>
        <rdfs:label>Alcoholic drinks including off-licences and wholesalers</rdfs:label>
    </owl:Class>
    


    <!-- https://www.theworldavatar.com/kg/ontopoi/Allotments -->


    <owl:Class rdf:about="https://www.theworldavatar.com/kg/ontopoi/Allotments">
        <rdfs:subClassOf rdf:resource="https://www.theworldavatar.com/kg/ontopoi/InfrastructureAndFacilities"/>
        <rdfs:comment>Allotments is a subcategory of infrastructure and facilities</rdfs:comment>
        <rdfs:isDefinedBy rdf:resource="https://www.theworldavatar.com/kg/ontopoi"/>
        <rdfs:label>Allotments</rdfs:label>
    </owl:Class>
    


    <!-- https://www.theworldavatar.com/kg/ontopoi/AlternativeAndNaturalAndComplementary -->


    <owl:Class rdf:about="https://www.theworldavatar.com/kg/ontopoi/AlternativeAndNaturalAndComplementary">
        <rdfs:subClassOf rdf:resource="https://www.theworldavatar.com/kg/ontopoi/HealthPractitionersAndEstablishments"/>
        <rdfs:comment>Alternative, natural and complementary is a subcategory of health practitioners and establishments</rdfs:comment>
        <rdfs:isDefinedBy rdf:resource="https://www.theworldavatar.com/kg/ontopoi"/>
        <rdfs:label>Alternative, natural and complementary</rdfs:label>
    </owl:Class>
    


    <!-- https://www.theworldavatar.com/kg/ontopoi/AmbulanceAndMedicalTransportationServices -->


    <owl:Class rdf:about="https://www.theworldavatar.com/kg/ontopoi/AmbulanceAndMedicalTransportationServices">
        <rdfs:subClassOf rdf:resource="https://www.theworldavatar.com/kg/ontopoi/HealthSupportServices"/>
        <rdfs:comment>Ambulance and medical transportation services is a subcategory of health support services</rdfs:comment>
        <rdfs:isDefinedBy rdf:resource="https://www.theworldavatar.com/kg/ontopoi"/>
        <rdfs:label>Ambulance and medical transportation services</rdfs:label>
    </owl:Class>
    


    <!-- https://www.theworldavatar.com/kg/ontopoi/AmusementParksAndArcades -->


    <owl:Class rdf:about="https://www.theworldavatar.com/kg/ontopoi/AmusementParksAndArcades">
        <rdfs:subClassOf rdf:resource="https://www.theworldavatar.com/kg/ontopoi/Gambling"/>
        <rdfs:comment>Amusement parks and arcades is a subcategory of gambling</rdfs:comment>
        <rdfs:isDefinedBy rdf:resource="https://www.theworldavatar.com/kg/ontopoi"/>
        <rdfs:label>Amusement parks and arcades</rdfs:label>
    </owl:Class>
    


    <!-- https://www.theworldavatar.com/kg/ontopoi/AnglingAndSportsFishing -->


    <owl:Class rdf:about="https://www.theworldavatar.com/kg/ontopoi/AnglingAndSportsFishing">
        <rdfs:subClassOf rdf:resource="https://www.theworldavatar.com/kg/ontopoi/OutdoorPursuits"/>
        <rdfs:comment>Angling and sports fishing is a subcategory of outdoor pursuits</rdfs:comment>
        <rdfs:isDefinedBy rdf:resource="https://www.theworldavatar.com/kg/ontopoi"/>
        <rdfs:label>Angling and sports fishing</rdfs:label>
    </owl:Class>
    


    <!-- https://www.theworldavatar.com/kg/ontopoi/AnimalClippingAndGrooming -->


    <owl:Class rdf:about="https://www.theworldavatar.com/kg/ontopoi/AnimalClippingAndGrooming">
        <rdfs:subClassOf rdf:resource="https://www.theworldavatar.com/kg/ontopoi/AnimalWelfare"/>
        <rdfs:comment>Animal clipping and grooming is a subcategory of animal welfare</rdfs:comment>
        <rdfs:isDefinedBy rdf:resource="https://www.theworldavatar.com/kg/ontopoi"/>
        <rdfs:label>Animal clipping and grooming</rdfs:label>
    </owl:Class>
    


    <!-- https://www.theworldavatar.com/kg/ontopoi/AnimalFeedsAndPetFoodsAndHayAndStraw -->


    <owl:Class rdf:about="https://www.theworldavatar.com/kg/ontopoi/AnimalFeedsAndPetFoodsAndHayAndStraw">
        <rdfs:subClassOf rdf:resource="https://www.theworldavatar.com/kg/ontopoi/Foodstuffs"/>
        <rdfs:comment>Animal feeds, pet foods, hay and straw is a subcategory of foodstuffs</rdfs:comment>
        <rdfs:isDefinedBy rdf:resource="https://www.theworldavatar.com/kg/ontopoi"/>
        <rdfs:label>Animal feeds, pet foods, hay and straw</rdfs:label>
    </owl:Class>
    


    <!-- https://www.theworldavatar.com/kg/ontopoi/AnimalTransportation -->


    <owl:Class rdf:about="https://www.theworldavatar.com/kg/ontopoi/AnimalTransportation">
        <rdfs:subClassOf rdf:resource="https://www.theworldavatar.com/kg/ontopoi/TransportAndStorageAndDelivery"/>
        <rdfs:comment>Animal transportation is a subcategory of transport, storage and delivery</rdfs:comment>
        <rdfs:isDefinedBy rdf:resource="https://www.theworldavatar.com/kg/ontopoi"/>
        <rdfs:label>Animal transportation</rdfs:label>
    </owl:Class>
    


    <!-- https://www.theworldavatar.com/kg/ontopoi/AnimalWelfare -->


    <owl:Class rdf:about="https://www.theworldavatar.com/kg/ontopoi/AnimalWelfare">
        <rdfs:subClassOf rdf:resource="https://www.theworldavatar.com/kg/ontopoi/EducationAndHealth"/>
        <rdfs:comment>Animal welfare is a subcategory of education and health</rdfs:comment>
        <rdfs:isDefinedBy rdf:resource="https://www.theworldavatar.com/kg/ontopoi"/>
        <rdfs:label>Animal welfare</rdfs:label>
    </owl:Class>
    


    <!-- https://www.theworldavatar.com/kg/ontopoi/AnimalWelfareOrganisations -->


    <owl:Class rdf:about="https://www.theworldavatar.com/kg/ontopoi/AnimalWelfareOrganisations">
        <rdfs:subClassOf rdf:resource="https://www.theworldavatar.com/kg/ontopoi/Organisations"/>
        <rdfs:comment>Animal welfare organisations is a subcategory of organisations</rdfs:comment>
        <rdfs:isDefinedBy rdf:resource="https://www.theworldavatar.com/kg/ontopoi"/>
        <rdfs:label>Animal welfare organisations</rdfs:label>
    </owl:Class>
    


    <!-- https://www.theworldavatar.com/kg/ontopoi/AquariaAndSeaLifeCentres -->


    <owl:Class rdf:about="https://www.theworldavatar.com/kg/ontopoi/AquariaAndSeaLifeCentres">
        <rdfs:subClassOf rdf:resource="https://www.theworldavatar.com/kg/ontopoi/BotanicalAndZoological"/>
        <rdfs:comment>Aquaria and sea life centres is a subcategory of botanical and zoological</rdfs:comment>
        <rdfs:isDefinedBy rdf:resource="https://www.theworldavatar.com/kg/ontopoi"/>
        <rdfs:label>Aquaria and sea life centres</rdfs:label>
    </owl:Class>
    


    <!-- https://www.theworldavatar.com/kg/ontopoi/Aqueducts -->


    <owl:Class rdf:about="https://www.theworldavatar.com/kg/ontopoi/Aqueducts">
        <rdfs:subClassOf rdf:resource="https://www.theworldavatar.com/kg/ontopoi/Water"/>
        <rdfs:comment>Aqueducts is a subcategory of water</rdfs:comment>
        <rdfs:isDefinedBy rdf:resource="https://www.theworldavatar.com/kg/ontopoi"/>
        <rdfs:label>Aqueducts</rdfs:label>
    </owl:Class>
    


    <!-- https://www.theworldavatar.com/kg/ontopoi/ArableFarming -->


    <owl:Class rdf:about="https://www.theworldavatar.com/kg/ontopoi/ArableFarming">
        <rdfs:subClassOf rdf:resource="https://www.theworldavatar.com/kg/ontopoi/Farming"/>
        <rdfs:comment>Arable farming is a subcategory of farming</rdfs:comment>
        <rdfs:isDefinedBy rdf:resource="https://www.theworldavatar.com/kg/ontopoi"/>
        <rdfs:label>Arable farming</rdfs:label>
    </owl:Class>
    


    <!-- https://www.theworldavatar.com/kg/ontopoi/ArchaeologicalSites -->


    <owl:Class rdf:about="https://www.theworldavatar.com/kg/ontopoi/ArchaeologicalSites">
        <rdfs:subClassOf rdf:resource="https://www.theworldavatar.com/kg/ontopoi/HistoricalAndCultural"/>
        <rdfs:comment>Archaeological sites is a subcategory of historical and cultural</rdfs:comment>
        <rdfs:isDefinedBy rdf:resource="https://www.theworldavatar.com/kg/ontopoi"/>
        <rdfs:label>Archaeological sites</rdfs:label>
    </owl:Class>
    


    <!-- https://www.theworldavatar.com/kg/ontopoi/ArchitecturalAndBuilding-RelatedConsultants -->


    <owl:Class rdf:about="https://www.theworldavatar.com/kg/ontopoi/ArchitecturalAndBuilding-RelatedConsultants">
        <rdfs:subClassOf rdf:resource="https://www.theworldavatar.com/kg/ontopoi/Consultancies"/>
        <rdfs:comment>Architectural and building-related consultants is a subcategory of consultancies</rdfs:comment>
        <rdfs:isDefinedBy rdf:resource="https://www.theworldavatar.com/kg/ontopoi"/>
        <rdfs:label>Architectural and building-related consultants</rdfs:label>
    </owl:Class>
    


    <!-- https://www.theworldavatar.com/kg/ontopoi/ArmedServices -->


    <owl:Class rdf:about="https://www.theworldavatar.com/kg/ontopoi/ArmedServices">
        <rdfs:subClassOf rdf:resource="https://www.theworldavatar.com/kg/ontopoi/CentralAndLocalGovernment"/>
        <rdfs:comment>Armed services is a subcategory of central and local government</rdfs:comment>
        <rdfs:isDefinedBy rdf:resource="https://www.theworldavatar.com/kg/ontopoi"/>
        <rdfs:label>Armed services</rdfs:label>
    </owl:Class>
    


    <!-- https://www.theworldavatar.com/kg/ontopoi/ArmsAndAmmunition -->


    <owl:Class rdf:about="https://www.theworldavatar.com/kg/ontopoi/ArmsAndAmmunition">
        <rdfs:subClassOf rdf:resource="https://www.theworldavatar.com/kg/ontopoi/IndustrialProducts"/>
        <rdfs:comment>Arms and ammunition is a subcategory of industrial products</rdfs:comment>
        <rdfs:isDefinedBy rdf:resource="https://www.theworldavatar.com/kg/ontopoi"/>
        <rdfs:label>Arms and ammunition</rdfs:label>
    </owl:Class>
    


    <!-- https://www.theworldavatar.com/kg/ontopoi/ArtAndAntiques -->


    <owl:Class rdf:about="https://www.theworldavatar.com/kg/ontopoi/ArtAndAntiques">
        <rdfs:subClassOf rdf:resource="https://www.theworldavatar.com/kg/ontopoi/HouseholdAndOfficeAndLeisureAndGarden"/>
        <rdfs:comment>Art and antiques is a subcategory of household, office, leisure and garden</rdfs:comment>
        <rdfs:isDefinedBy rdf:resource="https://www.theworldavatar.com/kg/ontopoi"/>
        <rdfs:label>Art and antiques</rdfs:label>
    </owl:Class>
    


    <!-- https://www.theworldavatar.com/kg/ontopoi/ArtGalleries -->


    <owl:Class rdf:about="https://www.theworldavatar.com/kg/ontopoi/ArtGalleries">
        <rdfs:subClassOf rdf:resource="https://www.theworldavatar.com/kg/ontopoi/HistoricalAndCultural"/>
        <rdfs:comment>Art galleries is a subcategory of historical and cultural</rdfs:comment>
        <rdfs:isDefinedBy rdf:resource="https://www.theworldavatar.com/kg/ontopoi"/>
        <rdfs:label>Art galleries</rdfs:label>
    </owl:Class>
    


    <!-- https://www.theworldavatar.com/kg/ontopoi/ArtistsAndIllustratorsAndCalligraphers -->


    <owl:Class rdf:about="https://www.theworldavatar.com/kg/ontopoi/ArtistsAndIllustratorsAndCalligraphers">
        <rdfs:subClassOf rdf:resource="https://www.theworldavatar.com/kg/ontopoi/ItAndAdvertisingAndMarketingAndMediaServiceS"/>
        <rdfs:comment>Artists, illustrators and calligraphers is a subcategory of it, advertising, marketing and media service s</rdfs:comment>
        <rdfs:isDefinedBy rdf:resource="https://www.theworldavatar.com/kg/ontopoi"/>
        <rdfs:label>Artists, illustrators and calligraphers</rdfs:label>
    </owl:Class>
    


    <!-- https://www.theworldavatar.com/kg/ontopoi/AstrologersAndClairvoyantsAndPalmists -->


    <owl:Class rdf:about="https://www.theworldavatar.com/kg/ontopoi/AstrologersAndClairvoyantsAndPalmists">
        <rdfs:subClassOf rdf:resource="https://www.theworldavatar.com/kg/ontopoi/PersonalAndConsumerAndOtherServices"/>
        <rdfs:comment>Astrologers, clairvoyants and palmists is a subcategory of personal, consumer and other services</rdfs:comment>
        <rdfs:isDefinedBy rdf:resource="https://www.theworldavatar.com/kg/ontopoi"/>
        <rdfs:label>Astrologers, clairvoyants and palmists</rdfs:label>
    </owl:Class>
    


    <!-- https://www.theworldavatar.com/kg/ontopoi/AthleticsFacilities -->


    <owl:Class rdf:about="https://www.theworldavatar.com/kg/ontopoi/AthleticsFacilities">
        <rdfs:subClassOf rdf:resource="https://www.theworldavatar.com/kg/ontopoi/SportsComplex"/>
        <rdfs:comment>Athletics facilities is a subcategory of sports complex</rdfs:comment>
        <rdfs:isDefinedBy rdf:resource="https://www.theworldavatar.com/kg/ontopoi"/>
        <rdfs:label>Athletics facilities</rdfs:label>
    </owl:Class>
    


    <!-- https://www.theworldavatar.com/kg/ontopoi/Attractions -->


    <owl:Class rdf:about="https://www.theworldavatar.com/kg/ontopoi/Attractions">
        <rdfs:subClassOf rdf:resource="https://www.theworldavatar.com/kg/ontopoi/PointOfInterest"/>
        <rdfs:comment>Places or sites that draw the attention of visitors, offering entertainment, education, or cultural value</rdfs:comment>
        <rdfs:isDefinedBy rdf:resource="https://www.theworldavatar.com/kg/ontopoi"/>
        <rdfs:label>Attractions</rdfs:label>
    </owl:Class>
    


    <!-- https://www.theworldavatar.com/kg/ontopoi/AuctioneersAndAuctionRoomsAndValuers -->


    <owl:Class rdf:about="https://www.theworldavatar.com/kg/ontopoi/AuctioneersAndAuctionRoomsAndValuers">
        <rdfs:subClassOf rdf:resource="https://www.theworldavatar.com/kg/ontopoi/LegalAndFinancial"/>
        <rdfs:comment>Auctioneers, auction rooms and valuers is a subcategory of legal and financial</rdfs:comment>
        <rdfs:isDefinedBy rdf:resource="https://www.theworldavatar.com/kg/ontopoi"/>
        <rdfs:label>Auctioneers, auction rooms and valuers</rdfs:label>
    </owl:Class>
    


    <!-- https://www.theworldavatar.com/kg/ontopoi/AviationEngineers -->


    <owl:Class rdf:about="https://www.theworldavatar.com/kg/ontopoi/AviationEngineers">
        <rdfs:subClassOf rdf:resource="https://www.theworldavatar.com/kg/ontopoi/EngineeringServices"/>
        <rdfs:comment>Aviation engineers is a subcategory of engineering services</rdfs:comment>
        <rdfs:isDefinedBy rdf:resource="https://www.theworldavatar.com/kg/ontopoi"/>
        <rdfs:label>Aviation engineers</rdfs:label>
    </owl:Class>
    


    <!-- https://www.theworldavatar.com/kg/ontopoi/BabyAndNurseryAndPlaygroundEquipment -->


    <owl:Class rdf:about="https://www.theworldavatar.com/kg/ontopoi/BabyAndNurseryAndPlaygroundEquipment">
        <rdfs:subClassOf rdf:resource="https://www.theworldavatar.com/kg/ontopoi/ConsumerProducts"/>
        <rdfs:comment>Baby, nursery and playground equipment is a subcategory of consumer products</rdfs:comment>
        <rdfs:isDefinedBy rdf:resource="https://www.theworldavatar.com/kg/ontopoi"/>
        <rdfs:label>Baby, nursery and playground equipment</rdfs:label>
    </owl:Class>
    


    <!-- https://www.theworldavatar.com/kg/ontopoi/BabyAndNurseryEquipmentAndChildrenClothes -->


    <owl:Class rdf:about="https://www.theworldavatar.com/kg/ontopoi/BabyAndNurseryEquipmentAndChildrenClothes">
        <rdfs:subClassOf rdf:resource="https://www.theworldavatar.com/kg/ontopoi/ClothingAndAccessories"/>
        <rdfs:comment>Baby and nursery equipment and children&apos;s clothes is a subcategory of clothing and accessories</rdfs:comment>
        <rdfs:isDefinedBy rdf:resource="https://www.theworldavatar.com/kg/ontopoi"/>
        <rdfs:label>Baby and nursery equipment and children&apos;s clothes</rdfs:label>
    </owl:Class>
    


    <!-- https://www.theworldavatar.com/kg/ontopoi/Bakeries -->


    <owl:Class rdf:about="https://www.theworldavatar.com/kg/ontopoi/Bakeries">
        <rdfs:subClassOf rdf:resource="https://www.theworldavatar.com/kg/ontopoi/FoodAndDrinkAndMultiItemRetail"/>
        <rdfs:comment>Bakeries is a subcategory of food, drink and multi item retail</rdfs:comment>
        <rdfs:isDefinedBy rdf:resource="https://www.theworldavatar.com/kg/ontopoi"/>
        <rdfs:label>Bakeries</rdfs:label>
    </owl:Class>
    


    <!-- https://www.theworldavatar.com/kg/ontopoi/BakingAndConfectionery -->


    <owl:Class rdf:about="https://www.theworldavatar.com/kg/ontopoi/BakingAndConfectionery">
        <rdfs:subClassOf rdf:resource="https://www.theworldavatar.com/kg/ontopoi/Foodstuffs"/>
        <rdfs:comment>Baking and confectionery is a subcategory of foodstuffs</rdfs:comment>
        <rdfs:isDefinedBy rdf:resource="https://www.theworldavatar.com/kg/ontopoi"/>
        <rdfs:label>Baking and confectionery</rdfs:label>
    </owl:Class>
    


    <!-- https://www.theworldavatar.com/kg/ontopoi/BalletAndDanceSchools -->


    <owl:Class rdf:about="https://www.theworldavatar.com/kg/ontopoi/BalletAndDanceSchools">
        <rdfs:subClassOf rdf:resource="https://www.theworldavatar.com/kg/ontopoi/RecreationalAndVocationalEducation"/>
        <rdfs:comment>Ballet and dance schools is a subcategory of recreational and vocational education</rdfs:comment>
        <rdfs:isDefinedBy rdf:resource="https://www.theworldavatar.com/kg/ontopoi"/>
        <rdfs:label>Ballet and dance schools</rdfs:label>
    </owl:Class>
    


    <!-- https://www.theworldavatar.com/kg/ontopoi/BanksAndBuildingSocieties -->


    <owl:Class rdf:about="https://www.theworldavatar.com/kg/ontopoi/BanksAndBuildingSocieties">
        <rdfs:subClassOf rdf:resource="https://www.theworldavatar.com/kg/ontopoi/LegalAndFinancial"/>
        <rdfs:comment>Banks and building societies is a subcategory of legal and financial</rdfs:comment>
        <rdfs:isDefinedBy rdf:resource="https://www.theworldavatar.com/kg/ontopoi"/>
        <rdfs:label>Banks and building societies</rdfs:label>
    </owl:Class>
    


    <!-- https://www.theworldavatar.com/kg/ontopoi/BanquetingAndFunctionRooms -->


    <owl:Class rdf:about="https://www.theworldavatar.com/kg/ontopoi/BanquetingAndFunctionRooms">
        <rdfs:subClassOf rdf:resource="https://www.theworldavatar.com/kg/ontopoi/EatingAndDrinking"/>
        <rdfs:comment>Banqueting and function rooms is a subcategory of eating and drinking</rdfs:comment>
        <rdfs:isDefinedBy rdf:resource="https://www.theworldavatar.com/kg/ontopoi"/>
        <rdfs:label>Banqueting and function rooms</rdfs:label>
    </owl:Class>
    


    <!-- https://www.theworldavatar.com/kg/ontopoi/BathroomFixturesAndFittingsAndSanitaryEquipment -->


    <owl:Class rdf:about="https://www.theworldavatar.com/kg/ontopoi/BathroomFixturesAndFittingsAndSanitaryEquipment">
        <rdfs:subClassOf rdf:resource="https://www.theworldavatar.com/kg/ontopoi/ConsumerProducts"/>
        <rdfs:comment>Bathroom fixtures, fittings and sanitary equipment is a subcategory of consumer products</rdfs:comment>
        <rdfs:isDefinedBy rdf:resource="https://www.theworldavatar.com/kg/ontopoi"/>
        <rdfs:label>Bathroom fixtures, fittings and sanitary equipment</rdfs:label>
    </owl:Class>
    


    <!-- https://www.theworldavatar.com/kg/ontopoi/Battlefields -->


    <owl:Class rdf:about="https://www.theworldavatar.com/kg/ontopoi/Battlefields">
        <rdfs:subClassOf rdf:resource="https://www.theworldavatar.com/kg/ontopoi/HistoricalAndCultural"/>
        <rdfs:comment>Battlefields is a subcategory of historical and cultural</rdfs:comment>
        <rdfs:isDefinedBy rdf:resource="https://www.theworldavatar.com/kg/ontopoi"/>
        <rdfs:label>Battlefields</rdfs:label>
    </owl:Class>
    


    <!-- https://www.theworldavatar.com/kg/ontopoi/BearingAndGearAndDriveElements -->


    <owl:Class rdf:about="https://www.theworldavatar.com/kg/ontopoi/BearingAndGearAndDriveElements">
        <rdfs:subClassOf rdf:resource="https://www.theworldavatar.com/kg/ontopoi/IndustrialProducts"/>
        <rdfs:comment>Bearing, gear and drive elements is a subcategory of industrial products</rdfs:comment>
        <rdfs:isDefinedBy rdf:resource="https://www.theworldavatar.com/kg/ontopoi"/>
        <rdfs:label>Bearing, gear and drive elements</rdfs:label>
    </owl:Class>
    


    <!-- https://www.theworldavatar.com/kg/ontopoi/BeautyAndHairdressingSchools -->


    <owl:Class rdf:about="https://www.theworldavatar.com/kg/ontopoi/BeautyAndHairdressingSchools">
        <rdfs:subClassOf rdf:resource="https://www.theworldavatar.com/kg/ontopoi/RecreationalAndVocationalEducation"/>
        <rdfs:comment>Beauty and hairdressing schools is a subcategory of recreational and vocational education</rdfs:comment>
        <rdfs:isDefinedBy rdf:resource="https://www.theworldavatar.com/kg/ontopoi"/>
        <rdfs:label>Beauty and hairdressing schools</rdfs:label>
    </owl:Class>
    


    <!-- https://www.theworldavatar.com/kg/ontopoi/BedAndBreakfastAndBackpackerAccommodation -->


    <owl:Class rdf:about="https://www.theworldavatar.com/kg/ontopoi/BedAndBreakfastAndBackpackerAccommodation">
        <rdfs:subClassOf rdf:resource="https://www.theworldavatar.com/kg/ontopoi/Accommodation"/>
        <rdfs:comment>Bed and breakfast and backpacker accommodation is a subcategory of accommodation</rdfs:comment>
        <rdfs:isDefinedBy rdf:resource="https://www.theworldavatar.com/kg/ontopoi"/>
        <rdfs:label>Bed and breakfast and backpacker accommodation</rdfs:label>
    </owl:Class>
    


    <!-- https://www.theworldavatar.com/kg/ontopoi/BedsAndBedding -->


    <owl:Class rdf:about="https://www.theworldavatar.com/kg/ontopoi/BedsAndBedding">
        <rdfs:subClassOf rdf:resource="https://www.theworldavatar.com/kg/ontopoi/ConsumerProducts"/>
        <rdfs:comment>Beds and bedding is a subcategory of consumer products</rdfs:comment>
        <rdfs:isDefinedBy rdf:resource="https://www.theworldavatar.com/kg/ontopoi"/>
        <rdfs:label>Beds and bedding</rdfs:label>
    </owl:Class>
    


    <!-- https://www.theworldavatar.com/kg/ontopoi/Bee-Keepers -->


    <owl:Class rdf:about="https://www.theworldavatar.com/kg/ontopoi/Bee-Keepers">
        <rdfs:subClassOf rdf:resource="https://www.theworldavatar.com/kg/ontopoi/Farming"/>
        <rdfs:comment>Bee-keepers is a subcategory of farming</rdfs:comment>
        <rdfs:isDefinedBy rdf:resource="https://www.theworldavatar.com/kg/ontopoi"/>
        <rdfs:label>Bee-keepers</rdfs:label>
    </owl:Class>
    


    <!-- https://www.theworldavatar.com/kg/ontopoi/Bee-KeepingSupplies -->


    <owl:Class rdf:about="https://www.theworldavatar.com/kg/ontopoi/Bee-KeepingSupplies">
        <rdfs:subClassOf rdf:resource="https://www.theworldavatar.com/kg/ontopoi/IndustrialProducts"/>
        <rdfs:comment>Bee-keeping supplies is a subcategory of industrial products</rdfs:comment>
        <rdfs:isDefinedBy rdf:resource="https://www.theworldavatar.com/kg/ontopoi"/>
        <rdfs:label>Bee-keeping supplies</rdfs:label>
    </owl:Class>
    


    <!-- https://www.theworldavatar.com/kg/ontopoi/BingoHalls -->


    <owl:Class rdf:about="https://www.theworldavatar.com/kg/ontopoi/BingoHalls">
        <rdfs:subClassOf rdf:resource="https://www.theworldavatar.com/kg/ontopoi/Gambling"/>
        <rdfs:comment>Bingo halls is a subcategory of gambling</rdfs:comment>
        <rdfs:isDefinedBy rdf:resource="https://www.theworldavatar.com/kg/ontopoi"/>
        <rdfs:label>Bingo halls</rdfs:label>
    </owl:Class>
    


    <!-- https://www.theworldavatar.com/kg/ontopoi/BirdReservesAndCollectionsAndSanctuaries -->


    <owl:Class rdf:about="https://www.theworldavatar.com/kg/ontopoi/BirdReservesAndCollectionsAndSanctuaries">
        <rdfs:subClassOf rdf:resource="https://www.theworldavatar.com/kg/ontopoi/BotanicalAndZoological"/>
        <rdfs:comment>Bird reserves, collections and sanctuaries is a subcategory of botanical and zoological</rdfs:comment>
        <rdfs:isDefinedBy rdf:resource="https://www.theworldavatar.com/kg/ontopoi"/>
        <rdfs:label>Bird reserves, collections and sanctuaries</rdfs:label>
    </owl:Class>
    


    <!-- https://www.theworldavatar.com/kg/ontopoi/BloodTransfusionService -->


    <owl:Class rdf:about="https://www.theworldavatar.com/kg/ontopoi/BloodTransfusionService">
        <rdfs:subClassOf rdf:resource="https://www.theworldavatar.com/kg/ontopoi/HealthSupportServices"/>
        <rdfs:comment>Blood transfusion service is a subcategory of health support services</rdfs:comment>
        <rdfs:isDefinedBy rdf:resource="https://www.theworldavatar.com/kg/ontopoi"/>
        <rdfs:label>Blood transfusion service</rdfs:label>
    </owl:Class>
    


    <!-- https://www.theworldavatar.com/kg/ontopoi/BoatHiringServices -->


    <owl:Class rdf:about="https://www.theworldavatar.com/kg/ontopoi/BoatHiringServices">
        <rdfs:subClassOf rdf:resource="https://www.theworldavatar.com/kg/ontopoi/HireServices"/>
        <rdfs:comment>Boat hiring services is a subcategory of hire services</rdfs:comment>
        <rdfs:isDefinedBy rdf:resource="https://www.theworldavatar.com/kg/ontopoi"/>
        <rdfs:label>Boat hiring services</rdfs:label>
    </owl:Class>
    


    <!-- https://www.theworldavatar.com/kg/ontopoi/BodiesOfWater -->


    <owl:Class rdf:about="https://www.theworldavatar.com/kg/ontopoi/BodiesOfWater">
        <rdfs:subClassOf rdf:resource="https://www.theworldavatar.com/kg/ontopoi/Attractions"/>
        <rdfs:comment>Bodies of water is a subcategory of attractions</rdfs:comment>
        <rdfs:isDefinedBy rdf:resource="https://www.theworldavatar.com/kg/ontopoi"/>
        <rdfs:label>Bodies of water</rdfs:label>
    </owl:Class>
    


    <!-- https://www.theworldavatar.com/kg/ontopoi/Bookmakers -->


    <owl:Class rdf:about="https://www.theworldavatar.com/kg/ontopoi/Bookmakers">
        <rdfs:subClassOf rdf:resource="https://www.theworldavatar.com/kg/ontopoi/Gambling"/>
        <rdfs:comment>Bookmakers is a subcategory of gambling</rdfs:comment>
        <rdfs:isDefinedBy rdf:resource="https://www.theworldavatar.com/kg/ontopoi"/>
        <rdfs:label>Bookmakers</rdfs:label>
    </owl:Class>
    


    <!-- https://www.theworldavatar.com/kg/ontopoi/BooksAndMaps -->


    <owl:Class rdf:about="https://www.theworldavatar.com/kg/ontopoi/BooksAndMaps">
        <rdfs:subClassOf rdf:resource="https://www.theworldavatar.com/kg/ontopoi/HouseholdAndOfficeAndLeisureAndGarden"/>
        <rdfs:comment>Books and maps is a subcategory of household, office, leisure and garden</rdfs:comment>
        <rdfs:isDefinedBy rdf:resource="https://www.theworldavatar.com/kg/ontopoi"/>
        <rdfs:label>Books and maps</rdfs:label>
    </owl:Class>
    


    <!-- https://www.theworldavatar.com/kg/ontopoi/BotanicalAndZoological -->


    <owl:Class rdf:about="https://www.theworldavatar.com/kg/ontopoi/BotanicalAndZoological">
        <rdfs:subClassOf rdf:resource="https://www.theworldavatar.com/kg/ontopoi/Attractions"/>
        <rdfs:comment>Botanical and zoological is a subcategory of attractions</rdfs:comment>
        <rdfs:isDefinedBy rdf:resource="https://www.theworldavatar.com/kg/ontopoi"/>
        <rdfs:label>Botanical and zoological</rdfs:label>
    </owl:Class>
    


    <!-- https://www.theworldavatar.com/kg/ontopoi/BouncyCastlesAndInflatablesHire -->


    <owl:Class rdf:about="https://www.theworldavatar.com/kg/ontopoi/BouncyCastlesAndInflatablesHire">
        <rdfs:subClassOf rdf:resource="https://www.theworldavatar.com/kg/ontopoi/HireServices"/>
        <rdfs:comment>Bouncy castles and inflatables hire is a subcategory of hire services</rdfs:comment>
        <rdfs:isDefinedBy rdf:resource="https://www.theworldavatar.com/kg/ontopoi"/>
        <rdfs:label>Bouncy castles and inflatables hire</rdfs:label>
    </owl:Class>
    


    <!-- https://www.theworldavatar.com/kg/ontopoi/BowlingFacilities -->


    <owl:Class rdf:about="https://www.theworldavatar.com/kg/ontopoi/BowlingFacilities">
        <rdfs:subClassOf rdf:resource="https://www.theworldavatar.com/kg/ontopoi/SportsComplex"/>
        <rdfs:comment>Bowling facilities is a subcategory of sports complex</rdfs:comment>
        <rdfs:isDefinedBy rdf:resource="https://www.theworldavatar.com/kg/ontopoi"/>
        <rdfs:label>Bowling facilities</rdfs:label>
    </owl:Class>
    


    <!-- https://www.theworldavatar.com/kg/ontopoi/BricksAndTilesAndClayAndCeramicProducts -->


    <owl:Class rdf:about="https://www.theworldavatar.com/kg/ontopoi/BricksAndTilesAndClayAndCeramicProducts">
        <rdfs:subClassOf rdf:resource="https://www.theworldavatar.com/kg/ontopoi/IndustrialProducts"/>
        <rdfs:comment>Bricks, tiles, clay and ceramic products is a subcategory of industrial products</rdfs:comment>
        <rdfs:isDefinedBy rdf:resource="https://www.theworldavatar.com/kg/ontopoi"/>
        <rdfs:label>Bricks, tiles, clay and ceramic products</rdfs:label>
    </owl:Class>
    


    <!-- https://www.theworldavatar.com/kg/ontopoi/Bridges -->


    <owl:Class rdf:about="https://www.theworldavatar.com/kg/ontopoi/Bridges">
        <rdfs:subClassOf rdf:resource="https://www.theworldavatar.com/kg/ontopoi/RoadAndRail"/>
        <rdfs:comment>Bridges is a subcategory of road and rail</rdfs:comment>
        <rdfs:isDefinedBy rdf:resource="https://www.theworldavatar.com/kg/ontopoi"/>
        <rdfs:label>Bridges</rdfs:label>
    </owl:Class>
    


    <!-- https://www.theworldavatar.com/kg/ontopoi/BroadAgeRangeAndSecondaryStateSchools -->


    <owl:Class rdf:about="https://www.theworldavatar.com/kg/ontopoi/BroadAgeRangeAndSecondaryStateSchools">
        <rdfs:subClassOf rdf:resource="https://www.theworldavatar.com/kg/ontopoi/PrimaryAndSecondaryAndTertiaryEducation"/>
        <rdfs:comment>Broad age range and secondary state schools is a subcategory of primary, secondary and tertiary education</rdfs:comment>
        <rdfs:isDefinedBy rdf:resource="https://www.theworldavatar.com/kg/ontopoi"/>
        <rdfs:label>Broad age range and secondary state schools</rdfs:label>
    </owl:Class>
    


    <!-- https://www.theworldavatar.com/kg/ontopoi/Brushes -->


    <owl:Class rdf:about="https://www.theworldavatar.com/kg/ontopoi/Brushes">
        <rdfs:subClassOf rdf:resource="https://www.theworldavatar.com/kg/ontopoi/ConsumerProducts"/>
        <rdfs:comment>Brushes is a subcategory of consumer products</rdfs:comment>
        <rdfs:isDefinedBy rdf:resource="https://www.theworldavatar.com/kg/ontopoi"/>
        <rdfs:label>Brushes</rdfs:label>
    </owl:Class>
    


    <!-- https://www.theworldavatar.com/kg/ontopoi/BuildingAndComponentSuppliers -->


    <owl:Class rdf:about="https://www.theworldavatar.com/kg/ontopoi/BuildingAndComponentSuppliers">
        <rdfs:subClassOf rdf:resource="https://www.theworldavatar.com/kg/ontopoi/ConstructionServices"/>
        <rdfs:comment>Building and component suppliers is a subcategory of construction services</rdfs:comment>
        <rdfs:isDefinedBy rdf:resource="https://www.theworldavatar.com/kg/ontopoi"/>
        <rdfs:label>Building and component suppliers</rdfs:label>
    </owl:Class>
    


    <!-- https://www.theworldavatar.com/kg/ontopoi/BuildingContractors -->


    <owl:Class rdf:about="https://www.theworldavatar.com/kg/ontopoi/BuildingContractors">
        <rdfs:subClassOf rdf:resource="https://www.theworldavatar.com/kg/ontopoi/ConstructionServices"/>
        <rdfs:comment>Building contractors is a subcategory of construction services</rdfs:comment>
        <rdfs:isDefinedBy rdf:resource="https://www.theworldavatar.com/kg/ontopoi"/>
        <rdfs:label>Building contractors</rdfs:label>
    </owl:Class>
    


    <!-- https://www.theworldavatar.com/kg/ontopoi/BuildingRepairs -->


    <owl:Class rdf:about="https://www.theworldavatar.com/kg/ontopoi/BuildingRepairs">
        <rdfs:subClassOf rdf:resource="https://www.theworldavatar.com/kg/ontopoi/RepairAndServicing"/>
        <rdfs:comment>Building repairs is a subcategory of repair and servicing</rdfs:comment>
        <rdfs:isDefinedBy rdf:resource="https://www.theworldavatar.com/kg/ontopoi"/>
        <rdfs:label>Building repairs</rdfs:label>
    </owl:Class>
    


    <!-- https://www.theworldavatar.com/kg/ontopoi/BusAndCoachStationsAndDepotsAndCompanies -->


    <owl:Class rdf:about="https://www.theworldavatar.com/kg/ontopoi/BusAndCoachStationsAndDepotsAndCompanies">
        <rdfs:subClassOf rdf:resource="https://www.theworldavatar.com/kg/ontopoi/PublicTransportAndStationsAndInfrastructure"/>
        <rdfs:comment>Bus and coach stations, depots and companies is a subcategory of public transport, stations and infrastructure</rdfs:comment>
        <rdfs:isDefinedBy rdf:resource="https://www.theworldavatar.com/kg/ontopoi"/>
        <rdfs:label>Bus and coach stations, depots and companies</rdfs:label>
    </owl:Class>
    


    <!-- https://www.theworldavatar.com/kg/ontopoi/BusStops -->


    <owl:Class rdf:about="https://www.theworldavatar.com/kg/ontopoi/BusStops">
        <rdfs:subClassOf rdf:resource="https://www.theworldavatar.com/kg/ontopoi/BusTransport"/>
        <rdfs:comment>Bus stops is a subcategory of bus transport</rdfs:comment>
        <rdfs:isDefinedBy rdf:resource="https://www.theworldavatar.com/kg/ontopoi"/>
        <rdfs:label>Bus stops</rdfs:label>
    </owl:Class>
    


    <!-- https://www.theworldavatar.com/kg/ontopoi/BusTransport -->


    <owl:Class rdf:about="https://www.theworldavatar.com/kg/ontopoi/BusTransport">
        <rdfs:subClassOf rdf:resource="https://www.theworldavatar.com/kg/ontopoi/Transport"/>
        <rdfs:comment>Bus transport is a subcategory of transport</rdfs:comment>
        <rdfs:isDefinedBy rdf:resource="https://www.theworldavatar.com/kg/ontopoi"/>
        <rdfs:label>Bus transport</rdfs:label>
    </owl:Class>
    


    <!-- https://www.theworldavatar.com/kg/ontopoi/Business-RelatedConsultants -->


    <owl:Class rdf:about="https://www.theworldavatar.com/kg/ontopoi/Business-RelatedConsultants">
        <rdfs:subClassOf rdf:resource="https://www.theworldavatar.com/kg/ontopoi/Consultancies"/>
        <rdfs:comment>Business-related consultants is a subcategory of consultancies</rdfs:comment>
        <rdfs:isDefinedBy rdf:resource="https://www.theworldavatar.com/kg/ontopoi"/>
        <rdfs:label>Business-related consultants</rdfs:label>
    </owl:Class>
    


    <!-- https://www.theworldavatar.com/kg/ontopoi/BusinessParksAndIndustrialEstates -->


    <owl:Class rdf:about="https://www.theworldavatar.com/kg/ontopoi/BusinessParksAndIndustrialEstates">
        <rdfs:subClassOf rdf:resource="https://www.theworldavatar.com/kg/ontopoi/IndustrialFeatures"/>
        <rdfs:comment>Business parks and industrial estates is a subcategory of industrial features</rdfs:comment>
        <rdfs:isDefinedBy rdf:resource="https://www.theworldavatar.com/kg/ontopoi"/>
        <rdfs:label>Business parks and industrial estates</rdfs:label>
    </owl:Class>
    


    <!-- https://www.theworldavatar.com/kg/ontopoi/Butchers -->


    <owl:Class rdf:about="https://www.theworldavatar.com/kg/ontopoi/Butchers">
        <rdfs:subClassOf rdf:resource="https://www.theworldavatar.com/kg/ontopoi/FoodAndDrinkAndMultiItemRetail"/>
        <rdfs:comment>Butchers is a subcategory of food, drink and multi item retail</rdfs:comment>
        <rdfs:isDefinedBy rdf:resource="https://www.theworldavatar.com/kg/ontopoi"/>
        <rdfs:label>Butchers</rdfs:label>
    </owl:Class>
    


    <!-- https://www.theworldavatar.com/kg/ontopoi/ButterflyFarms -->


    <owl:Class rdf:about="https://www.theworldavatar.com/kg/ontopoi/ButterflyFarms">
        <rdfs:subClassOf rdf:resource="https://www.theworldavatar.com/kg/ontopoi/BotanicalAndZoological"/>
        <rdfs:comment>Butterfly farms is a subcategory of botanical and zoological</rdfs:comment>
        <rdfs:isDefinedBy rdf:resource="https://www.theworldavatar.com/kg/ontopoi"/>
        <rdfs:label>Butterfly farms</rdfs:label>
    </owl:Class>
    


    <!-- https://www.theworldavatar.com/kg/ontopoi/CableAndWireAndFibreOptics -->


    <owl:Class rdf:about="https://www.theworldavatar.com/kg/ontopoi/CableAndWireAndFibreOptics">
        <rdfs:subClassOf rdf:resource="https://www.theworldavatar.com/kg/ontopoi/IndustrialProducts"/>
        <rdfs:comment>Cable, wire and fibre optics is a subcategory of industrial products</rdfs:comment>
        <rdfs:isDefinedBy rdf:resource="https://www.theworldavatar.com/kg/ontopoi"/>
        <rdfs:label>Cable, wire and fibre optics</rdfs:label>
    </owl:Class>
    


    <!-- https://www.theworldavatar.com/kg/ontopoi/CafesAndSnackBarsAndTeaRooms -->


    <owl:Class rdf:about="https://www.theworldavatar.com/kg/ontopoi/CafesAndSnackBarsAndTeaRooms">
        <rdfs:subClassOf rdf:resource="https://www.theworldavatar.com/kg/ontopoi/EatingAndDrinking"/>
        <rdfs:comment>Cafes, snack bars and tea rooms is a subcategory of eating and drinking</rdfs:comment>
        <rdfs:isDefinedBy rdf:resource="https://www.theworldavatar.com/kg/ontopoi"/>
        <rdfs:label>Cafes, snack bars and tea rooms</rdfs:label>
    </owl:Class>
    


    <!-- https://www.theworldavatar.com/kg/ontopoi/CampingAndCaravanning -->


    <owl:Class rdf:about="https://www.theworldavatar.com/kg/ontopoi/CampingAndCaravanning">
        <rdfs:subClassOf rdf:resource="https://www.theworldavatar.com/kg/ontopoi/HouseholdAndOfficeAndLeisureAndGarden"/>
        <rdfs:comment>Camping and caravanning is a subcategory of household, office, leisure and garden</rdfs:comment>
        <rdfs:isDefinedBy rdf:resource="https://www.theworldavatar.com/kg/ontopoi"/>
        <rdfs:label>Camping and caravanning</rdfs:label>
    </owl:Class>
    


    <!-- https://www.theworldavatar.com/kg/ontopoi/CampingAndCaravanningAndMobileHomesAndHolidayParksAndCentres -->


    <owl:Class rdf:about="https://www.theworldavatar.com/kg/ontopoi/CampingAndCaravanningAndMobileHomesAndHolidayParksAndCentres">
        <rdfs:subClassOf rdf:resource="https://www.theworldavatar.com/kg/ontopoi/Accommodation"/>
        <rdfs:comment>Camping, caravanning, mobile homes, holiday parks and centres is a subcategory of accommodation</rdfs:comment>
        <rdfs:isDefinedBy rdf:resource="https://www.theworldavatar.com/kg/ontopoi"/>
        <rdfs:label>Camping, caravanning, mobile homes, holiday parks and centres</rdfs:label>
    </owl:Class>
    


    <!-- https://www.theworldavatar.com/kg/ontopoi/Candles -->


    <owl:Class rdf:about="https://www.theworldavatar.com/kg/ontopoi/Candles">
        <rdfs:subClassOf rdf:resource="https://www.theworldavatar.com/kg/ontopoi/ConsumerProducts"/>
        <rdfs:comment>Candles is a subcategory of consumer products</rdfs:comment>
        <rdfs:isDefinedBy rdf:resource="https://www.theworldavatar.com/kg/ontopoi"/>
        <rdfs:label>Candles</rdfs:label>
    </owl:Class>
    


    <!-- https://www.theworldavatar.com/kg/ontopoi/CanvasGoods -->


    <owl:Class rdf:about="https://www.theworldavatar.com/kg/ontopoi/CanvasGoods">
        <rdfs:subClassOf rdf:resource="https://www.theworldavatar.com/kg/ontopoi/ConsumerProducts"/>
        <rdfs:comment>Canvas goods is a subcategory of consumer products</rdfs:comment>
        <rdfs:isDefinedBy rdf:resource="https://www.theworldavatar.com/kg/ontopoi"/>
        <rdfs:label>Canvas goods</rdfs:label>
    </owl:Class>
    


    <!-- https://www.theworldavatar.com/kg/ontopoi/CarPortsAndSteelBuildings -->


    <owl:Class rdf:about="https://www.theworldavatar.com/kg/ontopoi/CarPortsAndSteelBuildings">
        <rdfs:subClassOf rdf:resource="https://www.theworldavatar.com/kg/ontopoi/IndustrialProducts"/>
        <rdfs:comment>Car ports and steel buildings is a subcategory of industrial products</rdfs:comment>
        <rdfs:isDefinedBy rdf:resource="https://www.theworldavatar.com/kg/ontopoi"/>
        <rdfs:label>Car ports and steel buildings</rdfs:label>
    </owl:Class>
    


    <!-- https://www.theworldavatar.com/kg/ontopoi/CareersOfficesAndArmedForcesRecruitment -->


    <owl:Class rdf:about="https://www.theworldavatar.com/kg/ontopoi/CareersOfficesAndArmedForcesRecruitment">
        <rdfs:subClassOf rdf:resource="https://www.theworldavatar.com/kg/ontopoi/EmploymentAndCareerAgencies"/>
        <rdfs:comment>Careers offices and armed forces recruitment is a subcategory of employment and career agencies</rdfs:comment>
        <rdfs:isDefinedBy rdf:resource="https://www.theworldavatar.com/kg/ontopoi"/>
        <rdfs:label>Careers offices and armed forces recruitment</rdfs:label>
    </owl:Class>
    


    <!-- https://www.theworldavatar.com/kg/ontopoi/CarpetsAndFlooringAndRugsAndSoftFurnishings -->


    <owl:Class rdf:about="https://www.theworldavatar.com/kg/ontopoi/CarpetsAndFlooringAndRugsAndSoftFurnishings">
        <rdfs:subClassOf rdf:resource="https://www.theworldavatar.com/kg/ontopoi/ConsumerProducts"/>
        <rdfs:comment>Carpets, flooring, rugs and soft furnishings is a subcategory of consumer products</rdfs:comment>
        <rdfs:isDefinedBy rdf:resource="https://www.theworldavatar.com/kg/ontopoi"/>
        <rdfs:label>Carpets, flooring, rugs and soft furnishings</rdfs:label>
    </owl:Class>
    


    <!-- https://www.theworldavatar.com/kg/ontopoi/CarpetsAndRugsAndSoftFurnishingsAndNeedlecraft -->


    <owl:Class rdf:about="https://www.theworldavatar.com/kg/ontopoi/CarpetsAndRugsAndSoftFurnishingsAndNeedlecraft">
        <rdfs:subClassOf rdf:resource="https://www.theworldavatar.com/kg/ontopoi/HouseholdAndOfficeAndLeisureAndGarden"/>
        <rdfs:comment>Carpets, rugs, soft furnishings and needlecraft is a subcategory of household, office, leisure and garden</rdfs:comment>
        <rdfs:isDefinedBy rdf:resource="https://www.theworldavatar.com/kg/ontopoi"/>
        <rdfs:label>Carpets, rugs, soft furnishings and needlecraft</rdfs:label>
    </owl:Class>
    


    <!-- https://www.theworldavatar.com/kg/ontopoi/CashAndCarry -->


    <owl:Class rdf:about="https://www.theworldavatar.com/kg/ontopoi/CashAndCarry">
        <rdfs:subClassOf rdf:resource="https://www.theworldavatar.com/kg/ontopoi/FoodAndDrinkAndMultiItemRetail"/>
        <rdfs:comment>Cash and carry is a subcategory of food, drink and multi item retail</rdfs:comment>
        <rdfs:isDefinedBy rdf:resource="https://www.theworldavatar.com/kg/ontopoi"/>
        <rdfs:label>Cash and carry</rdfs:label>
    </owl:Class>
    


    <!-- https://www.theworldavatar.com/kg/ontopoi/CashMachines -->


    <owl:Class rdf:about="https://www.theworldavatar.com/kg/ontopoi/CashMachines">
        <rdfs:subClassOf rdf:resource="https://www.theworldavatar.com/kg/ontopoi/LegalAndFinancial"/>
        <rdfs:comment>Cash machines is a subcategory of legal and financial</rdfs:comment>
        <rdfs:isDefinedBy rdf:resource="https://www.theworldavatar.com/kg/ontopoi"/>
        <rdfs:label>Cash machines</rdfs:label>
    </owl:Class>
    


    <!-- https://www.theworldavatar.com/kg/ontopoi/Casinos -->


    <owl:Class rdf:about="https://www.theworldavatar.com/kg/ontopoi/Casinos">
        <rdfs:subClassOf rdf:resource="https://www.theworldavatar.com/kg/ontopoi/Gambling"/>
        <rdfs:comment>Casinos is a subcategory of gambling</rdfs:comment>
        <rdfs:isDefinedBy rdf:resource="https://www.theworldavatar.com/kg/ontopoi"/>
        <rdfs:label>Casinos</rdfs:label>
    </owl:Class>
    


    <!-- https://www.theworldavatar.com/kg/ontopoi/CateringAndNon-SpecificFoodProducts -->


    <owl:Class rdf:about="https://www.theworldavatar.com/kg/ontopoi/CateringAndNon-SpecificFoodProducts">
        <rdfs:subClassOf rdf:resource="https://www.theworldavatar.com/kg/ontopoi/Foodstuffs"/>
        <rdfs:comment>Catering and non-specific food products is a subcategory of foodstuffs</rdfs:comment>
        <rdfs:isDefinedBy rdf:resource="https://www.theworldavatar.com/kg/ontopoi"/>
        <rdfs:label>Catering and non-specific food products</rdfs:label>
    </owl:Class>
    


    <!-- https://www.theworldavatar.com/kg/ontopoi/CateringServices -->


    <owl:Class rdf:about="https://www.theworldavatar.com/kg/ontopoi/CateringServices">
        <rdfs:subClassOf rdf:resource="https://www.theworldavatar.com/kg/ontopoi/ContractServices"/>
        <rdfs:comment>Catering services is a subcategory of contract services</rdfs:comment>
        <rdfs:isDefinedBy rdf:resource="https://www.theworldavatar.com/kg/ontopoi"/>
        <rdfs:label>Catering services</rdfs:label>
    </owl:Class>
    


    <!-- https://www.theworldavatar.com/kg/ontopoi/CattleGrids -->


    <owl:Class rdf:about="https://www.theworldavatar.com/kg/ontopoi/CattleGrids">
        <rdfs:subClassOf rdf:resource="https://www.theworldavatar.com/kg/ontopoi/RoadAndRail"/>
        <rdfs:comment>Cattle grids is a subcategory of road and rail</rdfs:comment>
        <rdfs:isDefinedBy rdf:resource="https://www.theworldavatar.com/kg/ontopoi"/>
        <rdfs:label>Cattle grids</rdfs:label>
    </owl:Class>
    


    <!-- https://www.theworldavatar.com/kg/ontopoi/CemeteriesAndCrematoria -->


    <owl:Class rdf:about="https://www.theworldavatar.com/kg/ontopoi/CemeteriesAndCrematoria">
        <rdfs:subClassOf rdf:resource="https://www.theworldavatar.com/kg/ontopoi/InfrastructureAndFacilities"/>
        <rdfs:comment>Cemeteries and crematoria is a subcategory of infrastructure and facilities</rdfs:comment>
        <rdfs:isDefinedBy rdf:resource="https://www.theworldavatar.com/kg/ontopoi"/>
        <rdfs:label>Cemeteries and crematoria</rdfs:label>
    </owl:Class>
    


    <!-- https://www.theworldavatar.com/kg/ontopoi/CentralAndLocalGovernment -->


    <owl:Class rdf:about="https://www.theworldavatar.com/kg/ontopoi/CentralAndLocalGovernment">
        <rdfs:subClassOf rdf:resource="https://www.theworldavatar.com/kg/ontopoi/PublicInfrastructure"/>
        <rdfs:comment>Central and local government is a subcategory of public infrastructure</rdfs:comment>
        <rdfs:isDefinedBy rdf:resource="https://www.theworldavatar.com/kg/ontopoi"/>
        <rdfs:label>Central and local government</rdfs:label>
    </owl:Class>
    


    <!-- https://www.theworldavatar.com/kg/ontopoi/CentralGovernment -->


    <owl:Class rdf:about="https://www.theworldavatar.com/kg/ontopoi/CentralGovernment">
        <rdfs:subClassOf rdf:resource="https://www.theworldavatar.com/kg/ontopoi/CentralAndLocalGovernment"/>
        <rdfs:comment>Central government is a subcategory of central and local government</rdfs:comment>
        <rdfs:isDefinedBy rdf:resource="https://www.theworldavatar.com/kg/ontopoi"/>
        <rdfs:label>Central government</rdfs:label>
    </owl:Class>
    


    <!-- https://www.theworldavatar.com/kg/ontopoi/CharitableOrganisations -->


    <owl:Class rdf:about="https://www.theworldavatar.com/kg/ontopoi/CharitableOrganisations">
        <rdfs:subClassOf rdf:resource="https://www.theworldavatar.com/kg/ontopoi/Organisations"/>
        <rdfs:comment>Charitable organisations is a subcategory of organisations</rdfs:comment>
        <rdfs:isDefinedBy rdf:resource="https://www.theworldavatar.com/kg/ontopoi"/>
        <rdfs:label>Charitable organisations</rdfs:label>
    </owl:Class>
    


    <!-- https://www.theworldavatar.com/kg/ontopoi/CharityShops -->


    <owl:Class rdf:about="https://www.theworldavatar.com/kg/ontopoi/CharityShops">
        <rdfs:subClassOf rdf:resource="https://www.theworldavatar.com/kg/ontopoi/HouseholdAndOfficeAndLeisureAndGarden"/>
        <rdfs:comment>Charity shops is a subcategory of household, office, leisure and garden</rdfs:comment>
        <rdfs:isDefinedBy rdf:resource="https://www.theworldavatar.com/kg/ontopoi"/>
        <rdfs:label>Charity shops</rdfs:label>
    </owl:Class>
    


    <!-- https://www.theworldavatar.com/kg/ontopoi/ChemicalEngineers -->


    <owl:Class rdf:about="https://www.theworldavatar.com/kg/ontopoi/ChemicalEngineers">
        <rdfs:subClassOf rdf:resource="https://www.theworldavatar.com/kg/ontopoi/EngineeringServices"/>
        <rdfs:comment>Chemical engineers is a subcategory of engineering services</rdfs:comment>
        <rdfs:isDefinedBy rdf:resource="https://www.theworldavatar.com/kg/ontopoi"/>
        <rdfs:label>Chemical engineers</rdfs:label>
    </owl:Class>
    


    <!-- https://www.theworldavatar.com/kg/ontopoi/ChemistsAndPharmacies -->


    <owl:Class rdf:about="https://www.theworldavatar.com/kg/ontopoi/ChemistsAndPharmacies">
        <rdfs:subClassOf rdf:resource="https://www.theworldavatar.com/kg/ontopoi/HealthPractitionersAndEstablishments"/>
        <rdfs:comment>Chemists and pharmacies is a subcategory of health practitioners and establishments</rdfs:comment>
        <rdfs:isDefinedBy rdf:resource="https://www.theworldavatar.com/kg/ontopoi"/>
        <rdfs:label>Chemists and pharmacies</rdfs:label>
    </owl:Class>
    


    <!-- https://www.theworldavatar.com/kg/ontopoi/ChequeCashing -->


    <owl:Class rdf:about="https://www.theworldavatar.com/kg/ontopoi/ChequeCashing">
        <rdfs:subClassOf rdf:resource="https://www.theworldavatar.com/kg/ontopoi/LegalAndFinancial"/>
        <rdfs:comment>Cheque cashing is a subcategory of legal and financial</rdfs:comment>
        <rdfs:isDefinedBy rdf:resource="https://www.theworldavatar.com/kg/ontopoi"/>
        <rdfs:label>Cheque cashing</rdfs:label>
    </owl:Class>
    


    <!-- https://www.theworldavatar.com/kg/ontopoi/ChildrenActivityCentres -->


    <owl:Class rdf:about="https://www.theworldavatar.com/kg/ontopoi/ChildrenActivityCentres">
        <rdfs:subClassOf rdf:resource="https://www.theworldavatar.com/kg/ontopoi/SportAndEntertainmentSupportServices"/>
        <rdfs:comment>Children&apos;s activity centres is a subcategory of sport and entertainment support services</rdfs:comment>
        <rdfs:isDefinedBy rdf:resource="https://www.theworldavatar.com/kg/ontopoi"/>
        <rdfs:label>Children&apos;s activity centres</rdfs:label>
    </owl:Class>
    


    <!-- https://www.theworldavatar.com/kg/ontopoi/ChinaAndGlassware -->


    <owl:Class rdf:about="https://www.theworldavatar.com/kg/ontopoi/ChinaAndGlassware">
        <rdfs:subClassOf rdf:resource="https://www.theworldavatar.com/kg/ontopoi/ConsumerProducts"/>
        <rdfs:subClassOf rdf:resource="https://www.theworldavatar.com/kg/ontopoi/HouseholdAndOfficeAndLeisureAndGarden"/>
        <rdfs:comment>China and glassware is a subcategory of consumer products</rdfs:comment>
        <rdfs:comment>China and glassware is a subcategory of household, office, leisure and garden</rdfs:comment>
        <rdfs:isDefinedBy rdf:resource="https://www.theworldavatar.com/kg/ontopoi"/>
        <rdfs:label>China and glassware</rdfs:label>
    </owl:Class>
    


    <!-- https://www.theworldavatar.com/kg/ontopoi/Cinemas -->


    <owl:Class rdf:about="https://www.theworldavatar.com/kg/ontopoi/Cinemas">
        <rdfs:subClassOf rdf:resource="https://www.theworldavatar.com/kg/ontopoi/VenuesAndStageAndScreen"/>
        <rdfs:comment>Cinemas is a subcategory of venues, stage and screen</rdfs:comment>
        <rdfs:isDefinedBy rdf:resource="https://www.theworldavatar.com/kg/ontopoi"/>
        <rdfs:label>Cinemas</rdfs:label>
    </owl:Class>
    


    <!-- https://www.theworldavatar.com/kg/ontopoi/CivilEngineers -->


    <owl:Class rdf:about="https://www.theworldavatar.com/kg/ontopoi/CivilEngineers">
        <rdfs:subClassOf rdf:resource="https://www.theworldavatar.com/kg/ontopoi/EngineeringServices"/>
        <rdfs:comment>Civil engineers is a subcategory of engineering services</rdfs:comment>
        <rdfs:isDefinedBy rdf:resource="https://www.theworldavatar.com/kg/ontopoi"/>
        <rdfs:label>Civil engineers</rdfs:label>
    </owl:Class>
    


    <!-- https://www.theworldavatar.com/kg/ontopoi/CleaningEquipmentAndSupplies -->


    <owl:Class rdf:about="https://www.theworldavatar.com/kg/ontopoi/CleaningEquipmentAndSupplies">
        <rdfs:subClassOf rdf:resource="https://www.theworldavatar.com/kg/ontopoi/IndustrialProducts"/>
        <rdfs:comment>Cleaning equipment and supplies is a subcategory of industrial products</rdfs:comment>
        <rdfs:isDefinedBy rdf:resource="https://www.theworldavatar.com/kg/ontopoi"/>
        <rdfs:label>Cleaning equipment and supplies</rdfs:label>
    </owl:Class>
    


    <!-- https://www.theworldavatar.com/kg/ontopoi/CleaningServices -->


    <owl:Class rdf:about="https://www.theworldavatar.com/kg/ontopoi/CleaningServices">
        <rdfs:subClassOf rdf:resource="https://www.theworldavatar.com/kg/ontopoi/PersonalAndConsumerAndOtherServices"/>
        <rdfs:comment>Cleaning services is a subcategory of personal, consumer and other services</rdfs:comment>
        <rdfs:isDefinedBy rdf:resource="https://www.theworldavatar.com/kg/ontopoi"/>
        <rdfs:label>Cleaning services</rdfs:label>
    </owl:Class>
    


    <!-- https://www.theworldavatar.com/kg/ontopoi/ClearanceAndSalvageDealers -->


    <owl:Class rdf:about="https://www.theworldavatar.com/kg/ontopoi/ClearanceAndSalvageDealers">
        <rdfs:subClassOf rdf:resource="https://www.theworldavatar.com/kg/ontopoi/RecyclingServices"/>
        <rdfs:comment>Clearance and salvage dealers is a subcategory of recycling services</rdfs:comment>
        <rdfs:isDefinedBy rdf:resource="https://www.theworldavatar.com/kg/ontopoi"/>
        <rdfs:label>Clearance and salvage dealers</rdfs:label>
    </owl:Class>
    


    <!-- https://www.theworldavatar.com/kg/ontopoi/ClimbingFacilities -->


    <owl:Class rdf:about="https://www.theworldavatar.com/kg/ontopoi/ClimbingFacilities">
        <rdfs:subClassOf rdf:resource="https://www.theworldavatar.com/kg/ontopoi/SportsComplex"/>
        <rdfs:comment>Climbing facilities is a subcategory of sports complex</rdfs:comment>
        <rdfs:isDefinedBy rdf:resource="https://www.theworldavatar.com/kg/ontopoi"/>
        <rdfs:label>Climbing facilities</rdfs:label>
    </owl:Class>
    


    <!-- https://www.theworldavatar.com/kg/ontopoi/ClinicsAndHealthCentres -->


    <owl:Class rdf:about="https://www.theworldavatar.com/kg/ontopoi/ClinicsAndHealthCentres">
        <rdfs:subClassOf rdf:resource="https://www.theworldavatar.com/kg/ontopoi/HealthPractitionersAndEstablishments"/>
        <rdfs:comment>Clinics and health centres is a subcategory of health practitioners and establishments</rdfs:comment>
        <rdfs:isDefinedBy rdf:resource="https://www.theworldavatar.com/kg/ontopoi"/>
        <rdfs:label>Clinics and health centres</rdfs:label>
    </owl:Class>
    


    <!-- https://www.theworldavatar.com/kg/ontopoi/Clothing -->


    <owl:Class rdf:about="https://www.theworldavatar.com/kg/ontopoi/Clothing">
        <rdfs:subClassOf rdf:resource="https://www.theworldavatar.com/kg/ontopoi/ClothingAndAccessories"/>
        <rdfs:comment>Clothing is a subcategory of clothing and accessories</rdfs:comment>
        <rdfs:isDefinedBy rdf:resource="https://www.theworldavatar.com/kg/ontopoi"/>
        <rdfs:label>Clothing</rdfs:label>
    </owl:Class>
    


    <!-- https://www.theworldavatar.com/kg/ontopoi/ClothingAndAccessories -->


    <owl:Class rdf:about="https://www.theworldavatar.com/kg/ontopoi/ClothingAndAccessories">
        <rdfs:subClassOf rdf:resource="https://www.theworldavatar.com/kg/ontopoi/Retail"/>
        <rdfs:comment>Clothing and accessories is a subcategory of retail</rdfs:comment>
        <rdfs:isDefinedBy rdf:resource="https://www.theworldavatar.com/kg/ontopoi"/>
        <rdfs:label>Clothing and accessories</rdfs:label>
    </owl:Class>
    


    <!-- https://www.theworldavatar.com/kg/ontopoi/ClothingAndComponentsAndAccessories -->


    <owl:Class rdf:about="https://www.theworldavatar.com/kg/ontopoi/ClothingAndComponentsAndAccessories">
        <rdfs:subClassOf rdf:resource="https://www.theworldavatar.com/kg/ontopoi/ConsumerProducts"/>
        <rdfs:comment>Clothing, components and accessories is a subcategory of consumer products</rdfs:comment>
        <rdfs:isDefinedBy rdf:resource="https://www.theworldavatar.com/kg/ontopoi"/>
        <rdfs:label>Clothing, components and accessories</rdfs:label>
    </owl:Class>
    


    <!-- https://www.theworldavatar.com/kg/ontopoi/ClothingHire -->


    <owl:Class rdf:about="https://www.theworldavatar.com/kg/ontopoi/ClothingHire">
        <rdfs:subClassOf rdf:resource="https://www.theworldavatar.com/kg/ontopoi/HireServices"/>
        <rdfs:comment>Clothing hire is a subcategory of hire services</rdfs:comment>
        <rdfs:isDefinedBy rdf:resource="https://www.theworldavatar.com/kg/ontopoi"/>
        <rdfs:label>Clothing hire</rdfs:label>
    </owl:Class>
    


    <!-- https://www.theworldavatar.com/kg/ontopoi/CoalMining -->


    <owl:Class rdf:about="https://www.theworldavatar.com/kg/ontopoi/CoalMining">
        <rdfs:subClassOf rdf:resource="https://www.theworldavatar.com/kg/ontopoi/ExtractiveIndustries"/>
        <rdfs:comment>Coal mining is a subcategory of extractive industries</rdfs:comment>
        <rdfs:isDefinedBy rdf:resource="https://www.theworldavatar.com/kg/ontopoi"/>
        <rdfs:label>Coal mining</rdfs:label>
    </owl:Class>
    


    <!-- https://www.theworldavatar.com/kg/ontopoi/CoastalSafety -->


    <owl:Class rdf:about="https://www.theworldavatar.com/kg/ontopoi/CoastalSafety">
        <rdfs:subClassOf rdf:resource="https://www.theworldavatar.com/kg/ontopoi/CentralAndLocalGovernment"/>
        <rdfs:comment>Coastal safety is a subcategory of central and local government</rdfs:comment>
        <rdfs:isDefinedBy rdf:resource="https://www.theworldavatar.com/kg/ontopoi"/>
        <rdfs:label>Coastal Safety</rdfs:label>
    </owl:Class>
    


    <!-- https://www.theworldavatar.com/kg/ontopoi/ColoursAndChemicalsAndWaterSoftenersAndSupplies -->


    <owl:Class rdf:about="https://www.theworldavatar.com/kg/ontopoi/ColoursAndChemicalsAndWaterSoftenersAndSupplies">
        <rdfs:subClassOf rdf:resource="https://www.theworldavatar.com/kg/ontopoi/IndustrialProducts"/>
        <rdfs:comment>Colours, chemicals and water softeners and supplies is a subcategory of industrial products</rdfs:comment>
        <rdfs:isDefinedBy rdf:resource="https://www.theworldavatar.com/kg/ontopoi"/>
        <rdfs:label>Colours, chemicals and water softeners and supplies</rdfs:label>
    </owl:Class>
    


    <!-- https://www.theworldavatar.com/kg/ontopoi/CombatAndLaserAndPaintballGames -->


    <owl:Class rdf:about="https://www.theworldavatar.com/kg/ontopoi/CombatAndLaserAndPaintballGames">
        <rdfs:subClassOf rdf:resource="https://www.theworldavatar.com/kg/ontopoi/OutdoorPursuits"/>
        <rdfs:comment>Combat, laser and paintball games is a subcategory of outdoor pursuits</rdfs:comment>
        <rdfs:isDefinedBy rdf:resource="https://www.theworldavatar.com/kg/ontopoi"/>
        <rdfs:label>Combat, laser and paintball games</rdfs:label>
    </owl:Class>
    


    <!-- https://www.theworldavatar.com/kg/ontopoi/ComicBooks -->


    <owl:Class rdf:about="https://www.theworldavatar.com/kg/ontopoi/ComicBooks">
        <rdfs:subClassOf rdf:resource="https://www.theworldavatar.com/kg/ontopoi/HouseholdAndOfficeAndLeisureAndGarden"/>
        <rdfs:comment>Comic books is a subcategory of household, office, leisure and garden</rdfs:comment>
        <rdfs:isDefinedBy rdf:resource="https://www.theworldavatar.com/kg/ontopoi"/>
        <rdfs:label>Comic books</rdfs:label>
    </owl:Class>
    


    <!-- https://www.theworldavatar.com/kg/ontopoi/CommercialPropertyLetting -->


    <owl:Class rdf:about="https://www.theworldavatar.com/kg/ontopoi/CommercialPropertyLetting">
        <rdfs:subClassOf rdf:resource="https://www.theworldavatar.com/kg/ontopoi/PropertyAndDevelopmentServices"/>
        <rdfs:comment>Commercial property letting is a subcategory of property and development services</rdfs:comment>
        <rdfs:isDefinedBy rdf:resource="https://www.theworldavatar.com/kg/ontopoi"/>
        <rdfs:label>Commercial property letting</rdfs:label>
    </owl:Class>
    


    <!-- https://www.theworldavatar.com/kg/ontopoi/CommercialServices -->


    <owl:Class rdf:about="https://www.theworldavatar.com/kg/ontopoi/CommercialServices">
        <rdfs:subClassOf rdf:resource="https://www.theworldavatar.com/kg/ontopoi/PointOfInterest"/>
        <rdfs:comment>Services that are provided by businesses or organisations with the primary purpose of generating profit through the exchange of goods, services, or expertise</rdfs:comment>
        <rdfs:isDefinedBy rdf:resource="https://www.theworldavatar.com/kg/ontopoi"/>
        <rdfs:label>Commercial services</rdfs:label>
    </owl:Class>
    


    <!-- https://www.theworldavatar.com/kg/ontopoi/CommodityDealers -->


    <owl:Class rdf:about="https://www.theworldavatar.com/kg/ontopoi/CommodityDealers">
        <rdfs:subClassOf rdf:resource="https://www.theworldavatar.com/kg/ontopoi/LegalAndFinancial"/>
        <rdfs:comment>Commodity dealers is a subcategory of legal and financial</rdfs:comment>
        <rdfs:isDefinedBy rdf:resource="https://www.theworldavatar.com/kg/ontopoi"/>
        <rdfs:label>Commodity dealers</rdfs:label>
    </owl:Class>
    


    <!-- https://www.theworldavatar.com/kg/ontopoi/Commons -->


    <owl:Class rdf:about="https://www.theworldavatar.com/kg/ontopoi/Commons">
        <rdfs:subClassOf rdf:resource="https://www.theworldavatar.com/kg/ontopoi/Recreational"/>
        <rdfs:comment>Commons is a subcategory of recreational</rdfs:comment>
        <rdfs:isDefinedBy rdf:resource="https://www.theworldavatar.com/kg/ontopoi"/>
        <rdfs:label>Commons</rdfs:label>
    </owl:Class>
    


    <!-- https://www.theworldavatar.com/kg/ontopoi/CommunityNetworksAndProjects -->


    <owl:Class rdf:about="https://www.theworldavatar.com/kg/ontopoi/CommunityNetworksAndProjects">
        <rdfs:subClassOf rdf:resource="https://www.theworldavatar.com/kg/ontopoi/Organisations"/>
        <rdfs:comment>Community networks and projects is a subcategory of organisations</rdfs:comment>
        <rdfs:isDefinedBy rdf:resource="https://www.theworldavatar.com/kg/ontopoi"/>
        <rdfs:label>Community networks and projects</rdfs:label>
    </owl:Class>
    


    <!-- https://www.theworldavatar.com/kg/ontopoi/CompanyRegistrationAndTrademarks -->


    <owl:Class rdf:about="https://www.theworldavatar.com/kg/ontopoi/CompanyRegistrationAndTrademarks">
        <rdfs:subClassOf rdf:resource="https://www.theworldavatar.com/kg/ontopoi/LegalAndFinancial"/>
        <rdfs:comment>Company registration and trademarks is a subcategory of legal and financial</rdfs:comment>
        <rdfs:isDefinedBy rdf:resource="https://www.theworldavatar.com/kg/ontopoi"/>
        <rdfs:label>Company registration and trademarks</rdfs:label>
    </owl:Class>
    


    <!-- https://www.theworldavatar.com/kg/ontopoi/ComputerConsultants -->


    <owl:Class rdf:about="https://www.theworldavatar.com/kg/ontopoi/ComputerConsultants">
        <rdfs:subClassOf rdf:resource="https://www.theworldavatar.com/kg/ontopoi/Consultancies"/>
        <rdfs:comment>Computer consultants is a subcategory of consultancies</rdfs:comment>
        <rdfs:isDefinedBy rdf:resource="https://www.theworldavatar.com/kg/ontopoi"/>
        <rdfs:label>Computer consultants</rdfs:label>
    </owl:Class>
    


    <!-- https://www.theworldavatar.com/kg/ontopoi/ComputerSecurity -->


    <owl:Class rdf:about="https://www.theworldavatar.com/kg/ontopoi/ComputerSecurity">
        <rdfs:subClassOf rdf:resource="https://www.theworldavatar.com/kg/ontopoi/ItAndAdvertisingAndMarketingAndMediaServiceS"/>
        <rdfs:comment>Computer security is a subcategory of it, advertising, marketing and media service s</rdfs:comment>
        <rdfs:isDefinedBy rdf:resource="https://www.theworldavatar.com/kg/ontopoi"/>
        <rdfs:label>Computer security</rdfs:label>
    </owl:Class>
    


    <!-- https://www.theworldavatar.com/kg/ontopoi/ComputerShops -->


    <owl:Class rdf:about="https://www.theworldavatar.com/kg/ontopoi/ComputerShops">
        <rdfs:subClassOf rdf:resource="https://www.theworldavatar.com/kg/ontopoi/HouseholdAndOfficeAndLeisureAndGarden"/>
        <rdfs:comment>Computer shops is a subcategory of household, office, leisure and garden</rdfs:comment>
        <rdfs:isDefinedBy rdf:resource="https://www.theworldavatar.com/kg/ontopoi"/>
        <rdfs:label>Computer shops</rdfs:label>
    </owl:Class>
    


    <!-- https://www.theworldavatar.com/kg/ontopoi/ComputerSupplies -->


    <owl:Class rdf:about="https://www.theworldavatar.com/kg/ontopoi/ComputerSupplies">
        <rdfs:subClassOf rdf:resource="https://www.theworldavatar.com/kg/ontopoi/HouseholdAndOfficeAndLeisureAndGarden"/>
        <rdfs:comment>Computer supplies is a subcategory of household, office, leisure and garden</rdfs:comment>
        <rdfs:isDefinedBy rdf:resource="https://www.theworldavatar.com/kg/ontopoi"/>
        <rdfs:label>Computer supplies</rdfs:label>
    </owl:Class>
    


    <!-- https://www.theworldavatar.com/kg/ontopoi/ComputerSystemsServices -->


    <owl:Class rdf:about="https://www.theworldavatar.com/kg/ontopoi/ComputerSystemsServices">
        <rdfs:subClassOf rdf:resource="https://www.theworldavatar.com/kg/ontopoi/ItAndAdvertisingAndMarketingAndMediaServiceS"/>
        <rdfs:comment>Computer systems services is a subcategory of it, advertising, marketing and media service s</rdfs:comment>
        <rdfs:isDefinedBy rdf:resource="https://www.theworldavatar.com/kg/ontopoi"/>
        <rdfs:label>Computer systems services</rdfs:label>
    </owl:Class>
    


    <!-- https://www.theworldavatar.com/kg/ontopoi/ConcertOrExhibitionOrganisersAndServices -->


    <owl:Class rdf:about="https://www.theworldavatar.com/kg/ontopoi/ConcertOrExhibitionOrganisersAndServices">
        <rdfs:subClassOf rdf:resource="https://www.theworldavatar.com/kg/ontopoi/ItAndAdvertisingAndMarketingAndMediaServiceS"/>
        <rdfs:comment>Concert or exhibition organisers and services is a subcategory of it, advertising, marketing and media service s</rdfs:comment>
        <rdfs:isDefinedBy rdf:resource="https://www.theworldavatar.com/kg/ontopoi"/>
        <rdfs:label>Concert or exhibition organisers and services</rdfs:label>
    </owl:Class>
    


    <!-- https://www.theworldavatar.com/kg/ontopoi/ConcreteProducts -->


    <owl:Class rdf:about="https://www.theworldavatar.com/kg/ontopoi/ConcreteProducts">
        <rdfs:subClassOf rdf:resource="https://www.theworldavatar.com/kg/ontopoi/IndustrialProducts"/>
        <rdfs:comment>Concrete products is a subcategory of industrial products</rdfs:comment>
        <rdfs:isDefinedBy rdf:resource="https://www.theworldavatar.com/kg/ontopoi"/>
        <rdfs:label>Concrete products</rdfs:label>
    </owl:Class>
    


    <!-- https://www.theworldavatar.com/kg/ontopoi/Confectioners -->


    <owl:Class rdf:about="https://www.theworldavatar.com/kg/ontopoi/Confectioners">
        <rdfs:subClassOf rdf:resource="https://www.theworldavatar.com/kg/ontopoi/FoodAndDrinkAndMultiItemRetail"/>
        <rdfs:comment>Confectioners is a subcategory of food, drink and multi item retail</rdfs:comment>
        <rdfs:isDefinedBy rdf:resource="https://www.theworldavatar.com/kg/ontopoi"/>
        <rdfs:label>Confectioners</rdfs:label>
    </owl:Class>
    


    <!-- https://www.theworldavatar.com/kg/ontopoi/ConferenceAndExhibitionCentres -->


    <owl:Class rdf:about="https://www.theworldavatar.com/kg/ontopoi/ConferenceAndExhibitionCentres">
        <rdfs:subClassOf rdf:resource="https://www.theworldavatar.com/kg/ontopoi/VenuesAndStageAndScreen"/>
        <rdfs:comment>Conference and exhibition centres is a subcategory of venues, stage and screen</rdfs:comment>
        <rdfs:isDefinedBy rdf:resource="https://www.theworldavatar.com/kg/ontopoi"/>
        <rdfs:label>Conference and exhibition centres</rdfs:label>
    </owl:Class>
    


    <!-- https://www.theworldavatar.com/kg/ontopoi/ConservationOrganisations -->


    <owl:Class rdf:about="https://www.theworldavatar.com/kg/ontopoi/ConservationOrganisations">
        <rdfs:subClassOf rdf:resource="https://www.theworldavatar.com/kg/ontopoi/Organisations"/>
        <rdfs:comment>Conservation organisations is a subcategory of organisations</rdfs:comment>
        <rdfs:isDefinedBy rdf:resource="https://www.theworldavatar.com/kg/ontopoi"/>
        <rdfs:label>Conservation Organisations</rdfs:label>
    </owl:Class>
    


    <!-- https://www.theworldavatar.com/kg/ontopoi/Conservatories -->


    <owl:Class rdf:about="https://www.theworldavatar.com/kg/ontopoi/Conservatories">
        <rdfs:subClassOf rdf:resource="https://www.theworldavatar.com/kg/ontopoi/ConsumerProducts"/>
        <rdfs:comment>Conservatories is a subcategory of consumer products</rdfs:comment>
        <rdfs:isDefinedBy rdf:resource="https://www.theworldavatar.com/kg/ontopoi"/>
        <rdfs:label>Conservatories</rdfs:label>
    </owl:Class>
    


    <!-- https://www.theworldavatar.com/kg/ontopoi/ConstructionAndToolHire -->


    <owl:Class rdf:about="https://www.theworldavatar.com/kg/ontopoi/ConstructionAndToolHire">
        <rdfs:subClassOf rdf:resource="https://www.theworldavatar.com/kg/ontopoi/HireServices"/>
        <rdfs:comment>Construction and tool hire is a subcategory of hire services</rdfs:comment>
        <rdfs:isDefinedBy rdf:resource="https://www.theworldavatar.com/kg/ontopoi"/>
        <rdfs:label>Construction and tool hire</rdfs:label>
    </owl:Class>
    


    <!-- https://www.theworldavatar.com/kg/ontopoi/ConstructionCompletionServices -->


    <owl:Class rdf:about="https://www.theworldavatar.com/kg/ontopoi/ConstructionCompletionServices">
        <rdfs:subClassOf rdf:resource="https://www.theworldavatar.com/kg/ontopoi/ConstructionServices"/>
        <rdfs:comment>Construction completion services is a subcategory of construction services</rdfs:comment>
        <rdfs:isDefinedBy rdf:resource="https://www.theworldavatar.com/kg/ontopoi"/>
        <rdfs:label>Construction completion services</rdfs:label>
    </owl:Class>
    


    <!-- https://www.theworldavatar.com/kg/ontopoi/ConstructionPlant -->


    <owl:Class rdf:about="https://www.theworldavatar.com/kg/ontopoi/ConstructionPlant">
        <rdfs:subClassOf rdf:resource="https://www.theworldavatar.com/kg/ontopoi/ConstructionServices"/>
        <rdfs:comment>Construction plant is a subcategory of construction services</rdfs:comment>
        <rdfs:isDefinedBy rdf:resource="https://www.theworldavatar.com/kg/ontopoi"/>
        <rdfs:label>Construction plant</rdfs:label>
    </owl:Class>
    


    <!-- https://www.theworldavatar.com/kg/ontopoi/ConstructionServiceConsultants -->


    <owl:Class rdf:about="https://www.theworldavatar.com/kg/ontopoi/ConstructionServiceConsultants">
        <rdfs:subClassOf rdf:resource="https://www.theworldavatar.com/kg/ontopoi/Consultancies"/>
        <rdfs:comment>Construction service consultants is a subcategory of consultancies</rdfs:comment>
        <rdfs:isDefinedBy rdf:resource="https://www.theworldavatar.com/kg/ontopoi"/>
        <rdfs:label>Construction service consultants</rdfs:label>
    </owl:Class>
    


    <!-- https://www.theworldavatar.com/kg/ontopoi/ConstructionServices -->


    <owl:Class rdf:about="https://www.theworldavatar.com/kg/ontopoi/ConstructionServices">
        <rdfs:subClassOf rdf:resource="https://www.theworldavatar.com/kg/ontopoi/CommercialServices"/>
        <rdfs:comment>Construction services is a subcategory of commercial services</rdfs:comment>
        <rdfs:isDefinedBy rdf:resource="https://www.theworldavatar.com/kg/ontopoi"/>
        <rdfs:label>Construction services</rdfs:label>
    </owl:Class>
    


    <!-- https://www.theworldavatar.com/kg/ontopoi/ConsularServices -->


    <owl:Class rdf:about="https://www.theworldavatar.com/kg/ontopoi/ConsularServices">
        <rdfs:subClassOf rdf:resource="https://www.theworldavatar.com/kg/ontopoi/CentralAndLocalGovernment"/>
        <rdfs:comment>Consular services is a subcategory of central and local government</rdfs:comment>
        <rdfs:isDefinedBy rdf:resource="https://www.theworldavatar.com/kg/ontopoi"/>
        <rdfs:label>Consular services</rdfs:label>
    </owl:Class>
    


    <!-- https://www.theworldavatar.com/kg/ontopoi/Consultancies -->


    <owl:Class rdf:about="https://www.theworldavatar.com/kg/ontopoi/Consultancies">
        <rdfs:subClassOf rdf:resource="https://www.theworldavatar.com/kg/ontopoi/CommercialServices"/>
        <rdfs:comment>Consultancies is a subcategory of commercial services</rdfs:comment>
        <rdfs:isDefinedBy rdf:resource="https://www.theworldavatar.com/kg/ontopoi"/>
        <rdfs:label>Consultancies</rdfs:label>
    </owl:Class>
    


    <!-- https://www.theworldavatar.com/kg/ontopoi/ConsumerProducts -->


    <owl:Class rdf:about="https://www.theworldavatar.com/kg/ontopoi/ConsumerProducts">
        <rdfs:subClassOf rdf:resource="https://www.theworldavatar.com/kg/ontopoi/ManufacturingAndProduction"/>
        <rdfs:comment>Consumer products is a subcategory of manufacturing and production</rdfs:comment>
        <rdfs:isDefinedBy rdf:resource="https://www.theworldavatar.com/kg/ontopoi"/>
        <rdfs:label>Consumer products</rdfs:label>
    </owl:Class>
    


    <!-- https://www.theworldavatar.com/kg/ontopoi/ContainerAndStorage -->


    <owl:Class rdf:about="https://www.theworldavatar.com/kg/ontopoi/ContainerAndStorage">
        <rdfs:subClassOf rdf:resource="https://www.theworldavatar.com/kg/ontopoi/TransportAndStorageAndDelivery"/>
        <rdfs:comment>Container and storage is a subcategory of transport, storage and delivery</rdfs:comment>
        <rdfs:isDefinedBy rdf:resource="https://www.theworldavatar.com/kg/ontopoi"/>
        <rdfs:label>Container and storage</rdfs:label>
    </owl:Class>
    


    <!-- https://www.theworldavatar.com/kg/ontopoi/ContractCleaningServices -->


    <owl:Class rdf:about="https://www.theworldavatar.com/kg/ontopoi/ContractCleaningServices">
        <rdfs:subClassOf rdf:resource="https://www.theworldavatar.com/kg/ontopoi/ContractServices"/>
        <rdfs:comment>Contract cleaning services is a subcategory of contract services</rdfs:comment>
        <rdfs:isDefinedBy rdf:resource="https://www.theworldavatar.com/kg/ontopoi"/>
        <rdfs:label>Contract cleaning services</rdfs:label>
    </owl:Class>
    


    <!-- https://www.theworldavatar.com/kg/ontopoi/ContractServices -->


    <owl:Class rdf:about="https://www.theworldavatar.com/kg/ontopoi/ContractServices">
        <rdfs:subClassOf rdf:resource="https://www.theworldavatar.com/kg/ontopoi/CommercialServices"/>
        <rdfs:comment>Contract services is a subcategory of commercial services</rdfs:comment>
        <rdfs:isDefinedBy rdf:resource="https://www.theworldavatar.com/kg/ontopoi"/>
        <rdfs:label>Contract services</rdfs:label>
    </owl:Class>
    


    <!-- https://www.theworldavatar.com/kg/ontopoi/ConvenienceStoresAndIndependentSupermarkets -->


    <owl:Class rdf:about="https://www.theworldavatar.com/kg/ontopoi/ConvenienceStoresAndIndependentSupermarkets">
        <rdfs:subClassOf rdf:resource="https://www.theworldavatar.com/kg/ontopoi/FoodAndDrinkAndMultiItemRetail"/>
        <rdfs:comment>Convenience stores and independent supermarkets is a subcategory of food, drink and multi item retail</rdfs:comment>
        <rdfs:isDefinedBy rdf:resource="https://www.theworldavatar.com/kg/ontopoi"/>
        <rdfs:label>Convenience stores and independent supermarkets</rdfs:label>
    </owl:Class>
    


    <!-- https://www.theworldavatar.com/kg/ontopoi/CoolingAndRefrigeration -->


    <owl:Class rdf:about="https://www.theworldavatar.com/kg/ontopoi/CoolingAndRefrigeration">
        <rdfs:subClassOf rdf:resource="https://www.theworldavatar.com/kg/ontopoi/IndustrialProducts"/>
        <rdfs:comment>Cooling and refrigeration is a subcategory of industrial products</rdfs:comment>
        <rdfs:isDefinedBy rdf:resource="https://www.theworldavatar.com/kg/ontopoi"/>
        <rdfs:label>Cooling and refrigeration</rdfs:label>
    </owl:Class>
    


    <!-- https://www.theworldavatar.com/kg/ontopoi/CopyrightAndPatent -->


    <owl:Class rdf:about="https://www.theworldavatar.com/kg/ontopoi/CopyrightAndPatent">
        <rdfs:subClassOf rdf:resource="https://www.theworldavatar.com/kg/ontopoi/LegalAndFinancial"/>
        <rdfs:comment>Copyright and patent is a subcategory of legal and financial</rdfs:comment>
        <rdfs:isDefinedBy rdf:resource="https://www.theworldavatar.com/kg/ontopoi"/>
        <rdfs:label>Copyright and patent</rdfs:label>
    </owl:Class>
    


    <!-- https://www.theworldavatar.com/kg/ontopoi/CosmeticsAndToiletriesAndPerfumes -->


    <owl:Class rdf:about="https://www.theworldavatar.com/kg/ontopoi/CosmeticsAndToiletriesAndPerfumes">
        <rdfs:subClassOf rdf:resource="https://www.theworldavatar.com/kg/ontopoi/ConsumerProducts"/>
        <rdfs:comment>Cosmetics, toiletries and perfumes is a subcategory of consumer products</rdfs:comment>
        <rdfs:isDefinedBy rdf:resource="https://www.theworldavatar.com/kg/ontopoi"/>
        <rdfs:label>Cosmetics, toiletries and perfumes</rdfs:label>
    </owl:Class>
    


    <!-- https://www.theworldavatar.com/kg/ontopoi/CosmeticsAndToiletriesAndPerfumesAndHairdressingSupplies -->


    <owl:Class rdf:about="https://www.theworldavatar.com/kg/ontopoi/CosmeticsAndToiletriesAndPerfumesAndHairdressingSupplies">
        <rdfs:subClassOf rdf:resource="https://www.theworldavatar.com/kg/ontopoi/HouseholdAndOfficeAndLeisureAndGarden"/>
        <rdfs:comment>Cosmetics, toiletries, perfumes and hairdressing supplies is a subcategory of household, office, leisure and garden</rdfs:comment>
        <rdfs:isDefinedBy rdf:resource="https://www.theworldavatar.com/kg/ontopoi"/>
        <rdfs:label>Cosmetics, toiletries, perfumes and hairdressing supplies</rdfs:label>
    </owl:Class>
    


    <!-- https://www.theworldavatar.com/kg/ontopoi/CounsellingAndAdviceServices -->


    <owl:Class rdf:about="https://www.theworldavatar.com/kg/ontopoi/CounsellingAndAdviceServices">
        <rdfs:subClassOf rdf:resource="https://www.theworldavatar.com/kg/ontopoi/HealthSupportServices"/>
        <rdfs:comment>Counselling and advice services is a subcategory of health support services</rdfs:comment>
        <rdfs:isDefinedBy rdf:resource="https://www.theworldavatar.com/kg/ontopoi"/>
        <rdfs:label>Counselling and advice services</rdfs:label>
    </owl:Class>
    


    <!-- https://www.theworldavatar.com/kg/ontopoi/CountryAndNationalParks -->


    <owl:Class rdf:about="https://www.theworldavatar.com/kg/ontopoi/CountryAndNationalParks">
        <rdfs:subClassOf rdf:resource="https://www.theworldavatar.com/kg/ontopoi/Recreational"/>
        <rdfs:comment>Country and national parks is a subcategory of recreational</rdfs:comment>
        <rdfs:isDefinedBy rdf:resource="https://www.theworldavatar.com/kg/ontopoi"/>
        <rdfs:label>Country and national parks</rdfs:label>
    </owl:Class>
    


    <!-- https://www.theworldavatar.com/kg/ontopoi/CourierAndDeliveryAndMessenger -->


    <owl:Class rdf:about="https://www.theworldavatar.com/kg/ontopoi/CourierAndDeliveryAndMessenger">
        <rdfs:subClassOf rdf:resource="https://www.theworldavatar.com/kg/ontopoi/TransportAndStorageAndDelivery"/>
        <rdfs:comment>Courier, delivery and messenger is a subcategory of transport, storage and delivery</rdfs:comment>
        <rdfs:isDefinedBy rdf:resource="https://www.theworldavatar.com/kg/ontopoi"/>
        <rdfs:label>Courier, delivery and messenger</rdfs:label>
    </owl:Class>
    


    <!-- https://www.theworldavatar.com/kg/ontopoi/CourtsAndCourtServicesAndTribunals -->


    <owl:Class rdf:about="https://www.theworldavatar.com/kg/ontopoi/CourtsAndCourtServicesAndTribunals">
        <rdfs:subClassOf rdf:resource="https://www.theworldavatar.com/kg/ontopoi/CentralAndLocalGovernment"/>
        <rdfs:comment>Courts, court services and tribunals is a subcategory of central and local government</rdfs:comment>
        <rdfs:isDefinedBy rdf:resource="https://www.theworldavatar.com/kg/ontopoi"/>
        <rdfs:label>Courts, court services and tribunals</rdfs:label>
    </owl:Class>
    


    <!-- https://www.theworldavatar.com/kg/ontopoi/CraftSupplies -->


    <owl:Class rdf:about="https://www.theworldavatar.com/kg/ontopoi/CraftSupplies">
        <rdfs:subClassOf rdf:resource="https://www.theworldavatar.com/kg/ontopoi/HouseholdAndOfficeAndLeisureAndGarden"/>
        <rdfs:comment>Craft supplies is a subcategory of household, office, leisure and garden</rdfs:comment>
        <rdfs:isDefinedBy rdf:resource="https://www.theworldavatar.com/kg/ontopoi"/>
        <rdfs:label>Craft supplies</rdfs:label>
    </owl:Class>
    


    <!-- https://www.theworldavatar.com/kg/ontopoi/CreditReferenceAgencies -->


    <owl:Class rdf:about="https://www.theworldavatar.com/kg/ontopoi/CreditReferenceAgencies">
        <rdfs:subClassOf rdf:resource="https://www.theworldavatar.com/kg/ontopoi/LegalAndFinancial"/>
        <rdfs:comment>Credit reference agencies is a subcategory of legal and financial</rdfs:comment>
        <rdfs:isDefinedBy rdf:resource="https://www.theworldavatar.com/kg/ontopoi"/>
        <rdfs:label>Credit reference agencies</rdfs:label>
    </owl:Class>
    


    <!-- https://www.theworldavatar.com/kg/ontopoi/CurrencyConversionAndMoneyTransfers -->


    <owl:Class rdf:about="https://www.theworldavatar.com/kg/ontopoi/CurrencyConversionAndMoneyTransfers">
        <rdfs:subClassOf rdf:resource="https://www.theworldavatar.com/kg/ontopoi/LegalAndFinancial"/>
        <rdfs:comment>Currency conversion and money transfers is a subcategory of legal and financial</rdfs:comment>
        <rdfs:isDefinedBy rdf:resource="https://www.theworldavatar.com/kg/ontopoi"/>
        <rdfs:label>Currency conversion and money transfers</rdfs:label>
    </owl:Class>
    


    <!-- https://www.theworldavatar.com/kg/ontopoi/CurtainsAndBlinds -->


    <owl:Class rdf:about="https://www.theworldavatar.com/kg/ontopoi/CurtainsAndBlinds">
        <rdfs:subClassOf rdf:resource="https://www.theworldavatar.com/kg/ontopoi/ConsumerProducts"/>
        <rdfs:comment>Curtains and blinds is a subcategory of consumer products</rdfs:comment>
        <rdfs:isDefinedBy rdf:resource="https://www.theworldavatar.com/kg/ontopoi"/>
        <rdfs:label>Curtains and blinds</rdfs:label>
    </owl:Class>
    


    <!-- https://www.theworldavatar.com/kg/ontopoi/CustomerServiceCentres -->


    <owl:Class rdf:about="https://www.theworldavatar.com/kg/ontopoi/CustomerServiceCentres">
        <rdfs:subClassOf rdf:resource="https://www.theworldavatar.com/kg/ontopoi/PersonalAndConsumerAndOtherServices"/>
        <rdfs:comment>Customer service centres is a subcategory of personal, consumer and other services</rdfs:comment>
        <rdfs:isDefinedBy rdf:resource="https://www.theworldavatar.com/kg/ontopoi"/>
        <rdfs:label>Customer service centres</rdfs:label>
    </owl:Class>
    


    <!-- https://www.theworldavatar.com/kg/ontopoi/CutleryAndTableware -->


    <owl:Class rdf:about="https://www.theworldavatar.com/kg/ontopoi/CutleryAndTableware">
        <rdfs:subClassOf rdf:resource="https://www.theworldavatar.com/kg/ontopoi/ConsumerProducts"/>
        <rdfs:comment>Cutlery and tableware is a subcategory of consumer products</rdfs:comment>
        <rdfs:isDefinedBy rdf:resource="https://www.theworldavatar.com/kg/ontopoi"/>
        <rdfs:label>Cutlery and tableware</rdfs:label>
    </owl:Class>
    


    <!-- https://www.theworldavatar.com/kg/ontopoi/CuttingAndDrillingAndWeldingServices -->


    <owl:Class rdf:about="https://www.theworldavatar.com/kg/ontopoi/CuttingAndDrillingAndWeldingServices">
        <rdfs:subClassOf rdf:resource="https://www.theworldavatar.com/kg/ontopoi/ConstructionServices"/>
        <rdfs:comment>Cutting, drilling and welding services is a subcategory of construction services</rdfs:comment>
        <rdfs:isDefinedBy rdf:resource="https://www.theworldavatar.com/kg/ontopoi"/>
        <rdfs:label>Cutting, drilling and welding services</rdfs:label>
    </owl:Class>
    


    <!-- https://www.theworldavatar.com/kg/ontopoi/CvWriters -->


    <owl:Class rdf:about="https://www.theworldavatar.com/kg/ontopoi/CvWriters">
        <rdfs:subClassOf rdf:resource="https://www.theworldavatar.com/kg/ontopoi/PersonalAndConsumerAndOtherServices"/>
        <rdfs:comment>Cv writers is a subcategory of personal, consumer and other services</rdfs:comment>
        <rdfs:isDefinedBy rdf:resource="https://www.theworldavatar.com/kg/ontopoi"/>
        <rdfs:label>CV writers</rdfs:label>
    </owl:Class>
    


    <!-- https://www.theworldavatar.com/kg/ontopoi/CyclesAndAccessories -->


    <owl:Class rdf:about="https://www.theworldavatar.com/kg/ontopoi/CyclesAndAccessories">
        <rdfs:subClassOf rdf:resource="https://www.theworldavatar.com/kg/ontopoi/HouseholdAndOfficeAndLeisureAndGarden"/>
        <rdfs:comment>Cycles and accessories is a subcategory of household, office, leisure and garden</rdfs:comment>
        <rdfs:isDefinedBy rdf:resource="https://www.theworldavatar.com/kg/ontopoi"/>
        <rdfs:label>Cycles and accessories</rdfs:label>
    </owl:Class>
    


    <!-- https://www.theworldavatar.com/kg/ontopoi/DairyFarming -->


    <owl:Class rdf:about="https://www.theworldavatar.com/kg/ontopoi/DairyFarming">
        <rdfs:subClassOf rdf:resource="https://www.theworldavatar.com/kg/ontopoi/Farming"/>
        <rdfs:comment>Dairy farming is a subcategory of farming</rdfs:comment>
        <rdfs:isDefinedBy rdf:resource="https://www.theworldavatar.com/kg/ontopoi"/>
        <rdfs:label>Dairy farming</rdfs:label>
    </owl:Class>
    


    <!-- https://www.theworldavatar.com/kg/ontopoi/DairyProducts -->


    <owl:Class rdf:about="https://www.theworldavatar.com/kg/ontopoi/DairyProducts">
        <rdfs:subClassOf rdf:resource="https://www.theworldavatar.com/kg/ontopoi/Foodstuffs"/>
        <rdfs:comment>Dairy products is a subcategory of foodstuffs</rdfs:comment>
        <rdfs:isDefinedBy rdf:resource="https://www.theworldavatar.com/kg/ontopoi"/>
        <rdfs:label>Dairy products</rdfs:label>
    </owl:Class>
    


    <!-- https://www.theworldavatar.com/kg/ontopoi/DatabaseServices -->


    <owl:Class rdf:about="https://www.theworldavatar.com/kg/ontopoi/DatabaseServices">
        <rdfs:subClassOf rdf:resource="https://www.theworldavatar.com/kg/ontopoi/ItAndAdvertisingAndMarketingAndMediaServiceS"/>
        <rdfs:comment>Database services is a subcategory of it, advertising, marketing and media service s</rdfs:comment>
        <rdfs:isDefinedBy rdf:resource="https://www.theworldavatar.com/kg/ontopoi"/>
        <rdfs:label>Database services</rdfs:label>
    </owl:Class>
    


    <!-- https://www.theworldavatar.com/kg/ontopoi/DayAndCareCentres -->


    <owl:Class rdf:about="https://www.theworldavatar.com/kg/ontopoi/DayAndCareCentres">
        <rdfs:subClassOf rdf:resource="https://www.theworldavatar.com/kg/ontopoi/HealthPractitionersAndEstablishments"/>
        <rdfs:comment>Day and care centres is a subcategory of health practitioners and establishments</rdfs:comment>
        <rdfs:isDefinedBy rdf:resource="https://www.theworldavatar.com/kg/ontopoi"/>
        <rdfs:label>Day and Care Centres</rdfs:label>
    </owl:Class>
    


    <!-- https://www.theworldavatar.com/kg/ontopoi/DebtCollectingAgencies -->


    <owl:Class rdf:about="https://www.theworldavatar.com/kg/ontopoi/DebtCollectingAgencies">
        <rdfs:subClassOf rdf:resource="https://www.theworldavatar.com/kg/ontopoi/LegalAndFinancial"/>
        <rdfs:comment>Debt collecting agencies is a subcategory of legal and financial</rdfs:comment>
        <rdfs:isDefinedBy rdf:resource="https://www.theworldavatar.com/kg/ontopoi"/>
        <rdfs:label>Debt collecting agencies</rdfs:label>
    </owl:Class>
    


    <!-- https://www.theworldavatar.com/kg/ontopoi/Delicatessens -->


    <owl:Class rdf:about="https://www.theworldavatar.com/kg/ontopoi/Delicatessens">
        <rdfs:subClassOf rdf:resource="https://www.theworldavatar.com/kg/ontopoi/FoodAndDrinkAndMultiItemRetail"/>
        <rdfs:comment>Delicatessens is a subcategory of food, drink and multi item retail</rdfs:comment>
        <rdfs:isDefinedBy rdf:resource="https://www.theworldavatar.com/kg/ontopoi"/>
        <rdfs:label>Delicatessens</rdfs:label>
    </owl:Class>
    


    <!-- https://www.theworldavatar.com/kg/ontopoi/DemolitionServices -->


    <owl:Class rdf:about="https://www.theworldavatar.com/kg/ontopoi/DemolitionServices">
        <rdfs:subClassOf rdf:resource="https://www.theworldavatar.com/kg/ontopoi/ConstructionServices"/>
        <rdfs:comment>Demolition services is a subcategory of construction services</rdfs:comment>
        <rdfs:isDefinedBy rdf:resource="https://www.theworldavatar.com/kg/ontopoi"/>
        <rdfs:label>Demolition services</rdfs:label>
    </owl:Class>
    


    <!-- https://www.theworldavatar.com/kg/ontopoi/DentalAndMedicalLaboratories -->


    <owl:Class rdf:about="https://www.theworldavatar.com/kg/ontopoi/DentalAndMedicalLaboratories">
        <rdfs:subClassOf rdf:resource="https://www.theworldavatar.com/kg/ontopoi/HealthPractitionersAndEstablishments"/>
        <rdfs:comment>Dental and medical laboratories is a subcategory of health practitioners and establishments</rdfs:comment>
        <rdfs:isDefinedBy rdf:resource="https://www.theworldavatar.com/kg/ontopoi"/>
        <rdfs:label>Dental and medical laboratories</rdfs:label>
    </owl:Class>
    


    <!-- https://www.theworldavatar.com/kg/ontopoi/DentalSurgeries -->


    <owl:Class rdf:about="https://www.theworldavatar.com/kg/ontopoi/DentalSurgeries">
        <rdfs:subClassOf rdf:resource="https://www.theworldavatar.com/kg/ontopoi/HealthPractitionersAndEstablishments"/>
        <rdfs:comment>Dental surgeries is a subcategory of health practitioners and establishments</rdfs:comment>
        <rdfs:isDefinedBy rdf:resource="https://www.theworldavatar.com/kg/ontopoi"/>
        <rdfs:label>Dental surgeries</rdfs:label>
    </owl:Class>
    


    <!-- https://www.theworldavatar.com/kg/ontopoi/DentalTechnicians -->


    <owl:Class rdf:about="https://www.theworldavatar.com/kg/ontopoi/DentalTechnicians">
        <rdfs:subClassOf rdf:resource="https://www.theworldavatar.com/kg/ontopoi/HealthPractitionersAndEstablishments"/>
        <rdfs:comment>Dental technicians is a subcategory of health practitioners and establishments</rdfs:comment>
        <rdfs:isDefinedBy rdf:resource="https://www.theworldavatar.com/kg/ontopoi"/>
        <rdfs:label>Dental technicians</rdfs:label>
    </owl:Class>
    


    <!-- https://www.theworldavatar.com/kg/ontopoi/DepartmentStores -->


    <owl:Class rdf:about="https://www.theworldavatar.com/kg/ontopoi/DepartmentStores">
        <rdfs:subClassOf rdf:resource="https://www.theworldavatar.com/kg/ontopoi/HouseholdAndOfficeAndLeisureAndGarden"/>
        <rdfs:comment>Department stores is a subcategory of household, office, leisure and garden</rdfs:comment>
        <rdfs:isDefinedBy rdf:resource="https://www.theworldavatar.com/kg/ontopoi"/>
        <rdfs:label>Department stores</rdfs:label>
    </owl:Class>
    


    <!-- https://www.theworldavatar.com/kg/ontopoi/DesignServices -->


    <owl:Class rdf:about="https://www.theworldavatar.com/kg/ontopoi/DesignServices">
        <rdfs:subClassOf rdf:resource="https://www.theworldavatar.com/kg/ontopoi/ResearchAndDesign"/>
        <rdfs:comment>Design services is a subcategory of research and design</rdfs:comment>
        <rdfs:isDefinedBy rdf:resource="https://www.theworldavatar.com/kg/ontopoi"/>
        <rdfs:label>Design services</rdfs:label>
    </owl:Class>
    


    <!-- https://www.theworldavatar.com/kg/ontopoi/DesignatedScenicFeatures -->


    <owl:Class rdf:about="https://www.theworldavatar.com/kg/ontopoi/DesignatedScenicFeatures">
        <rdfs:subClassOf rdf:resource="https://www.theworldavatar.com/kg/ontopoi/LandscapeFeatures"/>
        <rdfs:comment>Designated scenic features is a subcategory of landscape features</rdfs:comment>
        <rdfs:isDefinedBy rdf:resource="https://www.theworldavatar.com/kg/ontopoi"/>
        <rdfs:label>Designated scenic features</rdfs:label>
    </owl:Class>
    


    <!-- https://www.theworldavatar.com/kg/ontopoi/DesktopPublishingServices -->


    <owl:Class rdf:about="https://www.theworldavatar.com/kg/ontopoi/DesktopPublishingServices">
        <rdfs:subClassOf rdf:resource="https://www.theworldavatar.com/kg/ontopoi/ItAndAdvertisingAndMarketingAndMediaServiceS"/>
        <rdfs:comment>Desktop publishing services is a subcategory of it, advertising, marketing and media service s</rdfs:comment>
        <rdfs:isDefinedBy rdf:resource="https://www.theworldavatar.com/kg/ontopoi"/>
        <rdfs:label>Desktop publishing services</rdfs:label>
    </owl:Class>
    


    <!-- https://www.theworldavatar.com/kg/ontopoi/DetectiveAndInvestigationAgencies -->


    <owl:Class rdf:about="https://www.theworldavatar.com/kg/ontopoi/DetectiveAndInvestigationAgencies">
        <rdfs:subClassOf rdf:resource="https://www.theworldavatar.com/kg/ontopoi/PersonalAndConsumerAndOtherServices"/>
        <rdfs:comment>Detective and investigation agencies is a subcategory of personal, consumer and other services</rdfs:comment>
        <rdfs:isDefinedBy rdf:resource="https://www.theworldavatar.com/kg/ontopoi"/>
        <rdfs:label>Detective and investigation agencies</rdfs:label>
    </owl:Class>
    


    <!-- https://www.theworldavatar.com/kg/ontopoi/DieticiansAndNutritionists -->


    <owl:Class rdf:about="https://www.theworldavatar.com/kg/ontopoi/DieticiansAndNutritionists">
        <rdfs:subClassOf rdf:resource="https://www.theworldavatar.com/kg/ontopoi/HealthPractitionersAndEstablishments"/>
        <rdfs:comment>Dieticians and nutritionists is a subcategory of health practitioners and establishments</rdfs:comment>
        <rdfs:isDefinedBy rdf:resource="https://www.theworldavatar.com/kg/ontopoi"/>
        <rdfs:label>Dieticians and nutritionists</rdfs:label>
    </owl:Class>
    


    <!-- https://www.theworldavatar.com/kg/ontopoi/DisabilityAndMobilityEquipment -->


    <owl:Class rdf:about="https://www.theworldavatar.com/kg/ontopoi/DisabilityAndMobilityEquipment">
        <rdfs:subClassOf rdf:resource="https://www.theworldavatar.com/kg/ontopoi/ConsumerProducts"/>
        <rdfs:comment>Disability and mobility equipment is a subcategory of consumer products</rdfs:comment>
        <rdfs:isDefinedBy rdf:resource="https://www.theworldavatar.com/kg/ontopoi"/>
        <rdfs:label>Disability and mobility equipment</rdfs:label>
    </owl:Class>
    


    <!-- https://www.theworldavatar.com/kg/ontopoi/DiscountStores -->


    <owl:Class rdf:about="https://www.theworldavatar.com/kg/ontopoi/DiscountStores">
        <rdfs:subClassOf rdf:resource="https://www.theworldavatar.com/kg/ontopoi/HouseholdAndOfficeAndLeisureAndGarden"/>
        <rdfs:comment>Discount stores is a subcategory of household, office, leisure and garden</rdfs:comment>
        <rdfs:isDefinedBy rdf:resource="https://www.theworldavatar.com/kg/ontopoi"/>
        <rdfs:label>Discount stores</rdfs:label>
    </owl:Class>
    


    <!-- https://www.theworldavatar.com/kg/ontopoi/DisplayAndWindowDressers -->


    <owl:Class rdf:about="https://www.theworldavatar.com/kg/ontopoi/DisplayAndWindowDressers">
        <rdfs:subClassOf rdf:resource="https://www.theworldavatar.com/kg/ontopoi/ContractServices"/>
        <rdfs:comment>Display and window dressers is a subcategory of contract services</rdfs:comment>
        <rdfs:isDefinedBy rdf:resource="https://www.theworldavatar.com/kg/ontopoi"/>
        <rdfs:label>Display and window dressers</rdfs:label>
    </owl:Class>
    


    <!-- https://www.theworldavatar.com/kg/ontopoi/DisposableProducts -->


    <owl:Class rdf:about="https://www.theworldavatar.com/kg/ontopoi/DisposableProducts">
        <rdfs:subClassOf rdf:resource="https://www.theworldavatar.com/kg/ontopoi/ConsumerProducts"/>
        <rdfs:comment>Disposable products is a subcategory of consumer products</rdfs:comment>
        <rdfs:isDefinedBy rdf:resource="https://www.theworldavatar.com/kg/ontopoi"/>
        <rdfs:label>Disposable products</rdfs:label>
    </owl:Class>
    


    <!-- https://www.theworldavatar.com/kg/ontopoi/Distance -->


    <owl:Class rdf:about="https://www.theworldavatar.com/kg/ontopoi/Distance">
        <rdfs:subClassOf rdf:resource="http://www.ontology-of-units-of-measure.org/resource/om-2/Quantity"/>
        <rdfs:comment>A quantity indicating the distance of the nearest ITN from the POI</rdfs:comment>
        <rdfs:isDefinedBy rdf:resource="https://www.theworldavatar.com/kg/ontopoi"/>
        <rdfs:label>Distance</rdfs:label>
    </owl:Class>
    


    <!-- https://www.theworldavatar.com/kg/ontopoi/DistributionAndHaulage -->


    <owl:Class rdf:about="https://www.theworldavatar.com/kg/ontopoi/DistributionAndHaulage">
        <rdfs:subClassOf rdf:resource="https://www.theworldavatar.com/kg/ontopoi/TransportAndStorageAndDelivery"/>
        <rdfs:comment>Distribution and haulage is a subcategory of transport, storage and delivery</rdfs:comment>
        <rdfs:isDefinedBy rdf:resource="https://www.theworldavatar.com/kg/ontopoi"/>
        <rdfs:label>Distribution and haulage</rdfs:label>
    </owl:Class>
    


    <!-- https://www.theworldavatar.com/kg/ontopoi/DivingSchools -->


    <owl:Class rdf:about="https://www.theworldavatar.com/kg/ontopoi/DivingSchools">
        <rdfs:subClassOf rdf:resource="https://www.theworldavatar.com/kg/ontopoi/RecreationalAndVocationalEducation"/>
        <rdfs:comment>Diving schools is a subcategory of recreational and vocational education</rdfs:comment>
        <rdfs:isDefinedBy rdf:resource="https://www.theworldavatar.com/kg/ontopoi"/>
        <rdfs:label>Diving schools</rdfs:label>
    </owl:Class>
    


    <!-- https://www.theworldavatar.com/kg/ontopoi/DivingServices -->


    <owl:Class rdf:about="https://www.theworldavatar.com/kg/ontopoi/DivingServices">
        <rdfs:subClassOf rdf:resource="https://www.theworldavatar.com/kg/ontopoi/ConstructionServices"/>
        <rdfs:comment>Diving services is a subcategory of construction services</rdfs:comment>
        <rdfs:isDefinedBy rdf:resource="https://www.theworldavatar.com/kg/ontopoi"/>
        <rdfs:label>Diving services</rdfs:label>
    </owl:Class>
    


    <!-- https://www.theworldavatar.com/kg/ontopoi/DiyAndHomeImprovement -->


    <owl:Class rdf:about="https://www.theworldavatar.com/kg/ontopoi/DiyAndHomeImprovement">
        <rdfs:subClassOf rdf:resource="https://www.theworldavatar.com/kg/ontopoi/HouseholdAndOfficeAndLeisureAndGarden"/>
        <rdfs:comment>Diy and home improvement is a subcategory of household, office, leisure and garden</rdfs:comment>
        <rdfs:isDefinedBy rdf:resource="https://www.theworldavatar.com/kg/ontopoi"/>
        <rdfs:label>DIY and home improvement</rdfs:label>
    </owl:Class>
    


    <!-- https://www.theworldavatar.com/kg/ontopoi/DoctorsSurgeries -->


    <owl:Class rdf:about="https://www.theworldavatar.com/kg/ontopoi/DoctorsSurgeries">
        <rdfs:subClassOf rdf:resource="https://www.theworldavatar.com/kg/ontopoi/HealthPractitionersAndEstablishments"/>
        <rdfs:comment>Doctors surgeries is a subcategory of health practitioners and establishments</rdfs:comment>
        <rdfs:isDefinedBy rdf:resource="https://www.theworldavatar.com/kg/ontopoi"/>
        <rdfs:label>Doctors surgeries</rdfs:label>
    </owl:Class>
    


    <!-- https://www.theworldavatar.com/kg/ontopoi/DogTraining -->


    <owl:Class rdf:about="https://www.theworldavatar.com/kg/ontopoi/DogTraining">
        <rdfs:subClassOf rdf:resource="https://www.theworldavatar.com/kg/ontopoi/AnimalWelfare"/>
        <rdfs:comment>Dog training is a subcategory of animal welfare</rdfs:comment>
        <rdfs:isDefinedBy rdf:resource="https://www.theworldavatar.com/kg/ontopoi"/>
        <rdfs:label>Dog training</rdfs:label>
    </owl:Class>
    


    <!-- https://www.theworldavatar.com/kg/ontopoi/DomesticAppliances -->


    <owl:Class rdf:about="https://www.theworldavatar.com/kg/ontopoi/DomesticAppliances">
        <rdfs:subClassOf rdf:resource="https://www.theworldavatar.com/kg/ontopoi/HouseholdAndOfficeAndLeisureAndGarden"/>
        <rdfs:comment>Domestic appliances is a subcategory of household, office, leisure and garden</rdfs:comment>
        <rdfs:isDefinedBy rdf:resource="https://www.theworldavatar.com/kg/ontopoi"/>
        <rdfs:label>Domestic appliances</rdfs:label>
    </owl:Class>
    


    <!-- https://www.theworldavatar.com/kg/ontopoi/DomesticStaffAndHomeHelp -->


    <owl:Class rdf:about="https://www.theworldavatar.com/kg/ontopoi/DomesticStaffAndHomeHelp">
        <rdfs:subClassOf rdf:resource="https://www.theworldavatar.com/kg/ontopoi/EmploymentAndCareerAgencies"/>
        <rdfs:comment>Domestic staff and home help is a subcategory of employment and career agencies</rdfs:comment>
        <rdfs:isDefinedBy rdf:resource="https://www.theworldavatar.com/kg/ontopoi"/>
        <rdfs:label>Domestic staff and home help</rdfs:label>
    </owl:Class>
    


    <!-- https://www.theworldavatar.com/kg/ontopoi/DrainAndSewageClearance -->


    <owl:Class rdf:about="https://www.theworldavatar.com/kg/ontopoi/DrainAndSewageClearance">
        <rdfs:subClassOf rdf:resource="https://www.theworldavatar.com/kg/ontopoi/ContractServices"/>
        <rdfs:comment>Drain and sewage clearance is a subcategory of contract services</rdfs:comment>
        <rdfs:isDefinedBy rdf:resource="https://www.theworldavatar.com/kg/ontopoi"/>
        <rdfs:label>Drain and sewage clearance</rdfs:label>
    </owl:Class>
    


    <!-- https://www.theworldavatar.com/kg/ontopoi/DramaSchools -->


    <owl:Class rdf:about="https://www.theworldavatar.com/kg/ontopoi/DramaSchools">
        <rdfs:subClassOf rdf:resource="https://www.theworldavatar.com/kg/ontopoi/RecreationalAndVocationalEducation"/>
        <rdfs:comment>Drama schools is a subcategory of recreational and vocational education</rdfs:comment>
        <rdfs:isDefinedBy rdf:resource="https://www.theworldavatar.com/kg/ontopoi"/>
        <rdfs:label>Drama schools</rdfs:label>
    </owl:Class>
    


    <!-- https://www.theworldavatar.com/kg/ontopoi/DrinkingFountainsAndWaterPoints -->


    <owl:Class rdf:about="https://www.theworldavatar.com/kg/ontopoi/DrinkingFountainsAndWaterPoints">
        <rdfs:subClassOf rdf:resource="https://www.theworldavatar.com/kg/ontopoi/InfrastructureAndFacilities"/>
        <rdfs:comment>Drinking fountains and water points is a subcategory of infrastructure and facilities</rdfs:comment>
        <rdfs:isDefinedBy rdf:resource="https://www.theworldavatar.com/kg/ontopoi"/>
        <rdfs:label>Drinking fountains and water points</rdfs:label>
    </owl:Class>
    


    <!-- https://www.theworldavatar.com/kg/ontopoi/DriverAgencies -->


    <owl:Class rdf:about="https://www.theworldavatar.com/kg/ontopoi/DriverAgencies">
        <rdfs:subClassOf rdf:resource="https://www.theworldavatar.com/kg/ontopoi/EmploymentAndCareerAgencies"/>
        <rdfs:comment>Driver agencies is a subcategory of employment and career agencies</rdfs:comment>
        <rdfs:isDefinedBy rdf:resource="https://www.theworldavatar.com/kg/ontopoi"/>
        <rdfs:label>Driver agencies</rdfs:label>
    </owl:Class>
    


    <!-- https://www.theworldavatar.com/kg/ontopoi/DrivingAndMotorcycleSchools -->


    <owl:Class rdf:about="https://www.theworldavatar.com/kg/ontopoi/DrivingAndMotorcycleSchools">
        <rdfs:subClassOf rdf:resource="https://www.theworldavatar.com/kg/ontopoi/RecreationalAndVocationalEducation"/>
        <rdfs:comment>Driving and motorcycle schools is a subcategory of recreational and vocational education</rdfs:comment>
        <rdfs:isDefinedBy rdf:resource="https://www.theworldavatar.com/kg/ontopoi"/>
        <rdfs:label>Driving and motorcycle schools</rdfs:label>
    </owl:Class>
    


    <!-- https://www.theworldavatar.com/kg/ontopoi/DrivingTestCentres -->


    <owl:Class rdf:about="https://www.theworldavatar.com/kg/ontopoi/DrivingTestCentres">
        <rdfs:subClassOf rdf:resource="https://www.theworldavatar.com/kg/ontopoi/CentralAndLocalGovernment"/>
        <rdfs:comment>Driving test centres is a subcategory of central and local government</rdfs:comment>
        <rdfs:isDefinedBy rdf:resource="https://www.theworldavatar.com/kg/ontopoi"/>
        <rdfs:label>Driving test centres</rdfs:label>
    </owl:Class>
    


    <!-- https://www.theworldavatar.com/kg/ontopoi/EatingAndDrinking -->


    <owl:Class rdf:about="https://www.theworldavatar.com/kg/ontopoi/EatingAndDrinking">
        <rdfs:subClassOf rdf:resource="https://www.theworldavatar.com/kg/ontopoi/AccommodationAndEatingAndDrinking"/>
        <rdfs:comment>Eating and drinking is a subcategory of accommodation, eating and drinking</rdfs:comment>
        <rdfs:isDefinedBy rdf:resource="https://www.theworldavatar.com/kg/ontopoi"/>
        <rdfs:label>Eating and drinking</rdfs:label>
    </owl:Class>
    


    <!-- https://www.theworldavatar.com/kg/ontopoi/EducationAndHealth -->


    <owl:Class rdf:about="https://www.theworldavatar.com/kg/ontopoi/EducationAndHealth">
        <rdfs:subClassOf rdf:resource="https://www.theworldavatar.com/kg/ontopoi/PointOfInterest"/>
        <rdfs:comment>Establishments and services that focus on the development, well-being, and overall quality of life of individuals, pets, or communities</rdfs:comment>
        <rdfs:isDefinedBy rdf:resource="https://www.theworldavatar.com/kg/ontopoi"/>
        <rdfs:label>Education and health</rdfs:label>
    </owl:Class>
    


    <!-- https://www.theworldavatar.com/kg/ontopoi/EducationAuthorities -->


    <owl:Class rdf:about="https://www.theworldavatar.com/kg/ontopoi/EducationAuthorities">
        <rdfs:subClassOf rdf:resource="https://www.theworldavatar.com/kg/ontopoi/EducationSupportServices"/>
        <rdfs:comment>Education authorities is a subcategory of education support services</rdfs:comment>
        <rdfs:isDefinedBy rdf:resource="https://www.theworldavatar.com/kg/ontopoi"/>
        <rdfs:label>Education authorities</rdfs:label>
    </owl:Class>
    


    <!-- https://www.theworldavatar.com/kg/ontopoi/EducationServices -->


    <owl:Class rdf:about="https://www.theworldavatar.com/kg/ontopoi/EducationServices">
        <rdfs:subClassOf rdf:resource="https://www.theworldavatar.com/kg/ontopoi/EducationSupportServices"/>
        <rdfs:comment>Education services is a subcategory of education support services</rdfs:comment>
        <rdfs:isDefinedBy rdf:resource="https://www.theworldavatar.com/kg/ontopoi"/>
        <rdfs:label>Education services</rdfs:label>
    </owl:Class>
    


    <!-- https://www.theworldavatar.com/kg/ontopoi/EducationSupportServices -->


    <owl:Class rdf:about="https://www.theworldavatar.com/kg/ontopoi/EducationSupportServices">
        <rdfs:subClassOf rdf:resource="https://www.theworldavatar.com/kg/ontopoi/EducationAndHealth"/>
        <rdfs:comment>Education support services is a subcategory of education and health</rdfs:comment>
        <rdfs:isDefinedBy rdf:resource="https://www.theworldavatar.com/kg/ontopoi"/>
        <rdfs:label>Education support services</rdfs:label>
    </owl:Class>
    


    <!-- https://www.theworldavatar.com/kg/ontopoi/EducationalEquipmentAndSupplies -->


    <owl:Class rdf:about="https://www.theworldavatar.com/kg/ontopoi/EducationalEquipmentAndSupplies">
        <rdfs:subClassOf rdf:resource="https://www.theworldavatar.com/kg/ontopoi/IndustrialProducts"/>
        <rdfs:comment>Educational equipment and supplies is a subcategory of industrial products</rdfs:comment>
        <rdfs:isDefinedBy rdf:resource="https://www.theworldavatar.com/kg/ontopoi"/>
        <rdfs:label>Educational equipment and supplies</rdfs:label>
    </owl:Class>
    


    <!-- https://www.theworldavatar.com/kg/ontopoi/ElectricalAndElectronicEngineers -->


    <owl:Class rdf:about="https://www.theworldavatar.com/kg/ontopoi/ElectricalAndElectronicEngineers">
        <rdfs:subClassOf rdf:resource="https://www.theworldavatar.com/kg/ontopoi/EngineeringServices"/>
        <rdfs:comment>Electrical and electronic engineers is a subcategory of engineering services</rdfs:comment>
        <rdfs:isDefinedBy rdf:resource="https://www.theworldavatar.com/kg/ontopoi"/>
        <rdfs:label>Electrical and electronic engineers</rdfs:label>
    </owl:Class>
    


    <!-- https://www.theworldavatar.com/kg/ontopoi/ElectricalComponents -->


    <owl:Class rdf:about="https://www.theworldavatar.com/kg/ontopoi/ElectricalComponents">
        <rdfs:subClassOf rdf:resource="https://www.theworldavatar.com/kg/ontopoi/IndustrialProducts"/>
        <rdfs:comment>Electrical components is a subcategory of industrial products</rdfs:comment>
        <rdfs:isDefinedBy rdf:resource="https://www.theworldavatar.com/kg/ontopoi"/>
        <rdfs:label>Electrical components</rdfs:label>
    </owl:Class>
    


    <!-- https://www.theworldavatar.com/kg/ontopoi/ElectricalContractors -->


    <owl:Class rdf:about="https://www.theworldavatar.com/kg/ontopoi/ElectricalContractors">
        <rdfs:subClassOf rdf:resource="https://www.theworldavatar.com/kg/ontopoi/ConstructionServices"/>
        <rdfs:comment>Electrical contractors is a subcategory of construction services</rdfs:comment>
        <rdfs:isDefinedBy rdf:resource="https://www.theworldavatar.com/kg/ontopoi"/>
        <rdfs:label>Electrical contractors</rdfs:label>
    </owl:Class>
    


    <!-- https://www.theworldavatar.com/kg/ontopoi/ElectricalEquipmentRepairAndServicing -->


    <owl:Class rdf:about="https://www.theworldavatar.com/kg/ontopoi/ElectricalEquipmentRepairAndServicing">
        <rdfs:subClassOf rdf:resource="https://www.theworldavatar.com/kg/ontopoi/RepairAndServicing"/>
        <rdfs:comment>Electrical equipment repair and servicing is a subcategory of repair and servicing</rdfs:comment>
        <rdfs:isDefinedBy rdf:resource="https://www.theworldavatar.com/kg/ontopoi"/>
        <rdfs:label>Electrical equipment repair and servicing</rdfs:label>
    </owl:Class>
    


    <!-- https://www.theworldavatar.com/kg/ontopoi/ElectricalFeatures -->


    <owl:Class rdf:about="https://www.theworldavatar.com/kg/ontopoi/ElectricalFeatures">
        <rdfs:subClassOf rdf:resource="https://www.theworldavatar.com/kg/ontopoi/InfrastructureAndFacilities"/>
        <rdfs:comment>Electrical features is a subcategory of infrastructure and facilities</rdfs:comment>
        <rdfs:isDefinedBy rdf:resource="https://www.theworldavatar.com/kg/ontopoi"/>
        <rdfs:label>Electrical features</rdfs:label>
    </owl:Class>
    


    <!-- https://www.theworldavatar.com/kg/ontopoi/ElectricalGoodsAndComponents -->


    <owl:Class rdf:about="https://www.theworldavatar.com/kg/ontopoi/ElectricalGoodsAndComponents">
        <rdfs:subClassOf rdf:resource="https://www.theworldavatar.com/kg/ontopoi/HouseholdAndOfficeAndLeisureAndGarden"/>
        <rdfs:comment>Electrical goods and components is a subcategory of household, office, leisure and garden</rdfs:comment>
        <rdfs:isDefinedBy rdf:resource="https://www.theworldavatar.com/kg/ontopoi"/>
        <rdfs:label>Electrical goods and components</rdfs:label>
    </owl:Class>
    


    <!-- https://www.theworldavatar.com/kg/ontopoi/ElectricalMotorsAndGenerators -->


    <owl:Class rdf:about="https://www.theworldavatar.com/kg/ontopoi/ElectricalMotorsAndGenerators">
        <rdfs:subClassOf rdf:resource="https://www.theworldavatar.com/kg/ontopoi/IndustrialProducts"/>
        <rdfs:comment>Electrical motors and generators is a subcategory of industrial products</rdfs:comment>
        <rdfs:isDefinedBy rdf:resource="https://www.theworldavatar.com/kg/ontopoi"/>
        <rdfs:label>Electrical motors and generators</rdfs:label>
    </owl:Class>
    


    <!-- https://www.theworldavatar.com/kg/ontopoi/ElectricalProductionAndManipulationEquipment -->


    <owl:Class rdf:about="https://www.theworldavatar.com/kg/ontopoi/ElectricalProductionAndManipulationEquipment">
        <rdfs:subClassOf rdf:resource="https://www.theworldavatar.com/kg/ontopoi/IndustrialProducts"/>
        <rdfs:comment>Electrical production and manipulation equipment is a subcategory of industrial products</rdfs:comment>
        <rdfs:isDefinedBy rdf:resource="https://www.theworldavatar.com/kg/ontopoi"/>
        <rdfs:label>Electrical production and manipulation equipment</rdfs:label>
    </owl:Class>
    


    <!-- https://www.theworldavatar.com/kg/ontopoi/ElectronicAndInternetPublishers -->


    <owl:Class rdf:about="https://www.theworldavatar.com/kg/ontopoi/ElectronicAndInternetPublishers">
        <rdfs:subClassOf rdf:resource="https://www.theworldavatar.com/kg/ontopoi/ItAndAdvertisingAndMarketingAndMediaServiceS"/>
        <rdfs:comment>Electronic and internet publishers is a subcategory of it, advertising, marketing and media service s</rdfs:comment>
        <rdfs:isDefinedBy rdf:resource="https://www.theworldavatar.com/kg/ontopoi"/>
        <rdfs:label>Electronic and Internet publishers</rdfs:label>
    </owl:Class>
    


    <!-- https://www.theworldavatar.com/kg/ontopoi/ElectronicEquipment -->


    <owl:Class rdf:about="https://www.theworldavatar.com/kg/ontopoi/ElectronicEquipment">
        <rdfs:subClassOf rdf:resource="https://www.theworldavatar.com/kg/ontopoi/IndustrialProducts"/>
        <rdfs:comment>Electronic equipment is a subcategory of industrial products</rdfs:comment>
        <rdfs:isDefinedBy rdf:resource="https://www.theworldavatar.com/kg/ontopoi"/>
        <rdfs:label>Electronic equipment</rdfs:label>
    </owl:Class>
    


    <!-- https://www.theworldavatar.com/kg/ontopoi/ElectronicMedia -->


    <owl:Class rdf:about="https://www.theworldavatar.com/kg/ontopoi/ElectronicMedia">
        <rdfs:subClassOf rdf:resource="https://www.theworldavatar.com/kg/ontopoi/IndustrialProducts"/>
        <rdfs:comment>Electronic media is a subcategory of industrial products</rdfs:comment>
        <rdfs:isDefinedBy rdf:resource="https://www.theworldavatar.com/kg/ontopoi"/>
        <rdfs:label>Electronic media</rdfs:label>
    </owl:Class>
    


    <!-- https://www.theworldavatar.com/kg/ontopoi/EmbassiesAndConsulates -->


    <owl:Class rdf:about="https://www.theworldavatar.com/kg/ontopoi/EmbassiesAndConsulates">
        <rdfs:subClassOf rdf:resource="https://www.theworldavatar.com/kg/ontopoi/CentralAndLocalGovernment"/>
        <rdfs:comment>Embassies and consulates is a subcategory of central and local government</rdfs:comment>
        <rdfs:isDefinedBy rdf:resource="https://www.theworldavatar.com/kg/ontopoi"/>
        <rdfs:label>Embassies and consulates</rdfs:label>
    </owl:Class>
    


    <!-- https://www.theworldavatar.com/kg/ontopoi/EmploymentAgencies -->


    <owl:Class rdf:about="https://www.theworldavatar.com/kg/ontopoi/EmploymentAgencies">
        <rdfs:subClassOf rdf:resource="https://www.theworldavatar.com/kg/ontopoi/EmploymentAndCareerAgencies"/>
        <rdfs:comment>Employment agencies is a subcategory of employment and career agencies</rdfs:comment>
        <rdfs:isDefinedBy rdf:resource="https://www.theworldavatar.com/kg/ontopoi"/>
        <rdfs:label>Employment agencies</rdfs:label>
    </owl:Class>
    


    <!-- https://www.theworldavatar.com/kg/ontopoi/EmploymentAndCareerAgencies -->


    <owl:Class rdf:about="https://www.theworldavatar.com/kg/ontopoi/EmploymentAndCareerAgencies">
        <rdfs:subClassOf rdf:resource="https://www.theworldavatar.com/kg/ontopoi/CommercialServices"/>
        <rdfs:comment>Employment and career agencies is a subcategory of commercial services</rdfs:comment>
        <rdfs:isDefinedBy rdf:resource="https://www.theworldavatar.com/kg/ontopoi"/>
        <rdfs:label>Employment and career agencies</rdfs:label>
    </owl:Class>
    


    <!-- https://www.theworldavatar.com/kg/ontopoi/EnergyProduction -->


    <owl:Class rdf:about="https://www.theworldavatar.com/kg/ontopoi/EnergyProduction">
        <rdfs:subClassOf rdf:resource="https://www.theworldavatar.com/kg/ontopoi/IndustrialFeatures"/>
        <rdfs:comment>Energy production is a subcategory of industrial features</rdfs:comment>
        <rdfs:isDefinedBy rdf:resource="https://www.theworldavatar.com/kg/ontopoi"/>
        <rdfs:label>Energy production</rdfs:label>
    </owl:Class>
    


    <!-- https://www.theworldavatar.com/kg/ontopoi/EngineeringServices -->


    <owl:Class rdf:about="https://www.theworldavatar.com/kg/ontopoi/EngineeringServices">
        <rdfs:subClassOf rdf:resource="https://www.theworldavatar.com/kg/ontopoi/CommercialServices"/>
        <rdfs:comment>Engineering services is a subcategory of commercial services</rdfs:comment>
        <rdfs:isDefinedBy rdf:resource="https://www.theworldavatar.com/kg/ontopoi"/>
        <rdfs:label>Engineering services</rdfs:label>
    </owl:Class>
    


    <!-- https://www.theworldavatar.com/kg/ontopoi/Engines -->


    <owl:Class rdf:about="https://www.theworldavatar.com/kg/ontopoi/Engines">
        <rdfs:subClassOf rdf:resource="https://www.theworldavatar.com/kg/ontopoi/IndustrialProducts"/>
        <rdfs:comment>Engines is a subcategory of industrial products</rdfs:comment>
        <rdfs:isDefinedBy rdf:resource="https://www.theworldavatar.com/kg/ontopoi"/>
        <rdfs:label>Engines</rdfs:label>
    </owl:Class>
    


    <!-- https://www.theworldavatar.com/kg/ontopoi/EntertainmentServices -->


    <owl:Class rdf:about="https://www.theworldavatar.com/kg/ontopoi/EntertainmentServices">
        <rdfs:subClassOf rdf:resource="https://www.theworldavatar.com/kg/ontopoi/SportAndEntertainmentSupportServices"/>
        <rdfs:comment>Entertainment services is a subcategory of sport and entertainment support services</rdfs:comment>
        <rdfs:isDefinedBy rdf:resource="https://www.theworldavatar.com/kg/ontopoi"/>
        <rdfs:label>Entertainment services</rdfs:label>
    </owl:Class>
    


    <!-- https://www.theworldavatar.com/kg/ontopoi/EstateAndPropertyManagement -->


    <owl:Class rdf:about="https://www.theworldavatar.com/kg/ontopoi/EstateAndPropertyManagement">
        <rdfs:subClassOf rdf:resource="https://www.theworldavatar.com/kg/ontopoi/PropertyAndDevelopmentServices"/>
        <rdfs:comment>Estate and property management is a subcategory of property and development services</rdfs:comment>
        <rdfs:isDefinedBy rdf:resource="https://www.theworldavatar.com/kg/ontopoi"/>
        <rdfs:label>Estate and property management</rdfs:label>
    </owl:Class>
    


    <!-- https://www.theworldavatar.com/kg/ontopoi/EventTicketAgentsAndBoxOffice -->


    <owl:Class rdf:about="https://www.theworldavatar.com/kg/ontopoi/EventTicketAgentsAndBoxOffice">
        <rdfs:subClassOf rdf:resource="https://www.theworldavatar.com/kg/ontopoi/PersonalAndConsumerAndOtherServices"/>
        <rdfs:comment>Event ticket agents and box office is a subcategory of personal, consumer and other services</rdfs:comment>
        <rdfs:isDefinedBy rdf:resource="https://www.theworldavatar.com/kg/ontopoi"/>
        <rdfs:label>Event Ticket Agents and Box Office</rdfs:label>
    </owl:Class>
    


    <!-- https://www.theworldavatar.com/kg/ontopoi/ExaminationBoards -->


    <owl:Class rdf:about="https://www.theworldavatar.com/kg/ontopoi/ExaminationBoards">
        <rdfs:subClassOf rdf:resource="https://www.theworldavatar.com/kg/ontopoi/EducationSupportServices"/>
        <rdfs:comment>Examination boards is a subcategory of education support services</rdfs:comment>
        <rdfs:isDefinedBy rdf:resource="https://www.theworldavatar.com/kg/ontopoi"/>
        <rdfs:label>Examination boards</rdfs:label>
    </owl:Class>
    


    <!-- https://www.theworldavatar.com/kg/ontopoi/ExtractiveIndustries -->


    <owl:Class rdf:about="https://www.theworldavatar.com/kg/ontopoi/ExtractiveIndustries">
        <rdfs:subClassOf rdf:resource="https://www.theworldavatar.com/kg/ontopoi/ManufacturingAndProduction"/>
        <rdfs:comment>Extractive industries is a subcategory of manufacturing and production</rdfs:comment>
        <rdfs:isDefinedBy rdf:resource="https://www.theworldavatar.com/kg/ontopoi"/>
        <rdfs:label>Extractive industries</rdfs:label>
    </owl:Class>
    


    <!-- https://www.theworldavatar.com/kg/ontopoi/FanClubsAndAssociations -->


    <owl:Class rdf:about="https://www.theworldavatar.com/kg/ontopoi/FanClubsAndAssociations">
        <rdfs:subClassOf rdf:resource="https://www.theworldavatar.com/kg/ontopoi/Organisations"/>
        <rdfs:comment>Fan clubs and associations is a subcategory of organisations</rdfs:comment>
        <rdfs:isDefinedBy rdf:resource="https://www.theworldavatar.com/kg/ontopoi"/>
        <rdfs:label>Fan clubs and associations</rdfs:label>
    </owl:Class>
    


    <!-- https://www.theworldavatar.com/kg/ontopoi/Farm-BasedAttractions -->


    <owl:Class rdf:about="https://www.theworldavatar.com/kg/ontopoi/Farm-BasedAttractions">
        <rdfs:subClassOf rdf:resource="https://www.theworldavatar.com/kg/ontopoi/BotanicalAndZoological"/>
        <rdfs:comment>Farm-based attractions is a subcategory of botanical and zoological</rdfs:comment>
        <rdfs:isDefinedBy rdf:resource="https://www.theworldavatar.com/kg/ontopoi"/>
        <rdfs:label>Farm-based attractions</rdfs:label>
    </owl:Class>
    


    <!-- https://www.theworldavatar.com/kg/ontopoi/Farming -->


    <owl:Class rdf:about="https://www.theworldavatar.com/kg/ontopoi/Farming">
        <rdfs:subClassOf rdf:resource="https://www.theworldavatar.com/kg/ontopoi/ManufacturingAndProduction"/>
        <rdfs:comment>Farming is a subcategory of manufacturing and production</rdfs:comment>
        <rdfs:isDefinedBy rdf:resource="https://www.theworldavatar.com/kg/ontopoi"/>
        <rdfs:label>Farming</rdfs:label>
    </owl:Class>
    


    <!-- https://www.theworldavatar.com/kg/ontopoi/FastFoodAndTakeawayOutlets -->


    <owl:Class rdf:about="https://www.theworldavatar.com/kg/ontopoi/FastFoodAndTakeawayOutlets">
        <rdfs:subClassOf rdf:resource="https://www.theworldavatar.com/kg/ontopoi/EatingAndDrinking"/>
        <rdfs:comment>Fast food and takeaway outlets is a subcategory of eating and drinking</rdfs:comment>
        <rdfs:isDefinedBy rdf:resource="https://www.theworldavatar.com/kg/ontopoi"/>
        <rdfs:label>Fast food and takeaway outlets</rdfs:label>
    </owl:Class>
    


    <!-- https://www.theworldavatar.com/kg/ontopoi/FastFoodDeliveryServices -->


    <owl:Class rdf:about="https://www.theworldavatar.com/kg/ontopoi/FastFoodDeliveryServices">
        <rdfs:subClassOf rdf:resource="https://www.theworldavatar.com/kg/ontopoi/EatingAndDrinking"/>
        <rdfs:comment>Fast food delivery services is a subcategory of eating and drinking</rdfs:comment>
        <rdfs:isDefinedBy rdf:resource="https://www.theworldavatar.com/kg/ontopoi"/>
        <rdfs:label>Fast food delivery services</rdfs:label>
    </owl:Class>
    


    <!-- https://www.theworldavatar.com/kg/ontopoi/FencesAndGatesAndRailings -->


    <owl:Class rdf:about="https://www.theworldavatar.com/kg/ontopoi/FencesAndGatesAndRailings">
        <rdfs:subClassOf rdf:resource="https://www.theworldavatar.com/kg/ontopoi/IndustrialProducts"/>
        <rdfs:comment>Fences, gates and railings is a subcategory of industrial products</rdfs:comment>
        <rdfs:isDefinedBy rdf:resource="https://www.theworldavatar.com/kg/ontopoi"/>
        <rdfs:label>Fences, gates and railings</rdfs:label>
    </owl:Class>
    


    <!-- https://www.theworldavatar.com/kg/ontopoi/FencingAndDrystoneWallingServices -->


    <owl:Class rdf:about="https://www.theworldavatar.com/kg/ontopoi/FencingAndDrystoneWallingServices">
        <rdfs:subClassOf rdf:resource="https://www.theworldavatar.com/kg/ontopoi/ConstructionServices"/>
        <rdfs:comment>Fencing and drystone walling services is a subcategory of construction services</rdfs:comment>
        <rdfs:isDefinedBy rdf:resource="https://www.theworldavatar.com/kg/ontopoi"/>
        <rdfs:label>Fencing and drystone walling services</rdfs:label>
    </owl:Class>
    


    <!-- https://www.theworldavatar.com/kg/ontopoi/FengShuiConsultantsAndFurnishersAndShopFitters -->


    <owl:Class rdf:about="https://www.theworldavatar.com/kg/ontopoi/FengShuiConsultantsAndFurnishersAndShopFitters">
        <rdfs:subClassOf rdf:resource="https://www.theworldavatar.com/kg/ontopoi/Consultancies"/>
        <rdfs:comment>Feng shui consultants, furnishers and shop fitters is a subcategory of consultancies</rdfs:comment>
        <rdfs:isDefinedBy rdf:resource="https://www.theworldavatar.com/kg/ontopoi"/>
        <rdfs:label>Feng shui consultants, furnishers and shop fitters</rdfs:label>
    </owl:Class>
    


    <!-- https://www.theworldavatar.com/kg/ontopoi/FerriesAndFerryTerminals -->


    <owl:Class rdf:about="https://www.theworldavatar.com/kg/ontopoi/FerriesAndFerryTerminals">
        <rdfs:subClassOf rdf:resource="https://www.theworldavatar.com/kg/ontopoi/Water"/>
        <rdfs:comment>Ferries and ferry terminals is a subcategory of water</rdfs:comment>
        <rdfs:isDefinedBy rdf:resource="https://www.theworldavatar.com/kg/ontopoi"/>
        <rdfs:label>Ferries and ferry terminals</rdfs:label>
    </owl:Class>
    


    <!-- https://www.theworldavatar.com/kg/ontopoi/FerryAndCruiseCompanies -->


    <owl:Class rdf:about="https://www.theworldavatar.com/kg/ontopoi/FerryAndCruiseCompanies">
        <rdfs:subClassOf rdf:resource="https://www.theworldavatar.com/kg/ontopoi/TransportAndStorageAndDelivery"/>
        <rdfs:comment>Ferry and cruise companies is a subcategory of transport, storage and delivery</rdfs:comment>
        <rdfs:isDefinedBy rdf:resource="https://www.theworldavatar.com/kg/ontopoi"/>
        <rdfs:label>Ferry and cruise companies</rdfs:label>
    </owl:Class>
    


    <!-- https://www.theworldavatar.com/kg/ontopoi/Fertilisers -->


    <owl:Class rdf:about="https://www.theworldavatar.com/kg/ontopoi/Fertilisers">
        <rdfs:subClassOf rdf:resource="https://www.theworldavatar.com/kg/ontopoi/IndustrialProducts"/>
        <rdfs:comment>Fertilisers is a subcategory of industrial products</rdfs:comment>
        <rdfs:isDefinedBy rdf:resource="https://www.theworldavatar.com/kg/ontopoi"/>
        <rdfs:label>Fertilisers</rdfs:label>
    </owl:Class>
    


    <!-- https://www.theworldavatar.com/kg/ontopoi/FilmAndVideoServices -->


    <owl:Class rdf:about="https://www.theworldavatar.com/kg/ontopoi/FilmAndVideoServices">
        <rdfs:subClassOf rdf:resource="https://www.theworldavatar.com/kg/ontopoi/ItAndAdvertisingAndMarketingAndMediaServiceS"/>
        <rdfs:comment>Film and video services is a subcategory of it, advertising, marketing and media service s</rdfs:comment>
        <rdfs:isDefinedBy rdf:resource="https://www.theworldavatar.com/kg/ontopoi"/>
        <rdfs:label>Film and video services</rdfs:label>
    </owl:Class>
    


    <!-- https://www.theworldavatar.com/kg/ontopoi/FinancialAdviceServices -->


    <owl:Class rdf:about="https://www.theworldavatar.com/kg/ontopoi/FinancialAdviceServices">
        <rdfs:subClassOf rdf:resource="https://www.theworldavatar.com/kg/ontopoi/LegalAndFinancial"/>
        <rdfs:comment>Financial advice services is a subcategory of legal and financial</rdfs:comment>
        <rdfs:isDefinedBy rdf:resource="https://www.theworldavatar.com/kg/ontopoi"/>
        <rdfs:label>Financial advice services</rdfs:label>
    </owl:Class>
    


    <!-- https://www.theworldavatar.com/kg/ontopoi/FireBrigadeStations -->


    <owl:Class rdf:about="https://www.theworldavatar.com/kg/ontopoi/FireBrigadeStations">
        <rdfs:subClassOf rdf:resource="https://www.theworldavatar.com/kg/ontopoi/CentralAndLocalGovernment"/>
        <rdfs:comment>Fire brigade stations is a subcategory of central and local government</rdfs:comment>
        <rdfs:isDefinedBy rdf:resource="https://www.theworldavatar.com/kg/ontopoi"/>
        <rdfs:label>Fire brigade stations</rdfs:label>
    </owl:Class>
    


    <!-- https://www.theworldavatar.com/kg/ontopoi/FireplacesAndMantelpieces -->


    <owl:Class rdf:about="https://www.theworldavatar.com/kg/ontopoi/FireplacesAndMantelpieces">
        <rdfs:subClassOf rdf:resource="https://www.theworldavatar.com/kg/ontopoi/ConsumerProducts"/>
        <rdfs:comment>Fireplaces and mantelpieces is a subcategory of consumer products</rdfs:comment>
        <rdfs:isDefinedBy rdf:resource="https://www.theworldavatar.com/kg/ontopoi"/>
        <rdfs:label>Fireplaces and mantelpieces</rdfs:label>
    </owl:Class>
    


    <!-- https://www.theworldavatar.com/kg/ontopoi/FireworkRelatedServices -->


    <owl:Class rdf:about="https://www.theworldavatar.com/kg/ontopoi/FireworkRelatedServices">
        <rdfs:subClassOf rdf:resource="https://www.theworldavatar.com/kg/ontopoi/SportAndEntertainmentSupportServices"/>
        <rdfs:comment>Firework related services is a subcategory of sport and entertainment support services</rdfs:comment>
        <rdfs:isDefinedBy rdf:resource="https://www.theworldavatar.com/kg/ontopoi"/>
        <rdfs:label>Firework related services</rdfs:label>
    </owl:Class>
    


    <!-- https://www.theworldavatar.com/kg/ontopoi/FirstAidTraining -->


    <owl:Class rdf:about="https://www.theworldavatar.com/kg/ontopoi/FirstAidTraining">
        <rdfs:subClassOf rdf:resource="https://www.theworldavatar.com/kg/ontopoi/RecreationalAndVocationalEducation"/>
        <rdfs:comment>First aid training is a subcategory of recreational and vocational education</rdfs:comment>
        <rdfs:isDefinedBy rdf:resource="https://www.theworldavatar.com/kg/ontopoi"/>
        <rdfs:label>First aid training</rdfs:label>
    </owl:Class>
    


    <!-- https://www.theworldavatar.com/kg/ontopoi/FirstAndPrimaryAndInfantSchools -->


    <owl:Class rdf:about="https://www.theworldavatar.com/kg/ontopoi/FirstAndPrimaryAndInfantSchools">
        <rdfs:subClassOf rdf:resource="https://www.theworldavatar.com/kg/ontopoi/PrimaryAndSecondaryAndTertiaryEducation"/>
        <rdfs:comment>First, primary and infant schools is a subcategory of primary, secondary and tertiary education</rdfs:comment>
        <rdfs:isDefinedBy rdf:resource="https://www.theworldavatar.com/kg/ontopoi"/>
        <rdfs:label>First, primary and infant schools</rdfs:label>
    </owl:Class>
    


    <!-- https://www.theworldavatar.com/kg/ontopoi/FishAndChipShops -->


    <owl:Class rdf:about="https://www.theworldavatar.com/kg/ontopoi/FishAndChipShops">
        <rdfs:subClassOf rdf:resource="https://www.theworldavatar.com/kg/ontopoi/EatingAndDrinking"/>
        <rdfs:comment>Fish and chip shops is a subcategory of eating and drinking</rdfs:comment>
        <rdfs:isDefinedBy rdf:resource="https://www.theworldavatar.com/kg/ontopoi"/>
        <rdfs:label>Fish and chip shops</rdfs:label>
    </owl:Class>
    


    <!-- https://www.theworldavatar.com/kg/ontopoi/FishAndMeatAndPoultryProducts -->


    <owl:Class rdf:about="https://www.theworldavatar.com/kg/ontopoi/FishAndMeatAndPoultryProducts">
        <rdfs:subClassOf rdf:resource="https://www.theworldavatar.com/kg/ontopoi/Foodstuffs"/>
        <rdfs:comment>Fish, meat and poultry products is a subcategory of foodstuffs</rdfs:comment>
        <rdfs:isDefinedBy rdf:resource="https://www.theworldavatar.com/kg/ontopoi"/>
        <rdfs:label>Fish, meat and poultry products</rdfs:label>
    </owl:Class>
    


    <!-- https://www.theworldavatar.com/kg/ontopoi/FishAndShellfish -->


    <owl:Class rdf:about="https://www.theworldavatar.com/kg/ontopoi/FishAndShellfish">
        <rdfs:subClassOf rdf:resource="https://www.theworldavatar.com/kg/ontopoi/Farming"/>
        <rdfs:comment>Fish and shellfish is a subcategory of farming</rdfs:comment>
        <rdfs:isDefinedBy rdf:resource="https://www.theworldavatar.com/kg/ontopoi"/>
        <rdfs:label>Fish and shellfish</rdfs:label>
    </owl:Class>
    


    <!-- https://www.theworldavatar.com/kg/ontopoi/Fishmongers -->


    <owl:Class rdf:about="https://www.theworldavatar.com/kg/ontopoi/Fishmongers">
        <rdfs:subClassOf rdf:resource="https://www.theworldavatar.com/kg/ontopoi/FoodAndDrinkAndMultiItemRetail"/>
        <rdfs:comment>Fishmongers is a subcategory of food, drink and multi item retail</rdfs:comment>
        <rdfs:isDefinedBy rdf:resource="https://www.theworldavatar.com/kg/ontopoi"/>
        <rdfs:label>Fishmongers</rdfs:label>
    </owl:Class>
    


    <!-- https://www.theworldavatar.com/kg/ontopoi/Florists -->


    <owl:Class rdf:about="https://www.theworldavatar.com/kg/ontopoi/Florists">
        <rdfs:subClassOf rdf:resource="https://www.theworldavatar.com/kg/ontopoi/HouseholdAndOfficeAndLeisureAndGarden"/>
        <rdfs:comment>Florists is a subcategory of household, office, leisure and garden</rdfs:comment>
        <rdfs:isDefinedBy rdf:resource="https://www.theworldavatar.com/kg/ontopoi"/>
        <rdfs:label>Florists</rdfs:label>
    </owl:Class>
    


    <!-- https://www.theworldavatar.com/kg/ontopoi/FlyingSchools -->


    <owl:Class rdf:about="https://www.theworldavatar.com/kg/ontopoi/FlyingSchools">
        <rdfs:subClassOf rdf:resource="https://www.theworldavatar.com/kg/ontopoi/RecreationalAndVocationalEducation"/>
        <rdfs:comment>Flying schools is a subcategory of recreational and vocational education</rdfs:comment>
        <rdfs:isDefinedBy rdf:resource="https://www.theworldavatar.com/kg/ontopoi"/>
        <rdfs:label>Flying schools</rdfs:label>
    </owl:Class>
    


    <!-- https://www.theworldavatar.com/kg/ontopoi/FoodAndBeverageIndustryMachinery -->


    <owl:Class rdf:about="https://www.theworldavatar.com/kg/ontopoi/FoodAndBeverageIndustryMachinery">
        <rdfs:subClassOf rdf:resource="https://www.theworldavatar.com/kg/ontopoi/IndustrialProducts"/>
        <rdfs:comment>Food and beverage industry machinery is a subcategory of industrial products</rdfs:comment>
        <rdfs:isDefinedBy rdf:resource="https://www.theworldavatar.com/kg/ontopoi"/>
        <rdfs:label>Food and beverage industry machinery</rdfs:label>
    </owl:Class>
    


    <!-- https://www.theworldavatar.com/kg/ontopoi/FoodAndDrinkAndMultiItemRetail -->


    <owl:Class rdf:about="https://www.theworldavatar.com/kg/ontopoi/FoodAndDrinkAndMultiItemRetail">
        <rdfs:subClassOf rdf:resource="https://www.theworldavatar.com/kg/ontopoi/Retail"/>
        <rdfs:comment>Food, drink and multi item retail is a subcategory of retail</rdfs:comment>
        <rdfs:isDefinedBy rdf:resource="https://www.theworldavatar.com/kg/ontopoi"/>
        <rdfs:label>Food, drink and multi item retail</rdfs:label>
    </owl:Class>
    


    <!-- https://www.theworldavatar.com/kg/ontopoi/FoodConsultants -->


    <owl:Class rdf:about="https://www.theworldavatar.com/kg/ontopoi/FoodConsultants">
        <rdfs:subClassOf rdf:resource="https://www.theworldavatar.com/kg/ontopoi/Consultancies"/>
        <rdfs:comment>Food consultants is a subcategory of consultancies</rdfs:comment>
        <rdfs:isDefinedBy rdf:resource="https://www.theworldavatar.com/kg/ontopoi"/>
        <rdfs:label>Food consultants</rdfs:label>
    </owl:Class>
    


    <!-- https://www.theworldavatar.com/kg/ontopoi/Foodstuffs -->


    <owl:Class rdf:about="https://www.theworldavatar.com/kg/ontopoi/Foodstuffs">
        <rdfs:subClassOf rdf:resource="https://www.theworldavatar.com/kg/ontopoi/ManufacturingAndProduction"/>
        <rdfs:comment>Foodstuffs is a subcategory of manufacturing and production</rdfs:comment>
        <rdfs:isDefinedBy rdf:resource="https://www.theworldavatar.com/kg/ontopoi"/>
        <rdfs:label>Foodstuffs</rdfs:label>
    </owl:Class>
    


    <!-- https://www.theworldavatar.com/kg/ontopoi/FootRelatedServices -->


    <owl:Class rdf:about="https://www.theworldavatar.com/kg/ontopoi/FootRelatedServices">
        <rdfs:subClassOf rdf:resource="https://www.theworldavatar.com/kg/ontopoi/HealthPractitionersAndEstablishments"/>
        <rdfs:comment>Foot related services is a subcategory of health practitioners and establishments</rdfs:comment>
        <rdfs:isDefinedBy rdf:resource="https://www.theworldavatar.com/kg/ontopoi"/>
        <rdfs:label>Foot related services</rdfs:label>
    </owl:Class>
    


    <!-- https://www.theworldavatar.com/kg/ontopoi/Footbridges -->


    <owl:Class rdf:about="https://www.theworldavatar.com/kg/ontopoi/Footbridges">
        <rdfs:subClassOf rdf:resource="https://www.theworldavatar.com/kg/ontopoi/Walking"/>
        <rdfs:comment>Footbridges is a subcategory of walking</rdfs:comment>
        <rdfs:isDefinedBy rdf:resource="https://www.theworldavatar.com/kg/ontopoi"/>
        <rdfs:label>Footbridges</rdfs:label>
    </owl:Class>
    


    <!-- https://www.theworldavatar.com/kg/ontopoi/Footwear -->


    <owl:Class rdf:about="https://www.theworldavatar.com/kg/ontopoi/Footwear">
        <rdfs:subClassOf rdf:resource="https://www.theworldavatar.com/kg/ontopoi/ClothingAndAccessories"/>
        <rdfs:subClassOf rdf:resource="https://www.theworldavatar.com/kg/ontopoi/ConsumerProducts"/>
        <rdfs:comment>Footwear is a subcategory of clothing and accessories</rdfs:comment>
        <rdfs:comment>Footwear is a subcategory of consumer products</rdfs:comment>
        <rdfs:isDefinedBy rdf:resource="https://www.theworldavatar.com/kg/ontopoi"/>
        <rdfs:label>Footwear</rdfs:label>
    </owl:Class>
    


    <!-- https://www.theworldavatar.com/kg/ontopoi/FordsAndLevelCrossings -->


    <owl:Class rdf:about="https://www.theworldavatar.com/kg/ontopoi/FordsAndLevelCrossings">
        <rdfs:subClassOf rdf:resource="https://www.theworldavatar.com/kg/ontopoi/RoadAndRail"/>
        <rdfs:comment>Fords and level crossings is a subcategory of road and rail</rdfs:comment>
        <rdfs:isDefinedBy rdf:resource="https://www.theworldavatar.com/kg/ontopoi"/>
        <rdfs:label>Fords and level crossings</rdfs:label>
    </owl:Class>
    


    <!-- https://www.theworldavatar.com/kg/ontopoi/ForeignCountrySupportActivities -->


    <owl:Class rdf:about="https://www.theworldavatar.com/kg/ontopoi/ForeignCountrySupportActivities">
        <rdfs:subClassOf rdf:resource="https://www.theworldavatar.com/kg/ontopoi/CentralAndLocalGovernment"/>
        <rdfs:comment>Foreign country support activities is a subcategory of central and local government</rdfs:comment>
        <rdfs:isDefinedBy rdf:resource="https://www.theworldavatar.com/kg/ontopoi"/>
        <rdfs:label>Foreign country support activities</rdfs:label>
    </owl:Class>
    


    <!-- https://www.theworldavatar.com/kg/ontopoi/Forestry -->


    <owl:Class rdf:about="https://www.theworldavatar.com/kg/ontopoi/Forestry">
        <rdfs:subClassOf rdf:resource="https://www.theworldavatar.com/kg/ontopoi/Farming"/>
        <rdfs:comment>Forestry is a subcategory of farming</rdfs:comment>
        <rdfs:isDefinedBy rdf:resource="https://www.theworldavatar.com/kg/ontopoi"/>
        <rdfs:label>Forestry</rdfs:label>
    </owl:Class>
    


    <!-- https://www.theworldavatar.com/kg/ontopoi/FranchiseAndHoldingCompanyServices -->


    <owl:Class rdf:about="https://www.theworldavatar.com/kg/ontopoi/FranchiseAndHoldingCompanyServices">
        <rdfs:subClassOf rdf:resource="https://www.theworldavatar.com/kg/ontopoi/LegalAndFinancial"/>
        <rdfs:comment>Franchise and holding company services is a subcategory of legal and financial</rdfs:comment>
        <rdfs:isDefinedBy rdf:resource="https://www.theworldavatar.com/kg/ontopoi"/>
        <rdfs:label>Franchise and holding company services</rdfs:label>
    </owl:Class>
    


    <!-- https://www.theworldavatar.com/kg/ontopoi/FrozenFoods -->


    <owl:Class rdf:about="https://www.theworldavatar.com/kg/ontopoi/FrozenFoods">
        <rdfs:subClassOf rdf:resource="https://www.theworldavatar.com/kg/ontopoi/FoodAndDrinkAndMultiItemRetail"/>
        <rdfs:comment>Frozen foods is a subcategory of food, drink and multi item retail</rdfs:comment>
        <rdfs:isDefinedBy rdf:resource="https://www.theworldavatar.com/kg/ontopoi"/>
        <rdfs:label>Frozen foods</rdfs:label>
    </owl:Class>
    


    <!-- https://www.theworldavatar.com/kg/ontopoi/FruitAndFlowerAndVegetableGrowers -->


    <owl:Class rdf:about="https://www.theworldavatar.com/kg/ontopoi/FruitAndFlowerAndVegetableGrowers">
        <rdfs:subClassOf rdf:resource="https://www.theworldavatar.com/kg/ontopoi/Farming"/>
        <rdfs:comment>Fruit, flower and vegetable growers is a subcategory of farming</rdfs:comment>
        <rdfs:isDefinedBy rdf:resource="https://www.theworldavatar.com/kg/ontopoi"/>
        <rdfs:label>Fruit, flower and vegetable growers</rdfs:label>
    </owl:Class>
    


    <!-- https://www.theworldavatar.com/kg/ontopoi/FuelDistributorsAndSuppliers -->


    <owl:Class rdf:about="https://www.theworldavatar.com/kg/ontopoi/FuelDistributorsAndSuppliers">
        <rdfs:subClassOf rdf:resource="https://www.theworldavatar.com/kg/ontopoi/HouseholdAndOfficeAndLeisureAndGarden"/>
        <rdfs:comment>Fuel distributors and suppliers is a subcategory of household, office, leisure and garden</rdfs:comment>
        <rdfs:isDefinedBy rdf:resource="https://www.theworldavatar.com/kg/ontopoi"/>
        <rdfs:label>Fuel distributors and suppliers</rdfs:label>
    </owl:Class>
    


    <!-- https://www.theworldavatar.com/kg/ontopoi/FundraisingServices -->


    <owl:Class rdf:about="https://www.theworldavatar.com/kg/ontopoi/FundraisingServices">
        <rdfs:subClassOf rdf:resource="https://www.theworldavatar.com/kg/ontopoi/LegalAndFinancial"/>
        <rdfs:comment>Fundraising services is a subcategory of legal and financial</rdfs:comment>
        <rdfs:isDefinedBy rdf:resource="https://www.theworldavatar.com/kg/ontopoi"/>
        <rdfs:label>Fundraising services</rdfs:label>
    </owl:Class>
    


    <!-- https://www.theworldavatar.com/kg/ontopoi/FuneralAndAssociatedServices -->


    <owl:Class rdf:about="https://www.theworldavatar.com/kg/ontopoi/FuneralAndAssociatedServices">
        <rdfs:subClassOf rdf:resource="https://www.theworldavatar.com/kg/ontopoi/PersonalAndConsumerAndOtherServices"/>
        <rdfs:comment>Funeral and associated services is a subcategory of personal, consumer and other services</rdfs:comment>
        <rdfs:isDefinedBy rdf:resource="https://www.theworldavatar.com/kg/ontopoi"/>
        <rdfs:label>Funeral and associated services</rdfs:label>
    </owl:Class>
    


    <!-- https://www.theworldavatar.com/kg/ontopoi/FunfairServices -->


    <owl:Class rdf:about="https://www.theworldavatar.com/kg/ontopoi/FunfairServices">
        <rdfs:subClassOf rdf:resource="https://www.theworldavatar.com/kg/ontopoi/SportAndEntertainmentSupportServices"/>
        <rdfs:comment>Funfair services is a subcategory of sport and entertainment support services</rdfs:comment>
        <rdfs:isDefinedBy rdf:resource="https://www.theworldavatar.com/kg/ontopoi"/>
        <rdfs:label>Funfair services</rdfs:label>
    </owl:Class>
    


    <!-- https://www.theworldavatar.com/kg/ontopoi/Furniture -->


    <owl:Class rdf:about="https://www.theworldavatar.com/kg/ontopoi/Furniture">
        <rdfs:subClassOf rdf:resource="https://www.theworldavatar.com/kg/ontopoi/ConsumerProducts"/>
        <rdfs:subClassOf rdf:resource="https://www.theworldavatar.com/kg/ontopoi/HouseholdAndOfficeAndLeisureAndGarden"/>
        <rdfs:comment>Furniture is a subcategory of consumer products</rdfs:comment>
        <rdfs:comment>Furniture is a subcategory of household, office, leisure and garden</rdfs:comment>
        <rdfs:isDefinedBy rdf:resource="https://www.theworldavatar.com/kg/ontopoi"/>
        <rdfs:label>Furniture</rdfs:label>
    </owl:Class>
    


    <!-- https://www.theworldavatar.com/kg/ontopoi/FurtherEducationEstablishments -->


    <owl:Class rdf:about="https://www.theworldavatar.com/kg/ontopoi/FurtherEducationEstablishments">
        <rdfs:subClassOf rdf:resource="https://www.theworldavatar.com/kg/ontopoi/PrimaryAndSecondaryAndTertiaryEducation"/>
        <rdfs:comment>Further education establishments is a subcategory of primary, secondary and tertiary education</rdfs:comment>
        <rdfs:isDefinedBy rdf:resource="https://www.theworldavatar.com/kg/ontopoi"/>
        <rdfs:label>Further education establishments</rdfs:label>
    </owl:Class>
    


    <!-- https://www.theworldavatar.com/kg/ontopoi/Gambling -->


    <owl:Class rdf:about="https://www.theworldavatar.com/kg/ontopoi/Gambling">
        <rdfs:subClassOf rdf:resource="https://www.theworldavatar.com/kg/ontopoi/SportAndEntertainment"/>
        <rdfs:comment>Gambling is a subcategory of sport and entertainment</rdfs:comment>
        <rdfs:isDefinedBy rdf:resource="https://www.theworldavatar.com/kg/ontopoi"/>
        <rdfs:label>Gambling</rdfs:label>
    </owl:Class>
    


    <!-- https://www.theworldavatar.com/kg/ontopoi/GaragesAndGardenAndPortableBuildings -->


    <owl:Class rdf:about="https://www.theworldavatar.com/kg/ontopoi/GaragesAndGardenAndPortableBuildings">
        <rdfs:subClassOf rdf:resource="https://www.theworldavatar.com/kg/ontopoi/HouseholdAndOfficeAndLeisureAndGarden"/>
        <rdfs:comment>Garages, garden and portable buildings is a subcategory of household, office, leisure and garden</rdfs:comment>
        <rdfs:isDefinedBy rdf:resource="https://www.theworldavatar.com/kg/ontopoi"/>
        <rdfs:label>Garages, garden and portable buildings</rdfs:label>
    </owl:Class>
    


    <!-- https://www.theworldavatar.com/kg/ontopoi/GardenCentresAndNurseries -->


    <owl:Class rdf:about="https://www.theworldavatar.com/kg/ontopoi/GardenCentresAndNurseries">
        <rdfs:subClassOf rdf:resource="https://www.theworldavatar.com/kg/ontopoi/HouseholdAndOfficeAndLeisureAndGarden"/>
        <rdfs:comment>Garden centres and nurseries is a subcategory of household, office, leisure and garden</rdfs:comment>
        <rdfs:isDefinedBy rdf:resource="https://www.theworldavatar.com/kg/ontopoi"/>
        <rdfs:label>Garden centres and nurseries</rdfs:label>
    </owl:Class>
    


    <!-- https://www.theworldavatar.com/kg/ontopoi/GardenGoods -->


    <owl:Class rdf:about="https://www.theworldavatar.com/kg/ontopoi/GardenGoods">
        <rdfs:subClassOf rdf:resource="https://www.theworldavatar.com/kg/ontopoi/ConsumerProducts"/>
        <rdfs:comment>Garden goods is a subcategory of consumer products</rdfs:comment>
        <rdfs:isDefinedBy rdf:resource="https://www.theworldavatar.com/kg/ontopoi"/>
        <rdfs:label>Garden goods</rdfs:label>
    </owl:Class>
    


    <!-- https://www.theworldavatar.com/kg/ontopoi/GardenMachineryAndFurniture -->


    <owl:Class rdf:about="https://www.theworldavatar.com/kg/ontopoi/GardenMachineryAndFurniture">
        <rdfs:subClassOf rdf:resource="https://www.theworldavatar.com/kg/ontopoi/HouseholdAndOfficeAndLeisureAndGarden"/>
        <rdfs:comment>Garden machinery and furniture is a subcategory of household, office, leisure and garden</rdfs:comment>
        <rdfs:isDefinedBy rdf:resource="https://www.theworldavatar.com/kg/ontopoi"/>
        <rdfs:label>Garden machinery and furniture</rdfs:label>
    </owl:Class>
    


    <!-- https://www.theworldavatar.com/kg/ontopoi/GardeningAndLandscapingAndTreeSurgeryServices -->


    <owl:Class rdf:about="https://www.theworldavatar.com/kg/ontopoi/GardeningAndLandscapingAndTreeSurgeryServices">
        <rdfs:subClassOf rdf:resource="https://www.theworldavatar.com/kg/ontopoi/ConstructionServices"/>
        <rdfs:comment>Gardening, landscaping and tree surgery services is a subcategory of construction services</rdfs:comment>
        <rdfs:isDefinedBy rdf:resource="https://www.theworldavatar.com/kg/ontopoi"/>
        <rdfs:label>Gardening, landscaping and tree surgery services</rdfs:label>
    </owl:Class>
    


    <!-- https://www.theworldavatar.com/kg/ontopoi/GasFeatures -->


    <owl:Class rdf:about="https://www.theworldavatar.com/kg/ontopoi/GasFeatures">
        <rdfs:subClassOf rdf:resource="https://www.theworldavatar.com/kg/ontopoi/InfrastructureAndFacilities"/>
        <rdfs:comment>Gas features is a subcategory of infrastructure and facilities</rdfs:comment>
        <rdfs:isDefinedBy rdf:resource="https://www.theworldavatar.com/kg/ontopoi"/>
        <rdfs:label>Gas features</rdfs:label>
    </owl:Class>
    


    <!-- https://www.theworldavatar.com/kg/ontopoi/General-PurposeMachinery -->


    <owl:Class rdf:about="https://www.theworldavatar.com/kg/ontopoi/General-PurposeMachinery">
        <rdfs:subClassOf rdf:resource="https://www.theworldavatar.com/kg/ontopoi/IndustrialProducts"/>
        <rdfs:comment>General-purpose machinery is a subcategory of industrial products</rdfs:comment>
        <rdfs:isDefinedBy rdf:resource="https://www.theworldavatar.com/kg/ontopoi"/>
        <rdfs:label>General-purpose machinery</rdfs:label>
    </owl:Class>
    


    <!-- https://www.theworldavatar.com/kg/ontopoi/GeneralComputerServices -->


    <owl:Class rdf:about="https://www.theworldavatar.com/kg/ontopoi/GeneralComputerServices">
        <rdfs:subClassOf rdf:resource="https://www.theworldavatar.com/kg/ontopoi/ItAndAdvertisingAndMarketingAndMediaServiceS"/>
        <rdfs:comment>General computer services is a subcategory of it, advertising, marketing and media service s</rdfs:comment>
        <rdfs:isDefinedBy rdf:resource="https://www.theworldavatar.com/kg/ontopoi"/>
        <rdfs:label>General computer services</rdfs:label>
    </owl:Class>
    


    <!-- https://www.theworldavatar.com/kg/ontopoi/GeneralConstructionSupplies -->


    <owl:Class rdf:about="https://www.theworldavatar.com/kg/ontopoi/GeneralConstructionSupplies">
        <rdfs:subClassOf rdf:resource="https://www.theworldavatar.com/kg/ontopoi/IndustrialProducts"/>
        <rdfs:comment>General construction supplies is a subcategory of industrial products</rdfs:comment>
        <rdfs:isDefinedBy rdf:resource="https://www.theworldavatar.com/kg/ontopoi"/>
        <rdfs:label>General construction supplies</rdfs:label>
    </owl:Class>
    


    <!-- https://www.theworldavatar.com/kg/ontopoi/GeneralHouseholdGoods -->


    <owl:Class rdf:about="https://www.theworldavatar.com/kg/ontopoi/GeneralHouseholdGoods">
        <rdfs:subClassOf rdf:resource="https://www.theworldavatar.com/kg/ontopoi/HouseholdAndOfficeAndLeisureAndGarden"/>
        <rdfs:comment>General household goods is a subcategory of household, office, leisure and garden</rdfs:comment>
        <rdfs:isDefinedBy rdf:resource="https://www.theworldavatar.com/kg/ontopoi"/>
        <rdfs:label>General household goods</rdfs:label>
    </owl:Class>
    


    <!-- https://www.theworldavatar.com/kg/ontopoi/GeneralManufacturing -->


    <owl:Class rdf:about="https://www.theworldavatar.com/kg/ontopoi/GeneralManufacturing">
        <rdfs:subClassOf rdf:resource="https://www.theworldavatar.com/kg/ontopoi/IndustrialProducts"/>
        <rdfs:comment>General manufacturing is a subcategory of industrial products</rdfs:comment>
        <rdfs:isDefinedBy rdf:resource="https://www.theworldavatar.com/kg/ontopoi"/>
        <rdfs:label>General manufacturing</rdfs:label>
    </owl:Class>
    


    <!-- https://www.theworldavatar.com/kg/ontopoi/GeographicCounty -->


    <owl:Class rdf:about="https://www.theworldavatar.com/kg/ontopoi/GeographicCounty">
        <rdfs:comment>A traditional, historical, or ceremonial division of land that defines a region for purposes such as cultural identity, historical boundaries, and geographic context</rdfs:comment>
        <rdfs:isDefinedBy rdf:resource="https://www.theworldavatar.com/kg/ontopoi"/>
        <rdfs:label>Geographic County</rdfs:label>
    </owl:Class>
    


    <!-- https://www.theworldavatar.com/kg/ontopoi/GiftsAndCards -->


    <owl:Class rdf:about="https://www.theworldavatar.com/kg/ontopoi/GiftsAndCards">
        <rdfs:subClassOf rdf:resource="https://www.theworldavatar.com/kg/ontopoi/HouseholdAndOfficeAndLeisureAndGarden"/>
        <rdfs:comment>Gifts and cards is a subcategory of household, office, leisure and garden</rdfs:comment>
        <rdfs:isDefinedBy rdf:resource="https://www.theworldavatar.com/kg/ontopoi"/>
        <rdfs:label>Gifts and cards</rdfs:label>
    </owl:Class>
    


    <!-- https://www.theworldavatar.com/kg/ontopoi/Giftware -->


    <owl:Class rdf:about="https://www.theworldavatar.com/kg/ontopoi/Giftware">
        <rdfs:subClassOf rdf:resource="https://www.theworldavatar.com/kg/ontopoi/ConsumerProducts"/>
        <rdfs:comment>Giftware is a subcategory of consumer products</rdfs:comment>
        <rdfs:isDefinedBy rdf:resource="https://www.theworldavatar.com/kg/ontopoi"/>
        <rdfs:label>Giftware</rdfs:label>
    </owl:Class>
    


    <!-- https://www.theworldavatar.com/kg/ontopoi/Glass -->


    <owl:Class rdf:about="https://www.theworldavatar.com/kg/ontopoi/Glass">
        <rdfs:subClassOf rdf:resource="https://www.theworldavatar.com/kg/ontopoi/IndustrialProducts"/>
        <rdfs:comment>Glass is a subcategory of industrial products</rdfs:comment>
        <rdfs:isDefinedBy rdf:resource="https://www.theworldavatar.com/kg/ontopoi"/>
        <rdfs:label>Glass</rdfs:label>
    </owl:Class>
    


    <!-- https://www.theworldavatar.com/kg/ontopoi/GlassFibreServices -->


    <owl:Class rdf:about="https://www.theworldavatar.com/kg/ontopoi/GlassFibreServices">
        <rdfs:subClassOf rdf:resource="https://www.theworldavatar.com/kg/ontopoi/IndustrialProducts"/>
        <rdfs:comment>Glass fibre services is a subcategory of industrial products</rdfs:comment>
        <rdfs:isDefinedBy rdf:resource="https://www.theworldavatar.com/kg/ontopoi"/>
        <rdfs:label>Glass fibre services</rdfs:label>
    </owl:Class>
    


    <!-- https://www.theworldavatar.com/kg/ontopoi/Glaziers -->


    <owl:Class rdf:about="https://www.theworldavatar.com/kg/ontopoi/Glaziers">
        <rdfs:subClassOf rdf:resource="https://www.theworldavatar.com/kg/ontopoi/ConstructionServices"/>
        <rdfs:comment>Glaziers is a subcategory of construction services</rdfs:comment>
        <rdfs:isDefinedBy rdf:resource="https://www.theworldavatar.com/kg/ontopoi"/>
        <rdfs:label>Glaziers</rdfs:label>
    </owl:Class>
    


    <!-- https://www.theworldavatar.com/kg/ontopoi/GolfRangesAndCoursesAndClubsAndProfessionals -->


    <owl:Class rdf:about="https://www.theworldavatar.com/kg/ontopoi/GolfRangesAndCoursesAndClubsAndProfessionals">
        <rdfs:subClassOf rdf:resource="https://www.theworldavatar.com/kg/ontopoi/SportsComplex"/>
        <rdfs:comment>Golf ranges, courses, clubs and professionals is a subcategory of sports complex</rdfs:comment>
        <rdfs:isDefinedBy rdf:resource="https://www.theworldavatar.com/kg/ontopoi"/>
        <rdfs:label>Golf ranges, courses, clubs and professionals</rdfs:label>
    </owl:Class>
    


    <!-- https://www.theworldavatar.com/kg/ontopoi/GreenAndNewAgeGoods -->


    <owl:Class rdf:about="https://www.theworldavatar.com/kg/ontopoi/GreenAndNewAgeGoods">
        <rdfs:subClassOf rdf:resource="https://www.theworldavatar.com/kg/ontopoi/FoodAndDrinkAndMultiItemRetail"/>
        <rdfs:comment>Green and new age goods is a subcategory of food, drink and multi item retail</rdfs:comment>
        <rdfs:isDefinedBy rdf:resource="https://www.theworldavatar.com/kg/ontopoi"/>
        <rdfs:label>Green and new age goods</rdfs:label>
    </owl:Class>
    


    <!-- https://www.theworldavatar.com/kg/ontopoi/GrocersAndFarmShopsAndPickYourOwn -->


    <owl:Class rdf:about="https://www.theworldavatar.com/kg/ontopoi/GrocersAndFarmShopsAndPickYourOwn">
        <rdfs:subClassOf rdf:resource="https://www.theworldavatar.com/kg/ontopoi/FoodAndDrinkAndMultiItemRetail"/>
        <rdfs:comment>Grocers, farm shops and pick your own is a subcategory of food, drink and multi item retail</rdfs:comment>
        <rdfs:isDefinedBy rdf:resource="https://www.theworldavatar.com/kg/ontopoi"/>
        <rdfs:label>Grocers, farm shops and pick your own</rdfs:label>
    </owl:Class>
    


    <!-- https://www.theworldavatar.com/kg/ontopoi/GymnasiumsAndSportsHallsAndLeisureCentres -->


    <owl:Class rdf:about="https://www.theworldavatar.com/kg/ontopoi/GymnasiumsAndSportsHallsAndLeisureCentres">
        <rdfs:subClassOf rdf:resource="https://www.theworldavatar.com/kg/ontopoi/SportsComplex"/>
        <rdfs:comment>Gymnasiums, sports halls and leisure centres is a subcategory of sports complex</rdfs:comment>
        <rdfs:isDefinedBy rdf:resource="https://www.theworldavatar.com/kg/ontopoi"/>
        <rdfs:label>Gymnasiums, sports halls and leisure centres</rdfs:label>
    </owl:Class>
    


    <!-- https://www.theworldavatar.com/kg/ontopoi/HailAndRideZones -->


    <owl:Class rdf:about="https://www.theworldavatar.com/kg/ontopoi/HailAndRideZones">
        <rdfs:subClassOf rdf:resource="https://www.theworldavatar.com/kg/ontopoi/BusTransport"/>
        <rdfs:comment>Hail and ride zones is a subcategory of bus transport</rdfs:comment>
        <rdfs:isDefinedBy rdf:resource="https://www.theworldavatar.com/kg/ontopoi"/>
        <rdfs:label>Hail and ride zones</rdfs:label>
    </owl:Class>
    


    <!-- https://www.theworldavatar.com/kg/ontopoi/HairAndBeautyServices -->


    <owl:Class rdf:about="https://www.theworldavatar.com/kg/ontopoi/HairAndBeautyServices">
        <rdfs:subClassOf rdf:resource="https://www.theworldavatar.com/kg/ontopoi/PersonalAndConsumerAndOtherServices"/>
        <rdfs:comment>Hair and beauty services is a subcategory of personal, consumer and other services</rdfs:comment>
        <rdfs:isDefinedBy rdf:resource="https://www.theworldavatar.com/kg/ontopoi"/>
        <rdfs:label>Hair and beauty services</rdfs:label>
    </owl:Class>
    


    <!-- https://www.theworldavatar.com/kg/ontopoi/HallsAndCommunityCentres -->


    <owl:Class rdf:about="https://www.theworldavatar.com/kg/ontopoi/HallsAndCommunityCentres">
        <rdfs:subClassOf rdf:resource="https://www.theworldavatar.com/kg/ontopoi/InfrastructureAndFacilities"/>
        <rdfs:comment>Halls and community centres is a subcategory of infrastructure and facilities</rdfs:comment>
        <rdfs:isDefinedBy rdf:resource="https://www.theworldavatar.com/kg/ontopoi"/>
        <rdfs:label>Halls and community centres</rdfs:label>
    </owl:Class>
    


    <!-- https://www.theworldavatar.com/kg/ontopoi/HeadquartersAndAdministrationAndCentralOffices -->


    <owl:Class rdf:about="https://www.theworldavatar.com/kg/ontopoi/HeadquartersAndAdministrationAndCentralOffices">
        <rdfs:subClassOf rdf:resource="https://www.theworldavatar.com/kg/ontopoi/PersonalAndConsumerAndOtherServices"/>
        <rdfs:comment>Headquarters, administration and central offices is a subcategory of personal, consumer and other services</rdfs:comment>
        <rdfs:isDefinedBy rdf:resource="https://www.theworldavatar.com/kg/ontopoi"/>
        <rdfs:label>Headquarters, administration and central offices</rdfs:label>
    </owl:Class>
    


    <!-- https://www.theworldavatar.com/kg/ontopoi/HealthAuthorities -->


    <owl:Class rdf:about="https://www.theworldavatar.com/kg/ontopoi/HealthAuthorities">
        <rdfs:subClassOf rdf:resource="https://www.theworldavatar.com/kg/ontopoi/HealthSupportServices"/>
        <rdfs:comment>Health authorities is a subcategory of health support services</rdfs:comment>
        <rdfs:isDefinedBy rdf:resource="https://www.theworldavatar.com/kg/ontopoi"/>
        <rdfs:label>Health authorities</rdfs:label>
    </owl:Class>
    


    <!-- https://www.theworldavatar.com/kg/ontopoi/HealthPractitionersAndEstablishments -->


    <owl:Class rdf:about="https://www.theworldavatar.com/kg/ontopoi/HealthPractitionersAndEstablishments">
        <rdfs:subClassOf rdf:resource="https://www.theworldavatar.com/kg/ontopoi/EducationAndHealth"/>
        <rdfs:comment>Health practitioners and establishments is a subcategory of education and health</rdfs:comment>
        <rdfs:isDefinedBy rdf:resource="https://www.theworldavatar.com/kg/ontopoi"/>
        <rdfs:label>Health practitioners and establishments</rdfs:label>
    </owl:Class>
    


    <!-- https://www.theworldavatar.com/kg/ontopoi/HealthSupportServices -->


    <owl:Class rdf:about="https://www.theworldavatar.com/kg/ontopoi/HealthSupportServices">
        <rdfs:subClassOf rdf:resource="https://www.theworldavatar.com/kg/ontopoi/EducationAndHealth"/>
        <rdfs:comment>Health support services is a subcategory of education and health</rdfs:comment>
        <rdfs:isDefinedBy rdf:resource="https://www.theworldavatar.com/kg/ontopoi"/>
        <rdfs:label>Health support services</rdfs:label>
    </owl:Class>
    


    <!-- https://www.theworldavatar.com/kg/ontopoi/Helipads -->


    <owl:Class rdf:about="https://www.theworldavatar.com/kg/ontopoi/Helipads">
        <rdfs:subClassOf rdf:resource="https://www.theworldavatar.com/kg/ontopoi/Air"/>
        <rdfs:comment>Helipads is a subcategory of air</rdfs:comment>
        <rdfs:isDefinedBy rdf:resource="https://www.theworldavatar.com/kg/ontopoi"/>
        <rdfs:label>Helipads</rdfs:label>
    </owl:Class>
    


    <!-- https://www.theworldavatar.com/kg/ontopoi/HerbsAndSpices -->


    <owl:Class rdf:about="https://www.theworldavatar.com/kg/ontopoi/HerbsAndSpices">
        <rdfs:subClassOf rdf:resource="https://www.theworldavatar.com/kg/ontopoi/FoodAndDrinkAndMultiItemRetail"/>
        <rdfs:comment>Herbs and spices is a subcategory of food, drink and multi item retail</rdfs:comment>
        <rdfs:isDefinedBy rdf:resource="https://www.theworldavatar.com/kg/ontopoi"/>
        <rdfs:label>Herbs and spices</rdfs:label>
    </owl:Class>
    


    <!-- https://www.theworldavatar.com/kg/ontopoi/HigherEducationEstablishments -->


    <owl:Class rdf:about="https://www.theworldavatar.com/kg/ontopoi/HigherEducationEstablishments">
        <rdfs:subClassOf rdf:resource="https://www.theworldavatar.com/kg/ontopoi/PrimaryAndSecondaryAndTertiaryEducation"/>
        <rdfs:comment>Higher education establishments is a subcategory of primary, secondary and tertiary education</rdfs:comment>
        <rdfs:isDefinedBy rdf:resource="https://www.theworldavatar.com/kg/ontopoi"/>
        <rdfs:label>Higher education establishments</rdfs:label>
    </owl:Class>
    


    <!-- https://www.theworldavatar.com/kg/ontopoi/HireServices -->


    <owl:Class rdf:about="https://www.theworldavatar.com/kg/ontopoi/HireServices">
        <rdfs:subClassOf rdf:resource="https://www.theworldavatar.com/kg/ontopoi/CommercialServices"/>
        <rdfs:comment>Hire services is a subcategory of commercial services</rdfs:comment>
        <rdfs:isDefinedBy rdf:resource="https://www.theworldavatar.com/kg/ontopoi"/>
        <rdfs:label>Hire services</rdfs:label>
    </owl:Class>
    


    <!-- https://www.theworldavatar.com/kg/ontopoi/HistoricAndCeremonialStructures -->


    <owl:Class rdf:about="https://www.theworldavatar.com/kg/ontopoi/HistoricAndCeremonialStructures">
        <rdfs:subClassOf rdf:resource="https://www.theworldavatar.com/kg/ontopoi/HistoricalAndCultural"/>
        <rdfs:comment>Historic and ceremonial structures is a subcategory of historical and cultural</rdfs:comment>
        <rdfs:isDefinedBy rdf:resource="https://www.theworldavatar.com/kg/ontopoi"/>
        <rdfs:label>Historic and ceremonial structures</rdfs:label>
    </owl:Class>
    


    <!-- https://www.theworldavatar.com/kg/ontopoi/HistoricBuildingsIncludingCastlesAndFortsAndAbbeys -->


    <owl:Class rdf:about="https://www.theworldavatar.com/kg/ontopoi/HistoricBuildingsIncludingCastlesAndFortsAndAbbeys">
        <rdfs:subClassOf rdf:resource="https://www.theworldavatar.com/kg/ontopoi/HistoricalAndCultural"/>
        <rdfs:comment>Historic buildings including castles, forts and abbeys is a subcategory of historical and cultural</rdfs:comment>
        <rdfs:isDefinedBy rdf:resource="https://www.theworldavatar.com/kg/ontopoi"/>
        <rdfs:label>Historic buildings including castles, forts and abbeys</rdfs:label>
    </owl:Class>
    


    <!-- https://www.theworldavatar.com/kg/ontopoi/HistoricalAndCultural -->


    <owl:Class rdf:about="https://www.theworldavatar.com/kg/ontopoi/HistoricalAndCultural">
        <rdfs:subClassOf rdf:resource="https://www.theworldavatar.com/kg/ontopoi/Attractions"/>
        <rdfs:comment>Historical and cultural is a subcategory of attractions</rdfs:comment>
        <rdfs:isDefinedBy rdf:resource="https://www.theworldavatar.com/kg/ontopoi"/>
        <rdfs:label>Historical and cultural</rdfs:label>
    </owl:Class>
    


    <!-- https://www.theworldavatar.com/kg/ontopoi/HistoricalResearch -->


    <owl:Class rdf:about="https://www.theworldavatar.com/kg/ontopoi/HistoricalResearch">
        <rdfs:subClassOf rdf:resource="https://www.theworldavatar.com/kg/ontopoi/PersonalAndConsumerAndOtherServices"/>
        <rdfs:comment>Historical research is a subcategory of personal, consumer and other services</rdfs:comment>
        <rdfs:isDefinedBy rdf:resource="https://www.theworldavatar.com/kg/ontopoi"/>
        <rdfs:label>Historical research</rdfs:label>
    </owl:Class>
    


    <!-- https://www.theworldavatar.com/kg/ontopoi/HistoricalShips -->


    <owl:Class rdf:about="https://www.theworldavatar.com/kg/ontopoi/HistoricalShips">
        <rdfs:subClassOf rdf:resource="https://www.theworldavatar.com/kg/ontopoi/HistoricalAndCultural"/>
        <rdfs:comment>Historical ships is a subcategory of historical and cultural</rdfs:comment>
        <rdfs:isDefinedBy rdf:resource="https://www.theworldavatar.com/kg/ontopoi"/>
        <rdfs:label>Historical ships</rdfs:label>
    </owl:Class>
    


    <!-- https://www.theworldavatar.com/kg/ontopoi/HobbyAndSportsAndPastimeProducts -->


    <owl:Class rdf:about="https://www.theworldavatar.com/kg/ontopoi/HobbyAndSportsAndPastimeProducts">
        <rdfs:subClassOf rdf:resource="https://www.theworldavatar.com/kg/ontopoi/ConsumerProducts"/>
        <rdfs:subClassOf rdf:resource="https://www.theworldavatar.com/kg/ontopoi/HouseholdAndOfficeAndLeisureAndGarden"/>
        <rdfs:comment>Hobby, sports and pastime products is a subcategory of consumer products</rdfs:comment>
        <rdfs:comment>Hobby, sports and pastime products is a subcategory of household, office, leisure and garden</rdfs:comment>
        <rdfs:isDefinedBy rdf:resource="https://www.theworldavatar.com/kg/ontopoi"/>
        <rdfs:label>Hobby, sports and pastime products</rdfs:label>
    </owl:Class>
    


    <!-- https://www.theworldavatar.com/kg/ontopoi/Homeopaths -->


    <owl:Class rdf:about="https://www.theworldavatar.com/kg/ontopoi/Homeopaths">
        <rdfs:subClassOf rdf:resource="https://www.theworldavatar.com/kg/ontopoi/HealthPractitionersAndEstablishments"/>
        <rdfs:comment>Homeopaths is a subcategory of health practitioners and establishments</rdfs:comment>
        <rdfs:isDefinedBy rdf:resource="https://www.theworldavatar.com/kg/ontopoi"/>
        <rdfs:label>Homeopaths</rdfs:label>
    </owl:Class>
    


    <!-- https://www.theworldavatar.com/kg/ontopoi/HorseBreedersAndDealers -->


    <owl:Class rdf:about="https://www.theworldavatar.com/kg/ontopoi/HorseBreedersAndDealers">
        <rdfs:subClassOf rdf:resource="https://www.theworldavatar.com/kg/ontopoi/Farming"/>
        <rdfs:comment>Horse breeders and dealers is a subcategory of farming</rdfs:comment>
        <rdfs:isDefinedBy rdf:resource="https://www.theworldavatar.com/kg/ontopoi"/>
        <rdfs:label>Horse breeders and dealers</rdfs:label>
    </owl:Class>
    


    <!-- https://www.theworldavatar.com/kg/ontopoi/HorseTraining -->


    <owl:Class rdf:about="https://www.theworldavatar.com/kg/ontopoi/HorseTraining">
        <rdfs:subClassOf rdf:resource="https://www.theworldavatar.com/kg/ontopoi/AnimalWelfare"/>
        <rdfs:comment>Horse training is a subcategory of animal welfare</rdfs:comment>
        <rdfs:isDefinedBy rdf:resource="https://www.theworldavatar.com/kg/ontopoi"/>
        <rdfs:label>Horse training</rdfs:label>
    </owl:Class>
    


    <!-- https://www.theworldavatar.com/kg/ontopoi/HorticulturalAttractions -->


    <owl:Class rdf:about="https://www.theworldavatar.com/kg/ontopoi/HorticulturalAttractions">
        <rdfs:subClassOf rdf:resource="https://www.theworldavatar.com/kg/ontopoi/BotanicalAndZoological"/>
        <rdfs:comment>Horticultural attractions is a subcategory of botanical and zoological</rdfs:comment>
        <rdfs:isDefinedBy rdf:resource="https://www.theworldavatar.com/kg/ontopoi"/>
        <rdfs:label>Horticultural attractions</rdfs:label>
    </owl:Class>
    


    <!-- https://www.theworldavatar.com/kg/ontopoi/HorticulturalEquipment -->


    <owl:Class rdf:about="https://www.theworldavatar.com/kg/ontopoi/HorticulturalEquipment">
        <rdfs:subClassOf rdf:resource="https://www.theworldavatar.com/kg/ontopoi/IndustrialProducts"/>
        <rdfs:comment>Horticultural equipment is a subcategory of industrial products</rdfs:comment>
        <rdfs:isDefinedBy rdf:resource="https://www.theworldavatar.com/kg/ontopoi"/>
        <rdfs:label>Horticultural equipment</rdfs:label>
    </owl:Class>
    


    <!-- https://www.theworldavatar.com/kg/ontopoi/Hospices -->


    <owl:Class rdf:about="https://www.theworldavatar.com/kg/ontopoi/Hospices">
        <rdfs:subClassOf rdf:resource="https://www.theworldavatar.com/kg/ontopoi/HealthPractitionersAndEstablishments"/>
        <rdfs:comment>Hospices is a subcategory of health practitioners and establishments</rdfs:comment>
        <rdfs:isDefinedBy rdf:resource="https://www.theworldavatar.com/kg/ontopoi"/>
        <rdfs:label>Hospices</rdfs:label>
    </owl:Class>
    


    <!-- https://www.theworldavatar.com/kg/ontopoi/Hospitals -->


    <owl:Class rdf:about="https://www.theworldavatar.com/kg/ontopoi/Hospitals">
        <rdfs:subClassOf rdf:resource="https://www.theworldavatar.com/kg/ontopoi/HealthPractitionersAndEstablishments"/>
        <rdfs:comment>Hospitals is a subcategory of health practitioners and establishments</rdfs:comment>
        <rdfs:isDefinedBy rdf:resource="https://www.theworldavatar.com/kg/ontopoi"/>
        <rdfs:label>Hospitals</rdfs:label>
    </owl:Class>
    


    <!-- https://www.theworldavatar.com/kg/ontopoi/HostelsAndRefugesForTheHomeless -->


    <owl:Class rdf:about="https://www.theworldavatar.com/kg/ontopoi/HostelsAndRefugesForTheHomeless">
        <rdfs:subClassOf rdf:resource="https://www.theworldavatar.com/kg/ontopoi/Accommodation"/>
        <rdfs:comment>Hostels and refuges for the homeless is a subcategory of accommodation</rdfs:comment>
        <rdfs:isDefinedBy rdf:resource="https://www.theworldavatar.com/kg/ontopoi"/>
        <rdfs:label>Hostels and refuges for the homeless</rdfs:label>
    </owl:Class>
    


    <!-- https://www.theworldavatar.com/kg/ontopoi/HotAirBallooning -->


    <owl:Class rdf:about="https://www.theworldavatar.com/kg/ontopoi/HotAirBallooning">
        <rdfs:subClassOf rdf:resource="https://www.theworldavatar.com/kg/ontopoi/OutdoorPursuits"/>
        <rdfs:comment>Hot air ballooning is a subcategory of outdoor pursuits</rdfs:comment>
        <rdfs:isDefinedBy rdf:resource="https://www.theworldavatar.com/kg/ontopoi"/>
        <rdfs:label>Hot air ballooning</rdfs:label>
    </owl:Class>
    


    <!-- https://www.theworldavatar.com/kg/ontopoi/HotelBookingAgencies -->


    <owl:Class rdf:about="https://www.theworldavatar.com/kg/ontopoi/HotelBookingAgencies">
        <rdfs:subClassOf rdf:resource="https://www.theworldavatar.com/kg/ontopoi/PersonalAndConsumerAndOtherServices"/>
        <rdfs:comment>Hotel booking agencies is a subcategory of personal, consumer and other services</rdfs:comment>
        <rdfs:isDefinedBy rdf:resource="https://www.theworldavatar.com/kg/ontopoi"/>
        <rdfs:label>Hotel Booking Agencies</rdfs:label>
    </owl:Class>
    


    <!-- https://www.theworldavatar.com/kg/ontopoi/HotelsAndMotelsAndCountryHousesAndInns -->


    <owl:Class rdf:about="https://www.theworldavatar.com/kg/ontopoi/HotelsAndMotelsAndCountryHousesAndInns">
        <rdfs:subClassOf rdf:resource="https://www.theworldavatar.com/kg/ontopoi/Accommodation"/>
        <rdfs:comment>Hotels, motels, country houses and inns is a subcategory of accommodation</rdfs:comment>
        <rdfs:isDefinedBy rdf:resource="https://www.theworldavatar.com/kg/ontopoi"/>
        <rdfs:label>Hotels, motels, country houses and inns</rdfs:label>
    </owl:Class>
    


    <!-- https://www.theworldavatar.com/kg/ontopoi/HouseholdAndOfficeAndLeisureAndGarden -->


    <owl:Class rdf:about="https://www.theworldavatar.com/kg/ontopoi/HouseholdAndOfficeAndLeisureAndGarden">
        <rdfs:subClassOf rdf:resource="https://www.theworldavatar.com/kg/ontopoi/Retail"/>
        <rdfs:comment>Household, office, leisure and garden is a subcategory of retail</rdfs:comment>
        <rdfs:isDefinedBy rdf:resource="https://www.theworldavatar.com/kg/ontopoi"/>
        <rdfs:label>Household, office, leisure and garden</rdfs:label>
    </owl:Class>
    


    <!-- https://www.theworldavatar.com/kg/ontopoi/HouseholdRepairsAndRestoration -->


    <owl:Class rdf:about="https://www.theworldavatar.com/kg/ontopoi/HouseholdRepairsAndRestoration">
        <rdfs:subClassOf rdf:resource="https://www.theworldavatar.com/kg/ontopoi/RepairAndServicing"/>
        <rdfs:comment>Household repairs and restoration is a subcategory of repair and servicing</rdfs:comment>
        <rdfs:isDefinedBy rdf:resource="https://www.theworldavatar.com/kg/ontopoi"/>
        <rdfs:label>Household repairs and restoration</rdfs:label>
    </owl:Class>
    


    <!-- https://www.theworldavatar.com/kg/ontopoi/HydraulicEngineers -->


    <owl:Class rdf:about="https://www.theworldavatar.com/kg/ontopoi/HydraulicEngineers">
        <rdfs:subClassOf rdf:resource="https://www.theworldavatar.com/kg/ontopoi/EngineeringServices"/>
        <rdfs:comment>Hydraulic engineers is a subcategory of engineering services</rdfs:comment>
        <rdfs:isDefinedBy rdf:resource="https://www.theworldavatar.com/kg/ontopoi"/>
        <rdfs:label>Hydraulic engineers</rdfs:label>
    </owl:Class>
    


    <!-- https://www.theworldavatar.com/kg/ontopoi/ITN -->


    <owl:Class rdf:about="https://www.theworldavatar.com/kg/ontopoi/ITN">
        <rdfs:comment>The Integrated Transport Network (ITN) infrastructure, including roads, paths, and transport networks in the UK</rdfs:comment>
        <rdfs:isDefinedBy rdf:resource="https://www.theworldavatar.com/kg/ontopoi"/>
        <rdfs:label>ITN</rdfs:label>
    </owl:Class>
    


    <!-- https://www.theworldavatar.com/kg/ontopoi/Ice -->


    <owl:Class rdf:about="https://www.theworldavatar.com/kg/ontopoi/Ice">
        <rdfs:subClassOf rdf:resource="https://www.theworldavatar.com/kg/ontopoi/IndustrialProducts"/>
        <rdfs:comment>Ice is a subcategory of industrial products</rdfs:comment>
        <rdfs:isDefinedBy rdf:resource="https://www.theworldavatar.com/kg/ontopoi"/>
        <rdfs:label>Ice</rdfs:label>
    </owl:Class>
    


    <!-- https://www.theworldavatar.com/kg/ontopoi/IceRinks -->


    <owl:Class rdf:about="https://www.theworldavatar.com/kg/ontopoi/IceRinks">
        <rdfs:subClassOf rdf:resource="https://www.theworldavatar.com/kg/ontopoi/SportsComplex"/>
        <rdfs:comment>Ice rinks is a subcategory of sports complex</rdfs:comment>
        <rdfs:isDefinedBy rdf:resource="https://www.theworldavatar.com/kg/ontopoi"/>
        <rdfs:label>Ice rinks</rdfs:label>
    </owl:Class>
    


    <!-- https://www.theworldavatar.com/kg/ontopoi/ImageConsultants -->


    <owl:Class rdf:about="https://www.theworldavatar.com/kg/ontopoi/ImageConsultants">
        <rdfs:subClassOf rdf:resource="https://www.theworldavatar.com/kg/ontopoi/Consultancies"/>
        <rdfs:comment>Image consultants is a subcategory of consultancies</rdfs:comment>
        <rdfs:isDefinedBy rdf:resource="https://www.theworldavatar.com/kg/ontopoi"/>
        <rdfs:label>Image consultants</rdfs:label>
    </owl:Class>
    


    <!-- https://www.theworldavatar.com/kg/ontopoi/ImportAndExportServices -->


    <owl:Class rdf:about="https://www.theworldavatar.com/kg/ontopoi/ImportAndExportServices">
        <rdfs:subClassOf rdf:resource="https://www.theworldavatar.com/kg/ontopoi/TransportAndStorageAndDelivery"/>
        <rdfs:comment>Import and export services is a subcategory of transport, storage and delivery</rdfs:comment>
        <rdfs:isDefinedBy rdf:resource="https://www.theworldavatar.com/kg/ontopoi"/>
        <rdfs:label>Import and export services</rdfs:label>
    </owl:Class>
    


    <!-- https://www.theworldavatar.com/kg/ontopoi/IndependentAndPreparatorySchools -->


    <owl:Class rdf:about="https://www.theworldavatar.com/kg/ontopoi/IndependentAndPreparatorySchools">
        <rdfs:subClassOf rdf:resource="https://www.theworldavatar.com/kg/ontopoi/PrimaryAndSecondaryAndTertiaryEducation"/>
        <rdfs:comment>Independent and preparatory schools is a subcategory of primary, secondary and tertiary education</rdfs:comment>
        <rdfs:isDefinedBy rdf:resource="https://www.theworldavatar.com/kg/ontopoi"/>
        <rdfs:label>Independent and preparatory schools</rdfs:label>
    </owl:Class>
    


    <!-- https://www.theworldavatar.com/kg/ontopoi/IndustrialCoatingsAndFinishings -->


    <owl:Class rdf:about="https://www.theworldavatar.com/kg/ontopoi/IndustrialCoatingsAndFinishings">
        <rdfs:subClassOf rdf:resource="https://www.theworldavatar.com/kg/ontopoi/IndustrialProducts"/>
        <rdfs:comment>Industrial coatings and finishings is a subcategory of industrial products</rdfs:comment>
        <rdfs:isDefinedBy rdf:resource="https://www.theworldavatar.com/kg/ontopoi"/>
        <rdfs:label>Industrial coatings and finishings</rdfs:label>
    </owl:Class>
    


    <!-- https://www.theworldavatar.com/kg/ontopoi/IndustrialEngineers -->


    <owl:Class rdf:about="https://www.theworldavatar.com/kg/ontopoi/IndustrialEngineers">
        <rdfs:subClassOf rdf:resource="https://www.theworldavatar.com/kg/ontopoi/EngineeringServices"/>
        <rdfs:comment>Industrial engineers is a subcategory of engineering services</rdfs:comment>
        <rdfs:isDefinedBy rdf:resource="https://www.theworldavatar.com/kg/ontopoi"/>
        <rdfs:label>Industrial engineers</rdfs:label>
    </owl:Class>
    


    <!-- https://www.theworldavatar.com/kg/ontopoi/IndustrialFeatures -->


    <owl:Class rdf:about="https://www.theworldavatar.com/kg/ontopoi/IndustrialFeatures">
        <rdfs:subClassOf rdf:resource="https://www.theworldavatar.com/kg/ontopoi/ManufacturingAndProduction"/>
        <rdfs:comment>Industrial features is a subcategory of manufacturing and production</rdfs:comment>
        <rdfs:isDefinedBy rdf:resource="https://www.theworldavatar.com/kg/ontopoi"/>
        <rdfs:label>Industrial features</rdfs:label>
    </owl:Class>
    


    <!-- https://www.theworldavatar.com/kg/ontopoi/IndustrialProducts -->


    <owl:Class rdf:about="https://www.theworldavatar.com/kg/ontopoi/IndustrialProducts">
        <rdfs:subClassOf rdf:resource="https://www.theworldavatar.com/kg/ontopoi/ManufacturingAndProduction"/>
        <rdfs:comment>Industrial products is a subcategory of manufacturing and production</rdfs:comment>
        <rdfs:isDefinedBy rdf:resource="https://www.theworldavatar.com/kg/ontopoi"/>
        <rdfs:label>Industrial products</rdfs:label>
    </owl:Class>
    


    <!-- https://www.theworldavatar.com/kg/ontopoi/IndustrialRepairsAndServicing -->


    <owl:Class rdf:about="https://www.theworldavatar.com/kg/ontopoi/IndustrialRepairsAndServicing">
        <rdfs:subClassOf rdf:resource="https://www.theworldavatar.com/kg/ontopoi/RepairAndServicing"/>
        <rdfs:comment>Industrial repairs and servicing is a subcategory of repair and servicing</rdfs:comment>
        <rdfs:isDefinedBy rdf:resource="https://www.theworldavatar.com/kg/ontopoi"/>
        <rdfs:label>Industrial repairs and servicing</rdfs:label>
    </owl:Class>
    


    <!-- https://www.theworldavatar.com/kg/ontopoi/InformationCentres -->


    <owl:Class rdf:about="https://www.theworldavatar.com/kg/ontopoi/InformationCentres">
        <rdfs:subClassOf rdf:resource="https://www.theworldavatar.com/kg/ontopoi/Tourism"/>
        <rdfs:comment>Information centres is a subcategory of tourism</rdfs:comment>
        <rdfs:isDefinedBy rdf:resource="https://www.theworldavatar.com/kg/ontopoi"/>
        <rdfs:label>Information centres</rdfs:label>
    </owl:Class>
    


    <!-- https://www.theworldavatar.com/kg/ontopoi/InfrastructureAndFacilities -->


    <owl:Class rdf:about="https://www.theworldavatar.com/kg/ontopoi/InfrastructureAndFacilities">
        <rdfs:subClassOf rdf:resource="https://www.theworldavatar.com/kg/ontopoi/PublicInfrastructure"/>
        <rdfs:comment>Infrastructure and facilities is a subcategory of public infrastructure</rdfs:comment>
        <rdfs:isDefinedBy rdf:resource="https://www.theworldavatar.com/kg/ontopoi"/>
        <rdfs:label>Infrastructure and facilities</rdfs:label>
    </owl:Class>
    


    <!-- https://www.theworldavatar.com/kg/ontopoi/InstitutesAndProfessionalOrganisations -->


    <owl:Class rdf:about="https://www.theworldavatar.com/kg/ontopoi/InstitutesAndProfessionalOrganisations">
        <rdfs:subClassOf rdf:resource="https://www.theworldavatar.com/kg/ontopoi/Organisations"/>
        <rdfs:comment>Institutes and professional organisations is a subcategory of organisations</rdfs:comment>
        <rdfs:isDefinedBy rdf:resource="https://www.theworldavatar.com/kg/ontopoi"/>
        <rdfs:label>Institutes and professional organisations</rdfs:label>
    </owl:Class>
    


    <!-- https://www.theworldavatar.com/kg/ontopoi/InstrumentationEngineers -->


    <owl:Class rdf:about="https://www.theworldavatar.com/kg/ontopoi/InstrumentationEngineers">
        <rdfs:subClassOf rdf:resource="https://www.theworldavatar.com/kg/ontopoi/EngineeringServices"/>
        <rdfs:comment>Instrumentation engineers is a subcategory of engineering services</rdfs:comment>
        <rdfs:isDefinedBy rdf:resource="https://www.theworldavatar.com/kg/ontopoi"/>
        <rdfs:label>Instrumentation engineers</rdfs:label>
    </owl:Class>
    


    <!-- https://www.theworldavatar.com/kg/ontopoi/InsurersAndSupportActivities -->


    <owl:Class rdf:about="https://www.theworldavatar.com/kg/ontopoi/InsurersAndSupportActivities">
        <rdfs:subClassOf rdf:resource="https://www.theworldavatar.com/kg/ontopoi/LegalAndFinancial"/>
        <rdfs:comment>Insurers and support activities is a subcategory of legal and financial</rdfs:comment>
        <rdfs:isDefinedBy rdf:resource="https://www.theworldavatar.com/kg/ontopoi"/>
        <rdfs:label>Insurers and support activities</rdfs:label>
    </owl:Class>
    


    <!-- https://www.theworldavatar.com/kg/ontopoi/InternetCafes -->


    <owl:Class rdf:about="https://www.theworldavatar.com/kg/ontopoi/InternetCafes">
        <rdfs:subClassOf rdf:resource="https://www.theworldavatar.com/kg/ontopoi/EatingAndDrinking"/>
        <rdfs:comment>Internet cafes is a subcategory of eating and drinking</rdfs:comment>
        <rdfs:isDefinedBy rdf:resource="https://www.theworldavatar.com/kg/ontopoi"/>
        <rdfs:label>Internet Cafes</rdfs:label>
    </owl:Class>
    


    <!-- https://www.theworldavatar.com/kg/ontopoi/InternetServices -->


    <owl:Class rdf:about="https://www.theworldavatar.com/kg/ontopoi/InternetServices">
        <rdfs:subClassOf rdf:resource="https://www.theworldavatar.com/kg/ontopoi/ItAndAdvertisingAndMarketingAndMediaServiceS"/>
        <rdfs:comment>Internet services is a subcategory of it, advertising, marketing and media service s</rdfs:comment>
        <rdfs:isDefinedBy rdf:resource="https://www.theworldavatar.com/kg/ontopoi"/>
        <rdfs:label>Internet services</rdfs:label>
    </owl:Class>
    


    <!-- https://www.theworldavatar.com/kg/ontopoi/InterpretationAndTranslationConsultants -->


    <owl:Class rdf:about="https://www.theworldavatar.com/kg/ontopoi/InterpretationAndTranslationConsultants">
        <rdfs:subClassOf rdf:resource="https://www.theworldavatar.com/kg/ontopoi/Consultancies"/>
        <rdfs:comment>Interpretation and translation consultants is a subcategory of consultancies</rdfs:comment>
        <rdfs:isDefinedBy rdf:resource="https://www.theworldavatar.com/kg/ontopoi"/>
        <rdfs:label>Interpretation and translation consultants</rdfs:label>
    </owl:Class>
    


    <!-- https://www.theworldavatar.com/kg/ontopoi/IntroductionAndDatingAgencies -->


    <owl:Class rdf:about="https://www.theworldavatar.com/kg/ontopoi/IntroductionAndDatingAgencies">
        <rdfs:subClassOf rdf:resource="https://www.theworldavatar.com/kg/ontopoi/PersonalAndConsumerAndOtherServices"/>
        <rdfs:comment>Introduction and dating agencies is a subcategory of personal, consumer and other services</rdfs:comment>
        <rdfs:isDefinedBy rdf:resource="https://www.theworldavatar.com/kg/ontopoi"/>
        <rdfs:label>Introduction and dating agencies</rdfs:label>
    </owl:Class>
    


    <!-- https://www.theworldavatar.com/kg/ontopoi/ItAndAdvertisingAndMarketingAndMediaServiceS -->


    <owl:Class rdf:about="https://www.theworldavatar.com/kg/ontopoi/ItAndAdvertisingAndMarketingAndMediaServiceS">
        <rdfs:subClassOf rdf:resource="https://www.theworldavatar.com/kg/ontopoi/CommercialServices"/>
        <rdfs:comment>It, advertising, marketing and media service s is a subcategory of commercial services</rdfs:comment>
        <rdfs:isDefinedBy rdf:resource="https://www.theworldavatar.com/kg/ontopoi"/>
        <rdfs:label>IT, advertising, marketing and media service s</rdfs:label>
    </owl:Class>
    


    <!-- https://www.theworldavatar.com/kg/ontopoi/JewelleryAndFashionAccessories -->


    <owl:Class rdf:about="https://www.theworldavatar.com/kg/ontopoi/JewelleryAndFashionAccessories">
        <rdfs:subClassOf rdf:resource="https://www.theworldavatar.com/kg/ontopoi/ClothingAndAccessories"/>
        <rdfs:comment>Jewellery and fashion accessories is a subcategory of clothing and accessories</rdfs:comment>
        <rdfs:isDefinedBy rdf:resource="https://www.theworldavatar.com/kg/ontopoi"/>
        <rdfs:label>Jewellery and fashion accessories</rdfs:label>
    </owl:Class>
    


    <!-- https://www.theworldavatar.com/kg/ontopoi/JewelleryAndGemsAndClocksAndWatches -->


    <owl:Class rdf:about="https://www.theworldavatar.com/kg/ontopoi/JewelleryAndGemsAndClocksAndWatches">
        <rdfs:subClassOf rdf:resource="https://www.theworldavatar.com/kg/ontopoi/ConsumerProducts"/>
        <rdfs:comment>Jewellery, gems, clocks and watches is a subcategory of consumer products</rdfs:comment>
        <rdfs:isDefinedBy rdf:resource="https://www.theworldavatar.com/kg/ontopoi"/>
        <rdfs:label>Jewellery, gems, clocks and watches</rdfs:label>
    </owl:Class>
    


    <!-- https://www.theworldavatar.com/kg/ontopoi/JobCentres -->


    <owl:Class rdf:about="https://www.theworldavatar.com/kg/ontopoi/JobCentres">
        <rdfs:subClassOf rdf:resource="https://www.theworldavatar.com/kg/ontopoi/CentralAndLocalGovernment"/>
        <rdfs:comment>Job centres is a subcategory of central and local government</rdfs:comment>
        <rdfs:isDefinedBy rdf:resource="https://www.theworldavatar.com/kg/ontopoi"/>
        <rdfs:label>Job centres</rdfs:label>
    </owl:Class>
    


    <!-- https://www.theworldavatar.com/kg/ontopoi/KennelsAndCatteries -->


    <owl:Class rdf:about="https://www.theworldavatar.com/kg/ontopoi/KennelsAndCatteries">
        <rdfs:subClassOf rdf:resource="https://www.theworldavatar.com/kg/ontopoi/AnimalWelfare"/>
        <rdfs:comment>Kennels and catteries is a subcategory of animal welfare</rdfs:comment>
        <rdfs:isDefinedBy rdf:resource="https://www.theworldavatar.com/kg/ontopoi"/>
        <rdfs:label>Kennels and catteries</rdfs:label>
    </owl:Class>
    


    <!-- https://www.theworldavatar.com/kg/ontopoi/LakesAndWaters -->


    <owl:Class rdf:about="https://www.theworldavatar.com/kg/ontopoi/LakesAndWaters">
        <rdfs:subClassOf rdf:resource="https://www.theworldavatar.com/kg/ontopoi/BodiesOfWater"/>
        <rdfs:comment>Lakes and waters is a subcategory of bodies of water</rdfs:comment>
        <rdfs:isDefinedBy rdf:resource="https://www.theworldavatar.com/kg/ontopoi"/>
        <rdfs:label>Lakes and waters</rdfs:label>
    </owl:Class>
    


    <!-- https://www.theworldavatar.com/kg/ontopoi/LampshadesAndLighting -->


    <owl:Class rdf:about="https://www.theworldavatar.com/kg/ontopoi/LampshadesAndLighting">
        <rdfs:subClassOf rdf:resource="https://www.theworldavatar.com/kg/ontopoi/ConsumerProducts"/>
        <rdfs:comment>Lampshades and lighting is a subcategory of consumer products</rdfs:comment>
        <rdfs:isDefinedBy rdf:resource="https://www.theworldavatar.com/kg/ontopoi"/>
        <rdfs:label>Lampshades and lighting</rdfs:label>
    </owl:Class>
    


    <!-- https://www.theworldavatar.com/kg/ontopoi/LandscapeFeatures -->


    <owl:Class rdf:about="https://www.theworldavatar.com/kg/ontopoi/LandscapeFeatures">
        <rdfs:subClassOf rdf:resource="https://www.theworldavatar.com/kg/ontopoi/Attractions"/>
        <rdfs:comment>Landscape features is a subcategory of attractions</rdfs:comment>
        <rdfs:isDefinedBy rdf:resource="https://www.theworldavatar.com/kg/ontopoi"/>
        <rdfs:label>Landscape features</rdfs:label>
    </owl:Class>
    


    <!-- https://www.theworldavatar.com/kg/ontopoi/LanguageSchools -->


    <owl:Class rdf:about="https://www.theworldavatar.com/kg/ontopoi/LanguageSchools">
        <rdfs:subClassOf rdf:resource="https://www.theworldavatar.com/kg/ontopoi/RecreationalAndVocationalEducation"/>
        <rdfs:comment>Language schools is a subcategory of recreational and vocational education</rdfs:comment>
        <rdfs:isDefinedBy rdf:resource="https://www.theworldavatar.com/kg/ontopoi"/>
        <rdfs:label>Language schools</rdfs:label>
    </owl:Class>
    


    <!-- https://www.theworldavatar.com/kg/ontopoi/LaseriaAndObservatoriesAndPlanetaria -->


    <owl:Class rdf:about="https://www.theworldavatar.com/kg/ontopoi/LaseriaAndObservatoriesAndPlanetaria">
        <rdfs:subClassOf rdf:resource="https://www.theworldavatar.com/kg/ontopoi/Tourism"/>
        <rdfs:comment>Laseria, observatories and planetaria is a subcategory of tourism</rdfs:comment>
        <rdfs:isDefinedBy rdf:resource="https://www.theworldavatar.com/kg/ontopoi"/>
        <rdfs:label>Laseria, observatories and planetaria</rdfs:label>
    </owl:Class>
    


    <!-- https://www.theworldavatar.com/kg/ontopoi/LeatherGoodsAndLuggageAndTravelAccessoriesIncludingHandbags -->


    <owl:Class rdf:about="https://www.theworldavatar.com/kg/ontopoi/LeatherGoodsAndLuggageAndTravelAccessoriesIncludingHandbags">
        <rdfs:subClassOf rdf:resource="https://www.theworldavatar.com/kg/ontopoi/HouseholdAndOfficeAndLeisureAndGarden"/>
        <rdfs:comment>Leather goods, luggage and travel accessories including handbags is a subcategory of household, office, leisure and garden</rdfs:comment>
        <rdfs:isDefinedBy rdf:resource="https://www.theworldavatar.com/kg/ontopoi"/>
        <rdfs:label>Leather goods, luggage and travel accessories including handbags</rdfs:label>
    </owl:Class>
    


    <!-- https://www.theworldavatar.com/kg/ontopoi/LeatherProducts -->


    <owl:Class rdf:about="https://www.theworldavatar.com/kg/ontopoi/LeatherProducts">
        <rdfs:subClassOf rdf:resource="https://www.theworldavatar.com/kg/ontopoi/ConsumerProducts"/>
        <rdfs:comment>Leather products is a subcategory of consumer products</rdfs:comment>
        <rdfs:isDefinedBy rdf:resource="https://www.theworldavatar.com/kg/ontopoi"/>
        <rdfs:label>Leather products</rdfs:label>
    </owl:Class>
    


    <!-- https://www.theworldavatar.com/kg/ontopoi/LegalAndFinancial -->


    <owl:Class rdf:about="https://www.theworldavatar.com/kg/ontopoi/LegalAndFinancial">
        <rdfs:subClassOf rdf:resource="https://www.theworldavatar.com/kg/ontopoi/CommercialServices"/>
        <rdfs:comment>Legal and financial is a subcategory of commercial services</rdfs:comment>
        <rdfs:isDefinedBy rdf:resource="https://www.theworldavatar.com/kg/ontopoi"/>
        <rdfs:label>Legal and financial</rdfs:label>
    </owl:Class>
    


    <!-- https://www.theworldavatar.com/kg/ontopoi/LeisureEquipmentHirings -->


    <owl:Class rdf:about="https://www.theworldavatar.com/kg/ontopoi/LeisureEquipmentHirings">
        <rdfs:subClassOf rdf:resource="https://www.theworldavatar.com/kg/ontopoi/HireServices"/>
        <rdfs:comment>Leisure equipment hirings is a subcategory of hire services</rdfs:comment>
        <rdfs:isDefinedBy rdf:resource="https://www.theworldavatar.com/kg/ontopoi"/>
        <rdfs:label>Leisure equipment hirings</rdfs:label>
    </owl:Class>
    


    <!-- https://www.theworldavatar.com/kg/ontopoi/LetterBoxes -->


    <owl:Class rdf:about="https://www.theworldavatar.com/kg/ontopoi/LetterBoxes">
        <rdfs:subClassOf rdf:resource="https://www.theworldavatar.com/kg/ontopoi/InfrastructureAndFacilities"/>
        <rdfs:comment>Letter boxes is a subcategory of infrastructure and facilities</rdfs:comment>
        <rdfs:isDefinedBy rdf:resource="https://www.theworldavatar.com/kg/ontopoi"/>
        <rdfs:label>Letter boxes</rdfs:label>
    </owl:Class>
    


    <!-- https://www.theworldavatar.com/kg/ontopoi/Libraries -->


    <owl:Class rdf:about="https://www.theworldavatar.com/kg/ontopoi/Libraries">
        <rdfs:subClassOf rdf:resource="https://www.theworldavatar.com/kg/ontopoi/InfrastructureAndFacilities"/>
        <rdfs:comment>Libraries is a subcategory of infrastructure and facilities</rdfs:comment>
        <rdfs:isDefinedBy rdf:resource="https://www.theworldavatar.com/kg/ontopoi"/>
        <rdfs:label>Libraries</rdfs:label>
    </owl:Class>
    


    <!-- https://www.theworldavatar.com/kg/ontopoi/LiftingAndHandlingEquipment -->


    <owl:Class rdf:about="https://www.theworldavatar.com/kg/ontopoi/LiftingAndHandlingEquipment">
        <rdfs:subClassOf rdf:resource="https://www.theworldavatar.com/kg/ontopoi/IndustrialProducts"/>
        <rdfs:comment>Lifting and handling equipment is a subcategory of industrial products</rdfs:comment>
        <rdfs:isDefinedBy rdf:resource="https://www.theworldavatar.com/kg/ontopoi"/>
        <rdfs:label>Lifting and handling equipment</rdfs:label>
    </owl:Class>
    


    <!-- https://www.theworldavatar.com/kg/ontopoi/Lighting -->


    <owl:Class rdf:about="https://www.theworldavatar.com/kg/ontopoi/Lighting">
        <rdfs:subClassOf rdf:resource="https://www.theworldavatar.com/kg/ontopoi/HouseholdAndOfficeAndLeisureAndGarden"/>
        <rdfs:comment>Lighting is a subcategory of household, office, leisure and garden</rdfs:comment>
        <rdfs:isDefinedBy rdf:resource="https://www.theworldavatar.com/kg/ontopoi"/>
        <rdfs:label>Lighting</rdfs:label>
    </owl:Class>
    


    <!-- https://www.theworldavatar.com/kg/ontopoi/LimeKilns -->


    <owl:Class rdf:about="https://www.theworldavatar.com/kg/ontopoi/LimeKilns">
        <rdfs:subClassOf rdf:resource="https://www.theworldavatar.com/kg/ontopoi/IndustrialFeatures"/>
        <rdfs:comment>Lime kilns is a subcategory of industrial features</rdfs:comment>
        <rdfs:isDefinedBy rdf:resource="https://www.theworldavatar.com/kg/ontopoi"/>
        <rdfs:label>Lime kilns</rdfs:label>
    </owl:Class>
    


    <!-- https://www.theworldavatar.com/kg/ontopoi/LinenHireAndWashroomServices -->


    <owl:Class rdf:about="https://www.theworldavatar.com/kg/ontopoi/LinenHireAndWashroomServices">
        <rdfs:subClassOf rdf:resource="https://www.theworldavatar.com/kg/ontopoi/ContractServices"/>
        <rdfs:comment>Linen hire and washroom services is a subcategory of contract services</rdfs:comment>
        <rdfs:isDefinedBy rdf:resource="https://www.theworldavatar.com/kg/ontopoi"/>
        <rdfs:label>Linen hire and washroom services</rdfs:label>
    </owl:Class>
    


    <!-- https://www.theworldavatar.com/kg/ontopoi/LingerieAndHosiery -->


    <owl:Class rdf:about="https://www.theworldavatar.com/kg/ontopoi/LingerieAndHosiery">
        <rdfs:subClassOf rdf:resource="https://www.theworldavatar.com/kg/ontopoi/ClothingAndAccessories"/>
        <rdfs:subClassOf rdf:resource="https://www.theworldavatar.com/kg/ontopoi/ConsumerProducts"/>
        <rdfs:comment>Lingerie and hosiery is a subcategory of clothing and accessories</rdfs:comment>
        <rdfs:comment>Lingerie and hosiery is a subcategory of consumer products</rdfs:comment>
        <rdfs:isDefinedBy rdf:resource="https://www.theworldavatar.com/kg/ontopoi"/>
        <rdfs:label>Lingerie and hosiery</rdfs:label>
    </owl:Class>
    


    <!-- https://www.theworldavatar.com/kg/ontopoi/LiteraryServices -->


    <owl:Class rdf:about="https://www.theworldavatar.com/kg/ontopoi/LiteraryServices">
        <rdfs:subClassOf rdf:resource="https://www.theworldavatar.com/kg/ontopoi/ItAndAdvertisingAndMarketingAndMediaServiceS"/>
        <rdfs:comment>Literary services is a subcategory of it, advertising, marketing and media service s</rdfs:comment>
        <rdfs:isDefinedBy rdf:resource="https://www.theworldavatar.com/kg/ontopoi"/>
        <rdfs:label>Literary services</rdfs:label>
    </owl:Class>
    


    <!-- https://www.theworldavatar.com/kg/ontopoi/LivestockFarming -->


    <owl:Class rdf:about="https://www.theworldavatar.com/kg/ontopoi/LivestockFarming">
        <rdfs:subClassOf rdf:resource="https://www.theworldavatar.com/kg/ontopoi/Farming"/>
        <rdfs:comment>Livestock farming is a subcategory of farming</rdfs:comment>
        <rdfs:isDefinedBy rdf:resource="https://www.theworldavatar.com/kg/ontopoi"/>
        <rdfs:label>Livestock farming</rdfs:label>
    </owl:Class>
    


    <!-- https://www.theworldavatar.com/kg/ontopoi/LivestockMarkets -->


    <owl:Class rdf:about="https://www.theworldavatar.com/kg/ontopoi/LivestockMarkets">
        <rdfs:subClassOf rdf:resource="https://www.theworldavatar.com/kg/ontopoi/FoodAndDrinkAndMultiItemRetail"/>
        <rdfs:comment>Livestock markets is a subcategory of food, drink and multi item retail</rdfs:comment>
        <rdfs:isDefinedBy rdf:resource="https://www.theworldavatar.com/kg/ontopoi"/>
        <rdfs:label>Livestock markets</rdfs:label>
    </owl:Class>
    


    <!-- https://www.theworldavatar.com/kg/ontopoi/LocalGovernment -->


    <owl:Class rdf:about="https://www.theworldavatar.com/kg/ontopoi/LocalGovernment">
        <rdfs:subClassOf rdf:resource="https://www.theworldavatar.com/kg/ontopoi/CentralAndLocalGovernment"/>
        <rdfs:comment>Local government is a subcategory of central and local government</rdfs:comment>
        <rdfs:isDefinedBy rdf:resource="https://www.theworldavatar.com/kg/ontopoi"/>
        <rdfs:label>Local government</rdfs:label>
    </owl:Class>
    


    <!-- https://www.theworldavatar.com/kg/ontopoi/Locality -->


    <owl:Class rdf:about="https://www.theworldavatar.com/kg/ontopoi/Locality"/>
    


    <!-- https://www.theworldavatar.com/kg/ontopoi/LochsAndLochans -->


    <owl:Class rdf:about="https://www.theworldavatar.com/kg/ontopoi/LochsAndLochans">
        <rdfs:subClassOf rdf:resource="https://www.theworldavatar.com/kg/ontopoi/BodiesOfWater"/>
        <rdfs:comment>Lochs and lochans is a subcategory of bodies of water</rdfs:comment>
        <rdfs:isDefinedBy rdf:resource="https://www.theworldavatar.com/kg/ontopoi"/>
        <rdfs:label>Lochs and lochans</rdfs:label>
    </owl:Class>
    


    <!-- https://www.theworldavatar.com/kg/ontopoi/LockAndKeyAndSecurityServices -->


    <owl:Class rdf:about="https://www.theworldavatar.com/kg/ontopoi/LockAndKeyAndSecurityServices">
        <rdfs:subClassOf rdf:resource="https://www.theworldavatar.com/kg/ontopoi/PersonalAndConsumerAndOtherServices"/>
        <rdfs:comment>Lock, key and security services is a subcategory of personal, consumer and other services</rdfs:comment>
        <rdfs:isDefinedBy rdf:resource="https://www.theworldavatar.com/kg/ontopoi"/>
        <rdfs:label>Lock, key and security services</rdfs:label>
    </owl:Class>
    


    <!-- https://www.theworldavatar.com/kg/ontopoi/Locks -->


    <owl:Class rdf:about="https://www.theworldavatar.com/kg/ontopoi/Locks">
        <rdfs:subClassOf rdf:resource="https://www.theworldavatar.com/kg/ontopoi/Water"/>
        <rdfs:comment>Locks is a subcategory of water</rdfs:comment>
        <rdfs:isDefinedBy rdf:resource="https://www.theworldavatar.com/kg/ontopoi"/>
        <rdfs:label>Locks</rdfs:label>
    </owl:Class>
    


    <!-- https://www.theworldavatar.com/kg/ontopoi/LondonUndergroundEntrances -->


    <owl:Class rdf:about="https://www.theworldavatar.com/kg/ontopoi/LondonUndergroundEntrances">
        <rdfs:subClassOf rdf:resource="https://www.theworldavatar.com/kg/ontopoi/PublicTransportAndStationsAndInfrastructure"/>
        <rdfs:comment>London underground entrances is a subcategory of public transport, stations and infrastructure</rdfs:comment>
        <rdfs:isDefinedBy rdf:resource="https://www.theworldavatar.com/kg/ontopoi"/>
        <rdfs:label>London Underground entrances</rdfs:label>
    </owl:Class>
    


    <!-- https://www.theworldavatar.com/kg/ontopoi/LubricantsAndLubricatingEquipment -->


    <owl:Class rdf:about="https://www.theworldavatar.com/kg/ontopoi/LubricantsAndLubricatingEquipment">
        <rdfs:subClassOf rdf:resource="https://www.theworldavatar.com/kg/ontopoi/IndustrialProducts"/>
        <rdfs:comment>Lubricants and lubricating equipment is a subcategory of industrial products</rdfs:comment>
        <rdfs:isDefinedBy rdf:resource="https://www.theworldavatar.com/kg/ontopoi"/>
        <rdfs:label>Lubricants and lubricating equipment</rdfs:label>
    </owl:Class>
    


    <!-- https://www.theworldavatar.com/kg/ontopoi/LuggageAndBagsAndUmbrellasAndTravelAccessories -->


    <owl:Class rdf:about="https://www.theworldavatar.com/kg/ontopoi/LuggageAndBagsAndUmbrellasAndTravelAccessories">
        <rdfs:subClassOf rdf:resource="https://www.theworldavatar.com/kg/ontopoi/ConsumerProducts"/>
        <rdfs:comment>Luggage, bags, umbrellas and travel accessories is a subcategory of consumer products</rdfs:comment>
        <rdfs:isDefinedBy rdf:resource="https://www.theworldavatar.com/kg/ontopoi"/>
        <rdfs:label>Luggage, bags, umbrellas and travel accessories</rdfs:label>
    </owl:Class>
    


    <!-- https://www.theworldavatar.com/kg/ontopoi/MailOrderAndCatalogueStores -->


    <owl:Class rdf:about="https://www.theworldavatar.com/kg/ontopoi/MailOrderAndCatalogueStores">
        <rdfs:subClassOf rdf:resource="https://www.theworldavatar.com/kg/ontopoi/HouseholdAndOfficeAndLeisureAndGarden"/>
        <rdfs:comment>Mail order and catalogue stores is a subcategory of household, office, leisure and garden</rdfs:comment>
        <rdfs:isDefinedBy rdf:resource="https://www.theworldavatar.com/kg/ontopoi"/>
        <rdfs:label>Mail order and catalogue stores</rdfs:label>
    </owl:Class>
    


    <!-- https://www.theworldavatar.com/kg/ontopoi/MailingAndOtherInformationServices -->


    <owl:Class rdf:about="https://www.theworldavatar.com/kg/ontopoi/MailingAndOtherInformationServices">
        <rdfs:subClassOf rdf:resource="https://www.theworldavatar.com/kg/ontopoi/ItAndAdvertisingAndMarketingAndMediaServiceS"/>
        <rdfs:comment>Mailing and other information services is a subcategory of it, advertising, marketing and media service s</rdfs:comment>
        <rdfs:isDefinedBy rdf:resource="https://www.theworldavatar.com/kg/ontopoi"/>
        <rdfs:label>Mailing and other information services</rdfs:label>
    </owl:Class>
    


    <!-- https://www.theworldavatar.com/kg/ontopoi/ManufacturingAndProduction -->


    <owl:Class rdf:about="https://www.theworldavatar.com/kg/ontopoi/ManufacturingAndProduction">
        <rdfs:subClassOf rdf:resource="https://www.theworldavatar.com/kg/ontopoi/PointOfInterest"/>
        <rdfs:comment>Places where the processes involved in creating goods and products from raw materials through various methods and techniques take place</rdfs:comment>
        <rdfs:isDefinedBy rdf:resource="https://www.theworldavatar.com/kg/ontopoi"/>
        <rdfs:label>Manufacturing and production</rdfs:label>
    </owl:Class>
    


    <!-- https://www.theworldavatar.com/kg/ontopoi/MarineEngineersAndServices -->


    <owl:Class rdf:about="https://www.theworldavatar.com/kg/ontopoi/MarineEngineersAndServices">
        <rdfs:subClassOf rdf:resource="https://www.theworldavatar.com/kg/ontopoi/EngineeringServices"/>
        <rdfs:comment>Marine engineers and services is a subcategory of engineering services</rdfs:comment>
        <rdfs:isDefinedBy rdf:resource="https://www.theworldavatar.com/kg/ontopoi"/>
        <rdfs:label>Marine engineers and services</rdfs:label>
    </owl:Class>
    


    <!-- https://www.theworldavatar.com/kg/ontopoi/MarineEquipmentIncludingBoatsAndShips -->


    <owl:Class rdf:about="https://www.theworldavatar.com/kg/ontopoi/MarineEquipmentIncludingBoatsAndShips">
        <rdfs:subClassOf rdf:resource="https://www.theworldavatar.com/kg/ontopoi/IndustrialProducts"/>
        <rdfs:comment>Marine equipment including boats and ships is a subcategory of industrial products</rdfs:comment>
        <rdfs:isDefinedBy rdf:resource="https://www.theworldavatar.com/kg/ontopoi"/>
        <rdfs:label>Marine equipment including boats and ships</rdfs:label>
    </owl:Class>
    


    <!-- https://www.theworldavatar.com/kg/ontopoi/MarketingServices -->


    <owl:Class rdf:about="https://www.theworldavatar.com/kg/ontopoi/MarketingServices">
        <rdfs:subClassOf rdf:resource="https://www.theworldavatar.com/kg/ontopoi/ItAndAdvertisingAndMarketingAndMediaServiceS"/>
        <rdfs:comment>Marketing services is a subcategory of it, advertising, marketing and media service s</rdfs:comment>
        <rdfs:isDefinedBy rdf:resource="https://www.theworldavatar.com/kg/ontopoi"/>
        <rdfs:label>Marketing services</rdfs:label>
    </owl:Class>
    


    <!-- https://www.theworldavatar.com/kg/ontopoi/Markets -->


    <owl:Class rdf:about="https://www.theworldavatar.com/kg/ontopoi/Markets">
        <rdfs:subClassOf rdf:resource="https://www.theworldavatar.com/kg/ontopoi/FoodAndDrinkAndMultiItemRetail"/>
        <rdfs:comment>Markets is a subcategory of food, drink and multi item retail</rdfs:comment>
        <rdfs:isDefinedBy rdf:resource="https://www.theworldavatar.com/kg/ontopoi"/>
        <rdfs:label>Markets</rdfs:label>
    </owl:Class>
    


    <!-- https://www.theworldavatar.com/kg/ontopoi/MartialArtsInstruction -->


    <owl:Class rdf:about="https://www.theworldavatar.com/kg/ontopoi/MartialArtsInstruction">
        <rdfs:subClassOf rdf:resource="https://www.theworldavatar.com/kg/ontopoi/RecreationalAndVocationalEducation"/>
        <rdfs:comment>Martial arts instruction is a subcategory of recreational and vocational education</rdfs:comment>
        <rdfs:isDefinedBy rdf:resource="https://www.theworldavatar.com/kg/ontopoi"/>
        <rdfs:label>Martial arts instruction</rdfs:label>
    </owl:Class>
    


    <!-- https://www.theworldavatar.com/kg/ontopoi/MeasurementAndInspectionEquipment -->


    <owl:Class rdf:about="https://www.theworldavatar.com/kg/ontopoi/MeasurementAndInspectionEquipment">
        <rdfs:subClassOf rdf:resource="https://www.theworldavatar.com/kg/ontopoi/IndustrialProducts"/>
        <rdfs:comment>Measurement and inspection equipment is a subcategory of industrial products</rdfs:comment>
        <rdfs:isDefinedBy rdf:resource="https://www.theworldavatar.com/kg/ontopoi"/>
        <rdfs:label>Measurement and inspection equipment</rdfs:label>
    </owl:Class>
    


    <!-- https://www.theworldavatar.com/kg/ontopoi/MechanicalEngineers -->


    <owl:Class rdf:about="https://www.theworldavatar.com/kg/ontopoi/MechanicalEngineers">
        <rdfs:subClassOf rdf:resource="https://www.theworldavatar.com/kg/ontopoi/EngineeringServices"/>
        <rdfs:comment>Mechanical engineers is a subcategory of engineering services</rdfs:comment>
        <rdfs:isDefinedBy rdf:resource="https://www.theworldavatar.com/kg/ontopoi"/>
        <rdfs:label>Mechanical engineers</rdfs:label>
    </owl:Class>
    


    <!-- https://www.theworldavatar.com/kg/ontopoi/MedalsAndTrophiesAndCeremonialAndReligiousGoods -->


    <owl:Class rdf:about="https://www.theworldavatar.com/kg/ontopoi/MedalsAndTrophiesAndCeremonialAndReligiousGoods">
        <rdfs:subClassOf rdf:resource="https://www.theworldavatar.com/kg/ontopoi/ConsumerProducts"/>
        <rdfs:comment>Medals, trophies, ceremonial and religious goods is a subcategory of consumer products</rdfs:comment>
        <rdfs:isDefinedBy rdf:resource="https://www.theworldavatar.com/kg/ontopoi"/>
        <rdfs:label>Medals, trophies, ceremonial and religious goods</rdfs:label>
    </owl:Class>
    


    <!-- https://www.theworldavatar.com/kg/ontopoi/MedicalEquipmentAndSuppliesAndPharmAceuticals -->


    <owl:Class rdf:about="https://www.theworldavatar.com/kg/ontopoi/MedicalEquipmentAndSuppliesAndPharmAceuticals">
        <rdfs:subClassOf rdf:resource="https://www.theworldavatar.com/kg/ontopoi/IndustrialProducts"/>
        <rdfs:comment>Medical equipment, supplies and pharm aceuticals is a subcategory of industrial products</rdfs:comment>
        <rdfs:isDefinedBy rdf:resource="https://www.theworldavatar.com/kg/ontopoi"/>
        <rdfs:label>Medical equipment, supplies and pharm aceuticals</rdfs:label>
    </owl:Class>
    


    <!-- https://www.theworldavatar.com/kg/ontopoi/MedicalEquipmentRentalAndLeasing -->


    <owl:Class rdf:about="https://www.theworldavatar.com/kg/ontopoi/MedicalEquipmentRentalAndLeasing">
        <rdfs:subClassOf rdf:resource="https://www.theworldavatar.com/kg/ontopoi/HealthSupportServices"/>
        <rdfs:comment>Medical equipment rental and leasing is a subcategory of health support services</rdfs:comment>
        <rdfs:isDefinedBy rdf:resource="https://www.theworldavatar.com/kg/ontopoi"/>
        <rdfs:label>Medical equipment rental and leasing</rdfs:label>
    </owl:Class>
    


    <!-- https://www.theworldavatar.com/kg/ontopoi/MedicalWasteDisposalServices -->


    <owl:Class rdf:about="https://www.theworldavatar.com/kg/ontopoi/MedicalWasteDisposalServices">
        <rdfs:subClassOf rdf:resource="https://www.theworldavatar.com/kg/ontopoi/HealthSupportServices"/>
        <rdfs:comment>Medical waste disposal services is a subcategory of health support services</rdfs:comment>
        <rdfs:isDefinedBy rdf:resource="https://www.theworldavatar.com/kg/ontopoi"/>
        <rdfs:label>Medical waste disposal services</rdfs:label>
    </owl:Class>
    


    <!-- https://www.theworldavatar.com/kg/ontopoi/MembersOfParliamentAndMembersOfEuropeanParliament -->


    <owl:Class rdf:about="https://www.theworldavatar.com/kg/ontopoi/MembersOfParliamentAndMembersOfEuropeanParliament">
        <rdfs:subClassOf rdf:resource="https://www.theworldavatar.com/kg/ontopoi/CentralAndLocalGovernment"/>
        <rdfs:comment>Members of parliament and members of european parliament is a subcategory of central and local government</rdfs:comment>
        <rdfs:isDefinedBy rdf:resource="https://www.theworldavatar.com/kg/ontopoi"/>
        <rdfs:label>Members of parliament and members of European parliament</rdfs:label>
    </owl:Class>
    


    <!-- https://www.theworldavatar.com/kg/ontopoi/MentalHealthCentresAndPractitioners -->


    <owl:Class rdf:about="https://www.theworldavatar.com/kg/ontopoi/MentalHealthCentresAndPractitioners">
        <rdfs:subClassOf rdf:resource="https://www.theworldavatar.com/kg/ontopoi/HealthPractitionersAndEstablishments"/>
        <rdfs:comment>Mental health centres and practitioners is a subcategory of health practitioners and establishments</rdfs:comment>
        <rdfs:isDefinedBy rdf:resource="https://www.theworldavatar.com/kg/ontopoi"/>
        <rdfs:label>Mental health centres and practitioners</rdfs:label>
    </owl:Class>
    


    <!-- https://www.theworldavatar.com/kg/ontopoi/MessageAndGreetingServices -->


    <owl:Class rdf:about="https://www.theworldavatar.com/kg/ontopoi/MessageAndGreetingServices">
        <rdfs:subClassOf rdf:resource="https://www.theworldavatar.com/kg/ontopoi/PersonalAndConsumerAndOtherServices"/>
        <rdfs:comment>Message and greeting services is a subcategory of personal, consumer and other services</rdfs:comment>
        <rdfs:isDefinedBy rdf:resource="https://www.theworldavatar.com/kg/ontopoi"/>
        <rdfs:label>Message and greeting services</rdfs:label>
    </owl:Class>
    


    <!-- https://www.theworldavatar.com/kg/ontopoi/MetalsManufacturersAndFabricatorsAndStockholders -->


    <owl:Class rdf:about="https://www.theworldavatar.com/kg/ontopoi/MetalsManufacturersAndFabricatorsAndStockholders">
        <rdfs:subClassOf rdf:resource="https://www.theworldavatar.com/kg/ontopoi/IndustrialProducts"/>
        <rdfs:comment>Metals manufacturers, fabricators and stockholders is a subcategory of industrial products</rdfs:comment>
        <rdfs:isDefinedBy rdf:resource="https://www.theworldavatar.com/kg/ontopoi"/>
        <rdfs:label>Metals manufacturers, fabricators and stockholders</rdfs:label>
    </owl:Class>
    


    <!-- https://www.theworldavatar.com/kg/ontopoi/MetalworkersIncludingBlacksmiths -->


    <owl:Class rdf:about="https://www.theworldavatar.com/kg/ontopoi/MetalworkersIncludingBlacksmiths">
        <rdfs:subClassOf rdf:resource="https://www.theworldavatar.com/kg/ontopoi/ConstructionServices"/>
        <rdfs:comment>Metalworkers including blacksmiths is a subcategory of construction services</rdfs:comment>
        <rdfs:isDefinedBy rdf:resource="https://www.theworldavatar.com/kg/ontopoi"/>
        <rdfs:label>Metalworkers including blacksmiths</rdfs:label>
    </owl:Class>
    


    <!-- https://www.theworldavatar.com/kg/ontopoi/MeteorologicalFeatures -->


    <owl:Class rdf:about="https://www.theworldavatar.com/kg/ontopoi/MeteorologicalFeatures">
        <rdfs:subClassOf rdf:resource="https://www.theworldavatar.com/kg/ontopoi/InfrastructureAndFacilities"/>
        <rdfs:comment>Meteorological features is a subcategory of infrastructure and facilities</rdfs:comment>
        <rdfs:isDefinedBy rdf:resource="https://www.theworldavatar.com/kg/ontopoi"/>
        <rdfs:label>Meteorological features</rdfs:label>
    </owl:Class>
    


    <!-- https://www.theworldavatar.com/kg/ontopoi/Midwifery -->


    <owl:Class rdf:about="https://www.theworldavatar.com/kg/ontopoi/Midwifery">
        <rdfs:subClassOf rdf:resource="https://www.theworldavatar.com/kg/ontopoi/HealthPractitionersAndEstablishments"/>
        <rdfs:comment>Midwifery is a subcategory of health practitioners and establishments</rdfs:comment>
        <rdfs:isDefinedBy rdf:resource="https://www.theworldavatar.com/kg/ontopoi"/>
        <rdfs:label>Midwifery</rdfs:label>
    </owl:Class>
    


    <!-- https://www.theworldavatar.com/kg/ontopoi/MillingAndRefiningAndFoodAdditives -->


    <owl:Class rdf:about="https://www.theworldavatar.com/kg/ontopoi/MillingAndRefiningAndFoodAdditives">
        <rdfs:subClassOf rdf:resource="https://www.theworldavatar.com/kg/ontopoi/Foodstuffs"/>
        <rdfs:comment>Milling, refining and food additives is a subcategory of foodstuffs</rdfs:comment>
        <rdfs:isDefinedBy rdf:resource="https://www.theworldavatar.com/kg/ontopoi"/>
        <rdfs:label>Milling, refining and food additives</rdfs:label>
    </owl:Class>
    


    <!-- https://www.theworldavatar.com/kg/ontopoi/MixedOrUnspecifiedFarming -->


    <owl:Class rdf:about="https://www.theworldavatar.com/kg/ontopoi/MixedOrUnspecifiedFarming">
        <rdfs:subClassOf rdf:resource="https://www.theworldavatar.com/kg/ontopoi/Farming"/>
        <rdfs:comment>Mixed or unspecified farming is a subcategory of farming</rdfs:comment>
        <rdfs:isDefinedBy rdf:resource="https://www.theworldavatar.com/kg/ontopoi"/>
        <rdfs:label>Mixed or unspecified farming</rdfs:label>
    </owl:Class>
    


    <!-- https://www.theworldavatar.com/kg/ontopoi/MobileDiscos -->


    <owl:Class rdf:about="https://www.theworldavatar.com/kg/ontopoi/MobileDiscos">
        <rdfs:subClassOf rdf:resource="https://www.theworldavatar.com/kg/ontopoi/SportAndEntertainmentSupportServices"/>
        <rdfs:comment>Mobile discos is a subcategory of sport and entertainment support services</rdfs:comment>
        <rdfs:isDefinedBy rdf:resource="https://www.theworldavatar.com/kg/ontopoi"/>
        <rdfs:label>Mobile discos</rdfs:label>
    </owl:Class>
    


    <!-- https://www.theworldavatar.com/kg/ontopoi/ModelVillages -->


    <owl:Class rdf:about="https://www.theworldavatar.com/kg/ontopoi/ModelVillages">
        <rdfs:subClassOf rdf:resource="https://www.theworldavatar.com/kg/ontopoi/Tourism"/>
        <rdfs:comment>Model villages is a subcategory of tourism</rdfs:comment>
        <rdfs:isDefinedBy rdf:resource="https://www.theworldavatar.com/kg/ontopoi"/>
        <rdfs:label>Model villages</rdfs:label>
    </owl:Class>
    


    <!-- https://www.theworldavatar.com/kg/ontopoi/ModellingAndTheatricalAgencies -->


    <owl:Class rdf:about="https://www.theworldavatar.com/kg/ontopoi/ModellingAndTheatricalAgencies">
        <rdfs:subClassOf rdf:resource="https://www.theworldavatar.com/kg/ontopoi/EmploymentAndCareerAgencies"/>
        <rdfs:comment>Modelling and theatrical agencies is a subcategory of employment and career agencies</rdfs:comment>
        <rdfs:isDefinedBy rdf:resource="https://www.theworldavatar.com/kg/ontopoi"/>
        <rdfs:label>Modelling and theatrical agencies</rdfs:label>
    </owl:Class>
    


    <!-- https://www.theworldavatar.com/kg/ontopoi/MooringsAndUnloadingFacilities -->


    <owl:Class rdf:about="https://www.theworldavatar.com/kg/ontopoi/MooringsAndUnloadingFacilities">
        <rdfs:subClassOf rdf:resource="https://www.theworldavatar.com/kg/ontopoi/Water"/>
        <rdfs:comment>Moorings and unloading facilities is a subcategory of water</rdfs:comment>
        <rdfs:isDefinedBy rdf:resource="https://www.theworldavatar.com/kg/ontopoi"/>
        <rdfs:label>Moorings and unloading facilities</rdfs:label>
    </owl:Class>
    


    <!-- https://www.theworldavatar.com/kg/ontopoi/MortgageAndFinancialLenders -->


    <owl:Class rdf:about="https://www.theworldavatar.com/kg/ontopoi/MortgageAndFinancialLenders">
        <rdfs:subClassOf rdf:resource="https://www.theworldavatar.com/kg/ontopoi/LegalAndFinancial"/>
        <rdfs:comment>Mortgage and financial lenders is a subcategory of legal and financial</rdfs:comment>
        <rdfs:isDefinedBy rdf:resource="https://www.theworldavatar.com/kg/ontopoi"/>
        <rdfs:label>Mortgage and financial lenders</rdfs:label>
    </owl:Class>
    


    <!-- https://www.theworldavatar.com/kg/ontopoi/Motoring -->


    <owl:Class rdf:about="https://www.theworldavatar.com/kg/ontopoi/Motoring">
        <rdfs:subClassOf rdf:resource="https://www.theworldavatar.com/kg/ontopoi/Retail"/>
        <rdfs:comment>Motoring is a subcategory of retail</rdfs:comment>
        <rdfs:isDefinedBy rdf:resource="https://www.theworldavatar.com/kg/ontopoi"/>
        <rdfs:label>Motoring</rdfs:label>
    </owl:Class>
    


    <!-- https://www.theworldavatar.com/kg/ontopoi/MotoringOrganisations -->


    <owl:Class rdf:about="https://www.theworldavatar.com/kg/ontopoi/MotoringOrganisations">
        <rdfs:subClassOf rdf:resource="https://www.theworldavatar.com/kg/ontopoi/PersonalAndConsumerAndOtherServices"/>
        <rdfs:comment>Motoring organisations is a subcategory of personal, consumer and other services</rdfs:comment>
        <rdfs:isDefinedBy rdf:resource="https://www.theworldavatar.com/kg/ontopoi"/>
        <rdfs:label>Motoring organisations</rdfs:label>
    </owl:Class>
    


    <!-- https://www.theworldavatar.com/kg/ontopoi/MotorsportServices -->


    <owl:Class rdf:about="https://www.theworldavatar.com/kg/ontopoi/MotorsportServices">
        <rdfs:subClassOf rdf:resource="https://www.theworldavatar.com/kg/ontopoi/SportAndEntertainmentSupportServices"/>
        <rdfs:comment>Motorsport services is a subcategory of sport and entertainment support services</rdfs:comment>
        <rdfs:isDefinedBy rdf:resource="https://www.theworldavatar.com/kg/ontopoi"/>
        <rdfs:label>Motorsport services</rdfs:label>
    </owl:Class>
    


    <!-- https://www.theworldavatar.com/kg/ontopoi/MotorsportVenues -->


    <owl:Class rdf:about="https://www.theworldavatar.com/kg/ontopoi/MotorsportVenues">
        <rdfs:subClassOf rdf:resource="https://www.theworldavatar.com/kg/ontopoi/SportsComplex"/>
        <rdfs:comment>Motorsport venues is a subcategory of sports complex</rdfs:comment>
        <rdfs:isDefinedBy rdf:resource="https://www.theworldavatar.com/kg/ontopoi"/>
        <rdfs:label>Motorsport venues</rdfs:label>
    </owl:Class>
    


    <!-- https://www.theworldavatar.com/kg/ontopoi/MotorwayServiceStations -->


    <owl:Class rdf:about="https://www.theworldavatar.com/kg/ontopoi/MotorwayServiceStations">
        <rdfs:subClassOf rdf:resource="https://www.theworldavatar.com/kg/ontopoi/RoadAndRail"/>
        <rdfs:comment>Motorway service stations is a subcategory of road and rail</rdfs:comment>
        <rdfs:isDefinedBy rdf:resource="https://www.theworldavatar.com/kg/ontopoi"/>
        <rdfs:label>Motorway service stations</rdfs:label>
    </owl:Class>
    


    <!-- https://www.theworldavatar.com/kg/ontopoi/MouldsAndDiesAndCastings -->


    <owl:Class rdf:about="https://www.theworldavatar.com/kg/ontopoi/MouldsAndDiesAndCastings">
        <rdfs:subClassOf rdf:resource="https://www.theworldavatar.com/kg/ontopoi/IndustrialProducts"/>
        <rdfs:comment>Moulds, dies and castings is a subcategory of industrial products</rdfs:comment>
        <rdfs:isDefinedBy rdf:resource="https://www.theworldavatar.com/kg/ontopoi"/>
        <rdfs:label>Moulds, dies and castings</rdfs:label>
    </owl:Class>
    


    <!-- https://www.theworldavatar.com/kg/ontopoi/MunicipalParksAndGardens -->


    <owl:Class rdf:about="https://www.theworldavatar.com/kg/ontopoi/MunicipalParksAndGardens">
        <rdfs:subClassOf rdf:resource="https://www.theworldavatar.com/kg/ontopoi/Recreational"/>
        <rdfs:comment>Municipal parks and gardens is a subcategory of recreational</rdfs:comment>
        <rdfs:isDefinedBy rdf:resource="https://www.theworldavatar.com/kg/ontopoi"/>
        <rdfs:label>Municipal Parks and Gardens</rdfs:label>
    </owl:Class>
    


    <!-- https://www.theworldavatar.com/kg/ontopoi/Museums -->


    <owl:Class rdf:about="https://www.theworldavatar.com/kg/ontopoi/Museums">
        <rdfs:subClassOf rdf:resource="https://www.theworldavatar.com/kg/ontopoi/HistoricalAndCultural"/>
        <rdfs:comment>Museums is a subcategory of historical and cultural</rdfs:comment>
        <rdfs:isDefinedBy rdf:resource="https://www.theworldavatar.com/kg/ontopoi"/>
        <rdfs:label>Museums</rdfs:label>
    </owl:Class>
    


    <!-- https://www.theworldavatar.com/kg/ontopoi/MusicAndVideo -->


    <owl:Class rdf:about="https://www.theworldavatar.com/kg/ontopoi/MusicAndVideo">
        <rdfs:subClassOf rdf:resource="https://www.theworldavatar.com/kg/ontopoi/HouseholdAndOfficeAndLeisureAndGarden"/>
        <rdfs:comment>Music and video is a subcategory of household, office, leisure and garden</rdfs:comment>
        <rdfs:isDefinedBy rdf:resource="https://www.theworldavatar.com/kg/ontopoi"/>
        <rdfs:label>Music and video</rdfs:label>
    </owl:Class>
    


    <!-- https://www.theworldavatar.com/kg/ontopoi/MusicTeachersAndSchools -->


    <owl:Class rdf:about="https://www.theworldavatar.com/kg/ontopoi/MusicTeachersAndSchools">
        <rdfs:subClassOf rdf:resource="https://www.theworldavatar.com/kg/ontopoi/RecreationalAndVocationalEducation"/>
        <rdfs:comment>Music teachers and schools is a subcategory of recreational and vocational education</rdfs:comment>
        <rdfs:isDefinedBy rdf:resource="https://www.theworldavatar.com/kg/ontopoi"/>
        <rdfs:label>Music teachers and schools</rdfs:label>
    </owl:Class>
    


    <!-- https://www.theworldavatar.com/kg/ontopoi/MusicalInstruments -->


    <owl:Class rdf:about="https://www.theworldavatar.com/kg/ontopoi/MusicalInstruments">
        <rdfs:subClassOf rdf:resource="https://www.theworldavatar.com/kg/ontopoi/ConsumerProducts"/>
        <rdfs:subClassOf rdf:resource="https://www.theworldavatar.com/kg/ontopoi/HouseholdAndOfficeAndLeisureAndGarden"/>
        <rdfs:comment>Musical instruments is a subcategory of consumer products</rdfs:comment>
        <rdfs:comment>Musical instruments is a subcategory of household, office, leisure and garden</rdfs:comment>
        <rdfs:isDefinedBy rdf:resource="https://www.theworldavatar.com/kg/ontopoi"/>
        <rdfs:label>Musical instruments</rdfs:label>
    </owl:Class>
    


    <!-- https://www.theworldavatar.com/kg/ontopoi/MusiciansAndOrchestrasAndComposers -->


    <owl:Class rdf:about="https://www.theworldavatar.com/kg/ontopoi/MusiciansAndOrchestrasAndComposers">
        <rdfs:subClassOf rdf:resource="https://www.theworldavatar.com/kg/ontopoi/PersonalAndConsumerAndOtherServices"/>
        <rdfs:comment>Musicians, orchestras and composers is a subcategory of personal, consumer and other services</rdfs:comment>
        <rdfs:isDefinedBy rdf:resource="https://www.theworldavatar.com/kg/ontopoi"/>
        <rdfs:label>Musicians, orchestras and composers</rdfs:label>
    </owl:Class>
    


    <!-- https://www.theworldavatar.com/kg/ontopoi/NewVehicles -->


    <owl:Class rdf:about="https://www.theworldavatar.com/kg/ontopoi/NewVehicles">
        <rdfs:subClassOf rdf:resource="https://www.theworldavatar.com/kg/ontopoi/Motoring"/>
        <rdfs:comment>New vehicles is a subcategory of motoring</rdfs:comment>
        <rdfs:isDefinedBy rdf:resource="https://www.theworldavatar.com/kg/ontopoi"/>
        <rdfs:label>New vehicles</rdfs:label>
    </owl:Class>
    


    <!-- https://www.theworldavatar.com/kg/ontopoi/Nightclubs -->


    <owl:Class rdf:about="https://www.theworldavatar.com/kg/ontopoi/Nightclubs">
        <rdfs:subClassOf rdf:resource="https://www.theworldavatar.com/kg/ontopoi/VenuesAndStageAndScreen"/>
        <rdfs:comment>Nightclubs is a subcategory of venues, stage and screen</rdfs:comment>
        <rdfs:isDefinedBy rdf:resource="https://www.theworldavatar.com/kg/ontopoi"/>
        <rdfs:label>Nightclubs</rdfs:label>
    </owl:Class>
    


    <!-- https://www.theworldavatar.com/kg/ontopoi/Non-AlcoholicDrinks -->


    <owl:Class rdf:about="https://www.theworldavatar.com/kg/ontopoi/Non-AlcoholicDrinks">
        <rdfs:subClassOf rdf:resource="https://www.theworldavatar.com/kg/ontopoi/Foodstuffs"/>
        <rdfs:comment>Non-alcoholic drinks is a subcategory of foodstuffs</rdfs:comment>
        <rdfs:isDefinedBy rdf:resource="https://www.theworldavatar.com/kg/ontopoi"/>
        <rdfs:label>Non-alcoholic drinks</rdfs:label>
    </owl:Class>
    


    <!-- https://www.theworldavatar.com/kg/ontopoi/NurserySchoolsAndPre-AndAfter-SchoolCare -->


    <owl:Class rdf:about="https://www.theworldavatar.com/kg/ontopoi/NurserySchoolsAndPre-AndAfter-SchoolCare">
        <rdfs:subClassOf rdf:resource="https://www.theworldavatar.com/kg/ontopoi/RecreationalAndVocationalEducation"/>
        <rdfs:comment>Nursery schools and pre- and after-school care is a subcategory of recreational and vocational education</rdfs:comment>
        <rdfs:isDefinedBy rdf:resource="https://www.theworldavatar.com/kg/ontopoi"/>
        <rdfs:label>Nursery schools and pre- and after-school care</rdfs:label>
    </owl:Class>
    


    <!-- https://www.theworldavatar.com/kg/ontopoi/NursingAgencies -->


    <owl:Class rdf:about="https://www.theworldavatar.com/kg/ontopoi/NursingAgencies">
        <rdfs:subClassOf rdf:resource="https://www.theworldavatar.com/kg/ontopoi/EmploymentAndCareerAgencies"/>
        <rdfs:comment>Nursing agencies is a subcategory of employment and career agencies</rdfs:comment>
        <rdfs:isDefinedBy rdf:resource="https://www.theworldavatar.com/kg/ontopoi"/>
        <rdfs:label>Nursing agencies</rdfs:label>
    </owl:Class>
    


    <!-- https://www.theworldavatar.com/kg/ontopoi/NursingAndResidentialCareHomes -->


    <owl:Class rdf:about="https://www.theworldavatar.com/kg/ontopoi/NursingAndResidentialCareHomes">
        <rdfs:subClassOf rdf:resource="https://www.theworldavatar.com/kg/ontopoi/HealthPractitionersAndEstablishments"/>
        <rdfs:comment>Nursing and residential care homes is a subcategory of health practitioners and establishments</rdfs:comment>
        <rdfs:isDefinedBy rdf:resource="https://www.theworldavatar.com/kg/ontopoi"/>
        <rdfs:label>Nursing and residential care homes</rdfs:label>
    </owl:Class>
    


    <!-- https://www.theworldavatar.com/kg/ontopoi/OastHouses -->


    <owl:Class rdf:about="https://www.theworldavatar.com/kg/ontopoi/OastHouses">
        <rdfs:subClassOf rdf:resource="https://www.theworldavatar.com/kg/ontopoi/IndustrialFeatures"/>
        <rdfs:comment>Oast houses is a subcategory of industrial features</rdfs:comment>
        <rdfs:isDefinedBy rdf:resource="https://www.theworldavatar.com/kg/ontopoi"/>
        <rdfs:label>Oast houses</rdfs:label>
    </owl:Class>
    


    <!-- https://www.theworldavatar.com/kg/ontopoi/OfficeAndShopEquipment -->


    <owl:Class rdf:about="https://www.theworldavatar.com/kg/ontopoi/OfficeAndShopEquipment">
        <rdfs:subClassOf rdf:resource="https://www.theworldavatar.com/kg/ontopoi/IndustrialProducts"/>
        <rdfs:comment>Office and shop equipment is a subcategory of industrial products</rdfs:comment>
        <rdfs:isDefinedBy rdf:resource="https://www.theworldavatar.com/kg/ontopoi"/>
        <rdfs:label>Office and shop equipment</rdfs:label>
    </owl:Class>
    


    <!-- https://www.theworldavatar.com/kg/ontopoi/OfficeServices -->


    <owl:Class rdf:about="https://www.theworldavatar.com/kg/ontopoi/OfficeServices">
        <rdfs:subClassOf rdf:resource="https://www.theworldavatar.com/kg/ontopoi/ContractServices"/>
        <rdfs:comment>Office services is a subcategory of contract services</rdfs:comment>
        <rdfs:isDefinedBy rdf:resource="https://www.theworldavatar.com/kg/ontopoi"/>
        <rdfs:label>Office services</rdfs:label>
    </owl:Class>
    


    <!-- https://www.theworldavatar.com/kg/ontopoi/OilAndGasExtractionAndRefineryAndProductManufacture -->


    <owl:Class rdf:about="https://www.theworldavatar.com/kg/ontopoi/OilAndGasExtractionAndRefineryAndProductManufacture">
        <rdfs:subClassOf rdf:resource="https://www.theworldavatar.com/kg/ontopoi/ExtractiveIndustries"/>
        <rdfs:comment>Oil and gas extraction, refinery and product manufacture is a subcategory of extractive industries</rdfs:comment>
        <rdfs:isDefinedBy rdf:resource="https://www.theworldavatar.com/kg/ontopoi"/>
        <rdfs:label>Oil and gas extraction, refinery and product manufacture</rdfs:label>
    </owl:Class>
    


    <!-- https://www.theworldavatar.com/kg/ontopoi/OptometristsAndOpticians -->


    <owl:Class rdf:about="https://www.theworldavatar.com/kg/ontopoi/OptometristsAndOpticians">
        <rdfs:subClassOf rdf:resource="https://www.theworldavatar.com/kg/ontopoi/HealthPractitionersAndEstablishments"/>
        <rdfs:comment>Optometrists and opticians is a subcategory of health practitioners and establishments</rdfs:comment>
        <rdfs:isDefinedBy rdf:resource="https://www.theworldavatar.com/kg/ontopoi"/>
        <rdfs:label>Optometrists and opticians</rdfs:label>
    </owl:Class>
    


    <!-- https://www.theworldavatar.com/kg/ontopoi/OreMining -->


    <owl:Class rdf:about="https://www.theworldavatar.com/kg/ontopoi/OreMining">
        <rdfs:subClassOf rdf:resource="https://www.theworldavatar.com/kg/ontopoi/ExtractiveIndustries"/>
        <rdfs:comment>Ore mining is a subcategory of extractive industries</rdfs:comment>
        <rdfs:isDefinedBy rdf:resource="https://www.theworldavatar.com/kg/ontopoi"/>
        <rdfs:label>Ore mining</rdfs:label>
    </owl:Class>
    


    <!-- https://www.theworldavatar.com/kg/ontopoi/OrganicAndHealthAndGourmetAndKosherFoods -->


    <owl:Class rdf:about="https://www.theworldavatar.com/kg/ontopoi/OrganicAndHealthAndGourmetAndKosherFoods">
        <rdfs:subClassOf rdf:resource="https://www.theworldavatar.com/kg/ontopoi/FoodAndDrinkAndMultiItemRetail"/>
        <rdfs:comment>Organic, health, gourmet and kosher foods is a subcategory of food, drink and multi item retail</rdfs:comment>
        <rdfs:isDefinedBy rdf:resource="https://www.theworldavatar.com/kg/ontopoi"/>
        <rdfs:label>Organic, health, gourmet and kosher foods</rdfs:label>
    </owl:Class>
    


    <!-- https://www.theworldavatar.com/kg/ontopoi/Organisations -->


    <owl:Class rdf:about="https://www.theworldavatar.com/kg/ontopoi/Organisations">
        <rdfs:subClassOf rdf:resource="https://www.theworldavatar.com/kg/ontopoi/PublicInfrastructure"/>
        <rdfs:comment>Organisations is a subcategory of public infrastructure</rdfs:comment>
        <rdfs:isDefinedBy rdf:resource="https://www.theworldavatar.com/kg/ontopoi"/>
        <rdfs:label>Organisations</rdfs:label>
    </owl:Class>
    


    <!-- https://www.theworldavatar.com/kg/ontopoi/OutdoorPursuitOrganisersAndEquipment -->


    <owl:Class rdf:about="https://www.theworldavatar.com/kg/ontopoi/OutdoorPursuitOrganisersAndEquipment">
        <rdfs:subClassOf rdf:resource="https://www.theworldavatar.com/kg/ontopoi/OutdoorPursuits"/>
        <rdfs:comment>Outdoor pursuit organisers and equipment is a subcategory of outdoor pursuits</rdfs:comment>
        <rdfs:isDefinedBy rdf:resource="https://www.theworldavatar.com/kg/ontopoi"/>
        <rdfs:label>Outdoor pursuit organisers and equipment</rdfs:label>
    </owl:Class>
    


    <!-- https://www.theworldavatar.com/kg/ontopoi/OutdoorPursuits -->


    <owl:Class rdf:about="https://www.theworldavatar.com/kg/ontopoi/OutdoorPursuits">
        <rdfs:subClassOf rdf:resource="https://www.theworldavatar.com/kg/ontopoi/SportAndEntertainment"/>
        <rdfs:comment>Outdoor pursuits is a subcategory of sport and entertainment</rdfs:comment>
        <rdfs:isDefinedBy rdf:resource="https://www.theworldavatar.com/kg/ontopoi"/>
        <rdfs:label>Outdoor pursuits</rdfs:label>
    </owl:Class>
    


    <!-- https://www.theworldavatar.com/kg/ontopoi/OvensAndFurnaces -->


    <owl:Class rdf:about="https://www.theworldavatar.com/kg/ontopoi/OvensAndFurnaces">
        <rdfs:subClassOf rdf:resource="https://www.theworldavatar.com/kg/ontopoi/IndustrialProducts"/>
        <rdfs:comment>Ovens and furnaces is a subcategory of industrial products</rdfs:comment>
        <rdfs:isDefinedBy rdf:resource="https://www.theworldavatar.com/kg/ontopoi"/>
        <rdfs:label>Ovens and furnaces</rdfs:label>
    </owl:Class>
    


    <!-- https://www.theworldavatar.com/kg/ontopoi/Packaging -->


    <owl:Class rdf:about="https://www.theworldavatar.com/kg/ontopoi/Packaging">
        <rdfs:subClassOf rdf:resource="https://www.theworldavatar.com/kg/ontopoi/IndustrialProducts"/>
        <rdfs:comment>Packaging is a subcategory of industrial products</rdfs:comment>
        <rdfs:isDefinedBy rdf:resource="https://www.theworldavatar.com/kg/ontopoi"/>
        <rdfs:label>Packaging</rdfs:label>
    </owl:Class>
    


    <!-- https://www.theworldavatar.com/kg/ontopoi/Packers -->


    <owl:Class rdf:about="https://www.theworldavatar.com/kg/ontopoi/Packers">
        <rdfs:subClassOf rdf:resource="https://www.theworldavatar.com/kg/ontopoi/ContractServices"/>
        <rdfs:comment>Packers is a subcategory of contract services</rdfs:comment>
        <rdfs:isDefinedBy rdf:resource="https://www.theworldavatar.com/kg/ontopoi"/>
        <rdfs:label>Packers</rdfs:label>
    </owl:Class>
    


    <!-- https://www.theworldavatar.com/kg/ontopoi/PaintingAndDecoratingServices -->


    <owl:Class rdf:about="https://www.theworldavatar.com/kg/ontopoi/PaintingAndDecoratingServices">
        <rdfs:subClassOf rdf:resource="https://www.theworldavatar.com/kg/ontopoi/ConstructionServices"/>
        <rdfs:comment>Painting and decorating services is a subcategory of construction services</rdfs:comment>
        <rdfs:isDefinedBy rdf:resource="https://www.theworldavatar.com/kg/ontopoi"/>
        <rdfs:label>Painting and decorating services</rdfs:label>
    </owl:Class>
    


    <!-- https://www.theworldavatar.com/kg/ontopoi/PaintsAndVarnishesAndLacquers -->


    <owl:Class rdf:about="https://www.theworldavatar.com/kg/ontopoi/PaintsAndVarnishesAndLacquers">
        <rdfs:subClassOf rdf:resource="https://www.theworldavatar.com/kg/ontopoi/IndustrialProducts"/>
        <rdfs:comment>Paints, varnishes and lacquers is a subcategory of industrial products</rdfs:comment>
        <rdfs:isDefinedBy rdf:resource="https://www.theworldavatar.com/kg/ontopoi"/>
        <rdfs:label>Paints, varnishes and lacquers</rdfs:label>
    </owl:Class>
    


    <!-- https://www.theworldavatar.com/kg/ontopoi/ParachutingAndBungeeJumping -->


    <owl:Class rdf:about="https://www.theworldavatar.com/kg/ontopoi/ParachutingAndBungeeJumping">
        <rdfs:subClassOf rdf:resource="https://www.theworldavatar.com/kg/ontopoi/OutdoorPursuits"/>
        <rdfs:comment>Parachuting and bungee jumping is a subcategory of outdoor pursuits</rdfs:comment>
        <rdfs:isDefinedBy rdf:resource="https://www.theworldavatar.com/kg/ontopoi"/>
        <rdfs:label>Parachuting and bungee jumping</rdfs:label>
    </owl:Class>
    


    <!-- https://www.theworldavatar.com/kg/ontopoi/ParaglidingAndHang-Gliding -->


    <owl:Class rdf:about="https://www.theworldavatar.com/kg/ontopoi/ParaglidingAndHang-Gliding">
        <rdfs:subClassOf rdf:resource="https://www.theworldavatar.com/kg/ontopoi/OutdoorPursuits"/>
        <rdfs:comment>Paragliding and hang-gliding is a subcategory of outdoor pursuits</rdfs:comment>
        <rdfs:isDefinedBy rdf:resource="https://www.theworldavatar.com/kg/ontopoi"/>
        <rdfs:label>Paragliding and hang-gliding</rdfs:label>
    </owl:Class>
    


    <!-- https://www.theworldavatar.com/kg/ontopoi/ParentingAndChildcareServices -->


    <owl:Class rdf:about="https://www.theworldavatar.com/kg/ontopoi/ParentingAndChildcareServices">
        <rdfs:subClassOf rdf:resource="https://www.theworldavatar.com/kg/ontopoi/HealthPractitionersAndEstablishments"/>
        <rdfs:comment>Parenting and childcare services is a subcategory of health practitioners and establishments</rdfs:comment>
        <rdfs:isDefinedBy rdf:resource="https://www.theworldavatar.com/kg/ontopoi"/>
        <rdfs:label>Parenting and childcare services</rdfs:label>
    </owl:Class>
    


    <!-- https://www.theworldavatar.com/kg/ontopoi/Parking -->


    <owl:Class rdf:about="https://www.theworldavatar.com/kg/ontopoi/Parking">
        <rdfs:subClassOf rdf:resource="https://www.theworldavatar.com/kg/ontopoi/RoadAndRail"/>
        <rdfs:comment>Parking is a subcategory of road and rail</rdfs:comment>
        <rdfs:isDefinedBy rdf:resource="https://www.theworldavatar.com/kg/ontopoi"/>
        <rdfs:label>Parking</rdfs:label>
    </owl:Class>
    


    <!-- https://www.theworldavatar.com/kg/ontopoi/PartyGoodsAndNovelties -->


    <owl:Class rdf:about="https://www.theworldavatar.com/kg/ontopoi/PartyGoodsAndNovelties">
        <rdfs:subClassOf rdf:resource="https://www.theworldavatar.com/kg/ontopoi/HouseholdAndOfficeAndLeisureAndGarden"/>
        <rdfs:comment>Party goods and novelties is a subcategory of household, office, leisure and garden</rdfs:comment>
        <rdfs:isDefinedBy rdf:resource="https://www.theworldavatar.com/kg/ontopoi"/>
        <rdfs:label>Party goods and novelties</rdfs:label>
    </owl:Class>
    


    <!-- https://www.theworldavatar.com/kg/ontopoi/PartyOrganisers -->


    <owl:Class rdf:about="https://www.theworldavatar.com/kg/ontopoi/PartyOrganisers">
        <rdfs:subClassOf rdf:resource="https://www.theworldavatar.com/kg/ontopoi/PersonalAndConsumerAndOtherServices"/>
        <rdfs:comment>Party organisers is a subcategory of personal, consumer and other services</rdfs:comment>
        <rdfs:isDefinedBy rdf:resource="https://www.theworldavatar.com/kg/ontopoi"/>
        <rdfs:label>Party organisers</rdfs:label>
    </owl:Class>
    


    <!-- https://www.theworldavatar.com/kg/ontopoi/Pawnbrokers -->


    <owl:Class rdf:about="https://www.theworldavatar.com/kg/ontopoi/Pawnbrokers">
        <rdfs:subClassOf rdf:resource="https://www.theworldavatar.com/kg/ontopoi/LegalAndFinancial"/>
        <rdfs:comment>Pawnbrokers is a subcategory of legal and financial</rdfs:comment>
        <rdfs:isDefinedBy rdf:resource="https://www.theworldavatar.com/kg/ontopoi"/>
        <rdfs:label>Pawnbrokers</rdfs:label>
    </owl:Class>
    


    <!-- https://www.theworldavatar.com/kg/ontopoi/PensionAndFundManagement -->


    <owl:Class rdf:about="https://www.theworldavatar.com/kg/ontopoi/PensionAndFundManagement">
        <rdfs:subClassOf rdf:resource="https://www.theworldavatar.com/kg/ontopoi/LegalAndFinancial"/>
        <rdfs:comment>Pension and fund management is a subcategory of legal and financial</rdfs:comment>
        <rdfs:isDefinedBy rdf:resource="https://www.theworldavatar.com/kg/ontopoi"/>
        <rdfs:label>Pension and fund management</rdfs:label>
    </owl:Class>
    


    <!-- https://www.theworldavatar.com/kg/ontopoi/PersonalAndConsumerAndOtherServices -->


    <owl:Class rdf:about="https://www.theworldavatar.com/kg/ontopoi/PersonalAndConsumerAndOtherServices">
        <rdfs:subClassOf rdf:resource="https://www.theworldavatar.com/kg/ontopoi/CommercialServices"/>
        <rdfs:comment>Personal, consumer and other services is a subcategory of commercial services</rdfs:comment>
        <rdfs:isDefinedBy rdf:resource="https://www.theworldavatar.com/kg/ontopoi"/>
        <rdfs:label>Personal, consumer and other services</rdfs:label>
    </owl:Class>
    


    <!-- https://www.theworldavatar.com/kg/ontopoi/Personalisation -->


    <owl:Class rdf:about="https://www.theworldavatar.com/kg/ontopoi/Personalisation">
        <rdfs:subClassOf rdf:resource="https://www.theworldavatar.com/kg/ontopoi/PersonalAndConsumerAndOtherServices"/>
        <rdfs:comment>Personalisation is a subcategory of personal, consumer and other services</rdfs:comment>
        <rdfs:isDefinedBy rdf:resource="https://www.theworldavatar.com/kg/ontopoi"/>
        <rdfs:label>Personalisation</rdfs:label>
    </owl:Class>
    


    <!-- https://www.theworldavatar.com/kg/ontopoi/PestAndVerminControl -->


    <owl:Class rdf:about="https://www.theworldavatar.com/kg/ontopoi/PestAndVerminControl">
        <rdfs:subClassOf rdf:resource="https://www.theworldavatar.com/kg/ontopoi/ContractServices"/>
        <rdfs:comment>Pest and vermin control is a subcategory of contract services</rdfs:comment>
        <rdfs:isDefinedBy rdf:resource="https://www.theworldavatar.com/kg/ontopoi"/>
        <rdfs:label>Pest and vermin control</rdfs:label>
    </owl:Class>
    


    <!-- https://www.theworldavatar.com/kg/ontopoi/Pesticides -->


    <owl:Class rdf:about="https://www.theworldavatar.com/kg/ontopoi/Pesticides">
        <rdfs:subClassOf rdf:resource="https://www.theworldavatar.com/kg/ontopoi/IndustrialProducts"/>
        <rdfs:comment>Pesticides is a subcategory of industrial products</rdfs:comment>
        <rdfs:isDefinedBy rdf:resource="https://www.theworldavatar.com/kg/ontopoi"/>
        <rdfs:label>Pesticides</rdfs:label>
    </owl:Class>
    


    <!-- https://www.theworldavatar.com/kg/ontopoi/PetCemeteriesAndCrematoria -->


    <owl:Class rdf:about="https://www.theworldavatar.com/kg/ontopoi/PetCemeteriesAndCrematoria">
        <rdfs:subClassOf rdf:resource="https://www.theworldavatar.com/kg/ontopoi/AnimalWelfare"/>
        <rdfs:comment>Pet cemeteries and crematoria is a subcategory of animal welfare</rdfs:comment>
        <rdfs:isDefinedBy rdf:resource="https://www.theworldavatar.com/kg/ontopoi"/>
        <rdfs:label>Pet cemeteries and crematoria</rdfs:label>
    </owl:Class>
    


    <!-- https://www.theworldavatar.com/kg/ontopoi/PetrolAndFuelStations -->


    <owl:Class rdf:about="https://www.theworldavatar.com/kg/ontopoi/PetrolAndFuelStations">
        <rdfs:subClassOf rdf:resource="https://www.theworldavatar.com/kg/ontopoi/RoadAndRail"/>
        <rdfs:comment>Petrol and fuel stations is a subcategory of road and rail</rdfs:comment>
        <rdfs:isDefinedBy rdf:resource="https://www.theworldavatar.com/kg/ontopoi"/>
        <rdfs:label>Petrol and fuel stations</rdfs:label>
    </owl:Class>
    


    <!-- https://www.theworldavatar.com/kg/ontopoi/PetsAndSuppliesAndServices -->


    <owl:Class rdf:about="https://www.theworldavatar.com/kg/ontopoi/PetsAndSuppliesAndServices">
        <rdfs:subClassOf rdf:resource="https://www.theworldavatar.com/kg/ontopoi/HouseholdAndOfficeAndLeisureAndGarden"/>
        <rdfs:comment>Pets, supplies and services is a subcategory of household, office, leisure and garden</rdfs:comment>
        <rdfs:isDefinedBy rdf:resource="https://www.theworldavatar.com/kg/ontopoi"/>
        <rdfs:label>Pets, supplies and services</rdfs:label>
    </owl:Class>
    


    <!-- https://www.theworldavatar.com/kg/ontopoi/PhotographicAndOpticalEquipment -->


    <owl:Class rdf:about="https://www.theworldavatar.com/kg/ontopoi/PhotographicAndOpticalEquipment">
        <rdfs:subClassOf rdf:resource="https://www.theworldavatar.com/kg/ontopoi/ConsumerProducts"/>
        <rdfs:subClassOf rdf:resource="https://www.theworldavatar.com/kg/ontopoi/HouseholdAndOfficeAndLeisureAndGarden"/>
        <rdfs:comment>Photographic and optical equipment is a subcategory of consumer products</rdfs:comment>
        <rdfs:comment>Photographic and optical equipment is a subcategory of household, office, leisure and garden</rdfs:comment>
        <rdfs:isDefinedBy rdf:resource="https://www.theworldavatar.com/kg/ontopoi"/>
        <rdfs:label>Photographic and optical equipment</rdfs:label>
    </owl:Class>
    


    <!-- https://www.theworldavatar.com/kg/ontopoi/PhotographicServices -->


    <owl:Class rdf:about="https://www.theworldavatar.com/kg/ontopoi/PhotographicServices">
        <rdfs:subClassOf rdf:resource="https://www.theworldavatar.com/kg/ontopoi/PersonalAndConsumerAndOtherServices"/>
        <rdfs:comment>Photographic services is a subcategory of personal, consumer and other services</rdfs:comment>
        <rdfs:isDefinedBy rdf:resource="https://www.theworldavatar.com/kg/ontopoi"/>
        <rdfs:label>Photographic services</rdfs:label>
    </owl:Class>
    


    <!-- https://www.theworldavatar.com/kg/ontopoi/PhysicalTherapy -->


    <owl:Class rdf:about="https://www.theworldavatar.com/kg/ontopoi/PhysicalTherapy">
        <rdfs:subClassOf rdf:resource="https://www.theworldavatar.com/kg/ontopoi/HealthPractitionersAndEstablishments"/>
        <rdfs:comment>Physical therapy is a subcategory of health practitioners and establishments</rdfs:comment>
        <rdfs:isDefinedBy rdf:resource="https://www.theworldavatar.com/kg/ontopoi"/>
        <rdfs:label>Physical therapy</rdfs:label>
    </owl:Class>
    


    <!-- https://www.theworldavatar.com/kg/ontopoi/PicnicAreas -->


    <owl:Class rdf:about="https://www.theworldavatar.com/kg/ontopoi/PicnicAreas">
        <rdfs:subClassOf rdf:resource="https://www.theworldavatar.com/kg/ontopoi/Recreational"/>
        <rdfs:comment>Picnic areas is a subcategory of recreational</rdfs:comment>
        <rdfs:isDefinedBy rdf:resource="https://www.theworldavatar.com/kg/ontopoi"/>
        <rdfs:label>Picnic areas</rdfs:label>
    </owl:Class>
    


    <!-- https://www.theworldavatar.com/kg/ontopoi/Pipelines -->


    <owl:Class rdf:about="https://www.theworldavatar.com/kg/ontopoi/Pipelines">
        <rdfs:subClassOf rdf:resource="https://www.theworldavatar.com/kg/ontopoi/IndustrialFeatures"/>
        <rdfs:comment>Pipelines is a subcategory of industrial features</rdfs:comment>
        <rdfs:isDefinedBy rdf:resource="https://www.theworldavatar.com/kg/ontopoi"/>
        <rdfs:label>Pipelines</rdfs:label>
    </owl:Class>
    


    <!-- https://www.theworldavatar.com/kg/ontopoi/PlacesOfWorship -->


    <owl:Class rdf:about="https://www.theworldavatar.com/kg/ontopoi/PlacesOfWorship">
        <rdfs:subClassOf rdf:resource="https://www.theworldavatar.com/kg/ontopoi/InfrastructureAndFacilities"/>
        <rdfs:comment>Places of worship is a subcategory of infrastructure and facilities</rdfs:comment>
        <rdfs:isDefinedBy rdf:resource="https://www.theworldavatar.com/kg/ontopoi"/>
        <rdfs:label>Places of worship</rdfs:label>
    </owl:Class>
    


    <!-- https://www.theworldavatar.com/kg/ontopoi/Plasterers -->


    <owl:Class rdf:about="https://www.theworldavatar.com/kg/ontopoi/Plasterers">
        <rdfs:subClassOf rdf:resource="https://www.theworldavatar.com/kg/ontopoi/ConstructionServices"/>
        <rdfs:comment>Plasterers is a subcategory of construction services</rdfs:comment>
        <rdfs:isDefinedBy rdf:resource="https://www.theworldavatar.com/kg/ontopoi"/>
        <rdfs:label>Plasterers</rdfs:label>
    </owl:Class>
    


    <!-- https://www.theworldavatar.com/kg/ontopoi/PlateMakersAndPrintFinishersAndTypesetters -->


    <owl:Class rdf:about="https://www.theworldavatar.com/kg/ontopoi/PlateMakersAndPrintFinishersAndTypesetters">
        <rdfs:subClassOf rdf:resource="https://www.theworldavatar.com/kg/ontopoi/ItAndAdvertisingAndMarketingAndMediaServiceS"/>
        <rdfs:comment>Plate makers, print finishers and typesetters is a subcategory of it, advertising, marketing and media service s</rdfs:comment>
        <rdfs:isDefinedBy rdf:resource="https://www.theworldavatar.com/kg/ontopoi"/>
        <rdfs:label>Plate makers, print finishers and typesetters</rdfs:label>
    </owl:Class>
    


    <!-- https://www.theworldavatar.com/kg/ontopoi/Playgrounds -->


    <owl:Class rdf:about="https://www.theworldavatar.com/kg/ontopoi/Playgrounds">
        <rdfs:subClassOf rdf:resource="https://www.theworldavatar.com/kg/ontopoi/Recreational"/>
        <rdfs:comment>Playgrounds is a subcategory of recreational</rdfs:comment>
        <rdfs:isDefinedBy rdf:resource="https://www.theworldavatar.com/kg/ontopoi"/>
        <rdfs:label>Playgrounds</rdfs:label>
    </owl:Class>
    


    <!-- https://www.theworldavatar.com/kg/ontopoi/PlumbingAndHeatingServices -->


    <owl:Class rdf:about="https://www.theworldavatar.com/kg/ontopoi/PlumbingAndHeatingServices">
        <rdfs:subClassOf rdf:resource="https://www.theworldavatar.com/kg/ontopoi/ConstructionServices"/>
        <rdfs:comment>Plumbing and heating services is a subcategory of construction services</rdfs:comment>
        <rdfs:isDefinedBy rdf:resource="https://www.theworldavatar.com/kg/ontopoi"/>
        <rdfs:label>Plumbing and heating services</rdfs:label>
    </owl:Class>
    


    <!-- https://www.theworldavatar.com/kg/ontopoi/PneumaticEngineers -->


    <owl:Class rdf:about="https://www.theworldavatar.com/kg/ontopoi/PneumaticEngineers">
        <rdfs:subClassOf rdf:resource="https://www.theworldavatar.com/kg/ontopoi/EngineeringServices"/>
        <rdfs:comment>Pneumatic engineers is a subcategory of engineering services</rdfs:comment>
        <rdfs:isDefinedBy rdf:resource="https://www.theworldavatar.com/kg/ontopoi"/>
        <rdfs:label>Pneumatic engineers</rdfs:label>
    </owl:Class>
    


    <!-- https://www.theworldavatar.com/kg/ontopoi/PointOfInterest -->


    <owl:Class rdf:about="https://www.theworldavatar.com/kg/ontopoi/PointOfInterest">
        <rdfs:comment>A specific location or place of significance in a geographical context</rdfs:comment>
        <rdfs:isDefinedBy rdf:resource="https://www.theworldavatar.com/kg/ontopoi"/>
        <rdfs:label>Point Of Interest</rdfs:label>
    </owl:Class>
    


    <!-- https://www.theworldavatar.com/kg/ontopoi/PointOfInterestEnd -->


    <owl:Class rdf:about="https://www.theworldavatar.com/kg/ontopoi/PointOfInterestEnd">
        <rdfs:subClassOf rdf:resource="http://ies.data.gov.uk/ontology/ies4#BoundingState"/>
        <rdfs:subClassOf>
            <owl:Restriction>
                <owl:onProperty rdf:resource="http://ies.data.gov.uk/ontology/ies4#isEndOf"/>
                <owl:allValuesFrom rdf:resource="https://www.theworldavatar.com/kg/ontopoi/PointOfInterest"/>
            </owl:Restriction>
        </rdfs:subClassOf>
        <rdfs:comment>The date of decommissioning or closure of a point-of-interest entity.</rdfs:comment>
        <rdfs:isDefinedBy rdf:resource="https://www.theworldavatar.com/kg/ontopoi"/>
        <rdfs:label>Point Of Interest End</rdfs:label>
    </owl:Class>
    


    <!-- https://www.theworldavatar.com/kg/ontopoi/PointOfInterestStart -->


    <owl:Class rdf:about="https://www.theworldavatar.com/kg/ontopoi/PointOfInterestStart">
        <rdfs:subClassOf rdf:resource="http://ies.data.gov.uk/ontology/ies4#BoundingState"/>
        <rdfs:subClassOf>
            <owl:Restriction>
                <owl:onProperty rdf:resource="http://ies.data.gov.uk/ontology/ies4#isStartOf"/>
                <owl:allValuesFrom rdf:resource="https://www.theworldavatar.com/kg/ontopoi/PointOfInterest"/>
            </owl:Restriction>
        </rdfs:subClassOf>
        <rdfs:comment>Tthe official date when a point-of-interest entity began operations or was inaugurated.</rdfs:comment>
        <rdfs:isDefinedBy rdf:resource="https://www.theworldavatar.com/kg/ontopoi"/>
        <rdfs:label>Point Of Interest Start</rdfs:label>
    </owl:Class>
    


    <!-- https://www.theworldavatar.com/kg/ontopoi/PoliceStations -->


    <owl:Class rdf:about="https://www.theworldavatar.com/kg/ontopoi/PoliceStations">
        <rdfs:subClassOf rdf:resource="https://www.theworldavatar.com/kg/ontopoi/CentralAndLocalGovernment"/>
        <rdfs:comment>Police stations is a subcategory of central and local government</rdfs:comment>
        <rdfs:isDefinedBy rdf:resource="https://www.theworldavatar.com/kg/ontopoi"/>
        <rdfs:label>Police stations</rdfs:label>
    </owl:Class>
    


    <!-- https://www.theworldavatar.com/kg/ontopoi/PoliticalPartiesAndRelatedOrganisations -->


    <owl:Class rdf:about="https://www.theworldavatar.com/kg/ontopoi/PoliticalPartiesAndRelatedOrganisations">
        <rdfs:subClassOf rdf:resource="https://www.theworldavatar.com/kg/ontopoi/Organisations"/>
        <rdfs:comment>Political parties and related organisations is a subcategory of organisations</rdfs:comment>
        <rdfs:isDefinedBy rdf:resource="https://www.theworldavatar.com/kg/ontopoi"/>
        <rdfs:label>Political parties and related organisations</rdfs:label>
    </owl:Class>
    


    <!-- https://www.theworldavatar.com/kg/ontopoi/PoolAndCourtConstruction -->


    <owl:Class rdf:about="https://www.theworldavatar.com/kg/ontopoi/PoolAndCourtConstruction">
        <rdfs:subClassOf rdf:resource="https://www.theworldavatar.com/kg/ontopoi/ConstructionServices"/>
        <rdfs:comment>Pool and court construction is a subcategory of construction services</rdfs:comment>
        <rdfs:isDefinedBy rdf:resource="https://www.theworldavatar.com/kg/ontopoi"/>
        <rdfs:label>Pool and court construction</rdfs:label>
    </owl:Class>
    


    <!-- https://www.theworldavatar.com/kg/ontopoi/PostOffices -->


    <owl:Class rdf:about="https://www.theworldavatar.com/kg/ontopoi/PostOffices">
        <rdfs:subClassOf rdf:resource="https://www.theworldavatar.com/kg/ontopoi/HouseholdAndOfficeAndLeisureAndGarden"/>
        <rdfs:comment>Post offices is a subcategory of household, office, leisure and garden</rdfs:comment>
        <rdfs:isDefinedBy rdf:resource="https://www.theworldavatar.com/kg/ontopoi"/>
        <rdfs:label>Post offices</rdfs:label>
    </owl:Class>
    


    <!-- https://www.theworldavatar.com/kg/ontopoi/Potteries -->


    <owl:Class rdf:about="https://www.theworldavatar.com/kg/ontopoi/Potteries">
        <rdfs:subClassOf rdf:resource="https://www.theworldavatar.com/kg/ontopoi/HouseholdAndOfficeAndLeisureAndGarden"/>
        <rdfs:comment>Potteries is a subcategory of household, office, leisure and garden</rdfs:comment>
        <rdfs:isDefinedBy rdf:resource="https://www.theworldavatar.com/kg/ontopoi"/>
        <rdfs:label>Potteries</rdfs:label>
    </owl:Class>
    


    <!-- https://www.theworldavatar.com/kg/ontopoi/PoultryFarmingAndEquipmentAndSupplies -->


    <owl:Class rdf:about="https://www.theworldavatar.com/kg/ontopoi/PoultryFarmingAndEquipmentAndSupplies">
        <rdfs:subClassOf rdf:resource="https://www.theworldavatar.com/kg/ontopoi/Farming"/>
        <rdfs:comment>Poultry farming, equipment and supplies is a subcategory of farming</rdfs:comment>
        <rdfs:isDefinedBy rdf:resource="https://www.theworldavatar.com/kg/ontopoi"/>
        <rdfs:label>Poultry farming, equipment and supplies</rdfs:label>
    </owl:Class>
    


    <!-- https://www.theworldavatar.com/kg/ontopoi/PrecisionEngineers -->


    <owl:Class rdf:about="https://www.theworldavatar.com/kg/ontopoi/PrecisionEngineers">
        <rdfs:subClassOf rdf:resource="https://www.theworldavatar.com/kg/ontopoi/EngineeringServices"/>
        <rdfs:comment>Precision engineers is a subcategory of engineering services</rdfs:comment>
        <rdfs:isDefinedBy rdf:resource="https://www.theworldavatar.com/kg/ontopoi"/>
        <rdfs:label>Precision engineers</rdfs:label>
    </owl:Class>
    


    <!-- https://www.theworldavatar.com/kg/ontopoi/PregnancyRelatedServicesAndHelpCentres -->


    <owl:Class rdf:about="https://www.theworldavatar.com/kg/ontopoi/PregnancyRelatedServicesAndHelpCentres">
        <rdfs:subClassOf rdf:resource="https://www.theworldavatar.com/kg/ontopoi/HealthSupportServices"/>
        <rdfs:comment>Pregnancy related services and help centres is a subcategory of health support services</rdfs:comment>
        <rdfs:isDefinedBy rdf:resource="https://www.theworldavatar.com/kg/ontopoi"/>
        <rdfs:label>Pregnancy related services and help centres</rdfs:label>
    </owl:Class>
    


    <!-- https://www.theworldavatar.com/kg/ontopoi/PressAndJournalismServices -->


    <owl:Class rdf:about="https://www.theworldavatar.com/kg/ontopoi/PressAndJournalismServices">
        <rdfs:subClassOf rdf:resource="https://www.theworldavatar.com/kg/ontopoi/ItAndAdvertisingAndMarketingAndMediaServiceS"/>
        <rdfs:comment>Press and journalism services is a subcategory of it, advertising, marketing and media service s</rdfs:comment>
        <rdfs:isDefinedBy rdf:resource="https://www.theworldavatar.com/kg/ontopoi"/>
        <rdfs:label>Press and journalism services</rdfs:label>
    </owl:Class>
    


    <!-- https://www.theworldavatar.com/kg/ontopoi/PrimaryAndSecondaryAndTertiaryEducation -->


    <owl:Class rdf:about="https://www.theworldavatar.com/kg/ontopoi/PrimaryAndSecondaryAndTertiaryEducation">
        <rdfs:subClassOf rdf:resource="https://www.theworldavatar.com/kg/ontopoi/EducationAndHealth"/>
        <rdfs:comment>Primary, secondary and tertiary education is a subcategory of education and health</rdfs:comment>
        <rdfs:isDefinedBy rdf:resource="https://www.theworldavatar.com/kg/ontopoi"/>
        <rdfs:label>Primary, secondary and tertiary education</rdfs:label>
    </owl:Class>
    


    <!-- https://www.theworldavatar.com/kg/ontopoi/Printing-RelatedMachinery -->


    <owl:Class rdf:about="https://www.theworldavatar.com/kg/ontopoi/Printing-RelatedMachinery">
        <rdfs:subClassOf rdf:resource="https://www.theworldavatar.com/kg/ontopoi/IndustrialProducts"/>
        <rdfs:comment>Printing-related machinery is a subcategory of industrial products</rdfs:comment>
        <rdfs:isDefinedBy rdf:resource="https://www.theworldavatar.com/kg/ontopoi"/>
        <rdfs:label>Printing-related machinery</rdfs:label>
    </owl:Class>
    


    <!-- https://www.theworldavatar.com/kg/ontopoi/PrintingAndPhotocopyingServices -->


    <owl:Class rdf:about="https://www.theworldavatar.com/kg/ontopoi/PrintingAndPhotocopyingServices">
        <rdfs:subClassOf rdf:resource="https://www.theworldavatar.com/kg/ontopoi/ItAndAdvertisingAndMarketingAndMediaServiceS"/>
        <rdfs:comment>Printing and photocopying services is a subcategory of it, advertising, marketing and media service s</rdfs:comment>
        <rdfs:isDefinedBy rdf:resource="https://www.theworldavatar.com/kg/ontopoi"/>
        <rdfs:label>Printing and photocopying services</rdfs:label>
    </owl:Class>
    


    <!-- https://www.theworldavatar.com/kg/ontopoi/PrintingOnGarments -->


    <owl:Class rdf:about="https://www.theworldavatar.com/kg/ontopoi/PrintingOnGarments">
        <rdfs:subClassOf rdf:resource="https://www.theworldavatar.com/kg/ontopoi/PersonalAndConsumerAndOtherServices"/>
        <rdfs:comment>Printing on garments is a subcategory of personal, consumer and other services</rdfs:comment>
        <rdfs:isDefinedBy rdf:resource="https://www.theworldavatar.com/kg/ontopoi"/>
        <rdfs:label>Printing on garments</rdfs:label>
    </owl:Class>
    


    <!-- https://www.theworldavatar.com/kg/ontopoi/Prisons -->


    <owl:Class rdf:about="https://www.theworldavatar.com/kg/ontopoi/Prisons">
        <rdfs:subClassOf rdf:resource="https://www.theworldavatar.com/kg/ontopoi/CentralAndLocalGovernment"/>
        <rdfs:comment>Prisons is a subcategory of central and local government</rdfs:comment>
        <rdfs:isDefinedBy rdf:resource="https://www.theworldavatar.com/kg/ontopoi"/>
        <rdfs:label>Prisons</rdfs:label>
    </owl:Class>
    


    <!-- https://www.theworldavatar.com/kg/ontopoi/ProbationOfficesAndPoliceSupportServices -->


    <owl:Class rdf:about="https://www.theworldavatar.com/kg/ontopoi/ProbationOfficesAndPoliceSupportServices">
        <rdfs:subClassOf rdf:resource="https://www.theworldavatar.com/kg/ontopoi/CentralAndLocalGovernment"/>
        <rdfs:comment>Probation offices and police support services is a subcategory of central and local government</rdfs:comment>
        <rdfs:isDefinedBy rdf:resource="https://www.theworldavatar.com/kg/ontopoi"/>
        <rdfs:label>Probation offices and police support services</rdfs:label>
    </owl:Class>
    


    <!-- https://www.theworldavatar.com/kg/ontopoi/PropertyAndDevelopmentServices -->


    <owl:Class rdf:about="https://www.theworldavatar.com/kg/ontopoi/PropertyAndDevelopmentServices">
        <rdfs:subClassOf rdf:resource="https://www.theworldavatar.com/kg/ontopoi/CommercialServices"/>
        <rdfs:comment>Property and development services is a subcategory of commercial services</rdfs:comment>
        <rdfs:isDefinedBy rdf:resource="https://www.theworldavatar.com/kg/ontopoi"/>
        <rdfs:label>Property and development services</rdfs:label>
    </owl:Class>
    


    <!-- https://www.theworldavatar.com/kg/ontopoi/PropertyDevelopmentServices -->


    <owl:Class rdf:about="https://www.theworldavatar.com/kg/ontopoi/PropertyDevelopmentServices">
        <rdfs:subClassOf rdf:resource="https://www.theworldavatar.com/kg/ontopoi/PropertyAndDevelopmentServices"/>
        <rdfs:comment>Property development services is a subcategory of property and development services</rdfs:comment>
        <rdfs:isDefinedBy rdf:resource="https://www.theworldavatar.com/kg/ontopoi"/>
        <rdfs:label>Property development services</rdfs:label>
    </owl:Class>
    


    <!-- https://www.theworldavatar.com/kg/ontopoi/PropertyInformationServices -->


    <owl:Class rdf:about="https://www.theworldavatar.com/kg/ontopoi/PropertyInformationServices">
        <rdfs:subClassOf rdf:resource="https://www.theworldavatar.com/kg/ontopoi/PropertyAndDevelopmentServices"/>
        <rdfs:comment>Property information services is a subcategory of property and development services</rdfs:comment>
        <rdfs:isDefinedBy rdf:resource="https://www.theworldavatar.com/kg/ontopoi"/>
        <rdfs:label>Property information services</rdfs:label>
    </owl:Class>
    


    <!-- https://www.theworldavatar.com/kg/ontopoi/PropertyLetting -->


    <owl:Class rdf:about="https://www.theworldavatar.com/kg/ontopoi/PropertyLetting">
        <rdfs:subClassOf rdf:resource="https://www.theworldavatar.com/kg/ontopoi/PropertyAndDevelopmentServices"/>
        <rdfs:comment>Property letting is a subcategory of property and development services</rdfs:comment>
        <rdfs:isDefinedBy rdf:resource="https://www.theworldavatar.com/kg/ontopoi"/>
        <rdfs:label>Property letting</rdfs:label>
    </owl:Class>
    


    <!-- https://www.theworldavatar.com/kg/ontopoi/PropertySales -->


    <owl:Class rdf:about="https://www.theworldavatar.com/kg/ontopoi/PropertySales">
        <rdfs:subClassOf rdf:resource="https://www.theworldavatar.com/kg/ontopoi/PropertyAndDevelopmentServices"/>
        <rdfs:comment>Property sales is a subcategory of property and development services</rdfs:comment>
        <rdfs:isDefinedBy rdf:resource="https://www.theworldavatar.com/kg/ontopoi"/>
        <rdfs:label>Property sales</rdfs:label>
    </owl:Class>
    


    <!-- https://www.theworldavatar.com/kg/ontopoi/PublicInfrastructure -->


    <owl:Class rdf:about="https://www.theworldavatar.com/kg/ontopoi/PublicInfrastructure">
        <rdfs:subClassOf rdf:resource="https://www.theworldavatar.com/kg/ontopoi/PointOfInterest"/>
        <rdfs:comment>Physical facilities, organisations, governmental entities, and services that are developed, maintained, and operated for the public good</rdfs:comment>
        <rdfs:isDefinedBy rdf:resource="https://www.theworldavatar.com/kg/ontopoi"/>
        <rdfs:label>Public infrastructure</rdfs:label>
    </owl:Class>
    


    <!-- https://www.theworldavatar.com/kg/ontopoi/PublicToilets -->


    <owl:Class rdf:about="https://www.theworldavatar.com/kg/ontopoi/PublicToilets">
        <rdfs:subClassOf rdf:resource="https://www.theworldavatar.com/kg/ontopoi/InfrastructureAndFacilities"/>
        <rdfs:comment>Public toilets is a subcategory of infrastructure and facilities</rdfs:comment>
        <rdfs:isDefinedBy rdf:resource="https://www.theworldavatar.com/kg/ontopoi"/>
        <rdfs:label>Public toilets</rdfs:label>
    </owl:Class>
    


    <!-- https://www.theworldavatar.com/kg/ontopoi/PublicTransportAndStationsAndInfrastructure -->


    <owl:Class rdf:about="https://www.theworldavatar.com/kg/ontopoi/PublicTransportAndStationsAndInfrastructure">
        <rdfs:subClassOf rdf:resource="https://www.theworldavatar.com/kg/ontopoi/Transport"/>
        <rdfs:comment>Public transport, stations and infrastructure is a subcategory of transport</rdfs:comment>
        <rdfs:isDefinedBy rdf:resource="https://www.theworldavatar.com/kg/ontopoi"/>
        <rdfs:label>Public transport, stations and infrastructure</rdfs:label>
    </owl:Class>
    


    <!-- https://www.theworldavatar.com/kg/ontopoi/PublishedGoods -->


    <owl:Class rdf:about="https://www.theworldavatar.com/kg/ontopoi/PublishedGoods">
        <rdfs:subClassOf rdf:resource="https://www.theworldavatar.com/kg/ontopoi/IndustrialProducts"/>
        <rdfs:comment>Published goods is a subcategory of industrial products</rdfs:comment>
        <rdfs:isDefinedBy rdf:resource="https://www.theworldavatar.com/kg/ontopoi"/>
        <rdfs:label>Published goods</rdfs:label>
    </owl:Class>
    


    <!-- https://www.theworldavatar.com/kg/ontopoi/PubsAndBarsAndInns -->


    <owl:Class rdf:about="https://www.theworldavatar.com/kg/ontopoi/PubsAndBarsAndInns">
        <rdfs:subClassOf rdf:resource="https://www.theworldavatar.com/kg/ontopoi/EatingAndDrinking"/>
        <rdfs:comment>Pubs, bars and inns is a subcategory of eating and drinking</rdfs:comment>
        <rdfs:isDefinedBy rdf:resource="https://www.theworldavatar.com/kg/ontopoi"/>
        <rdfs:label>Pubs, bars and inns</rdfs:label>
    </owl:Class>
    


    <!-- https://www.theworldavatar.com/kg/ontopoi/PumpsAndCompressors -->


    <owl:Class rdf:about="https://www.theworldavatar.com/kg/ontopoi/PumpsAndCompressors">
        <rdfs:subClassOf rdf:resource="https://www.theworldavatar.com/kg/ontopoi/IndustrialProducts"/>
        <rdfs:comment>Pumps and compressors is a subcategory of industrial products</rdfs:comment>
        <rdfs:isDefinedBy rdf:resource="https://www.theworldavatar.com/kg/ontopoi"/>
        <rdfs:label>Pumps and compressors</rdfs:label>
    </owl:Class>
    


    <!-- https://www.theworldavatar.com/kg/ontopoi/PupilReferralUnits -->


    <owl:Class rdf:about="https://www.theworldavatar.com/kg/ontopoi/PupilReferralUnits">
        <rdfs:subClassOf rdf:resource="https://www.theworldavatar.com/kg/ontopoi/PrimaryAndSecondaryAndTertiaryEducation"/>
        <rdfs:comment>Pupil referral units is a subcategory of primary, secondary and tertiary education</rdfs:comment>
        <rdfs:isDefinedBy rdf:resource="https://www.theworldavatar.com/kg/ontopoi"/>
        <rdfs:label>Pupil referral units</rdfs:label>
    </owl:Class>
    


    <!-- https://www.theworldavatar.com/kg/ontopoi/RacecoursesAndGreyhoundTracks -->


    <owl:Class rdf:about="https://www.theworldavatar.com/kg/ontopoi/RacecoursesAndGreyhoundTracks">
        <rdfs:subClassOf rdf:resource="https://www.theworldavatar.com/kg/ontopoi/SportsComplex"/>
        <rdfs:comment>Racecourses and greyhound tracks is a subcategory of sports complex</rdfs:comment>
        <rdfs:isDefinedBy rdf:resource="https://www.theworldavatar.com/kg/ontopoi"/>
        <rdfs:label>Racecourses and greyhound tracks</rdfs:label>
    </owl:Class>
    


    <!-- https://www.theworldavatar.com/kg/ontopoi/RadarAndTelecommunicationsEquipment -->


    <owl:Class rdf:about="https://www.theworldavatar.com/kg/ontopoi/RadarAndTelecommunicationsEquipment">
        <rdfs:subClassOf rdf:resource="https://www.theworldavatar.com/kg/ontopoi/IndustrialProducts"/>
        <rdfs:comment>Radar and telecommunications equipment is a subcategory of industrial products</rdfs:comment>
        <rdfs:isDefinedBy rdf:resource="https://www.theworldavatar.com/kg/ontopoi"/>
        <rdfs:label>Radar and telecommunications equipment</rdfs:label>
    </owl:Class>
    


    <!-- https://www.theworldavatar.com/kg/ontopoi/RagMerchants -->


    <owl:Class rdf:about="https://www.theworldavatar.com/kg/ontopoi/RagMerchants">
        <rdfs:subClassOf rdf:resource="https://www.theworldavatar.com/kg/ontopoi/RecyclingServices"/>
        <rdfs:comment>Rag merchants is a subcategory of recycling services</rdfs:comment>
        <rdfs:isDefinedBy rdf:resource="https://www.theworldavatar.com/kg/ontopoi"/>
        <rdfs:label>Rag merchants</rdfs:label>
    </owl:Class>
    


    <!-- https://www.theworldavatar.com/kg/ontopoi/RailwayRelatedServices -->


    <owl:Class rdf:about="https://www.theworldavatar.com/kg/ontopoi/RailwayRelatedServices">
        <rdfs:subClassOf rdf:resource="https://www.theworldavatar.com/kg/ontopoi/TransportAndStorageAndDelivery"/>
        <rdfs:comment>Railway related services is a subcategory of transport, storage and delivery</rdfs:comment>
        <rdfs:isDefinedBy rdf:resource="https://www.theworldavatar.com/kg/ontopoi"/>
        <rdfs:label>Railway related services</rdfs:label>
    </owl:Class>
    


    <!-- https://www.theworldavatar.com/kg/ontopoi/RailwayStationsAndJunctionsAndHalts -->


    <owl:Class rdf:about="https://www.theworldavatar.com/kg/ontopoi/RailwayStationsAndJunctionsAndHalts">
        <rdfs:subClassOf rdf:resource="https://www.theworldavatar.com/kg/ontopoi/PublicTransportAndStationsAndInfrastructure"/>
        <rdfs:comment>Railway stations, junctions and halts is a subcategory of public transport, stations and infrastructure</rdfs:comment>
        <rdfs:isDefinedBy rdf:resource="https://www.theworldavatar.com/kg/ontopoi"/>
        <rdfs:label>Railway stations, junctions and halts</rdfs:label>
    </owl:Class>
    


    <!-- https://www.theworldavatar.com/kg/ontopoi/RecordingStudiosAndRecordCompanies -->


    <owl:Class rdf:about="https://www.theworldavatar.com/kg/ontopoi/RecordingStudiosAndRecordCompanies">
        <rdfs:subClassOf rdf:resource="https://www.theworldavatar.com/kg/ontopoi/ItAndAdvertisingAndMarketingAndMediaServiceS"/>
        <rdfs:comment>Recording studios and record companies is a subcategory of it, advertising, marketing and media service s</rdfs:comment>
        <rdfs:isDefinedBy rdf:resource="https://www.theworldavatar.com/kg/ontopoi"/>
        <rdfs:label>Recording studios and record companies</rdfs:label>
    </owl:Class>
    


    <!-- https://www.theworldavatar.com/kg/ontopoi/Recreational -->


    <owl:Class rdf:about="https://www.theworldavatar.com/kg/ontopoi/Recreational">
        <rdfs:subClassOf rdf:resource="https://www.theworldavatar.com/kg/ontopoi/Attractions"/>
        <rdfs:comment>Recreational is a subcategory of attractions</rdfs:comment>
        <rdfs:isDefinedBy rdf:resource="https://www.theworldavatar.com/kg/ontopoi"/>
        <rdfs:label>Recreational</rdfs:label>
    </owl:Class>
    


    <!-- https://www.theworldavatar.com/kg/ontopoi/RecreationalAndVocationalEducation -->


    <owl:Class rdf:about="https://www.theworldavatar.com/kg/ontopoi/RecreationalAndVocationalEducation">
        <rdfs:subClassOf rdf:resource="https://www.theworldavatar.com/kg/ontopoi/EducationAndHealth"/>
        <rdfs:comment>Recreational and vocational education is a subcategory of education and health</rdfs:comment>
        <rdfs:isDefinedBy rdf:resource="https://www.theworldavatar.com/kg/ontopoi"/>
        <rdfs:label>Recreational and vocational education</rdfs:label>
    </owl:Class>
    


    <!-- https://www.theworldavatar.com/kg/ontopoi/RecyclingAndReclamationAndDisposal -->


    <owl:Class rdf:about="https://www.theworldavatar.com/kg/ontopoi/RecyclingAndReclamationAndDisposal">
        <rdfs:subClassOf rdf:resource="https://www.theworldavatar.com/kg/ontopoi/RecyclingServices"/>
        <rdfs:comment>Recycling, reclamation and disposal is a subcategory of recycling services</rdfs:comment>
        <rdfs:isDefinedBy rdf:resource="https://www.theworldavatar.com/kg/ontopoi"/>
        <rdfs:label>Recycling, reclamation and disposal</rdfs:label>
    </owl:Class>
    


    <!-- https://www.theworldavatar.com/kg/ontopoi/RecyclingCentres -->


    <owl:Class rdf:about="https://www.theworldavatar.com/kg/ontopoi/RecyclingCentres">
        <rdfs:subClassOf rdf:resource="https://www.theworldavatar.com/kg/ontopoi/InfrastructureAndFacilities"/>
        <rdfs:comment>Recycling centres is a subcategory of infrastructure and facilities</rdfs:comment>
        <rdfs:isDefinedBy rdf:resource="https://www.theworldavatar.com/kg/ontopoi"/>
        <rdfs:label>Recycling centres</rdfs:label>
    </owl:Class>
    


    <!-- https://www.theworldavatar.com/kg/ontopoi/RecyclingServices -->


    <owl:Class rdf:about="https://www.theworldavatar.com/kg/ontopoi/RecyclingServices">
        <rdfs:subClassOf rdf:resource="https://www.theworldavatar.com/kg/ontopoi/CommercialServices"/>
        <rdfs:comment>Recycling services is a subcategory of commercial services</rdfs:comment>
        <rdfs:isDefinedBy rdf:resource="https://www.theworldavatar.com/kg/ontopoi"/>
        <rdfs:label>Recycling services</rdfs:label>
    </owl:Class>
    


    <!-- https://www.theworldavatar.com/kg/ontopoi/RefrigerationAndFreezingAppliances -->


    <owl:Class rdf:about="https://www.theworldavatar.com/kg/ontopoi/RefrigerationAndFreezingAppliances">
        <rdfs:subClassOf rdf:resource="https://www.theworldavatar.com/kg/ontopoi/ConsumerProducts"/>
        <rdfs:comment>Refrigeration and freezing appliances is a subcategory of consumer products</rdfs:comment>
        <rdfs:isDefinedBy rdf:resource="https://www.theworldavatar.com/kg/ontopoi"/>
        <rdfs:label>Refrigeration and freezing appliances</rdfs:label>
    </owl:Class>
    


    <!-- https://www.theworldavatar.com/kg/ontopoi/RefuseDisposalFacilities -->


    <owl:Class rdf:about="https://www.theworldavatar.com/kg/ontopoi/RefuseDisposalFacilities">
        <rdfs:subClassOf rdf:resource="https://www.theworldavatar.com/kg/ontopoi/InfrastructureAndFacilities"/>
        <rdfs:comment>Refuse disposal facilities is a subcategory of infrastructure and facilities</rdfs:comment>
        <rdfs:isDefinedBy rdf:resource="https://www.theworldavatar.com/kg/ontopoi"/>
        <rdfs:label>Refuse disposal facilities</rdfs:label>
    </owl:Class>
    


    <!-- https://www.theworldavatar.com/kg/ontopoi/RegistrarsOffices -->


    <owl:Class rdf:about="https://www.theworldavatar.com/kg/ontopoi/RegistrarsOffices">
        <rdfs:subClassOf rdf:resource="https://www.theworldavatar.com/kg/ontopoi/CentralAndLocalGovernment"/>
        <rdfs:comment>Registrars offices is a subcategory of central and local government</rdfs:comment>
        <rdfs:isDefinedBy rdf:resource="https://www.theworldavatar.com/kg/ontopoi"/>
        <rdfs:label>Registrars offices</rdfs:label>
    </owl:Class>
    


    <!-- https://www.theworldavatar.com/kg/ontopoi/ReligiousOrganisations -->


    <owl:Class rdf:about="https://www.theworldavatar.com/kg/ontopoi/ReligiousOrganisations">
        <rdfs:subClassOf rdf:resource="https://www.theworldavatar.com/kg/ontopoi/Organisations"/>
        <rdfs:comment>Religious organisations is a subcategory of organisations</rdfs:comment>
        <rdfs:isDefinedBy rdf:resource="https://www.theworldavatar.com/kg/ontopoi"/>
        <rdfs:label>Religious organisations</rdfs:label>
    </owl:Class>
    


    <!-- https://www.theworldavatar.com/kg/ontopoi/RemovalsAndShippingAgents -->


    <owl:Class rdf:about="https://www.theworldavatar.com/kg/ontopoi/RemovalsAndShippingAgents">
        <rdfs:subClassOf rdf:resource="https://www.theworldavatar.com/kg/ontopoi/TransportAndStorageAndDelivery"/>
        <rdfs:comment>Removals and shipping agents is a subcategory of transport, storage and delivery</rdfs:comment>
        <rdfs:isDefinedBy rdf:resource="https://www.theworldavatar.com/kg/ontopoi"/>
        <rdfs:label>Removals and shipping agents</rdfs:label>
    </owl:Class>
    


    <!-- https://www.theworldavatar.com/kg/ontopoi/RentingAndLeasingOfPersonalAndHouseholdGoods -->


    <owl:Class rdf:about="https://www.theworldavatar.com/kg/ontopoi/RentingAndLeasingOfPersonalAndHouseholdGoods">
        <rdfs:subClassOf rdf:resource="https://www.theworldavatar.com/kg/ontopoi/HireServices"/>
        <rdfs:comment>Renting and leasing of personal and household goods is a subcategory of hire services</rdfs:comment>
        <rdfs:isDefinedBy rdf:resource="https://www.theworldavatar.com/kg/ontopoi"/>
        <rdfs:label>Renting and leasing of personal and household goods</rdfs:label>
    </owl:Class>
    


    <!-- https://www.theworldavatar.com/kg/ontopoi/RepairAndServicing -->


    <owl:Class rdf:about="https://www.theworldavatar.com/kg/ontopoi/RepairAndServicing">
        <rdfs:subClassOf rdf:resource="https://www.theworldavatar.com/kg/ontopoi/CommercialServices"/>
        <rdfs:comment>Repair and servicing is a subcategory of commercial services</rdfs:comment>
        <rdfs:isDefinedBy rdf:resource="https://www.theworldavatar.com/kg/ontopoi"/>
        <rdfs:label>Repair and servicing</rdfs:label>
    </owl:Class>
    


    <!-- https://www.theworldavatar.com/kg/ontopoi/ResearchAndDesign -->


    <owl:Class rdf:about="https://www.theworldavatar.com/kg/ontopoi/ResearchAndDesign">
        <rdfs:subClassOf rdf:resource="https://www.theworldavatar.com/kg/ontopoi/CommercialServices"/>
        <rdfs:comment>Research and design is a subcategory of commercial services</rdfs:comment>
        <rdfs:isDefinedBy rdf:resource="https://www.theworldavatar.com/kg/ontopoi"/>
        <rdfs:label>Research and design</rdfs:label>
    </owl:Class>
    


    <!-- https://www.theworldavatar.com/kg/ontopoi/ResearchServices -->


    <owl:Class rdf:about="https://www.theworldavatar.com/kg/ontopoi/ResearchServices">
        <rdfs:subClassOf rdf:resource="https://www.theworldavatar.com/kg/ontopoi/ResearchAndDesign"/>
        <rdfs:comment>Research services is a subcategory of research and design</rdfs:comment>
        <rdfs:isDefinedBy rdf:resource="https://www.theworldavatar.com/kg/ontopoi"/>
        <rdfs:label>Research services</rdfs:label>
    </owl:Class>
    


    <!-- https://www.theworldavatar.com/kg/ontopoi/Reservoirs -->


    <owl:Class rdf:about="https://www.theworldavatar.com/kg/ontopoi/Reservoirs">
        <rdfs:subClassOf rdf:resource="https://www.theworldavatar.com/kg/ontopoi/BodiesOfWater"/>
        <rdfs:comment>Reservoirs is a subcategory of bodies of water</rdfs:comment>
        <rdfs:isDefinedBy rdf:resource="https://www.theworldavatar.com/kg/ontopoi"/>
        <rdfs:label>Reservoirs</rdfs:label>
    </owl:Class>
    


    <!-- https://www.theworldavatar.com/kg/ontopoi/Restaurants -->


    <owl:Class rdf:about="https://www.theworldavatar.com/kg/ontopoi/Restaurants">
        <rdfs:subClassOf rdf:resource="https://www.theworldavatar.com/kg/ontopoi/EatingAndDrinking"/>
        <rdfs:comment>Restaurants is a subcategory of eating and drinking</rdfs:comment>
        <rdfs:isDefinedBy rdf:resource="https://www.theworldavatar.com/kg/ontopoi"/>
        <rdfs:label>Restaurants</rdfs:label>
    </owl:Class>
    


    <!-- https://www.theworldavatar.com/kg/ontopoi/RestorationAndPreservationServices -->


    <owl:Class rdf:about="https://www.theworldavatar.com/kg/ontopoi/RestorationAndPreservationServices">
        <rdfs:subClassOf rdf:resource="https://www.theworldavatar.com/kg/ontopoi/ConstructionServices"/>
        <rdfs:comment>Restoration and preservation services is a subcategory of construction services</rdfs:comment>
        <rdfs:isDefinedBy rdf:resource="https://www.theworldavatar.com/kg/ontopoi"/>
        <rdfs:label>Restoration and preservation services</rdfs:label>
    </owl:Class>
    


    <!-- https://www.theworldavatar.com/kg/ontopoi/Retail -->


    <owl:Class rdf:about="https://www.theworldavatar.com/kg/ontopoi/Retail">
        <rdfs:subClassOf rdf:resource="https://www.theworldavatar.com/kg/ontopoi/PointOfInterest"/>
        <rdfs:comment>Businesses that purchase products from manufacturers or wholesalers and sell them to end users through various channels, such as physical stores, online platforms, or direct sales</rdfs:comment>
        <rdfs:isDefinedBy rdf:resource="https://www.theworldavatar.com/kg/ontopoi"/>
        <rdfs:label>Retail</rdfs:label>
    </owl:Class>
    


    <!-- https://www.theworldavatar.com/kg/ontopoi/RevenueAndCustomsOffices -->


    <owl:Class rdf:about="https://www.theworldavatar.com/kg/ontopoi/RevenueAndCustomsOffices">
        <rdfs:subClassOf rdf:resource="https://www.theworldavatar.com/kg/ontopoi/CentralAndLocalGovernment"/>
        <rdfs:comment>Revenue and customs offices is a subcategory of central and local government</rdfs:comment>
        <rdfs:isDefinedBy rdf:resource="https://www.theworldavatar.com/kg/ontopoi"/>
        <rdfs:label>Revenue and customs offices</rdfs:label>
    </owl:Class>
    


    <!-- https://www.theworldavatar.com/kg/ontopoi/RidingSchoolsAndLiveryStablesAndEquestrianCentres -->


    <owl:Class rdf:about="https://www.theworldavatar.com/kg/ontopoi/RidingSchoolsAndLiveryStablesAndEquestrianCentres">
        <rdfs:subClassOf rdf:resource="https://www.theworldavatar.com/kg/ontopoi/OutdoorPursuits"/>
        <rdfs:comment>Riding schools, livery stables and equestrian centres is a subcategory of outdoor pursuits</rdfs:comment>
        <rdfs:isDefinedBy rdf:resource="https://www.theworldavatar.com/kg/ontopoi"/>
        <rdfs:label>Riding schools, livery stables and equestrian centres</rdfs:label>
    </owl:Class>
    


    <!-- https://www.theworldavatar.com/kg/ontopoi/RiversAndCanalOrganisationsAndInfrastructure -->


    <owl:Class rdf:about="https://www.theworldavatar.com/kg/ontopoi/RiversAndCanalOrganisationsAndInfrastructure">
        <rdfs:subClassOf rdf:resource="https://www.theworldavatar.com/kg/ontopoi/Water"/>
        <rdfs:comment>Rivers and canal organisations and infrastructure is a subcategory of water</rdfs:comment>
        <rdfs:isDefinedBy rdf:resource="https://www.theworldavatar.com/kg/ontopoi"/>
        <rdfs:label>Rivers and canal organisations and infrastructure</rdfs:label>
    </owl:Class>
    


    <!-- https://www.theworldavatar.com/kg/ontopoi/RoadAndRail -->


    <owl:Class rdf:about="https://www.theworldavatar.com/kg/ontopoi/RoadAndRail">
        <rdfs:subClassOf rdf:resource="https://www.theworldavatar.com/kg/ontopoi/Transport"/>
        <rdfs:comment>Road and rail is a subcategory of transport</rdfs:comment>
        <rdfs:isDefinedBy rdf:resource="https://www.theworldavatar.com/kg/ontopoi"/>
        <rdfs:label>Road and rail</rdfs:label>
    </owl:Class>
    


    <!-- https://www.theworldavatar.com/kg/ontopoi/RoadConstructionServices -->


    <owl:Class rdf:about="https://www.theworldavatar.com/kg/ontopoi/RoadConstructionServices">
        <rdfs:subClassOf rdf:resource="https://www.theworldavatar.com/kg/ontopoi/ConstructionServices"/>
        <rdfs:comment>Road construction services is a subcategory of construction services</rdfs:comment>
        <rdfs:isDefinedBy rdf:resource="https://www.theworldavatar.com/kg/ontopoi"/>
        <rdfs:label>Road construction services</rdfs:label>
    </owl:Class>
    


    <!-- https://www.theworldavatar.com/kg/ontopoi/RoadMaintenanceEquipment -->


    <owl:Class rdf:about="https://www.theworldavatar.com/kg/ontopoi/RoadMaintenanceEquipment">
        <rdfs:subClassOf rdf:resource="https://www.theworldavatar.com/kg/ontopoi/IndustrialProducts"/>
        <rdfs:comment>Road maintenance equipment is a subcategory of industrial products</rdfs:comment>
        <rdfs:isDefinedBy rdf:resource="https://www.theworldavatar.com/kg/ontopoi"/>
        <rdfs:label>Road maintenance equipment</rdfs:label>
    </owl:Class>
    


    <!-- https://www.theworldavatar.com/kg/ontopoi/RoofingAndChimneyServices -->


    <owl:Class rdf:about="https://www.theworldavatar.com/kg/ontopoi/RoofingAndChimneyServices">
        <rdfs:subClassOf rdf:resource="https://www.theworldavatar.com/kg/ontopoi/ConstructionServices"/>
        <rdfs:comment>Roofing and chimney services is a subcategory of construction services</rdfs:comment>
        <rdfs:isDefinedBy rdf:resource="https://www.theworldavatar.com/kg/ontopoi"/>
        <rdfs:label>Roofing and chimney services</rdfs:label>
    </owl:Class>
    


    <!-- https://www.theworldavatar.com/kg/ontopoi/RopesAndNetsAndCordage -->


    <owl:Class rdf:about="https://www.theworldavatar.com/kg/ontopoi/RopesAndNetsAndCordage">
        <rdfs:subClassOf rdf:resource="https://www.theworldavatar.com/kg/ontopoi/IndustrialProducts"/>
        <rdfs:comment>Ropes, nets and cordage is a subcategory of industrial products</rdfs:comment>
        <rdfs:isDefinedBy rdf:resource="https://www.theworldavatar.com/kg/ontopoi"/>
        <rdfs:label>Ropes, nets and cordage</rdfs:label>
    </owl:Class>
    


    <!-- https://www.theworldavatar.com/kg/ontopoi/RubberAndSiliconesAndPlastics -->


    <owl:Class rdf:about="https://www.theworldavatar.com/kg/ontopoi/RubberAndSiliconesAndPlastics">
        <rdfs:subClassOf rdf:resource="https://www.theworldavatar.com/kg/ontopoi/IndustrialProducts"/>
        <rdfs:comment>Rubber, silicones and plastics is a subcategory of industrial products</rdfs:comment>
        <rdfs:isDefinedBy rdf:resource="https://www.theworldavatar.com/kg/ontopoi"/>
        <rdfs:label>Rubber, silicones and plastics</rdfs:label>
    </owl:Class>
    


    <!-- https://www.theworldavatar.com/kg/ontopoi/SailingSchools -->


    <owl:Class rdf:about="https://www.theworldavatar.com/kg/ontopoi/SailingSchools">
        <rdfs:subClassOf rdf:resource="https://www.theworldavatar.com/kg/ontopoi/RecreationalAndVocationalEducation"/>
        <rdfs:comment>Sailing schools is a subcategory of recreational and vocational education</rdfs:comment>
        <rdfs:isDefinedBy rdf:resource="https://www.theworldavatar.com/kg/ontopoi"/>
        <rdfs:label>Sailing schools</rdfs:label>
    </owl:Class>
    


    <!-- https://www.theworldavatar.com/kg/ontopoi/SalmonLadders -->


    <owl:Class rdf:about="https://www.theworldavatar.com/kg/ontopoi/SalmonLadders">
        <rdfs:subClassOf rdf:resource="https://www.theworldavatar.com/kg/ontopoi/BotanicalAndZoological"/>
        <rdfs:comment>Salmon ladders is a subcategory of botanical and zoological</rdfs:comment>
        <rdfs:isDefinedBy rdf:resource="https://www.theworldavatar.com/kg/ontopoi"/>
        <rdfs:label>Salmon ladders</rdfs:label>
    </owl:Class>
    


    <!-- https://www.theworldavatar.com/kg/ontopoi/SandAndGravelAndClayExtractionAndMerchants -->


    <owl:Class rdf:about="https://www.theworldavatar.com/kg/ontopoi/SandAndGravelAndClayExtractionAndMerchants">
        <rdfs:subClassOf rdf:resource="https://www.theworldavatar.com/kg/ontopoi/ExtractiveIndustries"/>
        <rdfs:comment>Sand, gravel and clay extraction and merchants is a subcategory of extractive industries</rdfs:comment>
        <rdfs:isDefinedBy rdf:resource="https://www.theworldavatar.com/kg/ontopoi"/>
        <rdfs:label>Sand, gravel and clay extraction and merchants</rdfs:label>
    </owl:Class>
    


    <!-- https://www.theworldavatar.com/kg/ontopoi/SaunasAndSunbeds -->


    <owl:Class rdf:about="https://www.theworldavatar.com/kg/ontopoi/SaunasAndSunbeds">
        <rdfs:subClassOf rdf:resource="https://www.theworldavatar.com/kg/ontopoi/ConsumerProducts"/>
        <rdfs:comment>Saunas and sunbeds is a subcategory of consumer products</rdfs:comment>
        <rdfs:isDefinedBy rdf:resource="https://www.theworldavatar.com/kg/ontopoi"/>
        <rdfs:label>Saunas and sunbeds</rdfs:label>
    </owl:Class>
    


    <!-- https://www.theworldavatar.com/kg/ontopoi/ScrapMetaLdealersAndBreakersYards -->


    <owl:Class rdf:about="https://www.theworldavatar.com/kg/ontopoi/ScrapMetaLdealersAndBreakersYards">
        <rdfs:subClassOf rdf:resource="https://www.theworldavatar.com/kg/ontopoi/RecyclingServices"/>
        <rdfs:comment>Scrap meta ldealers and breakers yards is a subcategory of recycling services</rdfs:comment>
        <rdfs:isDefinedBy rdf:resource="https://www.theworldavatar.com/kg/ontopoi"/>
        <rdfs:label>Scrap meta ldealers and breakers yards</rdfs:label>
    </owl:Class>
    


    <!-- https://www.theworldavatar.com/kg/ontopoi/SculptorsAndWoodworkersAndStonemasons -->


    <owl:Class rdf:about="https://www.theworldavatar.com/kg/ontopoi/SculptorsAndWoodworkersAndStonemasons">
        <rdfs:subClassOf rdf:resource="https://www.theworldavatar.com/kg/ontopoi/PersonalAndConsumerAndOtherServices"/>
        <rdfs:comment>Sculptors, woodworkers and stonemasons is a subcategory of personal, consumer and other services</rdfs:comment>
        <rdfs:isDefinedBy rdf:resource="https://www.theworldavatar.com/kg/ontopoi"/>
        <rdfs:label>Sculptors, woodworkers and stonemasons</rdfs:label>
    </owl:Class>
    


    <!-- https://www.theworldavatar.com/kg/ontopoi/SealsAndTapesAndTapsAndValves -->


    <owl:Class rdf:about="https://www.theworldavatar.com/kg/ontopoi/SealsAndTapesAndTapsAndValves">
        <rdfs:subClassOf rdf:resource="https://www.theworldavatar.com/kg/ontopoi/IndustrialProducts"/>
        <rdfs:comment>Seals, tapes, taps and valves is a subcategory of industrial products</rdfs:comment>
        <rdfs:isDefinedBy rdf:resource="https://www.theworldavatar.com/kg/ontopoi"/>
        <rdfs:label>Seals, tapes, taps and valves</rdfs:label>
    </owl:Class>
    


    <!-- https://www.theworldavatar.com/kg/ontopoi/Second-HandGoods -->


    <owl:Class rdf:about="https://www.theworldavatar.com/kg/ontopoi/Second-HandGoods">
        <rdfs:subClassOf rdf:resource="https://www.theworldavatar.com/kg/ontopoi/HouseholdAndOfficeAndLeisureAndGarden"/>
        <rdfs:comment>Second-hand goods is a subcategory of household, office, leisure and garden</rdfs:comment>
        <rdfs:isDefinedBy rdf:resource="https://www.theworldavatar.com/kg/ontopoi"/>
        <rdfs:label>Second-hand goods</rdfs:label>
    </owl:Class>
    


    <!-- https://www.theworldavatar.com/kg/ontopoi/Second-HandVehicles -->


    <owl:Class rdf:about="https://www.theworldavatar.com/kg/ontopoi/Second-HandVehicles">
        <rdfs:subClassOf rdf:resource="https://www.theworldavatar.com/kg/ontopoi/Motoring"/>
        <rdfs:comment>Second-hand vehicles is a subcategory of motoring</rdfs:comment>
        <rdfs:isDefinedBy rdf:resource="https://www.theworldavatar.com/kg/ontopoi"/>
        <rdfs:label>Second-hand vehicles</rdfs:label>
    </owl:Class>
    


    <!-- https://www.theworldavatar.com/kg/ontopoi/SecureUnits -->


    <owl:Class rdf:about="https://www.theworldavatar.com/kg/ontopoi/SecureUnits">
        <rdfs:subClassOf rdf:resource="https://www.theworldavatar.com/kg/ontopoi/EducationSupportServices"/>
        <rdfs:comment>Secure units is a subcategory of education support services</rdfs:comment>
        <rdfs:isDefinedBy rdf:resource="https://www.theworldavatar.com/kg/ontopoi"/>
        <rdfs:label>Secure units</rdfs:label>
    </owl:Class>
    


    <!-- https://www.theworldavatar.com/kg/ontopoi/SecurityConsultants -->


    <owl:Class rdf:about="https://www.theworldavatar.com/kg/ontopoi/SecurityConsultants">
        <rdfs:subClassOf rdf:resource="https://www.theworldavatar.com/kg/ontopoi/Consultancies"/>
        <rdfs:comment>Security consultants is a subcategory of consultancies</rdfs:comment>
        <rdfs:isDefinedBy rdf:resource="https://www.theworldavatar.com/kg/ontopoi"/>
        <rdfs:label>Security consultants</rdfs:label>
    </owl:Class>
    


    <!-- https://www.theworldavatar.com/kg/ontopoi/SelfCatering -->


    <owl:Class rdf:about="https://www.theworldavatar.com/kg/ontopoi/SelfCatering">
        <rdfs:subClassOf rdf:resource="https://www.theworldavatar.com/kg/ontopoi/Accommodation"/>
        <rdfs:comment>Self catering is a subcategory of accommodation</rdfs:comment>
        <rdfs:isDefinedBy rdf:resource="https://www.theworldavatar.com/kg/ontopoi"/>
        <rdfs:label>Self catering</rdfs:label>
    </owl:Class>
    


    <!-- https://www.theworldavatar.com/kg/ontopoi/ServiceIndustryEquipmentRepairs -->


    <owl:Class rdf:about="https://www.theworldavatar.com/kg/ontopoi/ServiceIndustryEquipmentRepairs">
        <rdfs:subClassOf rdf:resource="https://www.theworldavatar.com/kg/ontopoi/RepairAndServicing"/>
        <rdfs:comment>Service industry equipment repairs is a subcategory of repair and servicing</rdfs:comment>
        <rdfs:isDefinedBy rdf:resource="https://www.theworldavatar.com/kg/ontopoi"/>
        <rdfs:label>Service industry equipment repairs</rdfs:label>
    </owl:Class>
    


    <!-- https://www.theworldavatar.com/kg/ontopoi/SewageServices -->


    <owl:Class rdf:about="https://www.theworldavatar.com/kg/ontopoi/SewageServices">
        <rdfs:subClassOf rdf:resource="https://www.theworldavatar.com/kg/ontopoi/PersonalAndConsumerAndOtherServices"/>
        <rdfs:comment>Sewage services is a subcategory of personal, consumer and other services</rdfs:comment>
        <rdfs:isDefinedBy rdf:resource="https://www.theworldavatar.com/kg/ontopoi"/>
        <rdfs:label>Sewage Services</rdfs:label>
    </owl:Class>
    


    <!-- https://www.theworldavatar.com/kg/ontopoi/ShelvingAndStorageAndSafesAndVaults -->


    <owl:Class rdf:about="https://www.theworldavatar.com/kg/ontopoi/ShelvingAndStorageAndSafesAndVaults">
        <rdfs:subClassOf rdf:resource="https://www.theworldavatar.com/kg/ontopoi/IndustrialProducts"/>
        <rdfs:comment>Shelving, storage, safes and vaults is a subcategory of industrial products</rdfs:comment>
        <rdfs:isDefinedBy rdf:resource="https://www.theworldavatar.com/kg/ontopoi"/>
        <rdfs:label>Shelving, storage, safes and vaults</rdfs:label>
    </owl:Class>
    


    <!-- https://www.theworldavatar.com/kg/ontopoi/ShoeRepairs -->


    <owl:Class rdf:about="https://www.theworldavatar.com/kg/ontopoi/ShoeRepairs">
        <rdfs:subClassOf rdf:resource="https://www.theworldavatar.com/kg/ontopoi/RepairAndServicing"/>
        <rdfs:comment>Shoe repairs is a subcategory of repair and servicing</rdfs:comment>
        <rdfs:isDefinedBy rdf:resource="https://www.theworldavatar.com/kg/ontopoi"/>
        <rdfs:label>Shoe repairs</rdfs:label>
    </owl:Class>
    


    <!-- https://www.theworldavatar.com/kg/ontopoi/ShootingFacilities -->


    <owl:Class rdf:about="https://www.theworldavatar.com/kg/ontopoi/ShootingFacilities">
        <rdfs:subClassOf rdf:resource="https://www.theworldavatar.com/kg/ontopoi/SportsComplex"/>
        <rdfs:comment>Shooting facilities is a subcategory of sports complex</rdfs:comment>
        <rdfs:isDefinedBy rdf:resource="https://www.theworldavatar.com/kg/ontopoi"/>
        <rdfs:label>Shooting facilities</rdfs:label>
    </owl:Class>
    


    <!-- https://www.theworldavatar.com/kg/ontopoi/ShoppingCentresAndRetailParks -->


    <owl:Class rdf:about="https://www.theworldavatar.com/kg/ontopoi/ShoppingCentresAndRetailParks">
        <rdfs:subClassOf rdf:resource="https://www.theworldavatar.com/kg/ontopoi/HouseholdAndOfficeAndLeisureAndGarden"/>
        <rdfs:comment>Shopping centres and retail parks is a subcategory of household, office, leisure and garden</rdfs:comment>
        <rdfs:isDefinedBy rdf:resource="https://www.theworldavatar.com/kg/ontopoi"/>
        <rdfs:label>Shopping centres and retail parks</rdfs:label>
    </owl:Class>
    


    <!-- https://www.theworldavatar.com/kg/ontopoi/SightseeingAndToursAndViewingAndVisitorCentres -->


    <owl:Class rdf:about="https://www.theworldavatar.com/kg/ontopoi/SightseeingAndToursAndViewingAndVisitorCentres">
        <rdfs:subClassOf rdf:resource="https://www.theworldavatar.com/kg/ontopoi/Tourism"/>
        <rdfs:comment>Sightseeing, tours, viewing and visitor centres is a subcategory of tourism</rdfs:comment>
        <rdfs:isDefinedBy rdf:resource="https://www.theworldavatar.com/kg/ontopoi"/>
        <rdfs:label>Sightseeing, tours, viewing and visitor centres</rdfs:label>
    </owl:Class>
    


    <!-- https://www.theworldavatar.com/kg/ontopoi/SignallingFacilities -->


    <owl:Class rdf:about="https://www.theworldavatar.com/kg/ontopoi/SignallingFacilities">
        <rdfs:subClassOf rdf:resource="https://www.theworldavatar.com/kg/ontopoi/RoadAndRail"/>
        <rdfs:comment>Signalling facilities is a subcategory of road and rail</rdfs:comment>
        <rdfs:isDefinedBy rdf:resource="https://www.theworldavatar.com/kg/ontopoi"/>
        <rdfs:label>Signalling facilities</rdfs:label>
    </owl:Class>
    


    <!-- https://www.theworldavatar.com/kg/ontopoi/Signs -->


    <owl:Class rdf:about="https://www.theworldavatar.com/kg/ontopoi/Signs">
        <rdfs:subClassOf rdf:resource="https://www.theworldavatar.com/kg/ontopoi/IndustrialProducts"/>
        <rdfs:comment>Signs is a subcategory of industrial products</rdfs:comment>
        <rdfs:isDefinedBy rdf:resource="https://www.theworldavatar.com/kg/ontopoi"/>
        <rdfs:label>Signs</rdfs:label>
    </owl:Class>
    


    <!-- https://www.theworldavatar.com/kg/ontopoi/SkiInfrastructureAndAerialCableways -->


    <owl:Class rdf:about="https://www.theworldavatar.com/kg/ontopoi/SkiInfrastructureAndAerialCableways">
        <rdfs:subClassOf rdf:resource="https://www.theworldavatar.com/kg/ontopoi/SportsComplex"/>
        <rdfs:comment>Ski infrastructure and aerial cableways is a subcategory of sports complex</rdfs:comment>
        <rdfs:isDefinedBy rdf:resource="https://www.theworldavatar.com/kg/ontopoi"/>
        <rdfs:label>Ski infrastructure and aerial cableways</rdfs:label>
    </owl:Class>
    


    <!-- https://www.theworldavatar.com/kg/ontopoi/SlimmingClubsAndServices -->


    <owl:Class rdf:about="https://www.theworldavatar.com/kg/ontopoi/SlimmingClubsAndServices">
        <rdfs:subClassOf rdf:resource="https://www.theworldavatar.com/kg/ontopoi/PersonalAndConsumerAndOtherServices"/>
        <rdfs:comment>Slimming clubs and services is a subcategory of personal, consumer and other services</rdfs:comment>
        <rdfs:isDefinedBy rdf:resource="https://www.theworldavatar.com/kg/ontopoi"/>
        <rdfs:label>Slimming clubs and services</rdfs:label>
    </owl:Class>
    


    <!-- https://www.theworldavatar.com/kg/ontopoi/SnookerAndPoolHalls -->


    <owl:Class rdf:about="https://www.theworldavatar.com/kg/ontopoi/SnookerAndPoolHalls">
        <rdfs:subClassOf rdf:resource="https://www.theworldavatar.com/kg/ontopoi/SportsComplex"/>
        <rdfs:comment>Snooker and pool halls is a subcategory of sports complex</rdfs:comment>
        <rdfs:isDefinedBy rdf:resource="https://www.theworldavatar.com/kg/ontopoi"/>
        <rdfs:label>Snooker and pool halls</rdfs:label>
    </owl:Class>
    


    <!-- https://www.theworldavatar.com/kg/ontopoi/SocialClubs -->


    <owl:Class rdf:about="https://www.theworldavatar.com/kg/ontopoi/SocialClubs">
        <rdfs:subClassOf rdf:resource="https://www.theworldavatar.com/kg/ontopoi/VenuesAndStageAndScreen"/>
        <rdfs:comment>Social clubs is a subcategory of venues, stage and screen</rdfs:comment>
        <rdfs:isDefinedBy rdf:resource="https://www.theworldavatar.com/kg/ontopoi"/>
        <rdfs:label>Social clubs</rdfs:label>
    </owl:Class>
    


    <!-- https://www.theworldavatar.com/kg/ontopoi/SocialServiceActivities -->


    <owl:Class rdf:about="https://www.theworldavatar.com/kg/ontopoi/SocialServiceActivities">
        <rdfs:subClassOf rdf:resource="https://www.theworldavatar.com/kg/ontopoi/CentralAndLocalGovernment"/>
        <rdfs:comment>Social service activities is a subcategory of central and local government</rdfs:comment>
        <rdfs:isDefinedBy rdf:resource="https://www.theworldavatar.com/kg/ontopoi"/>
        <rdfs:label>Social service activities</rdfs:label>
    </owl:Class>
    


    <!-- https://www.theworldavatar.com/kg/ontopoi/SolicitorsAndAdvocatesAndNotariesPublic -->


    <owl:Class rdf:about="https://www.theworldavatar.com/kg/ontopoi/SolicitorsAndAdvocatesAndNotariesPublic">
        <rdfs:subClassOf rdf:resource="https://www.theworldavatar.com/kg/ontopoi/LegalAndFinancial"/>
        <rdfs:comment>Solicitors, advocates and notaries public is a subcategory of legal and financial</rdfs:comment>
        <rdfs:isDefinedBy rdf:resource="https://www.theworldavatar.com/kg/ontopoi"/>
        <rdfs:label>Solicitors, advocates and notaries public</rdfs:label>
    </owl:Class>
    


    <!-- https://www.theworldavatar.com/kg/ontopoi/SoundAndLightAndVisionServiceAndEquipmentHire -->


    <owl:Class rdf:about="https://www.theworldavatar.com/kg/ontopoi/SoundAndLightAndVisionServiceAndEquipmentHire">
        <rdfs:subClassOf rdf:resource="https://www.theworldavatar.com/kg/ontopoi/HireServices"/>
        <rdfs:comment>Sound, light and vision service and equipment hire is a subcategory of hire services</rdfs:comment>
        <rdfs:isDefinedBy rdf:resource="https://www.theworldavatar.com/kg/ontopoi"/>
        <rdfs:label>Sound, light and vision service and equipment hire</rdfs:label>
    </owl:Class>
    


    <!-- https://www.theworldavatar.com/kg/ontopoi/SourceReference -->


    <owl:Class rdf:about="https://www.theworldavatar.com/kg/ontopoi/SourceReference">
        <rdfs:comment>Source or origin of the POI data, indicating where or how the information was gathered</rdfs:comment>
        <rdfs:isDefinedBy rdf:resource="https://www.theworldavatar.com/kg/ontopoi"/>
        <rdfs:label>Source Reference</rdfs:label>
    </owl:Class>
    


    <!-- https://www.theworldavatar.com/kg/ontopoi/Spas -->


    <owl:Class rdf:about="https://www.theworldavatar.com/kg/ontopoi/Spas">
        <rdfs:subClassOf rdf:resource="https://www.theworldavatar.com/kg/ontopoi/PersonalAndConsumerAndOtherServices"/>
        <rdfs:comment>Spas is a subcategory of personal, consumer and other services</rdfs:comment>
        <rdfs:isDefinedBy rdf:resource="https://www.theworldavatar.com/kg/ontopoi"/>
        <rdfs:label>Spas</rdfs:label>
    </owl:Class>
    


    <!-- https://www.theworldavatar.com/kg/ontopoi/SpecialPurposeMachineryAndEquipment -->


    <owl:Class rdf:about="https://www.theworldavatar.com/kg/ontopoi/SpecialPurposeMachineryAndEquipment">
        <rdfs:subClassOf rdf:resource="https://www.theworldavatar.com/kg/ontopoi/IndustrialProducts"/>
        <rdfs:comment>Special purpose machinery and equipment is a subcategory of industrial products</rdfs:comment>
        <rdfs:isDefinedBy rdf:resource="https://www.theworldavatar.com/kg/ontopoi"/>
        <rdfs:label>Special purpose machinery and equipment</rdfs:label>
    </owl:Class>
    


    <!-- https://www.theworldavatar.com/kg/ontopoi/SpecialSchoolsAndColleges -->


    <owl:Class rdf:about="https://www.theworldavatar.com/kg/ontopoi/SpecialSchoolsAndColleges">
        <rdfs:subClassOf rdf:resource="https://www.theworldavatar.com/kg/ontopoi/PrimaryAndSecondaryAndTertiaryEducation"/>
        <rdfs:comment>Special schools and colleges is a subcategory of primary, secondary and tertiary education</rdfs:comment>
        <rdfs:isDefinedBy rdf:resource="https://www.theworldavatar.com/kg/ontopoi"/>
        <rdfs:label>Special schools and colleges</rdfs:label>
    </owl:Class>
    


    <!-- https://www.theworldavatar.com/kg/ontopoi/SpeechTherapists -->


    <owl:Class rdf:about="https://www.theworldavatar.com/kg/ontopoi/SpeechTherapists">
        <rdfs:subClassOf rdf:resource="https://www.theworldavatar.com/kg/ontopoi/HealthPractitionersAndEstablishments"/>
        <rdfs:comment>Speech therapists is a subcategory of health practitioners and establishments</rdfs:comment>
        <rdfs:isDefinedBy rdf:resource="https://www.theworldavatar.com/kg/ontopoi"/>
        <rdfs:label>Speech therapists</rdfs:label>
    </owl:Class>
    


    <!-- https://www.theworldavatar.com/kg/ontopoi/SportAndEntertainment -->


    <owl:Class rdf:about="https://www.theworldavatar.com/kg/ontopoi/SportAndEntertainment">
        <rdfs:subClassOf rdf:resource="https://www.theworldavatar.com/kg/ontopoi/PointOfInterest"/>
        <rdfs:comment>Activities, events, or venues that provide enjoyment, or competition for individuals or audiences</rdfs:comment>
        <rdfs:isDefinedBy rdf:resource="https://www.theworldavatar.com/kg/ontopoi"/>
        <rdfs:label>Sport and entertainment</rdfs:label>
    </owl:Class>
    


    <!-- https://www.theworldavatar.com/kg/ontopoi/SportAndEntertainmentSupportServices -->


    <owl:Class rdf:about="https://www.theworldavatar.com/kg/ontopoi/SportAndEntertainmentSupportServices">
        <rdfs:subClassOf rdf:resource="https://www.theworldavatar.com/kg/ontopoi/SportAndEntertainment"/>
        <rdfs:comment>Sport and entertainment support services is a subcategory of sport and entertainment</rdfs:comment>
        <rdfs:isDefinedBy rdf:resource="https://www.theworldavatar.com/kg/ontopoi"/>
        <rdfs:label>Sport and entertainment support services</rdfs:label>
    </owl:Class>
    


    <!-- https://www.theworldavatar.com/kg/ontopoi/SportsAndFitnessCoaching -->


    <owl:Class rdf:about="https://www.theworldavatar.com/kg/ontopoi/SportsAndFitnessCoaching">
        <rdfs:subClassOf rdf:resource="https://www.theworldavatar.com/kg/ontopoi/RecreationalAndVocationalEducation"/>
        <rdfs:comment>Sports and fitness coaching is a subcategory of recreational and vocational education</rdfs:comment>
        <rdfs:isDefinedBy rdf:resource="https://www.theworldavatar.com/kg/ontopoi"/>
        <rdfs:label>Sports and fitness coaching</rdfs:label>
    </owl:Class>
    


    <!-- https://www.theworldavatar.com/kg/ontopoi/SportsAndLeisureEquipmentRepair -->


    <owl:Class rdf:about="https://www.theworldavatar.com/kg/ontopoi/SportsAndLeisureEquipmentRepair">
        <rdfs:subClassOf rdf:resource="https://www.theworldavatar.com/kg/ontopoi/RepairAndServicing"/>
        <rdfs:comment>Sports and leisure equipment repair is a subcategory of repair and servicing</rdfs:comment>
        <rdfs:isDefinedBy rdf:resource="https://www.theworldavatar.com/kg/ontopoi"/>
        <rdfs:label>Sports and leisure equipment repair</rdfs:label>
    </owl:Class>
    


    <!-- https://www.theworldavatar.com/kg/ontopoi/SportsClubsAndAssociations -->


    <owl:Class rdf:about="https://www.theworldavatar.com/kg/ontopoi/SportsClubsAndAssociations">
        <rdfs:subClassOf rdf:resource="https://www.theworldavatar.com/kg/ontopoi/Organisations"/>
        <rdfs:comment>Sports clubs and associations is a subcategory of organisations</rdfs:comment>
        <rdfs:isDefinedBy rdf:resource="https://www.theworldavatar.com/kg/ontopoi"/>
        <rdfs:label>Sports clubs and associations</rdfs:label>
    </owl:Class>
    


    <!-- https://www.theworldavatar.com/kg/ontopoi/SportsComplex -->


    <owl:Class rdf:about="https://www.theworldavatar.com/kg/ontopoi/SportsComplex">
        <rdfs:subClassOf rdf:resource="https://www.theworldavatar.com/kg/ontopoi/SportAndEntertainment"/>
        <rdfs:comment>Sports complex is a subcategory of sport and entertainment</rdfs:comment>
        <rdfs:isDefinedBy rdf:resource="https://www.theworldavatar.com/kg/ontopoi"/>
        <rdfs:label>Sports complex</rdfs:label>
    </owl:Class>
    


    <!-- https://www.theworldavatar.com/kg/ontopoi/SportsGroundsAndStadiaAndPitches -->


    <owl:Class rdf:about="https://www.theworldavatar.com/kg/ontopoi/SportsGroundsAndStadiaAndPitches">
        <rdfs:subClassOf rdf:resource="https://www.theworldavatar.com/kg/ontopoi/SportsComplex"/>
        <rdfs:comment>Sports grounds, stadia and pitches is a subcategory of sports complex</rdfs:comment>
        <rdfs:isDefinedBy rdf:resource="https://www.theworldavatar.com/kg/ontopoi"/>
        <rdfs:label>Sports grounds, stadia and pitches</rdfs:label>
    </owl:Class>
    


    <!-- https://www.theworldavatar.com/kg/ontopoi/SportsServices -->


    <owl:Class rdf:about="https://www.theworldavatar.com/kg/ontopoi/SportsServices">
        <rdfs:subClassOf rdf:resource="https://www.theworldavatar.com/kg/ontopoi/PersonalAndConsumerAndOtherServices"/>
        <rdfs:comment>Sports services is a subcategory of personal, consumer and other services</rdfs:comment>
        <rdfs:isDefinedBy rdf:resource="https://www.theworldavatar.com/kg/ontopoi"/>
        <rdfs:label>Sports services</rdfs:label>
    </owl:Class>
    


    <!-- https://www.theworldavatar.com/kg/ontopoi/SquashCourts -->


    <owl:Class rdf:about="https://www.theworldavatar.com/kg/ontopoi/SquashCourts">
        <rdfs:subClassOf rdf:resource="https://www.theworldavatar.com/kg/ontopoi/SportsComplex"/>
        <rdfs:comment>Squash courts is a subcategory of sports complex</rdfs:comment>
        <rdfs:isDefinedBy rdf:resource="https://www.theworldavatar.com/kg/ontopoi"/>
        <rdfs:label>Squash courts</rdfs:label>
    </owl:Class>
    


    <!-- https://www.theworldavatar.com/kg/ontopoi/StationeryAndOfficeSupplies -->


    <owl:Class rdf:about="https://www.theworldavatar.com/kg/ontopoi/StationeryAndOfficeSupplies">
        <rdfs:subClassOf rdf:resource="https://www.theworldavatar.com/kg/ontopoi/HouseholdAndOfficeAndLeisureAndGarden"/>
        <rdfs:comment>Stationery and office supplies is a subcategory of household, office, leisure and garden</rdfs:comment>
        <rdfs:isDefinedBy rdf:resource="https://www.theworldavatar.com/kg/ontopoi"/>
        <rdfs:label>Stationery and office supplies</rdfs:label>
    </owl:Class>
    


    <!-- https://www.theworldavatar.com/kg/ontopoi/StationeryAndStampsAndTagsAndLabels -->


    <owl:Class rdf:about="https://www.theworldavatar.com/kg/ontopoi/StationeryAndStampsAndTagsAndLabels">
        <rdfs:subClassOf rdf:resource="https://www.theworldavatar.com/kg/ontopoi/IndustrialProducts"/>
        <rdfs:comment>Stationery, stamps, tags and labels is a subcategory of industrial products</rdfs:comment>
        <rdfs:isDefinedBy rdf:resource="https://www.theworldavatar.com/kg/ontopoi"/>
        <rdfs:label>Stationery, stamps, tags and labels</rdfs:label>
    </owl:Class>
    


    <!-- https://www.theworldavatar.com/kg/ontopoi/StocksAndSharesAndUnitTrusts -->


    <owl:Class rdf:about="https://www.theworldavatar.com/kg/ontopoi/StocksAndSharesAndUnitTrusts">
        <rdfs:subClassOf rdf:resource="https://www.theworldavatar.com/kg/ontopoi/LegalAndFinancial"/>
        <rdfs:comment>Stocks, shares and unit trusts is a subcategory of legal and financial</rdfs:comment>
        <rdfs:isDefinedBy rdf:resource="https://www.theworldavatar.com/kg/ontopoi"/>
        <rdfs:label>Stocks, shares and unit trusts</rdfs:label>
    </owl:Class>
    


    <!-- https://www.theworldavatar.com/kg/ontopoi/StoneQuarryingAndPreparation -->


    <owl:Class rdf:about="https://www.theworldavatar.com/kg/ontopoi/StoneQuarryingAndPreparation">
        <rdfs:subClassOf rdf:resource="https://www.theworldavatar.com/kg/ontopoi/ExtractiveIndustries"/>
        <rdfs:comment>Stone quarrying and preparation is a subcategory of extractive industries</rdfs:comment>
        <rdfs:isDefinedBy rdf:resource="https://www.theworldavatar.com/kg/ontopoi"/>
        <rdfs:label>Stone quarrying and preparation</rdfs:label>
    </owl:Class>
    


    <!-- https://www.theworldavatar.com/kg/ontopoi/StructuralEngineers -->


    <owl:Class rdf:about="https://www.theworldavatar.com/kg/ontopoi/StructuralEngineers">
        <rdfs:subClassOf rdf:resource="https://www.theworldavatar.com/kg/ontopoi/EngineeringServices"/>
        <rdfs:comment>Structural engineers is a subcategory of engineering services</rdfs:comment>
        <rdfs:isDefinedBy rdf:resource="https://www.theworldavatar.com/kg/ontopoi"/>
        <rdfs:label>Structural engineers</rdfs:label>
    </owl:Class>
    


    <!-- https://www.theworldavatar.com/kg/ontopoi/SupermarketChains -->


    <owl:Class rdf:about="https://www.theworldavatar.com/kg/ontopoi/SupermarketChains">
        <rdfs:subClassOf rdf:resource="https://www.theworldavatar.com/kg/ontopoi/FoodAndDrinkAndMultiItemRetail"/>
        <rdfs:comment>Supermarket chains is a subcategory of food, drink and multi item retail</rdfs:comment>
        <rdfs:isDefinedBy rdf:resource="https://www.theworldavatar.com/kg/ontopoi"/>
        <rdfs:label>Supermarket chains</rdfs:label>
    </owl:Class>
    


    <!-- https://www.theworldavatar.com/kg/ontopoi/SurgeonsAndCosmeticSurgeries -->


    <owl:Class rdf:about="https://www.theworldavatar.com/kg/ontopoi/SurgeonsAndCosmeticSurgeries">
        <rdfs:subClassOf rdf:resource="https://www.theworldavatar.com/kg/ontopoi/HealthPractitionersAndEstablishments"/>
        <rdfs:comment>Surgeons and cosmetic surgeries is a subcategory of health practitioners and establishments</rdfs:comment>
        <rdfs:isDefinedBy rdf:resource="https://www.theworldavatar.com/kg/ontopoi"/>
        <rdfs:label>Surgeons and cosmetic surgeries</rdfs:label>
    </owl:Class>
    


    <!-- https://www.theworldavatar.com/kg/ontopoi/SurplusGoods -->


    <owl:Class rdf:about="https://www.theworldavatar.com/kg/ontopoi/SurplusGoods">
        <rdfs:subClassOf rdf:resource="https://www.theworldavatar.com/kg/ontopoi/HouseholdAndOfficeAndLeisureAndGarden"/>
        <rdfs:comment>Surplus goods is a subcategory of household, office, leisure and garden</rdfs:comment>
        <rdfs:isDefinedBy rdf:resource="https://www.theworldavatar.com/kg/ontopoi"/>
        <rdfs:label>Surplus goods</rdfs:label>
    </owl:Class>
    


    <!-- https://www.theworldavatar.com/kg/ontopoi/SwimmingPools -->


    <owl:Class rdf:about="https://www.theworldavatar.com/kg/ontopoi/SwimmingPools">
        <rdfs:subClassOf rdf:resource="https://www.theworldavatar.com/kg/ontopoi/SportsComplex"/>
        <rdfs:comment>Swimming pools is a subcategory of sports complex</rdfs:comment>
        <rdfs:isDefinedBy rdf:resource="https://www.theworldavatar.com/kg/ontopoi"/>
        <rdfs:label>Swimming pools</rdfs:label>
    </owl:Class>
    


    <!-- https://www.theworldavatar.com/kg/ontopoi/TailoringAndClothingAlteration -->


    <owl:Class rdf:about="https://www.theworldavatar.com/kg/ontopoi/TailoringAndClothingAlteration">
        <rdfs:subClassOf rdf:resource="https://www.theworldavatar.com/kg/ontopoi/PersonalAndConsumerAndOtherServices"/>
        <rdfs:comment>Tailoring and clothing alteration is a subcategory of personal, consumer and other services</rdfs:comment>
        <rdfs:isDefinedBy rdf:resource="https://www.theworldavatar.com/kg/ontopoi"/>
        <rdfs:label>Tailoring and clothing alteration</rdfs:label>
    </owl:Class>
    


    <!-- https://www.theworldavatar.com/kg/ontopoi/TarnsAndPoolsAndMeres -->


    <owl:Class rdf:about="https://www.theworldavatar.com/kg/ontopoi/TarnsAndPoolsAndMeres">
        <rdfs:subClassOf rdf:resource="https://www.theworldavatar.com/kg/ontopoi/BodiesOfWater"/>
        <rdfs:comment>Tarns, pools and meres is a subcategory of bodies of water</rdfs:comment>
        <rdfs:isDefinedBy rdf:resource="https://www.theworldavatar.com/kg/ontopoi"/>
        <rdfs:label>Tarns, pools and meres</rdfs:label>
    </owl:Class>
    


    <!-- https://www.theworldavatar.com/kg/ontopoi/TattooingAndPiercingServices -->


    <owl:Class rdf:about="https://www.theworldavatar.com/kg/ontopoi/TattooingAndPiercingServices">
        <rdfs:subClassOf rdf:resource="https://www.theworldavatar.com/kg/ontopoi/PersonalAndConsumerAndOtherServices"/>
        <rdfs:comment>Tattooing and piercing services is a subcategory of personal, consumer and other services</rdfs:comment>
        <rdfs:isDefinedBy rdf:resource="https://www.theworldavatar.com/kg/ontopoi"/>
        <rdfs:label>Tattooing and piercing services</rdfs:label>
    </owl:Class>
    


    <!-- https://www.theworldavatar.com/kg/ontopoi/TaxiRanks -->


    <owl:Class rdf:about="https://www.theworldavatar.com/kg/ontopoi/TaxiRanks">
        <rdfs:subClassOf rdf:resource="https://www.theworldavatar.com/kg/ontopoi/PublicTransportAndStationsAndInfrastructure"/>
        <rdfs:comment>Taxi ranks is a subcategory of public transport, stations and infrastructure</rdfs:comment>
        <rdfs:isDefinedBy rdf:resource="https://www.theworldavatar.com/kg/ontopoi"/>
        <rdfs:label>Taxi ranks</rdfs:label>
    </owl:Class>
    


    <!-- https://www.theworldavatar.com/kg/ontopoi/TaxiServices -->


    <owl:Class rdf:about="https://www.theworldavatar.com/kg/ontopoi/TaxiServices">
        <rdfs:subClassOf rdf:resource="https://www.theworldavatar.com/kg/ontopoi/TransportAndStorageAndDelivery"/>
        <rdfs:comment>Taxi services is a subcategory of transport, storage and delivery</rdfs:comment>
        <rdfs:isDefinedBy rdf:resource="https://www.theworldavatar.com/kg/ontopoi"/>
        <rdfs:label>Taxi services</rdfs:label>
    </owl:Class>
    


    <!-- https://www.theworldavatar.com/kg/ontopoi/TeaAndCoffeeMerchants -->


    <owl:Class rdf:about="https://www.theworldavatar.com/kg/ontopoi/TeaAndCoffeeMerchants">
        <rdfs:subClassOf rdf:resource="https://www.theworldavatar.com/kg/ontopoi/FoodAndDrinkAndMultiItemRetail"/>
        <rdfs:comment>Tea and coffee merchants is a subcategory of food, drink and multi item retail</rdfs:comment>
        <rdfs:isDefinedBy rdf:resource="https://www.theworldavatar.com/kg/ontopoi"/>
        <rdfs:label>Tea and coffee merchants</rdfs:label>
    </owl:Class>
    


    <!-- https://www.theworldavatar.com/kg/ontopoi/TelecommunicationsCompanies -->


    <owl:Class rdf:about="https://www.theworldavatar.com/kg/ontopoi/TelecommunicationsCompanies">
        <rdfs:subClassOf rdf:resource="https://www.theworldavatar.com/kg/ontopoi/InfrastructureAndFacilities"/>
        <rdfs:comment>Telecommunications companies is a subcategory of infrastructure and facilities</rdfs:comment>
        <rdfs:isDefinedBy rdf:resource="https://www.theworldavatar.com/kg/ontopoi"/>
        <rdfs:label>Telecommunications companies</rdfs:label>
    </owl:Class>
    


    <!-- https://www.theworldavatar.com/kg/ontopoi/TelecommunicationsConsultants -->


    <owl:Class rdf:about="https://www.theworldavatar.com/kg/ontopoi/TelecommunicationsConsultants">
        <rdfs:subClassOf rdf:resource="https://www.theworldavatar.com/kg/ontopoi/Consultancies"/>
        <rdfs:comment>Telecommunications consultants is a subcategory of consultancies</rdfs:comment>
        <rdfs:isDefinedBy rdf:resource="https://www.theworldavatar.com/kg/ontopoi"/>
        <rdfs:label>Telecommunications consultants</rdfs:label>
    </owl:Class>
    


    <!-- https://www.theworldavatar.com/kg/ontopoi/TelecommunicationsFeatures -->


    <owl:Class rdf:about="https://www.theworldavatar.com/kg/ontopoi/TelecommunicationsFeatures">
        <rdfs:subClassOf rdf:resource="https://www.theworldavatar.com/kg/ontopoi/InfrastructureAndFacilities"/>
        <rdfs:comment>Telecommunications features is a subcategory of infrastructure and facilities</rdfs:comment>
        <rdfs:isDefinedBy rdf:resource="https://www.theworldavatar.com/kg/ontopoi"/>
        <rdfs:label>Telecommunications features</rdfs:label>
    </owl:Class>
    


    <!-- https://www.theworldavatar.com/kg/ontopoi/TelephoneAndTelexAndFaxServices -->


    <owl:Class rdf:about="https://www.theworldavatar.com/kg/ontopoi/TelephoneAndTelexAndFaxServices">
        <rdfs:subClassOf rdf:resource="https://www.theworldavatar.com/kg/ontopoi/ItAndAdvertisingAndMarketingAndMediaServiceS"/>
        <rdfs:comment>Telephone, telex and fax services is a subcategory of it, advertising, marketing and media service s</rdfs:comment>
        <rdfs:isDefinedBy rdf:resource="https://www.theworldavatar.com/kg/ontopoi"/>
        <rdfs:label>Telephone, telex and fax services</rdfs:label>
    </owl:Class>
    


    <!-- https://www.theworldavatar.com/kg/ontopoi/TelephonesAndTelephoneCards -->


    <owl:Class rdf:about="https://www.theworldavatar.com/kg/ontopoi/TelephonesAndTelephoneCards">
        <rdfs:subClassOf rdf:resource="https://www.theworldavatar.com/kg/ontopoi/HouseholdAndOfficeAndLeisureAndGarden"/>
        <rdfs:comment>Telephones and telephone cards is a subcategory of household, office, leisure and garden</rdfs:comment>
        <rdfs:isDefinedBy rdf:resource="https://www.theworldavatar.com/kg/ontopoi"/>
        <rdfs:label>Telephones and telephone cards</rdfs:label>
    </owl:Class>
    


    <!-- https://www.theworldavatar.com/kg/ontopoi/TelevisionAndRadioServices -->


    <owl:Class rdf:about="https://www.theworldavatar.com/kg/ontopoi/TelevisionAndRadioServices">
        <rdfs:subClassOf rdf:resource="https://www.theworldavatar.com/kg/ontopoi/ItAndAdvertisingAndMarketingAndMediaServiceS"/>
        <rdfs:comment>Television and radio services is a subcategory of it, advertising, marketing and media service s</rdfs:comment>
        <rdfs:isDefinedBy rdf:resource="https://www.theworldavatar.com/kg/ontopoi"/>
        <rdfs:label>Television and radio services</rdfs:label>
    </owl:Class>
    


    <!-- https://www.theworldavatar.com/kg/ontopoi/TennisFacilities -->


    <owl:Class rdf:about="https://www.theworldavatar.com/kg/ontopoi/TennisFacilities">
        <rdfs:subClassOf rdf:resource="https://www.theworldavatar.com/kg/ontopoi/SportsComplex"/>
        <rdfs:comment>Tennis facilities is a subcategory of sports complex</rdfs:comment>
        <rdfs:isDefinedBy rdf:resource="https://www.theworldavatar.com/kg/ontopoi"/>
        <rdfs:label>Tennis facilities</rdfs:label>
    </owl:Class>
    


    <!-- https://www.theworldavatar.com/kg/ontopoi/TentsAndMarqueesAndCampingEquipment -->


    <owl:Class rdf:about="https://www.theworldavatar.com/kg/ontopoi/TentsAndMarqueesAndCampingEquipment">
        <rdfs:subClassOf rdf:resource="https://www.theworldavatar.com/kg/ontopoi/ConsumerProducts"/>
        <rdfs:comment>Tents, marquees and camping equipment is a subcategory of consumer products</rdfs:comment>
        <rdfs:isDefinedBy rdf:resource="https://www.theworldavatar.com/kg/ontopoi"/>
        <rdfs:label>Tents, marquees and camping equipment</rdfs:label>
    </owl:Class>
    


    <!-- https://www.theworldavatar.com/kg/ontopoi/TestingAndAnalysisServices -->


    <owl:Class rdf:about="https://www.theworldavatar.com/kg/ontopoi/TestingAndAnalysisServices">
        <rdfs:subClassOf rdf:resource="https://www.theworldavatar.com/kg/ontopoi/ResearchAndDesign"/>
        <rdfs:comment>Testing and analysis services is a subcategory of research and design</rdfs:comment>
        <rdfs:isDefinedBy rdf:resource="https://www.theworldavatar.com/kg/ontopoi"/>
        <rdfs:label>Testing and analysis services</rdfs:label>
    </owl:Class>
    


    <!-- https://www.theworldavatar.com/kg/ontopoi/TextilesAndFabricsAndSilkAndMachinery -->


    <owl:Class rdf:about="https://www.theworldavatar.com/kg/ontopoi/TextilesAndFabricsAndSilkAndMachinery">
        <rdfs:subClassOf rdf:resource="https://www.theworldavatar.com/kg/ontopoi/IndustrialProducts"/>
        <rdfs:comment>Textiles, fabrics, silk and machinery is a subcategory of industrial products</rdfs:comment>
        <rdfs:isDefinedBy rdf:resource="https://www.theworldavatar.com/kg/ontopoi"/>
        <rdfs:label>Textiles, fabrics, silk and machinery</rdfs:label>
    </owl:Class>
    


    <!-- https://www.theworldavatar.com/kg/ontopoi/TheatresAndConcertHalls -->


    <owl:Class rdf:about="https://www.theworldavatar.com/kg/ontopoi/TheatresAndConcertHalls">
        <rdfs:subClassOf rdf:resource="https://www.theworldavatar.com/kg/ontopoi/VenuesAndStageAndScreen"/>
        <rdfs:comment>Theatres and concert halls is a subcategory of venues, stage and screen</rdfs:comment>
        <rdfs:isDefinedBy rdf:resource="https://www.theworldavatar.com/kg/ontopoi"/>
        <rdfs:label>Theatres and concert halls</rdfs:label>
    </owl:Class>
    


    <!-- https://www.theworldavatar.com/kg/ontopoi/ThemeAndAdventureParks -->


    <owl:Class rdf:about="https://www.theworldavatar.com/kg/ontopoi/ThemeAndAdventureParks">
        <rdfs:subClassOf rdf:resource="https://www.theworldavatar.com/kg/ontopoi/Tourism"/>
        <rdfs:comment>Theme and adventure parks is a subcategory of tourism</rdfs:comment>
        <rdfs:isDefinedBy rdf:resource="https://www.theworldavatar.com/kg/ontopoi"/>
        <rdfs:label>Theme and adventure parks</rdfs:label>
    </owl:Class>
    


    <!-- https://www.theworldavatar.com/kg/ontopoi/Timeshare -->


    <owl:Class rdf:about="https://www.theworldavatar.com/kg/ontopoi/Timeshare">
        <rdfs:subClassOf rdf:resource="https://www.theworldavatar.com/kg/ontopoi/Accommodation"/>
        <rdfs:comment>Timeshare is a subcategory of accommodation</rdfs:comment>
        <rdfs:isDefinedBy rdf:resource="https://www.theworldavatar.com/kg/ontopoi"/>
        <rdfs:label>Timeshare</rdfs:label>
    </owl:Class>
    


    <!-- https://www.theworldavatar.com/kg/ontopoi/TobaccoProducts -->


    <owl:Class rdf:about="https://www.theworldavatar.com/kg/ontopoi/TobaccoProducts">
        <rdfs:subClassOf rdf:resource="https://www.theworldavatar.com/kg/ontopoi/ConsumerProducts"/>
        <rdfs:comment>Tobacco products is a subcategory of consumer products</rdfs:comment>
        <rdfs:isDefinedBy rdf:resource="https://www.theworldavatar.com/kg/ontopoi"/>
        <rdfs:label>Tobacco products</rdfs:label>
    </owl:Class>
    


    <!-- https://www.theworldavatar.com/kg/ontopoi/ToolRepairs -->


    <owl:Class rdf:about="https://www.theworldavatar.com/kg/ontopoi/ToolRepairs">
        <rdfs:subClassOf rdf:resource="https://www.theworldavatar.com/kg/ontopoi/RepairAndServicing"/>
        <rdfs:comment>Tool repairs is a subcategory of repair and servicing</rdfs:comment>
        <rdfs:isDefinedBy rdf:resource="https://www.theworldavatar.com/kg/ontopoi"/>
        <rdfs:label>Tool repairs</rdfs:label>
    </owl:Class>
    


    <!-- https://www.theworldavatar.com/kg/ontopoi/ToolsIncludingMachineShops -->


    <owl:Class rdf:about="https://www.theworldavatar.com/kg/ontopoi/ToolsIncludingMachineShops">
        <rdfs:subClassOf rdf:resource="https://www.theworldavatar.com/kg/ontopoi/IndustrialProducts"/>
        <rdfs:comment>Tools including machine shops is a subcategory of industrial products</rdfs:comment>
        <rdfs:isDefinedBy rdf:resource="https://www.theworldavatar.com/kg/ontopoi"/>
        <rdfs:label>Tools including machine shops</rdfs:label>
    </owl:Class>
    


    <!-- https://www.theworldavatar.com/kg/ontopoi/Tourism -->


    <owl:Class rdf:about="https://www.theworldavatar.com/kg/ontopoi/Tourism">
        <rdfs:subClassOf rdf:resource="https://www.theworldavatar.com/kg/ontopoi/Attractions"/>
        <rdfs:comment>Tourism is a subcategory of attractions</rdfs:comment>
        <rdfs:isDefinedBy rdf:resource="https://www.theworldavatar.com/kg/ontopoi"/>
        <rdfs:label>Tourism</rdfs:label>
    </owl:Class>
    


    <!-- https://www.theworldavatar.com/kg/ontopoi/TrafficManagementAndTransport-RelatedConsultants -->


    <owl:Class rdf:about="https://www.theworldavatar.com/kg/ontopoi/TrafficManagementAndTransport-RelatedConsultants">
        <rdfs:subClassOf rdf:resource="https://www.theworldavatar.com/kg/ontopoi/Consultancies"/>
        <rdfs:comment>Traffic management and transport-related consultants is a subcategory of consultancies</rdfs:comment>
        <rdfs:isDefinedBy rdf:resource="https://www.theworldavatar.com/kg/ontopoi"/>
        <rdfs:label>Traffic management and transport-related consultants</rdfs:label>
    </owl:Class>
    


    <!-- https://www.theworldavatar.com/kg/ontopoi/TrainingProvidersAndCentres -->


    <owl:Class rdf:about="https://www.theworldavatar.com/kg/ontopoi/TrainingProvidersAndCentres">
        <rdfs:subClassOf rdf:resource="https://www.theworldavatar.com/kg/ontopoi/RecreationalAndVocationalEducation"/>
        <rdfs:comment>Training providers and centres is a subcategory of recreational and vocational education</rdfs:comment>
        <rdfs:isDefinedBy rdf:resource="https://www.theworldavatar.com/kg/ontopoi"/>
        <rdfs:label>Training providers and centres</rdfs:label>
    </owl:Class>
    


    <!-- https://www.theworldavatar.com/kg/ontopoi/TramAndMetroAndLightRailwayStationsAndStops -->


    <owl:Class rdf:about="https://www.theworldavatar.com/kg/ontopoi/TramAndMetroAndLightRailwayStationsAndStops">
        <rdfs:subClassOf rdf:resource="https://www.theworldavatar.com/kg/ontopoi/PublicTransportAndStationsAndInfrastructure"/>
        <rdfs:comment>Tram, metro and light railway stations and stops is a subcategory of public transport, stations and infrastructure</rdfs:comment>
        <rdfs:isDefinedBy rdf:resource="https://www.theworldavatar.com/kg/ontopoi"/>
        <rdfs:label>Tram, metro and light railway stations and stops</rdfs:label>
    </owl:Class>
    


    <!-- https://www.theworldavatar.com/kg/ontopoi/Transport -->


    <owl:Class rdf:about="https://www.theworldavatar.com/kg/ontopoi/Transport">
        <rdfs:subClassOf rdf:resource="https://www.theworldavatar.com/kg/ontopoi/PointOfInterest"/>
        <rdfs:comment>Systems or infrastructure used to move people, goods, and services from one location to another</rdfs:comment>
        <rdfs:isDefinedBy rdf:resource="https://www.theworldavatar.com/kg/ontopoi"/>
        <rdfs:label>Transport</rdfs:label>
    </owl:Class>
    


    <!-- https://www.theworldavatar.com/kg/ontopoi/TransportAndStorageAndDelivery -->


    <owl:Class rdf:about="https://www.theworldavatar.com/kg/ontopoi/TransportAndStorageAndDelivery">
        <rdfs:subClassOf rdf:resource="https://www.theworldavatar.com/kg/ontopoi/CommercialServices"/>
        <rdfs:comment>Transport, storage and delivery is a subcategory of commercial services</rdfs:comment>
        <rdfs:isDefinedBy rdf:resource="https://www.theworldavatar.com/kg/ontopoi"/>
        <rdfs:label>Transport, storage and delivery</rdfs:label>
    </owl:Class>
    


    <!-- https://www.theworldavatar.com/kg/ontopoi/TravelAgencies -->


    <owl:Class rdf:about="https://www.theworldavatar.com/kg/ontopoi/TravelAgencies">
        <rdfs:subClassOf rdf:resource="https://www.theworldavatar.com/kg/ontopoi/HouseholdAndOfficeAndLeisureAndGarden"/>
        <rdfs:comment>Travel agencies is a subcategory of household, office, leisure and garden</rdfs:comment>
        <rdfs:isDefinedBy rdf:resource="https://www.theworldavatar.com/kg/ontopoi"/>
        <rdfs:label>Travel agencies</rdfs:label>
    </owl:Class>
    


    <!-- https://www.theworldavatar.com/kg/ontopoi/Tribunals -->


    <owl:Class rdf:about="https://www.theworldavatar.com/kg/ontopoi/Tribunals">
        <rdfs:subClassOf rdf:resource="https://www.theworldavatar.com/kg/ontopoi/CentralAndLocalGovernment"/>
        <rdfs:comment>Tribunals is a subcategory of central and local government</rdfs:comment>
        <rdfs:isDefinedBy rdf:resource="https://www.theworldavatar.com/kg/ontopoi"/>
        <rdfs:label>Tribunals</rdfs:label>
    </owl:Class>
    


    <!-- https://www.theworldavatar.com/kg/ontopoi/TrigonometricPoints -->


    <owl:Class rdf:about="https://www.theworldavatar.com/kg/ontopoi/TrigonometricPoints">
        <rdfs:subClassOf rdf:resource="https://www.theworldavatar.com/kg/ontopoi/LandscapeFeatures"/>
        <rdfs:comment>Trigonometric points is a subcategory of landscape features</rdfs:comment>
        <rdfs:isDefinedBy rdf:resource="https://www.theworldavatar.com/kg/ontopoi"/>
        <rdfs:label>Trigonometric points</rdfs:label>
    </owl:Class>
    


    <!-- https://www.theworldavatar.com/kg/ontopoi/TrophiesAndEngravingServices -->


    <owl:Class rdf:about="https://www.theworldavatar.com/kg/ontopoi/TrophiesAndEngravingServices">
        <rdfs:subClassOf rdf:resource="https://www.theworldavatar.com/kg/ontopoi/PersonalAndConsumerAndOtherServices"/>
        <rdfs:comment>Trophies and engraving services is a subcategory of personal, consumer and other services</rdfs:comment>
        <rdfs:isDefinedBy rdf:resource="https://www.theworldavatar.com/kg/ontopoi"/>
        <rdfs:label>Trophies and engraving services</rdfs:label>
    </owl:Class>
    


    <!-- https://www.theworldavatar.com/kg/ontopoi/UndergroundNetworkStations -->


    <owl:Class rdf:about="https://www.theworldavatar.com/kg/ontopoi/UndergroundNetworkStations">
        <rdfs:subClassOf rdf:resource="https://www.theworldavatar.com/kg/ontopoi/PublicTransportAndStationsAndInfrastructure"/>
        <rdfs:comment>Underground network stations is a subcategory of public transport, stations and infrastructure</rdfs:comment>
        <rdfs:isDefinedBy rdf:resource="https://www.theworldavatar.com/kg/ontopoi"/>
        <rdfs:label>Underground network stations</rdfs:label>
    </owl:Class>
    


    <!-- https://www.theworldavatar.com/kg/ontopoi/UnspecifiedAndOtherAttractions -->


    <owl:Class rdf:about="https://www.theworldavatar.com/kg/ontopoi/UnspecifiedAndOtherAttractions">
        <rdfs:subClassOf rdf:resource="https://www.theworldavatar.com/kg/ontopoi/Tourism"/>
        <rdfs:comment>Unspecified and other attractions is a subcategory of tourism</rdfs:comment>
        <rdfs:isDefinedBy rdf:resource="https://www.theworldavatar.com/kg/ontopoi"/>
        <rdfs:label>Unspecified and other attractions</rdfs:label>
    </owl:Class>
    


    <!-- https://www.theworldavatar.com/kg/ontopoi/UnspecifiedAndOtherSchools -->


    <owl:Class rdf:about="https://www.theworldavatar.com/kg/ontopoi/UnspecifiedAndOtherSchools">
        <rdfs:subClassOf rdf:resource="https://www.theworldavatar.com/kg/ontopoi/PrimaryAndSecondaryAndTertiaryEducation"/>
        <rdfs:comment>Unspecified and other schools is a subcategory of primary, secondary and tertiary education</rdfs:comment>
        <rdfs:isDefinedBy rdf:resource="https://www.theworldavatar.com/kg/ontopoi"/>
        <rdfs:label>Unspecified and other schools</rdfs:label>
    </owl:Class>
    


    <!-- https://www.theworldavatar.com/kg/ontopoi/UnspecifiedQuarriesOrMines -->


    <owl:Class rdf:about="https://www.theworldavatar.com/kg/ontopoi/UnspecifiedQuarriesOrMines">
        <rdfs:subClassOf rdf:resource="https://www.theworldavatar.com/kg/ontopoi/ExtractiveIndustries"/>
        <rdfs:comment>Unspecified quarries or mines is a subcategory of extractive industries</rdfs:comment>
        <rdfs:isDefinedBy rdf:resource="https://www.theworldavatar.com/kg/ontopoi"/>
        <rdfs:label>Unspecified quarries or mines</rdfs:label>
    </owl:Class>
    


    <!-- https://www.theworldavatar.com/kg/ontopoi/UnspecifiedWorksOrFactories -->


    <owl:Class rdf:about="https://www.theworldavatar.com/kg/ontopoi/UnspecifiedWorksOrFactories">
        <rdfs:subClassOf rdf:resource="https://www.theworldavatar.com/kg/ontopoi/IndustrialFeatures"/>
        <rdfs:comment>Unspecified works or factories is a subcategory of industrial features</rdfs:comment>
        <rdfs:isDefinedBy rdf:resource="https://www.theworldavatar.com/kg/ontopoi"/>
        <rdfs:label>Unspecified works or factories</rdfs:label>
    </owl:Class>
    


    <!-- https://www.theworldavatar.com/kg/ontopoi/UtilityCompaniesAndBrokers -->


    <owl:Class rdf:about="https://www.theworldavatar.com/kg/ontopoi/UtilityCompaniesAndBrokers">
        <rdfs:subClassOf rdf:resource="https://www.theworldavatar.com/kg/ontopoi/InfrastructureAndFacilities"/>
        <rdfs:comment>Utility companies and brokers is a subcategory of infrastructure and facilities</rdfs:comment>
        <rdfs:isDefinedBy rdf:resource="https://www.theworldavatar.com/kg/ontopoi"/>
        <rdfs:label>Utility companies and brokers</rdfs:label>
    </owl:Class>
    


    <!-- https://www.theworldavatar.com/kg/ontopoi/VehicleAuctions -->


    <owl:Class rdf:about="https://www.theworldavatar.com/kg/ontopoi/VehicleAuctions">
        <rdfs:subClassOf rdf:resource="https://www.theworldavatar.com/kg/ontopoi/Motoring"/>
        <rdfs:comment>Vehicle auctions is a subcategory of motoring</rdfs:comment>
        <rdfs:isDefinedBy rdf:resource="https://www.theworldavatar.com/kg/ontopoi"/>
        <rdfs:label>Vehicle auctions</rdfs:label>
    </owl:Class>
    


    <!-- https://www.theworldavatar.com/kg/ontopoi/VehicleBodybuilders -->


    <owl:Class rdf:about="https://www.theworldavatar.com/kg/ontopoi/VehicleBodybuilders">
        <rdfs:subClassOf rdf:resource="https://www.theworldavatar.com/kg/ontopoi/IndustrialProducts"/>
        <rdfs:comment>Vehicle bodybuilders is a subcategory of industrial products</rdfs:comment>
        <rdfs:isDefinedBy rdf:resource="https://www.theworldavatar.com/kg/ontopoi"/>
        <rdfs:label>Vehicle bodybuilders</rdfs:label>
    </owl:Class>
    


    <!-- https://www.theworldavatar.com/kg/ontopoi/VehicleBreakdownAndRecoveryServices -->


    <owl:Class rdf:about="https://www.theworldavatar.com/kg/ontopoi/VehicleBreakdownAndRecoveryServices">
        <rdfs:subClassOf rdf:resource="https://www.theworldavatar.com/kg/ontopoi/PersonalAndConsumerAndOtherServices"/>
        <rdfs:comment>Vehicle breakdown and recovery services is a subcategory of personal, consumer and other services</rdfs:comment>
        <rdfs:isDefinedBy rdf:resource="https://www.theworldavatar.com/kg/ontopoi"/>
        <rdfs:label>Vehicle breakdown and recovery services</rdfs:label>
    </owl:Class>
    


    <!-- https://www.theworldavatar.com/kg/ontopoi/VehicleCleaningServices -->


    <owl:Class rdf:about="https://www.theworldavatar.com/kg/ontopoi/VehicleCleaningServices">
        <rdfs:subClassOf rdf:resource="https://www.theworldavatar.com/kg/ontopoi/PersonalAndConsumerAndOtherServices"/>
        <rdfs:comment>Vehicle cleaning services is a subcategory of personal, consumer and other services</rdfs:comment>
        <rdfs:isDefinedBy rdf:resource="https://www.theworldavatar.com/kg/ontopoi"/>
        <rdfs:label>Vehicle cleaning services</rdfs:label>
    </owl:Class>
    


    <!-- https://www.theworldavatar.com/kg/ontopoi/VehicleComponents -->


    <owl:Class rdf:about="https://www.theworldavatar.com/kg/ontopoi/VehicleComponents">
        <rdfs:subClassOf rdf:resource="https://www.theworldavatar.com/kg/ontopoi/IndustrialProducts"/>
        <rdfs:comment>Vehicle components is a subcategory of industrial products</rdfs:comment>
        <rdfs:isDefinedBy rdf:resource="https://www.theworldavatar.com/kg/ontopoi"/>
        <rdfs:label>Vehicle components</rdfs:label>
    </owl:Class>
    


    <!-- https://www.theworldavatar.com/kg/ontopoi/VehicleHireAndRental -->


    <owl:Class rdf:about="https://www.theworldavatar.com/kg/ontopoi/VehicleHireAndRental">
        <rdfs:subClassOf rdf:resource="https://www.theworldavatar.com/kg/ontopoi/HireServices"/>
        <rdfs:comment>Vehicle hire and rental is a subcategory of hire services</rdfs:comment>
        <rdfs:isDefinedBy rdf:resource="https://www.theworldavatar.com/kg/ontopoi"/>
        <rdfs:label>Vehicle hire and rental</rdfs:label>
    </owl:Class>
    


    <!-- https://www.theworldavatar.com/kg/ontopoi/VehiclePartsAndAccessories -->


    <owl:Class rdf:about="https://www.theworldavatar.com/kg/ontopoi/VehiclePartsAndAccessories">
        <rdfs:subClassOf rdf:resource="https://www.theworldavatar.com/kg/ontopoi/Motoring"/>
        <rdfs:comment>Vehicle parts and accessories is a subcategory of motoring</rdfs:comment>
        <rdfs:isDefinedBy rdf:resource="https://www.theworldavatar.com/kg/ontopoi"/>
        <rdfs:label>Vehicle parts and accessories</rdfs:label>
    </owl:Class>
    


    <!-- https://www.theworldavatar.com/kg/ontopoi/VehicleRepairAndTestingAndServicing -->


    <owl:Class rdf:about="https://www.theworldavatar.com/kg/ontopoi/VehicleRepairAndTestingAndServicing">
        <rdfs:subClassOf rdf:resource="https://www.theworldavatar.com/kg/ontopoi/RepairAndServicing"/>
        <rdfs:comment>Vehicle repair, testing and servicing is a subcategory of repair and servicing</rdfs:comment>
        <rdfs:isDefinedBy rdf:resource="https://www.theworldavatar.com/kg/ontopoi"/>
        <rdfs:label>Vehicle repair, testing and servicing</rdfs:label>
    </owl:Class>
    


    <!-- https://www.theworldavatar.com/kg/ontopoi/Vehicles -->


    <owl:Class rdf:about="https://www.theworldavatar.com/kg/ontopoi/Vehicles">
        <rdfs:subClassOf rdf:resource="https://www.theworldavatar.com/kg/ontopoi/IndustrialProducts"/>
        <rdfs:comment>Vehicles is a subcategory of industrial products</rdfs:comment>
        <rdfs:isDefinedBy rdf:resource="https://www.theworldavatar.com/kg/ontopoi"/>
        <rdfs:label>Vehicles</rdfs:label>
    </owl:Class>
    


    <!-- https://www.theworldavatar.com/kg/ontopoi/Velodromes -->


    <owl:Class rdf:about="https://www.theworldavatar.com/kg/ontopoi/Velodromes">
        <rdfs:subClassOf rdf:resource="https://www.theworldavatar.com/kg/ontopoi/SportsComplex"/>
        <rdfs:comment>Velodromes is a subcategory of sports complex</rdfs:comment>
        <rdfs:isDefinedBy rdf:resource="https://www.theworldavatar.com/kg/ontopoi"/>
        <rdfs:label>Velodromes</rdfs:label>
    </owl:Class>
    


    <!-- https://www.theworldavatar.com/kg/ontopoi/VenuesAndStageAndScreen -->


    <owl:Class rdf:about="https://www.theworldavatar.com/kg/ontopoi/VenuesAndStageAndScreen">
        <rdfs:subClassOf rdf:resource="https://www.theworldavatar.com/kg/ontopoi/SportAndEntertainment"/>
        <rdfs:comment>Venues, stage and screen is a subcategory of sport and entertainment</rdfs:comment>
        <rdfs:isDefinedBy rdf:resource="https://www.theworldavatar.com/kg/ontopoi"/>
        <rdfs:label>Venues, stage and screen</rdfs:label>
    </owl:Class>
    


    <!-- https://www.theworldavatar.com/kg/ontopoi/VeterinariansAndAnimalHospitals -->


    <owl:Class rdf:about="https://www.theworldavatar.com/kg/ontopoi/VeterinariansAndAnimalHospitals">
        <rdfs:subClassOf rdf:resource="https://www.theworldavatar.com/kg/ontopoi/AnimalWelfare"/>
        <rdfs:comment>Veterinarians and animal hospitals is a subcategory of animal welfare</rdfs:comment>
        <rdfs:isDefinedBy rdf:resource="https://www.theworldavatar.com/kg/ontopoi"/>
        <rdfs:label>Veterinarians and animal hospitals</rdfs:label>
    </owl:Class>
    


    <!-- https://www.theworldavatar.com/kg/ontopoi/VeterinaryPharmacies -->


    <owl:Class rdf:about="https://www.theworldavatar.com/kg/ontopoi/VeterinaryPharmacies">
        <rdfs:subClassOf rdf:resource="https://www.theworldavatar.com/kg/ontopoi/AnimalWelfare"/>
        <rdfs:comment>Veterinary pharmacies is a subcategory of animal welfare</rdfs:comment>
        <rdfs:isDefinedBy rdf:resource="https://www.theworldavatar.com/kg/ontopoi"/>
        <rdfs:label>Veterinary pharmacies</rdfs:label>
    </owl:Class>
    


    <!-- https://www.theworldavatar.com/kg/ontopoi/Viaducts -->


    <owl:Class rdf:about="https://www.theworldavatar.com/kg/ontopoi/Viaducts">
        <rdfs:subClassOf rdf:resource="https://www.theworldavatar.com/kg/ontopoi/RoadAndRail"/>
        <rdfs:comment>Viaducts is a subcategory of road and rail</rdfs:comment>
        <rdfs:isDefinedBy rdf:resource="https://www.theworldavatar.com/kg/ontopoi"/>
        <rdfs:label>Viaducts</rdfs:label>
    </owl:Class>
    


    <!-- https://www.theworldavatar.com/kg/ontopoi/Walk-InCentres -->


    <owl:Class rdf:about="https://www.theworldavatar.com/kg/ontopoi/Walk-InCentres">
        <rdfs:subClassOf rdf:resource="https://www.theworldavatar.com/kg/ontopoi/HealthPractitionersAndEstablishments"/>
        <rdfs:comment>Walk-in centres is a subcategory of health practitioners and establishments</rdfs:comment>
        <rdfs:isDefinedBy rdf:resource="https://www.theworldavatar.com/kg/ontopoi"/>
        <rdfs:label>Walk-in centres</rdfs:label>
    </owl:Class>
    


    <!-- https://www.theworldavatar.com/kg/ontopoi/Walking -->


    <owl:Class rdf:about="https://www.theworldavatar.com/kg/ontopoi/Walking">
        <rdfs:subClassOf rdf:resource="https://www.theworldavatar.com/kg/ontopoi/Transport"/>
        <rdfs:comment>Walking is a subcategory of transport</rdfs:comment>
        <rdfs:isDefinedBy rdf:resource="https://www.theworldavatar.com/kg/ontopoi"/>
        <rdfs:label>Walking</rdfs:label>
    </owl:Class>
    


    <!-- https://www.theworldavatar.com/kg/ontopoi/WasteCollectionAndProcessingAndDisposalEquipment -->


    <owl:Class rdf:about="https://www.theworldavatar.com/kg/ontopoi/WasteCollectionAndProcessingAndDisposalEquipment">
        <rdfs:subClassOf rdf:resource="https://www.theworldavatar.com/kg/ontopoi/IndustrialProducts"/>
        <rdfs:comment>Waste collection, processing and disposal equipment is a subcategory of industrial products</rdfs:comment>
        <rdfs:isDefinedBy rdf:resource="https://www.theworldavatar.com/kg/ontopoi"/>
        <rdfs:label>Waste collection, processing and disposal equipment</rdfs:label>
    </owl:Class>
    


    <!-- https://www.theworldavatar.com/kg/ontopoi/WastePaperMerchants -->


    <owl:Class rdf:about="https://www.theworldavatar.com/kg/ontopoi/WastePaperMerchants">
        <rdfs:subClassOf rdf:resource="https://www.theworldavatar.com/kg/ontopoi/RecyclingServices"/>
        <rdfs:comment>Waste paper merchants is a subcategory of recycling services</rdfs:comment>
        <rdfs:isDefinedBy rdf:resource="https://www.theworldavatar.com/kg/ontopoi"/>
        <rdfs:label>Waste paper merchants</rdfs:label>
    </owl:Class>
    


    <!-- https://www.theworldavatar.com/kg/ontopoi/WasteStorageAndProcessingAndDisposal -->


    <owl:Class rdf:about="https://www.theworldavatar.com/kg/ontopoi/WasteStorageAndProcessingAndDisposal">
        <rdfs:subClassOf rdf:resource="https://www.theworldavatar.com/kg/ontopoi/InfrastructureAndFacilities"/>
        <rdfs:comment>Waste storage, processing and disposal is a subcategory of infrastructure and facilities</rdfs:comment>
        <rdfs:isDefinedBy rdf:resource="https://www.theworldavatar.com/kg/ontopoi"/>
        <rdfs:label>Waste storage, processing and disposal</rdfs:label>
    </owl:Class>
    


    <!-- https://www.theworldavatar.com/kg/ontopoi/Water -->


    <owl:Class rdf:about="https://www.theworldavatar.com/kg/ontopoi/Water">
        <rdfs:subClassOf rdf:resource="https://www.theworldavatar.com/kg/ontopoi/Transport"/>
        <rdfs:comment>Water is a subcategory of transport</rdfs:comment>
        <rdfs:isDefinedBy rdf:resource="https://www.theworldavatar.com/kg/ontopoi"/>
        <rdfs:label>Water</rdfs:label>
    </owl:Class>
    


    <!-- https://www.theworldavatar.com/kg/ontopoi/WaterPumpingStations -->


    <owl:Class rdf:about="https://www.theworldavatar.com/kg/ontopoi/WaterPumpingStations">
        <rdfs:subClassOf rdf:resource="https://www.theworldavatar.com/kg/ontopoi/IndustrialFeatures"/>
        <rdfs:comment>Water pumping stations is a subcategory of industrial features</rdfs:comment>
        <rdfs:isDefinedBy rdf:resource="https://www.theworldavatar.com/kg/ontopoi"/>
        <rdfs:label>Water pumping stations</rdfs:label>
    </owl:Class>
    


    <!-- https://www.theworldavatar.com/kg/ontopoi/WaterSports -->


    <owl:Class rdf:about="https://www.theworldavatar.com/kg/ontopoi/WaterSports">
        <rdfs:subClassOf rdf:resource="https://www.theworldavatar.com/kg/ontopoi/OutdoorPursuits"/>
        <rdfs:comment>Water sports is a subcategory of outdoor pursuits</rdfs:comment>
        <rdfs:isDefinedBy rdf:resource="https://www.theworldavatar.com/kg/ontopoi"/>
        <rdfs:label>Water sports</rdfs:label>
    </owl:Class>
    


    <!-- https://www.theworldavatar.com/kg/ontopoi/WeatherServices -->


    <owl:Class rdf:about="https://www.theworldavatar.com/kg/ontopoi/WeatherServices">
        <rdfs:subClassOf rdf:resource="https://www.theworldavatar.com/kg/ontopoi/PersonalAndConsumerAndOtherServices"/>
        <rdfs:comment>Weather services is a subcategory of personal, consumer and other services</rdfs:comment>
        <rdfs:isDefinedBy rdf:resource="https://www.theworldavatar.com/kg/ontopoi"/>
        <rdfs:label>Weather services</rdfs:label>
    </owl:Class>
    


    <!-- https://www.theworldavatar.com/kg/ontopoi/WeddingServices -->


    <owl:Class rdf:about="https://www.theworldavatar.com/kg/ontopoi/WeddingServices">
        <rdfs:subClassOf rdf:resource="https://www.theworldavatar.com/kg/ontopoi/PersonalAndConsumerAndOtherServices"/>
        <rdfs:comment>Wedding services is a subcategory of personal, consumer and other services</rdfs:comment>
        <rdfs:isDefinedBy rdf:resource="https://www.theworldavatar.com/kg/ontopoi"/>
        <rdfs:label>Wedding services</rdfs:label>
    </owl:Class>
    


    <!-- https://www.theworldavatar.com/kg/ontopoi/Weighbridges -->


    <owl:Class rdf:about="https://www.theworldavatar.com/kg/ontopoi/Weighbridges">
        <rdfs:subClassOf rdf:resource="https://www.theworldavatar.com/kg/ontopoi/RoadAndRail"/>
        <rdfs:comment>Weighbridges is a subcategory of road and rail</rdfs:comment>
        <rdfs:isDefinedBy rdf:resource="https://www.theworldavatar.com/kg/ontopoi"/>
        <rdfs:label>Weighbridges</rdfs:label>
    </owl:Class>
    


    <!-- https://www.theworldavatar.com/kg/ontopoi/WeirsAndSluicesAndDams -->


    <owl:Class rdf:about="https://www.theworldavatar.com/kg/ontopoi/WeirsAndSluicesAndDams">
        <rdfs:subClassOf rdf:resource="https://www.theworldavatar.com/kg/ontopoi/Water"/>
        <rdfs:comment>Weirs, sluices and dams is a subcategory of water</rdfs:comment>
        <rdfs:isDefinedBy rdf:resource="https://www.theworldavatar.com/kg/ontopoi"/>
        <rdfs:label>Weirs, sluices and dams</rdfs:label>
    </owl:Class>
    


    <!-- https://www.theworldavatar.com/kg/ontopoi/Wi-FiHotspots -->


    <owl:Class rdf:about="https://www.theworldavatar.com/kg/ontopoi/Wi-FiHotspots">
        <rdfs:subClassOf rdf:resource="https://www.theworldavatar.com/kg/ontopoi/InfrastructureAndFacilities"/>
        <rdfs:comment>Wi-fi hotspots is a subcategory of infrastructure and facilities</rdfs:comment>
        <rdfs:isDefinedBy rdf:resource="https://www.theworldavatar.com/kg/ontopoi"/>
        <rdfs:label>Wi-Fi hotspots</rdfs:label>
    </owl:Class>
    


    <!-- https://www.theworldavatar.com/kg/ontopoi/WindowCleaners -->


    <owl:Class rdf:about="https://www.theworldavatar.com/kg/ontopoi/WindowCleaners">
        <rdfs:subClassOf rdf:resource="https://www.theworldavatar.com/kg/ontopoi/PersonalAndConsumerAndOtherServices"/>
        <rdfs:comment>Window cleaners is a subcategory of personal, consumer and other services</rdfs:comment>
        <rdfs:isDefinedBy rdf:resource="https://www.theworldavatar.com/kg/ontopoi"/>
        <rdfs:label>Window cleaners</rdfs:label>
    </owl:Class>
    


    <!-- https://www.theworldavatar.com/kg/ontopoi/WoodProductsIncludingCharcoalAndPaperAndCardAndBoard -->


    <owl:Class rdf:about="https://www.theworldavatar.com/kg/ontopoi/WoodProductsIncludingCharcoalAndPaperAndCardAndBoard">
        <rdfs:subClassOf rdf:resource="https://www.theworldavatar.com/kg/ontopoi/IndustrialProducts"/>
        <rdfs:comment>Wood products including charcoal, paper, card and board is a subcategory of industrial products</rdfs:comment>
        <rdfs:isDefinedBy rdf:resource="https://www.theworldavatar.com/kg/ontopoi"/>
        <rdfs:label>Wood products including charcoal, paper, card and board</rdfs:label>
    </owl:Class>
    


    <!-- https://www.theworldavatar.com/kg/ontopoi/Workwear -->


    <owl:Class rdf:about="https://www.theworldavatar.com/kg/ontopoi/Workwear">
        <rdfs:subClassOf rdf:resource="https://www.theworldavatar.com/kg/ontopoi/IndustrialProducts"/>
        <rdfs:comment>Workwear is a subcategory of industrial products</rdfs:comment>
        <rdfs:isDefinedBy rdf:resource="https://www.theworldavatar.com/kg/ontopoi"/>
        <rdfs:label>Workwear</rdfs:label>
    </owl:Class>
    


    <!-- https://www.theworldavatar.com/kg/ontopoi/X-RayServices -->


    <owl:Class rdf:about="https://www.theworldavatar.com/kg/ontopoi/X-RayServices">
        <rdfs:subClassOf rdf:resource="https://www.theworldavatar.com/kg/ontopoi/HealthSupportServices"/>
        <rdfs:comment>X-ray services is a subcategory of health support services</rdfs:comment>
        <rdfs:isDefinedBy rdf:resource="https://www.theworldavatar.com/kg/ontopoi"/>
        <rdfs:label>X-ray services</rdfs:label>
    </owl:Class>
    


    <!-- https://www.theworldavatar.com/kg/ontopoi/YouthAccommodation -->


    <owl:Class rdf:about="https://www.theworldavatar.com/kg/ontopoi/YouthAccommodation">
        <rdfs:subClassOf rdf:resource="https://www.theworldavatar.com/kg/ontopoi/Accommodation"/>
        <rdfs:comment>Youth accommodation is a subcategory of accommodation</rdfs:comment>
        <rdfs:isDefinedBy rdf:resource="https://www.theworldavatar.com/kg/ontopoi"/>
        <rdfs:label>Youth accommodation</rdfs:label>
    </owl:Class>
    


    <!-- https://www.theworldavatar.com/kg/ontopoi/YouthOrganisations -->


    <owl:Class rdf:about="https://www.theworldavatar.com/kg/ontopoi/YouthOrganisations">
        <rdfs:subClassOf rdf:resource="https://www.theworldavatar.com/kg/ontopoi/Organisations"/>
        <rdfs:comment>Youth organisations is a subcategory of organisations</rdfs:comment>
        <rdfs:isDefinedBy rdf:resource="https://www.theworldavatar.com/kg/ontopoi"/>
        <rdfs:label>Youth organisations</rdfs:label>
    </owl:Class>
    


    <!-- https://www.theworldavatar.com/kg/ontopoi/ZoosAndAnimalCollections -->


    <owl:Class rdf:about="https://www.theworldavatar.com/kg/ontopoi/ZoosAndAnimalCollections">
        <rdfs:subClassOf rdf:resource="https://www.theworldavatar.com/kg/ontopoi/BotanicalAndZoological"/>
        <rdfs:comment>Zoos and animal collections is a subcategory of botanical and zoological</rdfs:comment>
        <rdfs:isDefinedBy rdf:resource="https://www.theworldavatar.com/kg/ontopoi"/>
        <rdfs:label>Zoos and animal collections</rdfs:label>
    </owl:Class>
    


    <!-- https://www.theworldavatar.com/kg/ontopoi/AnimalBreeders(NotHorses) -->


    <owl:Class rdf:about="https://www.theworldavatar.com/kg/ontopoi/AnimalBreeders(NotHorses)">
        <rdfs:subClassOf rdf:resource="https://www.theworldavatar.com/kg/ontopoi/Farming"/>
        <rdfs:comment>Animal breeders (not horses) is a subcategory of farming</rdfs:comment>
        <rdfs:isDefinedBy rdf:resource="https://www.theworldavatar.com/kg/ontopoi"/>
        <rdfs:label>Animal breeders (not horses)</rdfs:label>
    </owl:Class>
    


    <!-- https://www.theworldavatar.com/kg/ontopoi/CookersAndStovesNon-Electrical -->


    <owl:Class rdf:about="https://www.theworldavatar.com/kg/ontopoi/CookersAndStovesNon-Electrical">
        <rdfs:subClassOf rdf:resource="https://www.theworldavatar.com/kg/ontopoi/ConsumerProducts"/>
        <rdfs:comment>Cookers and stoves  non-electrical is a subcategory of consumer products</rdfs:comment>
        <rdfs:isDefinedBy rdf:resource="https://www.theworldavatar.com/kg/ontopoi"/>
        <rdfs:label>Cookers and stoves  non-electrical</rdfs:label>
    </owl:Class>
    


    <!-- https://www.theworldavatar.com/kg/ontopoi/PaypointLocations -->


    <owl:Class rdf:about="https://www.theworldavatar.com/kg/ontopoi/PaypointLocations">
        <rdfs:subClassOf rdf:resource="https://www.theworldavatar.com/kg/ontopoi/LegalAndFinancial"/>
        <rdfs:comment>Paypoint locations is a subcategory of legal and financial</rdfs:comment>
        <rdfs:isDefinedBy rdf:resource="https://www.theworldavatar.com/kg/ontopoi"/>
        <rdfs:label>PayPoint locations</rdfs:label>
    </owl:Class>
    


    <!-- https://www.theworldavatar.com/kg/ontopoi/Railways(HeritageAndSteamAndMiniature) -->


    <owl:Class rdf:about="https://www.theworldavatar.com/kg/ontopoi/Railways(HeritageAndSteamAndMiniature)">
        <rdfs:subClassOf rdf:resource="https://www.theworldavatar.com/kg/ontopoi/Tourism"/>
        <rdfs:comment>Railways (heritage, steam and miniature) is a subcategory of tourism</rdfs:comment>
        <rdfs:isDefinedBy rdf:resource="https://www.theworldavatar.com/kg/ontopoi"/>
        <rdfs:label>Railways (heritage, steam and miniature)</rdfs:label>
    </owl:Class>
</rdf:RDF>



<!-- Generated by the OWL API (version 5.5.0.2023-01-14T12:41:38Z) https://github.com/owlcs/owlapi/ -->


