<?xml version="1.0"?>
<rdf:RDF xmlns="https://www.theworldavatar.com/kg/ontoprofile/"
     xml:base="https://www.theworldavatar.com/kg/ontoprofile/"
     xmlns:dc="http://purl.org/dc/elements/1.1/"
     xmlns:owl="http://www.w3.org/2002/07/owl#"
     xmlns:rdf="http://www.w3.org/1999/02/22-rdf-syntax-ns#"
     xmlns:xml="http://www.w3.org/XML/1998/namespace"
     xmlns:xsd="http://www.w3.org/2001/XMLSchema#"
     xmlns:rdfs="http://www.w3.org/2000/01/rdf-schema#"
     xmlns:ontoprofile="https://www.theworldavatar.com/kg/ontoprofile/">
    <owl:Ontology rdf:about="https://www.theworldavatar.com/kg/ontoprofile/">
        <dc:date>03 September 2024</dc:date>
        <rdfs:comment>OntoProfile is designed to represent the profiles of organizations and people, inclusive of their names, roles, and responsibilities.</rdfs:comment>
        <owl:versionInfo>1</owl:versionInfo>
        <gitCommitHash>c0599beca8df55873a1ab061dee64e52c510c6a0</gitCommitHash>
    </owl:Ontology>
    


    <!-- 
    ///////////////////////////////////////////////////////////////////////////////////////
    //
    // Annotation properties
    //
    ///////////////////////////////////////////////////////////////////////////////////////
     -->


    


    <!-- http://purl.org/dc/elements/1.1/date -->


    <owl:AnnotationProperty rdf:about="http://purl.org/dc/elements/1.1/date"/>
    


    <!-- https://www.theworldavatar.com/kg/ontoprofile/gitCommitHash -->


    <owl:AnnotationProperty rdf:about="https://www.theworldavatar.com/kg/ontoprofile/gitCommitHash"/>
    


    <!-- 
    ///////////////////////////////////////////////////////////////////////////////////////
    //
    // Object Properties
    //
    ///////////////////////////////////////////////////////////////////////////////////////
     -->


    


    <!-- https://www.theworldavatar.com/kg/ontoprofile/hasFacility -->


    <owl:ObjectProperty rdf:about="https://www.theworldavatar.com/kg/ontoprofile/hasFacility">
        <rdfs:domain rdf:resource="https://spec.edmcouncil.org/fibo/ontology/FND/Organizations/FormalOrganizations/FormalOrganization"/>
        <rdfs:range rdf:resource="https://www.theworldavatar.com/kg/ontobim/Facility"/>
        <rdfs:comment>A relationship describing the facility that the organisation is using for any of their operational needs.</rdfs:comment>
        <rdfs:isDefinedBy rdf:resource="https://www.theworldavatar.com/kg/ontoprofile/"/>
        <rdfs:label>has facility</rdfs:label>
    </owl:ObjectProperty>
    


    <!-- https://www.theworldavatar.com/kg/ontoprofile/hasInitials -->


    <owl:ObjectProperty rdf:about="https://www.theworldavatar.com/kg/ontoprofile/hasInitials">
        <rdfs:domain rdf:resource="https://spec.edmcouncil.org/fibo/ontology/FND/AgentsAndPeople/People/PersonName"/>
        <rdfs:range rdf:resource="https://www.theworldavatar.com/kg/ontoprofile/Initials"/>
        <rdfs:comment>A relationship that describes a person&apos;s initials.</rdfs:comment>
        <rdfs:isDefinedBy rdf:resource="https://www.theworldavatar.com/kg/ontoprofile/"/>
        <rdfs:label>has initials</rdfs:label>
    </owl:ObjectProperty>
    


    <!-- https://www.theworldavatar.com/kg/ontoprofile/hasStatus -->


    <owl:ObjectProperty rdf:about="https://www.theworldavatar.com/kg/ontoprofile/hasStatus">
        <rdfs:domain rdf:resource="https://spec.edmcouncil.org/fibo/ontology/FND/Organizations/FormalOrganizations/Employee"/>
        <rdfs:range rdf:resource="https://www.theworldavatar.com/kg/ontoprofile/EmployeeStatus"/>
        <rdfs:comment>A relationship describing the current status of an employee.</rdfs:comment>
        <rdfs:isDefinedBy rdf:resource="https://www.theworldavatar.com/kg/ontoprofile/"/>
        <rdfs:label>has status</rdfs:label>
    </owl:ObjectProperty>
    


    <!-- https://www.theworldavatar.com/kg/ontoprofile/worksAt -->


    <owl:ObjectProperty rdf:about="https://www.theworldavatar.com/kg/ontoprofile/worksAt">
        <rdfs:domain rdf:resource="https://spec.edmcouncil.org/fibo/ontology/FND/Organizations/FormalOrganizations/Employee"/>
        <rdfs:range rdf:resource="https://www.theworldavatar.com/kg/ontobim/Facility"/>
        <rdfs:comment>A relationship describing the facility that the employee is working in.</rdfs:comment>
        <rdfs:isDefinedBy rdf:resource="https://www.theworldavatar.com/kg/ontoprofile/"/>
        <rdfs:label>works at</rdfs:label>
    </owl:ObjectProperty>
    


    <!-- 
    ///////////////////////////////////////////////////////////////////////////////////////
    //
    // Classes
    //
    ///////////////////////////////////////////////////////////////////////////////////////
     -->


    


    <!-- https://spec.edmcouncil.org/fibo/ontology/FND/AgentsAndPeople/People/PersonName -->


    <owl:Class rdf:about="https://spec.edmcouncil.org/fibo/ontology/FND/AgentsAndPeople/People/PersonName"/>
    


    <!-- https://spec.edmcouncil.org/fibo/ontology/FND/Organizations/FormalOrganizations/Employee -->


    <owl:Class rdf:about="https://spec.edmcouncil.org/fibo/ontology/FND/Organizations/FormalOrganizations/Employee"/>
    


    <!-- https://spec.edmcouncil.org/fibo/ontology/FND/Organizations/FormalOrganizations/FormalOrganization -->


    <owl:Class rdf:about="https://spec.edmcouncil.org/fibo/ontology/FND/Organizations/FormalOrganizations/FormalOrganization"/>
    


    <!-- https://spec.edmcouncil.org/fibo/ontology/FND/Organizations/Organizations/OrganizationMember -->


    <owl:Class rdf:about="https://spec.edmcouncil.org/fibo/ontology/FND/Organizations/Organizations/OrganizationMember"/>
    


    <!-- https://www.theworldavatar.com/kg/ontobim/Facility -->


    <owl:Class rdf:about="https://www.theworldavatar.com/kg/ontobim/Facility"/>
    


    <!-- https://www.theworldavatar.com/kg/ontoprofile/Driver -->


    <owl:Class rdf:about="https://www.theworldavatar.com/kg/ontoprofile/Driver">
        <rdfs:subClassOf rdf:resource="https://spec.edmcouncil.org/fibo/ontology/FND/Organizations/FormalOrganizations/Employee"/>
        <rdfs:comment>A person who is employed to drive a vehicle.</rdfs:comment>
        <rdfs:isDefinedBy rdf:resource="https://www.theworldavatar.com/kg/ontoprofile/"/>
        <rdfs:label>Driver</rdfs:label>
    </owl:Class>
    


    <!-- https://www.theworldavatar.com/kg/ontoprofile/EmployeeStatus -->


    <owl:Class rdf:about="https://www.theworldavatar.com/kg/ontoprofile/EmployeeStatus">
        <rdfs:comment>The work availability of an employee.</rdfs:comment>
        <rdfs:isDefinedBy rdf:resource="https://www.theworldavatar.com/kg/ontoprofile/"/>
        <rdfs:label>Employee status</rdfs:label>
    </owl:Class>
    


    <!-- https://www.theworldavatar.com/kg/ontoprofile/EmployeeStatusEnum -->


    <owl:Class rdf:about="https://www.theworldavatar.com/kg/ontoprofile/EmployeeStatusEnum">
        <rdfs:comment>The enumerated states belonging to the employee status: on work, on leave</rdfs:comment>
        <rdfs:isDefinedBy rdf:resource="https://www.theworldavatar.com/kg/ontoprofile/"/>
        <rdfs:label>Employee status enum</rdfs:label>
    </owl:Class>
    


    <!-- https://www.theworldavatar.com/kg/ontoprofile/Initials -->


    <owl:Class rdf:about="https://www.theworldavatar.com/kg/ontoprofile/Initials">
        <rdfs:comment>The initials of a person are the first letters of their first name and last name (and sometimes middle name).</rdfs:comment>
        <rdfs:isDefinedBy rdf:resource="https://www.theworldavatar.com/kg/ontoprofile/"/>
        <rdfs:label>Initials</rdfs:label>
    </owl:Class>
    


    <!-- https://www.theworldavatar.com/kg/ontoprofile/OperationManager -->


    <owl:Class rdf:about="https://www.theworldavatar.com/kg/ontoprofile/OperationManager">
        <rdfs:subClassOf rdf:resource="https://spec.edmcouncil.org/fibo/ontology/FND/Organizations/FormalOrganizations/Employee"/>
        <rdfs:comment>A person who is employed to manages and supervises the operational conditions of a service.</rdfs:comment>
        <rdfs:isDefinedBy rdf:resource="https://www.theworldavatar.com/kg/ontoprofile/"/>
        <rdfs:label>Operation manager</rdfs:label>
    </owl:Class>
    


    <!-- https://www.theworldavatar.com/kg/ontoprofile/OperationScheduler -->


    <owl:Class rdf:about="https://www.theworldavatar.com/kg/ontoprofile/OperationScheduler">
        <rdfs:subClassOf rdf:resource="https://spec.edmcouncil.org/fibo/ontology/FND/Organizations/FormalOrganizations/Employee"/>
        <rdfs:comment>A person who is employed to manage the operational schedule of a service.</rdfs:comment>
        <rdfs:isDefinedBy rdf:resource="https://www.theworldavatar.com/kg/ontoprofile/"/>
        <rdfs:label>Operation scheduler</rdfs:label>
    </owl:Class>
    


    <!-- https://www.theworldavatar.com/kg/ontoprofile/SalesAdmin -->


    <owl:Class rdf:about="https://www.theworldavatar.com/kg/ontoprofile/SalesAdmin">
        <rdfs:subClassOf rdf:resource="https://spec.edmcouncil.org/fibo/ontology/FND/Organizations/FormalOrganizations/Employee"/>
        <rdfs:comment>A person who is employed to communicate with clients about the company&apos;s products and/or services. The person is primarily based at the front-desk.</rdfs:comment>
        <rdfs:isDefinedBy rdf:resource="https://www.theworldavatar.com/kg/ontoprofile/"/>
        <rdfs:label>Sales admin</rdfs:label>
    </owl:Class>
    


    <!-- https://www.theworldavatar.com/kg/ontoprofile/Student -->


    <owl:Class rdf:about="https://www.theworldavatar.com/kg/ontoprofile/Student">
        <rdfs:subClassOf rdf:resource="https://spec.edmcouncil.org/fibo/ontology/FND/Organizations/Organizations/OrganizationMember"/>
        <rdfs:comment>A person who has a membership role within an educational institution, typically enrolled in a course of study or program, and is involved in learning or training activities under the supervision of educators.</rdfs:comment>
        <rdfs:isDefinedBy rdf:resource="https://www.theworldavatar.com/kg/ontoprofile/"/>
        <rdfs:label>Student</rdfs:label>
    </owl:Class>
    


    <!-- https://www.theworldavatar.com/kg/ontoprofile/WorkResponsibility -->


    <owl:Class rdf:about="https://www.theworldavatar.com/kg/ontoprofile/WorkResponsibility">
        <rdfs:comment>The specific duties and tasks that is expected of an individual to perform as part of their employee role. They are typically outlined in a job description and can include both routine tasks and broader objectives that contribute to the organization&apos;s overall success.</rdfs:comment>
        <rdfs:isDefinedBy rdf:resource="https://www.theworldavatar.com/kg/ontoprofile/"/>
        <rdfs:label>Work responsibility</rdfs:label>
    </owl:Class>
    


    <!-- https://www.theworldavatar.com/kg/ontoprofile/WorkResponsibilityEnum -->


    <owl:Class rdf:about="https://www.theworldavatar.com/kg/ontoprofile/WorkResponsibilityEnum">
        <rdfs:subClassOf rdf:resource="https://www.theworldavatar.com/kg/ontoprofile/WorkResponsibility"/>
        <rdfs:comment>The enumerated responsibilities available for the work responsibility.</rdfs:comment>
        <rdfs:isDefinedBy rdf:resource="https://www.theworldavatar.com/kg/ontoprofile/"/>
        <rdfs:label>Work responsibility enumerator</rdfs:label>
    </owl:Class>
</rdf:RDF>



<!-- Generated by the OWL API (version 5.5.0.2023-01-14T12:41:38Z) https://github.com/owlcs/owlapi/ -->


