<?xml version="1.0"?>
<rdf:RDF xmlns="https://www.theworldavatar.com/kg/ontoschool/"
     xml:base="https://www.theworldavatar.com/kg/ontoschool/"
     xmlns:dc="http://purl.org/dc/elements/1.1/"
     xmlns:owl="http://www.w3.org/2002/07/owl#"
     xmlns:rdf="http://www.w3.org/1999/02/22-rdf-syntax-ns#"
     xmlns:xml="http://www.w3.org/XML/1998/namespace"
     xmlns:xsd="http://www.w3.org/2001/XMLSchema#"
     xmlns:rdfs="http://www.w3.org/2000/01/rdf-schema#"
     xmlns:ontoschool="https://www.theworldavatar.com/kg/ontoschool/">
    <owl:Ontology rdf:about="https://www.theworldavatar.com/kg/ontoschool/">
        <owl:imports rdf:resource="https://raw.githubusercontent.com/cambridge-cares/TheWorldAvatar/main/JPS_Ontology/ontology/ontobuiltenv/OntoBuiltEnv.owl"/>
        <dc:date>25 March 2024</dc:date>
        <rdfs:comment>OntoSchool is an ontology to represent schools and their information such as (contact information, address, CCAs etc).</rdfs:comment>
        <owl:versionInfo>1</owl:versionInfo>
        <gitCommitHash>c0599beca8df55873a1ab061dee64e52c510c6a0</gitCommitHash>
    </owl:Ontology>
    


    <!-- 
    ///////////////////////////////////////////////////////////////////////////////////////
    //
    // Annotation properties
    //
    ///////////////////////////////////////////////////////////////////////////////////////
     -->


    


    <!-- http://purl.org/dc/elements/1.1/date -->


    <owl:AnnotationProperty rdf:about="http://purl.org/dc/elements/1.1/date"/>
    


    <!-- https://www.theworldavatar.com/kg/ontoschool/gitCommitHash -->


    <owl:AnnotationProperty rdf:about="https://www.theworldavatar.com/kg/ontoschool/gitCommitHash"/>
    


    <!-- 
    ///////////////////////////////////////////////////////////////////////////////////////
    //
    // Object Properties
    //
    ///////////////////////////////////////////////////////////////////////////////////////
     -->


    


    <!-- https://www.theworldavatar.com/kg/ontoschool/hasAddress -->


    <owl:ObjectProperty rdf:about="https://www.theworldavatar.com/kg/ontoschool/hasAddress">
        <rdfs:domain rdf:resource="https://www.theworldavatar.com/kg/ontoschool/School"/>
        <rdfs:range rdf:resource="http://ontology.eil.utoronto.ca/icontact.owl#Address"/>
        <rdfs:comment>A relationship that describes a school's address.</rdfs:comment>
        <rdfs:isDefinedBy rdf:resource="https://www.theworldavatar.com/kg/ontoschool/"/>
        <rdfs:label>has address</rdfs:label>
    </owl:ObjectProperty>
    


    <!-- https://www.theworldavatar.com/kg/ontoschool/hasCCA -->


    <owl:ObjectProperty rdf:about="https://www.theworldavatar.com/kg/ontoschool/hasCCA">
        <rdfs:domain rdf:resource="https://www.theworldavatar.com/kg/ontoschool/CCAGroups"/>
        <rdfs:range rdf:resource="https://www.theworldavatar.com/kg/ontoschool/CCA"/>
        <rdfs:comment>A relationship which decribes the different activities or programmes under each CCA group.</rdfs:comment>
        <rdfs:isDefinedBy rdf:resource="https://www.theworldavatar.com/kg/ontoschool/"/>
        <rdfs:label>has CCA</rdfs:label>
    </owl:ObjectProperty>
    


    <!-- https://www.theworldavatar.com/kg/ontoschool/hasCCAGroups -->


    <owl:ObjectProperty rdf:about="https://www.theworldavatar.com/kg/ontoschool/hasCCAGroups">
        <rdfs:domain rdf:resource="https://www.theworldavatar.com/kg/ontoschool/School"/>
        <rdfs:range rdf:resource="https://www.theworldavatar.com/kg/ontoschool/CCAGroups"/>
        <rdfs:comment>A relationship which decribes the CCA groups in a school.</rdfs:comment>
        <rdfs:isDefinedBy rdf:resource="https://www.theworldavatar.com/kg/ontoschool/"/>
        <rdfs:label>has CCA groups</rdfs:label>
    </owl:ObjectProperty>
    


    <!-- https://www.theworldavatar.com/kg/ontoschool/hasContactNumber -->


    <owl:ObjectProperty rdf:about="https://www.theworldavatar.com/kg/ontoschool/hasContactNumber">
        <rdfs:domain rdf:resource="https://www.theworldavatar.com/kg/ontoschool/School"/>
        <rdfs:range rdf:resource="http://ontology.eil.utoronto.ca/icontact.owl#PhoneNumber"/>
        <rdfs:comment>A relationship which describes the contact number of a school.</rdfs:comment>
        <rdfs:isDefinedBy rdf:resource="https://www.theworldavatar.com/kg/ontoschool/"/>
        <rdfs:label>has contact number</rdfs:label>
    </owl:ObjectProperty>
    


    <!-- https://www.theworldavatar.com/kg/ontoschool/hasEducationLevel -->


    <owl:ObjectProperty rdf:about="https://www.theworldavatar.com/kg/ontoschool/hasEducationLevel">
        <rdfs:domain rdf:resource="https://www.theworldavatar.com/kg/ontoschool/School"/>
        <rdfs:range rdf:resource="https://www.theworldavatar.com/kg/ontoschool/EducationLevel"/>
        <rdfs:comment>A relationship which describes the education level that a school provides.</rdfs:comment>
        <rdfs:isDefinedBy rdf:resource="https://www.theworldavatar.com/kg/ontoschool/"/>
        <rdfs:label>has education level</rdfs:label>
    </owl:ObjectProperty>
    


    <!-- https://www.theworldavatar.com/kg/ontoschool/hasGenderComposition -->


    <owl:ObjectProperty rdf:about="https://www.theworldavatar.com/kg/ontoschool/hasGenderComposition">
        <rdfs:domain rdf:resource="https://www.theworldavatar.com/kg/ontoschool/School"/>
        <rdfs:range rdf:resource="https://www.theworldavatar.com/kg/ontoschool/GenderComposition"/>
        <rdfs:comment>A relationship which describes the gender composition of a school (Boys only, girls only, mixed).</rdfs:comment>
        <rdfs:isDefinedBy rdf:resource="https://www.theworldavatar.com/kg/ontoschool/"/>
        <rdfs:label>has gender composition</rdfs:label>
    </owl:ObjectProperty>
    


    <!-- https://www.theworldavatar.com/kg/ontoschool/hasProperty -->


    <owl:ObjectProperty rdf:about="https://www.theworldavatar.com/kg/ontoschool/hasProperty">
        <rdfs:domain rdf:resource="https://www.theworldavatar.com/kg/ontoschool/School"/>
        <rdfs:range rdf:resource="https://www.theworldavatar.com/kg/ontobuiltenv/Property"/>
        <rdfs:comment>A relationship that relates a school to its built structures.</rdfs:comment>
        <rdfs:isDefinedBy rdf:resource="https://www.theworldavatar.com/kg/ontoschool/"/>
        <rdfs:label>has property</rdfs:label>
    </owl:ObjectProperty>
    


    <!-- 
    ///////////////////////////////////////////////////////////////////////////////////////
    //
    // Data properties
    //
    ///////////////////////////////////////////////////////////////////////////////////////
     -->


    


    <!-- http://ontology.eil.utoronto.ca/icontact.owl#hasEmail -->


    <owl:DatatypeProperty rdf:about="http://ontology.eil.utoronto.ca/icontact.owl#hasEmail">
        <rdfs:domain rdf:resource="https://www.theworldavatar.com/kg/ontoschool/School"/>
        <rdfs:range rdf:resource="http://www.w3.org/2001/XMLSchema#string"/>
        <rdfs:comment>Email address of a school.</rdfs:comment>
        <rdfs:isDefinedBy rdf:resource="https://www.theworldavatar.com/kg/ontoschool/"/>
        <rdfs:label>has email</rdfs:label>
    </owl:DatatypeProperty>
    


    <!-- http://ontology.eil.utoronto.ca/icontact.owl#hasWebSite -->


    <owl:DatatypeProperty rdf:about="http://ontology.eil.utoronto.ca/icontact.owl#hasWebSite">
        <rdfs:domain rdf:resource="https://www.theworldavatar.com/kg/ontoschool/School"/>
        <rdfs:range rdf:resource="http://www.w3.org/2001/XMLSchema#string"/>
        <rdfs:comment>Website of the school.</rdfs:comment>
        <rdfs:isDefinedBy rdf:resource="https://www.theworldavatar.com/kg/ontoschool/"/>
        <rdfs:label>hasWeb Site</rdfs:label>
    </owl:DatatypeProperty>
    


    <!-- https://www.theworldavatar.com/kg/ontoschool/offersProgramme -->


    <owl:DatatypeProperty rdf:about="https://www.theworldavatar.com/kg/ontoschool/offersProgramme">
        <rdfs:domain rdf:resource="https://www.theworldavatar.com/kg/ontoschool/School"/>
        <rdfs:range rdf:resource="http://www.w3.org/2001/XMLSchema#string"/>
        <rdfs:comment>Programmes offered by the school.</rdfs:comment>
        <rdfs:isDefinedBy rdf:resource="https://www.theworldavatar.com/kg/ontoschool/"/>
        <rdfs:label>offers programme</rdfs:label>
    </owl:DatatypeProperty>
    


    <!-- 
    ///////////////////////////////////////////////////////////////////////////////////////
    //
    // Classes
    //
    ///////////////////////////////////////////////////////////////////////////////////////
     -->


    


    <!-- http://ontology.eil.utoronto.ca/icontact.owl#Address -->


    <owl:Class rdf:about="http://ontology.eil.utoronto.ca/icontact.owl#Address"/>
    


    <!-- http://ontology.eil.utoronto.ca/icontact.owl#PhoneNumber -->


    <owl:Class rdf:about="http://ontology.eil.utoronto.ca/icontact.owl#PhoneNumber"/>
    


    <!-- https://spec.edmcouncil.org/fibo/ontology/FND/Organizations/Organizations/Organization -->


    <owl:Class rdf:about="https://spec.edmcouncil.org/fibo/ontology/FND/Organizations/Organizations/Organization"/>
    


    <!-- https://www.theworldavatar.com/kg/ontobuiltenv/Property -->


    <owl:Class rdf:about="https://www.theworldavatar.com/kg/ontobuiltenv/Property"/>
    


    <!-- https://www.theworldavatar.com/kg/ontoschool/AllBoys -->


    <owl:Class rdf:about="https://www.theworldavatar.com/kg/ontoschool/AllBoys">
        <rdfs:subClassOf rdf:resource="https://www.theworldavatar.com/kg/ontoschool/Monogender"/>
        <rdfs:comment>An educational setting or institution where only male students are enrolled.</rdfs:comment>
        <rdfs:isDefinedBy rdf:resource="https://www.theworldavatar.com/kg/ontoschool/"/>
        <rdfs:label>All boys</rdfs:label>
    </owl:Class>
    


    <!-- https://www.theworldavatar.com/kg/ontoschool/AllGirls -->


    <owl:Class rdf:about="https://www.theworldavatar.com/kg/ontoschool/AllGirls">
        <rdfs:subClassOf rdf:resource="https://www.theworldavatar.com/kg/ontoschool/Monogender"/>
        <rdfs:comment>An educational setting or institution where only female students are enrolled.</rdfs:comment>
        <rdfs:isDefinedBy rdf:resource="https://www.theworldavatar.com/kg/ontoschool/"/>
        <rdfs:label>All girls</rdfs:label>
    </owl:Class>
    


    <!-- https://www.theworldavatar.com/kg/ontoschool/CCA -->


    <owl:Class rdf:about="https://www.theworldavatar.com/kg/ontoschool/CCA">
        <rdfs:comment>An activity or program that complements the academic curriculum in educational institutions.</rdfs:comment>
        <rdfs:isDefinedBy rdf:resource="https://www.theworldavatar.com/kg/ontoschool/"/>
        <rdfs:label>CCA</rdfs:label>
    </owl:Class>
    


    <!-- https://www.theworldavatar.com/kg/ontoschool/CCAGroups -->


    <owl:Class rdf:about="https://www.theworldavatar.com/kg/ontoschool/CCAGroups">
        <rdfs:comment>Groups for different types of CCAs (Co-Curricular Activities).</rdfs:comment>
        <rdfs:isDefinedBy rdf:resource="https://www.theworldavatar.com/kg/ontoschool/"/>
        <rdfs:label>CCA groups</rdfs:label>
    </owl:Class>
    


    <!-- https://www.theworldavatar.com/kg/ontoschool/ClubsAndSocieties -->


    <owl:Class rdf:about="https://www.theworldavatar.com/kg/ontoschool/ClubsAndSocieties">
        <rdfs:subClassOf rdf:resource="https://www.theworldavatar.com/kg/ontoschool/CCAGroups"/>
        <rdfs:comment>Clubs and societies CCAs cover a diverse array of interests and hobbies beyond sports and arts.</rdfs:comment>
        <rdfs:isDefinedBy rdf:resource="https://www.theworldavatar.com/kg/ontoschool/"/>
        <rdfs:label>Clubs and societies</rdfs:label>
    </owl:Class>
    


    <!-- https://www.theworldavatar.com/kg/ontoschool/Coeducational -->


    <owl:Class rdf:about="https://www.theworldavatar.com/kg/ontoschool/Coeducational">
        <rdfs:subClassOf rdf:resource="https://www.theworldavatar.com/kg/ontoschool/GenderComposition"/>
        <rdfs:comment>An educational setting or institution where students of both genders—males and females—are enrolled together.</rdfs:comment>
        <rdfs:isDefinedBy rdf:resource="https://www.theworldavatar.com/kg/ontoschool/"/>
        <rdfs:label>Coeducational</rdfs:label>
    </owl:Class>
    


    <!-- https://www.theworldavatar.com/kg/ontoschool/EducationLevel -->


    <owl:Class rdf:about="https://www.theworldavatar.com/kg/ontoschool/EducationLevel">
        <rdfs:comment>A stage or phase of formal education that an individual has completed or is currently pursuing.</rdfs:comment>
        <rdfs:isDefinedBy rdf:resource="https://www.theworldavatar.com/kg/ontoschool/"/>
        <rdfs:label>Education level</rdfs:label>
    </owl:Class>
    


    <!-- https://www.theworldavatar.com/kg/ontoschool/GenderComposition -->


    <owl:Class rdf:about="https://www.theworldavatar.com/kg/ontoschool/GenderComposition">
        <rdfs:comment>The distribution of students based on their gender or sex.</rdfs:comment>
        <rdfs:isDefinedBy rdf:resource="https://www.theworldavatar.com/kg/ontoschool/"/>
        <rdfs:label>Gender composition</rdfs:label>
    </owl:Class>
    


    <!-- https://www.theworldavatar.com/kg/ontoschool/GovernmentAidedSchool -->


    <owl:Class rdf:about="https://www.theworldavatar.com/kg/ontoschool/GovernmentAidedSchool">
        <rdfs:subClassOf rdf:resource="https://www.theworldavatar.com/kg/ontoschool/School"/>
        <rdfs:comment>Educational institutions that receive partial funding from the government but are managed independently.</rdfs:comment>
        <rdfs:isDefinedBy rdf:resource="https://www.theworldavatar.com/kg/ontoschool/"/>
        <rdfs:label>Government aided school</rdfs:label>
    </owl:Class>
    


    <!-- https://www.theworldavatar.com/kg/ontoschool/GovernmentSchool -->


    <owl:Class rdf:about="https://www.theworldavatar.com/kg/ontoschool/GovernmentSchool">
        <rdfs:subClassOf rdf:resource="https://www.theworldavatar.com/kg/ontoschool/School"/>
        <rdfs:comment>Educational institutions funded and managed by the government.</rdfs:comment>
        <rdfs:isDefinedBy rdf:resource="https://www.theworldavatar.com/kg/ontoschool/"/>
        <rdfs:label>Government school</rdfs:label>
    </owl:Class>
    


    <!-- https://www.theworldavatar.com/kg/ontoschool/IndependentSchool -->


    <owl:Class rdf:about="https://www.theworldavatar.com/kg/ontoschool/IndependentSchool">
        <rdfs:subClassOf rdf:resource="https://www.theworldavatar.com/kg/ontoschool/School"/>
        <rdfs:comment>Educational institutions that are not administered by the government.</rdfs:comment>
        <rdfs:isDefinedBy rdf:resource="https://www.theworldavatar.com/kg/ontoschool/"/>
        <rdfs:label>Independent school</rdfs:label>
    </owl:Class>
    


    <!-- https://www.theworldavatar.com/kg/ontoschool/JuniorCollege -->


    <owl:Class rdf:about="https://www.theworldavatar.com/kg/ontoschool/JuniorCollege">
        <rdfs:subClassOf rdf:resource="https://www.theworldavatar.com/kg/ontoschool/SecondaryEducation"/>
        <rdfs:comment>This level offers advanced coursework, preparation for college or university admissions, and opportunities for students to pursue specialized subjects or interests in preparation for further academic study.</rdfs:comment>
        <rdfs:isDefinedBy rdf:resource="https://www.theworldavatar.com/kg/ontoschool/"/>
        <rdfs:label>Junior college</rdfs:label>
    </owl:Class>
    


    <!-- https://www.theworldavatar.com/kg/ontoschool/MixedLevels -->


    <owl:Class rdf:about="https://www.theworldavatar.com/kg/ontoschool/MixedLevels">
        <rdfs:subClassOf rdf:resource="https://www.theworldavatar.com/kg/ontoschool/EducationLevel"/>
        <rdfs:comment>This level integrate multiple education levels or age groups to provide a more flexible and inclusive learning environment.</rdfs:comment>
        <rdfs:isDefinedBy rdf:resource="https://www.theworldavatar.com/kg/ontoschool/"/>
        <rdfs:label>Mixed levels</rdfs:label>
    </owl:Class>
    


    <!-- https://www.theworldavatar.com/kg/ontoschool/Monogender -->


    <owl:Class rdf:about="https://www.theworldavatar.com/kg/ontoschool/Monogender">
        <rdfs:subClassOf rdf:resource="https://www.theworldavatar.com/kg/ontoschool/GenderComposition"/>
        <rdfs:comment>An educational setting or institution where students of only one gender are enrolled.</rdfs:comment>
        <rdfs:isDefinedBy rdf:resource="https://www.theworldavatar.com/kg/ontoschool/"/>
        <rdfs:label>Monogender</rdfs:label>
    </owl:Class>
    


    <!-- https://www.theworldavatar.com/kg/ontoschool/PhysicalSports -->


    <owl:Class rdf:about="https://www.theworldavatar.com/kg/ontoschool/PhysicalSports">
        <rdfs:subClassOf rdf:resource="https://www.theworldavatar.com/kg/ontoschool/CCAGroups"/>
        <rdfs:comment>Physical sports CCAs involve activities focused on physical fitness, teamwork, and competitive sportsmanship.</rdfs:comment>
        <rdfs:isDefinedBy rdf:resource="https://www.theworldavatar.com/kg/ontoschool/"/>
        <rdfs:label>Physical sports</rdfs:label>
    </owl:Class>
    


    <!-- https://www.theworldavatar.com/kg/ontoschool/PrimaryEducation -->


    <owl:Class rdf:about="https://www.theworldavatar.com/kg/ontoschool/PrimaryEducation">
        <rdfs:subClassOf rdf:resource="https://www.theworldavatar.com/kg/ontoschool/EducationLevel"/>
        <rdfs:comment>This level focuses on fundamental skills such as literacy, numeracy, and basic knowledge in subjects like science, social studies, and language arts.</rdfs:comment>
        <rdfs:isDefinedBy rdf:resource="https://www.theworldavatar.com/kg/ontoschool/"/>
        <rdfs:label>Primary education</rdfs:label>
    </owl:Class>
    


    <!-- https://www.theworldavatar.com/kg/ontoschool/School -->


    <owl:Class rdf:about="https://www.theworldavatar.com/kg/ontoschool/School">
        <rdfs:subClassOf rdf:resource="https://spec.edmcouncil.org/fibo/ontology/FND/Organizations/Organizations/Organization"/>
        <rdfs:comment>An educational institution designed to provide learning spaces and learning environments for the teaching of students under the direction of teachers.</rdfs:comment>
        <rdfs:isDefinedBy rdf:resource="https://www.theworldavatar.com/kg/ontoschool/"/>
        <rdfs:label>School</rdfs:label>
    </owl:Class>
    


    <!-- https://www.theworldavatar.com/kg/ontoschool/SecondaryEducation -->


    <owl:Class rdf:about="https://www.theworldavatar.com/kg/ontoschool/SecondaryEducation">
        <rdfs:subClassOf rdf:resource="https://www.theworldavatar.com/kg/ontoschool/EducationLevel"/>
        <rdfs:comment>This level builds upon the foundational knowledge acquired in primary school and offers more specialized subjects and opportunities for academic exploration.</rdfs:comment>
        <rdfs:isDefinedBy rdf:resource="https://www.theworldavatar.com/kg/ontoschool/"/>
        <rdfs:label>Secondary education</rdfs:label>
    </owl:Class>
    


    <!-- https://www.theworldavatar.com/kg/ontoschool/SpecialisedIndependentSchool -->


    <owl:Class rdf:about="https://www.theworldavatar.com/kg/ontoschool/SpecialisedIndependentSchool">
        <rdfs:subClassOf rdf:resource="https://www.theworldavatar.com/kg/ontoschool/School"/>
        <rdfs:comment>Educational institutions that are not administered by the government and focuses on a specific area of study or cater to students with particular needs or interests.</rdfs:comment>
        <rdfs:isDefinedBy rdf:resource="https://www.theworldavatar.com/kg/ontoschool/"/>
        <rdfs:label>Specialised independent school</rdfs:label>
    </owl:Class>
    


    <!-- https://www.theworldavatar.com/kg/ontoschool/SpecialisedSchool -->


    <owl:Class rdf:about="https://www.theworldavatar.com/kg/ontoschool/SpecialisedSchool">
        <rdfs:subClassOf rdf:resource="https://www.theworldavatar.com/kg/ontoschool/School"/>
        <rdfs:comment>Educational institutions that focus on a specific area of study or cater to students with particular needs or interests.</rdfs:comment>
        <rdfs:isDefinedBy rdf:resource="https://www.theworldavatar.com/kg/ontoschool/"/>
        <rdfs:label>Specialised school</rdfs:label>
    </owl:Class>
    


    <!-- https://www.theworldavatar.com/kg/ontoschool/StudentLeadership -->


    <owl:Class rdf:about="https://www.theworldavatar.com/kg/ontoschool/StudentLeadership">
        <rdfs:subClassOf rdf:resource="https://www.theworldavatar.com/kg/ontoschool/CCAGroups"/>
        <rdfs:comment>Student leadership CCAs focus on developing leadership skills, responsibility, and initiative among students.</rdfs:comment>
        <rdfs:isDefinedBy rdf:resource="https://www.theworldavatar.com/kg/ontoschool/"/>
        <rdfs:label>Student leadership</rdfs:label>
    </owl:Class>
    


    <!-- https://www.theworldavatar.com/kg/ontoschool/TertiaryEducation -->


    <owl:Class rdf:about="https://www.theworldavatar.com/kg/ontoschool/TertiaryEducation">
        <rdfs:subClassOf rdf:resource="https://www.theworldavatar.com/kg/ontoschool/EducationLevel"/>
        <rdfs:comment>This level provides specialized knowledge and skills in various academic disciplines or professional fields and prepares individuals for careers or advanced study.</rdfs:comment>
        <rdfs:isDefinedBy rdf:resource="https://www.theworldavatar.com/kg/ontoschool/"/>
        <rdfs:label>Tertiary education</rdfs:label>
    </owl:Class>
    


    <!-- https://www.theworldavatar.com/kg/ontoschool/UniformedGroups -->


    <owl:Class rdf:about="https://www.theworldavatar.com/kg/ontoschool/UniformedGroups">
        <rdfs:subClassOf rdf:resource="https://www.theworldavatar.com/kg/ontoschool/CCAGroups"/>
        <rdfs:comment>Uniformed groups CCAs involve organizations that promote leadership, discipline, and community service through structured programs and activities.</rdfs:comment>
        <rdfs:isDefinedBy rdf:resource="https://www.theworldavatar.com/kg/ontoschool/"/>
        <rdfs:label>Uniformed groups</rdfs:label>
    </owl:Class>
    


    <!-- https://www.theworldavatar.com/kg/ontoschool/VisualAndPerformingArts -->


    <owl:Class rdf:about="https://www.theworldavatar.com/kg/ontoschool/VisualAndPerformingArts">
        <rdfs:subClassOf rdf:resource="https://www.theworldavatar.com/kg/ontoschool/CCAGroups"/>
        <rdfs:comment>Visual and performing arts CCAs encompass a wide range of creative activities including drawing, painting, sculpture, photography, dance, drama, music, and choir.</rdfs:comment>
        <rdfs:isDefinedBy rdf:resource="https://www.theworldavatar.com/kg/ontoschool/"/>
        <rdfs:label>Visual and performing arts</rdfs:label>
    </owl:Class>
</rdf:RDF>



<!-- Generated by the OWL API (version 5.5.0.2023-01-14T12:41:38Z) https://github.com/owlcs/owlapi/ -->


