<?xml version="1.0"?>
<rdf:RDF xmlns="https://www.theworldavatar.com/kg/ontoservice/"
     xml:base="https://www.theworldavatar.com/kg/ontoservice/"
     xmlns:dc="http://purl.org/dc/elements/1.1/"
     xmlns:owl="http://www.w3.org/2002/07/owl#"
     xmlns:rdf="http://www.w3.org/1999/02/22-rdf-syntax-ns#"
     xmlns:xml="http://www.w3.org/XML/1998/namespace"
     xmlns:xsd="http://www.w3.org/2001/XMLSchema#"
     xmlns:rdfs="http://www.w3.org/2000/01/rdf-schema#"
     xmlns:ontoservice="https://www.theworldavatar.com/kg/ontoservice/">
    <owl:Ontology rdf:about="https://www.theworldavatar.com/kg/ontoservice/">
        <dc:date>11 October 2024</dc:date>
        <rdfs:comment>OntoService is designed to represent the terms, conditions, and obligations associated with service delivery as well as the execution details.</rdfs:comment>
        <owl:versionInfo>1.1</owl:versionInfo>
        <gitCommitHash>c0599beca8df55873a1ab061dee64e52c510c6a0</gitCommitHash>
    </owl:Ontology>
    


    <!-- 
    ///////////////////////////////////////////////////////////////////////////////////////
    //
    // Annotation properties
    //
    ///////////////////////////////////////////////////////////////////////////////////////
     -->


    


    <!-- http://purl.org/dc/elements/1.1/date -->


    <owl:AnnotationProperty rdf:about="http://purl.org/dc/elements/1.1/date"/>
    


    <!-- https://www.theworldavatar.com/kg/ontoservice/gitCommitHash -->


    <owl:AnnotationProperty rdf:about="https://www.theworldavatar.com/kg/ontoservice/gitCommitHash"/>
    


    <!-- 
    ///////////////////////////////////////////////////////////////////////////////////////
    //
    // Object Properties
    //
    ///////////////////////////////////////////////////////////////////////////////////////
     -->


    


    <!-- https://spec.edmcouncil.org/fibo/ontology/FND/Places/Locations/isLocatedAt -->


    <owl:ObjectProperty rdf:about="https://spec.edmcouncil.org/fibo/ontology/FND/Places/Locations/isLocatedAt"/>
    


    <!-- https://www.theworldavatar.com/kg/ontoservice/assignTransport -->


    <owl:ObjectProperty rdf:about="https://www.theworldavatar.com/kg/ontoservice/assignTransport">
        <rdfs:domain>
            <owl:Class>
                <owl:unionOf rdf:parseType="Collection">
                    <rdf:Description rdf:about="https://www.theworldavatar.com/kg/ontoservice/CompletedServiceOccurrence"/>
                    <rdf:Description rdf:about="https://www.theworldavatar.com/kg/ontoservice/ServiceInProgressOccurrence"/>
                    <rdf:Description rdf:about="https://www.theworldavatar.com/kg/ontoservice/UncompletedServiceOccurrence"/>
                </owl:unionOf>
            </owl:Class>
        </rdfs:domain>
        <rdfs:range rdf:resource="https://spec.edmcouncil.org/auto/ontology/VC/VehicleCore/Vehicle"/>
        <rdfs:comment>A relationship assigning a transport vehicle to a service event.</rdfs:comment>
        <rdfs:isDefinedBy rdf:resource="https://www.theworldavatar.com/kg/ontoservice/"/>
        <rdfs:label>assign transport</rdfs:label>
    </owl:ObjectProperty>
    


    <!-- https://www.theworldavatar.com/kg/ontoservice/charges -->


    <owl:ObjectProperty rdf:about="https://www.theworldavatar.com/kg/ontoservice/charges">
        <rdfs:domain rdf:resource="https://www.theworldavatar.com/kg/ontoservice/CompletedServiceOccurrence"/>
        <rdfs:range rdf:resource="https://www.theworldavatar.com/kg/ontoservice/TotalPrice"/>
        <rdfs:comment>A relationship describing the final charge of a service event.</rdfs:comment>
        <rdfs:isDefinedBy rdf:resource="https://www.theworldavatar.com/kg/ontoservice/"/>
        <rdfs:label>charges</rdfs:label>
    </owl:ObjectProperty>
    


    <!-- https://www.theworldavatar.com/kg/ontoservice/commitsTo -->


    <owl:ObjectProperty rdf:about="https://www.theworldavatar.com/kg/ontoservice/commitsTo">
        <rdfs:domain rdf:resource="https://spec.edmcouncil.org/fibo/ontology/FND/ProductsAndServices/ProductsAndServices/Service"/>
        <rdfs:range rdf:resource="https://spec.edmcouncil.org/fibo/ontology/FND/Agreements/Contracts/ContractualCommitment"/>
        <rdfs:comment>A relationship that links the commitments made when providing or engaging with the associated service.</rdfs:comment>
        <rdfs:isDefinedBy rdf:resource="https://www.theworldavatar.com/kg/ontoservice/"/>
        <rdfs:label>commits to</rdfs:label>
    </owl:ObjectProperty>
    


    <!-- https://www.theworldavatar.com/kg/ontoservice/dependsOn -->


    <owl:ObjectProperty rdf:about="https://www.theworldavatar.com/kg/ontoservice/dependsOn">
        <rdfs:domain rdf:resource="https://www.theworldavatar.com/kg/ontoservice/VariableRate"/>
        <rdfs:range rdf:resource="https://www.theworldavatar.com/kg/ontoservice/ServiceMetric"/>
        <rdfs:comment>A relationship describing the service metric that the variable rate is based on.</rdfs:comment>
        <rdfs:isDefinedBy rdf:resource="https://www.theworldavatar.com/kg/ontoservice/"/>
        <rdfs:label>depends on</rdfs:label>
    </owl:ObjectProperty>
    


    <!-- https://www.theworldavatar.com/kg/ontoservice/hasBaseCharge -->


    <owl:ObjectProperty rdf:about="https://www.theworldavatar.com/kg/ontoservice/hasBaseCharge">
        <rdfs:domain rdf:resource="https://www.theworldavatar.com/kg/ontoservice/ServicePaymentObligation"/>
        <rdfs:range rdf:resource="https://www.theworldavatar.com/kg/ontoservice/BaseCharge"/>
        <rdfs:comment>A relationship describing a legally enforceable base charge for each service.</rdfs:comment>
        <rdfs:isDefinedBy rdf:resource="https://www.theworldavatar.com/kg/ontoservice/"/>
        <rdfs:label>has base charge</rdfs:label>
    </owl:ObjectProperty>
    


    <!-- https://www.theworldavatar.com/kg/ontoservice/hasDenominator -->


    <owl:ObjectProperty rdf:about="https://www.theworldavatar.com/kg/ontoservice/hasDenominator">
        <rdfs:domain rdf:resource="https://www.theworldavatar.com/kg/ontoservice/VariableRate"/>
        <rdfs:range rdf:resource="http://www.ontology-of-units-of-measure.org/resource/om-2/Quantity"/>
        <rdfs:comment>A relationship defining the denominator of a monetary rate, which depends on the service metric.</rdfs:comment>
        <rdfs:isDefinedBy rdf:resource="https://www.theworldavatar.com/kg/ontoservice/"/>
        <rdfs:label>has denominator</rdfs:label>
    </owl:ObjectProperty>
    


    <!-- https://www.theworldavatar.com/kg/ontoservice/hasNumerator -->


    <owl:ObjectProperty rdf:about="https://www.theworldavatar.com/kg/ontoservice/hasNumerator">
        <rdfs:domain rdf:resource="https://www.theworldavatar.com/kg/ontoservice/VariableRate"/>
        <rdfs:range rdf:resource="http://www.ontology-of-units-of-measure.org/resource/om-2/AmountOfMoney"/>
        <rdfs:comment>A relationship defining the numerator of a monetary rate, which should be amount of money.</rdfs:comment>
        <rdfs:isDefinedBy rdf:resource="https://www.theworldavatar.com/kg/ontoservice/"/>
        <rdfs:label>has numerator</rdfs:label>
    </owl:ObjectProperty>
    


    <!-- https://www.theworldavatar.com/kg/ontoservice/hasQuantity -->


    <owl:ObjectProperty rdf:about="https://www.theworldavatar.com/kg/ontoservice/hasQuantity">
        <rdfs:domain rdf:resource="https://www.theworldavatar.com/kg/ontoservice/ServiceMetric"/>
        <rdfs:domain rdf:resource="https://www.theworldavatar.com/kg/ontoservice/ServiceTonnage"/>
        <rdfs:range rdf:resource="http://www.ontology-of-units-of-measure.org/resource/om-2/Mass"/>
        <rdfs:range rdf:resource="http://www.ontology-of-units-of-measure.org/resource/om-2/Quantity"/>
        <rdfs:comment>A relationship defining the quantity of a service metric.</rdfs:comment>
        <rdfs:isDefinedBy rdf:resource="https://www.theworldavatar.com/kg/ontoservice/"/>
        <rdfs:label>has quantity</rdfs:label>
    </owl:ObjectProperty>
    


    <!-- https://www.theworldavatar.com/kg/ontoservice/hasServiceLocation -->


    <owl:ObjectProperty rdf:about="https://www.theworldavatar.com/kg/ontoservice/hasServiceLocation">
        <rdfs:subPropertyOf rdf:resource="https://spec.edmcouncil.org/fibo/ontology/FND/Places/Locations/isLocatedAt"/>
        <rdfs:domain rdf:resource="https://w3id.org/bot#Zone"/>
        <rdfs:range rdf:resource="https://www.omg.org/spec/LCC/Countries/CountryRepresentation/Location"/>
        <rdfs:comment>A relationship describing the service location, typically a point, within the building or site.</rdfs:comment>
        <rdfs:isDefinedBy rdf:resource="https://www.theworldavatar.com/kg/ontoservice/"/>
        <rdfs:label>has service location</rdfs:label>
    </owl:ObjectProperty>
    


    <!-- https://www.theworldavatar.com/kg/ontoservice/hasTimeSlot -->


    <owl:ObjectProperty rdf:about="https://www.theworldavatar.com/kg/ontoservice/hasTimeSlot">
        <rdfs:domain rdf:resource="https://spec.edmcouncil.org/fibo/ontology/FND/DatesAndTimes/FinancialDates/RegularSchedule"/>
        <rdfs:range rdf:resource="https://www.omg.org/spec/Commons/DatesAndTimes/ExplicitTimePeriod"/>
        <rdfs:comment>A relationship describing the time window for the regular schedule with a corresponding start and end time.</rdfs:comment>
        <rdfs:isDefinedBy rdf:resource="https://www.theworldavatar.com/kg/ontoservice/"/>
        <rdfs:label>has time slot</rdfs:label>
    </owl:ObjectProperty>
    


    <!-- https://www.theworldavatar.com/kg/ontoservice/hasVariableRate -->


    <owl:ObjectProperty rdf:about="https://www.theworldavatar.com/kg/ontoservice/hasVariableRate">
        <rdfs:domain rdf:resource="https://www.theworldavatar.com/kg/ontoservice/ServicePaymentObligation"/>
        <rdfs:range rdf:resource="https://www.theworldavatar.com/kg/ontoservice/VariableRate"/>
        <rdfs:comment>A relationship describing a legally enforceable variable rate for a service based on certain parameters.</rdfs:comment>
        <rdfs:isDefinedBy rdf:resource="https://www.theworldavatar.com/kg/ontoservice/"/>
        <rdfs:label>has variable rate</rdfs:label>
    </owl:ObjectProperty>
    


    <!-- https://www.theworldavatar.com/kg/ontoservice/obligedTo -->


    <owl:ObjectProperty rdf:about="https://www.theworldavatar.com/kg/ontoservice/obligedTo">
        <rdfs:domain rdf:resource="https://spec.edmcouncil.org/fibo/ontology/FND/ProductsAndServices/ProductsAndServices/Service"/>
        <rdfs:range rdf:resource="https://spec.edmcouncil.org/fibo/ontology/FND/ProductsAndServices/PaymentsAndSchedules/PaymentObligation"/>
        <rdfs:comment>A relationship that links the obligations made when providing or engaging with the associated service.</rdfs:comment>
        <rdfs:isDefinedBy rdf:resource="https://www.theworldavatar.com/kg/ontoservice/"/>
        <rdfs:label>obliged to</rdfs:label>
    </owl:ObjectProperty>
    


    <!-- https://www.theworldavatar.com/kg/ontoservice/servesAsContactFor -->


    <owl:ObjectProperty rdf:about="https://www.theworldavatar.com/kg/ontoservice/servesAsContactFor">
        <rdfs:domain rdf:resource="https://www.theworldavatar.com/kg/ontoservice/ContactService"/>
        <rdfs:range rdf:resource="https://spec.edmcouncil.org/fibo/ontology/FND/ProductsAndServices/ProductsAndServices/Service"/>
        <rdfs:comment>A relationship describing the contact point for another service.</rdfs:comment>
        <rdfs:isDefinedBy rdf:resource="https://www.theworldavatar.com/kg/ontoservice/"/>
        <rdfs:label>serves as contact for</rdfs:label>
    </owl:ObjectProperty>
    


    <!-- 
    ///////////////////////////////////////////////////////////////////////////////////////
    //
    // Classes
    //
    ///////////////////////////////////////////////////////////////////////////////////////
     -->


    


    <!-- http://www.ontology-of-units-of-measure.org/resource/om-2/AmountOfMoney -->


    <owl:Class rdf:about="http://www.ontology-of-units-of-measure.org/resource/om-2/AmountOfMoney"/>
    


    <!-- http://www.ontology-of-units-of-measure.org/resource/om-2/Mass -->


    <owl:Class rdf:about="http://www.ontology-of-units-of-measure.org/resource/om-2/Mass"/>
    


    <!-- http://www.ontology-of-units-of-measure.org/resource/om-2/Percentage -->


    <owl:Class rdf:about="http://www.ontology-of-units-of-measure.org/resource/om-2/Percentage"/>
    


    <!-- http://www.ontology-of-units-of-measure.org/resource/om-2/Quantity -->


    <owl:Class rdf:about="http://www.ontology-of-units-of-measure.org/resource/om-2/Quantity"/>
    


    <!-- https://spec.edmcouncil.org/auto/ontology/VC/VehicleCore/Vehicle -->


    <owl:Class rdf:about="https://spec.edmcouncil.org/auto/ontology/VC/VehicleCore/Vehicle"/>
    


    <!-- https://spec.edmcouncil.org/fibo/ontology/FBC/ProductsAndServices/FinancialProductsAndServices/ContractLifecycleEvent -->


    <owl:Class rdf:about="https://spec.edmcouncil.org/fibo/ontology/FBC/ProductsAndServices/FinancialProductsAndServices/ContractLifecycleEvent"/>
    


    <!-- https://spec.edmcouncil.org/fibo/ontology/FBC/ProductsAndServices/FinancialProductsAndServices/ContractLifecycleEventOccurrence -->


    <owl:Class rdf:about="https://spec.edmcouncil.org/fibo/ontology/FBC/ProductsAndServices/FinancialProductsAndServices/ContractLifecycleEventOccurrence"/>
    


    <!-- https://spec.edmcouncil.org/fibo/ontology/FBC/ProductsAndServices/FinancialProductsAndServices/ContractLifecycleStage -->


    <owl:Class rdf:about="https://spec.edmcouncil.org/fibo/ontology/FBC/ProductsAndServices/FinancialProductsAndServices/ContractLifecycleStage"/>
    


    <!-- https://spec.edmcouncil.org/fibo/ontology/FND/Agreements/Contracts/ContractualCommitment -->


    <owl:Class rdf:about="https://spec.edmcouncil.org/fibo/ontology/FND/Agreements/Contracts/ContractualCommitment"/>
    


    <!-- https://spec.edmcouncil.org/fibo/ontology/FND/DatesAndTimes/FinancialDates/RegularSchedule -->


    <owl:Class rdf:about="https://spec.edmcouncil.org/fibo/ontology/FND/DatesAndTimes/FinancialDates/RegularSchedule"/>
    


    <!-- https://spec.edmcouncil.org/fibo/ontology/FND/ProductsAndServices/PaymentsAndSchedules/PaymentObligation -->


    <owl:Class rdf:about="https://spec.edmcouncil.org/fibo/ontology/FND/ProductsAndServices/PaymentsAndSchedules/PaymentObligation"/>
    


    <!-- https://spec.edmcouncil.org/fibo/ontology/FND/ProductsAndServices/ProductsAndServices/Service -->


    <owl:Class rdf:about="https://spec.edmcouncil.org/fibo/ontology/FND/ProductsAndServices/ProductsAndServices/Service"/>
    


    <!-- https://w3id.org/bot#Zone -->


    <owl:Class rdf:about="https://w3id.org/bot#Zone"/>
    


    <!-- https://www.omg.org/spec/Commons/DatesAndTimes/ExplicitTimePeriod -->


    <owl:Class rdf:about="https://www.omg.org/spec/Commons/DatesAndTimes/ExplicitTimePeriod"/>
    


    <!-- https://www.omg.org/spec/LCC/Countries/CountryRepresentation/Location -->


    <owl:Class rdf:about="https://www.omg.org/spec/LCC/Countries/CountryRepresentation/Location"/>
    


    <!-- https://www.theworldavatar.com/kg/ontoservice/BaseCharge -->


    <owl:Class rdf:about="https://www.theworldavatar.com/kg/ontoservice/BaseCharge">
        <rdfs:subClassOf rdf:resource="http://www.ontology-of-units-of-measure.org/resource/om-2/AmountOfMoney"/>
        <rdfs:comment>A base charge for the service agreed in the contract.</rdfs:comment>
        <rdfs:isDefinedBy rdf:resource="https://www.theworldavatar.com/kg/ontoservice/"/>
        <rdfs:label>Base charge</rdfs:label>
    </owl:Class>
    


    <!-- https://www.theworldavatar.com/kg/ontoservice/CompletedService -->


    <owl:Class rdf:about="https://www.theworldavatar.com/kg/ontoservice/CompletedService">
        <rdfs:subClassOf rdf:resource="https://spec.edmcouncil.org/fibo/ontology/FBC/ProductsAndServices/FinancialProductsAndServices/ContractLifecycleEvent"/>
        <rdfs:comment>A service event that has completed successfully during the service execution lifecycle stage of a contract.</rdfs:comment>
        <rdfs:isDefinedBy rdf:resource="https://www.theworldavatar.com/kg/ontoservice/"/>
        <rdfs:label>Completed service</rdfs:label>
    </owl:Class>
    


    <!-- https://www.theworldavatar.com/kg/ontoservice/CompletedServiceOccurrence -->


    <owl:Class rdf:about="https://www.theworldavatar.com/kg/ontoservice/CompletedServiceOccurrence">
        <rdfs:subClassOf rdf:resource="https://spec.edmcouncil.org/fibo/ontology/FBC/ProductsAndServices/FinancialProductsAndServices/ContractLifecycleEventOccurrence"/>
        <rdfs:comment>An actual occurrence of a completed service event.</rdfs:comment>
        <rdfs:isDefinedBy rdf:resource="https://www.theworldavatar.com/kg/ontoservice/"/>
        <rdfs:label>Completed service occurrence</rdfs:label>
    </owl:Class>
    


    <!-- https://www.theworldavatar.com/kg/ontoservice/ContactService -->


    <owl:Class rdf:about="https://www.theworldavatar.com/kg/ontoservice/ContactService">
        <rdfs:subClassOf rdf:resource="https://spec.edmcouncil.org/fibo/ontology/FND/ProductsAndServices/ProductsAndServices/Service"/>
        <rdfs:comment>A service that acts as a point of contact for communication, support, or assistance.</rdfs:comment>
        <rdfs:isDefinedBy rdf:resource="https://www.theworldavatar.com/kg/ontoservice/"/>
        <rdfs:label>Contact service</rdfs:label>
    </owl:Class>
    


    <!-- https://www.theworldavatar.com/kg/ontoservice/ContractApproval -->


    <owl:Class rdf:about="https://www.theworldavatar.com/kg/ontoservice/ContractApproval">
        <rdfs:subClassOf rdf:resource="https://spec.edmcouncil.org/fibo/ontology/FBC/ProductsAndServices/FinancialProductsAndServices/ContractLifecycleEvent"/>
        <rdfs:comment>An event to approve the contract during the creation lifecycle stage of a contract.</rdfs:comment>
        <rdfs:isDefinedBy rdf:resource="https://www.theworldavatar.com/kg/ontoservice/"/>
        <rdfs:label>Contract approval</rdfs:label>
    </owl:Class>
    


    <!-- https://www.theworldavatar.com/kg/ontoservice/ContractCreation -->


    <owl:Class rdf:about="https://www.theworldavatar.com/kg/ontoservice/ContractCreation">
        <rdfs:subClassOf rdf:resource="https://spec.edmcouncil.org/fibo/ontology/FBC/ProductsAndServices/FinancialProductsAndServices/ContractLifecycleEvent"/>
        <rdfs:comment>An event to draft and create a new contract during the creation lifecycle stage of a contract.</rdfs:comment>
        <rdfs:isDefinedBy rdf:resource="https://www.theworldavatar.com/kg/ontoservice/"/>
        <rdfs:label>Contract creation</rdfs:label>
    </owl:Class>
    


    <!-- https://www.theworldavatar.com/kg/ontoservice/ContractDischarge -->


    <owl:Class rdf:about="https://www.theworldavatar.com/kg/ontoservice/ContractDischarge">
        <rdfs:subClassOf rdf:resource="https://spec.edmcouncil.org/fibo/ontology/FBC/ProductsAndServices/FinancialProductsAndServices/ContractLifecycleEvent"/>
        <rdfs:comment>An event ending the contract as all contractual obligations have been performed.</rdfs:comment>
        <rdfs:isDefinedBy rdf:resource="https://www.theworldavatar.com/kg/ontoservice/"/>
        <rdfs:label>Contract discharge</rdfs:label>
    </owl:Class>
    


    <!-- https://www.theworldavatar.com/kg/ontoservice/ContractRescission -->


    <owl:Class rdf:about="https://www.theworldavatar.com/kg/ontoservice/ContractRescission">
        <rdfs:subClassOf rdf:resource="https://spec.edmcouncil.org/fibo/ontology/FBC/ProductsAndServices/FinancialProductsAndServices/ContractLifecycleEvent"/>
        <rdfs:comment>An event rendering the contract null, void, and no longer legally binding as one contractual party is a victim of a vitiating factor during the expiration lifecycle stage of a contract.</rdfs:comment>
        <rdfs:isDefinedBy rdf:resource="https://www.theworldavatar.com/kg/ontoservice/"/>
        <rdfs:label>Contract rescission</rdfs:label>
    </owl:Class>
    


    <!-- https://www.theworldavatar.com/kg/ontoservice/ContractTermination -->


    <owl:Class rdf:about="https://www.theworldavatar.com/kg/ontoservice/ContractTermination">
        <rdfs:subClassOf rdf:resource="https://spec.edmcouncil.org/fibo/ontology/FBC/ProductsAndServices/FinancialProductsAndServices/ContractLifecycleEvent"/>
        <rdfs:comment>An event ending the contract before all contractual obligations have been performed. Typically the contract may have been concluded earlier with the agreement of all parties involved.</rdfs:comment>
        <rdfs:isDefinedBy rdf:resource="https://www.theworldavatar.com/kg/ontoservice/"/>
        <rdfs:label>Contract termination</rdfs:label>
    </owl:Class>
    


    <!-- https://www.theworldavatar.com/kg/ontoservice/CreationStage -->


    <owl:Class rdf:about="https://www.theworldavatar.com/kg/ontoservice/CreationStage">
        <rdfs:subClassOf rdf:resource="https://spec.edmcouncil.org/fibo/ontology/FBC/ProductsAndServices/FinancialProductsAndServices/ContractLifecycleStage"/>
        <rdfs:comment>The phase in the lifecycle of a contract to create a new contract.</rdfs:comment>
        <rdfs:isDefinedBy rdf:resource="https://www.theworldavatar.com/kg/ontoservice/"/>
        <rdfs:label>Creation stage</rdfs:label>
    </owl:Class>
    


    <!-- https://www.theworldavatar.com/kg/ontoservice/ExcessVariableRate -->


    <owl:Class rdf:about="https://www.theworldavatar.com/kg/ontoservice/ExcessVariableRate">
        <rdfs:subClassOf rdf:resource="https://www.theworldavatar.com/kg/ontoservice/VariableRate"/>
        <rdfs:subClassOf>
            <owl:Restriction>
                <owl:onProperty rdf:resource="https://www.theworldavatar.com/kg/ontoservice/dependsOn"/>
                <owl:allValuesFrom rdf:resource="https://www.theworldavatar.com/kg/ontoservice/ServiceMetricCap"/>
            </owl:Restriction>
        </rdfs:subClassOf>
        <rdfs:comment>The rates that is dependent on the outcome of a service after execution, agreed upon in the contract. Specifically, this rate will be in effect once the service exceeds the cap specified.</rdfs:comment>
        <rdfs:isDefinedBy rdf:resource="https://www.theworldavatar.com/kg/ontoservice/"/>
        <rdfs:label>Excess variable rate</rdfs:label>
    </owl:Class>
    


    <!-- https://www.theworldavatar.com/kg/ontoservice/ExpirationStage -->


    <owl:Class rdf:about="https://www.theworldavatar.com/kg/ontoservice/ExpirationStage">
        <rdfs:subClassOf rdf:resource="https://spec.edmcouncil.org/fibo/ontology/FBC/ProductsAndServices/FinancialProductsAndServices/ContractLifecycleStage"/>
        <rdfs:comment>The phase in the lifecycle of a contract where the contract has ended.</rdfs:comment>
        <rdfs:isDefinedBy rdf:resource="https://www.theworldavatar.com/kg/ontoservice/"/>
        <rdfs:label>Expiration stage</rdfs:label>
    </owl:Class>
    


    <!-- https://www.theworldavatar.com/kg/ontoservice/GrossPrice -->


    <owl:Class rdf:about="https://www.theworldavatar.com/kg/ontoservice/GrossPrice">
        <rdfs:subClassOf rdf:resource="http://www.ontology-of-units-of-measure.org/resource/om-2/AmountOfMoney"/>
        <rdfs:comment>Gross service price for all service charges, excluding taxes.</rdfs:comment>
        <rdfs:isDefinedBy rdf:resource="https://www.theworldavatar.com/kg/ontoservice/"/>
        <rdfs:label>Gross price</rdfs:label>
    </owl:Class>
    


    <!-- https://www.theworldavatar.com/kg/ontoservice/PendingService -->


    <owl:Class rdf:about="https://www.theworldavatar.com/kg/ontoservice/PendingService">
        <rdfs:subClassOf rdf:resource="https://spec.edmcouncil.org/fibo/ontology/FBC/ProductsAndServices/FinancialProductsAndServices/ContractLifecycleEvent"/>
        <rdfs:comment>A service event that is currently scheduled but has not yet started during the service execution lifecycle stage of a contract.</rdfs:comment>
        <rdfs:isDefinedBy rdf:resource="https://www.theworldavatar.com/kg/ontoservice/"/>
        <rdfs:label>Pending service</rdfs:label>
    </owl:Class>
    


    <!-- https://www.theworldavatar.com/kg/ontoservice/ServiceCommitment -->


    <owl:Class rdf:about="https://www.theworldavatar.com/kg/ontoservice/ServiceCommitment">
        <rdfs:subClassOf rdf:resource="https://spec.edmcouncil.org/fibo/ontology/FND/Agreements/Contracts/ContractualCommitment"/>
        <rdfs:comment>General conditions for the services that the contracting parties agree to.</rdfs:comment>
        <rdfs:isDefinedBy rdf:resource="https://www.theworldavatar.com/kg/ontoservice/"/>
        <rdfs:label>Service commitment</rdfs:label>
    </owl:Class>
    


    <!-- https://www.theworldavatar.com/kg/ontoservice/ServiceExecutionStage -->


    <owl:Class rdf:about="https://www.theworldavatar.com/kg/ontoservice/ServiceExecutionStage">
        <rdfs:subClassOf rdf:resource="https://spec.edmcouncil.org/fibo/ontology/FBC/ProductsAndServices/FinancialProductsAndServices/ContractLifecycleStage"/>
        <rdfs:comment>The phase in the lifecycle of a contract where the services agreed should be executed.</rdfs:comment>
        <rdfs:isDefinedBy rdf:resource="https://www.theworldavatar.com/kg/ontoservice/"/>
        <rdfs:label>Service execution stage</rdfs:label>
    </owl:Class>
    


    <!-- https://www.theworldavatar.com/kg/ontoservice/ServiceInProgress -->


    <owl:Class rdf:about="https://www.theworldavatar.com/kg/ontoservice/ServiceInProgress">
        <rdfs:subClassOf rdf:resource="https://spec.edmcouncil.org/fibo/ontology/FBC/ProductsAndServices/FinancialProductsAndServices/ContractLifecycleEvent"/>
        <rdfs:comment>A service event that is currently in progress during the service execution lifecycle stage of a contract.</rdfs:comment>
        <rdfs:isDefinedBy rdf:resource="https://www.theworldavatar.com/kg/ontoservice/"/>
        <rdfs:label>Service in progress</rdfs:label>
    </owl:Class>
    


    <!-- https://www.theworldavatar.com/kg/ontoservice/ServiceInProgressOccurrence -->


    <owl:Class rdf:about="https://www.theworldavatar.com/kg/ontoservice/ServiceInProgressOccurrence">
        <rdfs:subClassOf rdf:resource="https://spec.edmcouncil.org/fibo/ontology/FBC/ProductsAndServices/FinancialProductsAndServices/ContractLifecycleEventOccurrence"/>
        <rdfs:comment>An actual occurrence of the service in progress event.</rdfs:comment>
        <rdfs:isDefinedBy rdf:resource="https://www.theworldavatar.com/kg/ontoservice/"/>
        <rdfs:label>Service in progress occurrence</rdfs:label>
    </owl:Class>
    


    <!-- https://www.theworldavatar.com/kg/ontoservice/ServiceMetric -->


    <owl:Class rdf:about="https://www.theworldavatar.com/kg/ontoservice/ServiceMetric">
        <rdfs:comment>A quantifiable measure to evaluate and track the performance, quality, or efficiency of a service against predefined standards and expectations. These metrics include response time, weight, and customer satisfaction, among others.</rdfs:comment>
        <rdfs:isDefinedBy rdf:resource="https://www.theworldavatar.com/kg/ontoservice/"/>
        <rdfs:label>Service metric</rdfs:label>
    </owl:Class>
    


    <!-- https://www.theworldavatar.com/kg/ontoservice/ServiceMetricCap -->


    <owl:Class rdf:about="https://www.theworldavatar.com/kg/ontoservice/ServiceMetricCap">
        <rdfs:subClassOf rdf:resource="https://www.theworldavatar.com/kg/ontoservice/ServiceMetric"/>
        <rdfs:comment>The maximum allowable value for the metric defined in the service agreement.</rdfs:comment>
        <rdfs:isDefinedBy rdf:resource="https://www.theworldavatar.com/kg/ontoservice/"/>
        <rdfs:label>Service metric cap</rdfs:label>
    </owl:Class>
    


    <!-- https://www.theworldavatar.com/kg/ontoservice/ServicePaymentObligation -->


    <owl:Class rdf:about="https://www.theworldavatar.com/kg/ontoservice/ServicePaymentObligation">
        <rdfs:subClassOf rdf:resource="https://spec.edmcouncil.org/fibo/ontology/FND/ProductsAndServices/PaymentsAndSchedules/PaymentObligation"/>
        <rdfs:comment>Legally enforceable duty and payment terms for the associated service stated in a service agreement.</rdfs:comment>
        <rdfs:isDefinedBy rdf:resource="https://www.theworldavatar.com/kg/ontoservice/"/>
        <rdfs:label>Service payment obligation</rdfs:label>
    </owl:Class>
    


    <!-- https://www.theworldavatar.com/kg/ontoservice/ServiceTonnage -->


    <owl:Class rdf:about="https://www.theworldavatar.com/kg/ontoservice/ServiceTonnage">
        <rdfs:subClassOf rdf:resource="https://www.theworldavatar.com/kg/ontoservice/ServiceMetric"/>
        <rdfs:subClassOf>
            <owl:Restriction>
                <owl:onProperty rdf:resource="https://www.theworldavatar.com/kg/ontoservice/hasQuantity"/>
                <owl:allValuesFrom rdf:resource="http://www.ontology-of-units-of-measure.org/resource/om-2/Mass"/>
            </owl:Restriction>
        </rdfs:subClassOf>
        <rdfs:comment>The quantifiable weight measured in tons when the service is performed.</rdfs:comment>
        <rdfs:isDefinedBy rdf:resource="https://www.theworldavatar.com/kg/ontoservice/"/>
        <rdfs:label>Service tonnage</rdfs:label>
    </owl:Class>
    


    <!-- https://www.theworldavatar.com/kg/ontoservice/Tax -->


    <owl:Class rdf:about="https://www.theworldavatar.com/kg/ontoservice/Tax">
        <rdfs:subClassOf rdf:resource="http://www.ontology-of-units-of-measure.org/resource/om-2/Percentage"/>
        <rdfs:comment>A tax rate incurred upon the service.</rdfs:comment>
        <rdfs:isDefinedBy rdf:resource="https://www.theworldavatar.com/kg/ontoservice/"/>
        <rdfs:label>Tax</rdfs:label>
    </owl:Class>
    


    <!-- https://www.theworldavatar.com/kg/ontoservice/TerminatedService -->


    <owl:Class rdf:about="https://www.theworldavatar.com/kg/ontoservice/TerminatedService">
        <rdfs:subClassOf rdf:resource="https://spec.edmcouncil.org/fibo/ontology/FBC/ProductsAndServices/FinancialProductsAndServices/ContractLifecycleEvent"/>
        <rdfs:comment>A service event that has not started and will not be delivered during the service execution lifecycle stage of a contract. Remarks should ideally be available to indicate reason for termination.</rdfs:comment>
        <rdfs:isDefinedBy rdf:resource="https://www.theworldavatar.com/kg/ontoservice/"/>
        <rdfs:label>Terminated service</rdfs:label>
    </owl:Class>
    


    <!-- https://www.theworldavatar.com/kg/ontoservice/TotalPrice -->


    <owl:Class rdf:about="https://www.theworldavatar.com/kg/ontoservice/TotalPrice">
        <rdfs:subClassOf rdf:resource="http://www.ontology-of-units-of-measure.org/resource/om-2/AmountOfMoney"/>
        <rdfs:comment>The final price that the client should pay for the service, inclusive of taxes.</rdfs:comment>
        <rdfs:isDefinedBy rdf:resource="https://www.theworldavatar.com/kg/ontoservice/"/>
        <rdfs:label>Total price</rdfs:label>
    </owl:Class>
    


    <!-- https://www.theworldavatar.com/kg/ontoservice/UncompletedService -->


    <owl:Class rdf:about="https://www.theworldavatar.com/kg/ontoservice/UncompletedService">
        <rdfs:subClassOf rdf:resource="https://spec.edmcouncil.org/fibo/ontology/FBC/ProductsAndServices/FinancialProductsAndServices/ContractLifecycleEvent"/>
        <rdfs:comment>A service event that has been started but is not completed during the service execution lifecycle stage of a contract. Remarks should ideally be available to indicate reason for the failure to complete.</rdfs:comment>
        <rdfs:isDefinedBy rdf:resource="https://www.theworldavatar.com/kg/ontoservice/"/>
        <rdfs:label>Uncompleted service</rdfs:label>
    </owl:Class>
    


    <!-- https://www.theworldavatar.com/kg/ontoservice/UncompletedServiceOccurrence -->


    <owl:Class rdf:about="https://www.theworldavatar.com/kg/ontoservice/UncompletedServiceOccurrence">
        <rdfs:subClassOf rdf:resource="https://spec.edmcouncil.org/fibo/ontology/FBC/ProductsAndServices/FinancialProductsAndServices/ContractLifecycleEventOccurrence"/>
        <rdfs:comment>An actual occurrence of an uncompleted service event.</rdfs:comment>
        <rdfs:isDefinedBy rdf:resource="https://www.theworldavatar.com/kg/ontoservice/"/>
        <rdfs:label>Uncompleted service occurrence</rdfs:label>
    </owl:Class>
    


    <!-- https://www.theworldavatar.com/kg/ontoservice/VariableCharge -->


    <owl:Class rdf:about="https://www.theworldavatar.com/kg/ontoservice/VariableCharge">
        <rdfs:subClassOf rdf:resource="http://www.ontology-of-units-of-measure.org/resource/om-2/AmountOfMoney"/>
        <rdfs:comment>A charge that depends on the outcome of a service after execution, agreed upon in the contract.</rdfs:comment>
        <rdfs:isDefinedBy rdf:resource="https://www.theworldavatar.com/kg/ontoservice/"/>
        <rdfs:label>Variable charge</rdfs:label>
    </owl:Class>
    


    <!-- https://www.theworldavatar.com/kg/ontoservice/VariableRate -->


    <owl:Class rdf:about="https://www.theworldavatar.com/kg/ontoservice/VariableRate">
        <rdfs:comment>The rates that is dependent on the outcome of a service after execution, agreed upon in the contract.</rdfs:comment>
        <rdfs:isDefinedBy rdf:resource="https://www.theworldavatar.com/kg/ontoservice/"/>
        <rdfs:label>Variable rate</rdfs:label>
    </owl:Class>
</rdf:RDF>



<!-- Generated by the OWL API (version 5.5.0.2023-01-14T12:41:38Z) https://github.com/owlcs/owlapi/ -->


