<?xml version="1.0"?>
<rdf:RDF xmlns="https://www.theworldavatar.com/kg/ontoservice/"
     xml:base="https://www.theworldavatar.com/kg/ontoservice/"
     xmlns:dc="http://purl.org/dc/elements/1.1/"
     xmlns:owl="http://www.w3.org/2002/07/owl#"
     xmlns:rdf="http://www.w3.org/1999/02/22-rdf-syntax-ns#"
     xmlns:xml="http://www.w3.org/XML/1998/namespace"
     xmlns:xsd="http://www.w3.org/2001/XMLSchema#"
     xmlns:rdfs="http://www.w3.org/2000/01/rdf-schema#"
     xmlns:ontoservice="https://www.theworldavatar.com/kg/ontoservice/">
    <owl:Ontology rdf:about="https://www.theworldavatar.com/kg/ontoservice/">
        <dc:date>23 August 2024</dc:date>
        <rdfs:comment>OntoService is designed to represent the terms, conditions, and obligations associated with service delivery as well as the execution details.</rdfs:comment>
        <owl:versionInfo>1</owl:versionInfo>
        <gitCommitHash>c0599beca8df55873a1ab061dee64e52c510c6a0</gitCommitHash>
    </owl:Ontology>
    


    <!-- 
    ///////////////////////////////////////////////////////////////////////////////////////
    //
    // Annotation properties
    //
    ///////////////////////////////////////////////////////////////////////////////////////
     -->


    


    <!-- http://purl.org/dc/elements/1.1/date -->


    <owl:AnnotationProperty rdf:about="http://purl.org/dc/elements/1.1/date"/>
    


    <!-- https://www.theworldavatar.com/kg/ontoservice/gitCommitHash -->


    <owl:AnnotationProperty rdf:about="https://www.theworldavatar.com/kg/ontoservice/gitCommitHash"/>
    


    <!-- 
    ///////////////////////////////////////////////////////////////////////////////////////
    //
    // Object Properties
    //
    ///////////////////////////////////////////////////////////////////////////////////////
     -->


    


    <!-- https://www.theworldavatar.com/kg/ontoservice/assignTransport -->


    <owl:ObjectProperty rdf:about="https://www.theworldavatar.com/kg/ontoservice/assignTransport">
        <rdfs:domain rdf:resource="https://www.theworldavatar.com/kg/ontoservice/ServiceEvent"/>
        <rdfs:range rdf:resource="https://spec.edmcouncil.org/auto/ontology/VC/VehicleCore/Vehicle"/>
        <rdfs:comment>A relationship assigning a transport vehicle to a service event.</rdfs:comment>
        <rdfs:isDefinedBy rdf:resource="https://www.theworldavatar.com/kg/ontoservice/"/>
        <rdfs:label>assign transport</rdfs:label>
    </owl:ObjectProperty>
    


    <!-- https://www.theworldavatar.com/kg/ontoservice/charges -->


    <owl:ObjectProperty rdf:about="https://www.theworldavatar.com/kg/ontoservice/charges">
        <rdfs:domain rdf:resource="https://www.theworldavatar.com/kg/ontoservice/ServiceEvent"/>
        <rdfs:range rdf:resource="https://www.theworldavatar.com/kg/ontoservice/TotalPrice"/>
        <rdfs:comment>A relationship describing the final charge of a service event.</rdfs:comment>
        <rdfs:isDefinedBy rdf:resource="https://www.theworldavatar.com/kg/ontoservice/"/>
        <rdfs:label>charges</rdfs:label>
    </owl:ObjectProperty>
    


    <!-- https://www.theworldavatar.com/kg/ontoservice/dependsOn -->


    <owl:ObjectProperty rdf:about="https://www.theworldavatar.com/kg/ontoservice/dependsOn">
        <rdfs:domain rdf:resource="https://www.theworldavatar.com/kg/ontoservice/VariableRate"/>
        <rdfs:range rdf:resource="https://www.theworldavatar.com/kg/ontoservice/ServiceMetric"/>
        <rdfs:comment>A relationship describing the service metric that the variable rate is based on.</rdfs:comment>
        <rdfs:isDefinedBy rdf:resource="https://www.theworldavatar.com/kg/ontoservice/"/>
        <rdfs:label>depends on</rdfs:label>
    </owl:ObjectProperty>
    


    <!-- https://www.theworldavatar.com/kg/ontoservice/hasBaseCharge -->


    <owl:ObjectProperty rdf:about="https://www.theworldavatar.com/kg/ontoservice/hasBaseCharge">
        <rdfs:domain rdf:resource="https://www.theworldavatar.com/kg/ontoservice/ServicePaymentObligation"/>
        <rdfs:range rdf:resource="https://www.theworldavatar.com/kg/ontoservice/BaseCharge"/>
        <rdfs:comment>A relationship describing a legally enforceable base charge for each service.</rdfs:comment>
        <rdfs:isDefinedBy rdf:resource="https://www.theworldavatar.com/kg/ontoservice/"/>
        <rdfs:label>has base charge</rdfs:label>
    </owl:ObjectProperty>
    


    <!-- https://www.theworldavatar.com/kg/ontoservice/hasDenominator -->


    <owl:ObjectProperty rdf:about="https://www.theworldavatar.com/kg/ontoservice/hasDenominator">
        <rdfs:domain rdf:resource="https://www.theworldavatar.com/kg/ontoservice/VariableRate"/>
        <rdfs:range rdf:resource="http://www.ontology-of-units-of-measure.org/resource/om-2/Quantity"/>
        <rdfs:comment>A relationship defining the denominator of a monetary rate, which depends on the service metric.</rdfs:comment>
        <rdfs:isDefinedBy rdf:resource="https://www.theworldavatar.com/kg/ontoservice/"/>
        <rdfs:label>has denominator</rdfs:label>
    </owl:ObjectProperty>
    


    <!-- https://www.theworldavatar.com/kg/ontoservice/hasEvent -->


    <owl:ObjectProperty rdf:about="https://www.theworldavatar.com/kg/ontoservice/hasEvent">
        <rdfs:domain rdf:resource="https://spec.edmcouncil.org/fibo/ontology/FND/ProductsAndServices/ProductsAndServices/Service"/>
        <rdfs:range rdf:resource="https://www.theworldavatar.com/kg/ontoservice/ServiceEvent"/>
        <rdfs:comment>A relationship defining the specific occurrences of each service performed for the corresponding service.</rdfs:comment>
        <rdfs:isDefinedBy rdf:resource="https://www.theworldavatar.com/kg/ontoservice/"/>
        <rdfs:label>has event</rdfs:label>
    </owl:ObjectProperty>
    


    <!-- https://www.theworldavatar.com/kg/ontoservice/hasNumerator -->


    <owl:ObjectProperty rdf:about="https://www.theworldavatar.com/kg/ontoservice/hasNumerator">
        <rdfs:domain rdf:resource="https://www.theworldavatar.com/kg/ontoservice/VariableRate"/>
        <rdfs:range rdf:resource="http://www.ontology-of-units-of-measure.org/resource/om-2/AmountOfMoney"/>
        <rdfs:comment>A relationship defining the numerator of a monetary rate, which should be amount of money.</rdfs:comment>
        <rdfs:isDefinedBy rdf:resource="https://www.theworldavatar.com/kg/ontoservice/"/>
        <rdfs:label>has numerator</rdfs:label>
    </owl:ObjectProperty>
    


    <!-- https://www.theworldavatar.com/kg/ontoservice/hasQuantity -->


    <owl:ObjectProperty rdf:about="https://www.theworldavatar.com/kg/ontoservice/hasQuantity">
        <rdfs:domain rdf:resource="https://www.theworldavatar.com/kg/ontoservice/ServiceMetric"/>
        <rdfs:domain rdf:resource="https://www.theworldavatar.com/kg/ontoservice/ServiceTonnage"/>
        <rdfs:range rdf:resource="http://www.ontology-of-units-of-measure.org/resource/om-2/Mass"/>
        <rdfs:range rdf:resource="http://www.ontology-of-units-of-measure.org/resource/om-2/Quantity"/>
        <rdfs:comment>A relationship defining the quantity of a service metric.</rdfs:comment>
        <rdfs:isDefinedBy rdf:resource="https://www.theworldavatar.com/kg/ontoservice/"/>
        <rdfs:label>has quantity</rdfs:label>
    </owl:ObjectProperty>
    


    <!-- https://www.theworldavatar.com/kg/ontoservice/hasStatus -->


    <owl:ObjectProperty rdf:about="https://www.theworldavatar.com/kg/ontoservice/hasStatus">
        <rdfs:domain rdf:resource="https://www.theworldavatar.com/kg/ontoservice/ServiceEvent"/>
        <rdfs:range rdf:resource="https://www.theworldavatar.com/kg/ontoservice/ServiceStatus"/>
        <rdfs:comment>A relationship describing the current status of a service event.</rdfs:comment>
        <rdfs:isDefinedBy rdf:resource="https://www.theworldavatar.com/kg/ontoservice/"/>
        <rdfs:label>has status</rdfs:label>
    </owl:ObjectProperty>
    


    <!-- https://www.theworldavatar.com/kg/ontoservice/hasVariableRate -->


    <owl:ObjectProperty rdf:about="https://www.theworldavatar.com/kg/ontoservice/hasVariableRate">
        <rdfs:domain rdf:resource="https://www.theworldavatar.com/kg/ontoservice/ServicePaymentObligation"/>
        <rdfs:range rdf:resource="https://www.theworldavatar.com/kg/ontoservice/VariableRate"/>
        <rdfs:comment>A relationship describing a legally enforceable variable rate for a service based on certain parameters.</rdfs:comment>
        <rdfs:isDefinedBy rdf:resource="https://www.theworldavatar.com/kg/ontoservice/"/>
        <rdfs:label>has variable rate</rdfs:label>
    </owl:ObjectProperty>
    


    <!-- https://www.theworldavatar.com/kg/ontoservice/services -->


    <owl:ObjectProperty rdf:about="https://www.theworldavatar.com/kg/ontoservice/services">
        <rdfs:domain rdf:resource="https://spec.edmcouncil.org/fibo/ontology/FND/ProductsAndServices/ProductsAndServices/Service"/>
        <rdfs:range rdf:resource="https://www.theworldavatar.com/kg/ontobim/Facility"/>
        <rdfs:comment>A relationship describing the facility that the service should be executed on.</rdfs:comment>
        <rdfs:isDefinedBy rdf:resource="https://www.theworldavatar.com/kg/ontoservice/"/>
        <rdfs:label>services</rdfs:label>
    </owl:ObjectProperty>
    


    <!-- 
    ///////////////////////////////////////////////////////////////////////////////////////
    //
    // Data properties
    //
    ///////////////////////////////////////////////////////////////////////////////////////
     -->


    


    <!-- https://www.theworldavatar.com/kg/ontoservice/completedOn -->


    <owl:DatatypeProperty rdf:about="https://www.theworldavatar.com/kg/ontoservice/completedOn">
        <rdfs:domain rdf:resource="https://www.theworldavatar.com/kg/ontoservice/ServiceEvent"/>
        <rdfs:range rdf:resource="http://www.w3.org/2001/XMLSchema#dateTime"/>
        <rdfs:comment>A relationship describing  the actual date and time of a completed service.</rdfs:comment>
        <rdfs:isDefinedBy rdf:resource="https://www.theworldavatar.com/kg/ontoservice/"/>
        <rdfs:label>completed on</rdfs:label>
    </owl:DatatypeProperty>
    


    <!-- https://www.theworldavatar.com/kg/ontoservice/hasOrderNumber -->


    <owl:DatatypeProperty rdf:about="https://www.theworldavatar.com/kg/ontoservice/hasOrderNumber">
        <rdfs:domain rdf:resource="https://www.theworldavatar.com/kg/ontoservice/ServiceEvent"/>
        <rdfs:range rdf:resource="http://www.w3.org/2001/XMLSchema#string"/>
        <rdfs:comment>A relationship definining the unique identifier of a service for reporting and billing.</rdfs:comment>
        <rdfs:isDefinedBy rdf:resource="https://www.theworldavatar.com/kg/ontoservice/"/>
        <rdfs:label>has order number</rdfs:label>
    </owl:DatatypeProperty>
    


    <!-- https://www.theworldavatar.com/kg/ontoservice/hasPreferredTime -->


    <owl:DatatypeProperty rdf:about="https://www.theworldavatar.com/kg/ontoservice/hasPreferredTime">
        <rdfs:domain rdf:resource="https://www.theworldavatar.com/kg/ontoservice/ServiceCommitment"/>
        <rdfs:range rdf:resource="http://www.w3.org/2001/XMLSchema#string"/>
        <rdfs:comment>The preferred time to perform the service. Note that the scheduler may not always be able to meet this time depending on various factors on the day of service.</rdfs:comment>
        <rdfs:isDefinedBy rdf:resource="https://www.theworldavatar.com/kg/ontoservice/"/>
        <rdfs:label>has preferred time</rdfs:label>
    </owl:DatatypeProperty>
    


    <!-- https://www.theworldavatar.com/kg/ontoservice/scheduledOn -->


    <owl:DatatypeProperty rdf:about="https://www.theworldavatar.com/kg/ontoservice/scheduledOn">
        <rdfs:domain rdf:resource="https://www.theworldavatar.com/kg/ontoservice/ServiceEvent"/>
        <rdfs:range rdf:resource="http://www.w3.org/2001/XMLSchema#dateTime"/>
        <rdfs:comment>A relationship describing  the scheduled date and time of a service.</rdfs:comment>
        <rdfs:isDefinedBy rdf:resource="https://www.theworldavatar.com/kg/ontoservice/"/>
        <rdfs:label>scheduled on</rdfs:label>
    </owl:DatatypeProperty>
    


    <!-- 
    ///////////////////////////////////////////////////////////////////////////////////////
    //
    // Classes
    //
    ///////////////////////////////////////////////////////////////////////////////////////
     -->


    


    <!-- http://www.ontology-of-units-of-measure.org/resource/om-2/AmountOfMoney -->


    <owl:Class rdf:about="http://www.ontology-of-units-of-measure.org/resource/om-2/AmountOfMoney"/>
    


    <!-- http://www.ontology-of-units-of-measure.org/resource/om-2/Mass -->


    <owl:Class rdf:about="http://www.ontology-of-units-of-measure.org/resource/om-2/Mass"/>
    


    <!-- http://www.ontology-of-units-of-measure.org/resource/om-2/Percentage -->


    <owl:Class rdf:about="http://www.ontology-of-units-of-measure.org/resource/om-2/Percentage"/>
    


    <!-- http://www.ontology-of-units-of-measure.org/resource/om-2/Quantity -->


    <owl:Class rdf:about="http://www.ontology-of-units-of-measure.org/resource/om-2/Quantity"/>
    


    <!-- https://spec.edmcouncil.org/auto/ontology/VC/VehicleCore/Vehicle -->


    <owl:Class rdf:about="https://spec.edmcouncil.org/auto/ontology/VC/VehicleCore/Vehicle"/>
    


    <!-- https://spec.edmcouncil.org/fibo/ontology/FND/Agreements/Contracts/ContractualCommitment -->


    <owl:Class rdf:about="https://spec.edmcouncil.org/fibo/ontology/FND/Agreements/Contracts/ContractualCommitment"/>
    


    <!-- https://spec.edmcouncil.org/fibo/ontology/FND/ProductsAndServices/PaymentsAndSchedules/PaymentObligation -->


    <owl:Class rdf:about="https://spec.edmcouncil.org/fibo/ontology/FND/ProductsAndServices/PaymentsAndSchedules/PaymentObligation"/>
    


    <!-- https://spec.edmcouncil.org/fibo/ontology/FND/ProductsAndServices/ProductsAndServices/Service -->


    <owl:Class rdf:about="https://spec.edmcouncil.org/fibo/ontology/FND/ProductsAndServices/ProductsAndServices/Service"/>
    


    <!-- https://www.theworldavatar.com/kg/ontobim/Facility -->


    <owl:Class rdf:about="https://www.theworldavatar.com/kg/ontobim/Facility"/>
    


    <!-- https://www.theworldavatar.com/kg/ontoservice/BaseCharge -->


    <owl:Class rdf:about="https://www.theworldavatar.com/kg/ontoservice/BaseCharge">
        <rdfs:subClassOf rdf:resource="http://www.ontology-of-units-of-measure.org/resource/om-2/AmountOfMoney"/>
        <rdfs:comment>A base charge for the service agreed in the contract.</rdfs:comment>
        <rdfs:isDefinedBy rdf:resource="https://www.theworldavatar.com/kg/ontoservice/"/>
        <rdfs:label>Base charge</rdfs:label>
    </owl:Class>
    


    <!-- https://www.theworldavatar.com/kg/ontoservice/ExcessVariableRate -->


    <owl:Class rdf:about="https://www.theworldavatar.com/kg/ontoservice/ExcessVariableRate">
        <rdfs:subClassOf rdf:resource="https://www.theworldavatar.com/kg/ontoservice/VariableRate"/>
        <rdfs:subClassOf>
            <owl:Restriction>
                <owl:onProperty rdf:resource="https://www.theworldavatar.com/kg/ontoservice/dependsOn"/>
                <owl:allValuesFrom rdf:resource="https://www.theworldavatar.com/kg/ontoservice/ServiceMetricCap"/>
            </owl:Restriction>
        </rdfs:subClassOf>
        <rdfs:comment>The rates that is dependent on the outcome of a service after execution, agreed upon in the contract. Specifically, this rate will be in effect once the service exceeds the cap specified.</rdfs:comment>
        <rdfs:isDefinedBy rdf:resource="https://www.theworldavatar.com/kg/ontoservice/"/>
        <rdfs:label>Excess variable rate</rdfs:label>
    </owl:Class>
    


    <!-- https://www.theworldavatar.com/kg/ontoservice/GrossPrice -->


    <owl:Class rdf:about="https://www.theworldavatar.com/kg/ontoservice/GrossPrice">
        <rdfs:subClassOf rdf:resource="http://www.ontology-of-units-of-measure.org/resource/om-2/AmountOfMoney"/>
        <rdfs:comment>Gross service price for all service charges, excluding taxes.</rdfs:comment>
        <rdfs:isDefinedBy rdf:resource="https://www.theworldavatar.com/kg/ontoservice/"/>
        <rdfs:label>Gross price</rdfs:label>
    </owl:Class>
    


    <!-- https://www.theworldavatar.com/kg/ontoservice/ServiceCommitment -->


    <owl:Class rdf:about="https://www.theworldavatar.com/kg/ontoservice/ServiceCommitment">
        <rdfs:subClassOf rdf:resource="https://spec.edmcouncil.org/fibo/ontology/FND/Agreements/Contracts/ContractualCommitment"/>
        <rdfs:comment>General conditions for the services that the contracting parties agree to.</rdfs:comment>
        <rdfs:isDefinedBy rdf:resource="https://www.theworldavatar.com/kg/ontoservice/"/>
        <rdfs:label>Service commitment</rdfs:label>
    </owl:Class>
    


    <!-- https://www.theworldavatar.com/kg/ontoservice/ServiceEvent -->


    <owl:Class rdf:about="https://www.theworldavatar.com/kg/ontoservice/ServiceEvent">
        <rdfs:comment>A specific occurrence or instance of a service being performed, characterised by a particular time and context. Each event capture details such as the date, time, and/or specific actions to record and analyse individual performances for quality, efficiency, and compliance with service agreements.</rdfs:comment>
        <rdfs:isDefinedBy rdf:resource="https://www.theworldavatar.com/kg/ontoservice/"/>
        <rdfs:label>Service event</rdfs:label>
    </owl:Class>
    


    <!-- https://www.theworldavatar.com/kg/ontoservice/ServiceMetric -->


    <owl:Class rdf:about="https://www.theworldavatar.com/kg/ontoservice/ServiceMetric">
        <rdfs:comment>A quantifiable measure to evaluate and track the performance, quality, or efficiency of a service against predefined standards and expectations. These metrics include response time, weight, and customer satisfaction, among others.</rdfs:comment>
        <rdfs:isDefinedBy rdf:resource="https://www.theworldavatar.com/kg/ontoservice/"/>
        <rdfs:label>Service metric</rdfs:label>
    </owl:Class>
    


    <!-- https://www.theworldavatar.com/kg/ontoservice/ServiceMetricCap -->


    <owl:Class rdf:about="https://www.theworldavatar.com/kg/ontoservice/ServiceMetricCap">
        <rdfs:subClassOf rdf:resource="https://www.theworldavatar.com/kg/ontoservice/ServiceMetric"/>
        <rdfs:comment>The maximum allowable value for the metric defined in the service agreement.</rdfs:comment>
        <rdfs:isDefinedBy rdf:resource="https://www.theworldavatar.com/kg/ontoservice/"/>
        <rdfs:label>Service metric cap</rdfs:label>
    </owl:Class>
    


    <!-- https://www.theworldavatar.com/kg/ontoservice/ServicePaymentObligation -->


    <owl:Class rdf:about="https://www.theworldavatar.com/kg/ontoservice/ServicePaymentObligation">
        <rdfs:subClassOf rdf:resource="https://spec.edmcouncil.org/fibo/ontology/FND/ProductsAndServices/PaymentsAndSchedules/PaymentObligation"/>
        <rdfs:comment>Legally enforceable duty and payment terms for the associated service stated in a service agreement.</rdfs:comment>
        <rdfs:isDefinedBy rdf:resource="https://www.theworldavatar.com/kg/ontoservice/"/>
        <rdfs:label>Service payment obligation</rdfs:label>
    </owl:Class>
    


    <!-- https://www.theworldavatar.com/kg/ontoservice/ServiceStatus -->


    <owl:Class rdf:about="https://www.theworldavatar.com/kg/ontoservice/ServiceStatus">
        <rdfs:comment>The current state of a service.</rdfs:comment>
        <rdfs:isDefinedBy rdf:resource="https://www.theworldavatar.com/kg/ontoservice/"/>
        <rdfs:label>Service status</rdfs:label>
    </owl:Class>
    


    <!-- https://www.theworldavatar.com/kg/ontoservice/ServiceStatusEnum -->


    <owl:Class rdf:about="https://www.theworldavatar.com/kg/ontoservice/ServiceStatusEnum">
        <rdfs:subClassOf rdf:resource="https://www.theworldavatar.com/kg/ontoservice/ServiceStatus"/>
        <rdfs:comment>The enumerated states belonging to the service status, including awaiting scheduling, in review, in queue, in progress, completed.</rdfs:comment>
        <rdfs:isDefinedBy rdf:resource="https://www.theworldavatar.com/kg/ontoservice/"/>
        <rdfs:label>Service status enum</rdfs:label>
    </owl:Class>
    


    <!-- https://www.theworldavatar.com/kg/ontoservice/ServiceTonnage -->


    <owl:Class rdf:about="https://www.theworldavatar.com/kg/ontoservice/ServiceTonnage">
        <rdfs:subClassOf rdf:resource="https://www.theworldavatar.com/kg/ontoservice/ServiceMetric"/>
        <rdfs:subClassOf>
            <owl:Restriction>
                <owl:onProperty rdf:resource="https://www.theworldavatar.com/kg/ontoservice/hasQuantity"/>
                <owl:allValuesFrom rdf:resource="http://www.ontology-of-units-of-measure.org/resource/om-2/Mass"/>
            </owl:Restriction>
        </rdfs:subClassOf>
        <rdfs:comment>The quantifiable weight measured in tons when the service is performed.</rdfs:comment>
        <rdfs:isDefinedBy rdf:resource="https://www.theworldavatar.com/kg/ontoservice/"/>
        <rdfs:label>Service tonnage</rdfs:label>
    </owl:Class>
    


    <!-- https://www.theworldavatar.com/kg/ontoservice/Tax -->


    <owl:Class rdf:about="https://www.theworldavatar.com/kg/ontoservice/Tax">
        <rdfs:subClassOf rdf:resource="http://www.ontology-of-units-of-measure.org/resource/om-2/Percentage"/>
        <rdfs:comment>A tax rate incurred upon the service.</rdfs:comment>
        <rdfs:isDefinedBy rdf:resource="https://www.theworldavatar.com/kg/ontoservice/"/>
        <rdfs:label>Tax</rdfs:label>
    </owl:Class>
    


    <!-- https://www.theworldavatar.com/kg/ontoservice/TotalPrice -->


    <owl:Class rdf:about="https://www.theworldavatar.com/kg/ontoservice/TotalPrice">
        <rdfs:subClassOf rdf:resource="http://www.ontology-of-units-of-measure.org/resource/om-2/AmountOfMoney"/>
        <rdfs:comment>The final price that the client should pay for the service, inclusive of taxes.</rdfs:comment>
        <rdfs:isDefinedBy rdf:resource="https://www.theworldavatar.com/kg/ontoservice/"/>
        <rdfs:label>Total price</rdfs:label>
    </owl:Class>
    


    <!-- https://www.theworldavatar.com/kg/ontoservice/VariableCharge -->


    <owl:Class rdf:about="https://www.theworldavatar.com/kg/ontoservice/VariableCharge">
        <rdfs:subClassOf rdf:resource="http://www.ontology-of-units-of-measure.org/resource/om-2/AmountOfMoney"/>
        <rdfs:comment>A charge that depends on the outcome of a service after execution, agreed upon in the contract.</rdfs:comment>
        <rdfs:isDefinedBy rdf:resource="https://www.theworldavatar.com/kg/ontoservice/"/>
        <rdfs:label>Variable charge</rdfs:label>
    </owl:Class>
    


    <!-- https://www.theworldavatar.com/kg/ontoservice/VariableRate -->


    <owl:Class rdf:about="https://www.theworldavatar.com/kg/ontoservice/VariableRate">
        <rdfs:comment>The rates that is dependent on the outcome of a service after execution, agreed upon in the contract.</rdfs:comment>
        <rdfs:isDefinedBy rdf:resource="https://www.theworldavatar.com/kg/ontoservice/"/>
        <rdfs:label>Variable rate</rdfs:label>
    </owl:Class>
</rdf:RDF>



<!-- Generated by the OWL API (version 5.5.0.2023-01-14T12:41:38Z) https://github.com/owlcs/owlapi/ -->


