<?xml version="1.0"?>
<rdf:RDF xmlns="https://www.theworldavatar.com/kg/ontodevice/"
     xml:base="https://www.theworldavatar.com/kg/ontodevice/"
     xmlns:dc="http://purl.org/dc/elements/1.1/"
     xmlns:owl="http://www.w3.org/2002/07/owl#"
     xmlns:rdf="http://www.w3.org/1999/02/22-rdf-syntax-ns#"
     xmlns:xml="http://www.w3.org/XML/1998/namespace"
     xmlns:xsd="http://www.w3.org/2001/XMLSchema#"
     xmlns:rdfs="http://www.w3.org/2000/01/rdf-schema#"
     xmlns:ontodevice="https://www.theworldavatar.com/kg/ontodevice/">
    <owl:Ontology rdf:about="https://www.theworldavatar.com/kg/ontodevice/">
        <owl:imports rdf:resource="https://saref.etsi.org/core/"/>
        <dc:date>04 June 2024</dc:date>
        <rdfs:comment>OntoDevice is an ontology for describing devices, their capabilities and properties.</rdfs:comment>
        <owl:versionInfo>1.5</owl:versionInfo>
        <gitCommitHash>c0599beca8df55873a1ab061dee64e52c510c6a0</gitCommitHash>
    </owl:Ontology>
    


    <!-- 
    ///////////////////////////////////////////////////////////////////////////////////////
    //
    // Annotation properties
    //
    ///////////////////////////////////////////////////////////////////////////////////////
     -->


    


    <!-- http://purl.org/dc/elements/1.1/date -->


    <owl:AnnotationProperty rdf:about="http://purl.org/dc/elements/1.1/date"/>
    


    <!-- https://www.theworldavatar.com/kg/ontodevice/gitCommitHash -->


    <owl:AnnotationProperty rdf:about="https://www.theworldavatar.com/kg/ontodevice/gitCommitHash"/>
    


    <!-- 
    ///////////////////////////////////////////////////////////////////////////////////////
    //
    // Object Properties
    //
    ///////////////////////////////////////////////////////////////////////////////////////
     -->


    


    <!-- https://www.theworldavatar.com/kg/ontodevice/hasA -->


    <owl:ObjectProperty rdf:about="https://www.theworldavatar.com/kg/ontodevice/hasA">
        <rdfs:domain rdf:resource="https://spec.edmcouncil.org/fibo/ontology/FND/Parties/Parties/IndependentParty"/>
        <rdfs:range rdf:resource="https://www.theworldavatar.com/kg/ontodevice/Device"/>
        <rdfs:comment>A relationship that describes a person or organization possessing a device.</rdfs:comment>
        <rdfs:isDefinedBy rdf:resource="https://www.theworldavatar.com/kg/ontodevice/"/>
        <rdfs:label>has a</rdfs:label>
    </owl:ObjectProperty>
    


    <!-- https://www.theworldavatar.com/kg/ontodevice/hasAcidity -->


    <owl:ObjectProperty rdf:about="https://www.theworldavatar.com/kg/ontodevice/hasAcidity">
        <rdfs:subPropertyOf rdf:resource="https://www.theworldavatar.com/kg/ontodevice/hasQuantity"/>
        <rdfs:domain rdf:resource="http://www.theworldavatar.com/kg/ontochemplant#Fluid"/>
        <rdfs:range rdf:resource="http://www.ontology-of-units-of-measure.org/resource/om-2/Acidity"/>
        <rdfs:comment>A relationship describing the acidity of a solution.</rdfs:comment>
        <rdfs:isDefinedBy rdf:resource="https://www.theworldavatar.com/kg/ontodevice/"/>
        <rdfs:label>has acidity</rdfs:label>
    </owl:ObjectProperty>
    


    <!-- https://www.theworldavatar.com/kg/ontodevice/hasControlParameter -->


    <owl:ObjectProperty rdf:about="https://www.theworldavatar.com/kg/ontodevice/hasControlParameter">
        <rdfs:domain rdf:resource="https://www.theworldavatar.com/kg/ontodevice/Device"/>
        <rdfs:range>
            <owl:Class>
                <owl:unionOf rdf:parseType="Collection">
                    <rdf:Description rdf:about="http://www.ontology-of-units-of-measure.org/resource/om-2/Frequency"/>
                    <rdf:Description rdf:about="http://www.ontology-of-units-of-measure.org/resource/om-2/Percentage"/>
                    <rdf:Description rdf:about="http://www.ontology-of-units-of-measure.org/resource/om-2/Pressure"/>
                </owl:unionOf>
            </owl:Class>
        </rdfs:range>
        <rdfs:comment>A relationship between a device and a control parameter.</rdfs:comment>
        <rdfs:isDefinedBy rdf:resource="https://www.theworldavatar.com/kg/ontodevice/"/>
        <rdfs:label>has control parameter</rdfs:label>
    </owl:ObjectProperty>
    


    <!-- https://www.theworldavatar.com/kg/ontodevice/hasCumulativeEnergyConsumption -->


    <owl:ObjectProperty rdf:about="https://www.theworldavatar.com/kg/ontodevice/hasCumulativeEnergyConsumption">
        <rdfs:subPropertyOf rdf:resource="https://www.theworldavatar.com/kg/ontodevice/hasQuantity"/>
        <rdfs:domain>
            <owl:Class>
                <owl:unionOf rdf:parseType="Collection">
                    <rdf:Description rdf:about="http://www.theworldavatar.com/ontology/ontocape/chemical_process_system/CPS_function/process.owl#TemperatureChange"/>
                    <rdf:Description rdf:about="https://www.theworldavatar.com/kg/ontodevice/Device"/>
                </owl:unionOf>
            </owl:Class>
        </rdfs:domain>
        <rdfs:range rdf:resource="http://www.ontology-of-units-of-measure.org/resource/om-2/Energy"/>
        <rdfs:comment>A relationship that describes the amount of cumulative energy used or consumed during a process or by a device.</rdfs:comment>
        <rdfs:isDefinedBy rdf:resource="https://www.theworldavatar.com/kg/ontodevice/"/>
        <rdfs:label>has cumulative energy consumption</rdfs:label>
    </owl:ObjectProperty>
    


    <!-- https://www.theworldavatar.com/kg/ontodevice/hasDefaultPosition -->


    <owl:ObjectProperty rdf:about="https://www.theworldavatar.com/kg/ontodevice/hasDefaultPosition">
        <rdfs:domain rdf:resource="https://www.theworldavatar.com/kg/ontodevice/Valve"/>
        <rdfs:range rdf:resource="https://www.theworldavatar.com/kg/ontodevice/DefaultValvePosition"/>
        <rdfs:comment>A relationship that describes a valve and it's default position (NC, NO etc).</rdfs:comment>
        <rdfs:isDefinedBy rdf:resource="https://www.theworldavatar.com/kg/ontodevice/"/>
        <rdfs:label>has default position</rdfs:label>
    </owl:ObjectProperty>
    


    <!-- https://www.theworldavatar.com/kg/ontodevice/hasFeedbackParameter -->


    <owl:ObjectProperty rdf:about="https://www.theworldavatar.com/kg/ontodevice/hasFeedbackParameter">
        <rdfs:domain rdf:resource="https://www.theworldavatar.com/kg/ontodevice/Device"/>
        <rdfs:range>
            <owl:Class>
                <owl:unionOf rdf:parseType="Collection">
                    <rdf:Description rdf:about="http://www.ontology-of-units-of-measure.org/resource/om-2/Frequency"/>
                    <rdf:Description rdf:about="http://www.ontology-of-units-of-measure.org/resource/om-2/Percentage"/>
                    <rdf:Description rdf:about="http://www.ontology-of-units-of-measure.org/resource/om-2/Pressure"/>
                </owl:unionOf>
            </owl:Class>
        </rdfs:range>
        <rdfs:comment>A relationship between a device and a feedback parameter.</rdfs:comment>
        <rdfs:isDefinedBy rdf:resource="https://www.theworldavatar.com/kg/ontodevice/"/>
        <rdfs:label>has feedback parameter</rdfs:label>
    </owl:ObjectProperty>
    


    <!-- https://www.theworldavatar.com/kg/ontodevice/hasGeoLocation -->


    <owl:ObjectProperty rdf:about="https://www.theworldavatar.com/kg/ontodevice/hasGeoLocation">
        <rdfs:domain rdf:resource="https://www.theworldavatar.com/kg/ontodevice/Device"/>
        <rdfs:range rdf:resource="http://www.opengis.net/ont/sf#Point"/>
        <rdfs:comment>A relationship that describes a device's location.</rdfs:comment>
        <rdfs:isDefinedBy rdf:resource="https://www.theworldavatar.com/kg/ontodevice/"/>
        <rdfs:label>has geo location</rdfs:label>
    </owl:ObjectProperty>
    


    <!-- https://www.theworldavatar.com/kg/ontodevice/hasHeight -->


    <owl:ObjectProperty rdf:about="https://www.theworldavatar.com/kg/ontodevice/hasHeight">
        <rdfs:subPropertyOf rdf:resource="https://www.theworldavatar.com/kg/ontodevice/hasQuantity"/>
        <rdfs:domain rdf:resource="https://www.theworldavatar.com/kg/ontodevice/Device"/>
        <rdfs:range rdf:resource="http://www.ontology-of-units-of-measure.org/resource/om-2/Height"/>
        <rdfs:comment>A relationship between a device and its height.</rdfs:comment>
        <rdfs:isDefinedBy rdf:resource="https://www.theworldavatar.com/kg/ontodevice/"/>
        <rdfs:label>has height</rdfs:label>
    </owl:ObjectProperty>
    


    <!-- https://www.theworldavatar.com/kg/ontodevice/hasLength -->


    <owl:ObjectProperty rdf:about="https://www.theworldavatar.com/kg/ontodevice/hasLength">
        <rdfs:subPropertyOf rdf:resource="https://www.theworldavatar.com/kg/ontodevice/hasQuantity"/>
        <rdfs:domain rdf:resource="https://www.theworldavatar.com/kg/ontodevice/Device"/>
        <rdfs:range rdf:resource="http://www.ontology-of-units-of-measure.org/resource/om-2/Length"/>
        <rdfs:comment>A relationship between a device and its length.</rdfs:comment>
        <rdfs:isDefinedBy rdf:resource="https://www.theworldavatar.com/kg/ontodevice/"/>
        <rdfs:label>has length</rdfs:label>
    </owl:ObjectProperty>
    


    <!-- https://www.theworldavatar.com/kg/ontodevice/hasMass -->


    <owl:ObjectProperty rdf:about="https://www.theworldavatar.com/kg/ontodevice/hasMass">
        <rdfs:subPropertyOf rdf:resource="https://www.theworldavatar.com/kg/ontodevice/hasQuantity"/>
        <rdfs:domain rdf:resource="https://www.theworldavatar.com/kg/ontodevice/Device"/>
        <rdfs:range rdf:resource="http://www.ontology-of-units-of-measure.org/resource/om-2/Mass"/>
        <rdfs:comment>A relationship between a device and its mass.</rdfs:comment>
        <rdfs:isDefinedBy rdf:resource="https://www.theworldavatar.com/kg/ontodevice/"/>
        <rdfs:label>has mass</rdfs:label>
    </owl:ObjectProperty>
    


    <!-- https://www.theworldavatar.com/kg/ontodevice/hasMaxThreshold -->


    <owl:ObjectProperty rdf:about="https://www.theworldavatar.com/kg/ontodevice/hasMaxThreshold">
        <rdfs:domain rdf:resource="https://w3id.org/bot#Zone"/>
        <rdfs:range rdf:resource="https://www.theworldavatar.com/kg/ontodevice/Threshold"/>
        <rdfs:comment>A relationship that defines a maximum threshold applied to a zone (e.g. temperature of a room).</rdfs:comment>
        <rdfs:isDefinedBy rdf:resource="https://www.theworldavatar.com/kg/ontodevice/"/>
        <rdfs:label>has max threshold</rdfs:label>
    </owl:ObjectProperty>
    


    <!-- https://www.theworldavatar.com/kg/ontodevice/hasMaximum -->


    <owl:ObjectProperty rdf:about="https://www.theworldavatar.com/kg/ontodevice/hasMaximum">
        <rdfs:domain rdf:resource="https://www.theworldavatar.com/kg/ontodevice/OperatingRange"/>
        <rdfs:range rdf:resource="http://www.ontology-of-units-of-measure.org/resource/om-2/Quantity"/>
        <rdfs:comment>A relationship that describes the maximum of a range.</rdfs:comment>
        <rdfs:isDefinedBy rdf:resource="https://www.theworldavatar.com/kg/ontodevice/"/>
        <rdfs:label>has maximum</rdfs:label>
    </owl:ObjectProperty>
    


    <!-- https://www.theworldavatar.com/kg/ontodevice/hasMinThreshold -->


    <owl:ObjectProperty rdf:about="https://www.theworldavatar.com/kg/ontodevice/hasMinThreshold">
        <rdfs:domain rdf:resource="https://w3id.org/bot#Zone"/>
        <rdfs:range rdf:resource="https://www.theworldavatar.com/kg/ontodevice/Threshold"/>
        <rdfs:comment>A relationship that defines a minimum threshold applied to a zone (e.g. temperature of a room).</rdfs:comment>
        <rdfs:isDefinedBy rdf:resource="https://www.theworldavatar.com/kg/ontodevice/"/>
        <rdfs:label>has min threshold</rdfs:label>
    </owl:ObjectProperty>
    


    <!-- https://www.theworldavatar.com/kg/ontodevice/hasMinimum -->


    <owl:ObjectProperty rdf:about="https://www.theworldavatar.com/kg/ontodevice/hasMinimum">
        <rdfs:domain rdf:resource="https://www.theworldavatar.com/kg/ontodevice/OperatingRange"/>
        <rdfs:range rdf:resource="http://www.ontology-of-units-of-measure.org/resource/om-2/Quantity"/>
        <rdfs:comment>A relationship that describes the minimum of a range.</rdfs:comment>
        <rdfs:isDefinedBy rdf:resource="https://www.theworldavatar.com/kg/ontodevice/"/>
        <rdfs:label>has minimum</rdfs:label>
    </owl:ObjectProperty>
    


    <!-- https://www.theworldavatar.com/kg/ontodevice/hasMode -->


    <owl:ObjectProperty rdf:about="https://www.theworldavatar.com/kg/ontodevice/hasMode">
        <rdfs:domain rdf:resource="https://www.theworldavatar.com/kg/ontodevice/Device"/>
        <rdfs:range rdf:resource="https://www.theworldavatar.com/kg/ontodevice/Mode"/>
        <rdfs:comment>A relationship that describes the mode that a device is operating in.</rdfs:comment>
        <rdfs:isDefinedBy rdf:resource="https://www.theworldavatar.com/kg/ontodevice/"/>
        <rdfs:label>has mode</rdfs:label>
    </owl:ObjectProperty>
    


    <!-- https://www.theworldavatar.com/kg/ontodevice/hasOperatingParameter -->


    <owl:ObjectProperty rdf:about="https://www.theworldavatar.com/kg/ontodevice/hasOperatingParameter">
        <rdfs:domain rdf:resource="https://www.theworldavatar.com/kg/ontodevice/Device"/>
        <rdfs:range rdf:resource="https://www.theworldavatar.com/kg/ontodevice/OperatingParameter"/>
        <rdfs:comment>A relationship between a device and its operating parameter.</rdfs:comment>
        <rdfs:isDefinedBy rdf:resource="https://www.theworldavatar.com/kg/ontodevice/"/>
        <rdfs:label>has operating parameter</rdfs:label>
    </owl:ObjectProperty>
    


    <!-- https://www.theworldavatar.com/kg/ontodevice/hasOperatingRange -->


    <owl:ObjectProperty rdf:about="https://www.theworldavatar.com/kg/ontodevice/hasOperatingRange">
        <rdfs:domain rdf:resource="https://saref.etsi.org/core/State"/>
        <rdfs:range rdf:resource="https://www.theworldavatar.com/kg/ontodevice/OperatingRange"/>
        <rdfs:comment>A relationship that relates a state to its operating range (e.g. a state of 0 to 100% corresponds to a range of 0 to 1000 rpm).</rdfs:comment>
        <rdfs:isDefinedBy rdf:resource="https://www.theworldavatar.com/kg/ontodevice/"/>
        <rdfs:label>has operating range</rdfs:label>
    </owl:ObjectProperty>
    


    <!-- https://www.theworldavatar.com/kg/ontodevice/hasPressure -->


    <owl:ObjectProperty rdf:about="https://www.theworldavatar.com/kg/ontodevice/hasPressure">
        <rdfs:subPropertyOf rdf:resource="https://www.theworldavatar.com/kg/ontodevice/hasQuantity"/>
        <rdfs:domain>
            <owl:Class>
                <owl:unionOf rdf:parseType="Collection">
                    <rdf:Description rdf:about="http://www.theworldavatar.com/ontology/ontocape/material/phase_system/phase_system.owl#SinglePhase"/>
                    <rdf:Description rdf:about="https://w3id.org/bot#Zone"/>
                </owl:unionOf>
            </owl:Class>
        </rdfs:domain>
        <rdfs:range rdf:resource="http://www.ontology-of-units-of-measure.org/resource/om-2/Pressure"/>
        <rdfs:comment>A relationship describing the pressure exerted on a substance, object or a space.</rdfs:comment>
        <rdfs:isDefinedBy rdf:resource="https://www.theworldavatar.com/kg/ontodevice/"/>
        <rdfs:label>has pressure</rdfs:label>
    </owl:ObjectProperty>
    


    <!-- https://www.theworldavatar.com/kg/ontodevice/hasPrice -->


    <owl:ObjectProperty rdf:about="https://www.theworldavatar.com/kg/ontodevice/hasPrice">
        <rdfs:subPropertyOf rdf:resource="https://www.theworldavatar.com/kg/ontodevice/hasQuantity"/>
        <rdfs:domain rdf:resource="https://www.theworldavatar.com/kg/ontodevice/Device"/>
        <rdfs:range rdf:resource="http://www.ontology-of-units-of-measure.org/resource/om-2/AmountOfMoney"/>
        <rdfs:comment>A relationship between a device and its price.</rdfs:comment>
        <rdfs:isDefinedBy rdf:resource="https://www.theworldavatar.com/kg/ontodevice/"/>
        <rdfs:label>has price</rdfs:label>
    </owl:ObjectProperty>
    


    <!-- https://www.theworldavatar.com/kg/ontodevice/hasProperty -->


    <owl:ObjectProperty rdf:about="https://www.theworldavatar.com/kg/ontodevice/hasProperty">
        <rdfs:domain rdf:resource="https://www.theworldavatar.com/kg/ontodevice/OperatingParameter"/>
        <rdfs:range rdf:resource="https://www.theworldavatar.com/kg/ontodevice/OperatingProperty"/>
        <rdfs:comment>A relationship between a operating parameter and it's property.</rdfs:comment>
        <rdfs:isDefinedBy rdf:resource="https://www.theworldavatar.com/kg/ontodevice/"/>
        <rdfs:label>has property</rdfs:label>
    </owl:ObjectProperty>
    


    <!-- https://www.theworldavatar.com/kg/ontodevice/hasQuantity -->


    <owl:ObjectProperty rdf:about="https://www.theworldavatar.com/kg/ontodevice/hasQuantity">
        <rdfs:domain>
            <owl:Class>
                <owl:unionOf rdf:parseType="Collection">
                    <rdf:Description rdf:about="http://www.theworldavatar.com/kg/ontochemplant#Fluid"/>
                    <rdf:Description rdf:about="http://www.theworldavatar.com/ontology/ontocape/chemical_process_system/CPS_behavior/behavior.owl#ConvectiveTransportRate"/>
                    <rdf:Description rdf:about="http://www.theworldavatar.com/ontology/ontocape/chemical_process_system/CPS_behavior/behavior.owl#MaterialAmount"/>
                    <rdf:Description rdf:about="http://www.theworldavatar.com/ontology/ontocape/chemical_process_system/CPS_function/process.owl#UnitOperation"/>
                    <rdf:Description rdf:about="http://www.theworldavatar.com/ontology/ontocape/material/phase_system/phase_system.owl#PhaseSystem"/>
                    <rdf:Description rdf:about="http://www.w3.org/ns/ssn/systems/Condition"/>
                    <rdf:Description rdf:about="https://saref.etsi.org/core/State"/>
                    <rdf:Description rdf:about="https://w3id.org/bot#Zone"/>
                    <rdf:Description rdf:about="https://www.theworldavatar.com/kg/ontodevice/Device"/>
                    <rdf:Description rdf:about="https://www.theworldavatar.com/kg/ontodevice/OperatingParameter"/>
                    <rdf:Description rdf:about="https://www.theworldavatar.com/kg/ontodevice/Setpoint"/>
                    <rdf:Description rdf:about="https://www.theworldavatar.com/kg/ontodevice/Threshold"/>
                </owl:unionOf>
            </owl:Class>
        </rdfs:domain>
        <rdfs:range rdf:resource="http://www.ontology-of-units-of-measure.org/resource/om-2/Quantity"/>
        <rdfs:comment>A relationship between something (it could be a device or space, a setpoint, an operating property etc) and the quantity it represents or has.</rdfs:comment>
        <rdfs:isDefinedBy rdf:resource="https://www.theworldavatar.com/kg/ontodevice/"/>
        <rdfs:label>has quantity</rdfs:label>
    </owl:ObjectProperty>
    


    <!-- https://www.theworldavatar.com/kg/ontodevice/hasRelativeHumidity -->


    <owl:ObjectProperty rdf:about="https://www.theworldavatar.com/kg/ontodevice/hasRelativeHumidity">
        <rdfs:subPropertyOf rdf:resource="https://www.theworldavatar.com/kg/ontodevice/hasQuantity"/>
        <rdfs:domain rdf:resource="https://w3id.org/bot#Zone"/>
        <rdfs:range rdf:resource="http://www.ontology-of-units-of-measure.org/resource/om-2/RelativeHumidity"/>
        <rdfs:comment>A relationship describing the relative humidity of a substance, object or space.</rdfs:comment>
        <rdfs:isDefinedBy rdf:resource="https://www.theworldavatar.com/kg/ontodevice/"/>
        <rdfs:label>has relative humidity</rdfs:label>
    </owl:ObjectProperty>
    


    <!-- https://www.theworldavatar.com/kg/ontodevice/hasSetpoint -->


    <owl:ObjectProperty rdf:about="https://www.theworldavatar.com/kg/ontodevice/hasSetpoint">
        <rdfs:domain rdf:resource="https://www.theworldavatar.com/kg/ontodevice/Device"/>
        <rdfs:range rdf:resource="https://www.theworldavatar.com/kg/ontodevice/Setpoint"/>
        <rdfs:comment>A relationship between a device and a setpoint.</rdfs:comment>
        <rdfs:isDefinedBy rdf:resource="https://www.theworldavatar.com/kg/ontodevice/"/>
        <rdfs:label>has setpoint</rdfs:label>
    </owl:ObjectProperty>
    


    <!-- https://www.theworldavatar.com/kg/ontodevice/hasSurvivalRange -->


    <owl:ObjectProperty rdf:about="https://www.theworldavatar.com/kg/ontodevice/hasSurvivalRange">
        <rdfs:domain rdf:resource="https://www.theworldavatar.com/kg/ontodevice/Device"/>
        <rdfs:range rdf:resource="http://www.w3.org/ns/ssn/systems/SurvivalRange"/>
        <rdfs:comment>A relationship between a device and its survival range.</rdfs:comment>
        <rdfs:isDefinedBy rdf:resource="https://www.theworldavatar.com/kg/ontodevice/"/>
        <rdfs:label>has survival range</rdfs:label>
    </owl:ObjectProperty>
    


    <!-- https://www.theworldavatar.com/kg/ontodevice/hasSystemCapability -->


    <owl:ObjectProperty rdf:about="https://www.theworldavatar.com/kg/ontodevice/hasSystemCapability">
        <rdfs:domain rdf:resource="https://www.theworldavatar.com/kg/ontodevice/Device"/>
        <rdfs:range rdf:resource="http://www.w3.org/ns/ssn/systems/SystemCapability"/>
        <rdfs:comment>A relationship between a device and its system capability.</rdfs:comment>
        <rdfs:isDefinedBy rdf:resource="https://www.theworldavatar.com/kg/ontodevice/"/>
        <rdfs:label>has system capability</rdfs:label>
    </owl:ObjectProperty>
    


    <!-- https://www.theworldavatar.com/kg/ontodevice/hasTemperature -->


    <owl:ObjectProperty rdf:about="https://www.theworldavatar.com/kg/ontodevice/hasTemperature">
        <rdfs:subPropertyOf rdf:resource="https://www.theworldavatar.com/kg/ontodevice/hasQuantity"/>
        <rdfs:domain>
            <owl:Class>
                <owl:unionOf rdf:parseType="Collection">
                    <rdf:Description rdf:about="http://www.theworldavatar.com/kg/ontochemplant#Fluid"/>
                    <rdf:Description rdf:about="http://www.theworldavatar.com/ontology/ontocape/material/phase_system/phase_system.owl#SinglePhase"/>
                    <rdf:Description rdf:about="https://w3id.org/bot#Zone"/>
                </owl:unionOf>
            </owl:Class>
        </rdfs:domain>
        <rdfs:range rdf:resource="http://www.ontology-of-units-of-measure.org/resource/om-2/Temperature"/>
        <rdfs:comment>A relationship describing the degree or intensity of heat present in a substance, object or space.</rdfs:comment>
        <rdfs:isDefinedBy rdf:resource="https://www.theworldavatar.com/kg/ontodevice/"/>
        <rdfs:label>has temperature</rdfs:label>
    </owl:ObjectProperty>
    


    <!-- https://www.theworldavatar.com/kg/ontodevice/hasWidth -->


    <owl:ObjectProperty rdf:about="https://www.theworldavatar.com/kg/ontodevice/hasWidth">
        <rdfs:subPropertyOf rdf:resource="https://www.theworldavatar.com/kg/ontodevice/hasQuantity"/>
        <rdfs:domain rdf:resource="https://www.theworldavatar.com/kg/ontodevice/Device"/>
        <rdfs:range rdf:resource="http://www.ontology-of-units-of-measure.org/resource/om-2/Width"/>
        <rdfs:comment>A relationship between a device and its width.</rdfs:comment>
        <rdfs:isDefinedBy rdf:resource="https://www.theworldavatar.com/kg/ontodevice/"/>
        <rdfs:label>has width</rdfs:label>
    </owl:ObjectProperty>
    


    <!-- https://www.theworldavatar.com/kg/ontodevice/hasXComponent -->


    <owl:ObjectProperty rdf:about="https://www.theworldavatar.com/kg/ontodevice/hasXComponent">
        <rdfs:domain rdf:resource="https://www.theworldavatar.com/kg/ontodevice/Vector"/>
        <rdfs:range rdf:resource="http://www.ontology-of-units-of-measure.org/resource/om-2/Quantity"/>
        <rdfs:comment>A relationship that defines the component of a vector in x-direction.</rdfs:comment>
        <rdfs:isDefinedBy rdf:resource="https://www.theworldavatar.com/kg/ontodevice/"/>
        <rdfs:label>has X component</rdfs:label>
    </owl:ObjectProperty>
    


    <!-- https://www.theworldavatar.com/kg/ontodevice/hasYComponent -->


    <owl:ObjectProperty rdf:about="https://www.theworldavatar.com/kg/ontodevice/hasYComponent">
        <rdfs:domain rdf:resource="https://www.theworldavatar.com/kg/ontodevice/Vector"/>
        <rdfs:range rdf:resource="http://www.ontology-of-units-of-measure.org/resource/om-2/Quantity"/>
        <rdfs:comment>A relationship that defines the component of a vector in y-direction.</rdfs:comment>
        <rdfs:isDefinedBy rdf:resource="https://www.theworldavatar.com/kg/ontodevice/"/>
        <rdfs:label>has Y component</rdfs:label>
    </owl:ObjectProperty>
    


    <!-- https://www.theworldavatar.com/kg/ontodevice/hasZComponent -->


    <owl:ObjectProperty rdf:about="https://www.theworldavatar.com/kg/ontodevice/hasZComponent">
        <rdfs:domain rdf:resource="https://www.theworldavatar.com/kg/ontodevice/Vector"/>
        <rdfs:range rdf:resource="http://www.ontology-of-units-of-measure.org/resource/om-2/Quantity"/>
        <rdfs:comment>A relationship that defines the component of a vector in z-direction.</rdfs:comment>
        <rdfs:isDefinedBy rdf:resource="https://www.theworldavatar.com/kg/ontodevice/"/>
        <rdfs:label>has Z component</rdfs:label>
    </owl:ObjectProperty>
    


    <!-- https://www.theworldavatar.com/kg/ontodevice/isAttachedTo -->


    <owl:ObjectProperty rdf:about="https://www.theworldavatar.com/kg/ontodevice/isAttachedTo">
        <rdfs:domain rdf:resource="https://www.theworldavatar.com/kg/ontodevice/Device"/>
        <rdfs:range>
            <owl:Class>
                <owl:unionOf rdf:parseType="Collection">
                    <rdf:Description rdf:about="http://www.theworldavatar.com/kg/ontocape/chemicalprocesssystem/cpsrealization/plant/PlantItem"/>
                    <rdf:Description rdf:about="https://w3id.org/bot#Element"/>
                </owl:unionOf>
            </owl:Class>
        </rdfs:range>
        <rdfs:comment>A relationship that describes a device being attached to another physical element or object.</rdfs:comment>
        <rdfs:isDefinedBy rdf:resource="https://www.theworldavatar.com/kg/ontodevice/"/>
        <rdfs:label>is attached to</rdfs:label>
    </owl:ObjectProperty>
    


    <!-- https://www.theworldavatar.com/kg/ontodevice/isConnectedTo -->


    <owl:ObjectProperty rdf:about="https://www.theworldavatar.com/kg/ontodevice/isConnectedTo">
        <rdfs:domain>
            <owl:Class>
                <owl:unionOf rdf:parseType="Collection">
                    <rdf:Description rdf:about="http://www.theworldavatar.com/kg/ontocape/chemicalprocesssystem/cpsrealization/plant/PlantItem"/>
                    <rdf:Description rdf:about="https://www.theworldavatar.com/kg/ontodevice/Device"/>
                </owl:unionOf>
            </owl:Class>
        </rdfs:domain>
        <rdfs:range>
            <owl:Class>
                <owl:unionOf rdf:parseType="Collection">
                    <rdf:Description rdf:about="http://www.theworldavatar.com/kg/ontocape/chemicalprocesssystem/cpsrealization/plant/PlantItem"/>
                    <rdf:Description rdf:about="https://www.theworldavatar.com/kg/ontodevice/Device"/>
                </owl:unionOf>
            </owl:Class>
        </rdfs:range>
        <rdfs:comment>A relationship that describes a device being connected to another device where the operation of one device will affect the other.</rdfs:comment>
        <rdfs:isDefinedBy rdf:resource="https://www.theworldavatar.com/kg/ontodevice/"/>
        <rdfs:label>is connected to</rdfs:label>
    </owl:ObjectProperty>
    


    <!-- https://www.theworldavatar.com/kg/ontodevice/measures -->


    <owl:ObjectProperty rdf:about="https://www.theworldavatar.com/kg/ontodevice/measures">
        <rdfs:domain rdf:resource="https://www.theworldavatar.com/kg/ontodevice/Device"/>
        <rdfs:range>
            <owl:Class>
                <owl:unionOf rdf:parseType="Collection">
                    <rdf:Description rdf:about="http://www.ontology-of-units-of-measure.org/resource/om-2/Quantity"/>
                    <rdf:Description rdf:about="https://www.theworldavatar.com/kg/ontodevice/Vector"/>
                </owl:unionOf>
            </owl:Class>
        </rdfs:range>
        <rdfs:comment>A relationship between a device and a quantity or vector that it is measuring.</rdfs:comment>
        <rdfs:isDefinedBy rdf:resource="https://www.theworldavatar.com/kg/ontodevice/"/>
        <rdfs:label>measures</rdfs:label>
    </owl:ObjectProperty>
    


    <!-- https://www.theworldavatar.com/kg/ontodevice/observes -->


    <owl:ObjectProperty rdf:about="https://www.theworldavatar.com/kg/ontodevice/observes">
        <rdfs:domain rdf:resource="https://www.theworldavatar.com/kg/ontodevice/Device"/>
        <rdfs:range rdf:resource="https://saref.etsi.org/core/State"/>
        <rdfs:comment>A relationship between a device and the state that it is observing.</rdfs:comment>
        <rdfs:isDefinedBy rdf:resource="https://www.theworldavatar.com/kg/ontodevice/"/>
        <rdfs:label>observes</rdfs:label>
    </owl:ObjectProperty>
    


    <!-- https://www.theworldavatar.com/kg/ontodevice/sendsSignalTo -->


    <owl:ObjectProperty rdf:about="https://www.theworldavatar.com/kg/ontodevice/sendsSignalTo">
        <rdfs:domain rdf:resource="https://www.theworldavatar.com/kg/ontodevice/Device"/>
        <rdfs:range rdf:resource="https://www.theworldavatar.com/kg/ontodevice/Device"/>
        <rdfs:comment>A relationship that describes a device sending a signal to another device.</rdfs:comment>
        <rdfs:isDefinedBy rdf:resource="https://www.theworldavatar.com/kg/ontodevice/"/>
        <rdfs:label>sends signal to</rdfs:label>
    </owl:ObjectProperty>
    


    <!-- https://www.theworldavatar.com/kg/ontodevice/sensesSubstance -->


    <owl:ObjectProperty rdf:about="https://www.theworldavatar.com/kg/ontodevice/sensesSubstance">
        <rdfs:domain>
            <owl:Class>
                <owl:unionOf rdf:parseType="Collection">
                    <rdf:Description rdf:about="https://saref.etsi.org/core/TemperatureSensor"/>
                    <rdf:Description rdf:about="https://www.theworldavatar.com/kg/ontodevice/FlowSensor"/>
                    <rdf:Description rdf:about="https://www.theworldavatar.com/kg/ontodevice/PressureSensor"/>
                </owl:unionOf>
            </owl:Class>
        </rdfs:domain>
        <rdfs:range rdf:resource="http://www.theworldavatar.com/ontology/ontocape/material/substance/substance.owl#Substance"/>
        <rdfs:comment>A relationship that describes the type of substance that a device is sensing or observing.</rdfs:comment>
        <rdfs:isDefinedBy rdf:resource="https://www.theworldavatar.com/kg/ontodevice/"/>
        <rdfs:label>senses substance</rdfs:label>
    </owl:ObjectProperty>
    


    <!-- https://www.theworldavatar.com/kg/ontodevice/services -->


    <owl:ObjectProperty rdf:about="https://www.theworldavatar.com/kg/ontodevice/services">
        <rdfs:domain>
            <owl:Class>
                <owl:unionOf rdf:parseType="Collection">
                    <rdf:Description rdf:about="http://www.theworldavatar.com/ontology/ontocape/upper_level/technical_system.owl#TechnicalSystem"/>
                    <rdf:Description rdf:about="https://www.theworldavatar.com/kg/ontodevice/Device"/>
                </owl:unionOf>
            </owl:Class>
        </rdfs:domain>
        <rdfs:range rdf:resource="https://w3id.org/bot#Zone"/>
        <rdfs:comment>A relationship between a device or technical system and the zone it is servicing or providing a service for.</rdfs:comment>
        <rdfs:isDefinedBy rdf:resource="https://www.theworldavatar.com/kg/ontodevice/"/>
        <rdfs:label>services</rdfs:label>
    </owl:ObjectProperty>
    


    <!-- 
    ///////////////////////////////////////////////////////////////////////////////////////
    //
    // Data properties
    //
    ///////////////////////////////////////////////////////////////////////////////////////
     -->


    


    <!-- https://www.theworldavatar.com/kg/ontodevice/hasID -->


    <owl:DatatypeProperty rdf:about="https://www.theworldavatar.com/kg/ontodevice/hasID">
        <rdfs:domain rdf:resource="https://www.theworldavatar.com/kg/ontodevice/Device"/>
        <rdfs:range rdf:resource="http://www.w3.org/2001/XMLSchema#string"/>
        <rdfs:comment>A relationship that describes the ID assigned to a device.</rdfs:comment>
        <rdfs:isDefinedBy rdf:resource="https://www.theworldavatar.com/kg/ontodevice/"/>
        <rdfs:label>has ID</rdfs:label>
    </owl:DatatypeProperty>
    


    <!-- 
    ///////////////////////////////////////////////////////////////////////////////////////
    //
    // Classes
    //
    ///////////////////////////////////////////////////////////////////////////////////////
     -->


    


    <!-- http://www.ontology-of-units-of-measure.org/resource/om-2/Acceleration -->


    <owl:Class rdf:about="http://www.ontology-of-units-of-measure.org/resource/om-2/Acceleration">
        <rdfs:subClassOf rdf:resource="http://www.ontology-of-units-of-measure.org/resource/om-2/Quantity"/>
        <rdfs:isDefinedBy rdf:resource="http://www.ontology-of-units-of-measure.org/resource/om-2/"/>
    </owl:Class>
    


    <!-- http://www.ontology-of-units-of-measure.org/resource/om-2/Acidity -->


    <owl:Class rdf:about="http://www.ontology-of-units-of-measure.org/resource/om-2/Acidity"/>
    


    <!-- http://www.ontology-of-units-of-measure.org/resource/om-2/AmountOfMoney -->


    <owl:Class rdf:about="http://www.ontology-of-units-of-measure.org/resource/om-2/AmountOfMoney"/>
    


    <!-- http://www.ontology-of-units-of-measure.org/resource/om-2/Energy -->


    <owl:Class rdf:about="http://www.ontology-of-units-of-measure.org/resource/om-2/Energy"/>
    


    <!-- http://www.ontology-of-units-of-measure.org/resource/om-2/Frequency -->


    <owl:Class rdf:about="http://www.ontology-of-units-of-measure.org/resource/om-2/Frequency"/>
    


    <!-- http://www.ontology-of-units-of-measure.org/resource/om-2/Height -->


    <owl:Class rdf:about="http://www.ontology-of-units-of-measure.org/resource/om-2/Height"/>
    


    <!-- http://www.ontology-of-units-of-measure.org/resource/om-2/Length -->


    <owl:Class rdf:about="http://www.ontology-of-units-of-measure.org/resource/om-2/Length"/>
    


    <!-- http://www.ontology-of-units-of-measure.org/resource/om-2/MagneticFluxDensity -->


    <owl:Class rdf:about="http://www.ontology-of-units-of-measure.org/resource/om-2/MagneticFluxDensity">
        <rdfs:subClassOf rdf:resource="http://www.ontology-of-units-of-measure.org/resource/om-2/Quantity"/>
        <rdfs:isDefinedBy rdf:resource="http://www.ontology-of-units-of-measure.org/resource/om-2/"/>
    </owl:Class>
    


    <!-- http://www.ontology-of-units-of-measure.org/resource/om-2/Mass -->


    <owl:Class rdf:about="http://www.ontology-of-units-of-measure.org/resource/om-2/Mass"/>
    


    <!-- http://www.ontology-of-units-of-measure.org/resource/om-2/Percentage -->


    <owl:Class rdf:about="http://www.ontology-of-units-of-measure.org/resource/om-2/Percentage"/>
    


    <!-- http://www.ontology-of-units-of-measure.org/resource/om-2/Pressure -->


    <owl:Class rdf:about="http://www.ontology-of-units-of-measure.org/resource/om-2/Pressure"/>
    


    <!-- http://www.ontology-of-units-of-measure.org/resource/om-2/Quantity -->


    <owl:Class rdf:about="http://www.ontology-of-units-of-measure.org/resource/om-2/Quantity"/>
    


    <!-- http://www.ontology-of-units-of-measure.org/resource/om-2/Ratio -->


    <owl:Class rdf:about="http://www.ontology-of-units-of-measure.org/resource/om-2/Ratio">
        <rdfs:subClassOf rdf:resource="http://www.ontology-of-units-of-measure.org/resource/om-2/Quantity"/>
        <rdfs:isDefinedBy rdf:resource="http://www.ontology-of-units-of-measure.org/resource/om-2/"/>
    </owl:Class>
    


    <!-- http://www.ontology-of-units-of-measure.org/resource/om-2/RelativeHumidity -->


    <owl:Class rdf:about="http://www.ontology-of-units-of-measure.org/resource/om-2/RelativeHumidity"/>
    


    <!-- http://www.ontology-of-units-of-measure.org/resource/om-2/Temperature -->


    <owl:Class rdf:about="http://www.ontology-of-units-of-measure.org/resource/om-2/Temperature"/>
    


    <!-- http://www.ontology-of-units-of-measure.org/resource/om-2/Width -->


    <owl:Class rdf:about="http://www.ontology-of-units-of-measure.org/resource/om-2/Width"/>
    


    <!-- http://www.opengis.net/ont/sf#Point -->


    <owl:Class rdf:about="http://www.opengis.net/ont/sf#Point"/>
    


    <!-- http://www.theworldavatar.com/kg/ontocape/chemicalprocesssystem/cpsrealization/plant/PlantItem -->


    <owl:Class rdf:about="http://www.theworldavatar.com/kg/ontocape/chemicalprocesssystem/cpsrealization/plant/PlantItem"/>
    


    <!-- http://www.theworldavatar.com/kg/ontochemplant#Fluid -->


    <owl:Class rdf:about="http://www.theworldavatar.com/kg/ontochemplant#Fluid"/>
    


    <!-- http://www.theworldavatar.com/ontology/ontocape/chemical_process_system/CPS_behavior/behavior.owl#ConvectiveTransportRate -->


    <owl:Class rdf:about="http://www.theworldavatar.com/ontology/ontocape/chemical_process_system/CPS_behavior/behavior.owl#ConvectiveTransportRate"/>
    


    <!-- http://www.theworldavatar.com/ontology/ontocape/chemical_process_system/CPS_behavior/behavior.owl#MaterialAmount -->


    <owl:Class rdf:about="http://www.theworldavatar.com/ontology/ontocape/chemical_process_system/CPS_behavior/behavior.owl#MaterialAmount"/>
    


    <!-- http://www.theworldavatar.com/ontology/ontocape/chemical_process_system/CPS_function/process.owl#TemperatureChange -->


    <owl:Class rdf:about="http://www.theworldavatar.com/ontology/ontocape/chemical_process_system/CPS_function/process.owl#TemperatureChange"/>
    


    <!-- http://www.theworldavatar.com/ontology/ontocape/chemical_process_system/CPS_function/process.owl#UnitOperation -->


    <owl:Class rdf:about="http://www.theworldavatar.com/ontology/ontocape/chemical_process_system/CPS_function/process.owl#UnitOperation"/>
    


    <!-- http://www.theworldavatar.com/ontology/ontocape/material/phase_system/phase_system.owl#PhaseSystem -->


    <owl:Class rdf:about="http://www.theworldavatar.com/ontology/ontocape/material/phase_system/phase_system.owl#PhaseSystem"/>
    


    <!-- http://www.theworldavatar.com/ontology/ontocape/material/phase_system/phase_system.owl#SinglePhase -->


    <owl:Class rdf:about="http://www.theworldavatar.com/ontology/ontocape/material/phase_system/phase_system.owl#SinglePhase"/>
    


    <!-- http://www.theworldavatar.com/ontology/ontocape/material/substance/substance.owl#Substance -->


    <owl:Class rdf:about="http://www.theworldavatar.com/ontology/ontocape/material/substance/substance.owl#Substance"/>
    


    <!-- http://www.theworldavatar.com/ontology/ontocape/upper_level/technical_system.owl#TechnicalSystem -->


    <owl:Class rdf:about="http://www.theworldavatar.com/ontology/ontocape/upper_level/technical_system.owl#TechnicalSystem"/>
    


    <!-- http://www.w3.org/ns/ssn/systems/Condition -->


    <owl:Class rdf:about="http://www.w3.org/ns/ssn/systems/Condition"/>
    


    <!-- http://www.w3.org/ns/ssn/systems/SurvivalRange -->


    <owl:Class rdf:about="http://www.w3.org/ns/ssn/systems/SurvivalRange"/>
    


    <!-- http://www.w3.org/ns/ssn/systems/SystemCapability -->


    <owl:Class rdf:about="http://www.w3.org/ns/ssn/systems/SystemCapability"/>
    


    <!-- https://saref.etsi.org/core/Appliance -->


    <owl:Class rdf:about="https://saref.etsi.org/core/Appliance"/>
    


    <!-- https://saref.etsi.org/core/Device -->


    <owl:Class rdf:about="https://saref.etsi.org/core/Device">
        <owl:equivalentClass rdf:resource="https://www.theworldavatar.com/kg/ontodevice/Device"/>
    </owl:Class>
    


    <!-- https://saref.etsi.org/core/Meter -->


    <owl:Class rdf:about="https://saref.etsi.org/core/Meter">
        <rdfs:subClassOf rdf:resource="https://www.theworldavatar.com/kg/ontodevice/Device"/>
        <rdfs:isDefinedBy rdf:resource="https://www.theworldavatar.com/kg/ontodevice/"/>
    </owl:Class>
    


    <!-- https://saref.etsi.org/core/MultiLevelState -->


    <owl:Class rdf:about="https://saref.etsi.org/core/MultiLevelState"/>
    


    <!-- https://saref.etsi.org/core/Sensor -->


    <owl:Class rdf:about="https://saref.etsi.org/core/Sensor">
        <rdfs:subClassOf rdf:resource="https://www.theworldavatar.com/kg/ontodevice/Device"/>
        <rdfs:isDefinedBy rdf:resource="https://www.theworldavatar.com/kg/ontodevice/"/>
    </owl:Class>
    


    <!-- https://saref.etsi.org/core/State -->


    <owl:Class rdf:about="https://saref.etsi.org/core/State"/>
    


    <!-- https://saref.etsi.org/core/TemperatureSensor -->


    <owl:Class rdf:about="https://saref.etsi.org/core/TemperatureSensor"/>
    


    <!-- https://spec.edmcouncil.org/fibo/ontology/FND/Parties/Parties/IndependentParty -->


    <owl:Class rdf:about="https://spec.edmcouncil.org/fibo/ontology/FND/Parties/Parties/IndependentParty"/>
    


    <!-- https://w3id.org/bot#Element -->


    <owl:Class rdf:about="https://w3id.org/bot#Element"/>
    


    <!-- https://w3id.org/bot#Zone -->


    <owl:Class rdf:about="https://w3id.org/bot#Zone"/>
    


    <!-- https://www.theworldavatar.com/kg/ontodevice/AccelerationVector -->


    <owl:Class rdf:about="https://www.theworldavatar.com/kg/ontodevice/AccelerationVector">
        <rdfs:subClassOf rdf:resource="https://www.theworldavatar.com/kg/ontodevice/Vector"/>
        <rdfs:subClassOf>
            <owl:Restriction>
                <owl:onProperty rdf:resource="https://www.theworldavatar.com/kg/ontodevice/hasXComponent"/>
                <owl:allValuesFrom rdf:resource="http://www.ontology-of-units-of-measure.org/resource/om-2/Acceleration"/>
            </owl:Restriction>
        </rdfs:subClassOf>
        <rdfs:subClassOf>
            <owl:Restriction>
                <owl:onProperty rdf:resource="https://www.theworldavatar.com/kg/ontodevice/hasYComponent"/>
                <owl:allValuesFrom rdf:resource="http://www.ontology-of-units-of-measure.org/resource/om-2/Acceleration"/>
            </owl:Restriction>
        </rdfs:subClassOf>
        <rdfs:subClassOf>
            <owl:Restriction>
                <owl:onProperty rdf:resource="https://www.theworldavatar.com/kg/ontodevice/hasZComponent"/>
                <owl:allValuesFrom rdf:resource="http://www.ontology-of-units-of-measure.org/resource/om-2/Acceleration"/>
            </owl:Restriction>
        </rdfs:subClassOf>
        <rdfs:comment>A vector quantity that represents the rate of change of velocity.</rdfs:comment>
        <rdfs:isDefinedBy rdf:resource="https://www.theworldavatar.com/kg/ontodevice/"/>
        <rdfs:label>Acceleration vector</rdfs:label>
    </owl:Class>
    


    <!-- https://www.theworldavatar.com/kg/ontodevice/Accelerometer -->


    <owl:Class rdf:about="https://www.theworldavatar.com/kg/ontodevice/Accelerometer">
        <rdfs:subClassOf rdf:resource="https://saref.etsi.org/core/Meter"/>
        <rdfs:subClassOf>
            <owl:Restriction>
                <owl:onProperty rdf:resource="https://www.theworldavatar.com/kg/ontodevice/measures"/>
                <owl:allValuesFrom rdf:resource="https://www.theworldavatar.com/kg/ontodevice/AccelerationVector"/>
            </owl:Restriction>
        </rdfs:subClassOf>
        <rdfs:comment>A tool that measures proper acceleration.</rdfs:comment>
        <rdfs:isDefinedBy rdf:resource="https://www.theworldavatar.com/kg/ontodevice/"/>
        <rdfs:label>Accelerometer</rdfs:label>
    </owl:Class>
    


    <!-- https://www.theworldavatar.com/kg/ontodevice/ActiveRFIDTag -->


    <owl:Class rdf:about="https://www.theworldavatar.com/kg/ontodevice/ActiveRFIDTag">
        <rdfs:subClassOf rdf:resource="https://www.theworldavatar.com/kg/ontodevice/RFIDTag"/>
        <rdfs:comment>An active RFID tag that requires batteries for operation.</rdfs:comment>
        <rdfs:isDefinedBy rdf:resource="https://www.theworldavatar.com/kg/ontodevice/"/>
        <rdfs:label>Active RFID tag</rdfs:label>
    </owl:Class>
    


    <!-- https://www.theworldavatar.com/kg/ontodevice/AirCompressor -->


    <owl:Class rdf:about="https://www.theworldavatar.com/kg/ontodevice/AirCompressor">
        <rdfs:subClassOf rdf:resource="https://www.theworldavatar.com/kg/ontodevice/Pump"/>
        <rdfs:comment>A type of pump that compresses the volume of air displaced for experiments that require high-pressure or high-speed air.</rdfs:comment>
        <rdfs:isDefinedBy rdf:resource="https://www.theworldavatar.com/kg/ontodevice/"/>
        <rdfs:label>Air compressor</rdfs:label>
    </owl:Class>
    


    <!-- https://www.theworldavatar.com/kg/ontodevice/AlarmState -->


    <owl:Class rdf:about="https://www.theworldavatar.com/kg/ontodevice/AlarmState">
        <rdfs:subClassOf rdf:resource="https://saref.etsi.org/core/MultiLevelState"/>
        <rdfs:comment>An alert status that is triggered due to an abnormal condition or change in condition.</rdfs:comment>
        <rdfs:isDefinedBy rdf:resource="https://www.theworldavatar.com/kg/ontodevice/"/>
        <rdfs:label>Alarm state</rdfs:label>
    </owl:Class>
    


    <!-- https://www.theworldavatar.com/kg/ontodevice/Antenna -->


    <owl:Class rdf:about="https://www.theworldavatar.com/kg/ontodevice/Antenna">
        <rdfs:subClassOf rdf:resource="https://www.theworldavatar.com/kg/ontodevice/CommunicationDevice"/>
        <rdfs:comment>A device that is used to transmit or receive signal via electromagnetic radiation.</rdfs:comment>
        <rdfs:isDefinedBy rdf:resource="https://www.theworldavatar.com/kg/ontodevice/"/>
        <rdfs:label>Antenna</rdfs:label>
    </owl:Class>
    


    <!-- https://www.theworldavatar.com/kg/ontodevice/CO2Sensor -->


    <owl:Class rdf:about="https://www.theworldavatar.com/kg/ontodevice/CO2Sensor">
        <rdfs:subClassOf rdf:resource="https://saref.etsi.org/core/Sensor"/>
        <rdfs:comment>A sensor that is able to measure the concentration of carbon dioxide gas in the atmosphere.</rdfs:comment>
        <rdfs:isDefinedBy rdf:resource="https://www.theworldavatar.com/kg/ontodevice/"/>
        <rdfs:label>CO2 sensor</rdfs:label>
    </owl:Class>
    


    <!-- https://www.theworldavatar.com/kg/ontodevice/CPU -->


    <owl:Class rdf:about="https://www.theworldavatar.com/kg/ontodevice/CPU">
        <rdfs:subClassOf rdf:resource="https://www.theworldavatar.com/kg/ontodevice/ComputerComponent"/>
        <rdfs:comment>A device that is responsible for the logical or arithmatic operation in a computer.</rdfs:comment>
        <rdfs:isDefinedBy rdf:resource="https://www.theworldavatar.com/kg/ontodevice/"/>
        <rdfs:label>CPU</rdfs:label>
    </owl:Class>
    


    <!-- https://www.theworldavatar.com/kg/ontodevice/Camera -->


    <owl:Class rdf:about="https://www.theworldavatar.com/kg/ontodevice/Camera">
        <rdfs:subClassOf rdf:resource="https://saref.etsi.org/core/Device"/>
        <rdfs:comment>An optical instrument that can capture an image.</rdfs:comment>
        <rdfs:isDefinedBy rdf:resource="https://www.theworldavatar.com/kg/ontodevice/"/>
        <rdfs:label>Camera</rdfs:label>
    </owl:Class>
    


    <!-- https://www.theworldavatar.com/kg/ontodevice/CheckValve -->


    <owl:Class rdf:about="https://www.theworldavatar.com/kg/ontodevice/CheckValve">
        <rdfs:subClassOf rdf:resource="https://www.theworldavatar.com/kg/ontodevice/Valve"/>
        <rdfs:comment>A mechanical device designed to allow fluid (liquid or gas) to flow through it in one direction only.</rdfs:comment>
        <rdfs:isDefinedBy rdf:resource="https://www.theworldavatar.com/kg/ontodevice/"/>
        <rdfs:label>Check valve</rdfs:label>
    </owl:Class>
    


    <!-- https://www.theworldavatar.com/kg/ontodevice/CommunicationDevice -->


    <owl:Class rdf:about="https://www.theworldavatar.com/kg/ontodevice/CommunicationDevice">
        <rdfs:subClassOf rdf:resource="https://saref.etsi.org/core/Device"/>
        <rdfs:comment>A device capable of transmitting an analog or digital signal over the telephone, other communication wire, or wirelessly.</rdfs:comment>
        <rdfs:isDefinedBy rdf:resource="https://www.theworldavatar.com/kg/ontodevice/"/>
        <rdfs:label>Communication device</rdfs:label>
    </owl:Class>
    


    <!-- https://www.theworldavatar.com/kg/ontodevice/Computer -->


    <owl:Class rdf:about="https://www.theworldavatar.com/kg/ontodevice/Computer">
        <rdfs:subClassOf rdf:resource="https://saref.etsi.org/core/Device"/>
        <rdfs:comment>A device that can be programmed to carry out a sequence of arithmetic or logical operations automatically.</rdfs:comment>
        <rdfs:isDefinedBy rdf:resource="https://www.theworldavatar.com/kg/ontodevice/"/>
        <rdfs:label>Computer</rdfs:label>
    </owl:Class>
    


    <!-- https://www.theworldavatar.com/kg/ontodevice/ComputerComponent -->


    <owl:Class rdf:about="https://www.theworldavatar.com/kg/ontodevice/ComputerComponent">
        <rdfs:subClassOf rdf:resource="https://saref.etsi.org/core/Device"/>
        <rdfs:comment>A physical part or element that makes up a computer system and contributes to its overall functionality.</rdfs:comment>
        <rdfs:isDefinedBy rdf:resource="https://www.theworldavatar.com/kg/ontodevice/"/>
        <rdfs:label>Computer component</rdfs:label>
    </owl:Class>
    


    <!-- https://www.theworldavatar.com/kg/ontodevice/ConductivitySensor -->


    <owl:Class rdf:about="https://www.theworldavatar.com/kg/ontodevice/ConductivitySensor">
        <rdfs:subClassOf rdf:resource="https://saref.etsi.org/core/Sensor"/>
        <rdfs:comment>A device that measures the ability of a material to conduct an electrical current.</rdfs:comment>
        <rdfs:isDefinedBy rdf:resource="https://www.theworldavatar.com/kg/ontodevice/"/>
        <rdfs:label>Conductivity sensor</rdfs:label>
    </owl:Class>
    


    <!-- https://www.theworldavatar.com/kg/ontodevice/ControlSensor -->


    <owl:Class rdf:about="https://www.theworldavatar.com/kg/ontodevice/ControlSensor">
        <rdfs:subClassOf rdf:resource="https://saref.etsi.org/core/Sensor"/>
        <rdfs:comment>A device that is used to measure, monitor, and control processes within various industrial and commercial applications.</rdfs:comment>
        <rdfs:isDefinedBy rdf:resource="https://www.theworldavatar.com/kg/ontodevice/"/>
        <rdfs:label>Control sensor</rdfs:label>
    </owl:Class>
    


    <!-- https://www.theworldavatar.com/kg/ontodevice/Controller -->


    <owl:Class rdf:about="https://www.theworldavatar.com/kg/ontodevice/Controller">
        <rdfs:subClassOf rdf:resource="https://saref.etsi.org/core/Device"/>
        <rdfs:comment>A device that controls a certain variable of its environment.</rdfs:comment>
        <rdfs:isDefinedBy rdf:resource="https://www.theworldavatar.com/kg/ontodevice/"/>
        <rdfs:label>Controller</rdfs:label>
    </owl:Class>
    


    <!-- https://www.theworldavatar.com/kg/ontodevice/DefaultValvePosition -->


    <owl:Class rdf:about="https://www.theworldavatar.com/kg/ontodevice/DefaultValvePosition">
        <rdfs:comment>The default position of a valve (NC, NO etc).</rdfs:comment>
        <rdfs:isDefinedBy rdf:resource="https://www.theworldavatar.com/kg/ontodevice/"/>
        <rdfs:label>Default valve position</rdfs:label>
    </owl:Class>
    


    <!-- https://www.theworldavatar.com/kg/ontodevice/Dehumidifier -->


    <owl:Class rdf:about="https://www.theworldavatar.com/kg/ontodevice/Dehumidifier">
        <rdfs:subClassOf rdf:resource="https://saref.etsi.org/core/Appliance"/>
        <rdfs:comment>A device that reduces the humidity of the surrounding atmosphere.</rdfs:comment>
        <rdfs:isDefinedBy rdf:resource="https://www.theworldavatar.com/kg/ontodevice/"/>
        <rdfs:label>Dehumidifier</rdfs:label>
    </owl:Class>
    


    <!-- https://www.theworldavatar.com/kg/ontodevice/Desktop -->


    <owl:Class rdf:about="https://www.theworldavatar.com/kg/ontodevice/Desktop">
        <rdfs:subClassOf rdf:resource="https://www.theworldavatar.com/kg/ontodevice/Computer"/>
        <rdfs:comment>A stationary computer placed on top of a platform, usually desks.</rdfs:comment>
        <rdfs:isDefinedBy rdf:resource="https://www.theworldavatar.com/kg/ontodevice/"/>
        <rdfs:label>Desktop</rdfs:label>
    </owl:Class>
    


    <!-- https://www.theworldavatar.com/kg/ontodevice/Device -->


    <owl:Class rdf:about="https://www.theworldavatar.com/kg/ontodevice/Device">
        <rdfs:subClassOf rdf:resource="https://w3id.org/bot#Element"/>
        <rdfs:comment>An object designed and manufactured to perform one or more functions.</rdfs:comment>
        <rdfs:isDefinedBy rdf:resource="https://www.theworldavatar.com/kg/ontodevice/"/>
        <rdfs:label>Device</rdfs:label>
    </owl:Class>
    


    <!-- https://www.theworldavatar.com/kg/ontodevice/DiaphragmPump -->


    <owl:Class rdf:about="https://www.theworldavatar.com/kg/ontodevice/DiaphragmPump">
        <rdfs:subClassOf rdf:resource="https://www.theworldavatar.com/kg/ontodevice/Pump"/>
        <rdfs:comment>A pump that uses a diaphragm membrane to displace gas or liquid.</rdfs:comment>
        <rdfs:isDefinedBy rdf:resource="https://www.theworldavatar.com/kg/ontodevice/"/>
        <rdfs:label>Diaphragm pump</rdfs:label>
    </owl:Class>
    


    <!-- https://www.theworldavatar.com/kg/ontodevice/Dock -->


    <owl:Class rdf:about="https://www.theworldavatar.com/kg/ontodevice/Dock">
        <rdfs:subClassOf rdf:resource="https://www.theworldavatar.com/kg/ontodevice/PeripheralDevice"/>
        <rdfs:comment>A device that simplifies a computers cable peripheral interface.</rdfs:comment>
        <rdfs:isDefinedBy rdf:resource="https://www.theworldavatar.com/kg/ontodevice/"/>
        <rdfs:label>Dock</rdfs:label>
    </owl:Class>
    


    <!-- https://www.theworldavatar.com/kg/ontodevice/Dongle -->


    <owl:Class rdf:about="https://www.theworldavatar.com/kg/ontodevice/Dongle">
        <rdfs:subClassOf rdf:resource="https://www.theworldavatar.com/kg/ontodevice/PeripheralDevice"/>
        <rdfs:comment>A small piece of computer hardware that connects to a port on another device to provide it with additional functionality, or enable a pass-through to such a device that adds functionality.</rdfs:comment>
        <rdfs:isDefinedBy rdf:resource="https://www.theworldavatar.com/kg/ontodevice/"/>
        <rdfs:label>Dongle</rdfs:label>
    </owl:Class>
    


    <!-- https://www.theworldavatar.com/kg/ontodevice/Drone -->


    <owl:Class rdf:about="https://www.theworldavatar.com/kg/ontodevice/Drone">
        <rdfs:subClassOf rdf:resource="https://www.theworldavatar.com/kg/ontodevice/UAV"/>
        <rdfs:comment>A small UAV controled from a range usually using  a remote controller.</rdfs:comment>
        <rdfs:isDefinedBy rdf:resource="https://www.theworldavatar.com/kg/ontodevice/"/>
        <rdfs:label>Drone</rdfs:label>
    </owl:Class>
    


    <!-- https://www.theworldavatar.com/kg/ontodevice/ElectricalCurrentSensor -->


    <owl:Class rdf:about="https://www.theworldavatar.com/kg/ontodevice/ElectricalCurrentSensor">
        <rdfs:subClassOf rdf:resource="https://saref.etsi.org/core/Sensor"/>
        <rdfs:comment>A device that measures the electrical current flowing through an electrical circuit.</rdfs:comment>
        <rdfs:isDefinedBy rdf:resource="https://www.theworldavatar.com/kg/ontodevice/"/>
        <rdfs:label>Electrical current sensor</rdfs:label>
    </owl:Class>
    


    <!-- https://www.theworldavatar.com/kg/ontodevice/ElectricityMeter -->


    <owl:Class rdf:about="https://www.theworldavatar.com/kg/ontodevice/ElectricityMeter">
        <rdfs:subClassOf rdf:resource="https://saref.etsi.org/core/Meter"/>
        <rdfs:comment>A device that measures the amount of electric energy consumed by a residence, a business, or an electrically powered device.</rdfs:comment>
        <rdfs:isDefinedBy rdf:resource="https://www.theworldavatar.com/kg/ontodevice/"/>
        <rdfs:label>Electricity meter</rdfs:label>
    </owl:Class>
    


    <!-- https://www.theworldavatar.com/kg/ontodevice/ElectronicTag -->


    <owl:Class rdf:about="https://www.theworldavatar.com/kg/ontodevice/ElectronicTag">
        <rdfs:subClassOf rdf:resource="https://saref.etsi.org/core/Device"/>
        <rdfs:comment>A tag that uses a form of electronic identification technology (Bluetooth, RFID etc).</rdfs:comment>
        <rdfs:isDefinedBy rdf:resource="https://www.theworldavatar.com/kg/ontodevice/"/>
        <rdfs:label>Electronic tag</rdfs:label>
    </owl:Class>
    


    <!-- https://www.theworldavatar.com/kg/ontodevice/EthernetCard -->


    <owl:Class rdf:about="https://www.theworldavatar.com/kg/ontodevice/EthernetCard">
        <rdfs:subClassOf rdf:resource="https://www.theworldavatar.com/kg/ontodevice/ComputerComponent"/>
        <rdfs:subClassOf rdf:resource="https://www.theworldavatar.com/kg/ontodevice/NetworkDevice"/>
        <rdfs:comment>A device that acts as a network interface betweena a computer and the internet via cable.</rdfs:comment>
        <rdfs:isDefinedBy rdf:resource="https://www.theworldavatar.com/kg/ontodevice/"/>
        <rdfs:label>Ethernet card</rdfs:label>
    </owl:Class>
    


    <!-- https://www.theworldavatar.com/kg/ontodevice/FeedbackSensor -->


    <owl:Class rdf:about="https://www.theworldavatar.com/kg/ontodevice/FeedbackSensor">
        <rdfs:subClassOf rdf:resource="https://saref.etsi.org/core/Sensor"/>
        <rdfs:comment>A device that is used to provide the control system with measurements of physical quantities necessary to close control loops.</rdfs:comment>
        <rdfs:isDefinedBy rdf:resource="https://www.theworldavatar.com/kg/ontodevice/"/>
        <rdfs:label>Feedback sensor</rdfs:label>
    </owl:Class>
    


    <!-- https://www.theworldavatar.com/kg/ontodevice/FlowChemistryPump -->


    <owl:Class rdf:about="https://www.theworldavatar.com/kg/ontodevice/FlowChemistryPump">
        <rdfs:subClassOf rdf:resource="https://www.theworldavatar.com/kg/ontodevice/Pump"/>
        <rdfs:comment>A pump to be used within a flow chemistry system for flowing liquid reactants.</rdfs:comment>
        <rdfs:isDefinedBy rdf:resource="https://www.theworldavatar.com/kg/ontodevice/"/>
        <rdfs:label>Flow chemistry pump</rdfs:label>
    </owl:Class>
    


    <!-- https://www.theworldavatar.com/kg/ontodevice/FlowController -->


    <owl:Class rdf:about="https://www.theworldavatar.com/kg/ontodevice/FlowController">
        <rdfs:subClassOf rdf:resource="https://www.theworldavatar.com/kg/ontodevice/Controller"/>
        <rdfs:comment>A device that manages the amount of gas or liquid flowing through.</rdfs:comment>
        <rdfs:isDefinedBy rdf:resource="https://www.theworldavatar.com/kg/ontodevice/"/>
        <rdfs:label>Flow controller</rdfs:label>
    </owl:Class>
    


    <!-- https://www.theworldavatar.com/kg/ontodevice/FlowMeter -->


    <owl:Class rdf:about="https://www.theworldavatar.com/kg/ontodevice/FlowMeter">
        <rdfs:subClassOf rdf:resource="https://saref.etsi.org/core/Meter"/>
        <rdfs:comment>A device that measure and communicate amount of liquid flowing through.</rdfs:comment>
        <rdfs:isDefinedBy rdf:resource="https://www.theworldavatar.com/kg/ontodevice/"/>
        <rdfs:label>Flow meter</rdfs:label>
    </owl:Class>
    


    <!-- https://www.theworldavatar.com/kg/ontodevice/FlowSensor -->


    <owl:Class rdf:about="https://www.theworldavatar.com/kg/ontodevice/FlowSensor">
        <rdfs:subClassOf rdf:resource="https://saref.etsi.org/core/Sensor"/>
        <rdfs:comment>A device that is used to measure the flow rate of fluids.</rdfs:comment>
        <rdfs:isDefinedBy rdf:resource="https://www.theworldavatar.com/kg/ontodevice/"/>
        <rdfs:label>Flow sensor</rdfs:label>
    </owl:Class>
    


    <!-- https://www.theworldavatar.com/kg/ontodevice/FluidTransferDevice -->


    <owl:Class rdf:about="https://www.theworldavatar.com/kg/ontodevice/FluidTransferDevice">
        <rdfs:subClassOf rdf:resource="https://saref.etsi.org/core/Device"/>
        <rdfs:comment>A device designed to move fluids (liquids or gases) from one location to another.</rdfs:comment>
        <rdfs:isDefinedBy rdf:resource="https://www.theworldavatar.com/kg/ontodevice/"/>
        <rdfs:label>Fluid transfer device</rdfs:label>
    </owl:Class>
    


    <!-- https://www.theworldavatar.com/kg/ontodevice/FomblinPump -->


    <owl:Class rdf:about="https://www.theworldavatar.com/kg/ontodevice/FomblinPump">
        <rdfs:subClassOf rdf:resource="https://www.theworldavatar.com/kg/ontodevice/Pump"/>
        <rdfs:comment>A pump designed to handle and circulate Fomblin lubricant fluids.</rdfs:comment>
        <rdfs:isDefinedBy rdf:resource="https://www.theworldavatar.com/kg/ontodevice/"/>
        <rdfs:label>Fomblin pump</rdfs:label>
    </owl:Class>
    


    <!-- https://www.theworldavatar.com/kg/ontodevice/Fridge -->


    <owl:Class rdf:about="https://www.theworldavatar.com/kg/ontodevice/Fridge">
        <rdfs:subClassOf rdf:resource="https://saref.etsi.org/core/Appliance"/>
        <rdfs:comment>A device that is usually used for the preservation of items like food via temperature regulation.</rdfs:comment>
        <rdfs:isDefinedBy rdf:resource="https://www.theworldavatar.com/kg/ontodevice/"/>
        <rdfs:label>Fridge</rdfs:label>
    </owl:Class>
    


    <!-- https://www.theworldavatar.com/kg/ontodevice/FurnaceController -->


    <owl:Class rdf:about="https://www.theworldavatar.com/kg/ontodevice/FurnaceController">
        <rdfs:subClassOf rdf:resource="https://www.theworldavatar.com/kg/ontodevice/Controller"/>
        <rdfs:comment>A device that manages the operations of a furnace.</rdfs:comment>
        <rdfs:isDefinedBy rdf:resource="https://www.theworldavatar.com/kg/ontodevice/"/>
        <rdfs:label>Furnace controller</rdfs:label>
    </owl:Class>
    


    <!-- https://www.theworldavatar.com/kg/ontodevice/GPSDevice -->


    <owl:Class rdf:about="https://www.theworldavatar.com/kg/ontodevice/GPSDevice">
        <rdfs:subClassOf rdf:resource="https://saref.etsi.org/core/Device"/>
        <rdfs:comment>A device used within Earth's planetary atmosphere to determine its precise geographical location.</rdfs:comment>
        <rdfs:isDefinedBy rdf:resource="https://www.theworldavatar.com/kg/ontodevice/"/>
        <rdfs:label>GPS device</rdfs:label>
    </owl:Class>
    


    <!-- https://www.theworldavatar.com/kg/ontodevice/GasSensor -->


    <owl:Class rdf:about="https://www.theworldavatar.com/kg/ontodevice/GasSensor">
        <rdfs:subClassOf rdf:resource="https://saref.etsi.org/core/Sensor"/>
        <rdfs:comment>A device that measures the amount or existence of specific gas in the surrounding atmosphere.</rdfs:comment>
        <rdfs:isDefinedBy rdf:resource="https://www.theworldavatar.com/kg/ontodevice/"/>
        <rdfs:label>Gas sensor</rdfs:label>
    </owl:Class>
    


    <!-- https://www.theworldavatar.com/kg/ontodevice/GearPump -->


    <owl:Class rdf:about="https://www.theworldavatar.com/kg/ontodevice/GearPump">
        <rdfs:subClassOf rdf:resource="https://www.theworldavatar.com/kg/ontodevice/Pump"/>
        <rdfs:comment>A type of positive displacement pump that moves fluid through the pump by using the meshing of gears to create a continuous flow.</rdfs:comment>
        <rdfs:isDefinedBy rdf:resource="https://www.theworldavatar.com/kg/ontodevice/"/>
        <rdfs:label>Gear pump</rdfs:label>
    </owl:Class>
    


    <!-- https://www.theworldavatar.com/kg/ontodevice/GravitySensor -->


    <owl:Class rdf:about="https://www.theworldavatar.com/kg/ontodevice/GravitySensor">
        <rdfs:subClassOf rdf:resource="https://saref.etsi.org/core/Sensor"/>
        <rdfs:subClassOf>
            <owl:Restriction>
                <owl:onProperty rdf:resource="https://www.theworldavatar.com/kg/ontodevice/measures"/>
                <owl:allValuesFrom rdf:resource="https://www.theworldavatar.com/kg/ontodevice/GravityVector"/>
            </owl:Restriction>
        </rdfs:subClassOf>
        <rdfs:comment>A sensor that detect minute localized changes in the force of Earth's gravity caused by variations in rock or other material's density underground.</rdfs:comment>
        <rdfs:isDefinedBy rdf:resource="https://www.theworldavatar.com/kg/ontodevice/"/>
        <rdfs:label>Gravity sensor</rdfs:label>
    </owl:Class>
    


    <!-- https://www.theworldavatar.com/kg/ontodevice/GravityVector -->


    <owl:Class rdf:about="https://www.theworldavatar.com/kg/ontodevice/GravityVector">
        <rdfs:subClassOf rdf:resource="https://www.theworldavatar.com/kg/ontodevice/Vector"/>
        <rdfs:subClassOf>
            <owl:Restriction>
                <owl:onProperty rdf:resource="https://www.theworldavatar.com/kg/ontodevice/hasXComponent"/>
                <owl:allValuesFrom rdf:resource="http://www.ontology-of-units-of-measure.org/resource/om-2/Acceleration"/>
            </owl:Restriction>
        </rdfs:subClassOf>
        <rdfs:subClassOf>
            <owl:Restriction>
                <owl:onProperty rdf:resource="https://www.theworldavatar.com/kg/ontodevice/hasYComponent"/>
                <owl:allValuesFrom rdf:resource="http://www.ontology-of-units-of-measure.org/resource/om-2/Acceleration"/>
            </owl:Restriction>
        </rdfs:subClassOf>
        <rdfs:subClassOf>
            <owl:Restriction>
                <owl:onProperty rdf:resource="https://www.theworldavatar.com/kg/ontodevice/hasZComponent"/>
                <owl:allValuesFrom rdf:resource="http://www.ontology-of-units-of-measure.org/resource/om-2/Acceleration"/>
            </owl:Restriction>
        </rdfs:subClassOf>
        <rdfs:comment>A vector quantity that represents the direction and magnitude of the gravitational acceleration.</rdfs:comment>
        <rdfs:isDefinedBy rdf:resource="https://www.theworldavatar.com/kg/ontodevice/"/>
        <rdfs:label>Gravity vector</rdfs:label>
    </owl:Class>
    


    <!-- https://www.theworldavatar.com/kg/ontodevice/HumiditySensor -->


    <owl:Class rdf:about="https://www.theworldavatar.com/kg/ontodevice/HumiditySensor">
        <rdfs:subClassOf rdf:resource="https://saref.etsi.org/core/Sensor"/>
        <rdfs:comment>A sensor that is able to measure the level of humidity in the atmosphere.</rdfs:comment>
        <rdfs:isDefinedBy rdf:resource="https://www.theworldavatar.com/kg/ontodevice/"/>
        <rdfs:label>Humidity sensor</rdfs:label>
    </owl:Class>
    


    <!-- https://www.theworldavatar.com/kg/ontodevice/IceMaker -->


    <owl:Class rdf:about="https://www.theworldavatar.com/kg/ontodevice/IceMaker">
        <rdfs:subClassOf rdf:resource="https://saref.etsi.org/core/Appliance"/>
        <rdfs:comment>A device that is used to create ice by freezing water.</rdfs:comment>
        <rdfs:isDefinedBy rdf:resource="https://www.theworldavatar.com/kg/ontodevice/"/>
        <rdfs:label>Ice maker</rdfs:label>
    </owl:Class>
    


    <!-- https://www.theworldavatar.com/kg/ontodevice/IlluminanceSensor -->


    <owl:Class rdf:about="https://www.theworldavatar.com/kg/ontodevice/IlluminanceSensor">
        <rdfs:subClassOf rdf:resource="https://saref.etsi.org/core/Sensor"/>
        <rdfs:comment>A sensor that is able to measure the level of illuminance.</rdfs:comment>
        <rdfs:isDefinedBy rdf:resource="https://www.theworldavatar.com/kg/ontodevice/"/>
        <rdfs:label>Illuminance sensor</rdfs:label>
    </owl:Class>
    


    <!-- https://www.theworldavatar.com/kg/ontodevice/IlluminationController -->


    <owl:Class rdf:about="https://www.theworldavatar.com/kg/ontodevice/IlluminationController">
        <rdfs:subClassOf rdf:resource="https://www.theworldavatar.com/kg/ontodevice/Controller"/>
        <rdfs:comment>A device that manages the level of light a device produces.</rdfs:comment>
        <rdfs:isDefinedBy rdf:resource="https://www.theworldavatar.com/kg/ontodevice/"/>
        <rdfs:label>Illuminance controller</rdfs:label>
    </owl:Class>
    


    <!-- https://www.theworldavatar.com/kg/ontodevice/InOutState -->


    <owl:Class rdf:about="https://www.theworldavatar.com/kg/ontodevice/InOutState">
        <rdfs:subClassOf rdf:resource="https://saref.etsi.org/core/State"/>
        <rdfs:comment>The current state of something on whether it is inside or outside of a space or object.</rdfs:comment>
        <rdfs:isDefinedBy rdf:resource="https://www.theworldavatar.com/kg/ontodevice/"/>
        <rdfs:label>In out state</rdfs:label>
    </owl:Class>
    


    <!-- https://www.theworldavatar.com/kg/ontodevice/Laptop -->


    <owl:Class rdf:about="https://www.theworldavatar.com/kg/ontodevice/Laptop">
        <rdfs:subClassOf rdf:resource="https://www.theworldavatar.com/kg/ontodevice/Computer"/>
        <rdfs:comment>A small and mobile computer.</rdfs:comment>
        <rdfs:isDefinedBy rdf:resource="https://www.theworldavatar.com/kg/ontodevice/"/>
        <rdfs:label>Laptop</rdfs:label>
    </owl:Class>
    


    <!-- https://www.theworldavatar.com/kg/ontodevice/LevelSensor -->


    <owl:Class rdf:about="https://www.theworldavatar.com/kg/ontodevice/LevelSensor">
        <rdfs:subClassOf rdf:resource="https://saref.etsi.org/core/Sensor"/>
        <rdfs:comment>A device designed to detect and measure the level of a substance, such as liquids, powders, or granular materials, within a container or a confined space. </rdfs:comment>
        <rdfs:isDefinedBy rdf:resource="https://www.theworldavatar.com/kg/ontodevice/"/>
        <rdfs:label>Level sensor</rdfs:label>
    </owl:Class>
    


    <!-- https://www.theworldavatar.com/kg/ontodevice/MagneticFluxDensityVector -->


    <owl:Class rdf:about="https://www.theworldavatar.com/kg/ontodevice/MagneticFluxDensityVector">
        <rdfs:subClassOf rdf:resource="https://www.theworldavatar.com/kg/ontodevice/Vector"/>
        <rdfs:subClassOf>
            <owl:Restriction>
                <owl:onProperty rdf:resource="https://www.theworldavatar.com/kg/ontodevice/hasXComponent"/>
                <owl:allValuesFrom rdf:resource="http://www.ontology-of-units-of-measure.org/resource/om-2/MagneticFluxDensity"/>
            </owl:Restriction>
        </rdfs:subClassOf>
        <rdfs:subClassOf>
            <owl:Restriction>
                <owl:onProperty rdf:resource="https://www.theworldavatar.com/kg/ontodevice/hasYComponent"/>
                <owl:allValuesFrom rdf:resource="http://www.ontology-of-units-of-measure.org/resource/om-2/MagneticFluxDensity"/>
            </owl:Restriction>
        </rdfs:subClassOf>
        <rdfs:subClassOf>
            <owl:Restriction>
                <owl:onProperty rdf:resource="https://www.theworldavatar.com/kg/ontodevice/hasZComponent"/>
                <owl:allValuesFrom rdf:resource="http://www.ontology-of-units-of-measure.org/resource/om-2/MagneticFluxDensity"/>
            </owl:Restriction>
        </rdfs:subClassOf>
        <rdfs:comment>A vector quantity that represents the strength and direction of a magnetic field.</rdfs:comment>
        <rdfs:isDefinedBy rdf:resource="https://www.theworldavatar.com/kg/ontodevice/"/>
        <rdfs:label>Magnetic flux density vector</rdfs:label>
    </owl:Class>
    


    <!-- https://www.theworldavatar.com/kg/ontodevice/Magnetometer -->


    <owl:Class rdf:about="https://www.theworldavatar.com/kg/ontodevice/Magnetometer">
        <rdfs:subClassOf rdf:resource="https://saref.etsi.org/core/Meter"/>
        <rdfs:subClassOf>
            <owl:Restriction>
                <owl:onProperty rdf:resource="https://www.theworldavatar.com/kg/ontodevice/measures"/>
                <owl:allValuesFrom rdf:resource="https://www.theworldavatar.com/kg/ontodevice/MagneticFluxDensityVector"/>
            </owl:Restriction>
        </rdfs:subClassOf>
        <rdfs:comment>A device that measures magnetic field or magnetic dipole moment.</rdfs:comment>
        <rdfs:isDefinedBy rdf:resource="https://www.theworldavatar.com/kg/ontodevice/"/>
        <rdfs:label>Magnetometer</rdfs:label>
    </owl:Class>
    


    <!-- https://www.theworldavatar.com/kg/ontodevice/Manometer -->


    <owl:Class rdf:about="https://www.theworldavatar.com/kg/ontodevice/Manometer">
        <rdfs:subClassOf rdf:resource="https://saref.etsi.org/core/Meter"/>
        <rdfs:comment>A device used to measure the pressure of a fluid.</rdfs:comment>
        <rdfs:isDefinedBy rdf:resource="https://www.theworldavatar.com/kg/ontodevice/"/>
        <rdfs:label>Manometer</rdfs:label>
    </owl:Class>
    


    <!-- https://www.theworldavatar.com/kg/ontodevice/MassFlowController -->


    <owl:Class rdf:about="https://www.theworldavatar.com/kg/ontodevice/MassFlowController">
        <rdfs:subClassOf rdf:resource="https://www.theworldavatar.com/kg/ontodevice/FlowController"/>
        <rdfs:comment>A device that manages the mass of gas or liquid flowing through.</rdfs:comment>
        <rdfs:isDefinedBy rdf:resource="https://www.theworldavatar.com/kg/ontodevice/"/>
        <rdfs:label>Mass flow controller</rdfs:label>
    </owl:Class>
    


    <!-- https://www.theworldavatar.com/kg/ontodevice/MassFlowSensor -->


    <owl:Class rdf:about="https://www.theworldavatar.com/kg/ontodevice/MassFlowSensor">
        <rdfs:subClassOf rdf:resource="https://saref.etsi.org/core/Sensor"/>
        <rdfs:comment>A device that measures the mass flow rate of gas or liquid.</rdfs:comment>
        <rdfs:isDefinedBy rdf:resource="https://www.theworldavatar.com/kg/ontodevice/"/>
        <rdfs:label>Mass flow sensor</rdfs:label>
    </owl:Class>
    


    <!-- https://www.theworldavatar.com/kg/ontodevice/MicroController -->


    <owl:Class rdf:about="https://www.theworldavatar.com/kg/ontodevice/MicroController">
        <rdfs:subClassOf rdf:resource="https://saref.etsi.org/core/Device"/>
        <rdfs:comment>A microcontroller is an integrated circuit (IC) designed to handle a specific task in embedded systems.</rdfs:comment>
        <rdfs:isDefinedBy rdf:resource="https://www.theworldavatar.com/kg/ontodevice/"/>
        <rdfs:label>MicroController</rdfs:label>
    </owl:Class>
    


    <!-- https://www.theworldavatar.com/kg/ontodevice/Microphone -->


    <owl:Class rdf:about="https://www.theworldavatar.com/kg/ontodevice/Microphone">
        <rdfs:subClassOf rdf:resource="https://saref.etsi.org/core/Device"/>
        <rdfs:comment>A transducer that converts sound into an electrical signal.</rdfs:comment>
        <rdfs:isDefinedBy rdf:resource="https://www.theworldavatar.com/kg/ontodevice/"/>
        <rdfs:label>Microphone</rdfs:label>
    </owl:Class>
    


    <!-- https://www.theworldavatar.com/kg/ontodevice/MobilePhone -->


    <owl:Class rdf:about="https://www.theworldavatar.com/kg/ontodevice/MobilePhone">
        <rdfs:subClassOf rdf:resource="https://www.theworldavatar.com/kg/ontodevice/CommunicationDevice"/>
        <rdfs:comment>A portable telephone that can make and receive calls over a radio frequency link.</rdfs:comment>
        <rdfs:isDefinedBy rdf:resource="https://www.theworldavatar.com/kg/ontodevice/"/>
        <rdfs:label>Mobile phone</rdfs:label>
    </owl:Class>
    


    <!-- https://www.theworldavatar.com/kg/ontodevice/Mode -->


    <owl:Class rdf:about="https://www.theworldavatar.com/kg/ontodevice/Mode">
        <rdfs:comment>An option allowing a change in the method of operation of a device.</rdfs:comment>
        <rdfs:isDefinedBy rdf:resource="https://www.theworldavatar.com/kg/ontodevice/"/>
        <rdfs:label>Mode</rdfs:label>
    </owl:Class>
    


    <!-- https://www.theworldavatar.com/kg/ontodevice/Monitor -->


    <owl:Class rdf:about="https://www.theworldavatar.com/kg/ontodevice/Monitor">
        <rdfs:subClassOf rdf:resource="https://www.theworldavatar.com/kg/ontodevice/PeripheralDevice"/>
        <rdfs:comment>A device that acts as a display of a computer.</rdfs:comment>
        <rdfs:isDefinedBy rdf:resource="https://www.theworldavatar.com/kg/ontodevice/"/>
        <rdfs:label>Monitor</rdfs:label>
    </owl:Class>
    


    <!-- https://www.theworldavatar.com/kg/ontodevice/MotorController -->


    <owl:Class rdf:about="https://www.theworldavatar.com/kg/ontodevice/MotorController">
        <rdfs:subClassOf rdf:resource="https://www.theworldavatar.com/kg/ontodevice/Controller"/>
        <rdfs:comment>A device that manages the operation of motors.</rdfs:comment>
        <rdfs:isDefinedBy rdf:resource="https://www.theworldavatar.com/kg/ontodevice/"/>
        <rdfs:label>Motor controller</rdfs:label>
    </owl:Class>
    


    <!-- https://www.theworldavatar.com/kg/ontodevice/NetworkDevice -->


    <owl:Class rdf:about="https://www.theworldavatar.com/kg/ontodevice/NetworkDevice">
        <rdfs:subClassOf rdf:resource="https://www.theworldavatar.com/kg/ontodevice/CommunicationDevice"/>
        <rdfs:comment>A device that allows communication within a computer network.</rdfs:comment>
        <rdfs:isDefinedBy rdf:resource="https://www.theworldavatar.com/kg/ontodevice/"/>
        <rdfs:label>Network device</rdfs:label>
    </owl:Class>
    


    <!-- https://www.theworldavatar.com/kg/ontodevice/NetworkSwitch -->


    <owl:Class rdf:about="https://www.theworldavatar.com/kg/ontodevice/NetworkSwitch">
        <rdfs:subClassOf rdf:resource="https://www.theworldavatar.com/kg/ontodevice/NetworkDevice"/>
        <rdfs:comment>A device that forwards and receive data from a computer network to a single specific device.</rdfs:comment>
        <rdfs:isDefinedBy rdf:resource="https://www.theworldavatar.com/kg/ontodevice/"/>
        <rdfs:label>Network switch</rdfs:label>
    </owl:Class>
    


    <!-- https://www.theworldavatar.com/kg/ontodevice/NetworkVideoRecorder -->


    <owl:Class rdf:about="https://www.theworldavatar.com/kg/ontodevice/NetworkVideoRecorder">
        <rdfs:subClassOf rdf:resource="https://www.theworldavatar.com/kg/ontodevice/RecordingDevice"/>
        <rdfs:comment>A device that converts video recording in a camera network to a computer-storable format.</rdfs:comment>
        <rdfs:isDefinedBy rdf:resource="https://www.theworldavatar.com/kg/ontodevice/"/>
        <rdfs:label>Network video recorder</rdfs:label>
    </owl:Class>
    


    <!-- https://www.theworldavatar.com/kg/ontodevice/OccupiedState -->


    <owl:Class rdf:about="https://www.theworldavatar.com/kg/ontodevice/OccupiedState">
        <rdfs:subClassOf rdf:resource="https://saref.etsi.org/core/State"/>
        <rdfs:comment>The current state of something on whether it is occupied or not.</rdfs:comment>
        <rdfs:isDefinedBy rdf:resource="https://www.theworldavatar.com/kg/ontodevice/"/>
        <rdfs:label>Occupied state</rdfs:label>
    </owl:Class>
    


    <!-- https://www.theworldavatar.com/kg/ontodevice/OilMeter -->


    <owl:Class rdf:about="https://www.theworldavatar.com/kg/ontodevice/OilMeter">
        <rdfs:subClassOf rdf:resource="https://saref.etsi.org/core/Meter"/>
        <rdfs:comment>A device for measuring the flow of oil.</rdfs:comment>
        <rdfs:isDefinedBy rdf:resource="https://www.theworldavatar.com/kg/ontodevice/"/>
        <rdfs:label>Oil meter</rdfs:label>
    </owl:Class>
    


    <!-- https://www.theworldavatar.com/kg/ontodevice/OperatingParameter -->


    <owl:Class rdf:about="https://www.theworldavatar.com/kg/ontodevice/OperatingParameter">
        <rdfs:comment>Operating parameters of a device refer to the specific conditions or variables within which the device is designed to function optimally.</rdfs:comment>
        <rdfs:isDefinedBy rdf:resource="https://www.theworldavatar.com/kg/ontodevice/"/>
        <rdfs:label>Operating parameter</rdfs:label>
    </owl:Class>
    


    <!-- https://www.theworldavatar.com/kg/ontodevice/OperatingProperty -->


    <owl:Class rdf:about="https://www.theworldavatar.com/kg/ontodevice/OperatingProperty">
        <rdfs:comment>A property of an operating parameter of a device (e.g. range of an operating temperature).</rdfs:comment>
        <rdfs:isDefinedBy rdf:resource="https://www.theworldavatar.com/kg/ontodevice/"/>
        <rdfs:label>Operating property</rdfs:label>
    </owl:Class>
    


    <!-- https://www.theworldavatar.com/kg/ontodevice/OperatingRange -->


    <owl:Class rdf:about="https://www.theworldavatar.com/kg/ontodevice/OperatingRange">
        <rdfs:subClassOf rdf:resource="https://www.theworldavatar.com/kg/ontodevice/OperatingProperty"/>
        <rdfs:comment>The range for an operating parameter of a device (e.g. range of an operating temperature).</rdfs:comment>
        <rdfs:isDefinedBy rdf:resource="https://www.theworldavatar.com/kg/ontodevice/"/>
        <rdfs:label>Operating range</rdfs:label>
    </owl:Class>
    


    <!-- https://www.theworldavatar.com/kg/ontodevice/OperatingTemperature -->


    <owl:Class rdf:about="https://www.theworldavatar.com/kg/ontodevice/OperatingTemperature">
        <rdfs:subClassOf rdf:resource="https://www.theworldavatar.com/kg/ontodevice/OperatingParameter"/>
        <rdfs:comment>The operating temperature of a device.</rdfs:comment>
        <rdfs:isDefinedBy rdf:resource="https://www.theworldavatar.com/kg/ontodevice/"/>
        <rdfs:label>Operating temperature</rdfs:label>
    </owl:Class>
    


    <!-- https://www.theworldavatar.com/kg/ontodevice/OperatingTemperatureRange -->


    <owl:Class rdf:about="https://www.theworldavatar.com/kg/ontodevice/OperatingTemperatureRange">
        <rdfs:subClassOf rdf:resource="https://www.theworldavatar.com/kg/ontodevice/OperatingRange"/>
        <rdfs:comment>The operating temperature range of a device.</rdfs:comment>
        <rdfs:isDefinedBy rdf:resource="https://www.theworldavatar.com/kg/ontodevice/"/>
        <rdfs:label>Operating temperature range</rdfs:label>
    </owl:Class>
    


    <!-- https://www.theworldavatar.com/kg/ontodevice/Oven -->


    <owl:Class rdf:about="https://www.theworldavatar.com/kg/ontodevice/Oven">
        <rdfs:subClassOf rdf:resource="https://saref.etsi.org/core/Appliance"/>
        <rdfs:comment>A device that is used for heating up items like food using a heating element.</rdfs:comment>
        <rdfs:isDefinedBy rdf:resource="https://www.theworldavatar.com/kg/ontodevice/"/>
        <rdfs:label>Oven</rdfs:label>
    </owl:Class>
    


    <!-- https://www.theworldavatar.com/kg/ontodevice/PCCooler -->


    <owl:Class rdf:about="https://www.theworldavatar.com/kg/ontodevice/PCCooler">
        <rdfs:subClassOf rdf:resource="https://www.theworldavatar.com/kg/ontodevice/ComputerComponent"/>
        <rdfs:comment>A device that lowers the operating temperature of a computer during operation.</rdfs:comment>
        <rdfs:isDefinedBy rdf:resource="https://www.theworldavatar.com/kg/ontodevice/"/>
        <rdfs:label>PC Cooler</rdfs:label>
    </owl:Class>
    


    <!-- https://www.theworldavatar.com/kg/ontodevice/PaperShredder -->


    <owl:Class rdf:about="https://www.theworldavatar.com/kg/ontodevice/PaperShredder">
        <rdfs:subClassOf rdf:resource="https://saref.etsi.org/core/Appliance"/>
        <rdfs:comment>A device used to destroy paper document via cutting the document to small pieces.</rdfs:comment>
        <rdfs:isDefinedBy rdf:resource="https://www.theworldavatar.com/kg/ontodevice/"/>
        <rdfs:label>Paper shredder</rdfs:label>
    </owl:Class>
    


    <!-- https://www.theworldavatar.com/kg/ontodevice/PassiveRFIDTag -->


    <owl:Class rdf:about="https://www.theworldavatar.com/kg/ontodevice/PassiveRFIDTag">
        <rdfs:subClassOf rdf:resource="https://www.theworldavatar.com/kg/ontodevice/RFIDTag"/>
        <rdfs:comment>A passive RFID tag that functions via the electromagnetic energy that gets transmitted from the RFID reader. </rdfs:comment>
        <rdfs:isDefinedBy rdf:resource="https://www.theworldavatar.com/kg/ontodevice/"/>
        <rdfs:label>Passive RFID tag</rdfs:label>
    </owl:Class>
    


    <!-- https://www.theworldavatar.com/kg/ontodevice/PeripheralDevice -->


    <owl:Class rdf:about="https://www.theworldavatar.com/kg/ontodevice/PeripheralDevice">
        <rdfs:subClassOf rdf:resource="https://saref.etsi.org/core/Device"/>
        <rdfs:comment>A device that connects to a computer and extends its functionality, providing additional input, output, or storage capabilities.</rdfs:comment>
        <rdfs:isDefinedBy rdf:resource="https://www.theworldavatar.com/kg/ontodevice/"/>
        <rdfs:label>Peripheral device</rdfs:label>
    </owl:Class>
    


    <!-- https://www.theworldavatar.com/kg/ontodevice/PeristalticPump -->


    <owl:Class rdf:about="https://www.theworldavatar.com/kg/ontodevice/PeristalticPump">
        <rdfs:subClassOf rdf:resource="https://www.theworldavatar.com/kg/ontodevice/Pump"/>
        <rdfs:comment>A pump that displaces liquid or gas by squeezing it through a flexible tube.</rdfs:comment>
        <rdfs:isDefinedBy rdf:resource="https://www.theworldavatar.com/kg/ontodevice/"/>
        <rdfs:label>Peristaltic pump</rdfs:label>
    </owl:Class>
    


    <!-- https://www.theworldavatar.com/kg/ontodevice/PollutionMeter -->


    <owl:Class rdf:about="https://www.theworldavatar.com/kg/ontodevice/PollutionMeter">
        <rdfs:subClassOf rdf:resource="https://saref.etsi.org/core/Meter"/>
        <rdfs:comment>A device for measuring air quality.</rdfs:comment>
        <rdfs:isDefinedBy rdf:resource="https://www.theworldavatar.com/kg/ontodevice/"/>
        <rdfs:label>Pollution meter</rdfs:label>
    </owl:Class>
    


    <!-- https://www.theworldavatar.com/kg/ontodevice/PowerFactor -->


    <owl:Class rdf:about="https://www.theworldavatar.com/kg/ontodevice/PowerFactor">
        <rdfs:subClassOf rdf:resource="http://www.ontology-of-units-of-measure.org/resource/om-2/Ratio"/>
        <rdfs:comment>The ratio of working power, measured in kilowatts (kW), to apparent power, measured in kilovolt amperes (kVA).</rdfs:comment>
        <rdfs:isDefinedBy rdf:resource="https://www.theworldavatar.com/kg/ontodevice/"/>
        <rdfs:label>Power factor</rdfs:label>
    </owl:Class>
    


    <!-- https://www.theworldavatar.com/kg/ontodevice/PressureContoller -->


    <owl:Class rdf:about="https://www.theworldavatar.com/kg/ontodevice/PressureContoller">
        <rdfs:subClassOf rdf:resource="https://www.theworldavatar.com/kg/ontodevice/Controller"/>
        <rdfs:comment>A device that manages the gas or liquid pressure of other apparatus.</rdfs:comment>
        <rdfs:isDefinedBy rdf:resource="https://www.theworldavatar.com/kg/ontodevice/"/>
        <rdfs:label>Pressure controller</rdfs:label>
    </owl:Class>
    


    <!-- https://www.theworldavatar.com/kg/ontodevice/PressureSensor -->


    <owl:Class rdf:about="https://www.theworldavatar.com/kg/ontodevice/PressureSensor">
        <rdfs:subClassOf rdf:resource="https://saref.etsi.org/core/Sensor"/>
        <rdfs:comment>A device that senses pressure and converts it into an electric signal where the amount depends upon the pressure applied.</rdfs:comment>
        <rdfs:isDefinedBy rdf:resource="https://www.theworldavatar.com/kg/ontodevice/"/>
        <rdfs:label>Pressure sensor</rdfs:label>
    </owl:Class>
    


    <!-- https://www.theworldavatar.com/kg/ontodevice/Printer -->


    <owl:Class rdf:about="https://www.theworldavatar.com/kg/ontodevice/Printer">
        <rdfs:subClassOf rdf:resource="https://www.theworldavatar.com/kg/ontodevice/PeripheralDevice"/>
        <rdfs:comment>A device that prints data or documents to a paper.</rdfs:comment>
        <rdfs:isDefinedBy rdf:resource="https://www.theworldavatar.com/kg/ontodevice/"/>
        <rdfs:label>Printer</rdfs:label>
    </owl:Class>
    


    <!-- https://www.theworldavatar.com/kg/ontodevice/Projector -->


    <owl:Class rdf:about="https://www.theworldavatar.com/kg/ontodevice/Projector">
        <rdfs:subClassOf rdf:resource="https://www.theworldavatar.com/kg/ontodevice/PeripheralDevice"/>
        <rdfs:comment>A device tht projects an image to a screen.</rdfs:comment>
        <rdfs:isDefinedBy rdf:resource="https://www.theworldavatar.com/kg/ontodevice/"/>
        <rdfs:label>Projector</rdfs:label>
    </owl:Class>
    


    <!-- https://www.theworldavatar.com/kg/ontodevice/ProximitySensor -->


    <owl:Class rdf:about="https://www.theworldavatar.com/kg/ontodevice/ProximitySensor">
        <rdfs:subClassOf rdf:resource="https://saref.etsi.org/core/Sensor"/>
        <rdfs:comment>A device that takes a continuous distance reading and returns a corresponding analog voltage.</rdfs:comment>
        <rdfs:isDefinedBy rdf:resource="https://www.theworldavatar.com/kg/ontodevice/"/>
        <rdfs:label>Proximity sensor</rdfs:label>
    </owl:Class>
    


    <!-- https://www.theworldavatar.com/kg/ontodevice/Pump -->


    <owl:Class rdf:about="https://www.theworldavatar.com/kg/ontodevice/Pump">
        <rdfs:subClassOf rdf:resource="https://www.theworldavatar.com/kg/ontodevice/FluidTransferDevice"/>
        <rdfs:comment>A device that moves fluids or gas, by mechanical action.</rdfs:comment>
        <rdfs:isDefinedBy rdf:resource="https://www.theworldavatar.com/kg/ontodevice/"/>
        <rdfs:label>Pump</rdfs:label>
    </owl:Class>
    


    <!-- https://www.theworldavatar.com/kg/ontodevice/RAM -->


    <owl:Class rdf:about="https://www.theworldavatar.com/kg/ontodevice/RAM">
        <rdfs:subClassOf rdf:resource="https://www.theworldavatar.com/kg/ontodevice/ComputerComponent"/>
        <rdfs:comment>A device that provides non-permanent memory during computation to a computer.</rdfs:comment>
        <rdfs:isDefinedBy rdf:resource="https://www.theworldavatar.com/kg/ontodevice/"/>
        <rdfs:label>RAM</rdfs:label>
    </owl:Class>
    


    <!-- https://www.theworldavatar.com/kg/ontodevice/RFIDSensor -->


    <owl:Class rdf:about="https://www.theworldavatar.com/kg/ontodevice/RFIDSensor">
        <rdfs:subClassOf rdf:resource="https://saref.etsi.org/core/Sensor"/>
        <rdfs:comment>A sensor used to gather information from an RFID tag, which is used to track individual objects.</rdfs:comment>
        <rdfs:isDefinedBy rdf:resource="https://www.theworldavatar.com/kg/ontodevice/"/>
        <rdfs:label>RFID sensor</rdfs:label>
    </owl:Class>
    


    <!-- https://www.theworldavatar.com/kg/ontodevice/RFIDTag -->


    <owl:Class rdf:about="https://www.theworldavatar.com/kg/ontodevice/RFIDTag">
        <rdfs:subClassOf rdf:resource="https://www.theworldavatar.com/kg/ontodevice/ElectronicTag"/>
        <rdfs:comment>An electronic tag that exchanges data with a RFID reader through radio waves.</rdfs:comment>
        <rdfs:isDefinedBy rdf:resource="https://www.theworldavatar.com/kg/ontodevice/"/>
        <rdfs:label>RFID tag</rdfs:label>
    </owl:Class>
    


    <!-- https://www.theworldavatar.com/kg/ontodevice/Reader -->


    <owl:Class rdf:about="https://www.theworldavatar.com/kg/ontodevice/Reader">
        <rdfs:subClassOf rdf:resource="https://www.theworldavatar.com/kg/ontodevice/PeripheralDevice"/>
        <rdfs:comment>A device that reads information from an external info storage, such as ID card, NFC tag, etc.</rdfs:comment>
        <rdfs:isDefinedBy rdf:resource="https://www.theworldavatar.com/kg/ontodevice/"/>
        <rdfs:label>Reader</rdfs:label>
    </owl:Class>
    


    <!-- https://www.theworldavatar.com/kg/ontodevice/RecordingDevice -->


    <owl:Class rdf:about="https://www.theworldavatar.com/kg/ontodevice/RecordingDevice">
        <rdfs:subClassOf rdf:resource="https://saref.etsi.org/core/Device"/>
        <rdfs:comment>A device that store the video footage, allowing for playback and analysis.</rdfs:comment>
        <rdfs:isDefinedBy rdf:resource="https://www.theworldavatar.com/kg/ontodevice/"/>
        <rdfs:label>Recording device</rdfs:label>
    </owl:Class>
    


    <!-- https://www.theworldavatar.com/kg/ontodevice/RegulatingValve -->


    <owl:Class rdf:about="https://www.theworldavatar.com/kg/ontodevice/RegulatingValve">
        <rdfs:subClassOf rdf:resource="https://www.theworldavatar.com/kg/ontodevice/Valve"/>
        <rdfs:comment>A type of valve used in fluid control systems to regulate the flow, pressure, or temperature of a fluid within a pipeline.</rdfs:comment>
        <rdfs:isDefinedBy rdf:resource="https://www.theworldavatar.com/kg/ontodevice/"/>
        <rdfs:label>Regulating valve</rdfs:label>
    </owl:Class>
    


    <!-- https://www.theworldavatar.com/kg/ontodevice/RelativeBrightness -->


    <owl:Class rdf:about="https://www.theworldavatar.com/kg/ontodevice/RelativeBrightness">
        <rdfs:subClassOf rdf:resource="http://www.ontology-of-units-of-measure.org/resource/om-2/Ratio"/>
        <rdfs:comment>Brightness measured as a ratio.</rdfs:comment>
        <rdfs:isDefinedBy rdf:resource="https://www.theworldavatar.com/kg/ontodevice/"/>
        <rdfs:label>Relative brightness</rdfs:label>
    </owl:Class>
    


    <!-- https://www.theworldavatar.com/kg/ontodevice/RetentateValve -->


    <owl:Class rdf:about="https://www.theworldavatar.com/kg/ontodevice/RetentateValve">
        <rdfs:subClassOf rdf:resource="https://www.theworldavatar.com/kg/ontodevice/RegulatingValve"/>
        <rdfs:comment>A type of valve that is used to control the flow of retentate.</rdfs:comment>
        <rdfs:isDefinedBy rdf:resource="https://www.theworldavatar.com/kg/ontodevice/"/>
        <rdfs:label>Retentate valve</rdfs:label>
    </owl:Class>
    


    <!-- https://www.theworldavatar.com/kg/ontodevice/RotationalSpeed -->


    <owl:Class rdf:about="https://www.theworldavatar.com/kg/ontodevice/RotationalSpeed">
        <rdfs:subClassOf rdf:resource="https://www.theworldavatar.com/kg/ontodevice/OperatingParameter"/>
        <rdfs:comment>The rotational speed of a device (e.g. a motor).</rdfs:comment>
        <rdfs:isDefinedBy rdf:resource="https://www.theworldavatar.com/kg/ontodevice/"/>
        <rdfs:label>Rotational speed</rdfs:label>
    </owl:Class>
    


    <!-- https://www.theworldavatar.com/kg/ontodevice/Router -->


    <owl:Class rdf:about="https://www.theworldavatar.com/kg/ontodevice/Router">
        <rdfs:subClassOf rdf:resource="https://www.theworldavatar.com/kg/ontodevice/NetworkDevice"/>
        <rdfs:comment>A device that forwards data packets in a computer network.</rdfs:comment>
        <rdfs:isDefinedBy rdf:resource="https://www.theworldavatar.com/kg/ontodevice/"/>
        <rdfs:label>Router</rdfs:label>
    </owl:Class>
    


    <!-- https://www.theworldavatar.com/kg/ontodevice/SSD -->


    <owl:Class rdf:about="https://www.theworldavatar.com/kg/ontodevice/SSD">
        <rdfs:subClassOf rdf:resource="https://www.theworldavatar.com/kg/ontodevice/ComputerComponent"/>
        <rdfs:comment>A device that provies permanent memory on a computer.</rdfs:comment>
        <rdfs:isDefinedBy rdf:resource="https://www.theworldavatar.com/kg/ontodevice/"/>
        <rdfs:label>SSD</rdfs:label>
    </owl:Class>
    


    <!-- https://www.theworldavatar.com/kg/ontodevice/SashOpeningSensor -->


    <owl:Class rdf:about="https://www.theworldavatar.com/kg/ontodevice/SashOpeningSensor">
        <rdfs:subClassOf rdf:resource="https://saref.etsi.org/core/Sensor"/>
        <rdfs:comment>A device that measures the sash opening of an object such as a fumehood.</rdfs:comment>
        <rdfs:isDefinedBy rdf:resource="https://www.theworldavatar.com/kg/ontodevice/"/>
        <rdfs:label>Sash opening sensor</rdfs:label>
    </owl:Class>
    


    <!-- https://www.theworldavatar.com/kg/ontodevice/Scanner -->


    <owl:Class rdf:about="https://www.theworldavatar.com/kg/ontodevice/Scanner">
        <rdfs:subClassOf rdf:resource="https://www.theworldavatar.com/kg/ontodevice/PeripheralDevice"/>
        <rdfs:comment>A device that  scans paper-based documents to a digital format.</rdfs:comment>
        <rdfs:isDefinedBy rdf:resource="https://www.theworldavatar.com/kg/ontodevice/"/>
        <rdfs:label>Scanner</rdfs:label>
    </owl:Class>
    


    <!-- https://www.theworldavatar.com/kg/ontodevice/Screen -->


    <owl:Class rdf:about="https://www.theworldavatar.com/kg/ontodevice/Screen">
        <rdfs:subClassOf rdf:resource="https://www.theworldavatar.com/kg/ontodevice/PeripheralDevice"/>
        <rdfs:comment>A device on which a computer interface is projected onto.</rdfs:comment>
        <rdfs:isDefinedBy rdf:resource="https://www.theworldavatar.com/kg/ontodevice/"/>
        <rdfs:label>Screen</rdfs:label>
    </owl:Class>
    


    <!-- https://www.theworldavatar.com/kg/ontodevice/ScreenBrightness -->


    <owl:Class rdf:about="https://www.theworldavatar.com/kg/ontodevice/ScreenBrightness">
        <rdfs:subClassOf rdf:resource="https://www.theworldavatar.com/kg/ontodevice/OperatingParameter"/>
        <rdfs:subClassOf>
            <owl:Restriction>
                <owl:onProperty rdf:resource="https://www.theworldavatar.com/kg/ontodevice/hasQuantity"/>
                <owl:allValuesFrom rdf:resource="https://www.theworldavatar.com/kg/ontodevice/RelativeBrightness"/>
            </owl:Restriction>
        </rdfs:subClassOf>
        <rdfs:comment>The screen brightness of a device.</rdfs:comment>
        <rdfs:isDefinedBy rdf:resource="https://www.theworldavatar.com/kg/ontodevice/"/>
        <rdfs:label>Screen brightness</rdfs:label>
    </owl:Class>
    


    <!-- https://www.theworldavatar.com/kg/ontodevice/ScrollPump -->


    <owl:Class rdf:about="https://www.theworldavatar.com/kg/ontodevice/ScrollPump">
        <rdfs:subClassOf rdf:resource="https://www.theworldavatar.com/kg/ontodevice/AirCompressor"/>
        <rdfs:comment>A type of air compressor that uses a pair of  interleaving scrolls for compression.</rdfs:comment>
        <rdfs:isDefinedBy rdf:resource="https://www.theworldavatar.com/kg/ontodevice/"/>
        <rdfs:label>Scroll pump</rdfs:label>
    </owl:Class>
    


    <!-- https://www.theworldavatar.com/kg/ontodevice/SelectorValve -->


    <owl:Class rdf:about="https://www.theworldavatar.com/kg/ontodevice/SelectorValve">
        <rdfs:subClassOf rdf:resource="https://www.theworldavatar.com/kg/ontodevice/Valve"/>
        <rdfs:comment>A valve that selects what gas or liquid pass through.</rdfs:comment>
        <rdfs:isDefinedBy rdf:resource="https://www.theworldavatar.com/kg/ontodevice/"/>
        <rdfs:label>Selector valve</rdfs:label>
    </owl:Class>
    


    <!-- https://www.theworldavatar.com/kg/ontodevice/Server -->


    <owl:Class rdf:about="https://www.theworldavatar.com/kg/ontodevice/Server">
        <rdfs:subClassOf rdf:resource="https://www.theworldavatar.com/kg/ontodevice/Computer"/>
        <rdfs:comment>A computer that provides functionality or programs for other computer.</rdfs:comment>
        <rdfs:isDefinedBy rdf:resource="https://www.theworldavatar.com/kg/ontodevice/"/>
        <rdfs:label>Server</rdfs:label>
    </owl:Class>
    


    <!-- https://www.theworldavatar.com/kg/ontodevice/ServerChassis -->


    <owl:Class rdf:about="https://www.theworldavatar.com/kg/ontodevice/ServerChassis">
        <rdfs:subClassOf rdf:resource="https://www.theworldavatar.com/kg/ontodevice/ComputerComponent"/>
        <rdfs:comment>A device where servers are mounted on.</rdfs:comment>
        <rdfs:isDefinedBy rdf:resource="https://www.theworldavatar.com/kg/ontodevice/"/>
        <rdfs:label>Server chassis</rdfs:label>
    </owl:Class>
    


    <!-- https://www.theworldavatar.com/kg/ontodevice/Setpoint -->


    <owl:Class rdf:about="https://www.theworldavatar.com/kg/ontodevice/Setpoint">
        <rdfs:comment>The desired or target value for an essential variable, or process value (PV) of a control system.</rdfs:comment>
        <rdfs:isDefinedBy rdf:resource="https://www.theworldavatar.com/kg/ontodevice/"/>
        <rdfs:label>Setpoint</rdfs:label>
    </owl:Class>
    


    <!-- https://www.theworldavatar.com/kg/ontodevice/SmartPhone -->


    <owl:Class rdf:about="https://www.theworldavatar.com/kg/ontodevice/SmartPhone">
        <rdfs:subClassOf rdf:resource="https://www.theworldavatar.com/kg/ontodevice/MobilePhone"/>
        <rdfs:comment>A portable computer device that combines mobile telephone and computing functions into one unit.</rdfs:comment>
        <rdfs:isDefinedBy rdf:resource="https://www.theworldavatar.com/kg/ontodevice/"/>
        <rdfs:label>Smart phone</rdfs:label>
    </owl:Class>
    


    <!-- https://www.theworldavatar.com/kg/ontodevice/SmartSensor -->


    <owl:Class rdf:about="https://www.theworldavatar.com/kg/ontodevice/SmartSensor">
        <rdfs:subClassOf rdf:resource="https://saref.etsi.org/core/Sensor"/>
        <rdfs:comment>A device that is composed of one or more Sensors together with a MicroController.</rdfs:comment>
        <rdfs:isDefinedBy rdf:resource="https://www.theworldavatar.com/kg/ontodevice/"/>
        <rdfs:label>Smart sensor</rdfs:label>
    </owl:Class>
    


    <!-- https://www.theworldavatar.com/kg/ontodevice/Speaker -->


    <owl:Class rdf:about="https://www.theworldavatar.com/kg/ontodevice/Speaker">
        <rdfs:subClassOf rdf:resource="https://www.theworldavatar.com/kg/ontodevice/PeripheralDevice"/>
        <rdfs:comment>A device that converts electrical signal from  a computer to sound waves.</rdfs:comment>
        <rdfs:isDefinedBy rdf:resource="https://www.theworldavatar.com/kg/ontodevice/"/>
        <rdfs:label>Speaker</rdfs:label>
    </owl:Class>
    


    <!-- https://www.theworldavatar.com/kg/ontodevice/StatusSensor -->


    <owl:Class rdf:about="https://www.theworldavatar.com/kg/ontodevice/StatusSensor">
        <rdfs:subClassOf rdf:resource="https://saref.etsi.org/core/Sensor"/>
        <rdfs:comment>A device that observes the status of another device.</rdfs:comment>
        <rdfs:isDefinedBy rdf:resource="https://www.theworldavatar.com/kg/ontodevice/"/>
        <rdfs:label>Status sensor</rdfs:label>
    </owl:Class>
    


    <!-- https://www.theworldavatar.com/kg/ontodevice/SwitchState -->


    <owl:Class rdf:about="https://www.theworldavatar.com/kg/ontodevice/SwitchState">
        <rdfs:subClassOf rdf:resource="https://saref.etsi.org/core/MultiLevelState"/>
        <rdfs:comment>The current state of a switch.</rdfs:comment>
        <rdfs:isDefinedBy rdf:resource="https://www.theworldavatar.com/kg/ontodevice/"/>
        <rdfs:label>Switch state</rdfs:label>
    </owl:Class>
    


    <!-- https://www.theworldavatar.com/kg/ontodevice/SyringePump -->


    <owl:Class rdf:about="https://www.theworldavatar.com/kg/ontodevice/SyringePump">
        <rdfs:subClassOf rdf:resource="https://www.theworldavatar.com/kg/ontodevice/Pump"/>
        <rdfs:comment>A pump that displaces gas or liquid via pushing or sucking with a syringe.</rdfs:comment>
        <rdfs:isDefinedBy rdf:resource="https://www.theworldavatar.com/kg/ontodevice/"/>
        <rdfs:label>Syringe pump</rdfs:label>
    </owl:Class>
    


    <!-- https://www.theworldavatar.com/kg/ontodevice/Tablet -->


    <owl:Class rdf:about="https://www.theworldavatar.com/kg/ontodevice/Tablet">
        <rdfs:subClassOf rdf:resource="https://www.theworldavatar.com/kg/ontodevice/Computer"/>
        <rdfs:comment>A small and mobile computer that uses touch-screens as user interface.</rdfs:comment>
        <rdfs:isDefinedBy rdf:resource="https://www.theworldavatar.com/kg/ontodevice/"/>
        <rdfs:label>Tablet</rdfs:label>
    </owl:Class>
    


    <!-- https://www.theworldavatar.com/kg/ontodevice/TemperatureController -->


    <owl:Class rdf:about="https://www.theworldavatar.com/kg/ontodevice/TemperatureController">
        <rdfs:subClassOf rdf:resource="https://www.theworldavatar.com/kg/ontodevice/Controller"/>
        <rdfs:comment>A device that manages the temperature of the surrounding environment.</rdfs:comment>
        <rdfs:isDefinedBy rdf:resource="https://www.theworldavatar.com/kg/ontodevice/"/>
        <rdfs:label>Temperature controller</rdfs:label>
    </owl:Class>
    


    <!-- https://www.theworldavatar.com/kg/ontodevice/ThermalEnergyMeter -->


    <owl:Class rdf:about="https://www.theworldavatar.com/kg/ontodevice/ThermalEnergyMeter">
        <rdfs:subClassOf rdf:resource="https://saref.etsi.org/core/Meter"/>
        <rdfs:comment>A device that is able to measure thermal energy and is usually used to measure energy from hydronic-based heating and cooling systems.</rdfs:comment>
        <rdfs:isDefinedBy rdf:resource="https://www.theworldavatar.com/kg/ontodevice/"/>
        <rdfs:label>Thermal energy meter</rdfs:label>
    </owl:Class>
    


    <!-- https://www.theworldavatar.com/kg/ontodevice/Thermostat -->


    <owl:Class rdf:about="https://www.theworldavatar.com/kg/ontodevice/Thermostat">
        <rdfs:subClassOf rdf:resource="https://saref.etsi.org/core/Device"/>
        <rdfs:comment>A device that measures and manages the temperature of the surrounding environment.</rdfs:comment>
        <rdfs:isDefinedBy rdf:resource="https://www.theworldavatar.com/kg/ontodevice/"/>
        <rdfs:label>Thermostat</rdfs:label>
    </owl:Class>
    


    <!-- https://www.theworldavatar.com/kg/ontodevice/Threshold -->


    <owl:Class rdf:about="https://www.theworldavatar.com/kg/ontodevice/Threshold">
        <rdfs:comment>A magnitude or intensity that must be exceeded for a certain reaction, phenomenon, result, or condition to occur or be manifested. </rdfs:comment>
        <rdfs:isDefinedBy rdf:resource="https://www.theworldavatar.com/kg/ontodevice/"/>
        <rdfs:label>Threshold</rdfs:label>
    </owl:Class>
    


    <!-- https://www.theworldavatar.com/kg/ontodevice/Tower -->


    <owl:Class rdf:about="https://www.theworldavatar.com/kg/ontodevice/Tower">
        <rdfs:subClassOf rdf:resource="https://www.theworldavatar.com/kg/ontodevice/ComputerComponent"/>
        <rdfs:comment>A device that holds computational component and interface of a computer in an enclosed space.</rdfs:comment>
        <rdfs:isDefinedBy rdf:resource="https://www.theworldavatar.com/kg/ontodevice/"/>
        <rdfs:label>Tower</rdfs:label>
    </owl:Class>
    


    <!-- https://www.theworldavatar.com/kg/ontodevice/TurboPump -->


    <owl:Class rdf:about="https://www.theworldavatar.com/kg/ontodevice/TurboPump">
        <rdfs:subClassOf rdf:resource="https://www.theworldavatar.com/kg/ontodevice/Pump"/>
        <rdfs:comment>A pump that used a turbo pump propeller to move the gas or liquid.</rdfs:comment>
        <rdfs:isDefinedBy rdf:resource="https://www.theworldavatar.com/kg/ontodevice/"/>
        <rdfs:label>Turbo pump</rdfs:label>
    </owl:Class>
    


    <!-- https://www.theworldavatar.com/kg/ontodevice/UAV -->


    <owl:Class rdf:about="https://www.theworldavatar.com/kg/ontodevice/UAV">
        <rdfs:subClassOf rdf:resource="https://saref.etsi.org/core/Device"/>
        <rdfs:comment>A robot that does aerial movement without human on board.</rdfs:comment>
        <rdfs:isDefinedBy rdf:resource="https://www.theworldavatar.com/kg/ontodevice/"/>
        <rdfs:label>UAV</rdfs:label>
    </owl:Class>
    


    <!-- https://www.theworldavatar.com/kg/ontodevice/VacuumCleaner -->


    <owl:Class rdf:about="https://www.theworldavatar.com/kg/ontodevice/VacuumCleaner">
        <rdfs:subClassOf rdf:resource="https://saref.etsi.org/core/Appliance"/>
        <rdfs:comment>A device that cleans a surface by creating a vacuum to suck up dirt.</rdfs:comment>
        <rdfs:isDefinedBy rdf:resource="https://www.theworldavatar.com/kg/ontodevice/"/>
        <rdfs:label>Vacuum cleaner</rdfs:label>
    </owl:Class>
    


    <!-- https://www.theworldavatar.com/kg/ontodevice/VacuumPump -->


    <owl:Class rdf:about="https://www.theworldavatar.com/kg/ontodevice/VacuumPump">
        <rdfs:subClassOf rdf:resource="https://www.theworldavatar.com/kg/ontodevice/Pump"/>
        <rdfs:comment>A pump that is designed to create a vacuum in a designated area.</rdfs:comment>
        <rdfs:isDefinedBy rdf:resource="https://www.theworldavatar.com/kg/ontodevice/"/>
        <rdfs:label>Vacuum pump</rdfs:label>
    </owl:Class>
    


    <!-- https://www.theworldavatar.com/kg/ontodevice/Valve -->


    <owl:Class rdf:about="https://www.theworldavatar.com/kg/ontodevice/Valve">
        <rdfs:subClassOf rdf:resource="https://www.theworldavatar.com/kg/ontodevice/FlowController"/>
        <rdfs:comment>A device that manages the amount of gas or liquid flowing through via changing the area the material can pass through.</rdfs:comment>
        <rdfs:isDefinedBy rdf:resource="https://www.theworldavatar.com/kg/ontodevice/"/>
        <rdfs:label>Valve</rdfs:label>
    </owl:Class>
    


    <!-- https://www.theworldavatar.com/kg/ontodevice/Vector -->


    <owl:Class rdf:about="https://www.theworldavatar.com/kg/ontodevice/Vector">
        <rdfs:comment>A quantity that has magnitude and direction.</rdfs:comment>
        <rdfs:isDefinedBy rdf:resource="https://www.theworldavatar.com/kg/ontodevice/"/>
        <rdfs:label>Vector</rdfs:label>
    </owl:Class>
    


    <!-- https://www.theworldavatar.com/kg/ontodevice/WaterChiller -->


    <owl:Class rdf:about="https://www.theworldavatar.com/kg/ontodevice/WaterChiller">
        <rdfs:subClassOf rdf:resource="https://saref.etsi.org/core/Appliance"/>
        <rdfs:comment>A device that is used to reduce water temperature.</rdfs:comment>
        <rdfs:isDefinedBy rdf:resource="https://www.theworldavatar.com/kg/ontodevice/"/>
        <rdfs:label>Water chiller</rdfs:label>
    </owl:Class>
    


    <!-- https://www.theworldavatar.com/kg/ontodevice/WaterDispenser -->


    <owl:Class rdf:about="https://www.theworldavatar.com/kg/ontodevice/WaterDispenser">
        <rdfs:subClassOf rdf:resource="https://saref.etsi.org/core/Appliance"/>
        <rdfs:comment>A device that stores and dispenses water for consumption.</rdfs:comment>
        <rdfs:isDefinedBy rdf:resource="https://www.theworldavatar.com/kg/ontodevice/"/>
        <rdfs:label>Water dispenser</rdfs:label>
    </owl:Class>
    


    <!-- https://www.theworldavatar.com/kg/ontodevice/WaterMeter -->


    <owl:Class rdf:about="https://www.theworldavatar.com/kg/ontodevice/WaterMeter">
        <rdfs:subClassOf rdf:resource="https://saref.etsi.org/core/Meter"/>
        <rdfs:comment>A device that measure and communicate water usage from consumer to provider to facilitate water management and proper billing.</rdfs:comment>
        <rdfs:isDefinedBy rdf:resource="https://www.theworldavatar.com/kg/ontodevice/"/>
        <rdfs:label>Water meter</rdfs:label>
    </owl:Class>
    


    <!-- https://www.theworldavatar.com/kg/ontodevice/Workstation -->


    <owl:Class rdf:about="https://www.theworldavatar.com/kg/ontodevice/Workstation">
        <rdfs:subClassOf rdf:resource="https://www.theworldavatar.com/kg/ontodevice/Computer"/>
        <rdfs:comment>A workstation is a special computer designed for technical or scientific applications.</rdfs:comment>
        <rdfs:isDefinedBy rdf:resource="https://www.theworldavatar.com/kg/ontodevice/"/>
        <rdfs:label>Workstation</rdfs:label>
    </owl:Class>
    


    <!-- https://www.theworldavatar.com/kg/ontodevice/pHLevelSensor -->


    <owl:Class rdf:about="https://www.theworldavatar.com/kg/ontodevice/pHLevelSensor">
        <rdfs:subClassOf rdf:resource="https://saref.etsi.org/core/Sensor"/>
        <rdfs:comment>A device used to measure the acidity or alkalinity of a solution.</rdfs:comment>
        <rdfs:isDefinedBy rdf:resource="https://www.theworldavatar.com/kg/ontodevice/"/>
        <rdfs:label>pH level sensor</rdfs:label>
    </owl:Class>
    


    <!-- https://www.theworldavatar.com/kg/ontoems/ReportingStation -->


    <owl:Class rdf:about="https://www.theworldavatar.com/kg/ontoems/ReportingStation">
        <rdfs:subClassOf rdf:resource="https://saref.etsi.org/core/Device"/>
        <rdfs:isDefinedBy rdf:resource="https://www.theworldavatar.com/kg/ontodevice/"/>
        <rdfs:label>Reporting station</rdfs:label>
    </owl:Class>
</rdf:RDF>



<!-- Generated by the OWL API (version 5.5.0.2023-01-14T12:41:38Z) https://github.com/owlcs/owlapi/ -->


